# baseURI: http://unifiedcyberontology.org/pattern

@prefix owl: <http://www.w3.org/2002/07/owl#> .
@prefix rdfs: <http://www.w3.org/2000/01/rdf-schema#> .
@prefix xsd: <http://www.w3.org/2001/XMLSchema#> .

<http://unifiedcyberontology.org/pattern>
  rdf:type owl:Ontology ;
  rdfs:label "uco-pattern"@en .

xsd:PatternExpression a rdfs:Datatype .
<http://unifiedcyberontology.org/pattern#patternExpression>
  rdf:type owl:DatatypeProperty ;
  rdfs:domain <http://unifiedcyberontology.org/pattern#LogicalPattern> ;
  rdfs:range xsd:PatternExpression ;
  rdfs:comment ""@en ;
  rdfs:label "patternExpression"@en .

<http://unifiedcyberontology.org/pattern#LogicalPattern>
  rdf:type owl:Class ;
  rdfs:subClassOf <http://unifiedcyberontology.org/pattern#Pattern>, [
    rdf:type owl:Restriction ;
    owl:onProperty <http://unifiedcyberontology.org/pattern#patternExpression> ;
    owl:maxQualifiedCardinality "1"^^xsd:nonNegativeInteger ;
    owl:onDataRange xsd:PatternExpression
  ] ;
  rdfs:comment "An informational pattern instantiated in UCO content and expressed as a logical pattern expression."@en ;
  rdfs:label "LogicalPattern"@en .

<http://unifiedcyberontology.org/pattern#Pattern>
  rdf:type owl:Class ;
  rdfs:subClassOf <http://unifiedcyberontology.org/core#UcoObject> ;
  rdfs:comment "A combination of properties, acts, tendencies, etc., forming a consistent or characteristic arrangement."@en ;
  rdfs:label "Pattern"@en .

<http://unifiedcyberontology.org/pattern#PatternExpression> rdfs:comment "An explicit logical specification of a UCO informational pattern."@en .
