# baseURI: http://unifiedcyberontology.org/pattern

@prefix pattern: <http://unifiedcyberontology.org/pattern#> .
@prefix owl: <http://www.w3.org/2002/07/owl#> .
@prefix rdf: <http://www.w3.org/1999/02/22-rdf-syntax-ns#> .
@prefix rdfs: <http://www.w3.org/2000/01/rdf-schema#> .
@prefix xsd: <http://www.w3.org/2001/XMLSchema#> .

<http://unifiedcyberontology.org/pattern>
  rdf:type owl:Ontology ;
  rdfs:label "uco-pattern"@en .



pattern:LogicalPattern
  rdf:type owl:Class ;
  rdfs:comment "An informational pattern instantiated in UCO content and expressed as a logical pattern expression."@en ;
  rdfs:label "LogicalPattern"@en ;
  rdfs:subClassOf pattern:Pattern, [
    rdf:type owl:Restriction ;
    owl:onProperty pattern:patternExpression ;
    owl:maxQualifiedCardinality "1"^^xsd:nonNegativeInteger ;
    owl:onDataRange pattern:PatternExpression
  ] ;
  .

pattern:Pattern
  rdf:type owl:Class ;
  rdfs:comment "An explicit logical specification of a UCO informational pattern."@en ;
  rdfs:label "Pattern"@en ;
  rdfs:subClassOf <http://unifiedcyberontology.org/core#UcoObject> ;
  rdfs:comment "A combination of properties, acts, tendencies, etc., forming a consistent or characteristic arrangement."@en ;
  rdfs:label "Pattern"@en
  .

pattern:PatternExpression
rdfs:comment "An explicit logical pattern expression."@en ;
rdf:type owl:Class ;
rdfs:label "PatternExpression"@en ;
.


pattern:patternExpression
  rdf:type owl:DatatypeProperty ;
  rdfs:comment "An explicit logical pattern expression."@en ;
  rdfs:label "patternExpression"@en ;
  rdfs:domain pattern:LogicalPattern ;
  rdfs:range pattern:PatternExpression ;
  .
