#  imports: https://ontology.unifiedcyberontology.org/uco/role/1.1.0
#  imports: http://purl.org/co
#  imports: https://ontology.unifiedcyberontology.org/uco/core/1.1.0
#  imports: https://ontology.unifiedcyberontology.org/co/1.1.0
#  imports: https://ontology.unifiedcyberontology.org/uco/core/1.1.0
#  imports: https://ontology.unifiedcyberontology.org/uco/core/1.1.0
@prefix co: <http://purl.org/co/> .
#  imports: https://ontology.unifiedcyberontology.org/uco/core/1.1.0
#  imports: https://ontology.unifiedcyberontology.org/uco/action/1.1.0
@prefix core: <https://ontology.unifiedcyberontology.org/uco/core/> .
#  imports: https://ontology.unifiedcyberontology.org/owl/1.1.0
@prefix owl: <http://www.w3.org/2002/07/owl#> .
@prefix action: <https://ontology.unifiedcyberontology.org/uco/action/> .
@prefix configuration: <https://ontology.unifiedcyberontology.org/uco/configuration/> .
#  imports: https://ontology.unifiedcyberontology.org/uco/action/1.1.0
@prefix rdf: <http://www.w3.org/1999/02/22-rdf-syntax-ns#> .
@prefix analysis: <https://ontology.unifiedcyberontology.org/uco/analysis/> .
@prefix pattern: <https://ontology.unifiedcyberontology.org/uco/pattern/> .
#  imports: https://ontology.unifiedcyberontology.org/uco/analysis/1.1.0
@prefix rdfs: <http://www.w3.org/2000/01/rdf-schema#> .
#  imports: https://ontology.unifiedcyberontology.org/uco/core/1.1.0
@prefix sh: <http://www.w3.org/ns/shacl#> .
#  imports: https://ontology.unifiedcyberontology.org/uco/configuration/1.1.0
@prefix role: <https://ontology.unifiedcyberontology.org/uco/role/> .
@prefix uco-co: <https://ontology.unifiedcyberontology.org/co/> .
#  imports: https://ontology.unifiedcyberontology.org/uco/core/1.1.0
#  imports: https://ontology.unifiedcyberontology.org/uco/core/1.1.0
@prefix xsd: <http://www.w3.org/2001/XMLSchema#> .
@prefix time: <https://ontology.unifiedcyberontology.org/uco/time/> .
@prefix location: <https://ontology.unifiedcyberontology.org/uco/location/> .
@prefix victim: <https://ontology.unifiedcyberontology.org/uco/victim/> .
#  imports: https://ontology.unifiedcyberontology.org/uco/location/1.1.0
#  imports: https://ontology.unifiedcyberontology.org/uco/core/1.1.0
#  imports: https://ontology.unifiedcyberontology.org/uco/identity/1.1.0
#  imports: https://ontology.unifiedcyberontology.org/uco/location/1.1.0
@prefix identity: <https://ontology.unifiedcyberontology.org/uco/identity/> .
@prefix marking: <https://ontology.unifiedcyberontology.org/uco/marking/> .
#  imports: https://ontology.unifiedcyberontology.org/uco/configuration/1.1.0
#  imports: https://ontology.unifiedcyberontology.org/co/1.1.0
#  imports: https://ontology.unifiedcyberontology.org/uco/marking/1.1.0
#  imports: https://ontology.unifiedcyberontology.org/uco/identity/1.1.0
#  imports: https://ontology.unifiedcyberontology.org/uco/core/1.1.0
#  imports: https://ontology.unifiedcyberontology.org/uco/observable/1.1.0
#  imports: https://ontology.unifiedcyberontology.org/uco/vocabulary/1.1.0
#  imports: https://ontology.unifiedcyberontology.org/uco/core/1.1.0
@prefix uco-owl: <https://ontology.unifiedcyberontology.org/owl/> .
#  imports: https://ontology.unifiedcyberontology.org/uco/pattern/1.1.0
#  imports: https://ontology.unifiedcyberontology.org/uco/location/1.1.0
#  imports: https://ontology.unifiedcyberontology.org/uco/role/1.1.0
#  imports: https://ontology.unifiedcyberontology.org/uco/pattern/1.1.0
#  imports: https://ontology.unifiedcyberontology.org/uco/time/1.1.0
#  imports: https://ontology.unifiedcyberontology.org/uco/types/1.1.0
#  imports: https://ontology.unifiedcyberontology.org/uco/tool/1.1.0
#  imports: https://ontology.unifiedcyberontology.org/uco/vocabulary/1.1.0
@prefix tool: <https://ontology.unifiedcyberontology.org/uco/tool/> .
#  imports: https://ontology.unifiedcyberontology.org/uco/action/1.1.0
#  imports: https://ontology.unifiedcyberontology.org/uco/types/1.1.0
@prefix types: <https://ontology.unifiedcyberontology.org/uco/types/> .
#  imports: https://ontology.unifiedcyberontology.org/uco/configuration/1.1.0
#  imports: https://ontology.unifiedcyberontology.org/uco/victim/1.1.0
#  imports: https://ontology.unifiedcyberontology.org/uco/vocabulary/1.1.0
#  imports: https://ontology.unifiedcyberontology.org/uco/core/1.1.0
@prefix vocabulary: <https://ontology.unifiedcyberontology.org/uco/vocabulary/> .
#  imports: https://ontology.unifiedcyberontology.org/uco/identity/1.1.0
#  imports: https://ontology.unifiedcyberontology.org/uco/location/1.1.0
#  imports: https://ontology.unifiedcyberontology.org/uco/types/1.1.0
#  imports: https://ontology.unifiedcyberontology.org/uco/vocabulary/1.1.0
@prefix observable: <https://ontology.unifiedcyberontology.org/uco/observable/> .

<https://ontology.unifiedcyberontology.org/uco/victim> a owl:Ontology .

<https://ontology.unifiedcyberontology.org/uco/time> a owl:Ontology .

<https://ontology.unifiedcyberontology.org/uco/role> a owl:Ontology .

<https://ontology.unifiedcyberontology.org/uco/configuration> a owl:Ontology .

<https://ontology.unifiedcyberontology.org/co> a owl:Ontology .

<https://ontology.unifiedcyberontology.org/uco/pattern> a owl:Ontology .

<https://ontology.unifiedcyberontology.org/uco/analysis> a owl:Ontology .

<https://ontology.unifiedcyberontology.org/co> rdfs:label "uco-co"@en .

<https://ontology.unifiedcyberontology.org/uco/configuration> rdfs:label "uco-configuration"@en .

<https://ontology.unifiedcyberontology.org/uco/time> rdfs:label "uco-time"@en .

<https://ontology.unifiedcyberontology.org/uco/victim> rdfs:label "uco-victim"@en .

<https://ontology.unifiedcyberontology.org/uco/role> rdfs:label "uco-role"@en .

<https://ontology.unifiedcyberontology.org/uco/analysis> rdfs:label "uco-analysis"@en .

<https://ontology.unifiedcyberontology.org/uco/pattern> rdfs:label "uco-pattern"@en .

<https://ontology.unifiedcyberontology.org/uco/location> a owl:Ontology .

<https://ontology.unifiedcyberontology.org/uco/role> owl:backwardCompatibleWith role:1.0.0 .

<https://ontology.unifiedcyberontology.org/uco/victim> owl:backwardCompatibleWith victim:1.0.0 .

<https://ontology.unifiedcyberontology.org/uco/time> owl:backwardCompatibleWith time:1.0.0 .

<https://ontology.unifiedcyberontology.org/uco/pattern> owl:backwardCompatibleWith pattern:1.0.0 .

<https://ontology.unifiedcyberontology.org/uco/location> rdfs:label "uco-location"@en .

<https://ontology.unifiedcyberontology.org/uco/role> owl:imports core:1.1.0 .

<https://ontology.unifiedcyberontology.org/uco/victim> owl:imports role:1.1.0 .

<https://ontology.unifiedcyberontology.org/uco/time> owl:imports core:1.1.0 .

<https://ontology.unifiedcyberontology.org/uco/pattern> owl:imports core:1.1.0 .

<https://ontology.unifiedcyberontology.org/uco/victim> owl:priorVersion victim:1.0.0 .

<https://ontology.unifiedcyberontology.org/uco/role> owl:priorVersion role:1.0.0 .

<https://ontology.unifiedcyberontology.org/uco/configuration> rdfs:comment "This ontology defines classes and properties for characterizing configurations."@en-us .

<https://ontology.unifiedcyberontology.org/co> rdfs:comment "This ontology defines SHACL shapes to supplement the OWL 2 DL definitions in the Collections Ontology."@en .

<https://ontology.unifiedcyberontology.org/uco/time> owl:priorVersion time:1.0.0 .

<https://ontology.unifiedcyberontology.org/uco/location> owl:backwardCompatibleWith location:1.0.0 .

<https://ontology.unifiedcyberontology.org/uco/victim> owl:versionIRI victim:1.1.0 .

<https://ontology.unifiedcyberontology.org/uco/pattern> owl:priorVersion pattern:1.0.0 .

<https://ontology.unifiedcyberontology.org/uco/marking> a owl:Ontology .

<https://ontology.unifiedcyberontology.org/uco/analysis> rdfs:comment "This ontology defines classes and properties for characterizing analytic actions and results."@en-us .

<https://ontology.unifiedcyberontology.org/uco/role> owl:versionIRI role:1.1.0 .

<https://ontology.unifiedcyberontology.org/uco/location> owl:imports core:1.1.0 .

<https://ontology.unifiedcyberontology.org/uco/time> owl:versionIRI time:1.1.0 .

<https://ontology.unifiedcyberontology.org/owl> a owl:Ontology .

<https://ontology.unifiedcyberontology.org/uco/identity> a owl:Ontology .

<https://ontology.unifiedcyberontology.org/co> owl:backwardCompatibleWith uco-co:1.0.0 .

victim:Victim a owl:Class .

<https://ontology.unifiedcyberontology.org/uco/pattern> owl:versionIRI pattern:1.1.0 .

<https://ontology.unifiedcyberontology.org/uco/marking> rdfs:label "uco-marking"@en .

<https://ontology.unifiedcyberontology.org/uco/configuration> rdfs:seeAlso <https://github.com/ucoProject/UCO/issues/432> .

victim:Victim a sh:NodeShape .

<https://ontology.unifiedcyberontology.org/owl> rdfs:label "uco-owl"@en .

<https://ontology.unifiedcyberontology.org/uco/identity> rdfs:label "uco-identity"@en .

<https://ontology.unifiedcyberontology.org/co> owl:imports <http://purl.org/co> .

<https://ontology.unifiedcyberontology.org/uco/location> owl:priorVersion location:1.0.0 .

role:BenevolentRole a owl:Class .

time:Time a rdfs:Datatype .

<https://ontology.unifiedcyberontology.org/uco/analysis> rdfs:seeAlso <https://github.com/ucoProject/UCO/issues/400> .

role:BenevolentRole a sh:NodeShape .

victim:Victim rdfs:subClassOf role:NeutralRole .

<https://ontology.unifiedcyberontology.org/uco/configuration> owl:backwardCompatibleWith configuration:1.0.0 .

<https://ontology.unifiedcyberontology.org/co> owl:priorVersion uco-co:1.0.0 .

pattern:LogicalPattern a owl:Class .

<https://ontology.unifiedcyberontology.org/uco/location> owl:versionIRI location:1.1.0 .

<https://ontology.unifiedcyberontology.org/uco/analysis> owl:imports action:1.1.0 .

<https://ontology.unifiedcyberontology.org/uco/identity> owl:backwardCompatibleWith identity:1.0.0 .

time:TimeRange a rdfs:Datatype .

victim:Victim rdfs:label "Victim"@en .

role:BenevolentRole rdfs:subClassOf role:Role .

pattern:LogicalPattern a sh:NodeShape .

<https://ontology.unifiedcyberontology.org/uco/configuration> owl:imports core:1.1.0 .

<https://ontology.unifiedcyberontology.org/co> owl:versionIRI uco-co:1.1.0 .

<https://ontology.unifiedcyberontology.org/uco/identity> owl:imports core:1.1.0 .

<https://ontology.unifiedcyberontology.org/uco/analysis> owl:versionIRI analysis:1.1.0 .

<https://ontology.unifiedcyberontology.org/uco/marking> rdfs:comment "Data markings represent restrictions, permissions, and other guidance for how data can be used and shared."@en .

role:BenevolentRole rdfs:label "BenevolentRole"@en .

<https://ontology.unifiedcyberontology.org/uco/identity> owl:imports location:1.1.0 .

time:Timestamp a rdfs:Datatype .

pattern:LogicalPattern rdfs:subClassOf pattern:Pattern .

location:GPSCoordinatesFacet a owl:Class .

<https://ontology.unifiedcyberontology.org/uco/configuration> owl:priorVersion configuration:1.0.0 .

location:GPSCoordinatesFacet a sh:NodeShape .

analysis:Analysis a owl:Class .

co:ListItem rdfs:subClassOf co:Item .

<https://ontology.unifiedcyberontology.org/uco/marking> owl:backwardCompatibleWith marking:1.0.0 .

<https://ontology.unifiedcyberontology.org/uco/identity> owl:priorVersion identity:1.0.0 .

pattern:LogicalPattern rdfs:label "LogicalPattern"@en .

analysis:Analysis a sh:NodeShape .

<https://ontology.unifiedcyberontology.org/uco/configuration> owl:versionIRI configuration:1.1.0 .

location:GPSCoordinatesFacet rdfs:subClassOf core:Facet .

victim:Victim rdfs:comment "A victim is a role played by a person or organization that is/was the target of some malicious action."@en .

<https://ontology.unifiedcyberontology.org/uco/marking> owl:imports core:1.1.0 .

uco-co:List-shape a sh:NodeShape .

<https://ontology.unifiedcyberontology.org/uco/identity> owl:versionIRI identity:1.1.0 .

analysis:Analysis rdfs:subClassOf action:Action .

role:BenevolentRole rdfs:comment "A benevolent role is a role with positive and/or beneficial intent."@en .

victim:Victim sh:targetClass victim:Victim .

<https://ontology.unifiedcyberontology.org/uco/tool> a owl:Ontology .

<https://ontology.unifiedcyberontology.org/uco/marking> owl:priorVersion marking:1.0.0 .

location:GPSCoordinatesFacet rdfs:label "GPSCoordinatesFacet"@en .

analysis:Analysis rdfs:label "Analysis"@en .

configuration:Configuration a owl:Class .

identity:AddressFacet a owl:Class .

role:BenevolentRole sh:targetClass role:BenevolentRole .

<https://ontology.unifiedcyberontology.org/uco/tool> rdfs:label "uco-tool"@en .

configuration:Configuration a sh:NodeShape .

identity:AddressFacet a sh:NodeShape .

_:node1gm7uj6vjx1 sh:class co:ListItem .

<https://ontology.unifiedcyberontology.org/uco/marking> owl:versionIRI marking:1.1.0 .

victim:VictimTargeting a owl:Class , sh:NodeShape .

_:node1gm7uj6vjx1 sh:path co:item .

configuration:Configuration rdfs:subClassOf core:UcoObject .

uco-co:List-shape sh:property _:node1gm7uj6vjx1 .

<https://ontology.unifiedcyberontology.org/uco/tool> owl:backwardCompatibleWith tool:1.0.0 .

role:MaliciousRole a owl:Class .

identity:AddressFacet rdfs:subClassOf identity:IdentityFacet .

role:MaliciousRole a sh:NodeShape .

victim:VictimTargeting rdfs:subClassOf victim:Victim .

marking:GranularMarking a owl:Class .

uco-co:List-shape sh:targetClass co:List .

configuration:Configuration rdfs:label "Configuration"@en .

<https://ontology.unifiedcyberontology.org/uco/tool> owl:imports configuration:1.1.0 .

identity:AddressFacet rdfs:label "AddressFacet"@en .

marking:GranularMarking a sh:NodeShape .

role:MaliciousRole rdfs:subClassOf role:Role .

<https://ontology.unifiedcyberontology.org/uco/tool> owl:imports identity:1.1.0 .

victim:VictimTargeting rdfs:label "VictimTargeting"@en .

<https://ontology.unifiedcyberontology.org/uco/core> a owl:Ontology .

pattern:LogicalPattern rdfs:comment "A logical pattern is a grouping of characteristics unique to an informational pattern expressed via a structured pattern expression following the rules of logic."@en .

uco-co:ListItem-shape a sh:NodeShape .

<https://ontology.unifiedcyberontology.org/uco/tool> owl:priorVersion tool:1.0.0 .

role:MaliciousRole rdfs:label "MaliciousRole"@en .

<https://ontology.unifiedcyberontology.org/uco/core> rdfs:label "uco-core"@en .

analysis:Analysis rdfs:comment "An analysis is an action of detailed examination of something in order to understand its nature, context or essential features."@en .

<https://ontology.unifiedcyberontology.org/uco/types> a owl:Ontology .

<https://ontology.unifiedcyberontology.org/uco/tool> owl:versionIRI tool:1.1.0 .

marking:GranularMarking rdfs:subClassOf core:UcoInherentCharacterizationThing .

analysis:Analysis sh:targetClass action:Analysis .

_:node1gm7uj6vjx2 sh:datatype pattern:PatternExpression .

<https://ontology.unifiedcyberontology.org/uco/vocabulary> a owl:Ontology .

<https://ontology.unifiedcyberontology.org/uco/types> rdfs:label "uco-types"@en .

marking:GranularMarking rdfs:label "GranularMarking"@en .

_:node1gm7uj6vjx3 rdfs:comment "Adapted from restriction on co:ListItem."@en .

tool:AnalyticTool a owl:Class .

role:MaliciousRole rdfs:comment "A malicious role is a role with malevolent intent."@en .

configuration:Configuration rdfs:comment "A configuration is a grouping of characteristics unique to a set of parameters or initial settings for the use of a tool, application, software, or other cyber object."@en .

tool:AnalyticTool a sh:NodeShape .

<https://ontology.unifiedcyberontology.org/uco/vocabulary> rdfs:label "uco-vocabularies"@en .

analysis:AnalyticResult a owl:Class .

victim:VictimTargeting rdfs:comment "A victim targeting is a grouping of characteristics unique to people or organizations that are the target of some malicious activity."@en .

role:MaliciousRole sh:targetClass role:MaliciousRole .

<https://ontology.unifiedcyberontology.org/owl> rdfs:comment "This ontology defines SHACL shapes to perform conformance testing of OWL 2 DL.  Some of these shapes follow rules specified from the canonical, subtractive parsing process of Section 3 of the OWL 2 mapping to RDF.  From the last line of that document's Section 3, 'At the end of this process, the graph G MUST be empty,' anything not strictly matching patterns specified in that section cause the input graph to be non-conformant with OWL 2 DL."@en .

analysis:AnalyticResult a sh:NodeShape .

identity:AddressFacet rdfs:comment "An address facet is a grouping of characteristics unique to an administrative identifier for a geolocation associated with a specific identity."@en .

<https://ontology.unifiedcyberontology.org/uco/types> owl:backwardCompatibleWith types:1.0.0 .

tool:AnalyticTool rdfs:subClassOf tool:Tool .

<https://ontology.unifiedcyberontology.org/uco/vocabulary> owl:backwardCompatibleWith vocabulary:1.0.0 .

configuration:Configuration rdfs:seeAlso <https://github.com/ucoProject/UCO/issues/432> .

location:GPSCoordinatesFacet rdfs:comment "A GPS coordinates facet is a grouping of characteristics unique to the expression of quantified dilution of precision (DOP) for an asserted set of geolocation coordinates typically associated with satellite navigation such as the Global Positioning System (GPS)."@en .

victim:VictimTargeting sh:targetClass victim:VictimTargeting .

<https://ontology.unifiedcyberontology.org/uco/types> owl:imports uco-co:1.1.0 .

<https://ontology.unifiedcyberontology.org/uco/uco> a owl:Ontology .

role:NeutralRole a owl:Class .

analysis:AnalyticResult rdfs:subClassOf core:Assertion .

tool:AnalyticTool rdfs:label "AnalyticTool"@en .

_:node1gm7uj6vjx4 sh:class location:Location .

<https://ontology.unifiedcyberontology.org/uco/vocabulary> owl:priorVersion vocabulary:1.0.0 .

<https://ontology.unifiedcyberontology.org/uco/types> owl:imports core:1.1.0 .

role:NeutralRole a sh:NodeShape .

<https://ontology.unifiedcyberontology.org/uco/uco> rdfs:label "uco-master"@en .

<https://ontology.unifiedcyberontology.org/uco/types> owl:imports vocabulary:1.1.0 .

analysis:AnalyticResult rdfs:label "AnalyticResult"@en .

<https://ontology.unifiedcyberontology.org/uco/vocabulary> owl:versionIRI vocabulary:1.1.0 .

_:node1gm7uj6vjx6 sh:datatype xsd:decimal .

<https://ontology.unifiedcyberontology.org/uco/core> rdfs:comment "This ontology defines classes and properties that are shared across the various UCO ontologies.  At a high-level, the UCO core ontology provides base classes, relationship-oriented classes, content-aggregation classes, and shared classes."@en .

role:NeutralRole rdfs:subClassOf role:Role .

_:node1gm7uj6vjx5 sh:class configuration:ConfigurationEntry .

<https://ontology.unifiedcyberontology.org/uco/types> owl:priorVersion types:1.0.0 .

<https://ontology.unifiedcyberontology.org/owl> rdfs:seeAlso <https://www.w3.org/TR/2012/REC-owl2-mapping-to-rdf-20121211/#Mapping_from_RDF_Graphs_to_the_Structural_Specification> .

role:NeutralRole rdfs:label "NeutralRole"@en .

<https://ontology.unifiedcyberontology.org/uco/core> owl:backwardCompatibleWith core:1.0.0 .

vocabulary:AccountTypeVocab a rdfs:Datatype .

_:node1gm7uj6vjx5 sh:nodeKind sh:BlankNodeOrIRI .

<https://ontology.unifiedcyberontology.org/uco/types> owl:versionIRI types:1.1.0 .

<https://ontology.unifiedcyberontology.org/uco/uco> owl:backwardCompatibleWith <https://ontology.unifiedcyberontology.org/uco/uco/1.0.0> .

<https://ontology.unifiedcyberontology.org/owl> owl:backwardCompatibleWith uco-owl:1.0.0 .

marking:GranularMarking rdfs:comment "A granular marking is a grouping of characteristics unique to specification of marking definitions (restrictions, permissions, and other guidance for how data can be used and shared) that apply to particular portions of a particular UCO object."@en .

<https://ontology.unifiedcyberontology.org/uco/core> owl:priorVersion core:1.0.0 .

tool:AnalyticTool rdfs:comment "An analytic tool is an artifact of hardware and/or software utilized to accomplish a task or purpose of explanation, interpretation or logical reasoning."@en .

analysis:AnalyticResult rdfs:comment "An analytic result is a characterization of the understanding resulting from an analysis action."@en .

_:node1gm7uj6vjx5 sh:path configuration:configurationEntry .

vocabulary:AccountTypeVocab rdfs:label "Account Type Vocabulary"@en-us .

configuration:Configuration sh:property _:node1gm7uj6vjx5 .

role:NeutralRole rdfs:comment "A neutral role is a role with impartial intent."@en .

_:node1gm7uj6vjx6 sh:maxCount 1 .

_:node1gm7uj6vjx4 sh:maxCount 1 .

_:node1gm7uj6vjx3 sh:maxCount 1 .

_:node1gm7uj6vjx2 sh:maxCount 1 .

types:ControlledDictionary a owl:Class .

<https://ontology.unifiedcyberontology.org/uco/uco> owl:imports uco-co:1.1.0 .

<https://ontology.unifiedcyberontology.org/owl> owl:priorVersion uco-owl:1.0.0 .

<https://ontology.unifiedcyberontology.org/uco/core> owl:versionIRI core:1.1.0 .

types:ControlledDictionary a sh:NodeShape .

tool:AnalyticTool sh:targetClass tool:AnalyticTool .

_:node1gm7uj6vjx4 sh:nodeKind sh:IRI .

_:node1gm7uj6vjx3 sh:path co:index .

_:node1gm7uj6vjx2 sh:nodeKind sh:Literal .

uco-co:ListItem-shape sh:property _:node1gm7uj6vjx3 .

<https://ontology.unifiedcyberontology.org/uco/action> a owl:Ontology .

_:node1gm7uj6vjx6 sh:nodeKind sh:Literal .

_:node1gm7uj6vjx7 sh:class marking:MarkingDefinition .

_:node1gm7uj6vjx9 sh:class analysis:Analysis .

_:node1gm7uj6vjx10 a rdfs:Datatype .

<https://ontology.unifiedcyberontology.org/uco/uco> owl:imports uco-owl:1.1.0 .

role:NeutralRole sh:targetClass role:NeutralRole .

_:node1gm7uj6vjx8 sh:class configuration:Dependency .

<https://ontology.unifiedcyberontology.org/owl> owl:versionIRI uco-owl:1.1.0 .

types:ControlledDictionary rdfs:subClassOf types:Dictionary .

_:node1gm7uj6vjx4 sh:path identity:address .

_:node1gm7uj6vjx6 sh:path location:hdop .

<https://ontology.unifiedcyberontology.org/uco/action> rdfs:label "uco-action"@en .

core:Annotation a owl:Class .

identity:AddressFacet sh:property _:node1gm7uj6vjx4 .

location:GPSCoordinatesFacet sh:property _:node1gm7uj6vjx6 .

tool:BuildFacet a owl:Class .

_:node1gm7uj6vjx7 sh:nodeKind sh:IRI .

uco-co:ListItem-shape sh:targetClass co:ListItem .

_:node1gm7uj6vjx2 sh:path pattern:patternExpression .

pattern:LogicalPattern sh:property _:node1gm7uj6vjx2 .

tool:BuildFacet a sh:NodeShape .

_:node1gm7uj6vjx10 owl:onDatatype xsd:string .

core:Annotation a sh:NodeShape .

role:Role a owl:Class .

types:ControlledDictionary rdfs:label "ControlledDictionary"@en .

<https://ontology.unifiedcyberontology.org/uco/uco> owl:imports action:1.1.0 .

_:node1gm7uj6vjx9 sh:maxCount 1 .

_:node1gm7uj6vjx8 sh:nodeKind sh:BlankNodeOrIRI .

_:node1gm7uj6vjx7 sh:path marking:marking .

marking:GranularMarking sh:property _:node1gm7uj6vjx7 .

_:node1gm7uj6vjx11 sh:datatype xsd:decimal .

uco-owl:Axiom-shape a sh:NodeShape .

role:Role a sh:NodeShape .

identity:AddressFacet sh:targetClass identity:AddressFacet .

tool:BuildFacet rdfs:subClassOf core:Facet .

pattern:LogicalPattern sh:targetClass pattern:LogicalPattern .

_:node1gm7uj6vjx9 sh:nodeKind sh:IRI .

core:Annotation rdfs:subClassOf core:Assertion .

<https://ontology.unifiedcyberontology.org/uco/uco> owl:imports analysis:1.1.0 .

<https://ontology.unifiedcyberontology.org/uco/action> rdfs:comment "This ontology defines classes and properties for characterizing actions."@en-us .

_:node1gm7uj6vjx13 sh:datatype xsd:string .

tool:BuildFacet rdfs:label "BuildFacet"@en .

_:node1gm7uj6vjx8 sh:path configuration:dependencies .

configuration:Configuration sh:property _:node1gm7uj6vjx8 .

_:node1gm7uj6vjx12 rdf:first "ldap"^^vocabulary:AccountTypeVocab ;
	rdf:rest _:node1gm7uj6vjx16 .

_:node1gm7uj6vjx11 sh:maxCount 1 .

role:Role rdfs:subClassOf core:UcoObject .

_:node1gm7uj6vjx14 a sh:SPARQLConstraint .

identity:AffiliationFacet a owl:Class .

core:Annotation rdfs:label "Annotation"@en .

uco-co:firstItem-subjects-previousItem-shape a sh:PropertyShape .

pattern:Pattern a owl:Class .

_:node1gm7uj6vjx13 sh:nodeKind sh:Literal .

_:node1gm7uj6vjx9 sh:path analysis:originatingAnalysis .

role:Role rdfs:label "Role"@en .

analysis:AnalyticResult sh:property _:node1gm7uj6vjx9 .

identity:AffiliationFacet a sh:NodeShape .

_:node1gm7uj6vjx15 sh:datatype xsd:string .

_:node1gm7uj6vjx11 sh:nodeKind sh:Literal .

<https://ontology.unifiedcyberontology.org/uco/action> owl:backwardCompatibleWith action:1.0.0 .

<https://ontology.unifiedcyberontology.org/uco/uco> owl:imports configuration:1.1.0 .

pattern:Pattern a sh:NodeShape .

_:node1gm7uj6vjx16 rdf:first "nis"^^vocabulary:AccountTypeVocab ;
	rdf:rest _:node1gm7uj6vjx18 .

_:node1gm7uj6vjx13 sh:path marking:contentSelectors .

<https://ontology.unifiedcyberontology.org/uco/action> owl:imports core:1.1.0 .

_:node1gm7uj6vjx11 sh:path location:pdop .

marking:GranularMarking sh:property _:node1gm7uj6vjx13 .

_:node1gm7uj6vjx15 sh:nodeKind sh:Literal .

_:node1gm7uj6vjx17 sh:class core:UcoObject .

location:GPSCoordinatesFacet sh:property _:node1gm7uj6vjx11 .

tool:BuildFacet rdfs:comment "A build facet is a grouping of characteristics unique to a particular version of a software."@en .

<https://ontology.unifiedcyberontology.org/uco/action> owl:imports location:1.1.0 , pattern:1.1.0 .

role:Role rdfs:comment "A role is a usual or customary function based on contextual perspective."@en .

<https://ontology.unifiedcyberontology.org/uco/uco> owl:imports core:1.1.0 .

pattern:Pattern rdfs:subClassOf core:UcoObject .

<https://ontology.unifiedcyberontology.org/uco/action> owl:imports types:1.1.0 .

types:ControlledDictionary rdfs:comment "A controlled dictionary is a list of (term/key, value) pairs where each term/key exists no more than once and is constrained to an explicitly defined set of values."@en .

_:node1gm7uj6vjx17 sh:nodeKind sh:IRI .

core:Annotation rdfs:comment "An annotation is an assertion made in relation to one or more objects."@en .

identity:AffiliationFacet rdfs:subClassOf identity:IdentityFacet .

uco-co:firstItem-subjects-previousItem-shape sh:description "The first item in a list must not have a previous item."@en .

_:node1gm7uj6vjx18 rdf:first "openid"^^vocabulary:AccountTypeVocab ;
	rdf:rest _:node1gm7uj6vjx21 .

role:Role sh:targetClass role:Role .

<https://ontology.unifiedcyberontology.org/uco/action> owl:imports vocabulary:1.1.0 .

_:node1gm7uj6vjx19 sh:datatype xsd:decimal .

<https://ontology.unifiedcyberontology.org/uco/uco> owl:imports identity:1.1.0 .

_:node1gm7uj6vjx20 sh:class tool:BuildInformationType .

marking:GranularMarking sh:targetClass marking:GranularMarking .

_:node1gm7uj6vjx15 sh:path configuration:usageContextAssumptions .

pattern:Pattern rdfs:label "Pattern"@en .

configuration:Configuration sh:property _:node1gm7uj6vjx15 .

identity:AffiliationFacet rdfs:label "AffiliationFacet"@en .

_:node1gm7uj6vjx17 sh:path analysis:resultContent .

analysis:AnalyticResult sh:property _:node1gm7uj6vjx17 .

uco-co:firstItem-subjects-previousItem-shape sh:maxCount 0 .

<https://ontology.unifiedcyberontology.org/uco/action> owl:priorVersion action:1.0.0 .

<https://ontology.unifiedcyberontology.org/uco/uco> owl:imports location:1.1.0 .

_:node1gm7uj6vjx23 sh:class core:UcoObject .

_:node1gm7uj6vjx21 rdf:first "radius"^^vocabulary:AccountTypeVocab .

_:node1gm7uj6vjx20 sh:maxCount 1 .

_:node1gm7uj6vjx21 rdf:rest _:node1gm7uj6vjx24 .

_:node1gm7uj6vjx19 sh:maxCount 1 .

_:node1gm7uj6vjx22 sh:class types:ControlledDictionaryEntry .

marking:LicenseMarking a owl:Class .

<https://ontology.unifiedcyberontology.org/uco/action> owl:versionIRI action:1.1.0 .

_:node1gm7uj6vjx25 rdf:first co:firstItem .

configuration:Configuration sh:targetClass configuration:Configuration .

_:node1gm7uj6vjx25 rdf:rest _:node1gm7uj6vjx26 .

_:node1gm7uj6vjx20 sh:nodeKind sh:IRI .

<https://ontology.unifiedcyberontology.org/uco/uco> owl:imports marking:1.1.0 .

_:node1gm7uj6vjx23 sh:minCount 1 .

marking:LicenseMarking a sh:NodeShape .

analysis:AnalyticResult sh:targetClass analysis:AnalysicResult .

_:node1gm7uj6vjx19 sh:nodeKind sh:Literal .

_:node1gm7uj6vjx26 rdf:first co:previousItem .

_:node1gm7uj6vjx22 sh:path types:entry .

_:node1gm7uj6vjx26 rdf:rest rdf:nil .

uco-co:firstItem-subjects-previousItem-shape sh:path _:node1gm7uj6vjx25 .

types:ControlledDictionary sh:property _:node1gm7uj6vjx22 .

_:node1gm7uj6vjx24 rdf:first "tacacs"^^vocabulary:AccountTypeVocab ;
	rdf:rest _:node1gm7uj6vjx27 .

_:node1gm7uj6vjx14 rdfs:comment "This requirement is determined from review of the canonical parsing process in Section 3 of the OWL 2 mapping to RDF.  All references to owl:Axioms are identified as blank nodes.  Therefore, any non-blank node that is an owl:Axiom will not be mapped and consumed by the mapping process."@en .

pattern:Pattern rdfs:comment "A pattern is a combination of properties, acts, tendencies, etc., forming a consistent or characteristic arrangement."@en .

<https://ontology.unifiedcyberontology.org/uco/uco> owl:imports observable:1.1.0 .

identity:AffiliationFacet rdfs:comment "An affiliation is a grouping of characteristics unique to the established affiliations of an entity."@en .

<https://ontology.unifiedcyberontology.org/uco/uco> owl:imports pattern:1.1.0 .

_:node1gm7uj6vjx23 sh:nodeKind sh:IRI .

configuration:ConfigurationEntry a owl:Class .

action:Action a owl:Class .

<https://ontology.unifiedcyberontology.org/uco/uco> owl:imports role:1.1.0 .

analysis:AnalyticResultFacet a owl:Class .

pattern:Pattern sh:targetClass pattern:Pattern .

marking:LicenseMarking rdfs:subClassOf marking:MarkingModel .

_:node1gm7uj6vjx20 sh:path tool:buildInformation .

tool:BuildFacet sh:property _:node1gm7uj6vjx20 .

_:node1gm7uj6vjx19 sh:path location:tdop .

action:Action a sh:NodeShape .

location:GPSCoordinatesFacet sh:property _:node1gm7uj6vjx19 .

configuration:ConfigurationEntry a sh:NodeShape .

_:node1gm7uj6vjx23 sh:path core:object .

_:node1gm7uj6vjx27 rdf:first "unix"^^vocabulary:AccountTypeVocab .

core:Annotation sh:property _:node1gm7uj6vjx23 .

_:node1gm7uj6vjx27 rdf:rest _:node1gm7uj6vjx29 .

identity:AffiliationFacet sh:targetClass identity:AffiliationFacet .

analysis:AnalyticResultFacet a sh:NodeShape .

types:ControlledDictionary sh:targetClass types:ControlledDictionary .

uco-co:firstItem-subjects-previousItem-shape sh:targetSubjectsOf co:firstItem .

<https://ontology.unifiedcyberontology.org/uco/uco> owl:imports time:1.1.0 .

marking:LicenseMarking rdfs:label "License Marking"@en .

tool:BuildFacet sh:targetClass tool:BuildFacet .

action:Action rdfs:subClassOf core:UcoObject .

_:node1gm7uj6vjx28 sh:datatype xsd:decimal .

pattern:PatternExpression a owl:Class .

core:Annotation sh:targetClass core:Annotation .

analysis:AnalyticResultFacet rdfs:subClassOf core:Facet .

_:node1gm7uj6vjx29 rdf:first "windows_domain"^^vocabulary:AccountTypeVocab ;
	rdf:rest _:node1gm7uj6vjx30 .

action:Action rdfs:label "Action"@en .

pattern:PatternExpression a sh:NodeShape .

<https://ontology.unifiedcyberontology.org/uco/uco> owl:imports tool:1.1.0 .

_:node1gm7uj6vjx14 rdfs:seeAlso <https://www.w3.org/TR/2012/REC-owl2-mapping-to-rdf-20121211/#Mapping_from_RDF_Graphs_to_the_Structural_Specification> .

identity:BirthInformationFacet a owl:Class .

configuration:ConfigurationEntry rdfs:subClassOf core:UcoInherentCharacterizationThing .

<https://ontology.unifiedcyberontology.org/uco/observable> a owl:Ontology .

types:ControlledDictionaryEntry a owl:Class .

_:node1gm7uj6vjx28 sh:maxCount 1 .

tool:BuildInformationType a owl:Class .

core:Assertion a owl:Class .

identity:BirthInformationFacet a sh:NodeShape .

analysis:AnalyticResultFacet rdfs:label "AnalyticResultFacet"@en .

uco-co:firstItem-subjects-shape a sh:PropertyShape .

_:node1gm7uj6vjx30 rdf:first "windows_local"^^vocabulary:AccountTypeVocab .

<https://ontology.unifiedcyberontology.org/uco/uco> owl:imports types:1.1.0 .

types:ControlledDictionaryEntry a sh:NodeShape .

_:node1gm7uj6vjx30 rdf:rest rdf:nil .

_:node1gm7uj6vjx10 owl:oneOf _:node1gm7uj6vjx12 .

vocabulary:AccountTypeVocab owl:equivalentClass _:node1gm7uj6vjx10 .

tool:BuildInformationType a sh:NodeShape .

core:Assertion a sh:NodeShape .

<https://ontology.unifiedcyberontology.org/uco/observable> rdfs:label "uco-observable"@en .

action:Action rdfs:comment "An action is something that may be done or performed."@en .

_:node1gm7uj6vjx14 sh:message "An owl:Axiom must be a blank node."@en .

configuration:ConfigurationEntry rdfs:label "ConfigurationEntry"@en .

_:node1gm7uj6vjx28 sh:nodeKind sh:Literal .

pattern:PatternExpression rdfs:subClassOf core:UcoInherentCharacterizationThing .

uco-co:firstItem-subjects-shape sh:class co:ListItem .

<https://ontology.unifiedcyberontology.org/uco/uco> owl:imports victim:1.1.0 .

identity:BirthInformationFacet rdfs:subClassOf identity:IdentityFacet .

types:ControlledDictionaryEntry rdfs:subClassOf types:DictionaryEntry .

core:Assertion rdfs:subClassOf core:UcoObject .

_:node1gm7uj6vjx28 sh:path location:vdop .

location:GPSCoordinatesFacet sh:property _:node1gm7uj6vjx28 .

<https://ontology.unifiedcyberontology.org/uco/observable> owl:backwardCompatibleWith observable:1.0.0 .

pattern:PatternExpression rdfs:label "PatternExpression"@en .

_:node1gm7uj6vjx31 sh:class action:Action .

vocabulary:ActionArgumentNameVocab a rdfs:Datatype .

identity:BirthInformationFacet rdfs:label "BirthInformationFacet"@en .

tool:BuildInformationType rdfs:subClassOf core:UcoInherentCharacterizationThing .

uco-co:firstItem-subjects-shape sh:maxCount 1 .

types:ControlledDictionaryEntry rdfs:label "ControlledDictionaryEntry"@en .

<https://ontology.unifiedcyberontology.org/uco/uco> owl:imports vocabulary:1.1.0 .

analysis:AnalyticResultFacet rdfs:comment "An analytic result facet is a grouping of characteristics unique to the results of an analysis action."@en .

core:Assertion rdfs:label "Assertion"@en .

marking:LicenseMarking rdfs:comment "A license marking is a grouping of characteristics unique to the expression of data marking definitions (restrictions, permissions, and other guidance for how data can be used and shared) to convey details of license restrictions that apply to the data."@en-us .

_:node1gm7uj6vjx14 sh:select """
			PREFIX owl: <http://www.w3.org/2002/07/owl#>
			SELECT $this
			WHERE {
				$this a owl:Axiom .
				FILTER isIRI($this)
			}
		""" .

uco-owl:Axiom-shape sh:sparql _:node1gm7uj6vjx14 .

_:node1gm7uj6vjx31 sh:nodeKind sh:IRI .

tool:BuildInformationType rdfs:label "BuildInformationType"@en .

configuration:ConfigurationEntry rdfs:comment "A configuration entry is a grouping of characteristics unique to a particular parameter or initial setting for the use of a tool, application, software, or other cyber object."@en .

<https://ontology.unifiedcyberontology.org/uco/observable> owl:imports action:1.1.0 .

vocabulary:ActionArgumentNameVocab rdfs:label "Action Argument Name Vocabulary"@en-us .

uco-co:firstItem-subjects-shape sh:nodeKind sh:BlankNodeOrIRI .

core:Assertion rdfs:comment "An assertion is a statement declared to be true."@en .

location:GPSCoordinatesFacet sh:targetClass location:GPSCoordinatesFacet .

uco-owl:Axiom-shape sh:targetClass owl:Axiom .

identity:BirthInformationFacet rdfs:comment "Birth information is a grouping of characteristics unique to information pertaining to the birth of an entity."@en .

_:node1gm7uj6vjx31 sh:path action:subaction .

<https://ontology.unifiedcyberontology.org/uco/observable> owl:imports configuration:1.1.0 .

action:Action sh:property _:node1gm7uj6vjx31 .

<https://ontology.unifiedcyberontology.org/uco/uco> owl:priorVersion <https://ontology.unifiedcyberontology.org/uco/uco/1.0.0> .

analysis:AnalyticResultFacet sh:targetClass analysis:AnalyticResultFacet .

types:ControlledDictionaryEntry rdfs:comment "A controlled dictionary entry is a single (term/key, value) pair where the term/key is constrained to an explicitly defined set of values."@en .

_:node1gm7uj6vjx32 sh:datatype xsd:string .

pattern:PatternExpression rdfs:comment "A pattern expression is a grouping of characteristics unique to an explicit logical expression defining a pattern (e.g., regular expression, SQL Select expression, etc.)."@en .

vocabulary:ActionArgumentNameVocab rdfs:comment "Defines an open-vocabulary for common arguments of cyber actions."@en .

<https://ontology.unifiedcyberontology.org/uco/observable> owl:imports core:1.1.0 .

uco-co:firstItem-subjects-shape sh:path co:firstItem .

tool:BuildInformationType rdfs:comment "A build information type is a grouping of characteristics that describe how a particular version of software was converted from source code to executable code."@en .

<https://ontology.unifiedcyberontology.org/uco/observable> owl:imports identity:1.1.0 .

<https://ontology.unifiedcyberontology.org/uco/uco> owl:versionIRI <https://ontology.unifiedcyberontology.org/uco/uco/1.1.0> .

_:node1gm7uj6vjx35 sh:datatype xsd:string .

_:node1gm7uj6vjx33 sh:class core:UcoObject .

_:node1gm7uj6vjx34 sh:class core:UcoObject .

_:node1gm7uj6vjx32 sh:hasValue "license" .

uco-owl:DataOneOf-shape a sh:NodeShape .

location:LatLongCoordinatesFacet a owl:Class .

analysis:ArtifactClassification a owl:Class .

<https://ontology.unifiedcyberontology.org/uco/observable> owl:imports location:1.1.0 .

<https://ontology.unifiedcyberontology.org/uco/uco> owl:versionInfo "1.1.0" .

_:node1gm7uj6vjx36 sh:datatype xsd:dateTime .

uco-co:firstItem-subjects-shape sh:targetSubjectsOf co:firstItem .

<https://ontology.unifiedcyberontology.org/uco/observable> owl:imports types:1.1.0 .

_:node1gm7uj6vjx32 sh:nodeKind sh:Literal .

_:node1gm7uj6vjx35 sh:nodeKind sh:Literal .

_:node1gm7uj6vjx38 a rdfs:Datatype .

pattern:PatternExpression sh:targetClass pattern:PatternExpression .

location:LatLongCoordinatesFacet a sh:NodeShape .

analysis:ArtifactClassification a sh:NodeShape .

types:ControlledDictionaryEntry sh:targetClass types:ControlledDictionaryEntry .

_:node1gm7uj6vjx33 sh:nodeKind sh:BlankNodeOrIRI .

_:node1gm7uj6vjx34 sh:maxCount 1 .

<https://ontology.unifiedcyberontology.org/uco/observable> owl:imports vocabulary:1.1.0 .

_:node1gm7uj6vjx37 sh:class configuration:Configuration .

_:node1gm7uj6vjx36 sh:maxCount 1 .

_:node1gm7uj6vjx39 a sh:SPARQLConstraint .

_:node1gm7uj6vjx35 sh:path core:statement .

core:Assertion sh:property _:node1gm7uj6vjx35 .

_:node1gm7uj6vjx34 sh:nodeKind sh:IRI .

_:node1gm7uj6vjx38 owl:onDatatype xsd:string .

_:node1gm7uj6vjx32 sh:path marking:definitionType .

marking:LicenseMarking sh:property _:node1gm7uj6vjx32 .

_:node1gm7uj6vjx33 sh:path configuration:itemObject .

configuration:ConfigurationEntry sh:property _:node1gm7uj6vjx33 .

types:Dictionary a owl:Class .

location:LatLongCoordinatesFacet rdfs:subClassOf core:Facet .

_:node1gm7uj6vjx37 sh:maxCount 1 .

_:node1gm7uj6vjx36 sh:nodeKind sh:Literal .

<https://ontology.unifiedcyberontology.org/uco/observable> owl:priorVersion observable:1.0.0 .

types:Dictionary a sh:NodeShape .

pattern:patternExpression a owl:DatatypeProperty .

uco-co:followedBy-subjects-shape a sh:PropertyShape .

core:Assertion sh:targetClass core:Assertion .

_:node1gm7uj6vjx40 sh:datatype xsd:string .

_:node1gm7uj6vjx34 sh:path action:environment .

_:node1gm7uj6vjx37 sh:nodeKind sh:IRI .

action:Action sh:property _:node1gm7uj6vjx34 .

analysis:ArtifactClassification rdfs:subClassOf core:UcoInherentCharacterizationThing .

_:node1gm7uj6vjx41 sh:datatype xsd:string .

location:LatLongCoordinatesFacet rdfs:label "LatLongCoordinatesFacet"@en .

_:node1gm7uj6vjx36 sh:path identity:birthdate .

identity:BirthInformationFacet sh:property _:node1gm7uj6vjx36 .

_:node1gm7uj6vjx39 rdfs:comment "This requirement is determined from review of the canonical parsing process in Section 3.2.4, Table 12, row 4 of the OWL 2 mapping to RDF.  All datatypes using owl:oneOf must be blank nodes.  Any non-blank node will not be mapped and consumed by the mapping process.  See also DataOneOf in the OWL 2 Syntax document, especially with 'Show RDF in Examples' turned on."@en .

_:node1gm7uj6vjx37 sh:path tool:buildConfiguration .

<https://ontology.unifiedcyberontology.org/uco/observable> owl:versionIRI observable:1.1.0 .

tool:BuildInformationType sh:property _:node1gm7uj6vjx37 .

uco-co:followedBy-subjects-shape sh:class co:Item .

_:node1gm7uj6vjx42 rdf:first "APC Address"^^vocabulary:ActionArgumentNameVocab .

_:node1gm7uj6vjx44 sh:class tool:BuildUtilityType .

_:node1gm7uj6vjx42 rdf:rest _:node1gm7uj6vjx45 .

pattern:patternExpression rdfs:label "patternExpression"@en .

analysis:ArtifactClassification rdfs:label "ArtifactClassification"@en .

_:node1gm7uj6vjx40 sh:maxCount 1 .

_:node1gm7uj6vjx44 sh:maxCount 1 .

location:LatLongCoordinatesFacet rdfs:comment "A lat long coordinates facet is a grouping of characteristics unique to the expression of a geolocation as the intersection of specific latitude, longitude, and altitude values."@en .

_:node1gm7uj6vjx43 sh:class core:UcoObject .

uco-co:followedBy-subjects-shape sh:description "This shape encodes in SHACL that co:followedBy has range co:Item (induced via the propertyChainAxiom on co:item and superproperty relationship with co:nextItem)."@en .

observable:API a owl:Class .

_:node1gm7uj6vjx41 sh:maxCount 1 .

core:AttributedName a owl:Class .

types:Dictionary rdfs:subClassOf core:UcoInherentCharacterizationThing .

pattern:patternExpression rdfs:comment "An explicit logical pattern expression."@en .

_:node1gm7uj6vjx44 sh:nodeKind sh:IRI .

identity:BirthInformationFacet sh:targetClass identity:BirthInformationFacet .

observable:API a sh:NodeShape .

_:node1gm7uj6vjx39 rdfs:seeAlso <https://www.w3.org/TR/owl2-mapping-to-rdf/#Parsing_of_Expressions> .

core:AttributedName a sh:NodeShape .

_:node1gm7uj6vjx43 sh:maxCount 1 .

_:node1gm7uj6vjx40 sh:minCount 1 .

types:Dictionary rdfs:label "Dictionary"@en .

_:node1gm7uj6vjx41 sh:nodeKind sh:Literal .

_:node1gm7uj6vjx46 sh:datatype xsd:decimal .

uco-co:followedBy-subjects-shape sh:nodeKind sh:BlankNodeOrIRI .

_:node1gm7uj6vjx39 rdfs:seeAlso <https://www.w3.org/TR/owl2-syntax/#Enumeration_of_Literals> .

analysis:ArtifactClassification rdfs:comment "An artifact classification is a single specific assertion that a particular class of a classification taxonomy applies to something."@en .

_:node1gm7uj6vjx45 rdf:first "APC Mode"^^vocabulary:ActionArgumentNameVocab ;
	rdf:rest _:node1gm7uj6vjx47 .

_:node1gm7uj6vjx44 sh:path tool:buildUtility .

tool:BuildInformationType sh:property _:node1gm7uj6vjx44 .

_:node1gm7uj6vjx43 sh:nodeKind sh:IRI .

pattern:patternExpression rdfs:range pattern:PatternExpression .

core:AttributedName rdfs:subClassOf core:UcoObject .

_:node1gm7uj6vjx40 sh:nodeKind sh:Literal .

observable:API rdfs:subClassOf observable:ObservableObject .

identity:CountryOfResidenceFacet a owl:Class .

uco-co:followedBy-subjects-shape sh:path co:followedBy .

types:Dictionary rdfs:comment "A dictionary is list of (term/key, value) pairs with each term/key existing no more than once."@en .

_:node1gm7uj6vjx41 sh:path configuration:itemDescription .

_:node1gm7uj6vjx46 sh:maxCount 1 .

configuration:ConfigurationEntry sh:property _:node1gm7uj6vjx41 .

_:node1gm7uj6vjx39 sh:message "For data ranges that are sets of literals, owl:oneOf must only be used on blank nodes." .

_:node1gm7uj6vjx43 sh:path action:performer .

core:AttributedName rdfs:label "AttributedName"@en .

action:Action sh:property _:node1gm7uj6vjx43 .

observable:API rdfs:label "API"@en .

identity:CountryOfResidenceFacet a sh:NodeShape .

_:node1gm7uj6vjx48 sh:class tool:CompilerType .

_:node1gm7uj6vjx47 rdf:first "API"^^vocabulary:ActionArgumentNameVocab ;
	rdf:rest _:node1gm7uj6vjx53 .

_:node1gm7uj6vjx40 sh:path marking:license .

_:node1gm7uj6vjx49 sh:datatype xsd:decimal .

marking:LicenseMarking sh:property _:node1gm7uj6vjx40 .

_:node1gm7uj6vjx46 sh:nodeKind sh:Literal .

uco-co:followedBy-subjects-shape sh:targetSubjectsOf co:followedBy .

_:node1gm7uj6vjx50 sh:datatype xsd:string .

_:node1gm7uj6vjx48 sh:nodeKind sh:IRI .

_:node1gm7uj6vjx51 sh:class core:UcoObject .

_:node1gm7uj6vjx39 sh:select """
			PREFIX rdfs: <http://www.w3.org/2000/01/rdf-schema#>
			SELECT $this
			WHERE {
				$this a rdfs:Datatype .
				FILTER ( isIRI($this) )
			}
		""" .

uco-owl:DataOneOf-shape sh:sparql _:node1gm7uj6vjx39 .

core:AttributedName rdfs:comment "An attributed name is a name of an entity issued by some attributed naming authority."@en .

_:node1gm7uj6vjx52 sh:class types:DictionaryEntry .

identity:CountryOfResidenceFacet rdfs:subClassOf identity:IdentityFacet .

_:node1gm7uj6vjx46 sh:path location:altitude .

location:LatLongCoordinatesFacet sh:property _:node1gm7uj6vjx46 .

_:node1gm7uj6vjx48 sh:path tool:compilers .

marking:LicenseMarking sh:targetClass marking:LicenseMarking .

tool:BuildInformationType sh:property _:node1gm7uj6vjx48 .

_:node1gm7uj6vjx51 sh:nodeKind sh:IRI .

_:node1gm7uj6vjx53 rdf:first "Access Mode"^^vocabulary:ActionArgumentNameVocab .

_:node1gm7uj6vjx50 sh:maxCount 1 .

_:node1gm7uj6vjx49 sh:maxCount 1 .

_:node1gm7uj6vjx53 rdf:rest _:node1gm7uj6vjx57 .

observable:API rdfs:comment "An API (application programming interface) is a computing interface that defines interactions between multiple software or mixed hardware-software intermediaries. It defines the kinds of calls or requests that can be made, how to make them, the data formats that should be used, the conventions to follow, etc. [based on https://en.wikipedia.org/wiki/API]"@en .

uco-owl:DataOneOf-shape sh:targetSubjectsOf owl:oneOf .

identity:CountryOfResidenceFacet rdfs:label "CountryOfResidenceFacet"@en .

uco-co:index-subjects-shape a sh:PropertyShape .

_:node1gm7uj6vjx52 sh:minCount 1 .

_:node1gm7uj6vjx54 sh:datatype xsd:string .

_:node1gm7uj6vjx51 sh:path action:error .

action:Action sh:property _:node1gm7uj6vjx51 .

_:node1gm7uj6vjx56 sh:class tool:LibraryType .

_:node1gm7uj6vjx50 sh:nodeKind sh:Literal .

_:node1gm7uj6vjx49 sh:nodeKind sh:Literal .

_:node1gm7uj6vjx55 sh:datatype xsd:decimal .

observable:API sh:targetClass observable:API .

identity:CountryOfResidenceFacet rdfs:comment "Country of residence is a grouping of characteristics unique to information related to the country, or countries, where an entity resides."@en .

marking:MarkingDefinition a owl:Class .

_:node1gm7uj6vjx52 sh:nodeKind sh:IRI .

marking:MarkingDefinition a sh:NodeShape .

_:node1gm7uj6vjx56 sh:nodeKind sh:IRI .

_:node1gm7uj6vjx58 sh:class core:UcoObject .

_:node1gm7uj6vjx54 sh:maxCount 1 .

_:node1gm7uj6vjx57 rdf:first "Application Name"^^vocabulary:ActionArgumentNameVocab ;
	rdf:rest _:node1gm7uj6vjx59 .

uco-co:index-subjects-shape sh:datatype xsd:positiveInteger .

_:node1gm7uj6vjx50 sh:path configuration:itemName .

uco-owl:DatatypeProperty-shacl-constraints-shape a sh:NodeShape .

_:node1gm7uj6vjx52 sh:path types:entry .

configuration:ConfigurationEntry sh:property _:node1gm7uj6vjx50 .

observable:ARPCache a owl:Class .

_:node1gm7uj6vjx56 sh:path tool:libraries .

types:Dictionary sh:property _:node1gm7uj6vjx52 .

_:node1gm7uj6vjx49 sh:path analysis:classificationConfidence .

tool:BuildInformationType sh:property _:node1gm7uj6vjx56 .

analysis:ArtifactClassification sh:property _:node1gm7uj6vjx49 .

_:node1gm7uj6vjx55 sh:maxCount 1 .

_:node1gm7uj6vjx58 sh:nodeKind sh:IRI .

identity:CountryOfResidenceFacet sh:targetClass identity:CountryOfResidenceFacet .

_:node1gm7uj6vjx54 sh:nodeKind sh:Literal .

uco-co:index-subjects-shape sh:nodeKind sh:Literal .

observable:ARPCache a sh:NodeShape .

marking:MarkingDefinition rdfs:subClassOf core:MarkingDefinitionAbstraction .

_:node1gm7uj6vjx62 a sh:SPARQLConstraint .

_:node1gm7uj6vjx59 rdf:first "Base Address"^^vocabulary:ActionArgumentNameVocab .

_:node1gm7uj6vjx60 sh:datatype xsd:string .

_:node1gm7uj6vjx59 rdf:rest _:node1gm7uj6vjx64 .

_:node1gm7uj6vjx55 sh:nodeKind sh:Literal .

uco-co:index-subjects-shape sh:path co:index .

_:node1gm7uj6vjx63 sh:datatype xsd:string .

_:node1gm7uj6vjx61 sh:datatype xsd:dateTime .

_:node1gm7uj6vjx58 sh:path action:instrument .

types:Dictionary sh:targetClass types:Dictionary .

observable:ARPCache rdfs:subClassOf observable:ObservableObject .

_:node1gm7uj6vjx54 sh:path core:namingAuthority .

action:Action sh:property _:node1gm7uj6vjx58 .

core:AttributedName sh:property _:node1gm7uj6vjx54 .

identity:EventsFacet a owl:Class .

marking:MarkingDefinition rdfs:label "MarkingDefinition"@en .

_:node1gm7uj6vjx64 rdf:first "Callback Address"^^vocabulary:ActionArgumentNameVocab .

_:node1gm7uj6vjx55 sh:path location:latitude .

_:node1gm7uj6vjx64 rdf:rest _:node1gm7uj6vjx66 .

uco-co:index-subjects-shape sh:targetSubjectsOf co:index .

location:LatLongCoordinatesFacet sh:property _:node1gm7uj6vjx55 .

_:node1gm7uj6vjx60 sh:maxCount 1 .

observable:ARPCache rdfs:label "ARPCache"@en .

_:node1gm7uj6vjx63 sh:minCount 1 .

identity:EventsFacet a sh:NodeShape .

_:node1gm7uj6vjx65 sh:class core:UcoObject .

_:node1gm7uj6vjx61 sh:maxCount 1 .

_:node1gm7uj6vjx62 sh:message "An OWL Datatype Property cannot use a SHACL ClassConstraintComponent."@en .

types:DictionaryEntry a owl:Class .

_:node1gm7uj6vjx67 sh:datatype xsd:decimal .

_:node1gm7uj6vjx63 sh:nodeKind sh:Literal .

_:node1gm7uj6vjx60 sh:nodeKind sh:Literal .

types:DictionaryEntry a sh:NodeShape .

core:AttributedName sh:targetClass core:AttributedName .

_:node1gm7uj6vjx65 sh:nodeKind sh:IRI .

identity:EventsFacet rdfs:subClassOf identity:IdentityFacet .

_:node1gm7uj6vjx61 sh:nodeKind sh:Literal .

uco-co:item-subjects-shape a sh:PropertyShape .

_:node1gm7uj6vjx63 sh:path analysis:class .

_:node1gm7uj6vjx66 rdf:first "Code Address"^^vocabulary:ActionArgumentNameVocab ;
	rdf:rest _:node1gm7uj6vjx68 .

analysis:ArtifactClassification sh:property _:node1gm7uj6vjx63 .

_:node1gm7uj6vjx67 sh:maxCount 1 .

_:node1gm7uj6vjx65 sh:path action:object .

_:node1gm7uj6vjx60 sh:path configuration:itemType .

action:Action sh:property _:node1gm7uj6vjx65 .

uco-co:item-subjects-shape sh:class co:Item .

configuration:ConfigurationEntry sh:property _:node1gm7uj6vjx60 .

identity:EventsFacet rdfs:label "EventsFacet"@en .

core:Bundle a owl:Class .

_:node1gm7uj6vjx61 sh:path tool:compilationDate .

tool:BuildInformationType sh:property _:node1gm7uj6vjx61 .

_:node1gm7uj6vjx67 sh:nodeKind sh:Literal .

core:Bundle a sh:NodeShape .

_:node1gm7uj6vjx69 sh:class core:UcoObject .

_:node1gm7uj6vjx62 sh:select """
				PREFIX rdf: <http://www.w3.org/1999/02/22-rdf-syntax-ns#>
				PREFIX sh: <http://www.w3.org/ns/shacl#>
				SELECT $this ?value
				WHERE {
					?value
						sh:class ?nClass ;
						sh:path / rdf:rest* ?nLastSequenceMember ;
						.
					?nLastSequenceMember
						rdf:first $this ;
						rdf:rest rdf:nil ;
						.
				}
			""" .

uco-owl:DatatypeProperty-shacl-constraints-shape sh:sparql _:node1gm7uj6vjx62 .

_:node1gm7uj6vjx70 sh:datatype xsd:string .

types:DictionaryEntry rdfs:subClassOf core:UcoInherentCharacterizationThing .

marking:MarkingDefinition rdfs:comment "A marking definition is a grouping of characteristics unique to the expression of a specific data marking conveying restrictions, permissions, and other guidance for how marked data can be used and shared."@en .

uco-co:item-subjects-shape sh:nodeKind sh:BlankNodeOrIRI .

analysis:ArtifactClassification sh:targetClass analysis:ArtifactClassification .

_:node1gm7uj6vjx68 rdf:first "Command"^^vocabulary:ActionArgumentNameVocab .

_:node1gm7uj6vjx71 sh:datatype xsd:string .

_:node1gm7uj6vjx68 rdf:rest _:node1gm7uj6vjx73 .

_:node1gm7uj6vjx67 sh:path location:longitude .

location:LatLongCoordinatesFacet sh:property _:node1gm7uj6vjx67 .

_:node1gm7uj6vjx69 sh:nodeKind sh:IRI .

uco-co:item-subjects-shape sh:path co:item .

_:node1gm7uj6vjx72 a sh:SPARQLConstraint .

types:DictionaryEntry rdfs:label "DictionaryEntry"@en .

core:Bundle rdfs:subClassOf core:EnclosingCompilation .

_:node1gm7uj6vjx70 sh:nodeKind sh:Literal .

observable:ARPCache rdfs:comment "An ARP cache is a collection of Address Resolution Protocol (ARP) entries (mostly dynamic) that are created when an IP address is resolved to a MAC address (so the computer can effectively communicate with the IP address). [based on https://en.wikipedia.org/wiki/ARP_cache]"@en .

_:node1gm7uj6vjx71 sh:maxCount 1 .

identity:EventsFacet rdfs:comment "Events is a grouping of characteristics unique to information related to specific relevant things that happen in the lifetime of an entity."@en .

_:node1gm7uj6vjx69 sh:path action:participant .

_:node1gm7uj6vjx73 rdf:first "Control Code"^^vocabulary:ActionArgumentNameVocab .

_:node1gm7uj6vjx74 sh:class marking:MarkingModel .

core:Bundle rdfs:label "Bundle"@en .

_:node1gm7uj6vjx73 rdf:rest _:node1gm7uj6vjx75 .

action:Action sh:property _:node1gm7uj6vjx69 .

uco-co:item-subjects-shape sh:targetSubjectsOf co:item .

_:node1gm7uj6vjx70 sh:path configuration:itemValue .

configuration:ConfigurationEntry sh:property _:node1gm7uj6vjx70 .

types:DictionaryEntry rdfs:comment "A dictionary entry is a single (term/key, value) pair."@en .

observable:ARPCache sh:targetClass observable:ARPCache .

_:node1gm7uj6vjx71 sh:nodeKind sh:Literal .

location:LatLongCoordinatesFacet sh:targetClass location:LatLongCoordinatesFacet .

identity:EventsFacet sh:targetClass identity:EventsFacet .

_:node1gm7uj6vjx74 sh:nodeKind sh:IRI .

analysis:ArtifactClassificationResultFacet a owl:Class .

_:node1gm7uj6vjx76 sh:class core:UcoObject .

_:node1gm7uj6vjx72 sh:message "An OWL Datatype Property must not permit a non-Literal value via SHACL constraints."@en .

_:node1gm7uj6vjx75 rdf:first "Control Parameter"^^vocabulary:ActionArgumentNameVocab ;
	rdf:rest _:node1gm7uj6vjx78 .

analysis:ArtifactClassificationResultFacet a sh:NodeShape .

_:node1gm7uj6vjx71 sh:path tool:buildID .

tool:BuildInformationType sh:property _:node1gm7uj6vjx71 .

_:node1gm7uj6vjx74 sh:path marking:definition .

core:Bundle rdfs:comment "A bundle is a container for a grouping of UCO content with no presumption of shared context."@en .

_:node1gm7uj6vjx76 sh:nodeKind sh:IRI .

uco-co:itemContent-subjects-shape a sh:NodeShape .

configuration:ConfigurationEntry sh:targetClass configuration:ConfigurationEntry .

marking:MarkingDefinition sh:property _:node1gm7uj6vjx74 .

_:node1gm7uj6vjx77 sh:datatype xsd:string .

identity:IdentifierFacet a owl:Class .

location:Location a owl:Class .

observable:ARPCacheEntry a owl:Class .

_:node1gm7uj6vjx79 sh:datatype xsd:string .

_:node1gm7uj6vjx78 rdf:first "Creation Flags"^^vocabulary:ActionArgumentNameVocab ;
	rdf:rest _:node1gm7uj6vjx82 .

_:node1gm7uj6vjx76 sh:path action:result .

action:Action sh:property _:node1gm7uj6vjx76 .

analysis:ArtifactClassificationResultFacet rdfs:subClassOf analysis:AnalyticResultFacet .

core:Bundle sh:targetClass core:Bundle .

identity:IdentifierFacet a sh:NodeShape .

location:Location a sh:NodeShape .

_:node1gm7uj6vjx80 sh:datatype xsd:string .

observable:ARPCacheEntry a sh:NodeShape .

_:node1gm7uj6vjx81 a sh:PropertyShape .

_:node1gm7uj6vjx77 sh:maxCount 1 .

_:node1gm7uj6vjx85 sh:class location:Location .

_:node1gm7uj6vjx79 sh:maxCount 1 .

_:node1gm7uj6vjx81 sh:class co:Item .

analysis:ArtifactClassificationResultFacet rdfs:label "ArtifactClassificationResultFacet"@en .

_:node1gm7uj6vjx82 rdf:first "Database Name"^^vocabulary:ActionArgumentNameVocab .

core:Compilation a owl:Class .

identity:IdentifierFacet rdfs:subClassOf identity:IdentityFacet .

_:node1gm7uj6vjx82 rdf:rest _:node1gm7uj6vjx87 .

location:Location rdfs:subClassOf core:UcoObject .

_:node1gm7uj6vjx85 sh:nodeKind sh:IRI .

_:node1gm7uj6vjx77 sh:minCount 1 .

observable:ARPCacheEntry rdfs:subClassOf observable:ObservableObject .

core:Compilation a sh:NodeShape .

_:node1gm7uj6vjx80 sh:maxCount 1 .

_:node1gm7uj6vjx72 sh:select """
				PREFIX rdf: <http://www.w3.org/1999/02/22-rdf-syntax-ns#>
				PREFIX sh: <http://www.w3.org/ns/shacl#>
				SELECT $this ?value
				WHERE {
					?value
						sh:path / rdf:rest* ?nLastSequenceMember ;
						.
					?nLastSequenceMember
						rdf:first $this ;
						rdf:rest rdf:nil ;
						.

					{ ?value sh:nodeKind sh:BlankNode . }
					UNION
					{ ?value sh:nodeKind sh:BlankNodeOrIRI . }
					UNION
					{ ?value sh:nodeKind sh:BlankNodeOrLiteral . }
					UNION
					{ ?value sh:nodeKind sh:IRI . }
					UNION
					{ ?value sh:nodeKind sh:IRIOrLiteral . }
				}
			""" .

_:node1gm7uj6vjx86 sh:maxCount 0 .

uco-owl:DatatypeProperty-shacl-constraints-shape sh:sparql _:node1gm7uj6vjx72 .

_:node1gm7uj6vjx79 sh:nodeKind sh:Literal .

location:Location rdfs:label "Location"@en .

identity:IdentifierFacet rdfs:label "IdentifierFacet"@en .

_:node1gm7uj6vjx85 sh:path action:location .

_:node1gm7uj6vjx77 sh:nodeKind sh:Literal .

action:Action sh:property _:node1gm7uj6vjx85 .

observable:ARPCacheEntry rdfs:label "ARPCacheEntry"@en .

core:Compilation rdfs:subClassOf core:UcoObject .

_:node1gm7uj6vjx87 rdf:first "Delay Time (ms)"^^vocabulary:ActionArgumentNameVocab ;
	rdf:rest _:node1gm7uj6vjx89 .

_:node1gm7uj6vjx79 sh:path tool:buildLabel .

tool:BuildInformationType sh:property _:node1gm7uj6vjx79 .

_:node1gm7uj6vjx77 sh:path types:key .

_:node1gm7uj6vjx80 sh:minCount 1 .

uco-owl:DatatypeProperty-shacl-constraints-shape sh:targetClass owl:DatatypeProperty .

_:node1gm7uj6vjx86 sh:path configuration:itemObject .

_:node1gm7uj6vjx88 sh:datatype xsd:dateTime .

types:DictionaryEntry sh:property _:node1gm7uj6vjx77 .

_:node1gm7uj6vjx84 sh:property _:node1gm7uj6vjx86 .

_:node1gm7uj6vjx81 sh:description "This shape encodes in SHACL that the range of co:itemContent is the complement of co:Item."@en .

core:Compilation rdfs:label "Compilation"@en .

_:node1gm7uj6vjx90 sh:datatype xsd:string .

_:node1gm7uj6vjx91 sh:datatype xsd:string .

_:node1gm7uj6vjx80 sh:nodeKind sh:Literal .

_:node1gm7uj6vjx89 rdf:first "Destination Address"^^vocabulary:ActionArgumentNameVocab ;
	rdf:rest _:node1gm7uj6vjx93 .

_:node1gm7uj6vjx81 sh:path co:itemContent .

_:node1gm7uj6vjx88 sh:maxCount 1 .

location:Location rdfs:comment "A location is a geospatial place, site, or position."@en .

uco-co:itemContent-subjects-shape sh:not _:node1gm7uj6vjx81 .

_:node1gm7uj6vjx92 sh:maxCount 0 .

analysis:ArtifactClassificationResultFacet rdfs:comment "An artifact classification result facet is a grouping of characteristics unique to the results of an artifact classification analysis action."@en .

uco-owl:Disjointedness-AP-DP-shape a sh:NodeShape .

_:node1gm7uj6vjx90 sh:maxCount 1 .

_:node1gm7uj6vjx88 sh:nodeKind sh:Literal .

core:Compilation rdfs:comment "A compilation is a grouping of things."@en .

_:node1gm7uj6vjx91 sh:maxCount 1 .

_:node1gm7uj6vjx80 sh:path marking:definitionType .

identity:IdentifierFacet rdfs:comment "Identifier is a grouping of characteristics unique to information that uniquely and specifically identities an entity."@en .

marking:MarkingDefinition sh:property _:node1gm7uj6vjx80 .

location:Location sh:targetClass location:Location .

_:node1gm7uj6vjx94 a sh:PropertyShape .

_:node1gm7uj6vjx88 sh:path action:endTime .

_:node1gm7uj6vjx92 sh:path configuration:itemValue .

observable:ARPCacheEntry rdfs:comment "An ARP cache entry is a single Address Resolution Protocol (ARP) response record that is created when an IP address is resolved to a MAC address (so the computer can effectively communicate with the IP address). [based on https://en.wikipedia.org/wiki/ARP_cache]"@en .

_:node1gm7uj6vjx93 rdf:first "Error Control"^^vocabulary:ActionArgumentNameVocab .

action:Action sh:property _:node1gm7uj6vjx88 .

_:node1gm7uj6vjx93 rdf:rest _:node1gm7uj6vjx97 .

_:node1gm7uj6vjx96 a sh:SPARQLConstraint .

_:node1gm7uj6vjx91 sh:minCount 1 .

_:node1gm7uj6vjx84 sh:property _:node1gm7uj6vjx92 .

_:node1gm7uj6vjx90 sh:nodeKind sh:Literal .

_:node1gm7uj6vjx83 rdf:first _:node1gm7uj6vjx84 ;
	rdf:rest _:node1gm7uj6vjx99 .

identity:IdentifierFacet sh:targetClass identity:IdentifierFacet .

observable:ARPCacheEntry sh:targetClass observable:ARPCacheEntry .

marking:MarkingDefinition sh:targetClass marking:MarkingDefinition .

core:Compilation sh:targetClass core:Compilation .

_:node1gm7uj6vjx98 sh:datatype xsd:dateTime .

location:SimpleAddressFacet a owl:Class .

_:node1gm7uj6vjx91 sh:nodeKind sh:Literal .

_:node1gm7uj6vjx95 sh:class analysis:ArtifactClassification .

_:node1gm7uj6vjx90 sh:path tool:buildOutputLog .

tool:BuildInformationType sh:property _:node1gm7uj6vjx90 .

location:SimpleAddressFacet a sh:NodeShape .

identity:Identity a owl:Class .

observable:Account a owl:Class .

_:node1gm7uj6vjx91 sh:path types:value .

types:DictionaryEntry sh:property _:node1gm7uj6vjx91 .

_:node1gm7uj6vjx97 rdf:first "File Information Class"^^vocabulary:ActionArgumentNameVocab .

_:node1gm7uj6vjx98 sh:maxCount 1 .

_:node1gm7uj6vjx97 rdf:rest _:node1gm7uj6vjx103 .

marking:MarkingModel a owl:Class .

identity:Identity a sh:NodeShape .

_:node1gm7uj6vjx95 sh:nodeKind sh:IRI .

observable:Account a sh:NodeShape .

_:node1gm7uj6vjx96 rdfs:seeAlso <https://www.w3.org/TR/2012/REC-owl2-syntax-20121211/#Typing_Constraints_of_OWL_2_DL> .

_:node1gm7uj6vjx102 sh:datatype xsd:string .

_:node1gm7uj6vjx101 sh:minCount 1 .

core:ConfidenceFacet a owl:Class .

_:node1gm7uj6vjx94 sh:description "This shape encodes in SHACL that co:itemContent is an OWL FunctionalProperty (giving the sh:maxCount constraint)."@en .

location:SimpleAddressFacet rdfs:subClassOf core:Facet .

marking:MarkingModel a sh:NodeShape .

_:node1gm7uj6vjx98 sh:nodeKind sh:Literal .

core:ConfidenceFacet a sh:NodeShape .

_:node1gm7uj6vjx102 sh:maxCount 1 .

identity:Identity rdfs:subClassOf core:IdentityAbstraction .

types:DictionaryEntry sh:targetClass types:DictionaryEntry .

_:node1gm7uj6vjx95 sh:path analysis:classification .

_:node1gm7uj6vjx101 sh:path configuration:itemObject .

_:node1gm7uj6vjx103 rdf:first "Flags"^^vocabulary:ActionArgumentNameVocab .

analysis:ArtifactClassificationResultFacet sh:property _:node1gm7uj6vjx95 .

_:node1gm7uj6vjx98 sh:path action:startTime .

core:ConfidenceFacet rdfs:subClassOf core:Facet .

observable:Account rdfs:subClassOf observable:ObservableObject .

location:SimpleAddressFacet rdfs:label "SimpleAddressFacet"@en .

_:node1gm7uj6vjx103 rdf:rest _:node1gm7uj6vjx104 .

_:node1gm7uj6vjx100 sh:property _:node1gm7uj6vjx101 .

action:Action sh:property _:node1gm7uj6vjx98 .

_:node1gm7uj6vjx102 sh:nodeKind sh:Literal .

_:node1gm7uj6vjx94 sh:maxCount 1 .

_:node1gm7uj6vjx99 rdf:first _:node1gm7uj6vjx100 .

_:node1gm7uj6vjx96 sh:message "An IRI may not be a member of both an owl:AnnotationProperty and owl:DatatypeProperty."@en .

marking:MarkingModel rdfs:subClassOf core:UcoInherentCharacterizationThing .

_:node1gm7uj6vjx99 rdf:rest _:node1gm7uj6vjx106 .

identity:Identity rdfs:label "Identity"@en .

types:Hash a owl:Class .

observable:Account rdfs:label "Account"@en .

_:node1gm7uj6vjx96 sh:select """
			PREFIX owl: <http://www.w3.org/2002/07/owl#>
			SELECT $this
			WHERE {
				$this a owl:DatatypeProperty ;
			}
		""" .

core:ConfidenceFacet rdfs:label "ConfidenceFacet"@en .

types:Hash a sh:NodeShape .

uco-owl:Disjointedness-AP-DP-shape sh:sparql _:node1gm7uj6vjx96 .

_:node1gm7uj6vjx102 sh:path tool:buildProject .

marking:MarkingModel rdfs:label "MarkingModel"@en .

tool:BuildInformationType sh:property _:node1gm7uj6vjx102 .

_:node1gm7uj6vjx94 sh:nodeKind sh:BlankNodeOrIRI .

_:node1gm7uj6vjx105 sh:datatype xsd:nonNegativeInteger .

analysis:ArtifactClassificationResultFacet sh:targetClass analysis:ArtifactClassificationResultFacet .

_:node1gm7uj6vjx104 rdf:first "Function Address"^^vocabulary:ActionArgumentNameVocab ;
	rdf:rest _:node1gm7uj6vjx110 .

_:node1gm7uj6vjx109 sh:datatype xsd:string .

_:node1gm7uj6vjx108 sh:minCount 1 .

_:node1gm7uj6vjx94 sh:path co:itemContent .

uco-owl:Disjointedness-AP-DP-shape sh:targetClass owl:AnnotationProperty .

uco-co:itemContent-subjects-shape sh:property _:node1gm7uj6vjx94 .

types:Hash rdfs:subClassOf core:UcoInherentCharacterizationThing .

_:node1gm7uj6vjx105 sh:maxCount 1 .

identity:Identity rdfs:comment "An identity is a grouping of identifying characteristics unique to an individual or organization."@en .

analysis:class a owl:DatatypeProperty .

_:node1gm7uj6vjx109 sh:maxCount 1 .

_:node1gm7uj6vjx108 sh:path configuration:itemValue .

location:SimpleAddressFacet rdfs:comment "A simple address facet is a grouping of characteristics unique to a geolocation expressed as an administrative address."@en .

types:Hash rdfs:label "Hash"@en .

_:node1gm7uj6vjx107 sh:property _:node1gm7uj6vjx108 .

uco-co:itemContent-subjects-shape sh:targetSubjectsOf co:itemContent .

_:node1gm7uj6vjx110 rdf:first "Function Name"^^vocabulary:ActionArgumentNameVocab .

_:node1gm7uj6vjx106 rdf:first _:node1gm7uj6vjx107 .

_:node1gm7uj6vjx105 sh:nodeKind sh:Literal .

_:node1gm7uj6vjx106 rdf:rest rdf:nil .

configuration:ConfigurationEntry sh:xone _:node1gm7uj6vjx83 .

_:node1gm7uj6vjx110 rdf:rest _:node1gm7uj6vjx111 .

analysis:class rdfs:label "class"@en .

observable:Account rdfs:comment "An account is an arrangement with an entity to enable and control the provision of some capability or service."@en .

identity:Identity sh:targetClass identity:Identity .

_:node1gm7uj6vjx109 sh:nodeKind sh:Literal .

uco-owl:Disjointedness-AP-OP-shape a sh:NodeShape .

_:node1gm7uj6vjx105 sh:path action:actionCount .

action:Action sh:property _:node1gm7uj6vjx105 .

observable:Account sh:targetClass observable:Account .

_:node1gm7uj6vjx109 sh:path tool:buildScript .

_:node1gm7uj6vjx112 sh:datatype xsd:string .

tool:BuildInformationType sh:property _:node1gm7uj6vjx109 .

core:ConfidenceFacet rdfs:comment "A confidence is a grouping of characteristics unique to an asserted level of certainty in the accuracy of some information."@en .

identity:IdentityFacet a owl:Class .

configuration:Dependency a owl:Class .

_:node1gm7uj6vjx111 rdf:first "Function Ordinal"^^vocabulary:ActionArgumentNameVocab .

_:node1gm7uj6vjx113 a sh:SPARQLConstraint .

analysis:class rdfs:comment "A specific classification class."@en .

_:node1gm7uj6vjx111 rdf:rest _:node1gm7uj6vjx116 .

uco-co:lastItem-subjects-shape sh:class co:ListItem .

identity:IdentityFacet a sh:NodeShape .

configuration:Dependency a sh:NodeShape .

_:node1gm7uj6vjx115 sh:datatype xsd:string .

_:node1gm7uj6vjx112 sh:maxCount 1 .

analysis:class rdfs:range xsd:string .

marking:MarkingModel rdfs:comment "A marking model is a grouping of characteristics unique to the expression of a particular form of data marking definitions (restrictions, permissions, and other guidance for how data can be used and shared)."@en .

_:node1gm7uj6vjx114 sh:datatype vocabulary:ActionStatusTypeVocab .

identity:IdentityFacet rdfs:subClassOf core:Facet .

_:node1gm7uj6vjx117 sh:datatype xsd:nonNegativeInteger .

uco-co:lastItem-subjects-shape sh:maxCount 1 .

_:node1gm7uj6vjx115 sh:maxCount 1 .

_:node1gm7uj6vjx116 rdf:first "Hook Type"^^vocabulary:ActionArgumentNameVocab .

_:node1gm7uj6vjx112 sh:nodeKind sh:Literal .

observable:AccountAuthenticationFacet a owl:Class .

_:node1gm7uj6vjx116 rdf:rest _:node1gm7uj6vjx118 .

_:node1gm7uj6vjx113 rdfs:seeAlso <https://www.w3.org/TR/2012/REC-owl2-syntax-20121211/#Typing_Constraints_of_OWL_2_DL> .

marking:MarkingModel sh:targetClass marking:MarkingModel .

observable:AccountAuthenticationFacet a sh:NodeShape .

identity:IdentityFacet rdfs:label "IdentityFacet"@en .

_:node1gm7uj6vjx115 sh:nodeKind sh:Literal .

analysis:classification a owl:ObjectProperty .

configuration:Dependency rdfs:subClassOf core:UcoInherentCharacterizationThing .

_:node1gm7uj6vjx117 sh:maxCount 1 .

uco-co:lastItem-subjects-shape sh:nodeKind sh:BlankNodeOrIRI .

_:node1gm7uj6vjx112 sh:path location:addressType .

_:node1gm7uj6vjx114 sh:message "Value is outside the default vocabulary ActionStatusTypeVocab." .

location:SimpleAddressFacet sh:property _:node1gm7uj6vjx112 .

observable:AccountAuthenticationFacet rdfs:subClassOf core:Facet .

_:node1gm7uj6vjx118 rdf:first "Host Name"^^vocabulary:ActionArgumentNameVocab .

_:node1gm7uj6vjx115 sh:path tool:buildVersion .

marking:ReleaseToMarking a owl:Class .

_:node1gm7uj6vjx118 rdf:rest _:node1gm7uj6vjx120 .

tool:BuildInformationType sh:property _:node1gm7uj6vjx115 .

configuration:Dependency rdfs:label "Dependency"@en .

uco-co:lastItem-subjects-shape sh:path co:lastItem .

analysis:classification rdfs:label "classification"@en .

_:node1gm7uj6vjx117 sh:minCount 1 .

marking:ReleaseToMarking a sh:NodeShape .

_:node1gm7uj6vjx114 sh:path action:actionStatus .

_:node1gm7uj6vjx119 sh:datatype xsd:string .

observable:AccountAuthenticationFacet rdfs:label "AccountAuthenticationFacet"@en .

_:node1gm7uj6vjx113 sh:message "An IRI may not be a member of both an owl:AnnotationProperty and owl:ObjectProperty."@en .

tool:BuildInformationType sh:targetClass tool:BuildInformationType .

_:node1gm7uj6vjx114 sh:severity sh:Info .

_:node1gm7uj6vjx120 rdf:first "Hostname"^^vocabulary:ActionArgumentNameVocab .

_:node1gm7uj6vjx117 sh:nodeKind sh:Literal .

_:node1gm7uj6vjx120 rdf:rest _:node1gm7uj6vjx121 .

action:Action sh:property _:node1gm7uj6vjx114 .

uco-co:lastItem-subjects-shape sh:targetSubjectsOf co:lastItem .

marking:ReleaseToMarking rdfs:subClassOf marking:MarkingModel .

_:node1gm7uj6vjx113 sh:select """
			PREFIX owl: <http://www.w3.org/2002/07/owl#>
			SELECT $this
			WHERE {
				$this a owl:ObjectProperty ;
			}
		""" .

identity:IdentityFacet rdfs:comment "An identity facet is a grouping of characteristics unique to a particular aspect of an identity."@en .

uco-owl:Disjointedness-AP-OP-shape sh:sparql _:node1gm7uj6vjx113 .

_:node1gm7uj6vjx119 sh:maxCount 1 .

_:node1gm7uj6vjx117 sh:path core:confidence .

tool:BuildUtilityType a owl:Class .

core:ConfidenceFacet sh:property _:node1gm7uj6vjx117 .

marking:ReleaseToMarking rdfs:label "Release-To Marking"@en .

_:node1gm7uj6vjx122 sh:maxCount 1 .

identity:IdentityFacet sh:targetClass identity:IdentityFacet .

_:node1gm7uj6vjx119 sh:nodeKind sh:Literal .

_:node1gm7uj6vjx121 rdf:first "Initial Owner"^^vocabulary:ActionArgumentNameVocab .

analysis:classification rdfs:comment "An asserted classification of an analyzed artifact resulting from the analysis."@en .

tool:BuildUtilityType a sh:NodeShape .

types:Hash rdfs:comment "A hash is a grouping of characteristics unique to the result of applying a mathematical algorithm that maps data of arbitrary size to a bit string (the 'hash') and is a one-way function, that is, a function which is practically infeasible to invert. This is commonly used for integrity checking of data. [based on https://en.wikipedia.org/wiki/Cryptographic_hash_function]"@en .

uco-owl:Disjointedness-AP-OP-shape sh:targetClass owl:AnnotationProperty .

_:node1gm7uj6vjx121 rdf:rest _:node1gm7uj6vjx123 .

uco-co:nextItem-subjects-shape a sh:PropertyShape .

_:node1gm7uj6vjx122 sh:nodeKind sh:Literal .

_:node1gm7uj6vjx119 sh:path location:country .

core:ConfidenceFacet sh:targetClass core:ConfidenceFacet .

configuration:Dependency rdfs:comment "A dependency is a grouping of characteristics unique to something that a tool or other software relies on to function as intended."@en .

uco-co:nextItem-subjects-shape sh:class co:Item .

location:SimpleAddressFacet sh:property _:node1gm7uj6vjx119 .

observable:AccountAuthenticationFacet rdfs:comment "An account authentication facet is a grouping of characteristics unique to the mechanism of accessing an account."@en .

identity:LanguagesFacet a owl:Class .

analysis:classification rdfs:range analysis:ArtifactClassification .

_:node1gm7uj6vjx124 sh:datatype xsd:hexBinary .

_:node1gm7uj6vjx123 rdf:first "Mapping Offset"^^vocabulary:ActionArgumentNameVocab ;
	rdf:rest _:node1gm7uj6vjx128 .

uco-owl:Disjointedness-C-DT-shape a sh:NodeShape .

tool:BuildUtilityType rdfs:subClassOf core:UcoInherentCharacterizationThing .

identity:LanguagesFacet a sh:NodeShape .

_:node1gm7uj6vjx127 sh:datatype xsd:string .

_:node1gm7uj6vjx124 sh:maxCount 1 .

_:node1gm7uj6vjx126 sh:datatype vocabulary:ActionStatusTypeVocab .

_:node1gm7uj6vjx125 rdf:first _:node1gm7uj6vjx126 ;
	rdf:rest _:node1gm7uj6vjx132 .

tool:BuildUtilityType rdfs:label "BuildUtilityType"@en .

_:node1gm7uj6vjx130 sh:datatype xsd:dateTime .

_:node1gm7uj6vjx131 a sh:SPARQLConstraint .

_:node1gm7uj6vjx129 sh:datatype xsd:string .

core:ContextualCompilation a owl:Class .

identity:LanguagesFacet rdfs:subClassOf identity:IdentityFacet .

_:node1gm7uj6vjx128 rdf:first "Number of Bytes Per Send"^^vocabulary:ActionArgumentNameVocab ;
	rdf:rest _:node1gm7uj6vjx134 .

_:node1gm7uj6vjx133 sh:datatype xsd:string .

_:node1gm7uj6vjx124 sh:minCount 1 .

analysis:classificationConfidence a owl:DatatypeProperty .

_:node1gm7uj6vjx127 sh:maxCount 1 .

core:ContextualCompilation a sh:NodeShape .

_:node1gm7uj6vjx132 rdf:first _:node1gm7uj6vjx133 ;
	rdf:rest rdf:nil .

_:node1gm7uj6vjx122 sh:or _:node1gm7uj6vjx125 .

_:node1gm7uj6vjx130 sh:maxCount 1 .

identity:LanguagesFacet rdfs:label "LanguagesFacet"@en .

_:node1gm7uj6vjx124 sh:nodeKind sh:Literal .

_:node1gm7uj6vjx129 sh:maxCount 1 .

_:node1gm7uj6vjx127 sh:nodeKind sh:Literal .

_:node1gm7uj6vjx134 rdf:first "Options"^^vocabulary:ActionArgumentNameVocab .

_:node1gm7uj6vjx122 sh:path action:actionStatus .

_:node1gm7uj6vjx130 sh:nodeKind sh:Literal .

_:node1gm7uj6vjx134 rdf:rest _:node1gm7uj6vjx135 .

action:Action sh:property _:node1gm7uj6vjx122 .

core:ContextualCompilation rdfs:subClassOf core:Compilation .

analysis:classificationConfidence rdfs:label "classificationConfidence"@en .

_:node1gm7uj6vjx131 rdfs:seeAlso <https://www.w3.org/TR/2012/REC-owl2-syntax-20121211/#Typing_Constraints_of_OWL_2_DL> .

_:node1gm7uj6vjx124 sh:path types:hashValue .

types:Hash sh:property _:node1gm7uj6vjx124 .

_:node1gm7uj6vjx129 sh:nodeKind sh:Literal .

_:node1gm7uj6vjx127 sh:path location:locality .

location:SimpleAddressFacet sh:property _:node1gm7uj6vjx127 .

_:node1gm7uj6vjx130 sh:path observable:passwordLastChanged .

observable:AccountAuthenticationFacet sh:property _:node1gm7uj6vjx130 .

_:node1gm7uj6vjx138 sh:datatype xsd:string .

_:node1gm7uj6vjx137 sh:datatype vocabulary:HashNameVocab .

_:node1gm7uj6vjx135 rdf:first "Parameter Address"^^vocabulary:ActionArgumentNameVocab .

uco-co:nextItem-subjects-shape sh:description "This shape encodes in SHACL that co:nextItem is a FunctionalProperty (giving the sh:maxCount constraint), and has range co:Item (induced via the propertyChainAxiom on co:item)."@en .

core:ContextualCompilation rdfs:label "ContextualCompilation"@en .

_:node1gm7uj6vjx135 rdf:rest _:node1gm7uj6vjx140 .

_:node1gm7uj6vjx129 sh:path configuration:dependencyDescription .

_:node1gm7uj6vjx139 sh:datatype xsd:string .

configuration:Dependency sh:property _:node1gm7uj6vjx129 .

tool:BuildUtilityType rdfs:comment "A build utility type characterizes the tool used to convert from source code to executable code for a particular version of software."@en .

_:node1gm7uj6vjx136 sh:message "Value is not member of the vocabulary ActionStatusTypeVocab." .

_:node1gm7uj6vjx131 sh:message "An IRI may not be a member of both an owl:Class and owl:Datatype."@en .

_:node1gm7uj6vjx138 sh:maxCount 1 .

uco-co:nextItem-subjects-shape sh:maxCount 1 .

analysis:classificationConfidence rdfs:comment "The level of confidence that a classification assertion is correct."@en .

_:node1gm7uj6vjx141 sh:datatype xsd:string .

_:node1gm7uj6vjx139 sh:maxCount 1 .

_:node1gm7uj6vjx140 rdf:first "Password"^^vocabulary:ActionArgumentNameVocab .

_:node1gm7uj6vjx131 sh:select """
			PREFIX owl: <http://www.w3.org/2002/07/owl#>
			SELECT $this
			WHERE {
				$this a owl:Datatype ;
			}
		""" .

_:node1gm7uj6vjx140 rdf:rest _:node1gm7uj6vjx145 .

uco-owl:Disjointedness-C-DT-shape sh:sparql _:node1gm7uj6vjx131 .

_:node1gm7uj6vjx137 sh:message "Value is outside the default vocabulary HashNameVocab." .

_:node1gm7uj6vjx142 sh:datatype xsd:string .

_:node1gm7uj6vjx138 sh:nodeKind sh:Literal .

analysis:classificationConfidence rdfs:range xsd:decimal .

_:node1gm7uj6vjx139 sh:nodeKind sh:Literal .

uco-owl:Disjointedness-C-DT-shape sh:targetClass owl:Class .

uco-co:nextItem-subjects-shape sh:nodeKind sh:BlankNodeOrIRI .

_:node1gm7uj6vjx144 sh:datatype vocabulary:ActionStatusTypeVocab .

_:node1gm7uj6vjx137 sh:path types:hashMethod .

_:node1gm7uj6vjx141 sh:maxCount 1 .

_:node1gm7uj6vjx138 sh:path location:postalCode .

_:node1gm7uj6vjx142 sh:maxCount 1 .

_:node1gm7uj6vjx139 sh:path observable:password .

_:node1gm7uj6vjx137 sh:severity sh:Info .

uco-co:nextItem-subjects-shape sh:path co:nextItem .

location:SimpleAddressFacet sh:property _:node1gm7uj6vjx138 .

observable:AccountAuthenticationFacet sh:property _:node1gm7uj6vjx139 .

types:Hash sh:property _:node1gm7uj6vjx137 .

_:node1gm7uj6vjx141 sh:nodeKind sh:Literal .

_:node1gm7uj6vjx145 rdf:first "Privilege Name"^^vocabulary:ActionArgumentNameVocab ;
	rdf:rest _:node1gm7uj6vjx150 .

uco-owl:Disjointedness-DP-OP-shape a sh:NodeShape .

analysis:originatingAnalysis a owl:ObjectProperty .

_:node1gm7uj6vjx142 sh:nodeKind sh:Literal .

_:node1gm7uj6vjx147 sh:datatype xsd:string .

uco-co:nextItem-subjects-shape sh:targetSubjectsOf co:nextItem .

identity:LanguagesFacet rdfs:comment "Languages is a grouping of characteristics unique to specific syntactically and grammatically standardized forms of communication (human or computer) in which an entity has proficiency (comprehends, speaks, reads, or writes)."@en .

_:node1gm7uj6vjx146 rdf:first "Complete/Finish"^^vocabulary:ActionStatusTypeVocab .

_:node1gm7uj6vjx148 sh:datatype xsd:string .

_:node1gm7uj6vjx146 rdf:rest _:node1gm7uj6vjx152 .

_:node1gm7uj6vjx141 sh:path configuration:dependencyType .

_:node1gm7uj6vjx149 sh:maxCount 1 .

core:ContextualCompilation rdfs:comment "A contextual compilation is a grouping of things sharing some context (e.g., a set of network connections observed on a given day, all accounts associated with a given person)."@en .

configuration:Dependency sh:property _:node1gm7uj6vjx141 .

analysis:originatingAnalysis rdfs:label "originatingAnalysis"@en .

marking:ReleaseToMarking rdfs:comment "A release-to marking is a grouping of characteristics unique to the expression of data marking definitions (restrictions, permissions, and other guidance for how data can be used and shared) to convey details of authorized persons and/or organizations to which to the associated content may be released. The existence of the Release-To marking restricts access to ONLY those identities explicitly listed, regardless of whether another data marking exists that allows sharing with other members of the community."@en-us .

_:node1gm7uj6vjx151 a sh:SPARQLConstraint .

_:node1gm7uj6vjx142 sh:path tool:buildUtilityName .

tool:BuildUtilityType sh:property _:node1gm7uj6vjx142 .

_:node1gm7uj6vjx147 sh:maxCount 1 .

identity:LanguagesFacet sh:targetClass identity:LanguagesFacet .

_:node1gm7uj6vjx150 rdf:first "Protection"^^vocabulary:ActionArgumentNameVocab .

_:node1gm7uj6vjx153 sh:class core:UcoObject .

_:node1gm7uj6vjx150 rdf:rest _:node1gm7uj6vjx156 .

analysis:originatingAnalysis rdfs:comment "The analysis action that resulted in an analytic result."@en .

_:node1gm7uj6vjx154 sh:datatype xsd:string .

configuration:Dependency sh:targetClass configuration:Dependency .

_:node1gm7uj6vjx149 sh:minCount 1 .

_:node1gm7uj6vjx155 sh:datatype xsd:string .

uco-co:precededBy-subjects-shape a sh:PropertyShape .

_:node1gm7uj6vjx152 rdf:first "Error"^^vocabulary:ActionStatusTypeVocab .

_:node1gm7uj6vjx148 sh:maxCount 1 .

_:node1gm7uj6vjx152 rdf:rest _:node1gm7uj6vjx157 .

_:node1gm7uj6vjx147 sh:nodeKind sh:Literal .

_:node1gm7uj6vjx151 rdfs:seeAlso <https://www.w3.org/TR/2012/REC-owl2-syntax-20121211/#Typing_Constraints_of_OWL_2_DL> .

uco-co:precededBy-subjects-shape sh:class co:Item .

analysis:originatingAnalysis rdfs:range analysis:Analysis .

_:node1gm7uj6vjx153 sh:minCount 1 .

_:node1gm7uj6vjx149 sh:nodeKind sh:Literal .

_:node1gm7uj6vjx155 sh:hasValue "release-to" .

identity:NationalityFacet a owl:Class .

_:node1gm7uj6vjx154 sh:maxCount 1 .

_:node1gm7uj6vjx148 sh:nodeKind sh:Literal .

_:node1gm7uj6vjx147 sh:path location:region .

location:SimpleAddressFacet sh:property _:node1gm7uj6vjx147 .

_:node1gm7uj6vjx151 sh:message "An IRI may not be a member of both owl:DatatypeProperty and owl:ObjectProperty."@en .

identity:NationalityFacet a sh:NodeShape .

_:node1gm7uj6vjx153 sh:nodeKind sh:IRI .

configuration:configurationEntry a owl:ObjectProperty .

_:node1gm7uj6vjx157 rdf:first "Fail"^^vocabulary:ActionStatusTypeVocab .

_:node1gm7uj6vjx156 rdf:first "Proxy Bypass"^^vocabulary:ActionArgumentNameVocab .

_:node1gm7uj6vjx157 rdf:rest _:node1gm7uj6vjx161 .

_:node1gm7uj6vjx154 sh:nodeKind sh:Literal .

_:node1gm7uj6vjx155 sh:nodeKind sh:Literal .

_:node1gm7uj6vjx148 sh:path observable:passwordType .

_:node1gm7uj6vjx160 sh:datatype xsd:string .

_:node1gm7uj6vjx156 rdf:rest _:node1gm7uj6vjx162 .

_:node1gm7uj6vjx151 sh:select """
			PREFIX owl: <http://www.w3.org/2002/07/owl#>
			SELECT $this
			WHERE {
				$this a owl:ObjectProperty ;
			}
		""" .

observable:AccountAuthenticationFacet sh:property _:node1gm7uj6vjx148 .

_:node1gm7uj6vjx159 sh:datatype vocabulary:HashNameVocab .

uco-owl:Disjointedness-DP-OP-shape sh:sparql _:node1gm7uj6vjx151 .

analysis:resultContent a owl:ObjectProperty .

_:node1gm7uj6vjx158 rdf:first _:node1gm7uj6vjx159 .

identity:NationalityFacet rdfs:subClassOf identity:IdentityFacet .

_:node1gm7uj6vjx158 rdf:rest _:node1gm7uj6vjx163 .

_:node1gm7uj6vjx153 sh:path core:object .

core:ContextualCompilation sh:property _:node1gm7uj6vjx153 .

_:node1gm7uj6vjx154 sh:path tool:cpeid .

tool:BuildUtilityType sh:property _:node1gm7uj6vjx154 .

analysis:resultContent rdfs:label "resultContent"@en .

_:node1gm7uj6vjx155 sh:path marking:definitionType .

_:node1gm7uj6vjx164 sh:datatype xsd:string .

uco-owl:Disjointedness-DP-OP-shape sh:targetClass owl:DatatypeProperty .

marking:ReleaseToMarking sh:property _:node1gm7uj6vjx155 .

_:node1gm7uj6vjx160 sh:maxCount 1 .

identity:NationalityFacet rdfs:label "NationalityFacet"@en .

_:node1gm7uj6vjx161 rdf:first "Ongoing"^^vocabulary:ActionStatusTypeVocab .

_:node1gm7uj6vjx163 rdf:first _:node1gm7uj6vjx164 .

_:node1gm7uj6vjx165 sh:datatype xsd:string .

_:node1gm7uj6vjx163 rdf:rest rdf:nil .

_:node1gm7uj6vjx149 sh:or _:node1gm7uj6vjx158 .

_:node1gm7uj6vjx161 rdf:rest _:node1gm7uj6vjx167 .

configuration:configurationEntry rdfs:comment "A single configuration setting entry item for a tool or other software."@en .

observable:AccountAuthenticationFacet sh:targetClass observable:AccountAuthenticationFacet .

_:node1gm7uj6vjx162 rdf:first "Proxy Name"^^vocabulary:ActionArgumentNameVocab .

core:ContextualCompilation sh:targetClass core:ContextualCompilation .

_:node1gm7uj6vjx162 rdf:rest _:node1gm7uj6vjx168 .

_:node1gm7uj6vjx149 sh:path types:hashMethod .

types:Hash sh:property _:node1gm7uj6vjx149 .

_:node1gm7uj6vjx160 sh:nodeKind sh:Literal .

_:node1gm7uj6vjx166 sh:datatype xsd:string .

uco-owl:List-shape a sh:NodeShape .

uco-co:precededBy-subjects-shape sh:description "This shape encodes in SHACL that co:precededBy has range co:Item (induced via the propertyChainAxiom on co:item and superproperty relationship with co:previousItem)."@en .

observable:AccountFacet a owl:Class .

_:node1gm7uj6vjx167 rdf:first "Pending"^^vocabulary:ActionStatusTypeVocab .

_:node1gm7uj6vjx165 sh:maxCount 1 .

_:node1gm7uj6vjx167 rdf:rest _:node1gm7uj6vjx171 .

configuration:configurationEntry rdfs:range configuration:ConfigurationEntry .

analysis:resultContent rdfs:comment "Structured content expressing the results of an analysis action."@en .

core:ControlledVocabulary a owl:Class .

_:node1gm7uj6vjx160 sh:path location:street .

location:SimpleAddressFacet sh:property _:node1gm7uj6vjx160 .

_:node1gm7uj6vjx168 rdf:first "Reason"^^vocabulary:ActionArgumentNameVocab .

observable:AccountFacet a sh:NodeShape .

_:node1gm7uj6vjx168 rdf:rest _:node1gm7uj6vjx172 .

_:node1gm7uj6vjx170 a sh:PropertyShape .

core:ControlledVocabulary a sh:NodeShape .

_:node1gm7uj6vjx166 sh:minCount 1 .

_:node1gm7uj6vjx165 sh:nodeKind sh:Literal .

uco-co:precededBy-subjects-shape sh:nodeKind sh:BlankNodeOrIRI .

_:node1gm7uj6vjx169 sh:message "Value is not member of the vocabulary HashNameVocab." .

analysis:resultContent rdfs:range core:UcoObject .

identity:NationalityFacet rdfs:comment "Nationality is a grouping of characteristics unique to the condition of an entity belonging to a particular nation."@en .

observable:AccountFacet rdfs:subClassOf core:Facet .

_:node1gm7uj6vjx165 sh:path tool:swid .

location:SimpleAddressFacet sh:targetClass location:SimpleAddressFacet .

tool:BuildUtilityType sh:property _:node1gm7uj6vjx165 .

_:node1gm7uj6vjx171 rdf:first "Success"^^vocabulary:ActionStatusTypeVocab .

configuration:configurationEntry rdfs:seeAlso <https://github.com/ucoProject/UCO/issues/432> .

uco-co:precededBy-subjects-shape sh:path co:precededBy .

_:node1gm7uj6vjx171 rdf:rest _:node1gm7uj6vjx175 .

_:node1gm7uj6vjx166 sh:nodeKind sh:Literal .

_:node1gm7uj6vjx170 sh:maxCount 1 .

core:ControlledVocabulary rdfs:subClassOf core:UcoObject .

observable:AccountFacet rdfs:label "AccountFacet"@en .

_:node1gm7uj6vjx172 rdf:first "Request Size"^^vocabulary:ActionArgumentNameVocab ;
	rdf:rest _:node1gm7uj6vjx176 .

identity:NationalityFacet sh:targetClass identity:NationalityFacet .

_:node1gm7uj6vjx170 sh:path rdf:first .

uco-owl:List-shape sh:property _:node1gm7uj6vjx170 .

tool:BuildUtilityType sh:targetClass tool:BuildUtilityType .

core:ControlledVocabulary rdfs:label "ControlledVocabulary"@en .

_:node1gm7uj6vjx174 sh:datatype vocabulary:HashNameVocab .

uco-co:precededBy-subjects-shape sh:targetSubjectsOf co:precededBy .

location:addressType a owl:DatatypeProperty .

_:node1gm7uj6vjx166 sh:path marking:authorizedIdentities .

_:node1gm7uj6vjx175 rdf:first "Unknown"^^vocabulary:ActionStatusTypeVocab .

marking:ReleaseToMarking sh:property _:node1gm7uj6vjx166 .

_:node1gm7uj6vjx177 a sh:SPARQLConstraint .

_:node1gm7uj6vjx175 rdf:rest rdf:nil .

_:node1gm7uj6vjx144 sh:in _:node1gm7uj6vjx146 .

identity:OccupationFacet a owl:Class .

configuration:dependencies a owl:ObjectProperty .

_:node1gm7uj6vjx143 rdf:first _:node1gm7uj6vjx144 .

tool:CompilerType a owl:Class .

_:node1gm7uj6vjx176 rdf:first "Requested Version"^^vocabulary:ActionArgumentNameVocab .

_:node1gm7uj6vjx143 rdf:rest _:node1gm7uj6vjx179 .

_:node1gm7uj6vjx176 rdf:rest _:node1gm7uj6vjx181 .

location:addressType rdfs:label "addressType"@en .

identity:OccupationFacet a sh:NodeShape .

_:node1gm7uj6vjx178 rdf:first "MD5"^^vocabulary:HashNameVocab .

tool:CompilerType a sh:NodeShape .

_:node1gm7uj6vjx178 rdf:rest _:node1gm7uj6vjx182 .

marking:ReleaseToMarking sh:targetClass marking:ReleaseToMarking .

configuration:dependencies rdfs:label "dependencies"@en .

_:node1gm7uj6vjx180 sh:datatype xsd:string .

_:node1gm7uj6vjx179 rdf:first _:node1gm7uj6vjx180 ;
	rdf:rest rdf:nil .

_:node1gm7uj6vjx136 sh:or _:node1gm7uj6vjx143 .

uco-co:previousItem-subjects-shape a sh:PropertyShape .

identity:OccupationFacet rdfs:subClassOf identity:IdentityFacet .

_:node1gm7uj6vjx182 rdf:first "MD6"^^vocabulary:HashNameVocab .

core:ControlledVocabulary rdfs:comment "A controlled vocabulary is an explicitly constrained set of string values."@en .

_:node1gm7uj6vjx182 rdf:rest _:node1gm7uj6vjx183 .

uco-co:previousItem-subjects-shape sh:class co:Item .

_:node1gm7uj6vjx181 rdf:first "Server"^^vocabulary:ActionArgumentNameVocab .

_:node1gm7uj6vjx136 sh:path action:actionStatus .

observable:AccountFacet rdfs:comment "An account facet is a grouping of characteristics unique to an arrangement with an entity to enable and control the provision of some capability or service."@en .

action:Action sh:property _:node1gm7uj6vjx136 .

_:node1gm7uj6vjx181 rdf:rest _:node1gm7uj6vjx184 .

location:addressType rdfs:comment "The type of the address, for instance home or work."@en .

tool:CompilerType rdfs:subClassOf core:UcoInherentCharacterizationThing .

identity:OccupationFacet rdfs:label "OccupationFacet"@en .

marking:StatementMarking a owl:Class .

_:node1gm7uj6vjx183 rdf:first "SHA1"^^vocabulary:HashNameVocab .

location:addressType rdfs:range xsd:string .

marking:StatementMarking a sh:NodeShape .

_:node1gm7uj6vjx183 rdf:rest _:node1gm7uj6vjx187 .

tool:CompilerType rdfs:label "CompilerType"@en .

_:node1gm7uj6vjx185 sh:datatype xsd:anyURI .

_:node1gm7uj6vjx184 rdf:first "Service Name"^^vocabulary:ActionArgumentNameVocab .

action:Action sh:targetClass action:Action .

_:node1gm7uj6vjx184 rdf:rest _:node1gm7uj6vjx188 .

_:node1gm7uj6vjx186 sh:class core:UcoObject .

configuration:dependencies rdfs:comment "The relevant configuration dependencies for a tool, application, software, or other cyber object."@en .

_:node1gm7uj6vjx187 rdf:first "SHA224"^^vocabulary:HashNameVocab ;
	rdf:rest _:node1gm7uj6vjx189 .

location:altitude a owl:DatatypeProperty .

marking:StatementMarking rdfs:subClassOf marking:MarkingModel .

_:node1gm7uj6vjx185 sh:maxCount 1 .

_:node1gm7uj6vjx186 sh:maxCount 1 .

action:ActionArgumentFacet a owl:Class .

identity:OccupationFacet rdfs:comment "Occupation is a grouping of characteristics unique to the job or profession of an entity."@en .

location:altitude rdfs:label "altitude"@en .

configuration:dependencies rdfs:range configuration:Dependency .

action:ActionArgumentFacet a sh:NodeShape .

_:node1gm7uj6vjx186 sh:nodeKind sh:IRI .

marking:StatementMarking rdfs:label "Statement Marking"@en .

_:node1gm7uj6vjx188 rdf:first "Service State"^^vocabulary:ActionArgumentNameVocab .

_:node1gm7uj6vjx185 sh:nodeKind sh:Literal .

_:node1gm7uj6vjx189 rdf:first "SHA256"^^vocabulary:HashNameVocab .

_:node1gm7uj6vjx188 rdf:rest _:node1gm7uj6vjx190 .

_:node1gm7uj6vjx189 rdf:rest _:node1gm7uj6vjx191 .

identity:OccupationFacet sh:targetClass identity:OccupationFacet .

action:ActionArgumentFacet rdfs:subClassOf core:Facet .

_:node1gm7uj6vjx186 sh:path observable:accountIssuer .

observable:AccountFacet sh:property _:node1gm7uj6vjx186 .

location:altitude rdfs:comment "The altitude coordinate of a geolocation."@en .

_:node1gm7uj6vjx191 rdf:first "SHA384"^^vocabulary:HashNameVocab .

_:node1gm7uj6vjx185 sh:path core:constrainingVocabularyReference .

_:node1gm7uj6vjx191 rdf:rest _:node1gm7uj6vjx193 .

core:ControlledVocabulary sh:property _:node1gm7uj6vjx185 .

configuration:dependencyDescription a owl:DatatypeProperty .

action:ActionArgumentFacet rdfs:label "ActionArgumentFacet"@en .

_:node1gm7uj6vjx190 rdf:first "Service Type"^^vocabulary:ActionArgumentNameVocab .

location:altitude rdfs:range xsd:decimal .

_:node1gm7uj6vjx190 rdf:rest _:node1gm7uj6vjx195 .

identity:Organization a owl:Class .

_:node1gm7uj6vjx192 sh:class core:UcoObject .

uco-co:previousItem-subjects-shape sh:description "This shape encodes in SHACL that co:previousItem is a FunctionalProperty (giving the sh:maxCount constraint), and has range co:Item (induced via the propertyChainAxiom on co:item)."@en .

_:node1gm7uj6vjx193 rdf:first "SHA512"^^vocabulary:HashNameVocab .

_:node1gm7uj6vjx194 sh:datatype xsd:string .

identity:Organization a sh:NodeShape .

_:node1gm7uj6vjx193 rdf:rest _:node1gm7uj6vjx196 .

configuration:dependencyDescription rdfs:label "dependencyDescription"@en .

_:node1gm7uj6vjx192 sh:maxCount 1 .

location:country a owl:DatatypeProperty .

identity:Organization rdfs:subClassOf identity:Identity .

_:node1gm7uj6vjx192 sh:nodeKind sh:IRI .

location:country rdfs:label "country"@en .

_:node1gm7uj6vjx196 rdf:first "SSDEEP"^^vocabulary:HashNameVocab .

uco-co:previousItem-subjects-shape sh:maxCount 1 .

_:node1gm7uj6vjx194 sh:maxCount 1 .

_:node1gm7uj6vjx195 rdf:first "Share Mode"^^vocabulary:ActionArgumentNameVocab .

_:node1gm7uj6vjx196 rdf:rest rdf:nil .

_:node1gm7uj6vjx174 sh:in _:node1gm7uj6vjx178 .

_:node1gm7uj6vjx195 rdf:rest _:node1gm7uj6vjx197 .

_:node1gm7uj6vjx173 rdf:first _:node1gm7uj6vjx174 ;
	rdf:rest _:node1gm7uj6vjx198 .

_:node1gm7uj6vjx192 sh:path observable:owner .

observable:AccountFacet sh:property _:node1gm7uj6vjx192 .

identity:Organization rdfs:label "Organization"@en .

action:ActionArgumentFacet rdfs:comment "An action argument facet is a grouping of characteristics unique to a single parameter of an action."@en .

uco-co:previousItem-subjects-shape sh:nodeKind sh:BlankNodeOrIRI .

_:node1gm7uj6vjx199 sh:datatype xsd:string .

configuration:dependencyDescription rdfs:comment "A description of a tool or other software dependency."@en .

_:node1gm7uj6vjx198 rdf:first _:node1gm7uj6vjx199 ;
	rdf:rest rdf:nil .

_:node1gm7uj6vjx169 sh:or _:node1gm7uj6vjx173 .

_:node1gm7uj6vjx194 sh:minCount 1 .

location:country rdfs:comment "The name of the geolocation country."@en .

_:node1gm7uj6vjx200 sh:datatype xsd:boolean .

uco-co:previousItem-subjects-shape sh:path co:previousItem .

configuration:dependencyDescription rdfs:range xsd:string .

_:node1gm7uj6vjx197 rdf:first "Shutdown Flag"^^vocabulary:ActionArgumentNameVocab .

_:node1gm7uj6vjx177 rdfs:comment "This requirement is determined from review of the canonical parsing process in Section 3 of the OWL 2 mapping to RDF.  Table 5 removes any triple matching the pattern 'x a rdf:List`.  All other references throughout Section 3 to rdf:first are identified as blank nodes.  Therefore, any non-blank node that is an rdf:List will not be mapped and consumed by the mapping process, making the graph non-conformant with OWL 2 DL."@en .

_:node1gm7uj6vjx197 rdf:rest _:node1gm7uj6vjx202 .

_:node1gm7uj6vjx169 sh:path types:hashMethod .

_:node1gm7uj6vjx201 sh:datatype xsd:string .

location:country rdfs:range xsd:string .

types:Hash sh:property _:node1gm7uj6vjx169 .

_:node1gm7uj6vjx194 sh:nodeKind sh:Literal .

uco-co:previousItem-subjects-shape sh:targetSubjectsOf co:previousItem .

_:node1gm7uj6vjx194 sh:path core:value .

_:node1gm7uj6vjx200 sh:maxCount 1 .

types:Hash sh:targetClass types:Hash .

core:ControlledVocabulary sh:property _:node1gm7uj6vjx194 .

_:node1gm7uj6vjx201 sh:maxCount 1 .

location:hdop a owl:DatatypeProperty .

configuration:dependencyType a owl:DatatypeProperty .

_:node1gm7uj6vjx200 sh:nodeKind sh:Literal .

_:node1gm7uj6vjx202 rdf:first "Size (bytes)"^^vocabulary:ActionArgumentNameVocab ;
	rdf:rest _:node1gm7uj6vjx204 .

location:hdop rdfs:label "hdop"@en .

types:Identifier a rdfs:Datatype .

_:node1gm7uj6vjx203 sh:datatype xsd:string .

_:node1gm7uj6vjx201 sh:minCount 1 .

uco-co:size-subjects-shape a sh:PropertyShape .

configuration:dependencyType rdfs:label "dependencyType"@en .

_:node1gm7uj6vjx177 rdfs:seeAlso <https://www.w3.org/TR/2012/REC-owl2-mapping-to-rdf-20121211/#Mapping_from_RDF_Graphs_to_the_Structural_Specification> .

_:node1gm7uj6vjx200 sh:path observable:isActive .

observable:AccountFacet sh:property _:node1gm7uj6vjx200 .

_:node1gm7uj6vjx201 sh:nodeKind sh:Literal .

_:node1gm7uj6vjx203 sh:maxCount 1 .

uco-co:size-subjects-shape sh:datatype xsd:nonNegativeInteger .

tool:CompilerType rdfs:comment "A compiler type is a grouping of characteristics unique to a specific program that translates computer code written in one programming language (the source language) into another language (the target language). Typically a program that translates source code from a high-level programming language to a lower-level language (e.g., assembly language, object code, or machine code) to create an executable program. [based on https://en.wikipedia.org/wiki/Compiler]"@en .

_:node1gm7uj6vjx201 sh:path action:argumentName .

_:node1gm7uj6vjx205 sh:datatype xsd:dateTime .

_:node1gm7uj6vjx204 rdf:first "Sleep Time (ms)"^^vocabulary:ActionArgumentNameVocab .

action:ActionArgumentFacet sh:property _:node1gm7uj6vjx201 .

_:node1gm7uj6vjx204 rdf:rest _:node1gm7uj6vjx206 .

_:node1gm7uj6vjx203 sh:nodeKind sh:Literal .

location:hdop rdfs:comment "The horizontal dilution of precision of the GPS location."@en .

configuration:dependencyType rdfs:comment "The type of a tool or other software dependency."@en .

uco-co:size-subjects-shape sh:maxCount 1 .

_:node1gm7uj6vjx207 sh:datatype xsd:string .

_:node1gm7uj6vjx205 sh:maxCount 1 .

location:hdop rdfs:range xsd:decimal .

_:node1gm7uj6vjx208 sh:datatype xsd:string .

identity:Organization rdfs:comment "An organization is a grouping of identifying characteristics unique to a group of people who work together in an organized way for a shared purpose. [based on https://dictionary.cambridge.org/us/dictionary/english/organization]"@en .

types:Identifier rdfs:comment "An identifier is a string conformant to the specified UUID-based format for UCO object identifiers."@en .

_:node1gm7uj6vjx203 sh:path core:constrainingVocabularyName .

_:node1gm7uj6vjx177 sh:message "The subject of a triple with rdf:first as predicate must be a blank node."@en .

core:ControlledVocabulary sh:property _:node1gm7uj6vjx203 .

configuration:dependencyType rdfs:range xsd:string .

uco-co:size-subjects-shape sh:nodeKind sh:Literal .

_:node1gm7uj6vjx205 sh:nodeKind sh:Literal .

_:node1gm7uj6vjx177 sh:select """
			SELECT $this
			WHERE {
				FILTER isIRI($this)
			}
		""" .

_:node1gm7uj6vjx207 sh:maxCount 1 .

uco-owl:List-shape sh:sparql _:node1gm7uj6vjx177 .

_:node1gm7uj6vjx206 rdf:first "Source Address"^^vocabulary:ActionArgumentNameVocab .

_:node1gm7uj6vjx208 sh:maxCount 1 .

uco-co:size-subjects-shape sh:path co:size .

_:node1gm7uj6vjx206 rdf:rest _:node1gm7uj6vjx209 .

identity:Organization sh:targetClass identity:Organization .

types:NativeFormatString a rdfs:Datatype .

marking:StatementMarking rdfs:comment "A statement marking is a grouping of characteristics unique to the expression of data marking definitions (restrictions, permissions, and other guidance for how data can be used and shared) to convey details of a textual marking statement, (e.g., copyright) whose semantic meaning should apply to the associated content. Statement markings are generally not machine-readable. An example of this would be a simple marking to apply copyright information, such as 'Copyright 2014 Acme Inc.'."@en .

location:latitude a owl:DatatypeProperty .

_:node1gm7uj6vjx205 sh:path observable:expirationTime .

observable:AccountFacet sh:property _:node1gm7uj6vjx205 .

core:ControlledVocabulary sh:targetClass core:ControlledVocabulary .

_:node1gm7uj6vjx208 sh:nodeKind sh:Literal .

uco-owl:List-shape sh:targetSubjectsOf rdf:first .

_:node1gm7uj6vjx207 sh:minCount 1 .

location:latitude rdfs:label "latitude"@en .

uco-co:size-subjects-shape sh:targetSubjectsOf co:size .

_:node1gm7uj6vjx209 rdf:first "Starting Address"^^vocabulary:ActionArgumentNameVocab .

identity:OrganizationDetailsFacet a owl:Class .

_:node1gm7uj6vjx209 rdf:rest _:node1gm7uj6vjx213 .

configuration:isConfigurationOf a owl:ObjectProperty .

_:node1gm7uj6vjx210 sh:datatype xsd:dateTime .

_:node1gm7uj6vjx211 sh:datatype xsd:string .

_:node1gm7uj6vjx212 a owl:Axiom .

_:node1gm7uj6vjx207 sh:nodeKind sh:Literal .

identity:OrganizationDetailsFacet a sh:NodeShape .

_:node1gm7uj6vjx208 sh:path tool:compilerInformalDescription .

tool:CompilerType sh:property _:node1gm7uj6vjx208 .

location:latitude rdfs:comment "The latitude coordinate of a geolocation."@en .

configuration:isConfigurationOf a owl:IrreflexiveProperty .

core:EnclosingCompilation a owl:Class .

uco-owl:ObjectProperty-shacl-constraints-shape a sh:NodeShape .

_:node1gm7uj6vjx210 sh:maxCount 1 .

_:node1gm7uj6vjx207 sh:path action:value .

_:node1gm7uj6vjx211 sh:hasValue "statement" .

action:ActionArgumentFacet sh:property _:node1gm7uj6vjx207 .

_:node1gm7uj6vjx214 sh:datatype xsd:string .

core:EnclosingCompilation a sh:NodeShape .

location:latitude rdfs:range xsd:decimal .

identity:OrganizationDetailsFacet rdfs:subClassOf identity:IdentityFacet .

_:node1gm7uj6vjx213 rdf:first "System Metric Index"^^vocabulary:ActionArgumentNameVocab ;
	rdf:rest _:node1gm7uj6vjx216 .

_:node1gm7uj6vjx210 sh:nodeKind sh:Literal .

configuration:isConfigurationOf rdfs:label "isConfigurationOf"@en .

types:NativeFormatString rdfs:comment "Specifies data in its native format of some external language. The data may be encoded in Base64 per [RFC4648]. Data encoded in Base64 must be denoted as such using the encoded property."@en .

_:node1gm7uj6vjx211 sh:nodeKind sh:Literal .

_:node1gm7uj6vjx215 a sh:SPARQLConstraint .

_:node1gm7uj6vjx212 rdfs:comment "This triple is repeated from the Collections Ontology."@en .

action:ActionArgumentFacet sh:targetClass action:ActionArgumentFacet .

identity:OrganizationDetailsFacet rdfs:label "OrganizationDetailsFacet"@en .

core:EnclosingCompilation rdfs:subClassOf core:Compilation .

_:node1gm7uj6vjx214 sh:maxCount 1 .

_:node1gm7uj6vjx210 sh:path observable:modifiedTime .

observable:AccountFacet sh:property _:node1gm7uj6vjx210 .

_:node1gm7uj6vjx211 sh:path marking:definitionType .

marking:StatementMarking sh:property _:node1gm7uj6vjx211 .

types:StructuredText a rdfs:Datatype .

_:node1gm7uj6vjx216 rdf:first "Target PID"^^vocabulary:ActionArgumentNameVocab .

location:locality a owl:DatatypeProperty .

_:node1gm7uj6vjx212 owl:annotatedProperty rdfs:subClassOf .

_:node1gm7uj6vjx216 rdf:rest _:node1gm7uj6vjx219 .

_:node1gm7uj6vjx214 sh:nodeKind sh:Literal .

core:EnclosingCompilation rdfs:label "EnclosingCompilation"@en .

_:node1gm7uj6vjx217 sh:datatype xsd:dateTime .

location:locality rdfs:label "locality"@en .

_:node1gm7uj6vjx214 sh:path tool:cpeid .

_:node1gm7uj6vjx218 sh:datatype xsd:string .

action:ActionEstimationFacet a owl:Class .

tool:CompilerType sh:property _:node1gm7uj6vjx214 .

_:node1gm7uj6vjx212 owl:annotatedSource co:ListItem .

_:node1gm7uj6vjx215 sh:message "An OWL Object Property cannot use a SHACL DatatypeConstraintComponent."@en .

_:node1gm7uj6vjx217 sh:maxCount 1 .

action:ActionEstimationFacet a sh:NodeShape .

_:node1gm7uj6vjx219 rdf:first "Transfer Flags"^^vocabulary:ActionArgumentNameVocab .

_:node1gm7uj6vjx220 sh:datatype xsd:string .

_:node1gm7uj6vjx219 rdf:rest _:node1gm7uj6vjx221 .

_:node1gm7uj6vjx212 owl:annotatedTarget co:Item .

_:node1gm7uj6vjx215 sh:select """
				PREFIX rdf: <http://www.w3.org/1999/02/22-rdf-syntax-ns#>
				PREFIX sh: <http://www.w3.org/ns/shacl#>
				SELECT $this ?value
				WHERE {
					?value
						sh:datatype ?nDatatype ;
						sh:path / rdf:rest* ?nLastSequenceMember ;
						.
					?nLastSequenceMember
						rdf:first $this ;
						rdf:rest rdf:nil ;
						.
				}
		""" .

uco-owl:ObjectProperty-shacl-constraints-shape sh:sparql _:node1gm7uj6vjx215 .

_:node1gm7uj6vjx217 sh:nodeKind sh:Literal .

action:ActionEstimationFacet rdfs:subClassOf core:Facet .

_:node1gm7uj6vjx218 sh:maxCount 1 .

types:StructuredText rdfs:comment "Expresses string-based data in some information structuring format (e.g., HTML5)."@en .

location:locality rdfs:comment "The name of the geolocation locality (e.g., city)."@en .

_:node1gm7uj6vjx220 sh:maxCount 1 .

core:EnclosingCompilation rdfs:comment "An enclosing compilation is a container for a grouping of things."@en .

_:node1gm7uj6vjx222 a sh:SPARQLConstraint .

identity:OrganizationDetailsFacet rdfs:comment "Organization details is a grouping of characteristics unique to an identity representing an administrative and functional structure."@en .

_:node1gm7uj6vjx217 sh:path observable:observableCreatedTime .

action:ActionEstimationFacet rdfs:label "ActionEstimationFacet"@en .

observable:AccountFacet sh:property _:node1gm7uj6vjx217 .

_:node1gm7uj6vjx221 rdf:first "Username"^^vocabulary:ActionArgumentNameVocab ;
	rdf:rest rdf:nil .

_:node1gm7uj6vjx38 owl:oneOf _:node1gm7uj6vjx42 .

location:locality rdfs:range xsd:string .

vocabulary:ActionArgumentNameVocab owl:equivalentClass _:node1gm7uj6vjx38 .

_:node1gm7uj6vjx220 sh:nodeKind sh:Literal .

_:node1gm7uj6vjx218 sh:minCount 1 .

types:Thread a owl:Class .

_:node1gm7uj6vjx224 sh:datatype xsd:string .

_:node1gm7uj6vjx223 sh:class core:UcoObject .

_:node1gm7uj6vjx220 sh:path tool:swid .

tool:CompilerType sh:property _:node1gm7uj6vjx220 .

types:Thread a sh:NodeShape .

_:node1gm7uj6vjx218 sh:nodeKind sh:Literal .

identity:OrganizationDetailsFacet sh:targetClass identity:OrganizationDetailsFacet .

configuration:isConfigurationOf rdfs:comment "The object which has been configured to run in a more specified manner than another object.  This property is expected to have a more specific range when associated with a class, such as a configured Tool having this property have a range of a Tool."@en .

location:longitude a owl:DatatypeProperty .

_:node1gm7uj6vjx222 sh:message "An OWL Object Property must not permit a Literal value via SHACL consraints."@en .

_:node1gm7uj6vjx224 sh:maxCount 1 .

tool:CompilerType sh:targetClass tool:CompilerType .

vocabulary:ActionNameVocab a rdfs:Datatype .

_:node1gm7uj6vjx223 sh:minCount 1 .

types:Thread rdfs:subClassOf co:Bag .

configuration:isConfigurationOf rdfs:range core:UcoObject .

_:node1gm7uj6vjx218 sh:path marking:statement .

marking:StatementMarking sh:property _:node1gm7uj6vjx218 .

location:longitude rdfs:label "longitude"@en .

identity:Person a owl:Class .

types:Thread rdfs:subClassOf core:UcoThing .

_:node1gm7uj6vjx224 sh:nodeKind sh:Literal .

_:node1gm7uj6vjx223 sh:nodeKind sh:IRI .

_:node1gm7uj6vjx222 sh:select """
				PREFIX sh: <http://www.w3.org/ns/shacl#>
				SELECT $this ?value
				WHERE {
					?value
						sh:path / rdf:rest* ?nLastSequenceMember ;
						.
					?nLastSequenceMember
						rdf:first $this ;
						rdf:rest rdf:nil ;
						.

					{ ?value sh:nodeKind sh:BlankNodeOrLiteral . }
					UNION
					{ ?value sh:nodeKind sh:IRIOrLiteral . }
					UNION
					{ ?value sh:nodeKind sh:Literal . }
				}
		""" .

uco-owl:ObjectProperty-shacl-constraints-shape sh:sparql _:node1gm7uj6vjx222 .

tool:ConfiguredTool a owl:Class .

vocabulary:ActionNameVocab rdfs:label "Action Name Vocabulary"@en-us .

identity:Person a sh:NodeShape .

action:ActionEstimationFacet rdfs:comment "An action estimation facet is a grouping of characteristics unique to decision-focused approximation aspects for an action that may potentially be performed."@en .

types:Thread rdfs:label "Thread"@en .

_:node1gm7uj6vjx223 sh:path core:object .

tool:ConfiguredTool a sh:NodeShape .

core:EnclosingCompilation sh:property _:node1gm7uj6vjx223 .

location:longitude rdfs:comment "The longitude coordinate of a geolocation."@en .

_:node1gm7uj6vjx224 sh:path observable:accountIdentifier .

marking:StatementMarking sh:targetClass marking:StatementMarking .

uco-owl:ObjectProperty-shacl-constraints-shape sh:targetClass owl:ObjectProperty .

configuration:itemDescription a owl:DatatypeProperty .

observable:AccountFacet sh:property _:node1gm7uj6vjx224 .

identity:Person rdfs:subClassOf identity:Identity .

location:longitude rdfs:range xsd:decimal .

tool:ConfiguredTool rdfs:subClassOf tool:Tool .

_:node1gm7uj6vjx225 sh:datatype xsd:string .

core:EnclosingCompilation sh:targetClass core:EnclosingCompilation .

_:node1gm7uj6vjx226 sh:datatype vocabulary:AccountTypeVocab .

marking:TermsOfUseMarking a owl:Class .

location:pdop a owl:DatatypeProperty .

marking:TermsOfUseMarking a sh:NodeShape .

uco-owl:incompatibleWith-direct-import-shape a sh:PropertyShape .

identity:Person rdfs:label "Person"@en .

core:ExternalReference a owl:Class .

tool:ConfiguredTool rdfs:label "ConfiguredTool"@en .

vocabulary:ActionNameVocab rdfs:comment "Defines an open-vocabulary of common specific cyber action names."@en .

configuration:itemDescription rdfs:label "itemDescription"@en .

location:pdop rdfs:label "pdop"@en .

core:ExternalReference a sh:NodeShape .

_:node1gm7uj6vjx225 sh:maxCount 1 .

marking:TermsOfUseMarking rdfs:subClassOf marking:MarkingModel .

_:node1gm7uj6vjx226 sh:message "Value is outside the default vocabulary AccountTypeVocab." .

uco-owl:incompatibleWith-direct-import-shape rdfs:seeAlso <https://www.w3.org/TR/owl2-syntax/#Imports> .

_:node1gm7uj6vjx225 sh:nodeKind sh:Literal .

_:node1gm7uj6vjx227 a rdfs:Datatype .

_:node1gm7uj6vjx226 sh:path observable:accountType .

core:ExternalReference rdfs:subClassOf core:UcoInherentCharacterizationThing .

uco-owl:incompatibleWith-direct-import-shape sh:disjoint owl:incompatibleWith .

marking:TermsOfUseMarking rdfs:label "Terms Of Use Marking"@en .

_:node1gm7uj6vjx225 sh:path action:estimatedCost .

configuration:itemDescription rdfs:comment "A description of a configuration setting entry item."@en .

_:node1gm7uj6vjx227 owl:onDatatype xsd:string .

action:ActionEstimationFacet sh:property _:node1gm7uj6vjx225 .

location:pdop rdfs:comment "The positional (3D) dilution of precision of the GPS location."@en .

_:node1gm7uj6vjx226 sh:severity sh:Info .

observable:AccountFacet sh:property _:node1gm7uj6vjx226 .

configuration:itemDescription rdfs:range xsd:string .

location:pdop rdfs:range xsd:decimal .

_:node1gm7uj6vjx228 sh:datatype xsd:string .

core:ExternalReference rdfs:label "ExternalReference"@en .

_:node1gm7uj6vjx230 sh:maxCount 1 .

types:Thread rdfs:comment "A semi-ordered array of items, that can be present in multiple copies.  Implemetation of a UCO Thread is similar to a Collections Ontology List, except a Thread may fork and merge - that is, one of its members may have two or more direct successors, and two or more direct predecessors."@en .

_:node1gm7uj6vjx228 sh:maxCount 1 .

tool:ConfiguredTool rdfs:comment "A ConfiguredTool is a Tool that is known to be configured to run in a more specified manner than some unconfigured or less-configured Tool."@en .

configuration:itemName a owl:DatatypeProperty .

location:postalCode a owl:DatatypeProperty .

identity:Person rdfs:comment "A person is a grouping of identifying characteristics unique to a human being regarded as an individual. [based on https://www.lexico.com/en/definition/person]"@en .

_:node1gm7uj6vjx230 sh:nodeKind sh:Literal .

_:node1gm7uj6vjx229 rdf:first "Accept Socket Connection"^^vocabulary:ActionNameVocab ;
	rdf:rest _:node1gm7uj6vjx232 .

types:Thread owl:disjointWith co:List .

_:node1gm7uj6vjx228 sh:nodeKind sh:Literal .

configuration:itemName rdfs:label "itemName"@en .

location:postalCode rdfs:label "postalCode"@en .

identity:Person sh:targetClass identity:Person .

_:node1gm7uj6vjx231 sh:class configuration:Configuration .

core:ExternalReference rdfs:comment "Characteristics of a reference to a resource outside of the UCO."@en .

_:node1gm7uj6vjx228 sh:path action:estimatedEfficacy .

action:ActionEstimationFacet sh:property _:node1gm7uj6vjx228 .

_:node1gm7uj6vjx235 sh:class types:ThreadItem .

_:node1gm7uj6vjx234 sh:datatype vocabulary:AccountTypeVocab .

location:postalCode rdfs:comment "The zip-code."@en .

_:node1gm7uj6vjx233 rdf:first _:node1gm7uj6vjx234 ;
	rdf:rest _:node1gm7uj6vjx238 .

_:node1gm7uj6vjx235 sh:path co:item .

_:node1gm7uj6vjx231 sh:maxCount 1 .

_:node1gm7uj6vjx232 rdf:first "Add Connection to Network Share"^^vocabulary:ActionNameVocab .

_:node1gm7uj6vjx236 sh:datatype xsd:string .

types:Thread sh:property _:node1gm7uj6vjx235 .

_:node1gm7uj6vjx232 rdf:rest _:node1gm7uj6vjx240 .

configuration:itemName rdfs:comment "The name of a configuration setting entry item."@en .

location:postalCode rdfs:range xsd:string .

_:node1gm7uj6vjx237 sh:datatype xsd:anyURI .

_:node1gm7uj6vjx239 sh:datatype xsd:string .

identity:PersonalDetailsFacet a owl:Class .

_:node1gm7uj6vjx238 rdf:first _:node1gm7uj6vjx239 ;
	rdf:rest rdf:nil .

_:node1gm7uj6vjx230 sh:or _:node1gm7uj6vjx233 .

identity:PersonalDetailsFacet a sh:NodeShape .

configuration:itemName rdfs:range xsd:string .

_:node1gm7uj6vjx231 sh:nodeKind sh:BlankNodeOrIRI .

types:ThreadItem a owl:Class .

_:node1gm7uj6vjx236 sh:maxCount 1 .

_:node1gm7uj6vjx237 sh:maxCount 1 .

_:node1gm7uj6vjx230 sh:path observable:accountType .

_:node1gm7uj6vjx240 rdf:first "Add Network Share"^^vocabulary:ActionNameVocab .

observable:AccountFacet sh:property _:node1gm7uj6vjx230 .

_:node1gm7uj6vjx240 rdf:rest _:node1gm7uj6vjx241 .

location:region a owl:DatatypeProperty .

types:ThreadItem a sh:NodeShape .

identity:PersonalDetailsFacet rdfs:subClassOf identity:IdentityFacet .

_:node1gm7uj6vjx236 sh:nodeKind sh:Literal .

_:node1gm7uj6vjx231 sh:path configuration:usesConfiguration .

_:node1gm7uj6vjx237 sh:nodeKind sh:Literal .

tool:ConfiguredTool sh:property _:node1gm7uj6vjx231 .

location:region rdfs:label "region"@en .

configuration:itemObject a owl:ObjectProperty .

types:ThreadItem rdfs:subClassOf co:Item .

uco-owl:incompatibleWith-direct-import-shape sh:message "'The import closure of [ontology] O SHOULD NOT contain ontologies O_1 and O_2 such that ... O_1 contains an ontology annotation owl:incompatibleWith with the value equal to either the ontology IRI or the version IRI of O_2.'  The focusNode directly imported an incompatibility it declared (the value node)."@en .

identity:PersonalDetailsFacet rdfs:label "PersonalDetailsFacet"@en .

_:node1gm7uj6vjx242 sh:message "Value is not member of the vocabulary AccountTypeVocab." .

types:ThreadItem rdfs:subClassOf core:UcoThing .

_:node1gm7uj6vjx243 sh:class tool:Tool .

_:node1gm7uj6vjx237 sh:path core:referenceURL .

_:node1gm7uj6vjx236 sh:path action:estimatedImpact .

uco-owl:incompatibleWith-direct-import-shape sh:path owl:imports .

core:ExternalReference sh:property _:node1gm7uj6vjx237 .

action:ActionEstimationFacet sh:property _:node1gm7uj6vjx236 .

_:node1gm7uj6vjx241 rdf:first "Add Scheduled Task"^^vocabulary:ActionNameVocab ;
	rdf:rest _:node1gm7uj6vjx248 .

types:ThreadItem rdfs:label "ThreadItem"@en .

uco-owl:incompatibleWith-direct-import-shape sh:severity sh:Warning .

_:node1gm7uj6vjx243 sh:maxCount 1 .

_:node1gm7uj6vjx245 sh:datatype vocabulary:AccountTypeVocab .

_:node1gm7uj6vjx246 sh:datatype xsd:string .

location:region rdfs:comment "The name of the geolocation region (e.g., state)."@en .

_:node1gm7uj6vjx247 sh:datatype xsd:string .

configuration:itemObject rdfs:comment "The structured value of a configuration setting entry instance."@en .

uco-owl:incompatibleWith-direct-import-shape sh:targetClass owl:Ontology .

_:node1gm7uj6vjx243 sh:nodeKind sh:BlankNodeOrIRI .

location:region rdfs:range xsd:string .

types:ThreadItem rdfs:comment "A ThreadItem is a member of a thread."@en .

_:node1gm7uj6vjx248 rdf:first "Add System Call Hook"^^vocabulary:ActionNameVocab .

_:node1gm7uj6vjx246 sh:maxCount 1 .

configuration:itemObject rdfs:range core:UcoObject .

_:node1gm7uj6vjx247 sh:maxCount 1 .

_:node1gm7uj6vjx248 rdf:rest _:node1gm7uj6vjx250 .

_:node1gm7uj6vjx249 rdf:first "ldap"^^vocabulary:AccountTypeVocab .

identity:PersonalDetailsFacet rdfs:comment "Personal details is a grouping of characteristics unique to an identity representing an individual person."@en .

_:node1gm7uj6vjx249 rdf:rest _:node1gm7uj6vjx251 .

_:node1gm7uj6vjx246 sh:nodeKind sh:Literal .

marking:TermsOfUseMarking rdfs:comment "A terms of use marking is a grouping of characteristics unique to the expression of data marking definitions (restrictions, permissions, and other guidance for how data can be used and shared) to convey details of a textual statement specifying the Terms of Use (that is, the conditions under which the content may be shared, applied, or otherwise used) of the marked content. An example of this would be used to communicate a simple statement, such as 'Acme Inc. is not responsible for the content of this file'."@en .

_:node1gm7uj6vjx247 sh:nodeKind sh:Literal .

types:ThreadItem owl:disjointWith co:ListItem .

_:node1gm7uj6vjx243 sh:path configuration:isConfigurationOf .

tool:ConfiguredTool sh:property _:node1gm7uj6vjx243 .

location:street a owl:DatatypeProperty .

_:node1gm7uj6vjx246 sh:path action:objective .

action:ActionEstimationFacet sh:property _:node1gm7uj6vjx246 .

_:node1gm7uj6vjx250 rdf:first "Add User"^^vocabulary:ActionNameVocab .

_:node1gm7uj6vjx247 sh:path core:definingContext .

_:node1gm7uj6vjx251 rdf:first "nis"^^vocabulary:AccountTypeVocab .

_:node1gm7uj6vjx250 rdf:rest _:node1gm7uj6vjx254 .

core:ExternalReference sh:property _:node1gm7uj6vjx247 .

location:street rdfs:label "street"@en .

identity:PersonalDetailsFacet sh:targetClass identity:PersonalDetailsFacet .

configuration:itemObject rdfs:seeAlso <https://github.com/ucoProject/UCO/issues/432> .

_:node1gm7uj6vjx253 sh:class core:UcoObject .

_:node1gm7uj6vjx252 sh:datatype xsd:string .

_:node1gm7uj6vjx251 rdf:rest _:node1gm7uj6vjx255 .

tool:ConfiguredTool sh:targetClass tool:ConfiguredTool .

uco-owl:incompatibleWith-imported-ontology-iri-shape a sh:NodeShape .

action:ActionEstimationFacet sh:targetClass action:ActionEstimationFacet .

location:street rdfs:comment "The name of the street."@en .

_:node1gm7uj6vjx253 sh:path co:itemContent .

types:ThreadItem sh:property _:node1gm7uj6vjx253 .

_:node1gm7uj6vjx252 sh:hasValue "terms-of-use" .

_:node1gm7uj6vjx255 rdf:first "openid"^^vocabulary:AccountTypeVocab .

_:node1gm7uj6vjx256 sh:datatype xsd:string .

_:node1gm7uj6vjx254 rdf:first "Add Windows Hook"^^vocabulary:ActionNameVocab ;
	rdf:rest _:node1gm7uj6vjx257 .

uco-owl:incompatibleWith-imported-ontology-iri-shape rdfs:seeAlso <https://www.w3.org/TR/owl2-syntax/#Imports> .

location:street rdfs:range xsd:string .

tool:DefensiveTool a owl:Class .

_:node1gm7uj6vjx252 sh:nodeKind sh:Literal .

identity:PhysicalInfoFacet a owl:Class .

configuration:itemType a owl:DatatypeProperty .

tool:DefensiveTool a sh:NodeShape .

action:ActionFrequencyFacet a owl:Class .

types:entry a owl:ObjectProperty .

identity:PhysicalInfoFacet a sh:NodeShape .

_:node1gm7uj6vjx252 sh:path marking:definitionType .

_:node1gm7uj6vjx256 sh:maxCount 1 .

marking:TermsOfUseMarking sh:property _:node1gm7uj6vjx252 .

configuration:itemType rdfs:label "itemType"@en .

_:node1gm7uj6vjx257 rdf:first "Allocate Virtual Memory in Process"^^vocabulary:ActionNameVocab .

action:ActionFrequencyFacet a sh:NodeShape .

_:node1gm7uj6vjx257 rdf:rest _:node1gm7uj6vjx259 .

location:tdop a owl:DatatypeProperty .

tool:DefensiveTool rdfs:subClassOf tool:Tool .

_:node1gm7uj6vjx256 sh:nodeKind sh:Literal .

_:node1gm7uj6vjx258 sh:datatype xsd:string .

action:ActionFrequencyFacet rdfs:subClassOf core:Facet .

types:entry rdfs:label "entry"@en .

identity:PhysicalInfoFacet rdfs:subClassOf identity:IdentityFacet .

_:node1gm7uj6vjx255 rdf:rest _:node1gm7uj6vjx260 .

location:tdop rdfs:label "tdop"@en .

_:node1gm7uj6vjx256 sh:path core:externalIdentifier .

_:node1gm7uj6vjx259 rdf:first "Bind Address to Socket"^^vocabulary:ActionNameVocab .

core:ExternalReference sh:property _:node1gm7uj6vjx256 .

_:node1gm7uj6vjx259 rdf:rest _:node1gm7uj6vjx261 .

core:ExternalReference sh:targetClass core:ExternalReference .

tool:DefensiveTool rdfs:label "DefensiveTool"@en .

action:ActionFrequencyFacet rdfs:label "ActionFrequencyFacet"@en .

configuration:itemType rdfs:comment "The type of a configuration setting entry item."@en .

location:tdop rdfs:comment "The temporal dilution of precision of the GPS location."@en .

types:entry rdfs:comment "A dictionary entry."@en .

_:node1gm7uj6vjx258 sh:maxCount 1 .

identity:PhysicalInfoFacet rdfs:label "PhysicalInfoFacet"@en .

core:Facet a owl:Class .

configuration:itemType rdfs:range xsd:string .

location:tdop rdfs:range xsd:decimal .

core:Facet a sh:NodeShape .

types:entry rdfs:range types:DictionaryEntry .

_:node1gm7uj6vjx261 rdf:first "Change Service Configuration"^^vocabulary:ActionNameVocab .

_:node1gm7uj6vjx260 rdf:first "radius"^^vocabulary:AccountTypeVocab .

_:node1gm7uj6vjx261 rdf:rest _:node1gm7uj6vjx262 .

_:node1gm7uj6vjx260 rdf:rest _:node1gm7uj6vjx263 .

_:node1gm7uj6vjx258 sh:minCount 1 .

location:vdop a owl:DatatypeProperty .

_:node1gm7uj6vjx258 sh:nodeKind sh:Literal .

configuration:itemValue a owl:DatatypeProperty .

types:hashMethod a owl:DatatypeProperty .

core:Facet rdfs:subClassOf core:UcoInherentCharacterizationThing .

_:node1gm7uj6vjx263 rdf:first "tacacs"^^vocabulary:AccountTypeVocab .

_:node1gm7uj6vjx262 rdf:first "Check for Remote Debugger"^^vocabulary:ActionNameVocab .

location:vdop rdfs:label "vdop"@en .

_:node1gm7uj6vjx262 rdf:rest _:node1gm7uj6vjx265 .

_:node1gm7uj6vjx263 rdf:rest _:node1gm7uj6vjx264 .

_:node1gm7uj6vjx258 sh:path marking:termsOfUse .

configuration:itemValue rdfs:label "itemValue"@en .

tool:DefensiveTool rdfs:comment "A defensive tool is an artifact of hardware and/or software utilized to accomplish a task or purpose of guarding."@en .

marking:TermsOfUseMarking sh:property _:node1gm7uj6vjx258 .

types:hashMethod rdfs:label "hashMethod"@en .

core:Facet rdfs:label "Facet"@en .

action:ActionFrequencyFacet rdfs:comment "An action frequency facet is a grouping of characteristics unique to the frequency of occurrence for an action."@en .

identity:PhysicalInfoFacet rdfs:comment "Physical info is a grouping of characteristics unique to the outwardly observable nature of an individual person."@en .

uco-owl:incompatibleWith-imported-ontology-iri-shape sh:message "'The import closure of [ontology] O SHOULD NOT contain ontologies O_1 and O_2 such that ... O_1 contains an ontology annotation owl:incompatibleWith with the value equal to either the ontology IRI or the version IRI of O_2.'  The focusNode, or a versionIRI of it, is imported within the transitive closure of some O, but is incompatible with some O_1 also within the transitive closure of O."@en .

tool:DefensiveTool sh:targetClass tool:DefensiveTool .

_:node1gm7uj6vjx265 rdf:first "Close Port"^^vocabulary:ActionNameVocab .

_:node1gm7uj6vjx264 rdf:first "unix"^^vocabulary:AccountTypeVocab .

marking:TermsOfUseMarking sh:targetClass marking:TermsOfUseMarking .

_:node1gm7uj6vjx265 rdf:rest _:node1gm7uj6vjx268 .

_:node1gm7uj6vjx264 rdf:rest _:node1gm7uj6vjx269 .

location:vdop rdfs:comment "The vertical dilution of precision of the GPS location."@en .

_:node1gm7uj6vjx267 a sh:NodeShape .

_:node1gm7uj6vjx266 sh:datatype xsd:decimal .

configuration:itemValue rdfs:comment "The value of a configuration setting entry instance."@en .

identity:PhysicalInfoFacet sh:targetClass identity:PhysicalInfoFacet .

types:hashMethod rdfs:comment "A particular cryptographic hashing method (e.g., MD5)."@en .

tool:LibraryType a owl:Class .

location:vdop rdfs:range xsd:decimal .

_:node1gm7uj6vjx267 sh:class owl:Ontology .

configuration:itemValue rdfs:range xsd:string .

tool:LibraryType a sh:NodeShape .

core:Facet rdfs:comment "A facet is a grouping of characteristics singularly unique to a particular inherent aspect of a UCO domain object."@en .

_:node1gm7uj6vjx268 rdf:first "Close Registry Key"^^vocabulary:ActionNameVocab .

_:node1gm7uj6vjx269 rdf:first "windows_domain"^^vocabulary:AccountTypeVocab .

_:node1gm7uj6vjx270 a rdfs:Datatype .

_:node1gm7uj6vjx266 sh:maxCount 1 .

_:node1gm7uj6vjx268 rdf:rest _:node1gm7uj6vjx271 .

marking:authorizedIdentities a owl:DatatypeProperty .

_:node1gm7uj6vjx269 rdf:rest _:node1gm7uj6vjx272 .

identity:QualificationFacet a owl:Class .

core:Facet sh:targetClass core:Facet .

configuration:usageContextAssumptions a owl:DatatypeProperty .

identity:QualificationFacet a sh:NodeShape .

marking:authorizedIdentities rdfs:label "Authorized Identities"@en .

_:node1gm7uj6vjx266 sh:minCount 1 .

_:node1gm7uj6vjx273 rdf:first vocabulary:HashNameVocab ;
	rdf:rest _:node1gm7uj6vjx274 .

tool:LibraryType rdfs:subClassOf core:UcoInherentCharacterizationThing .

configuration:usageContextAssumptions rdfs:label "usageContextAssumptions"@en .

_:node1gm7uj6vjx274 rdf:first xsd:string .

_:node1gm7uj6vjx272 rdf:first "windows_local"^^vocabulary:AccountTypeVocab .

_:node1gm7uj6vjx274 rdf:rest rdf:nil .

_:node1gm7uj6vjx270 owl:unionOf _:node1gm7uj6vjx273 .

core:Grouping a owl:Class .

_:node1gm7uj6vjx272 rdf:rest rdf:nil .

_:node1gm7uj6vjx245 sh:in _:node1gm7uj6vjx249 .

_:node1gm7uj6vjx271 rdf:first "Close Socket"^^vocabulary:ActionNameVocab .

types:hashMethod rdfs:range _:node1gm7uj6vjx270 .

_:node1gm7uj6vjx266 sh:nodeKind sh:Literal .

identity:QualificationFacet rdfs:subClassOf identity:IdentityFacet .

_:node1gm7uj6vjx271 rdf:rest _:node1gm7uj6vjx275 .

_:node1gm7uj6vjx244 rdf:first _:node1gm7uj6vjx245 .

core:Grouping a sh:NodeShape .

_:node1gm7uj6vjx244 rdf:rest _:node1gm7uj6vjx276 .

tool:LibraryType rdfs:label "LibraryType"@en .

_:node1gm7uj6vjx266 sh:path action:rate .

action:ActionFrequencyFacet sh:property _:node1gm7uj6vjx266 .

_:node1gm7uj6vjx277 sh:datatype xsd:string .

_:node1gm7uj6vjx276 rdf:first _:node1gm7uj6vjx277 .

identity:QualificationFacet rdfs:label "QualificationFacet"@en .

_:node1gm7uj6vjx276 rdf:rest rdf:nil .

_:node1gm7uj6vjx242 sh:or _:node1gm7uj6vjx244 .

types:hashValue a owl:DatatypeProperty .

_:node1gm7uj6vjx278 sh:datatype xsd:string .

core:Grouping rdfs:subClassOf core:ContextualCompilation .

_:node1gm7uj6vjx275 rdf:first "Configure Service"^^vocabulary:ActionNameVocab ;
	rdf:rest _:node1gm7uj6vjx279 .

_:node1gm7uj6vjx267 sh:description "This node having a class-designation of owl:Ontology implies it is an ontology 'O_2' defined in the transitive closure of an ontology 'O_1' that declared itself incompatible with 'O_2'."@en .

uco-owl:incompatibleWith-imported-ontology-iri-shape sh:not _:node1gm7uj6vjx267 .

_:node1gm7uj6vjx242 sh:path observable:accountType .

observable:AccountFacet sh:property _:node1gm7uj6vjx242 .

types:hashValue rdfs:label "hashValue"@en .

uco-owl:incompatibleWith-imported-ontology-iri-shape sh:severity sh:Warning .

_:node1gm7uj6vjx278 sh:maxCount 1 .

configuration:usageContextAssumptions rdfs:comment "Description of the various relevant usage context assumptions for a tool or other software ."@en .

core:Grouping rdfs:label "Grouping"@en .

_:node1gm7uj6vjx279 rdf:first "Connect to IP"^^vocabulary:ActionNameVocab ;
	rdf:rest _:node1gm7uj6vjx280 .

configuration:usageContextAssumptions rdfs:range xsd:string .

observable:AccountFacet sh:targetClass observable:AccountFacet .

uco-owl:incompatibleWith-imported-ontology-iri-shape sh:targetObjectsOf owl:incompatibleWith .

types:hashValue rdfs:comment "A cryptographic hash value."@en .

_:node1gm7uj6vjx278 sh:minCount 1 .

marking:authorizedIdentities rdfs:comment "Specifies the identities that are authorized to access the data to which the data marking is associated.  The list of authorized identities are represented as UUIDs."@en .

tool:LibraryType rdfs:comment "A library type is a grouping of characteristics unique to a collection of resources incorporated into the build of a software."@en .

types:hashValue rdfs:range xsd:hexBinary .

_:node1gm7uj6vjx278 sh:nodeKind sh:Literal .

marking:authorizedIdentities rdfs:range xsd:string .

observable:Adaptor a owl:Class .

_:node1gm7uj6vjx280 rdf:first "Connect to Named Pipe"^^vocabulary:ActionNameVocab .

core:Grouping rdfs:comment "A grouping is a compilation of referenced UCO content with a shared context."@en .

_:node1gm7uj6vjx280 rdf:rest _:node1gm7uj6vjx282 .

identity:QualificationFacet rdfs:comment "Qualification is a grouping of characteristics unique to particular skills, capabilities or their related achievements (educational, professional, etc.) of an entity."@en .

observable:Adaptor a sh:NodeShape .

_:node1gm7uj6vjx278 sh:path action:scale .

configuration:usesConfiguration a owl:ObjectProperty .

action:ActionFrequencyFacet sh:property _:node1gm7uj6vjx278 .

types:key a owl:DatatypeProperty .

_:node1gm7uj6vjx281 sh:datatype xsd:string .

uco-owl:incompatibleWith-imported-version-iri-shape a sh:PropertyShape .

observable:Adaptor rdfs:subClassOf observable:Device .

types:key rdfs:label "key"@en .

configuration:usesConfiguration rdfs:label "usesConfiguration"@en .

marking:contentSelectors a owl:DatatypeProperty .

identity:QualificationFacet sh:targetClass identity:QualificationFacet .

_:node1gm7uj6vjx284 sh:datatype xsd:string .

_:node1gm7uj6vjx281 sh:maxCount 1 .

_:node1gm7uj6vjx282 rdf:first "Connect to Network Share"^^vocabulary:ActionNameVocab .

_:node1gm7uj6vjx283 sh:datatype xsd:string .

_:node1gm7uj6vjx282 rdf:rest _:node1gm7uj6vjx285 .

uco-owl:incompatibleWith-imported-version-iri-shape rdfs:seeAlso <https://www.w3.org/TR/owl2-syntax/#Imports> .

marking:contentSelectors rdfs:label "contentSelectors"@en .

observable:Adaptor rdfs:label "Adaptor"@en-us .

_:node1gm7uj6vjx284 sh:nodeKind sh:Literal .

_:node1gm7uj6vjx281 sh:nodeKind sh:Literal .

configuration:usesConfiguration rdfs:comment "A configuration used by an object."@en .

types:key rdfs:comment "A key property of a single dictionary entry."@en .

identity:RelatedIdentityFacet a owl:Class .

_:node1gm7uj6vjx283 sh:maxCount 1 .

identity:RelatedIdentityFacet a sh:NodeShape .

observable:Adaptor rdfs:comment "An adaptor is a device that physically converts the pin outputs but does not alter the underlying protocol (e.g. uSD to SD, CF to ATA, etc.)"@en-us .

uco-owl:incompatibleWith-imported-version-iri-shape sh:maxCount 0 .

_:node1gm7uj6vjx281 sh:path tool:libraryName .

_:node1gm7uj6vjx284 sh:path core:context .

types:key rdfs:range xsd:string .

_:node1gm7uj6vjx285 rdf:first "Connect to Socket"^^vocabulary:ActionNameVocab .

marking:contentSelectors rdfs:comment """Explicit specification of exactly which portions of a UCO object to apply marking definitions to.
  Specific syntax for how to specify the UCO object portions is dependent on the particular syntactic serialization implementation (XML, JSON, etc.) of UCO and MUST be explicitly specified in a separate binding specification for that syntactic serialization implementation (e.g. a UCO XML Binding Specification). """@en .

tool:LibraryType sh:property _:node1gm7uj6vjx281 .

core:Grouping sh:property _:node1gm7uj6vjx284 .

_:node1gm7uj6vjx285 rdf:rest _:node1gm7uj6vjx286 .

configuration:usesConfiguration rdfs:range configuration:Configuration .

marking:contentSelectors rdfs:range xsd:string .

_:node1gm7uj6vjx287 sh:datatype xsd:string .

observable:Adaptor sh:targetClass observable:Adaptor .

_:node1gm7uj6vjx283 sh:minCount 1 .

identity:RelatedIdentityFacet rdfs:subClassOf identity:IdentityFacet .

core:Grouping sh:targetClass core:Grouping .

_:node1gm7uj6vjx286 rdf:first "Connect to URL"^^vocabulary:ActionNameVocab ;
	rdf:rest _:node1gm7uj6vjx288 .

types:threadNextItem a owl:ObjectProperty .

_:node1gm7uj6vjx283 sh:nodeKind sh:Literal .

_:node1gm7uj6vjx287 sh:maxCount 1 .

marking:definition a owl:ObjectProperty .

observable:Address a owl:Class .

identity:RelatedIdentityFacet rdfs:label "RelatedIdentityFacet"@en .

_:node1gm7uj6vjx288 rdf:first "Control Driver"^^vocabulary:ActionNameVocab ;
	rdf:rest _:node1gm7uj6vjx289 .

core:IdentityAbstraction a owl:Class .

_:node1gm7uj6vjx283 sh:path action:units .

marking:definition rdfs:label "definition"@en .

action:ActionFrequencyFacet sh:property _:node1gm7uj6vjx283 .

types:threadNextItem rdfs:subPropertyOf types:threadSuccessor .

observable:Address a sh:NodeShape .

_:node1gm7uj6vjx287 sh:nodeKind sh:Literal .

core:IdentityAbstraction a sh:NodeShape .

identity:RelatedIdentityFacet rdfs:comment "<Needs fleshed out from CIQ>"@en .

_:node1gm7uj6vjx287 sh:path tool:libraryVersion .

types:threadNextItem rdfs:label "threadNextItem"@en .

_:node1gm7uj6vjx289 rdf:first "Control Service"^^vocabulary:ActionNameVocab .

tool:LibraryType sh:property _:node1gm7uj6vjx287 .

_:node1gm7uj6vjx290 sh:datatype vocabulary:TrendVocab .

core:IdentityAbstraction rdfs:subClassOf core:UcoObject .

_:node1gm7uj6vjx289 rdf:rest _:node1gm7uj6vjx291 .

observable:Address rdfs:subClassOf observable:ObservableObject .

marking:definition rdfs:comment "Explicit specification of a data marking instance."@en .

tool:LibraryType sh:targetClass tool:LibraryType .

identity:RelatedIdentityFacet sh:targetClass identity:RelatedIdentityFacet .

observable:Address rdfs:label "Address"@en .

_:node1gm7uj6vjx291 rdf:first "Copy File"^^vocabulary:ActionNameVocab .

marking:definition rdfs:range marking:MarkingModel .

_:node1gm7uj6vjx291 rdf:rest _:node1gm7uj6vjx292 .

types:threadNextItem rdfs:comment "The link to a next item in a thread."@en .

core:IdentityAbstraction rdfs:label "IdentityAbstraction"@en .

_:node1gm7uj6vjx290 sh:message "Value is outside the default vocabulary TrendVocab." .

tool:MaliciousTool a owl:Class .

uco-owl:incompatibleWith-imported-version-iri-shape sh:message "'The import closure of [ontology] O SHOULD NOT contain ontologies O_1 and O_2 such that ... O_1 contains an ontology annotation owl:incompatibleWith with the value equal to ... the version IRI of O_2.'  The focusNode is incompatible with some O_1 within the transitive closure of some O."@en .

identity:SimpleNameFacet a owl:Class .

types:threadNextItem rdfs:seeAlso co:nextItem .

identity:SimpleNameFacet a sh:NodeShape .

tool:MaliciousTool a sh:NodeShape .

_:node1gm7uj6vjx292 rdf:first "Create Dialog Box"^^vocabulary:ActionNameVocab .

_:node1gm7uj6vjx290 sh:path action:trend .

_:node1gm7uj6vjx292 rdf:rest _:node1gm7uj6vjx294 .

marking:definitionType a owl:DatatypeProperty .

observable:Address rdfs:comment "An address is an identifier assigned to enable routing and management of information."@en .

_:node1gm7uj6vjx293 sh:inversePath owl:versionIRI .

tool:MaliciousTool rdfs:subClassOf tool:Tool .

uco-owl:incompatibleWith-imported-version-iri-shape sh:path _:node1gm7uj6vjx293 .

marking:definitionType rdfs:label "definitionType"@en .

_:node1gm7uj6vjx290 sh:severity sh:Info .

action:ActionFrequencyFacet sh:property _:node1gm7uj6vjx290 .

identity:SimpleNameFacet rdfs:subClassOf identity:IdentityFacet .

tool:MaliciousTool rdfs:label "MaliciousTool"@en .

observable:Address sh:targetClass observable:Address .

uco-owl:incompatibleWith-imported-version-iri-shape sh:severity sh:Warning .

_:node1gm7uj6vjx294 rdf:first "Create Directory"^^vocabulary:ActionNameVocab ;
	rdf:rest _:node1gm7uj6vjx296 .

_:node1gm7uj6vjx295 sh:maxCount 1 .

identity:SimpleNameFacet rdfs:label "SimpleNameFacet"@en .

types:threadNextItem-subjects-shape a sh:PropertyShape .

marking:definitionType rdfs:comment "Specifies the Marking Model for a Marking Definition."@en .

core:IdentityAbstraction rdfs:comment "An identity abstraction is a grouping of identifying characteristics unique to an individual or organization. This class is an ontological structural abstraction for this concept. Implementations of this concept should utilize the identity:Identity class."@en .

uco-owl:incompatibleWith-imported-version-iri-shape sh:targetObjectsOf owl:incompatibleWith .

tool:MaliciousTool rdfs:comment "A malicious tool is an artifact of hardware and/or software utilized to accomplish a malevolent task or purpose."@en .

types:threadNextItem-subjects-shape sh:class types:ThreadItem .

marking:definitionType rdfs:range xsd:string .

_:node1gm7uj6vjx295 sh:minCount 1 .

_:node1gm7uj6vjx296 rdf:first "Create Event"^^vocabulary:ActionNameVocab ;
	rdf:rest _:node1gm7uj6vjx297 .

observable:AlternateDataStream a owl:Class .

identity:SimpleNameFacet rdfs:comment "A simple name facet is a grouping of characteristics unique to the personal name (e.g., Dr. John Smith Jr.) held by an identity."@en .

types:threadNextItem-subjects-shape sh:nodeKind sh:IRI .

core:IdentityAbstraction sh:targetClass core:IdentityAbstraction .

observable:AlternateDataStream a sh:NodeShape .

_:node1gm7uj6vjx295 sh:nodeKind sh:Literal .

tool:MaliciousTool sh:targetClass tool:MaliciousTool .

core:Item a owl:Class .

types:threadNextItem-subjects-shape sh:path types:threadNextItem .

_:node1gm7uj6vjx297 rdf:first "Create File"^^vocabulary:ActionNameVocab ;
	rdf:rest _:node1gm7uj6vjx301 .

tool:Tool a owl:Class .

marking:license a owl:DatatypeProperty .

_:node1gm7uj6vjx298 sh:datatype xsd:string .

core:Item a sh:NodeShape .

observable:AlternateDataStream rdfs:subClassOf observable:ObservableObject .

_:node1gm7uj6vjx300 sh:datatype vocabulary:TrendVocab .

_:node1gm7uj6vjx299 rdf:first _:node1gm7uj6vjx300 ;
	rdf:rest _:node1gm7uj6vjx302 .

tool:Tool a sh:NodeShape .

uco-owl:ontologyIRI-versionIRI-prerequisite-shape a sh:NodeShape .

marking:license rdfs:label "License" .

_:node1gm7uj6vjx298 sh:nodeKind sh:Literal .

_:node1gm7uj6vjx301 rdf:first "Create File Alternate Data Stream"^^vocabulary:ActionNameVocab .

observable:AlternateDataStream rdfs:label "AlternateDataStream"@en .

_:node1gm7uj6vjx301 rdf:rest _:node1gm7uj6vjx304 .

core:Item rdfs:subClassOf core:UcoObject .

_:node1gm7uj6vjx303 sh:datatype xsd:string .

_:node1gm7uj6vjx302 rdf:first _:node1gm7uj6vjx303 ;
	rdf:rest rdf:nil .

_:node1gm7uj6vjx295 sh:or _:node1gm7uj6vjx299 .

tool:Tool rdfs:subClassOf core:UcoObject .

types:threadNextItem-subjects-shape sh:targetSubjectsOf types:threadNextItem .

marking:license rdfs:comment "Specifies the identifier for the type of license" .

_:node1gm7uj6vjx298 sh:path identity:familyName .

core:Item rdfs:label "Item"@en .

identity:SimpleNameFacet sh:property _:node1gm7uj6vjx298 .

uco-owl:ontologyIRI-versionIRI-prerequisite-shape rdfs:seeAlso <https://www.w3.org/TR/owl2-syntax/#Ontology_IRI_and_Version_IRI> .

_:node1gm7uj6vjx295 sh:path action:trend .

action:ActionFrequencyFacet sh:property _:node1gm7uj6vjx295 .

tool:Tool rdfs:label "Tool"@en .

_:node1gm7uj6vjx304 rdf:first "Create File Mapping"^^vocabulary:ActionNameVocab ;
	rdf:rest _:node1gm7uj6vjx307 .

marking:license rdfs:range xsd:string .

_:node1gm7uj6vjx305 sh:datatype xsd:string .

types:threadOriginItem a owl:ObjectProperty .

_:node1gm7uj6vjx305 sh:nodeKind sh:Literal .

types:threadOriginItem rdfs:subPropertyOf co:item .

_:node1gm7uj6vjx305 sh:path identity:givenName .

identity:SimpleNameFacet sh:property _:node1gm7uj6vjx305 .

marking:marking a owl:ObjectProperty .

_:node1gm7uj6vjx307 rdf:first "Create File Symbolic Link"^^vocabulary:ActionNameVocab .

core:Item rdfs:comment "An item is a distinct article or unit."@en .

_:node1gm7uj6vjx307 rdf:rest _:node1gm7uj6vjx309 .

_:node1gm7uj6vjx306 sh:message "Value is not member of the vocabulary TrendVocab." .

uco-owl:ontologyIRI-versionIRI-prerequisite-shape sh:message "'An ontology without an ontology IRI MUST NOT contain a version IRI.'"@en .

_:node1gm7uj6vjx308 sh:datatype xsd:string .

types:threadOriginItem rdfs:label "threadOriginItem"@en .

core:Item sh:targetClass core:Item .

marking:marking rdfs:label "marking"@en .

uco-owl:ontologyIRI-versionIRI-prerequisite-shape sh:nodeKind sh:IRI .

tool:Tool rdfs:comment "A tool is an element of hardware and/or software utilized to carry out a particular function."@en .

_:node1gm7uj6vjx308 sh:nodeKind sh:Literal .

_:node1gm7uj6vjx311 sh:datatype vocabulary:TrendVocab .

observable:AlternateDataStream rdfs:comment "An alternate data stream is data content stored within an NTFS file that is independent of the standard content stream of the file and is hidden from access by default NTFS file viewing mechanisms."@en .

_:node1gm7uj6vjx309 rdf:first "Create Hidden File"^^vocabulary:ActionNameVocab ;
	rdf:rest _:node1gm7uj6vjx314 .

uco-owl:ontologyIRI-versionIRI-prerequisite-shape sh:targetSubjectsOf owl:versionIRI .

_:node1gm7uj6vjx308 sh:path identity:honorificPrefix .

identity:SimpleNameFacet sh:property _:node1gm7uj6vjx308 .

_:node1gm7uj6vjx313 sh:class identity:Identity .

core:MarkingDefinitionAbstraction a owl:Class .

_:node1gm7uj6vjx312 rdf:first "Decreasing"^^vocabulary:TrendVocab ;
	rdf:rest _:node1gm7uj6vjx316 .

types:threadOriginItem rdfs:comment "A link to an item of the thread known to have no predecessor."@en .

core:MarkingDefinitionAbstraction a sh:NodeShape .

_:node1gm7uj6vjx315 sh:datatype xsd:string .

_:node1gm7uj6vjx314 rdf:first "Create Mailslot"^^vocabulary:ActionNameVocab ;
	rdf:rest _:node1gm7uj6vjx317 .

observable:AlternateDataStream sh:targetClass observable:AlternateDataStream .

marking:marking rdfs:comment "Represents specific marking definitions to be applied to UCO data."@en .

_:node1gm7uj6vjx313 sh:maxCount 1 .

types:threadOriginItem rdfs:domain types:Thread .

_:node1gm7uj6vjx315 sh:nodeKind sh:Literal .

core:MarkingDefinitionAbstraction rdfs:subClassOf core:UcoObject .

_:node1gm7uj6vjx313 sh:nodeKind sh:IRI .

_:node1gm7uj6vjx316 rdf:first "Increasing"^^vocabulary:TrendVocab .

uco-owl:versionIRI-multiversion-shape a sh:PropertyShape .

_:node1gm7uj6vjx316 rdf:rest rdf:nil .

marking:marking rdfs:range marking:MarkingDefinition .

_:node1gm7uj6vjx311 sh:in _:node1gm7uj6vjx312 .

_:node1gm7uj6vjx310 rdf:first _:node1gm7uj6vjx311 ;
	rdf:rest _:node1gm7uj6vjx319 .

_:node1gm7uj6vjx317 rdf:first "Create Module"^^vocabulary:ActionNameVocab ;
	rdf:rest _:node1gm7uj6vjx321 .

_:node1gm7uj6vjx318 a owl:Class .

observable:AlternateDataStreamFacet a owl:Class .

_:node1gm7uj6vjx313 sh:path tool:creator .

tool:Tool sh:property _:node1gm7uj6vjx313 .

_:node1gm7uj6vjx315 sh:path identity:honorificSuffix .

identity:SimpleNameFacet sh:property _:node1gm7uj6vjx315 .

core:MarkingDefinitionAbstraction rdfs:label "MarkingDefinitionAbstraction"@en .

observable:AlternateDataStreamFacet a sh:NodeShape .

_:node1gm7uj6vjx320 sh:datatype xsd:string .

_:node1gm7uj6vjx319 rdf:first _:node1gm7uj6vjx320 ;
	rdf:rest rdf:nil .

_:node1gm7uj6vjx306 sh:or _:node1gm7uj6vjx310 .

uco-owl:versionIRI-multiversion-shape rdfs:seeAlso <https://www.w3.org/TR/owl2-syntax/#Imports> .

_:node1gm7uj6vjx321 rdf:first "Create Mutex"^^vocabulary:ActionNameVocab ;
	rdf:rest _:node1gm7uj6vjx324 .

_:node1gm7uj6vjx323 rdf:first types:ThreadItem .

_:node1gm7uj6vjx322 sh:datatype xsd:anyURI .

_:node1gm7uj6vjx323 rdf:rest _:node1gm7uj6vjx325 .

marking:statement a owl:DatatypeProperty .

observable:AlternateDataStreamFacet rdfs:subClassOf core:Facet .

_:node1gm7uj6vjx306 sh:path action:trend .

action:ActionFrequencyFacet sh:property _:node1gm7uj6vjx306 .

identity:SimpleNameFacet sh:targetClass identity:SimpleNameFacet .

_:node1gm7uj6vjx326 a owl:Restriction .

_:node1gm7uj6vjx322 sh:nodeKind sh:Literal .

marking:statement rdfs:label "Statement"@en-us .

uco-owl:versionIRI-multiversion-shape sh:maxCount 1 .

_:node1gm7uj6vjx324 rdf:first "Create Named Pipe"^^vocabulary:ActionNameVocab ;
	rdf:rest _:node1gm7uj6vjx327 .

observable:AlternateDataStreamFacet rdfs:label "AlternateDataStreamFacet"@en .

_:node1gm7uj6vjx322 sh:path tool:references .

tool:Tool sh:property _:node1gm7uj6vjx322 .

action:ActionFrequencyFacet sh:targetClass action:ActionFrequencyFacet .

identity:VisaFacet a owl:Class .

_:node1gm7uj6vjx326 owl:onProperty types:threadPreviousItem .

identity:VisaFacet a sh:NodeShape .

_:node1gm7uj6vjx328 sh:datatype xsd:string .

_:node1gm7uj6vjx327 rdf:first "Create Process"^^vocabulary:ActionNameVocab ;
	rdf:rest _:node1gm7uj6vjx329 .

action:ActionLifecycle a owl:Class .

identity:VisaFacet rdfs:subClassOf identity:IdentityFacet .

_:node1gm7uj6vjx328 sh:maxCount 1 .

action:ActionLifecycle a sh:NodeShape .

_:node1gm7uj6vjx326 owl:cardinality "0"^^xsd:nonNegativeInteger .

_:node1gm7uj6vjx325 rdf:first _:node1gm7uj6vjx326 ;
	rdf:rest rdf:nil .

_:node1gm7uj6vjx318 owl:intersectionOf _:node1gm7uj6vjx323 .

types:threadOriginItem rdfs:range _:node1gm7uj6vjx318 .

_:node1gm7uj6vjx329 rdf:first "Create Process as User"^^vocabulary:ActionNameVocab ;
	rdf:rest _:node1gm7uj6vjx330 .

marking:statement rdfs:comment "Specifies the statement to apply to the structure for which the Marking is to be applied."@en-us .

_:node1gm7uj6vjx328 sh:nodeKind sh:Literal .

identity:VisaFacet rdfs:label "VisaFacet"@en .

action:ActionLifecycle rdfs:subClassOf action:Action .

types:threadOriginItem rdfs:seeAlso co:firstItem .

marking:statement rdfs:range xsd:string .

_:node1gm7uj6vjx328 sh:path tool:servicePack .

tool:Tool sh:property _:node1gm7uj6vjx328 .

_:node1gm7uj6vjx330 rdf:first "Create Registry Key"^^vocabulary:ActionNameVocab ;
	rdf:rest _:node1gm7uj6vjx332 .

action:ActionLifecycle rdfs:label "ActionLifecycle"@en .

_:node1gm7uj6vjx331 sh:datatype xsd:string .

uco-owl:versionIRI-multiversion-shape sh:message "'The import closure of [ontology] O SHOULD NOT contain ontologies O_1 and O_2 such that O_1 and O_2 are different ontology versions from the same ontology series.'"@en .

marking:termsOfUse a owl:DatatypeProperty .

_:node1gm7uj6vjx331 sh:maxCount 1 .

uco-owl:versionIRI-multiversion-shape sh:path owl:versionIRI .

types:threadOriginItem-subjects-shape a sh:PropertyShape .

_:node1gm7uj6vjx332 rdf:first "Create Registry Key Value"^^vocabulary:ActionNameVocab ;
	rdf:rest _:node1gm7uj6vjx333 .

_:node1gm7uj6vjx331 sh:nodeKind sh:Literal .

uco-owl:versionIRI-multiversion-shape sh:severity sh:Warning .

marking:termsOfUse rdfs:label "Terms of Use"@en-us .

types:threadOriginItem-subjects-shape sh:class types:ThreadItem .

_:node1gm7uj6vjx331 sh:path tool:toolType .

tool:Tool sh:property _:node1gm7uj6vjx331 .

types:threadOriginItem-subjects-shape sh:nodeKind sh:IRI .

uco-owl:versionIRI-multiversion-shape sh:targetSubjectsOf owl:versionIRI .

_:node1gm7uj6vjx334 sh:datatype xsd:string .

observable:AlternateDataStreamFacet rdfs:comment "An alternate data stream facet is a grouping of characteristics unique to data content stored within an NTFS file that is independent of the standard content stream of the file and is hidden from access by default NTFS file viewing mechanisms."@en .

_:node1gm7uj6vjx333 rdf:first "Create Remote Thread in Process"^^vocabulary:ActionNameVocab ;
	rdf:rest _:node1gm7uj6vjx335 .

types:threadOriginItem-subjects-shape sh:path types:threadOriginItem .

identity:VisaFacet rdfs:comment "Visa is a grouping of characteristics unique to information related to a person's ability to enter, leave, or stay for a specified period of time in a country."@en .

_:node1gm7uj6vjx336 sh:class types:Hash .

_:node1gm7uj6vjx334 sh:maxCount 1 .

action:ActionLifecycle rdfs:comment "An action lifecycle is an action pattern consisting of an ordered set of multiple actions or subordinate action lifecycles."@en .

core:MarkingDefinitionAbstraction rdfs:comment "A marking definition abstraction is a grouping of characteristics unique to the expression of a specific data marking conveying restrictions, permissions, and other guidance for how marked data can be used and shared. This class is an ontological structural abstraction for this concept. Implementations of this concept should utilize the marking:MarkingDefinition class."@en .

identity:VisaFacet sh:targetClass identity:VisaFacet .

marking:termsOfUse rdfs:comment "Specifies the terms of use that apply to the structure for which the Marking is to be applied."@en-us .

types:threadOriginItem-subjects-shape sh:targetSubjectsOf types:threadOriginItem .

uco-owl:versionIRI-nodeKind-shape a sh:PropertyShape .

_:node1gm7uj6vjx335 rdf:first "Create Service"^^vocabulary:ActionNameVocab ;
	rdf:rest _:node1gm7uj6vjx337 .

_:node1gm7uj6vjx334 sh:nodeKind sh:Literal .

marking:termsOfUse rdfs:range xsd:string .

uco-owl:versionIRI-nodeKind-shape sh:nodeKind sh:IRI .

_:node1gm7uj6vjx336 sh:maxCount 1 .

_:node1gm7uj6vjx334 sh:path tool:version .

tool:Tool sh:property _:node1gm7uj6vjx334 .

_:node1gm7uj6vjx337 rdf:first "Create Socket"^^vocabulary:ActionNameVocab ;
	rdf:rest _:node1gm7uj6vjx339 .

identity:address a owl:ObjectProperty .

_:node1gm7uj6vjx336 sh:nodeKind sh:IRI .

_:node1gm7uj6vjx338 sh:class action:ArrayOfAction .

uco-owl:versionIRI-nodeKind-shape sh:path owl:versionIRI .

identity:address rdfs:label "address"@en .

_:node1gm7uj6vjx336 sh:path observable:hashes .

tool:Tool sh:targetClass tool:Tool .

observable:AlternateDataStreamFacet sh:property _:node1gm7uj6vjx336 .

identity:address rdfs:comment ""@en .

core:MarkingDefinitionAbstraction sh:targetClass core:MarkingDefinitionAbstraction .

_:node1gm7uj6vjx339 rdf:first "Create Symbolic Link"^^vocabulary:ActionNameVocab ;
	rdf:rest _:node1gm7uj6vjx341 .

_:node1gm7uj6vjx338 sh:maxCount 1 .

_:node1gm7uj6vjx340 sh:datatype xsd:integer .

identity:address rdfs:range location:Location .

uco-owl:versionIRI-nodeKind-shape sh:targetSubjectsOf owl:versionIRI .

types:threadOriginItem-subjects-threadPredecessor-shape a sh:PropertyShape .

tool:buildConfiguration a owl:ObjectProperty .

core:ModusOperandi a owl:Class , sh:NodeShape .

tool:buildConfiguration rdfs:label "buildConfiguration"@en .

_:node1gm7uj6vjx338 sh:minCount 1 .

_:node1gm7uj6vjx341 rdf:first "Create Thread"^^vocabulary:ActionNameVocab ;
	rdf:rest _:node1gm7uj6vjx342 .

_:node1gm7uj6vjx340 sh:maxCount 1 .

_:node1gm7uj6vjx338 sh:nodeKind sh:IRI .

core:ModusOperandi rdfs:subClassOf core:UcoObject .

identity:birthdate a owl:DatatypeProperty .

_:node1gm7uj6vjx340 sh:nodeKind sh:Literal .

_:node1gm7uj6vjx338 sh:path action:phase .

action:ActionLifecycle sh:property _:node1gm7uj6vjx338 .

identity:birthdate rdfs:label "birthdate"@en .

core:ModusOperandi rdfs:label "ModusOperandi"@en .

types:threadOriginItem-subjects-threadPredecessor-shape sh:description "An origin item in a thread must not have a predecessor."@en .

_:node1gm7uj6vjx340 sh:path observable:size .

observable:AlternateDataStreamFacet sh:property _:node1gm7uj6vjx340 .

tool:buildConfiguration rdfs:comment "How the build utility was configured for a particular build of a particular software."@en .

identity:birthdate rdfs:comment ""@en .

_:node1gm7uj6vjx342 rdf:first "Create Window"^^vocabulary:ActionNameVocab .

_:node1gm7uj6vjx343 sh:class core:UcoObject .

_:node1gm7uj6vjx342 rdf:rest _:node1gm7uj6vjx345 .

_:node1gm7uj6vjx344 sh:datatype xsd:string .

identity:birthdate rdfs:range xsd:dateTime .

types:threadOriginItem-subjects-threadPredecessor-shape sh:maxCount 0 .

tool:buildConfiguration rdfs:range configuration:Configuration .

types:threadOriginItem-subjects-threadPredecessor-shape sh:nodeKind sh:IRI .

core:ModusOperandi rdfs:comment "A modus operandi is a particular method of operation (how a particular entity behaves or the resources they use)."@en .

_:node1gm7uj6vjx343 sh:maxCount 0 .

_:node1gm7uj6vjx344 sh:maxCount 1 .

_:node1gm7uj6vjx343 sh:nodeKind sh:IRI .

tool:buildID a owl:DatatypeProperty .

_:node1gm7uj6vjx345 rdf:first "Delete Directory"^^vocabulary:ActionNameVocab .

identity:familyName a owl:DatatypeProperty .

_:node1gm7uj6vjx345 rdf:rest _:node1gm7uj6vjx347 .

core:ModusOperandi sh:targetClass core:ModusOperandi .

_:node1gm7uj6vjx344 sh:nodeKind sh:Literal .

tool:buildID rdfs:label "buildID"@en .

_:node1gm7uj6vjx346 rdf:first types:threadOriginItem ;
	rdf:rest _:node1gm7uj6vjx348 .

_:node1gm7uj6vjx343 sh:path action:error .

identity:familyName rdfs:label "familyName"@en .

action:ActionLifecycle sh:property _:node1gm7uj6vjx343 .

_:node1gm7uj6vjx344 sh:path core:name .

observable:AlternateDataStreamFacet sh:property _:node1gm7uj6vjx344 .

_:node1gm7uj6vjx348 rdf:first types:threadPredecessor ;
	rdf:rest rdf:nil .

_:node1gm7uj6vjx347 rdf:first "Delete File"^^vocabulary:ActionNameVocab .

types:threadOriginItem-subjects-threadPredecessor-shape sh:path _:node1gm7uj6vjx346 .

_:node1gm7uj6vjx347 rdf:rest _:node1gm7uj6vjx350 .

identity:familyName rdfs:comment ""@en .

tool:buildID rdfs:comment "An externally defined unique identifier for a particular build of a software."@en .

core:Relationship a owl:Class .

_:node1gm7uj6vjx349 sh:datatype xsd:dateTime .

identity:familyName rdfs:range xsd:string .

core:Relationship a sh:NodeShape .

tool:buildID rdfs:range xsd:string .

observable:AlternateDataStreamFacet sh:targetClass observable:AlternateDataStreamFacet .

types:threadOriginItem-subjects-threadPredecessor-shape sh:targetSubjectsOf types:threadOriginItem .

core:Relationship rdfs:subClassOf core:UcoObject .

identity:givenName a owl:DatatypeProperty .

observable:AndroidDevice a owl:Class .

tool:buildInformation a owl:ObjectProperty .

_:node1gm7uj6vjx349 sh:maxCount 0 .

_:node1gm7uj6vjx350 rdf:first "Delete Named Pipe"^^vocabulary:ActionNameVocab ;
	rdf:rest _:node1gm7uj6vjx351 .

observable:AndroidDevice a sh:NodeShape .

core:Relationship rdfs:label "Relationship"@en .

identity:givenName rdfs:label "givenName"@en .

tool:buildInformation rdfs:label "buildInformation"@en .

_:node1gm7uj6vjx349 sh:nodeKind sh:Literal .

identity:givenName rdfs:comment ""@en .

observable:AndroidDevice rdfs:subClassOf observable:Device .

types:threadOriginItem-subjects-threadPreviousItem-shape a sh:PropertyShape .

_:node1gm7uj6vjx351 rdf:first "Delete Network Share"^^vocabulary:ActionNameVocab ;
	rdf:rest _:node1gm7uj6vjx352 .

_:node1gm7uj6vjx349 sh:path action:endTime .

action:ActionLifecycle sh:property _:node1gm7uj6vjx349 .

identity:givenName rdfs:range xsd:string .

observable:AndroidDevice rdfs:label "AndroidDevice"@en .

tool:buildInformation rdfs:comment "Describes how a particular tool was built."@en .

_:node1gm7uj6vjx353 sh:datatype xsd:dateTime .

tool:buildInformation rdfs:range tool:BuildInformationType .

identity:honorificPrefix a owl:DatatypeProperty .

_:node1gm7uj6vjx353 sh:maxCount 0 .

types:threadOriginItem-subjects-threadPreviousItem-shape sh:description "An origin item in a thread must not have a previous item."@en .

_:node1gm7uj6vjx352 rdf:first "Delete Registry Key"^^vocabulary:ActionNameVocab ;
	rdf:rest _:node1gm7uj6vjx354 .

identity:honorificPrefix rdfs:label "honorificPrefix"@en .

_:node1gm7uj6vjx353 sh:nodeKind sh:Literal .

core:Relationship rdfs:comment "A relationship is a grouping of characteristics unique to an assertion that one or more objects are related to another object in some way."@en .

tool:buildLabel a owl:DatatypeProperty .

observable:AndroidDevice rdfs:comment "An Android device is a device running the Android operating system. [based on https://en.wikipedia.org/wiki/Android_(operating_system)]"@en .

identity:honorificPrefix rdfs:comment ""@en .

tool:buildLabel rdfs:label "buildLabel"@en .

types:threadOriginItem-subjects-threadPreviousItem-shape sh:maxCount 0 .

_:node1gm7uj6vjx353 sh:path action:startTime .

action:ActionLifecycle sh:property _:node1gm7uj6vjx353 .

identity:honorificPrefix rdfs:range xsd:string .

tool:buildLabel rdfs:comment "Relevant label for a particular build of a particular software."@en .

types:threadOriginItem-subjects-threadPreviousItem-shape sh:nodeKind sh:IRI .

_:node1gm7uj6vjx355 sh:class core:UcoObject .

_:node1gm7uj6vjx354 rdf:first "Delete Registry Key Value"^^vocabulary:ActionNameVocab ;
	rdf:rest _:node1gm7uj6vjx358 .

observable:AndroidDevice sh:targetClass observable:AndroidDevice .

_:node1gm7uj6vjx356 sh:datatype xsd:nonNegativeInteger .

tool:buildLabel rdfs:range xsd:string .

_:node1gm7uj6vjx357 rdf:first types:threadOriginItem ;
	rdf:rest _:node1gm7uj6vjx359 .

_:node1gm7uj6vjx355 sh:maxCount 1 .

identity:honorificSuffix a owl:DatatypeProperty .

_:node1gm7uj6vjx358 rdf:first "Delete Service"^^vocabulary:ActionNameVocab ;
	rdf:rest _:node1gm7uj6vjx360 .

_:node1gm7uj6vjx359 rdf:first types:threadPreviousItem .

_:node1gm7uj6vjx356 sh:maxCount 0 .

_:node1gm7uj6vjx359 rdf:rest rdf:nil .

types:threadOriginItem-subjects-threadPreviousItem-shape sh:path _:node1gm7uj6vjx357 .

observable:AndroidDeviceFacet a owl:Class .

tool:buildOutputLog a owl:DatatypeProperty .

identity:honorificSuffix rdfs:label "honorificSuffix"@en .

observable:AndroidDeviceFacet a sh:NodeShape .

_:node1gm7uj6vjx355 sh:minCount 1 .

_:node1gm7uj6vjx356 sh:nodeKind sh:Literal .

tool:buildOutputLog rdfs:label "buildOutputLog"@en .

_:node1gm7uj6vjx360 rdf:first "Delete User"^^vocabulary:ActionNameVocab ;
	rdf:rest _:node1gm7uj6vjx361 .

identity:honorificSuffix rdfs:comment ""@en .

types:threadOriginItem-subjects-threadPreviousItem-shape sh:targetSubjectsOf types:threadOriginItem .

_:node1gm7uj6vjx355 sh:nodeKind sh:IRI .

observable:AndroidDeviceFacet rdfs:subClassOf core:Facet .

identity:honorificSuffix rdfs:range xsd:string .

_:node1gm7uj6vjx361 rdf:first "Disconnect from Named Pipe"^^vocabulary:ActionNameVocab ;
	rdf:rest _:node1gm7uj6vjx362 .

_:node1gm7uj6vjx355 sh:path core:target .

core:Relationship sh:property _:node1gm7uj6vjx355 .

_:node1gm7uj6vjx356 sh:path action:actionCount .

action:ActionLifecycle sh:property _:node1gm7uj6vjx356 .

observable:AndroidDeviceFacet rdfs:label "AndroidDeviceFacet"@en .

tool:buildOutputLog rdfs:comment "The output log of the build process for a software."@en .

_:node1gm7uj6vjx363 sh:class core:UcoObject .

types:threadPredecessor a owl:ObjectProperty .

_:node1gm7uj6vjx364 sh:maxCount 0 .

_:node1gm7uj6vjx362 rdf:first "Disconnect from Network Share"^^vocabulary:ActionNameVocab ;
	rdf:rest _:node1gm7uj6vjx365 .

tool:buildOutputLog rdfs:range xsd:string .

_:node1gm7uj6vjx363 sh:minCount 1 .

types:threadPredecessor a owl:TransitiveProperty .

observable:AndroidDeviceFacet rdfs:comment "An Android device facet is a grouping of characteristics unique to an Android device. [based on https://en.wikipedia.org/wiki/Android_(operating_system)]"@en .

types:threadPredecessor rdfs:label "threadPredecessor"@en .

_:node1gm7uj6vjx363 sh:nodeKind sh:IRI .

_:node1gm7uj6vjx364 sh:path action:actionStatus .

action:ActionLifecycle sh:property _:node1gm7uj6vjx364 .

_:node1gm7uj6vjx365 rdf:first "Disconnect from Socket"^^vocabulary:ActionNameVocab ;
	rdf:rest _:node1gm7uj6vjx367 .

tool:buildProject a owl:DatatypeProperty .

_:node1gm7uj6vjx363 sh:path core:source .

core:Relationship sh:property _:node1gm7uj6vjx363 .

types:threadPredecessor rdfs:comment "The link to the preceding item in a thread."@en .

action:ActionLifecycle sh:targetClass action:ActionLifecycle .

_:node1gm7uj6vjx366 sh:datatype xsd:boolean .

tool:buildProject rdfs:label "buildProject"@en .

_:node1gm7uj6vjx367 rdf:first "Download File"^^vocabulary:ActionNameVocab ;
	rdf:rest _:node1gm7uj6vjx369 .

_:node1gm7uj6vjx368 sh:datatype xsd:boolean .

types:threadPredecessor rdfs:domain types:ThreadItem .

_:node1gm7uj6vjx366 sh:maxCount 1 .

tool:buildProject rdfs:comment "The project name of a build of a software."@en .

_:node1gm7uj6vjx369 rdf:first "Enumerate DLLs"^^vocabulary:ActionNameVocab ;
	rdf:rest _:node1gm7uj6vjx370 .

action:ActionPattern a owl:Class .

_:node1gm7uj6vjx366 sh:nodeKind sh:Literal .

_:node1gm7uj6vjx368 sh:maxCount 1 .

tool:buildProject rdfs:range xsd:string .

types:threadPredecessor rdfs:range types:ThreadItem .

action:ActionPattern a sh:NodeShape .

_:node1gm7uj6vjx370 rdf:first "Enumerate Network Shares"^^vocabulary:ActionNameVocab ;
	rdf:rest _:node1gm7uj6vjx371 .

_:node1gm7uj6vjx368 sh:minCount 1 .

_:node1gm7uj6vjx366 sh:path observable:isADBRootEnabled .

types:threadPredecessor rdfs:seeAlso co:precededBy .

observable:AndroidDeviceFacet sh:property _:node1gm7uj6vjx366 .

action:ActionPattern rdfs:subClassOf action:Action .

tool:buildScript a owl:DatatypeProperty .

action:ActionPattern rdfs:subClassOf pattern:Pattern .

_:node1gm7uj6vjx368 sh:nodeKind sh:Literal .

_:node1gm7uj6vjx372 sh:datatype xsd:boolean .

_:node1gm7uj6vjx371 rdf:first "Enumerate Processes"^^vocabulary:ActionNameVocab .

types:threadPredecessor owl:inverseOf types:threadSuccessor .

_:node1gm7uj6vjx371 rdf:rest _:node1gm7uj6vjx373 .

tool:buildScript rdfs:label "buildScript"@en .

_:node1gm7uj6vjx368 sh:path core:isDirectional .

core:Relationship sh:property _:node1gm7uj6vjx368 .

_:node1gm7uj6vjx372 sh:maxCount 1 .

action:ActionPattern rdfs:label "ActionPattern"@en .

tool:buildScript rdfs:comment "The actual build script for a particular build of a particular software."@en .

_:node1gm7uj6vjx373 rdf:first "Enumerate Protocols"^^vocabulary:ActionNameVocab ;
	rdf:rest _:node1gm7uj6vjx375 .

_:node1gm7uj6vjx374 sh:datatype xsd:dateTime .

_:node1gm7uj6vjx372 sh:nodeKind sh:Literal .

tool:buildScript rdfs:range xsd:string .

_:node1gm7uj6vjx375 rdf:first "Enumerate Registry Key Subkeys"^^vocabulary:ActionNameVocab ;
	rdf:rest _:node1gm7uj6vjx376 .

_:node1gm7uj6vjx374 sh:nodeKind sh:Literal .

types:threadPredecessor-subjects-shape a sh:PropertyShape .

_:node1gm7uj6vjx372 sh:path observable:isSURootEnabled .

observable:AndroidDeviceFacet sh:property _:node1gm7uj6vjx372 .

_:node1gm7uj6vjx374 sh:path core:endTime .

core:Relationship sh:property _:node1gm7uj6vjx374 .

types:threadPredecessor-subjects-shape sh:class types:ThreadItem .

action:ActionPattern rdfs:comment "An action pattern is a grouping of characteristics unique to a combination of actions forming a consistent or characteristic arrangement."@en .

tool:buildUtility a owl:ObjectProperty .

_:node1gm7uj6vjx376 rdf:first "Enumerate Registry Key Values"^^vocabulary:ActionNameVocab ;
	rdf:rest _:node1gm7uj6vjx379 .

_:node1gm7uj6vjx377 sh:datatype xsd:hexBinary .

tool:buildUtility rdfs:label "buildUtility"@en .

types:threadPredecessor-subjects-shape sh:nodeKind sh:IRI .

_:node1gm7uj6vjx378 sh:datatype xsd:dateTime .

_:node1gm7uj6vjx377 sh:maxCount 1 .

_:node1gm7uj6vjx379 rdf:first "Enumerate Services"^^vocabulary:ActionNameVocab ;
	rdf:rest _:node1gm7uj6vjx380 .

types:threadPredecessor-subjects-shape sh:path types:threadPredecessor .

_:node1gm7uj6vjx378 sh:nodeKind sh:Literal .

action:ActionPattern sh:targetClass action:ActionPattern .

tool:buildUtility rdfs:comment "Identifies the utility used to build a software."@en .

_:node1gm7uj6vjx377 sh:nodeKind sh:Literal .

_:node1gm7uj6vjx378 sh:path core:startTime .

core:Relationship sh:property _:node1gm7uj6vjx378 .

_:node1gm7uj6vjx380 rdf:first "Enumerate System Handles"^^vocabulary:ActionNameVocab ;
	rdf:rest _:node1gm7uj6vjx382 .

action:ArrayOfAction a owl:Class .

_:node1gm7uj6vjx377 sh:path observable:androidID .

observable:AndroidDeviceFacet sh:property _:node1gm7uj6vjx377 .

tool:buildUtility rdfs:range tool:BuildUtilityType .

types:threadPredecessor-subjects-shape sh:targetSubjectsOf types:threadPredecessor .

_:node1gm7uj6vjx381 sh:datatype xsd:string .

action:ArrayOfAction a sh:NodeShape .

_:node1gm7uj6vjx382 rdf:first "Enumerate Threads"^^vocabulary:ActionNameVocab ;
	rdf:rest _:node1gm7uj6vjx384 .

_:node1gm7uj6vjx383 sh:datatype xsd:string .

_:node1gm7uj6vjx381 sh:maxCount 1 .

tool:buildUtilityName a owl:DatatypeProperty .

_:node1gm7uj6vjx384 rdf:first "Enumerate Threads in Process"^^vocabulary:ActionNameVocab ;
	rdf:rest _:node1gm7uj6vjx385 .

_:node1gm7uj6vjx383 sh:maxCount 1 .

action:ArrayOfAction rdfs:subClassOf core:UcoInherentCharacterizationThing .

_:node1gm7uj6vjx381 sh:nodeKind sh:Literal .

types:threadPreviousItem a owl:ObjectProperty .

tool:buildUtilityName rdfs:label "buildUtilityName"@en .

_:node1gm7uj6vjx385 rdf:first "Enumerate Users"^^vocabulary:ActionNameVocab ;
	rdf:rest _:node1gm7uj6vjx386 .

_:node1gm7uj6vjx383 sh:nodeKind sh:Literal .

_:node1gm7uj6vjx381 sh:path core:kindOfRelationship .

action:ArrayOfAction rdfs:label "ArrayOfAction"@en .

core:Relationship sh:property _:node1gm7uj6vjx381 .

types:threadPreviousItem rdfs:subPropertyOf types:threadPredecessor .

_:node1gm7uj6vjx383 sh:path observable:androidFingerprint .

_:node1gm7uj6vjx386 rdf:first "Enumerate Windows"^^vocabulary:ActionNameVocab .

observable:AndroidDeviceFacet sh:property _:node1gm7uj6vjx383 .

_:node1gm7uj6vjx386 rdf:rest _:node1gm7uj6vjx387 .

core:Relationship sh:targetClass core:Relationship .

_:node1gm7uj6vjx388 sh:datatype xsd:string .

_:node1gm7uj6vjx387 rdf:first "Find File"^^vocabulary:ActionNameVocab ;
	rdf:rest _:node1gm7uj6vjx389 .

types:threadPreviousItem rdfs:label "threadPreviousItem"@en .

tool:buildUtilityName rdfs:comment "The informally defined name of the utility used to build a particular software."@en .

_:node1gm7uj6vjx388 sh:maxCount 1 .

core:UcoInherentCharacterizationThing a owl:Class .

tool:buildUtilityName rdfs:range xsd:string .

_:node1gm7uj6vjx388 sh:nodeKind sh:Literal .

_:node1gm7uj6vjx389 rdf:first "Find Window"^^vocabulary:ActionNameVocab ;
	rdf:rest _:node1gm7uj6vjx390 .

action:ArrayOfAction rdfs:comment "An array of action is an ordered list of references to things that may be done or performed."@en .

core:UcoInherentCharacterizationThing a sh:NodeShape .

_:node1gm7uj6vjx388 sh:path observable:androidVersion .

observable:AndroidDeviceFacet sh:property _:node1gm7uj6vjx388 .

core:UcoInherentCharacterizationThing rdfs:subClassOf core:UcoThing .

types:threadPreviousItem rdfs:comment "A direct link to a previous item in a thread."@en .

_:node1gm7uj6vjx391 sh:class action:Action .

tool:buildVersion a owl:DatatypeProperty .

_:node1gm7uj6vjx390 rdf:first "Flush Process Instruction Cache"^^vocabulary:ActionNameVocab ;
	rdf:rest _:node1gm7uj6vjx392 .

types:threadPreviousItem rdfs:seeAlso co:previousItem .

observable:AndroidDeviceFacet sh:targetClass observable:AndroidDeviceFacet .

_:node1gm7uj6vjx391 sh:minCount 1 .

tool:buildVersion rdfs:label "buildVersion"@en .

core:UcoInherentCharacterizationThing rdfs:label "UcoInherentCharacterizationThing"@en .

_:node1gm7uj6vjx391 sh:nodeKind sh:IRI .

core:UcoInherentCharacterizationThing rdfs:comment "A UCO inherent characterization thing is a grouping of characteristics unique to a particular inherent aspect of a UCO domain object."@en .

tool:buildVersion rdfs:comment "The appropriate version descriptor of a particular build of a particular software."@en .

types:threadPreviousItem owl:inverseOf types:threadNextItem .

_:node1gm7uj6vjx392 rdf:first "Free Library"^^vocabulary:ActionNameVocab ;
	rdf:rest _:node1gm7uj6vjx393 .

_:node1gm7uj6vjx391 sh:path action:action .

observable:AndroidPhone a owl:Class .

tool:buildVersion rdfs:range xsd:string .

action:ArrayOfAction sh:property _:node1gm7uj6vjx391 .

observable:AndroidPhone a sh:NodeShape .

_:node1gm7uj6vjx393 rdf:first "Free Process Virtual Memory"^^vocabulary:ActionNameVocab ;
	rdf:rest _:node1gm7uj6vjx394 .

core:UcoInherentCharacterizationThing sh:targetClass core:UcoInherentCharacterizationThing .

action:ArrayOfAction sh:targetClass action:ArrayOfAction .

tool:compilationDate a owl:DatatypeProperty .

observable:AndroidPhone rdfs:subClassOf observable:AndroidDevice .

_:node1gm7uj6vjx394 rdf:first "Get Disk Free Space"^^vocabulary:ActionNameVocab ;
	rdf:rest _:node1gm7uj6vjx395 .

core:UcoObject a owl:Class .

types:threadPreviousItem-subjects-shape a sh:PropertyShape .

tool:compilationDate rdfs:label "compilationDate"@en .

core:UcoObject a sh:NodeShape .

observable:AndroidPhone rdfs:subClassOf observable:SmartPhone .

_:node1gm7uj6vjx395 rdf:first "Get Disk Type"^^vocabulary:ActionNameVocab ;
	rdf:rest _:node1gm7uj6vjx396 .

tool:compilationDate rdfs:comment "The compilation date for the build of a software."@en .

action:action a owl:ObjectProperty .

types:threadPreviousItem-subjects-shape sh:class types:ThreadItem .

_:node1gm7uj6vjx396 rdf:first "Get Elapsed System Up Time"^^vocabulary:ActionNameVocab ;
	rdf:rest _:node1gm7uj6vjx397 .

core:UcoObject rdfs:subClassOf core:UcoThing .

tool:compilationDate rdfs:range xsd:dateTime .

observable:AndroidPhone rdfs:label "AndroidPhone"@en-us .

types:threadPreviousItem-subjects-shape sh:nodeKind sh:IRI .

action:action rdfs:label "action"@en .

core:UcoObject rdfs:label "UcoObject"@en .

types:threadPreviousItem-subjects-shape sh:path types:threadPreviousItem .

_:node1gm7uj6vjx397 rdf:first "Get File Attributes"^^vocabulary:ActionNameVocab ;
	rdf:rest _:node1gm7uj6vjx398 .

tool:compilerInformalDescription a owl:DatatypeProperty .

types:threadPreviousItem-subjects-shape sh:targetSubjectsOf types:threadPreviousItem .

action:action rdfs:comment "A characterization of a single action."@en .

_:node1gm7uj6vjx398 rdf:first "Get Function Address"^^vocabulary:ActionNameVocab ;
	rdf:rest _:node1gm7uj6vjx399 .

tool:compilerInformalDescription rdfs:label "compilerInformalDescription"@en .

observable:AndroidPhone rdfs:comment "An android phone is a smart phone that applies the Android mobile operating system."@en-us .

action:action rdfs:range action:Action .

types:threadSuccessor a owl:ObjectProperty .

observable:AndroidPhone sh:targetClass observable:AndroidPhone .

tool:compilerInformalDescription rdfs:comment "An informal description of a compiler."@en .

core:UcoObject rdfs:comment "A UCO object is a representation of a fundamental concept either directly inherent to the cyber domain or indirectly related to the cyber domain and necessary for contextually characterizing cyber domain concepts and relationships. Within the Unified Cyber Ontology (UCO) structure this is the base class acting as a consistent, unifying and interoperable foundation for all explicit and inter-relatable content objects."@en .

_:node1gm7uj6vjx399 rdf:first "Get Host By Address"^^vocabulary:ActionNameVocab ;
	rdf:rest _:node1gm7uj6vjx400 .

types:threadSuccessor a owl:TransitiveProperty .

tool:compilerInformalDescription rdfs:range xsd:string .

action:actionCount a owl:DatatypeProperty .

observable:AntennaFacet a owl:Class .

_:node1gm7uj6vjx400 rdf:first "Get Host By Name"^^vocabulary:ActionNameVocab ;
	rdf:rest _:node1gm7uj6vjx402 .

observable:AntennaFacet a sh:NodeShape .

_:node1gm7uj6vjx401 sh:class core:ExternalReference .

types:threadSuccessor rdfs:label "threadSuccessor"@en .

action:actionCount rdfs:label "actionCount"@en .

observable:AntennaFacet rdfs:subClassOf core:Facet .

tool:compilers a owl:ObjectProperty .

_:node1gm7uj6vjx402 rdf:first "Get Host Name"^^vocabulary:ActionNameVocab ;
	rdf:rest _:node1gm7uj6vjx403 .

tool:compilers rdfs:label "compilers"@en .

_:node1gm7uj6vjx401 sh:minCount 0 .

_:node1gm7uj6vjx403 rdf:first "Get Library File Name"^^vocabulary:ActionNameVocab ;
	rdf:rest _:node1gm7uj6vjx404 .

observable:AntennaFacet rdfs:label "AntennaFacet"@en .

_:node1gm7uj6vjx401 sh:nodeKind sh:IRI .

_:node1gm7uj6vjx404 rdf:first "Get Library Handle"^^vocabulary:ActionNameVocab ;
	rdf:rest _:node1gm7uj6vjx405 .

_:node1gm7uj6vjx401 sh:path core:externalReference .

core:UcoObject sh:property _:node1gm7uj6vjx401 .

types:threadSuccessor rdfs:comment "A link to a following item in a thread."@en .

action:actionCount rdfs:comment "The number of times that the action was performed."@en .

_:node1gm7uj6vjx406 sh:class core:Facet .

tool:compilers rdfs:comment "The compilers utilized during a particular build of a particular software."@en .

_:node1gm7uj6vjx405 rdf:first "Get NetBIOS Name"^^vocabulary:ActionNameVocab ;
	rdf:rest _:node1gm7uj6vjx407 .

types:threadSuccessor rdfs:domain types:ThreadItem .

_:node1gm7uj6vjx406 sh:nodeKind sh:IRI .

action:actionCount rdfs:range xsd:nonNegativeInteger .

observable:AntennaFacet rdfs:comment "An antenna alignment facet contains the metadata surrounding the cell tower's antenna position."@en .

tool:compilers rdfs:range tool:CompilerType .

_:node1gm7uj6vjx406 sh:path core:hasFacet .

core:UcoObject sh:property _:node1gm7uj6vjx406 .

types:threadSuccessor rdfs:range types:ThreadItem .

_:node1gm7uj6vjx407 rdf:first "Get Process Current Directory"^^vocabulary:ActionNameVocab ;
	rdf:rest _:node1gm7uj6vjx410 .

_:node1gm7uj6vjx408 sh:class core:IdentityAbstraction .

_:node1gm7uj6vjx409 sh:datatype xsd:decimal .

tool:cpeid a owl:DatatypeProperty .

types:threadSuccessor rdfs:seeAlso co:followedBy .

tool:cpeid rdfs:label "cpeid"@en .

action:actionStatus a owl:DatatypeProperty .

_:node1gm7uj6vjx410 rdf:first "Get Process Environment Variable"^^vocabulary:ActionNameVocab ;
	rdf:rest _:node1gm7uj6vjx411 .

_:node1gm7uj6vjx409 sh:maxCount 1 .

_:node1gm7uj6vjx408 sh:maxCount 1 ;
	sh:nodeKind sh:IRI .

action:actionStatus rdfs:label "actionStatus"@en .

_:node1gm7uj6vjx409 sh:nodeKind sh:Literal .

types:threadSuccessor-subjects-shape a sh:PropertyShape .

_:node1gm7uj6vjx408 sh:path core:createdBy .

_:node1gm7uj6vjx411 rdf:first "Get Process Startup Information"^^vocabulary:ActionNameVocab .

core:UcoObject sh:property _:node1gm7uj6vjx408 .

_:node1gm7uj6vjx411 rdf:rest _:node1gm7uj6vjx412 .

_:node1gm7uj6vjx409 sh:path observable:antennaHeight .

observable:AntennaFacet sh:property _:node1gm7uj6vjx409 .

types:threadSuccessor-subjects-shape sh:class types:ThreadItem .

tool:cpeid rdfs:comment "Specifies the Common Platform Enumeration identifier for the software."@en .

action:actionStatus rdfs:comment "The current state of the action."@en .

tool:cpeid rdfs:range xsd:string .

_:node1gm7uj6vjx414 sh:datatype xsd:decimal .

types:threadSuccessor-subjects-shape sh:nodeKind sh:IRI .

_:node1gm7uj6vjx412 rdf:first "Get Processes Snapshot"^^vocabulary:ActionNameVocab .

_:node1gm7uj6vjx804 rdf:first "Overlay"^^vocabulary:MemoryBlockTypeVocab .

_:node1gm7uj6vjx413 sh:class core:MarkingDefinitionAbstraction .

observable:CapturedTelecommunicationsInformation sh:targetClass observable:CapturedTelecommunicationsInformation .

_:node1gm7uj6vjx412 rdf:rest _:node1gm7uj6vjx416 .

_:node1gm7uj6vjx804 rdf:rest _:node1gm7uj6vjx805 .

_:node1gm7uj6vjx415 a rdfs:Datatype .

_:node1gm7uj6vjx805 rdf:first "Uninitialized"^^vocabulary:MemoryBlockTypeVocab .

_:node1gm7uj6vjx414 sh:maxCount 1 .

_:node1gm7uj6vjx805 rdf:rest rdf:nil .

_:node1gm7uj6vjx413 sh:nodeKind sh:IRI .

_:node1gm7uj6vjx798 owl:oneOf _:node1gm7uj6vjx800 .

tool:creator a owl:ObjectProperty .

vocabulary:MemoryBlockTypeVocab owl:equivalentClass _:node1gm7uj6vjx798 .

types:threadSuccessor-subjects-shape sh:path types:threadSuccessor .

observable:CapturedTelecommunicationsInformationFacet a owl:Class .

_:node1gm7uj6vjx414 sh:nodeKind sh:Literal .

observable:CapturedTelecommunicationsInformationFacet a sh:NodeShape .

tool:creator rdfs:label "creator"@en .

vocabulary:ObservableObjectRelationshipVocab a rdfs:Datatype .

_:node1gm7uj6vjx413 sh:path core:objectMarking .

observable:CapturedTelecommunicationsInformationFacet rdfs:subClassOf core:Facet .

core:UcoObject sh:property _:node1gm7uj6vjx413 .

observable:CapturedTelecommunicationsInformationFacet rdfs:label "CapturedTelecommunicationsInformationFacet"@en .

_:node1gm7uj6vjx414 sh:path observable:azimuth .

vocabulary:ObservableObjectRelationshipVocab rdfs:label "Cyber Item Relationship Vocabulary"@en-us .

observable:AntennaFacet sh:property _:node1gm7uj6vjx414 .

observable:CapturedTelecommunicationsInformationFacet rdfs:comment "A captured telecommunications information facet represents certain information within captured or intercepted telecommunications data."@en .

_:node1gm7uj6vjx416 rdf:first "Get Registry Key Attributes"^^vocabulary:ActionNameVocab .

vocabulary:ObservableObjectRelationshipVocab rdfs:comment "Defines an open-vocabulary of inter-observable object relationships."@en .

_:node1gm7uj6vjx416 rdf:rest _:node1gm7uj6vjx420 .

_:node1gm7uj6vjx806 sh:class observable:CellSite .

tool:creator rdfs:comment "The creator organization for a particular tool."@en .

_:node1gm7uj6vjx807 a rdfs:Datatype .

_:node1gm7uj6vjx418 sh:datatype xsd:dateTime .

_:node1gm7uj6vjx807 owl:onDatatype xsd:string .

_:node1gm7uj6vjx417 rdf:first vocabulary:ActionStatusTypeVocab .

_:node1gm7uj6vjx806 sh:maxCount 1 .

_:node1gm7uj6vjx420 rdf:first "Get Service Status"^^vocabulary:ActionNameVocab .

_:node1gm7uj6vjx806 sh:minCount 1 .

_:node1gm7uj6vjx417 rdf:rest _:node1gm7uj6vjx421 .

_:node1gm7uj6vjx806 sh:nodeKind sh:IRI .

_:node1gm7uj6vjx420 rdf:rest _:node1gm7uj6vjx422 .

_:node1gm7uj6vjx806 sh:path observable:captureCellSite .

tool:creator rdfs:range identity:Identity .

observable:CapturedTelecommunicationsInformationFacet sh:property _:node1gm7uj6vjx806 .

_:node1gm7uj6vjx419 sh:datatype xsd:decimal .

_:node1gm7uj6vjx809 sh:datatype xsd:dateTime .

types:threadSuccessor-subjects-shape sh:targetSubjectsOf types:threadSuccessor .

_:node1gm7uj6vjx809 sh:maxCount 1 .

_:node1gm7uj6vjx421 rdf:first xsd:string .

_:node1gm7uj6vjx809 sh:nodeKind sh:Literal .

_:node1gm7uj6vjx421 rdf:rest rdf:nil .

_:node1gm7uj6vjx809 sh:path observable:endTime .

_:node1gm7uj6vjx415 owl:unionOf _:node1gm7uj6vjx417 .

_:node1gm7uj6vjx808 rdf:first "Allocated"^^vocabulary:ObservableObjectRelationshipVocab .

action:actionStatus rdfs:range _:node1gm7uj6vjx415 .

observable:CapturedTelecommunicationsInformationFacet sh:property _:node1gm7uj6vjx809 .

_:node1gm7uj6vjx418 sh:maxCount 1 .

_:node1gm7uj6vjx808 rdf:rest _:node1gm7uj6vjx810 .

_:node1gm7uj6vjx419 sh:maxCount 1 .

_:node1gm7uj6vjx811 sh:datatype xsd:dateTime .

tool:libraries a owl:ObjectProperty .

_:node1gm7uj6vjx811 sh:maxCount 1 .

_:node1gm7uj6vjx418 sh:nodeKind sh:Literal .

_:node1gm7uj6vjx811 sh:nodeKind sh:Literal .

tool:libraries rdfs:label "libraries"@en .

_:node1gm7uj6vjx811 sh:path observable:startTime .

_:node1gm7uj6vjx422 rdf:first "Get System Global Flags"^^vocabulary:ActionNameVocab .

observable:CapturedTelecommunicationsInformationFacet sh:property _:node1gm7uj6vjx811 .

_:node1gm7uj6vjx422 rdf:rest _:node1gm7uj6vjx423 .

_:node1gm7uj6vjx812 sh:datatype xsd:string .

_:node1gm7uj6vjx419 sh:nodeKind sh:Literal .

_:node1gm7uj6vjx812 sh:maxCount 1 .

action:argumentName a owl:DatatypeProperty .

_:node1gm7uj6vjx812 sh:nodeKind sh:Literal .

_:node1gm7uj6vjx418 sh:path core:objectCreatedTime .

_:node1gm7uj6vjx812 sh:path observable:interceptedCallState .

core:UcoObject sh:property _:node1gm7uj6vjx418 .

observable:CapturedTelecommunicationsInformationFacet sh:property _:node1gm7uj6vjx812 .

types:threadTerminalItem a owl:ObjectProperty .

observable:CapturedTelecommunicationsInformationFacet sh:targetClass observable:CapturedTelecommunicationsInformationFacet .

_:node1gm7uj6vjx423 rdf:first "Get System Host Name"^^vocabulary:ActionNameVocab .

_:node1gm7uj6vjx810 rdf:first "Allocated_By"^^vocabulary:ObservableObjectRelationshipVocab .

_:node1gm7uj6vjx423 rdf:rest _:node1gm7uj6vjx425 .

_:node1gm7uj6vjx810 rdf:rest _:node1gm7uj6vjx813 .

_:node1gm7uj6vjx419 sh:path observable:elevation .

observable:CellSite a owl:Class .

observable:AntennaFacet sh:property _:node1gm7uj6vjx419 .

observable:CellSite a sh:NodeShape .

tool:libraries rdfs:comment "The libraries incorporated into a particular build of a software."@en .

observable:CellSite rdfs:subClassOf observable:ObservableObject .

action:argumentName rdfs:label "argumentName"@en .

_:node1gm7uj6vjx813 rdf:first "Attachment_Of"^^vocabulary:ObservableObjectRelationshipVocab .

_:node1gm7uj6vjx424 sh:datatype xsd:dateTime .

_:node1gm7uj6vjx813 rdf:rest _:node1gm7uj6vjx814 .

_:node1gm7uj6vjx426 sh:datatype xsd:decimal .

observable:CellSite rdfs:label "CellSite"@en .

_:node1gm7uj6vjx425 rdf:first "Get System Local Time"^^vocabulary:ActionNameVocab .

observable:CellSite sh:targetClass observable:CellSite .

_:node1gm7uj6vjx425 rdf:rest _:node1gm7uj6vjx427 .

observable:CellSiteFacet a owl:Class .

types:threadTerminalItem rdfs:subPropertyOf co:item .

_:node1gm7uj6vjx814 rdf:first "Bound"^^vocabulary:ObservableObjectRelationshipVocab .

tool:libraries rdfs:range tool:LibraryType .

observable:CellSiteFacet a sh:NodeShape .

_:node1gm7uj6vjx424 sh:nodeKind sh:Literal .

_:node1gm7uj6vjx814 rdf:rest _:node1gm7uj6vjx815 .

_:node1gm7uj6vjx426 sh:maxCount 1 .

observable:CellSiteFacet rdfs:subClassOf core:Facet .

_:node1gm7uj6vjx426 sh:nodeKind sh:Literal .

observable:CellSiteFacet rdfs:label "CellSiteFacet"@en .

_:node1gm7uj6vjx424 sh:path core:modifiedTime .

_:node1gm7uj6vjx815 rdf:first "Bound_By"^^vocabulary:ObservableObjectRelationshipVocab .

_:node1gm7uj6vjx427 rdf:first "Get System NetBIOS Name"^^vocabulary:ActionNameVocab .

_:node1gm7uj6vjx815 rdf:rest _:node1gm7uj6vjx816 .

core:UcoObject sh:property _:node1gm7uj6vjx424 .

observable:CellSiteFacet rdfs:comment "A cell site facet contains the metadata surrounding the cell site."@en .

_:node1gm7uj6vjx427 rdf:rest _:node1gm7uj6vjx428 .

_:node1gm7uj6vjx817 sh:datatype xsd:string .

action:argumentName rdfs:comment "The identifying label of an argument."@en .

_:node1gm7uj6vjx816 rdf:first "Characterized_By"^^vocabulary:ObservableObjectRelationshipVocab .

types:threadTerminalItem rdfs:label "threadTerminalItem"@en .

_:node1gm7uj6vjx816 rdf:rest _:node1gm7uj6vjx818 .

tool:libraryName a owl:DatatypeProperty .

_:node1gm7uj6vjx817 sh:maxCount 1 .

tool:libraryName rdfs:label "libraryName"@en .

_:node1gm7uj6vjx817 sh:nodeKind sh:Literal .

_:node1gm7uj6vjx429 sh:datatype xsd:string .

_:node1gm7uj6vjx817 sh:path observable:cellSiteCountryCode .

action:argumentName rdfs:range xsd:string .

observable:CellSiteFacet sh:property _:node1gm7uj6vjx817 .

_:node1gm7uj6vjx426 sh:path observable:horizontalBeamWidth .

_:node1gm7uj6vjx819 sh:datatype xsd:string .

observable:AntennaFacet sh:property _:node1gm7uj6vjx426 .

_:node1gm7uj6vjx818 rdf:first "Characterizes"^^vocabulary:ObservableObjectRelationshipVocab .

_:node1gm7uj6vjx428 rdf:first "Get System Network Parameters"^^vocabulary:ActionNameVocab .

_:node1gm7uj6vjx818 rdf:rest _:node1gm7uj6vjx820 .

_:node1gm7uj6vjx428 rdf:rest _:node1gm7uj6vjx431 .

_:node1gm7uj6vjx819 sh:maxCount 1 .

tool:libraryName rdfs:comment "The name of the library."@en .

_:node1gm7uj6vjx820 rdf:first "Child_Of"^^vocabulary:ObservableObjectRelationshipVocab .

types:threadTerminalItem rdfs:comment "A link to an item of the thread known to have no successor."@en .

_:node1gm7uj6vjx820 rdf:rest _:node1gm7uj6vjx821 .

_:node1gm7uj6vjx430 sh:datatype xsd:decimal .

_:node1gm7uj6vjx819 sh:nodeKind sh:Literal .

_:node1gm7uj6vjx429 sh:maxCount 1 .

_:node1gm7uj6vjx819 sh:path observable:cellSiteIdentifier .

_:node1gm7uj6vjx431 rdf:first "Get System Time"^^vocabulary:ActionNameVocab .

observable:CellSiteFacet sh:property _:node1gm7uj6vjx819 .

_:node1gm7uj6vjx431 rdf:rest _:node1gm7uj6vjx432 .

_:node1gm7uj6vjx822 sh:datatype xsd:string .

tool:libraryName rdfs:range xsd:string .

_:node1gm7uj6vjx821 rdf:first "Closed"^^vocabulary:ObservableObjectRelationshipVocab .

types:threadTerminalItem rdfs:domain types:Thread .

_:node1gm7uj6vjx821 rdf:rest _:node1gm7uj6vjx823 .

_:node1gm7uj6vjx430 sh:maxCount 1 .

_:node1gm7uj6vjx822 sh:maxCount 1 .

action:endTime a owl:DatatypeProperty .

_:node1gm7uj6vjx822 sh:nodeKind sh:Literal .

_:node1gm7uj6vjx429 sh:nodeKind sh:Literal .

_:node1gm7uj6vjx822 sh:path observable:cellSiteLocationAreaCode .

_:node1gm7uj6vjx432 rdf:first "Get Thread Context"^^vocabulary:ActionNameVocab .

_:node1gm7uj6vjx823 rdf:first "Closed_By"^^vocabulary:ObservableObjectRelationshipVocab .

_:node1gm7uj6vjx432 rdf:rest _:node1gm7uj6vjx434 .

observable:CellSiteFacet sh:property _:node1gm7uj6vjx822 .

_:node1gm7uj6vjx433 a owl:Class .

_:node1gm7uj6vjx823 rdf:rest _:node1gm7uj6vjx824 .

_:node1gm7uj6vjx429 sh:path core:name .

_:node1gm7uj6vjx825 sh:datatype xsd:string .

core:UcoObject sh:property _:node1gm7uj6vjx429 .

_:node1gm7uj6vjx824 rdf:first "Compressed"^^vocabulary:ObservableObjectRelationshipVocab .

tool:libraryVersion a owl:DatatypeProperty .

_:node1gm7uj6vjx824 rdf:rest _:node1gm7uj6vjx826 .

action:endTime rdfs:label "endTime"@en .

_:node1gm7uj6vjx825 sh:maxCount 1 .

_:node1gm7uj6vjx430 sh:nodeKind sh:Literal .

_:node1gm7uj6vjx825 sh:nodeKind sh:Literal .

_:node1gm7uj6vjx434 rdf:first "Get Thread Username"^^vocabulary:ActionNameVocab .

_:node1gm7uj6vjx825 sh:path observable:cellSiteNetworkCode .

_:node1gm7uj6vjx434 rdf:rest _:node1gm7uj6vjx437 .

observable:CellSiteFacet sh:property _:node1gm7uj6vjx825 .

_:node1gm7uj6vjx435 sh:datatype xsd:string .

_:node1gm7uj6vjx827 sh:datatype xsd:string .

tool:libraryVersion rdfs:label "libraryVersion"@en .

_:node1gm7uj6vjx826 rdf:first "Compressed_By"^^vocabulary:ObservableObjectRelationshipVocab .

_:node1gm7uj6vjx436 rdf:first types:ThreadItem .

_:node1gm7uj6vjx826 rdf:rest _:node1gm7uj6vjx828 .

_:node1gm7uj6vjx436 rdf:rest _:node1gm7uj6vjx438 .

_:node1gm7uj6vjx827 sh:maxCount 1 .

_:node1gm7uj6vjx430 sh:path observable:signalStrength .

_:node1gm7uj6vjx828 rdf:first "Compressed_From"^^vocabulary:ObservableObjectRelationshipVocab .

observable:AntennaFacet sh:property _:node1gm7uj6vjx430 .

_:node1gm7uj6vjx828 rdf:rest _:node1gm7uj6vjx829 .

_:node1gm7uj6vjx435 sh:maxCount 1 .

_:node1gm7uj6vjx827 sh:nodeKind sh:Literal .

tool:libraryVersion rdfs:comment "The version of the library."@en .

_:node1gm7uj6vjx827 sh:path observable:cellSiteType .

_:node1gm7uj6vjx439 a owl:Restriction .

observable:CellSiteFacet sh:property _:node1gm7uj6vjx827 .

_:node1gm7uj6vjx437 rdf:first "Get User Attributes"^^vocabulary:ActionNameVocab .

observable:CellSiteFacet sh:targetClass observable:CellSiteFacet .

_:node1gm7uj6vjx440 sh:datatype xsd:decimal .

_:node1gm7uj6vjx829 rdf:first "Compressed_Into"^^vocabulary:ObservableObjectRelationshipVocab .

_:node1gm7uj6vjx437 rdf:rest _:node1gm7uj6vjx441 .

_:node1gm7uj6vjx829 rdf:rest _:node1gm7uj6vjx830 .

action:endTime rdfs:comment "The time at which performance of the action ended."@en .

observable:CharacterDeviceNode a owl:Class .

_:node1gm7uj6vjx435 sh:nodeKind sh:Literal .

observable:CharacterDeviceNode a sh:NodeShape .

tool:libraryVersion rdfs:range xsd:string .

observable:CharacterDeviceNode rdfs:subClassOf observable:FileSystemObject .

action:endTime rdfs:range xsd:dateTime .

_:node1gm7uj6vjx830 rdf:first "Connected_From"^^vocabulary:ObservableObjectRelationshipVocab .

_:node1gm7uj6vjx440 sh:maxCount 1 .

_:node1gm7uj6vjx830 rdf:rest _:node1gm7uj6vjx831 .

_:node1gm7uj6vjx441 rdf:first "Get Username"^^vocabulary:ActionNameVocab .

observable:CharacterDeviceNode rdfs:label "CharacterDeviceNode"@en .

_:node1gm7uj6vjx441 rdf:rest _:node1gm7uj6vjx442 .

_:node1gm7uj6vjx831 rdf:first "Connected_To"^^vocabulary:ObservableObjectRelationshipVocab .

_:node1gm7uj6vjx435 sh:path core:specVersion .

_:node1gm7uj6vjx831 rdf:rest _:node1gm7uj6vjx832 .

core:UcoObject sh:property _:node1gm7uj6vjx435 .

observable:CharacterDeviceNode rdfs:comment "A character device node is a UNIX filesystem special file that serves as a conduit to communicate with devices, providing only a serial stream of input or accepting a serial stream of output. Character device nodes are used to apply access rights to the devices and to direct operations on the files to the appropriate device drivers. [based on https://en.wikipedia.org/wiki/Unix_file_types]"@en .

_:node1gm7uj6vjx439 owl:onProperty types:threadNextItem .

_:node1gm7uj6vjx832 rdf:first "Contained_Within"^^vocabulary:ObservableObjectRelationshipVocab .

_:node1gm7uj6vjx442 rdf:first "Get Windows Directory"^^vocabulary:ActionNameVocab .

_:node1gm7uj6vjx832 rdf:rest _:node1gm7uj6vjx833 .

_:node1gm7uj6vjx442 rdf:rest _:node1gm7uj6vjx444 .

observable:CharacterDeviceNode sh:targetClass observable:CharacterDeviceNode .

_:node1gm7uj6vjx440 sh:nodeKind sh:Literal .

observable:Code a owl:Class .

_:node1gm7uj6vjx443 sh:datatype xsd:string .

observable:Code a sh:NodeShape .

tool:references a owl:DatatypeProperty .

_:node1gm7uj6vjx833 rdf:first "Contains"^^vocabulary:ObservableObjectRelationshipVocab .

tool:references rdfs:label "references"@en .

observable:Code rdfs:subClassOf observable:ObservableObject .

_:node1gm7uj6vjx440 sh:path observable:skew .

_:node1gm7uj6vjx833 rdf:rest _:node1gm7uj6vjx834 .

observable:AntennaFacet sh:property _:node1gm7uj6vjx440 .

observable:Code rdfs:label "Code"@en .

_:node1gm7uj6vjx443 sh:nodeKind sh:Literal .

_:node1gm7uj6vjx834 rdf:first "Copied"^^vocabulary:ObservableObjectRelationshipVocab .

tool:references rdfs:comment "References to information describing a particular tool."@en .

_:node1gm7uj6vjx834 rdf:rest _:node1gm7uj6vjx835 .

action:environment a owl:ObjectProperty .

observable:Code rdfs:comment "Code is a direct representation (source, byte or binary) of a collection of computer instructions that form software which tell a computer how to work. [based on https://en.wikipedia.org/wiki/Software]"@en .

_:node1gm7uj6vjx444 rdf:first "Get Windows System Directory"^^vocabulary:ActionNameVocab .

observable:Code sh:targetClass observable:Code .

_:node1gm7uj6vjx444 rdf:rest _:node1gm7uj6vjx445 .

observable:CompressedStreamFacet a owl:Class .

_:node1gm7uj6vjx443 sh:path core:description .

observable:CompressedStreamFacet a sh:NodeShape .

_:node1gm7uj6vjx439 owl:cardinality "0"^^xsd:nonNegativeInteger .

_:node1gm7uj6vjx835 rdf:first "Copied_By"^^vocabulary:ObservableObjectRelationshipVocab .

core:UcoObject sh:property _:node1gm7uj6vjx443 .

_:node1gm7uj6vjx835 rdf:rest _:node1gm7uj6vjx836 .

observable:AntennaFacet sh:targetClass observable:AntennaFacet .

observable:CompressedStreamFacet rdfs:subClassOf core:Facet .

_:node1gm7uj6vjx438 rdf:first _:node1gm7uj6vjx439 .

observable:CompressedStreamFacet rdfs:label "CompressedStreamFacet"@en .

_:node1gm7uj6vjx445 rdf:first "Get Windows Temporary Files Directory"^^vocabulary:ActionNameVocab .

_:node1gm7uj6vjx836 rdf:first "Copied_From"^^vocabulary:ObservableObjectRelationshipVocab .

_:node1gm7uj6vjx438 rdf:rest rdf:nil .

_:node1gm7uj6vjx836 rdf:rest _:node1gm7uj6vjx837 .

_:node1gm7uj6vjx445 rdf:rest _:node1gm7uj6vjx447 .

observable:CompressedStreamFacet rdfs:comment "A compressed stream facet is a grouping of characteristics unique to the application of a size-reduction process to a body of data content."@en .

_:node1gm7uj6vjx433 owl:intersectionOf _:node1gm7uj6vjx436 .

_:node1gm7uj6vjx838 sh:datatype xsd:decimal .

types:threadTerminalItem rdfs:range _:node1gm7uj6vjx433 .

_:node1gm7uj6vjx837 rdf:first "Copied_To"^^vocabulary:ObservableObjectRelationshipVocab .

tool:references rdfs:range xsd:anyURI .

_:node1gm7uj6vjx837 rdf:rest _:node1gm7uj6vjx839 .

action:environment rdfs:label "environment"@en .

_:node1gm7uj6vjx838 sh:maxCount 1 .

_:node1gm7uj6vjx446 sh:datatype xsd:string .

_:node1gm7uj6vjx838 sh:nodeKind sh:Literal .

observable:AppleDevice a owl:Class .

_:node1gm7uj6vjx839 rdf:first "Created"^^vocabulary:ObservableObjectRelationshipVocab .

types:threadTerminalItem rdfs:seeAlso co:lastItem .

_:node1gm7uj6vjx839 rdf:rest _:node1gm7uj6vjx840 .

_:node1gm7uj6vjx447 rdf:first "Hide Window"^^vocabulary:ActionNameVocab .

_:node1gm7uj6vjx838 sh:path observable:compressionRatio .

_:node1gm7uj6vjx447 rdf:rest _:node1gm7uj6vjx448 .

observable:CompressedStreamFacet sh:property _:node1gm7uj6vjx838 .

tool:servicePack a owl:DatatypeProperty .

_:node1gm7uj6vjx841 sh:datatype xsd:string .

observable:AppleDevice a sh:NodeShape .

_:node1gm7uj6vjx840 rdf:first "Created_By"^^vocabulary:ObservableObjectRelationshipVocab .

_:node1gm7uj6vjx446 sh:nodeKind sh:Literal .

_:node1gm7uj6vjx840 rdf:rest _:node1gm7uj6vjx842 .

action:environment rdfs:comment "The environment wherein an action occurs."@en .

_:node1gm7uj6vjx841 sh:maxCount 1 .

_:node1gm7uj6vjx446 sh:path core:tag .

_:node1gm7uj6vjx841 sh:nodeKind sh:Literal .

core:UcoObject sh:property _:node1gm7uj6vjx446 .

_:node1gm7uj6vjx841 sh:path observable:compressionMethod .

tool:servicePack rdfs:label "servicePack"@en .

observable:CompressedStreamFacet sh:property _:node1gm7uj6vjx841 .

observable:AppleDevice rdfs:subClassOf observable:Device .

observable:CompressedStreamFacet sh:targetClass observable:CompressedStreamFacet .

action:environment rdfs:range core:UcoObject .

_:node1gm7uj6vjx842 rdf:first "Decoded"^^vocabulary:ObservableObjectRelationshipVocab .

_:node1gm7uj6vjx448 rdf:first "Impersonate Process"^^vocabulary:ActionNameVocab .

_:node1gm7uj6vjx842 rdf:rest _:node1gm7uj6vjx843 .

_:node1gm7uj6vjx448 rdf:rest _:node1gm7uj6vjx449 .

observable:Computer a owl:Class .

core:UcoObject sh:targetClass core:UcoObject .

observable:Computer a sh:NodeShape .

observable:AppleDevice rdfs:label "AppleDevice"@en-us .

_:node1gm7uj6vjx843 rdf:first "Decoded_By"^^vocabulary:ObservableObjectRelationshipVocab .

tool:servicePack rdfs:comment "An appropriate service pack descriptor for a particular tool."@en .

observable:Computer rdfs:subClassOf observable:Device .

types:threadTerminalItem-subjects-shape a sh:PropertyShape .

_:node1gm7uj6vjx843 rdf:rest _:node1gm7uj6vjx844 .

_:node1gm7uj6vjx449 rdf:first "Impersonate Thread"^^vocabulary:ActionNameVocab .

observable:Computer rdfs:label "Computer"@en-us .

_:node1gm7uj6vjx449 rdf:rest _:node1gm7uj6vjx450 .

_:node1gm7uj6vjx844 rdf:first "Decompressed"^^vocabulary:ObservableObjectRelationshipVocab .

core:UcoThing a owl:Class .

_:node1gm7uj6vjx844 rdf:rest _:node1gm7uj6vjx845 .

observable:AppleDevice rdfs:comment "An apple device is a smart device that applies either the MacOS or iOS operating system."@en-us .

_:node1gm7uj6vjx845 rdf:first "Decompressed_By"^^vocabulary:ObservableObjectRelationshipVocab .

action:error a owl:ObjectProperty .

_:node1gm7uj6vjx845 rdf:rest _:node1gm7uj6vjx846 .

tool:servicePack rdfs:range xsd:string .

observable:Computer rdfs:comment "A computer is an electronic device for storing and processing data, typically in binary, according to instructions given to it in a variable program. [based on 'Computer.' Oxford English Dictionary, Oxford University Press, 2022.]"@en-us .

core:UcoThing a sh:NodeShape .

observable:Computer sh:targetClass observable:Computer .

_:node1gm7uj6vjx450 rdf:first "Inject Memory Page"^^vocabulary:ActionNameVocab .

observable:ComputerSpecification a owl:Class .

_:node1gm7uj6vjx450 rdf:rest _:node1gm7uj6vjx451 .

_:node1gm7uj6vjx846 rdf:first "Decrypted"^^vocabulary:ObservableObjectRelationshipVocab .

types:threadTerminalItem-subjects-shape sh:class types:ThreadItem .

_:node1gm7uj6vjx846 rdf:rest _:node1gm7uj6vjx847 .

action:error rdfs:label "error"@en .

observable:ComputerSpecification a sh:NodeShape .

core:UcoThing rdfs:subClassOf owl:Thing .

observable:ComputerSpecification rdfs:subClassOf observable:ObservableObject .

observable:AppleDevice sh:targetClass observable:AppleDevice .

observable:ComputerSpecification rdfs:label "ComputerSpecification"@en .

types:threadTerminalItem-subjects-shape sh:nodeKind sh:IRI .

_:node1gm7uj6vjx847 rdf:first "Decrypted_By"^^vocabulary:ObservableObjectRelationshipVocab .

core:UcoThing rdfs:label "UcoThing"@en .

_:node1gm7uj6vjx847 rdf:rest _:node1gm7uj6vjx848 .

tool:swid a owl:DatatypeProperty .

observable:ComputerSpecification rdfs:comment "A computer specification is the hardware and software of a programmable electronic device that can store, retrieve, and process data. {based on merriam-webster.com/dictionary/computer]"@en .

_:node1gm7uj6vjx451 rdf:first "Kill Process"^^vocabulary:ActionNameVocab .

_:node1gm7uj6vjx848 rdf:first "Deleted"^^vocabulary:ObservableObjectRelationshipVocab .

_:node1gm7uj6vjx451 rdf:rest _:node1gm7uj6vjx452 .

_:node1gm7uj6vjx848 rdf:rest _:node1gm7uj6vjx849 .

tool:swid rdfs:label "swid"@en .

observable:ComputerSpecification sh:targetClass observable:ComputerSpecification .

types:threadTerminalItem-subjects-shape sh:path types:threadTerminalItem .

observable:ComputerSpecificationFacet a owl:Class .

observable:Appliance a owl:Class .

observable:ComputerSpecificationFacet a sh:NodeShape .

_:node1gm7uj6vjx452 rdf:first "Kill Thread"^^vocabulary:ActionNameVocab .

observable:ComputerSpecificationFacet rdfs:subClassOf core:Facet .

_:node1gm7uj6vjx452 rdf:rest _:node1gm7uj6vjx453 .

_:node1gm7uj6vjx849 rdf:first "Deleted_By"^^vocabulary:ObservableObjectRelationshipVocab .

observable:Appliance a sh:NodeShape .

_:node1gm7uj6vjx849 rdf:rest _:node1gm7uj6vjx850 .

action:error rdfs:comment "A characterization of the differences between the expected and the actual performance of the action."@en .

observable:ComputerSpecificationFacet rdfs:label "ComputerSpecificationFacet"@en .

core:UcoThing rdfs:comment "UcoThing is the top-level class within UCO."@en .

_:node1gm7uj6vjx850 rdf:first "Deleted_From"^^vocabulary:ObservableObjectRelationshipVocab .

tool:swid rdfs:comment "Specifies the SWID tag for the software."@en .

observable:ComputerSpecificationFacet rdfs:comment "A computer specificaiton facet is a grouping of characteristics unique to the hardware and software of a programmable electronic device that can store, retrieve, and process data. [based on merriam-webster.com/dictionary/computer]"@en .

observable:Appliance rdfs:subClassOf observable:Device .

_:node1gm7uj6vjx850 rdf:rest _:node1gm7uj6vjx851 .

action:error rdfs:range core:UcoObject .

_:node1gm7uj6vjx852 sh:class observable:ObservableObject .

types:threadTerminalItem-subjects-shape sh:targetSubjectsOf types:threadTerminalItem .

_:node1gm7uj6vjx852 sh:nodeKind sh:IRI .

tool:swid rdfs:range xsd:string .

_:node1gm7uj6vjx852 sh:path observable:networkInterface .

observable:ComputerSpecificationFacet sh:property _:node1gm7uj6vjx852 .

_:node1gm7uj6vjx453 rdf:first "Kill Window"^^vocabulary:ActionNameVocab .

_:node1gm7uj6vjx851 rdf:first "Downloaded"^^vocabulary:ObservableObjectRelationshipVocab .

_:node1gm7uj6vjx453 rdf:rest _:node1gm7uj6vjx454 .

_:node1gm7uj6vjx851 rdf:rest _:node1gm7uj6vjx854 .

observable:Appliance rdfs:label "Appliance"@en .

_:node1gm7uj6vjx853 sh:datatype xsd:dateTime .

core:UcoThing rdfs:seeAlso core:UcoThing-identifier-shape .

_:node1gm7uj6vjx854 rdf:first "Downloaded_By"^^vocabulary:ObservableObjectRelationshipVocab .

_:node1gm7uj6vjx454 rdf:first "Listen on Port"^^vocabulary:ActionNameVocab .

_:node1gm7uj6vjx854 rdf:rest _:node1gm7uj6vjx855 .

_:node1gm7uj6vjx454 rdf:rest _:node1gm7uj6vjx455 .

_:node1gm7uj6vjx853 sh:maxCount 1 .

observable:Appliance rdfs:comment "An appliance is a purpose-built computer with software or firmware that is designed to provide a specific computing capability or resource. [based on https://en.wikipedia.org/wiki/Computer_appliance]"@en .

_:node1gm7uj6vjx853 sh:nodeKind sh:Literal .

tool:toolType a owl:DatatypeProperty .

_:node1gm7uj6vjx853 sh:path observable:biosDate .

_:node1gm7uj6vjx456 a sh:SPARQLConstraint .

observable:ComputerSpecificationFacet sh:property _:node1gm7uj6vjx853 .

observable:Appliance sh:targetClass observable:Appliance .

_:node1gm7uj6vjx856 sh:datatype xsd:dateTime .

_:node1gm7uj6vjx455 rdf:first "Listen on Socket"^^vocabulary:ActionNameVocab .

_:node1gm7uj6vjx855 rdf:first "Downloaded_From"^^vocabulary:ObservableObjectRelationshipVocab .

_:node1gm7uj6vjx455 rdf:rest _:node1gm7uj6vjx457 .

_:node1gm7uj6vjx855 rdf:rest _:node1gm7uj6vjx857 .

tool:toolType rdfs:label "toolType"@en .

_:node1gm7uj6vjx856 sh:maxCount 1 .

tool:toolType rdfs:comment "The type of tool."@en .

_:node1gm7uj6vjx856 sh:nodeKind sh:Literal .

_:node1gm7uj6vjx457 rdf:first "Load Driver"^^vocabulary:ActionNameVocab .

_:node1gm7uj6vjx857 rdf:first "Downloaded_To"^^vocabulary:ObservableObjectRelationshipVocab .

_:node1gm7uj6vjx457 rdf:rest _:node1gm7uj6vjx458 .

_:node1gm7uj6vjx857 rdf:rest _:node1gm7uj6vjx858 .

_:node1gm7uj6vjx456 sh:message "UcoThings are required to not be blank nodes."@en .

_:node1gm7uj6vjx856 sh:path observable:biosReleaseDate .

observable:Application a owl:Class .

observable:ComputerSpecificationFacet sh:property _:node1gm7uj6vjx856 .

tool:toolType rdfs:range xsd:string .

_:node1gm7uj6vjx858 rdf:first "Dropped"^^vocabulary:ObservableObjectRelationshipVocab .

action:estimatedCost a owl:DatatypeProperty .

_:node1gm7uj6vjx858 rdf:rest _:node1gm7uj6vjx860 .

observable:Application a sh:NodeShape .

_:node1gm7uj6vjx859 sh:datatype xsd:dateTime .

_:node1gm7uj6vjx456 sh:select """
			PREFIX uco-core: <https://ontology.unifiedcyberontology.org/uco/core/>
			SELECT $this
			WHERE {
			        $this a/rdfs:subClassOf* uco-core:UcoThing .
			        FILTER isBlank ($this)
			}
		""" .

_:node1gm7uj6vjx859 sh:maxCount 1 .

core:UcoThing sh:sparql _:node1gm7uj6vjx456 .

_:node1gm7uj6vjx860 rdf:first "Dropped_By"^^vocabulary:ObservableObjectRelationshipVocab .

_:node1gm7uj6vjx458 rdf:first "Load Library"^^vocabulary:ActionNameVocab .

_:node1gm7uj6vjx860 rdf:rest _:node1gm7uj6vjx861 .

_:node1gm7uj6vjx458 rdf:rest _:node1gm7uj6vjx459 .

_:node1gm7uj6vjx859 sh:nodeKind sh:Literal .

action:estimatedCost rdfs:label "estimatedCost"@en .

tool:version a owl:DatatypeProperty .

_:node1gm7uj6vjx459 rdf:first "Load Module"^^vocabulary:ActionNameVocab ;
	rdf:rest _:node1gm7uj6vjx460 .

_:node1gm7uj6vjx859 sh:path observable:currentSystemDate .

core:UcoThing sh:targetClass core:UcoThing .

observable:ComputerSpecificationFacet sh:property _:node1gm7uj6vjx859 .

observable:Application rdfs:subClassOf observable:ObservableObject .

_:node1gm7uj6vjx862 sh:datatype xsd:dateTime .

tool:version rdfs:label "version"@en .

_:node1gm7uj6vjx861 rdf:first "Encoded"^^vocabulary:ObservableObjectRelationshipVocab .

_:node1gm7uj6vjx460 rdf:first "Load and Call Driver"^^vocabulary:ActionNameVocab .

_:node1gm7uj6vjx861 rdf:rest _:node1gm7uj6vjx863 .

_:node1gm7uj6vjx460 rdf:rest _:node1gm7uj6vjx461 .

_:node1gm7uj6vjx862 sh:maxCount 1 .

types:threadTerminalItem-subjects-threadNextItem-shape a sh:PropertyShape .

_:node1gm7uj6vjx863 rdf:first "Encoded_By"^^vocabulary:ObservableObjectRelationshipVocab .

observable:Application rdfs:label "Application"@en .

_:node1gm7uj6vjx863 rdf:rest _:node1gm7uj6vjx864 .

_:node1gm7uj6vjx461 rdf:first "Lock File"^^vocabulary:ActionNameVocab .

_:node1gm7uj6vjx862 sh:nodeKind sh:Literal .

_:node1gm7uj6vjx461 rdf:rest _:node1gm7uj6vjx462 .

_:node1gm7uj6vjx862 sh:path observable:localTime .

core:UcoThing-identifier-regex-shape a sh:NodeShape .

observable:ComputerSpecificationFacet sh:property _:node1gm7uj6vjx862 .

action:estimatedCost rdfs:comment "An estimation of the cost if the action is performed."@en .

_:node1gm7uj6vjx865 sh:datatype xsd:dateTime .

tool:version rdfs:comment "An appropriate version descriptor of a particular tool."@en .

_:node1gm7uj6vjx864 rdf:first "Encrypted"^^vocabulary:ObservableObjectRelationshipVocab .

action:estimatedCost rdfs:range xsd:string .

_:node1gm7uj6vjx864 rdf:rest _:node1gm7uj6vjx866 .

_:node1gm7uj6vjx462 rdf:first "Logon as User"^^vocabulary:ActionNameVocab .

_:node1gm7uj6vjx865 sh:maxCount 1 .

_:node1gm7uj6vjx462 rdf:rest _:node1gm7uj6vjx463 .

_:node1gm7uj6vjx865 sh:nodeKind sh:Literal .

tool:version rdfs:range xsd:string .

_:node1gm7uj6vjx865 sh:path observable:systemTime .

types:threadTerminalItem-subjects-threadNextItem-shape sh:description "A terminal item in a thread must not have a next item."@en .

_:node1gm7uj6vjx866 rdf:first "Encrypted_By"^^vocabulary:ObservableObjectRelationshipVocab .

observable:Application rdfs:comment "An application is a particular software program designed for end users."@en .

observable:ComputerSpecificationFacet sh:property _:node1gm7uj6vjx865 .

_:node1gm7uj6vjx463 rdf:first "Map File"^^vocabulary:ActionNameVocab .

_:node1gm7uj6vjx866 rdf:rest _:node1gm7uj6vjx867 .

_:node1gm7uj6vjx463 rdf:rest _:node1gm7uj6vjx464 .

_:node1gm7uj6vjx868 sh:datatype xsd:integer .

types:threadTerminalItem-subjects-threadNextItem-shape sh:maxCount 0 .

_:node1gm7uj6vjx867 rdf:first "Encrypted_From"^^vocabulary:ObservableObjectRelationshipVocab .

action:estimatedEfficacy a owl:DatatypeProperty .

_:node1gm7uj6vjx867 rdf:rest _:node1gm7uj6vjx869 .

core:UcoThing-identifier-regex-shape rdfs:comment "This shape is given an independent IRI for applications that have sufficient controls in place to deactivate this advisory of node identification practice."@en .

_:node1gm7uj6vjx868 sh:maxCount 1 .

types:threadTerminalItem-subjects-threadNextItem-shape sh:nodeKind sh:IRI .

_:node1gm7uj6vjx868 sh:nodeKind sh:Literal .

observable:Application sh:targetClass observable:Application .

_:node1gm7uj6vjx868 sh:path observable:availableRam .

core:UcoThing-identifier-regex-shape rdfs:seeAlso sh:deactivated .

observable:ComputerSpecificationFacet sh:property _:node1gm7uj6vjx868 .

action:estimatedEfficacy rdfs:label "estimatedEfficacy"@en .

_:node1gm7uj6vjx869 rdf:first "Encrypted_To"^^vocabulary:ObservableObjectRelationshipVocab .

_:node1gm7uj6vjx464 rdf:first "Map Library"^^vocabulary:ActionNameVocab .

_:node1gm7uj6vjx870 sh:datatype xsd:integer .

_:node1gm7uj6vjx464 rdf:rest _:node1gm7uj6vjx466 .

_:node1gm7uj6vjx869 rdf:rest _:node1gm7uj6vjx871 .

observable:ApplicationAccount a owl:Class .

_:node1gm7uj6vjx870 sh:maxCount 1 .

core:UcoThing-identifier-regex-shape sh:severity sh:Info .

_:node1gm7uj6vjx871 rdf:first "Extracted_From"^^vocabulary:ObservableObjectRelationshipVocab .

observable:ApplicationAccount a sh:NodeShape .

_:node1gm7uj6vjx871 rdf:rest _:node1gm7uj6vjx872 .

_:node1gm7uj6vjx465 rdf:first types:threadTerminalItem .

_:node1gm7uj6vjx870 sh:nodeKind sh:Literal .

_:node1gm7uj6vjx465 rdf:rest _:node1gm7uj6vjx468 .

_:node1gm7uj6vjx870 sh:path observable:totalRam .

_:node1gm7uj6vjx467 a sh:SPARQLConstraint .

observable:ComputerSpecificationFacet sh:property _:node1gm7uj6vjx870 .

_:node1gm7uj6vjx466 rdf:first "Map View of File"^^vocabulary:ActionNameVocab .

_:node1gm7uj6vjx873 sh:datatype xsd:string .

_:node1gm7uj6vjx466 rdf:rest _:node1gm7uj6vjx469 .

_:node1gm7uj6vjx872 rdf:first "FQDN_Of"^^vocabulary:ObservableObjectRelationshipVocab .

_:node1gm7uj6vjx468 rdf:first types:threadNextItem .

_:node1gm7uj6vjx872 rdf:rest _:node1gm7uj6vjx874 .

_:node1gm7uj6vjx468 rdf:rest rdf:nil .

_:node1gm7uj6vjx873 sh:maxCount 1 .

types:threadTerminalItem-subjects-threadNextItem-shape sh:path _:node1gm7uj6vjx465 .

_:node1gm7uj6vjx873 sh:nodeKind sh:Literal .

observable:ApplicationAccount rdfs:subClassOf observable:DigitalAccount .

_:node1gm7uj6vjx873 sh:path observable:biosManufacturer .

_:node1gm7uj6vjx469 rdf:first "Modify File"^^vocabulary:ActionNameVocab .

observable:ComputerSpecificationFacet sh:property _:node1gm7uj6vjx873 .

_:node1gm7uj6vjx469 rdf:rest _:node1gm7uj6vjx470 .

_:node1gm7uj6vjx874 rdf:first "Freed"^^vocabulary:ObservableObjectRelationshipVocab .

types:threadTerminalItem-subjects-threadNextItem-shape sh:targetSubjectsOf types:threadTerminalItem .

_:node1gm7uj6vjx875 sh:datatype xsd:string .

observable:ApplicationAccount rdfs:label "ApplicationAccount"@en .

_:node1gm7uj6vjx874 rdf:rest _:node1gm7uj6vjx876 .

_:node1gm7uj6vjx467 rdfs:seeAlso <https://datatracker.ietf.org/doc/html/rfc4122#section-4.1.3> .

_:node1gm7uj6vjx875 sh:maxCount 1 .

action:estimatedEfficacy rdfs:comment "An estimation of the effectiveness of the action at achieving its objective if the action is performed."@en .

_:node1gm7uj6vjx875 sh:nodeKind sh:Literal .

_:node1gm7uj6vjx470 rdf:first "Modify Named Pipe"^^vocabulary:ActionNameVocab .

_:node1gm7uj6vjx876 rdf:first "Freed_By"^^vocabulary:ObservableObjectRelationshipVocab .

_:node1gm7uj6vjx470 rdf:rest _:node1gm7uj6vjx471 .

_:node1gm7uj6vjx875 sh:path observable:biosSerialNumber .

action:estimatedEfficacy rdfs:range xsd:string .

observable:ComputerSpecificationFacet sh:property _:node1gm7uj6vjx875 .

types:threadTerminalItem-subjects-threadSuccessor-shape a sh:PropertyShape .

_:node1gm7uj6vjx876 rdf:rest _:node1gm7uj6vjx877 .

_:node1gm7uj6vjx467 sh:message "UcoThings are suggested to end with a UUID."@en .

_:node1gm7uj6vjx878 sh:datatype xsd:string .

_:node1gm7uj6vjx471 rdf:first "Modify Process"^^vocabulary:ActionNameVocab .

_:node1gm7uj6vjx877 rdf:first "Had_Attachment"^^vocabulary:ObservableObjectRelationshipVocab .

_:node1gm7uj6vjx471 rdf:rest _:node1gm7uj6vjx472 .

_:node1gm7uj6vjx877 rdf:rest _:node1gm7uj6vjx879 .

observable:ApplicationAccount rdfs:comment "An application account is an account within a particular software program designed for end users."@en .

_:node1gm7uj6vjx878 sh:maxCount 1 .

action:estimatedImpact a owl:DatatypeProperty .

_:node1gm7uj6vjx878 sh:nodeKind sh:Literal .

_:node1gm7uj6vjx467 sh:select """
			PREFIX uco-core: <https://ontology.unifiedcyberontology.org/uco/core/>
			SELECT $this
			WHERE {
			        $this a/rdfs:subClassOf* uco-core:UcoThing .
			        FILTER (
			                ! REGEX (
			                        STR($this),
			                        \"[0-9a-f]{8}-[0-9a-f]{4}-[0-5][0-9a-f]{3}-[0-9a-f]{4}-[0-9a-f]{12}$\",
			                        \"i\"
			                )
			        )
			}
		""" .

_:node1gm7uj6vjx878 sh:path observable:biosVersion .

core:UcoThing-identifier-regex-shape sh:sparql _:node1gm7uj6vjx467 .

observable:ComputerSpecificationFacet sh:property _:node1gm7uj6vjx878 .

_:node1gm7uj6vjx472 rdf:first "Modify Registry Key"^^vocabulary:ActionNameVocab .

_:node1gm7uj6vjx880 sh:datatype xsd:string .

_:node1gm7uj6vjx472 rdf:rest _:node1gm7uj6vjx473 .

_:node1gm7uj6vjx879 rdf:first "Hooked"^^vocabulary:ObservableObjectRelationshipVocab .

observable:ApplicationAccount sh:targetClass observable:ApplicationAccount .

_:node1gm7uj6vjx879 rdf:rest _:node1gm7uj6vjx881 .

core:UcoThing-identifier-regex-shape sh:targetClass core:UcoThing .

_:node1gm7uj6vjx880 sh:maxCount 1 .

action:estimatedImpact rdfs:label "estimatedImpact"@en .

_:node1gm7uj6vjx880 sh:nodeKind sh:Literal .

types:threadTerminalItem-subjects-threadSuccessor-shape sh:description "A terminal item in a thread must not have a successor."@en .

_:node1gm7uj6vjx881 rdf:first "Hooked_By"^^vocabulary:ObservableObjectRelationshipVocab .

_:node1gm7uj6vjx473 rdf:first "Modify Registry Key Value"^^vocabulary:ActionNameVocab .

_:node1gm7uj6vjx881 rdf:rest _:node1gm7uj6vjx882 .

_:node1gm7uj6vjx473 rdf:rest _:node1gm7uj6vjx474 .

_:node1gm7uj6vjx880 sh:path observable:cpu .

core:confidence a owl:DatatypeProperty .

observable:ComputerSpecificationFacet sh:property _:node1gm7uj6vjx880 .

_:node1gm7uj6vjx474 rdf:first "Modify Service"^^vocabulary:ActionNameVocab .

_:node1gm7uj6vjx883 sh:datatype xsd:string .

_:node1gm7uj6vjx474 rdf:rest _:node1gm7uj6vjx475 .

_:node1gm7uj6vjx883 sh:maxCount 1 .

types:threadTerminalItem-subjects-threadSuccessor-shape sh:maxCount 0 .

_:node1gm7uj6vjx883 sh:nodeKind sh:Literal .

action:estimatedImpact rdfs:comment "An estimation of the impact if the action is performed."@en .

_:node1gm7uj6vjx882 rdf:first "Initialized_By"^^vocabulary:ObservableObjectRelationshipVocab .

observable:ApplicationAccountFacet a owl:Class .

_:node1gm7uj6vjx882 rdf:rest _:node1gm7uj6vjx884 .

core:confidence rdfs:label "confidence"@en .

_:node1gm7uj6vjx883 sh:path observable:cpuFamily .

types:threadTerminalItem-subjects-threadSuccessor-shape sh:nodeKind sh:IRI .

observable:ComputerSpecificationFacet sh:property _:node1gm7uj6vjx883 .

observable:ApplicationAccountFacet a sh:NodeShape .

_:node1gm7uj6vjx885 sh:datatype xsd:string .

action:estimatedImpact rdfs:range xsd:string .

_:node1gm7uj6vjx884 rdf:first "Initialized_To"^^vocabulary:ObservableObjectRelationshipVocab .

_:node1gm7uj6vjx475 rdf:first "Monitor Registry Key"^^vocabulary:ActionNameVocab .

_:node1gm7uj6vjx884 rdf:rest _:node1gm7uj6vjx886 .

_:node1gm7uj6vjx475 rdf:rest _:node1gm7uj6vjx476 .

_:node1gm7uj6vjx885 sh:maxCount 1 .

observable:ApplicationAccountFacet rdfs:subClassOf core:Facet .

_:node1gm7uj6vjx885 sh:nodeKind sh:Literal .

_:node1gm7uj6vjx477 rdf:first types:threadTerminalItem .

_:node1gm7uj6vjx885 sh:path observable:gpu .

_:node1gm7uj6vjx477 rdf:rest _:node1gm7uj6vjx478 .

observable:ComputerSpecificationFacet sh:property _:node1gm7uj6vjx885 .

core:confidence rdfs:comment "An asserted level of certainty in the accuracy of some information."@en .

_:node1gm7uj6vjx887 sh:datatype xsd:string .

_:node1gm7uj6vjx476 rdf:first "Move File"^^vocabulary:ActionNameVocab .

_:node1gm7uj6vjx886 rdf:first "Injected"^^vocabulary:ObservableObjectRelationshipVocab .

_:node1gm7uj6vjx476 rdf:rest _:node1gm7uj6vjx479 .

_:node1gm7uj6vjx886 rdf:rest _:node1gm7uj6vjx888 .

observable:ApplicationAccountFacet rdfs:label "ApplicationAccountFacet"@en .

_:node1gm7uj6vjx887 sh:maxCount 1 .

_:node1gm7uj6vjx478 rdf:first types:threadSuccessor .

_:node1gm7uj6vjx888 rdf:first "Injected_As"^^vocabulary:ObservableObjectRelationshipVocab .

_:node1gm7uj6vjx478 rdf:rest rdf:nil .

_:node1gm7uj6vjx888 rdf:rest _:node1gm7uj6vjx889 .

types:threadTerminalItem-subjects-threadSuccessor-shape sh:path _:node1gm7uj6vjx477 .

_:node1gm7uj6vjx887 sh:nodeKind sh:Literal .

action:instrument a owl:ObjectProperty .

_:node1gm7uj6vjx887 sh:path observable:gpuFamily .

_:node1gm7uj6vjx480 a rdfs:Datatype .

observable:ComputerSpecificationFacet sh:property _:node1gm7uj6vjx887 .

_:node1gm7uj6vjx479 rdf:first "Open File"^^vocabulary:ActionNameVocab .

_:node1gm7uj6vjx890 sh:datatype xsd:string .

_:node1gm7uj6vjx479 rdf:rest _:node1gm7uj6vjx481 .

_:node1gm7uj6vjx889 rdf:first "Injected_By"^^vocabulary:ObservableObjectRelationshipVocab .

action:instrument rdfs:label "instrument"@en .

_:node1gm7uj6vjx889 rdf:rest _:node1gm7uj6vjx891 .

types:threadTerminalItem-subjects-threadSuccessor-shape sh:targetSubjectsOf types:threadTerminalItem .

_:node1gm7uj6vjx890 sh:maxCount 1 .

_:node1gm7uj6vjx480 owl:onDatatype xsd:nonNegativeInteger .

_:node1gm7uj6vjx890 sh:nodeKind sh:Literal .

_:node1gm7uj6vjx481 rdf:first "Open File Mapping"^^vocabulary:ActionNameVocab .

_:node1gm7uj6vjx890 sh:path observable:hostname .

_:node1gm7uj6vjx481 rdf:rest _:node1gm7uj6vjx484 .

observable:ComputerSpecificationFacet sh:property _:node1gm7uj6vjx890 .

types:value a owl:DatatypeProperty .

_:node1gm7uj6vjx891 rdf:first "Injected_Into"^^vocabulary:ObservableObjectRelationshipVocab .

action:instrument rdfs:comment "The things used to perform an action."@en .

_:node1gm7uj6vjx891 rdf:rest _:node1gm7uj6vjx893 .

types:value rdfs:label "value"@en .

_:node1gm7uj6vjx892 sh:datatype xsd:string .

_:node1gm7uj6vjx484 rdf:first "Open Mutex"^^vocabulary:ActionNameVocab .

_:node1gm7uj6vjx892 sh:maxCount 1 .

_:node1gm7uj6vjx484 rdf:rest _:node1gm7uj6vjx485 .

_:node1gm7uj6vjx893 rdf:first "Installed"^^vocabulary:ObservableObjectRelationshipVocab .

observable:ApplicationAccountFacet rdfs:comment "An application account facet is a grouping of characteristics unique to an account within a particular software program designed for end users."@en .

_:node1gm7uj6vjx893 rdf:rest _:node1gm7uj6vjx894 .

_:node1gm7uj6vjx483 xsd:maxInclusive "100"^^xsd:nonNegativeInteger .

_:node1gm7uj6vjx892 sh:nodeKind sh:Literal .

_:node1gm7uj6vjx482 rdf:first _:node1gm7uj6vjx483 .

_:node1gm7uj6vjx892 sh:path observable:processorArchitecture .

_:node1gm7uj6vjx482 rdf:rest rdf:nil .

observable:ComputerSpecificationFacet sh:property _:node1gm7uj6vjx892 .

_:node1gm7uj6vjx480 owl:withRestrictions _:node1gm7uj6vjx482 .

_:node1gm7uj6vjx895 sh:datatype xsd:string .

_:node1gm7uj6vjx485 rdf:first "Open Port"^^vocabulary:ActionNameVocab .

_:node1gm7uj6vjx894 rdf:first "Installed_By"^^vocabulary:ObservableObjectRelationshipVocab .

core:confidence rdfs:range _:node1gm7uj6vjx480 .

_:node1gm7uj6vjx894 rdf:rest _:node1gm7uj6vjx896 .

_:node1gm7uj6vjx485 rdf:rest _:node1gm7uj6vjx486 .

_:node1gm7uj6vjx895 sh:maxCount 1 .

action:instrument rdfs:range core:UcoObject .

_:node1gm7uj6vjx895 sh:nodeKind sh:Literal .

types:value rdfs:comment "A specific property value."@en .

_:node1gm7uj6vjx895 sh:path observable:timezoneDST .

types:value rdfs:range xsd:string .

observable:ComputerSpecificationFacet sh:property _:node1gm7uj6vjx895 .

_:node1gm7uj6vjx487 sh:class observable:ObservableObject .

_:node1gm7uj6vjx897 sh:datatype xsd:string .

_:node1gm7uj6vjx486 rdf:first "Open Process"^^vocabulary:ActionNameVocab .

_:node1gm7uj6vjx896 rdf:first "Joined"^^vocabulary:ObservableObjectRelationshipVocab .

_:node1gm7uj6vjx486 rdf:rest _:node1gm7uj6vjx488 .

_:node1gm7uj6vjx896 rdf:rest _:node1gm7uj6vjx898 .

action:location a owl:ObjectProperty .

_:node1gm7uj6vjx897 sh:maxCount 1 .

core:constrainingVocabularyName a owl:DatatypeProperty .

_:node1gm7uj6vjx897 sh:nodeKind sh:Literal .

_:node1gm7uj6vjx488 rdf:first "Open Registry Key"^^vocabulary:ActionNameVocab .

_:node1gm7uj6vjx898 rdf:first "Joined_By"^^vocabulary:ObservableObjectRelationshipVocab .

_:node1gm7uj6vjx487 sh:maxCount 1 .

_:node1gm7uj6vjx898 rdf:rest _:node1gm7uj6vjx899 .

_:node1gm7uj6vjx488 rdf:rest _:node1gm7uj6vjx489 .

_:node1gm7uj6vjx897 sh:path observable:timezoneStandard .

_:node1gm7uj6vjx487 sh:nodeKind sh:IRI .

observable:ComputerSpecificationFacet sh:property _:node1gm7uj6vjx897 .

action:location rdfs:label "location"@en .

_:node1gm7uj6vjx900 sh:datatype xsd:string .

_:node1gm7uj6vjx487 sh:path observable:application .

_:node1gm7uj6vjx899 rdf:first "Killed"^^vocabulary:ObservableObjectRelationshipVocab .

core:constrainingVocabularyName rdfs:label "constrainingVocabularyName"@en .

_:node1gm7uj6vjx899 rdf:rest _:node1gm7uj6vjx901 .

_:node1gm7uj6vjx489 rdf:first "Open Service"^^vocabulary:ActionNameVocab .

_:node1gm7uj6vjx900 sh:maxCount 1 .

observable:ApplicationAccountFacet sh:property _:node1gm7uj6vjx487 .

_:node1gm7uj6vjx900 sh:nodeKind sh:Literal .

_:node1gm7uj6vjx489 rdf:rest _:node1gm7uj6vjx490 .

_:node1gm7uj6vjx900 sh:path observable:uptime .

core:constrainingVocabularyName rdfs:comment "The name of an explicitly constrained set of string values."@en .

observable:ComputerSpecificationFacet sh:property _:node1gm7uj6vjx900 .

_:node1gm7uj6vjx490 rdf:first "Open Service Control Manager"^^vocabulary:ActionNameVocab .

observable:ComputerSpecificationFacet sh:targetClass observable:ComputerSpecificationFacet .

_:node1gm7uj6vjx490 rdf:rest _:node1gm7uj6vjx491 .

_:node1gm7uj6vjx901 rdf:first "Killed_By"^^vocabulary:ObservableObjectRelationshipVocab .

core:constrainingVocabularyName rdfs:range xsd:string .

_:node1gm7uj6vjx901 rdf:rest _:node1gm7uj6vjx902 .

observable:ApplicationAccountFacet sh:targetClass observable:ApplicationAccountFacet .

observable:ConfiguredSoftware a owl:Class .

action:location rdfs:comment "The locations where an action occurs."@en .

observable:ConfiguredSoftware a sh:NodeShape .

_:node1gm7uj6vjx491 rdf:first "Protect Virtual Memory"^^vocabulary:ActionNameVocab .

observable:ConfiguredSoftware rdfs:subClassOf observable:Software .

_:node1gm7uj6vjx491 rdf:rest _:node1gm7uj6vjx492 .

_:node1gm7uj6vjx902 rdf:first "Listened_On"^^vocabulary:ObservableObjectRelationshipVocab .

observable:ApplicationFacet a owl:Class .

_:node1gm7uj6vjx902 rdf:rest _:node1gm7uj6vjx903 .

core:constrainingVocabularyReference a owl:DatatypeProperty .

observable:ConfiguredSoftware rdfs:label "ConfiguredSoftware"@en .

observable:ApplicationFacet a sh:NodeShape .

_:node1gm7uj6vjx903 rdf:first "Listened_On_By"^^vocabulary:ObservableObjectRelationshipVocab .

action:location rdfs:range location:Location .

_:node1gm7uj6vjx903 rdf:rest _:node1gm7uj6vjx904 .

_:node1gm7uj6vjx492 rdf:first "Query DNS"^^vocabulary:ActionNameVocab .

observable:ConfiguredSoftware rdfs:comment "A ConfiguredSoftware is a Software that is known to be configured to run in a more specified manner than some unconfigured or less-configured Software."@en .

_:node1gm7uj6vjx492 rdf:rest _:node1gm7uj6vjx493 .

_:node1gm7uj6vjx905 sh:class configuration:Configuration .

observable:ApplicationFacet rdfs:subClassOf core:Facet .

_:node1gm7uj6vjx904 rdf:first "Loaded_From"^^vocabulary:ObservableObjectRelationshipVocab .

core:constrainingVocabularyReference rdfs:label "constrainingVocabularyReference"@en .

_:node1gm7uj6vjx904 rdf:rest _:node1gm7uj6vjx906 .

observable:ApplicationFacet rdfs:label "ApplicationFacet"@en .

_:node1gm7uj6vjx905 sh:maxCount 1 .

_:node1gm7uj6vjx493 rdf:first "Query Disk Attributes"^^vocabulary:ActionNameVocab .

_:node1gm7uj6vjx905 sh:nodeKind sh:IRI .

_:node1gm7uj6vjx493 rdf:rest _:node1gm7uj6vjx494 .

_:node1gm7uj6vjx906 rdf:first "Loaded_Into"^^vocabulary:ObservableObjectRelationshipVocab .

action:object a owl:ObjectProperty .

_:node1gm7uj6vjx906 rdf:rest _:node1gm7uj6vjx907 .

_:node1gm7uj6vjx494 rdf:first "Query Process Virtual Memory"^^vocabulary:ActionNameVocab .

_:node1gm7uj6vjx905 sh:path configuration:usesConfiguration .

_:node1gm7uj6vjx494 rdf:rest _:node1gm7uj6vjx495 .

observable:ConfiguredSoftware sh:property _:node1gm7uj6vjx905 .

action:object rdfs:label "object"@en .

_:node1gm7uj6vjx908 sh:class observable:Software .

_:node1gm7uj6vjx495 rdf:first "Queue APC in Thread"^^vocabulary:ActionNameVocab .

_:node1gm7uj6vjx907 rdf:first "Locked"^^vocabulary:ObservableObjectRelationshipVocab .

_:node1gm7uj6vjx495 rdf:rest _:node1gm7uj6vjx496 .

_:node1gm7uj6vjx907 rdf:rest _:node1gm7uj6vjx909 .

observable:ApplicationFacet rdfs:comment "An application facet is a grouping of characteristics unique to a particular software program designed for end users."@en .

_:node1gm7uj6vjx908 sh:maxCount 1 .

_:node1gm7uj6vjx496 rdf:first "Read File"^^vocabulary:ActionNameVocab .

_:node1gm7uj6vjx908 sh:nodeKind sh:IRI .

_:node1gm7uj6vjx496 rdf:rest _:node1gm7uj6vjx498 .

_:node1gm7uj6vjx908 sh:path configuration:isConfigurationOf .

_:node1gm7uj6vjx497 sh:class observable:ApplicationVersion .

observable:ConfiguredSoftware sh:property _:node1gm7uj6vjx908 .

action:object rdfs:comment "The things that the action is performed on/against."@en .

_:node1gm7uj6vjx909 rdf:first "Locked_By"^^vocabulary:ObservableObjectRelationshipVocab .

core:constrainingVocabularyReference rdfs:comment "A reference to a specification for an explicitly constrained set of string values. The specification may be unstructured (e.g., web page listing string values) or structured (e.g. RDF/OWL enumeration)."@en .

observable:ConfiguredSoftware sh:targetClass observable:ConfiguredSoftware .

_:node1gm7uj6vjx497 sh:nodeKind sh:IRI .

_:node1gm7uj6vjx909 rdf:rest _:node1gm7uj6vjx910 .

_:node1gm7uj6vjx498 rdf:first "Read From Named Pipe"^^vocabulary:ActionNameVocab .

observable:Contact a owl:Class .

_:node1gm7uj6vjx498 rdf:rest _:node1gm7uj6vjx499 .

observable:Contact a sh:NodeShape .

_:node1gm7uj6vjx497 sh:path observable:installedVersionHistory .

observable:Contact rdfs:subClassOf observable:ObservableObject .

_:node1gm7uj6vjx499 rdf:first "Read From Process Memory"^^vocabulary:ActionNameVocab .

_:node1gm7uj6vjx910 rdf:first "Mapped_By"^^vocabulary:ObservableObjectRelationshipVocab .

observable:ApplicationFacet sh:property _:node1gm7uj6vjx497 .

observable:Contact rdfs:label "Contact"@en .

_:node1gm7uj6vjx499 rdf:rest _:node1gm7uj6vjx500 .

_:node1gm7uj6vjx910 rdf:rest _:node1gm7uj6vjx911 .

core:constrainingVocabularyReference rdfs:range xsd:anyURI .

observable:Contact rdfs:comment "A contact is a set of identification and communication related details for a single entity."@en .

action:object rdfs:range core:UcoObject .

observable:Contact sh:targetClass observable:Contact .

_:node1gm7uj6vjx501 sh:class observable:ObservableObject .

_:node1gm7uj6vjx911 rdf:first "Mapped_Into"^^vocabulary:ObservableObjectRelationshipVocab .

_:node1gm7uj6vjx500 rdf:first "Read Registry Key Value"^^vocabulary:ActionNameVocab .

_:node1gm7uj6vjx911 rdf:rest _:node1gm7uj6vjx912 .

_:node1gm7uj6vjx500 rdf:rest _:node1gm7uj6vjx502 .

observable:ContactAddress a owl:Class .

core:context a owl:DatatypeProperty .

observable:ContactAddress a sh:NodeShape .

_:node1gm7uj6vjx502 rdf:first "Receive Data on Socket"^^vocabulary:ActionNameVocab .

observable:ContactAddress rdfs:subClassOf core:UcoInherentCharacterizationThing .

_:node1gm7uj6vjx502 rdf:rest _:node1gm7uj6vjx503 .

_:node1gm7uj6vjx912 rdf:first "Merged"^^vocabulary:ObservableObjectRelationshipVocab .

core:context rdfs:label "context"@en .

_:node1gm7uj6vjx912 rdf:rest _:node1gm7uj6vjx913 .

_:node1gm7uj6vjx501 sh:maxCount 1 .

observable:ContactAddress rdfs:label "ContactAddress"@en .

_:node1gm7uj6vjx503 rdf:first "Receive Email Message"^^vocabulary:ActionNameVocab .

observable:ContactAddress rdfs:comment "A contact address is a grouping of characteristics unique to a geolocation address of a contact entity."@en .

_:node1gm7uj6vjx503 rdf:rest _:node1gm7uj6vjx504 .

_:node1gm7uj6vjx913 rdf:first "Merged_By"^^vocabulary:ObservableObjectRelationshipVocab .

core:context rdfs:comment "A description of particular contextual affinity."@en .

_:node1gm7uj6vjx913 rdf:rest _:node1gm7uj6vjx914 .

_:node1gm7uj6vjx501 sh:nodeKind sh:IRI .

_:node1gm7uj6vjx915 sh:class location:Location .

action:objective a owl:DatatypeProperty .

_:node1gm7uj6vjx915 sh:maxCount 1 .

core:context rdfs:range xsd:string .

_:node1gm7uj6vjx914 rdf:first "Modified_Properties_Of"^^vocabulary:ObservableObjectRelationshipVocab .

_:node1gm7uj6vjx501 sh:path observable:operatingSystem .

_:node1gm7uj6vjx914 rdf:rest _:node1gm7uj6vjx916 .

observable:ApplicationFacet sh:property _:node1gm7uj6vjx501 .

_:node1gm7uj6vjx915 sh:nodeKind sh:IRI .

_:node1gm7uj6vjx504 rdf:first "Release Mutex"^^vocabulary:ActionNameVocab .

_:node1gm7uj6vjx915 sh:path observable:geolocationAddress .

_:node1gm7uj6vjx504 rdf:rest _:node1gm7uj6vjx506 .

observable:ContactAddress sh:property _:node1gm7uj6vjx915 .

_:node1gm7uj6vjx506 rdf:first "Rename File"^^vocabulary:ActionNameVocab .

_:node1gm7uj6vjx917 sh:datatype vocabulary:ContactAddressScopeVocab .

_:node1gm7uj6vjx506 rdf:rest _:node1gm7uj6vjx507 .

_:node1gm7uj6vjx917 sh:message "Value is outside the default vocabulary ContactAddressScopeVocab." .

_:node1gm7uj6vjx505 sh:datatype xsd:integer .

_:node1gm7uj6vjx916 rdf:first "Monitored"^^vocabulary:ObservableObjectRelationshipVocab .

core:createdBy a owl:ObjectProperty .

_:node1gm7uj6vjx916 rdf:rest _:node1gm7uj6vjx918 .

action:objective rdfs:label "objective"@en .

_:node1gm7uj6vjx917 sh:path observable:contactAddressScope .

_:node1gm7uj6vjx505 sh:maxCount 1 .

_:node1gm7uj6vjx917 sh:severity sh:Info .

core:createdBy rdfs:label "createdBy"@en .

observable:ContactAddress sh:property _:node1gm7uj6vjx917 .

_:node1gm7uj6vjx507 rdf:first "Revert Thread to Self"^^vocabulary:ActionNameVocab .

_:node1gm7uj6vjx918 rdf:first "Monitored_By"^^vocabulary:ObservableObjectRelationshipVocab .

_:node1gm7uj6vjx507 rdf:rest _:node1gm7uj6vjx508 .

_:node1gm7uj6vjx918 rdf:rest _:node1gm7uj6vjx920 .

_:node1gm7uj6vjx505 sh:nodeKind sh:Literal .

_:node1gm7uj6vjx919 sh:maxCount 1 .

_:node1gm7uj6vjx508 rdf:first "Send Control Code to File"^^vocabulary:ActionNameVocab .

_:node1gm7uj6vjx919 sh:nodeKind sh:Literal .

_:node1gm7uj6vjx508 rdf:rest _:node1gm7uj6vjx509 .

_:node1gm7uj6vjx922 sh:datatype vocabulary:ContactAddressScopeVocab .

_:node1gm7uj6vjx505 sh:path observable:numberOfLaunches .

_:node1gm7uj6vjx921 rdf:first _:node1gm7uj6vjx922 .

observable:ApplicationFacet sh:property _:node1gm7uj6vjx505 .

_:node1gm7uj6vjx920 rdf:first "Moved"^^vocabulary:ObservableObjectRelationshipVocab .

_:node1gm7uj6vjx510 sh:datatype xsd:string .

_:node1gm7uj6vjx921 rdf:rest _:node1gm7uj6vjx923 .

_:node1gm7uj6vjx509 rdf:first "Send Control Code to Pipe"^^vocabulary:ActionNameVocab .

_:node1gm7uj6vjx920 rdf:rest _:node1gm7uj6vjx924 .

_:node1gm7uj6vjx509 rdf:rest _:node1gm7uj6vjx511 .

_:node1gm7uj6vjx925 sh:datatype xsd:string .

_:node1gm7uj6vjx510 sh:maxCount 1 .

_:node1gm7uj6vjx923 rdf:first _:node1gm7uj6vjx925 .

_:node1gm7uj6vjx510 sh:nodeKind sh:Literal .

_:node1gm7uj6vjx923 rdf:rest rdf:nil .

core:createdBy rdfs:comment "The identity that created a characterization of a concept."@en .

_:node1gm7uj6vjx919 sh:or _:node1gm7uj6vjx921 .

_:node1gm7uj6vjx511 rdf:first "Send Control Code to Service"^^vocabulary:ActionNameVocab .

_:node1gm7uj6vjx919 sh:path observable:contactAddressScope .

action:objective rdfs:comment "The intended purpose for performing the action."@en .

observable:ContactAddress sh:property _:node1gm7uj6vjx919 .

_:node1gm7uj6vjx511 rdf:rest _:node1gm7uj6vjx512 .

_:node1gm7uj6vjx926 sh:message "Value is not member of the vocabulary ContactAddressScopeVocab." .

_:node1gm7uj6vjx510 sh:path observable:applicationIdentifier .

_:node1gm7uj6vjx924 rdf:first "Moved_By"^^vocabulary:ObservableObjectRelationshipVocab .

observable:ApplicationFacet sh:property _:node1gm7uj6vjx510 .

_:node1gm7uj6vjx924 rdf:rest _:node1gm7uj6vjx929 .

core:createdBy rdfs:range core:IdentityAbstraction .

_:node1gm7uj6vjx928 sh:datatype vocabulary:ContactAddressScopeVocab .

_:node1gm7uj6vjx512 rdf:first "Send DNS Query"^^vocabulary:ActionNameVocab .

_:node1gm7uj6vjx929 rdf:first "Moved_From"^^vocabulary:ObservableObjectRelationshipVocab .

_:node1gm7uj6vjx512 rdf:rest _:node1gm7uj6vjx514 .

_:node1gm7uj6vjx929 rdf:rest _:node1gm7uj6vjx931 .

action:objective rdfs:range xsd:string .

_:node1gm7uj6vjx930 rdf:first "home"^^vocabulary:ContactAddressScopeVocab .

_:node1gm7uj6vjx513 sh:datatype xsd:string .

_:node1gm7uj6vjx930 rdf:rest _:node1gm7uj6vjx932 .

_:node1gm7uj6vjx514 rdf:first "Send Data on Socket"^^vocabulary:ActionNameVocab .

_:node1gm7uj6vjx931 rdf:first "Moved_To"^^vocabulary:ObservableObjectRelationshipVocab .

_:node1gm7uj6vjx514 rdf:rest _:node1gm7uj6vjx515 .

_:node1gm7uj6vjx931 rdf:rest _:node1gm7uj6vjx933 .

core:definingContext a owl:DatatypeProperty .

_:node1gm7uj6vjx932 rdf:first "work"^^vocabulary:ContactAddressScopeVocab .

_:node1gm7uj6vjx513 sh:maxCount 1 .

_:node1gm7uj6vjx932 rdf:rest _:node1gm7uj6vjx934 .

core:definingContext rdfs:label "definingContext"@en .

_:node1gm7uj6vjx933 rdf:first "Opened"^^vocabulary:ObservableObjectRelationshipVocab .

_:node1gm7uj6vjx513 sh:nodeKind sh:Literal .

_:node1gm7uj6vjx933 rdf:rest _:node1gm7uj6vjx935 .

_:node1gm7uj6vjx515 rdf:first "Send Data to Address on Socket"^^vocabulary:ActionNameVocab .

_:node1gm7uj6vjx934 rdf:first "school"^^vocabulary:ContactAddressScopeVocab .

_:node1gm7uj6vjx515 rdf:rest _:node1gm7uj6vjx516 .

_:node1gm7uj6vjx934 rdf:rest rdf:nil .

action:participant a owl:ObjectProperty .

_:node1gm7uj6vjx928 sh:in _:node1gm7uj6vjx930 .

_:node1gm7uj6vjx513 sh:path observable:version .

_:node1gm7uj6vjx927 rdf:first _:node1gm7uj6vjx928 .

observable:ApplicationFacet sh:property _:node1gm7uj6vjx513 .

_:node1gm7uj6vjx927 rdf:rest _:node1gm7uj6vjx936 .

_:node1gm7uj6vjx516 rdf:first "Send Email Message"^^vocabulary:ActionNameVocab .

_:node1gm7uj6vjx937 sh:datatype xsd:string .

_:node1gm7uj6vjx516 rdf:rest _:node1gm7uj6vjx517 .

_:node1gm7uj6vjx936 rdf:first _:node1gm7uj6vjx937 .

core:definingContext rdfs:comment "A description of the context relevant to the definition of a particular external reference identifier."@en .

_:node1gm7uj6vjx936 rdf:rest rdf:nil .

_:node1gm7uj6vjx517 rdf:first "Send ICMP Request"^^vocabulary:ActionNameVocab .

_:node1gm7uj6vjx926 sh:or _:node1gm7uj6vjx927 .

_:node1gm7uj6vjx517 rdf:rest _:node1gm7uj6vjx518 .

_:node1gm7uj6vjx926 sh:path observable:contactAddressScope .

core:definingContext rdfs:range xsd:string .

observable:ContactAddress sh:property _:node1gm7uj6vjx926 .

observable:ApplicationFacet sh:targetClass observable:ApplicationFacet .

_:node1gm7uj6vjx935 rdf:first "Opened_By"^^vocabulary:ObservableObjectRelationshipVocab .

action:participant rdfs:label "participant"@en .

_:node1gm7uj6vjx935 rdf:rest _:node1gm7uj6vjx938 .

_:node1gm7uj6vjx518 rdf:first "Send Reverse DNS Query"^^vocabulary:ActionNameVocab .

observable:ContactAddress sh:targetClass observable:ContactAddress .

_:node1gm7uj6vjx518 rdf:rest _:node1gm7uj6vjx519 .

observable:ContactAffiliation a owl:Class .

core:description a owl:DatatypeProperty .

observable:ContactAffiliation a sh:NodeShape .

observable:ApplicationVersion a owl:Class .

_:node1gm7uj6vjx938 rdf:first "Packed"^^vocabulary:ObservableObjectRelationshipVocab .

_:node1gm7uj6vjx519 rdf:first "Set File Attributes"^^vocabulary:ActionNameVocab .

observable:ContactAffiliation rdfs:subClassOf core:UcoInherentCharacterizationThing .

_:node1gm7uj6vjx519 rdf:rest _:node1gm7uj6vjx520 .

_:node1gm7uj6vjx938 rdf:rest _:node1gm7uj6vjx939 .

observable:ApplicationVersion a sh:NodeShape .

observable:ContactAffiliation rdfs:label "ContactListAffiliation"@en .

core:description rdfs:label "description"@en .

observable:ContactAffiliation rdfs:comment "A contact affiliation is a grouping of characteristics unique to details of an organizational affiliation for a single contact entity."@en .

observable:ApplicationVersion rdfs:subClassOf core:UcoInherentCharacterizationThing .

_:node1gm7uj6vjx939 rdf:first "Packed_By"^^vocabulary:ObservableObjectRelationshipVocab .

action:participant rdfs:comment "The supporting (non-primary) performers of an action."@en .

_:node1gm7uj6vjx939 rdf:rest _:node1gm7uj6vjx941 .

_:node1gm7uj6vjx520 rdf:first "Set NetBIOS Name"^^vocabulary:ActionNameVocab .

_:node1gm7uj6vjx940 sh:class identity:Organization .

_:node1gm7uj6vjx520 rdf:rest _:node1gm7uj6vjx521 .

_:node1gm7uj6vjx940 sh:maxCount 1 .

core:description rdfs:comment "A description of a particular concept characterization."@en .

_:node1gm7uj6vjx941 rdf:first "Packed_From"^^vocabulary:ObservableObjectRelationshipVocab .

observable:ApplicationVersion rdfs:label "ApplicationVersion"@en .

_:node1gm7uj6vjx941 rdf:rest _:node1gm7uj6vjx942 .

core:description rdfs:range xsd:string .

_:node1gm7uj6vjx940 sh:nodeKind sh:IRI .

observable:ApplicationVersion rdfs:comment "An application version is a grouping of characteristics unique to a particular software program version."@en .

_:node1gm7uj6vjx940 sh:path observable:contactOrganization .

action:participant rdfs:range core:UcoObject .

observable:ContactAffiliation sh:property _:node1gm7uj6vjx940 .

_:node1gm7uj6vjx521 rdf:first "Set Process Current Directory"^^vocabulary:ActionNameVocab .

_:node1gm7uj6vjx943 sh:class observable:ContactAddress .

_:node1gm7uj6vjx521 rdf:rest _:node1gm7uj6vjx523 .

_:node1gm7uj6vjx942 rdf:first "Packed_Into"^^vocabulary:ObservableObjectRelationshipVocab .

core:endTime a owl:DatatypeProperty .

_:node1gm7uj6vjx942 rdf:rest _:node1gm7uj6vjx944 .

_:node1gm7uj6vjx522 sh:datatype xsd:dateTime .

_:node1gm7uj6vjx943 sh:minCount 0 .

core:endTime rdfs:label "endTime"@en .

_:node1gm7uj6vjx943 sh:nodeKind sh:IRI .

_:node1gm7uj6vjx523 rdf:first "Set Process Environment Variable"^^vocabulary:ActionNameVocab .

_:node1gm7uj6vjx943 sh:path observable:organizationLocation .

_:node1gm7uj6vjx523 rdf:rest _:node1gm7uj6vjx524 .

observable:ContactAffiliation sh:property _:node1gm7uj6vjx943 .

_:node1gm7uj6vjx522 sh:maxCount 1 .

_:node1gm7uj6vjx945 sh:class observable:ContactEmail .

core:endTime rdfs:comment "The ending time of a time range."@en .

_:node1gm7uj6vjx944 rdf:first "Parent_Of"^^vocabulary:ObservableObjectRelationshipVocab .

core:endTime rdfs:range xsd:dateTime .

_:node1gm7uj6vjx944 rdf:rest _:node1gm7uj6vjx946 .

_:node1gm7uj6vjx524 rdf:first "Set System Global Flags"^^vocabulary:ActionNameVocab .

_:node1gm7uj6vjx945 sh:minCount 0 .

_:node1gm7uj6vjx522 sh:nodeKind sh:Literal .

_:node1gm7uj6vjx945 sh:nodeKind sh:IRI .

action:performer a owl:ObjectProperty .

_:node1gm7uj6vjx946 rdf:first "Paused"^^vocabulary:ObservableObjectRelationshipVocab .

_:node1gm7uj6vjx524 rdf:rest _:node1gm7uj6vjx525 .

_:node1gm7uj6vjx946 rdf:rest _:node1gm7uj6vjx947 .

_:node1gm7uj6vjx522 sh:path observable:installDate .

_:node1gm7uj6vjx945 sh:path observable:contactEmail .

observable:ApplicationVersion sh:property _:node1gm7uj6vjx522 .

observable:ContactAffiliation sh:property _:node1gm7uj6vjx945 .

_:node1gm7uj6vjx525 rdf:first "Set System Host Name"^^vocabulary:ActionNameVocab .

_:node1gm7uj6vjx948 sh:class observable:ContactMessaging .

_:node1gm7uj6vjx525 rdf:rest _:node1gm7uj6vjx527 .

_:node1gm7uj6vjx947 rdf:first "Paused_By"^^vocabulary:ObservableObjectRelationshipVocab .

_:node1gm7uj6vjx526 sh:datatype xsd:dateTime .

_:node1gm7uj6vjx947 rdf:rest _:node1gm7uj6vjx949 .

action:performer rdfs:label "performer"@en .

_:node1gm7uj6vjx948 sh:minCount 0 .

core:externalIdentifier a owl:DatatypeProperty .

_:node1gm7uj6vjx948 sh:nodeKind sh:IRI .

_:node1gm7uj6vjx527 rdf:first "Set System Time"^^vocabulary:ActionNameVocab .

_:node1gm7uj6vjx949 rdf:first "Previously_Contained"^^vocabulary:ObservableObjectRelationshipVocab .

_:node1gm7uj6vjx527 rdf:rest _:node1gm7uj6vjx528 .

_:node1gm7uj6vjx948 sh:path observable:contactMessaging .

_:node1gm7uj6vjx526 sh:maxCount 1 .

_:node1gm7uj6vjx949 rdf:rest _:node1gm7uj6vjx950 .

core:externalIdentifier rdfs:label "externalIdentifier"@en .

observable:ContactAffiliation sh:property _:node1gm7uj6vjx948 .

_:node1gm7uj6vjx526 sh:nodeKind sh:Literal .

_:node1gm7uj6vjx951 sh:class observable:ContactPhone .

_:node1gm7uj6vjx528 rdf:first "Set Thread Context"^^vocabulary:ActionNameVocab .

_:node1gm7uj6vjx950 rdf:first "Properties_Modified_By"^^vocabulary:ObservableObjectRelationshipVocab .

_:node1gm7uj6vjx528 rdf:rest _:node1gm7uj6vjx529 .

_:node1gm7uj6vjx951 sh:minCount 0 .

_:node1gm7uj6vjx526 sh:path observable:uninstallDate .

_:node1gm7uj6vjx950 rdf:rest _:node1gm7uj6vjx952 .

observable:ApplicationVersion sh:property _:node1gm7uj6vjx526 .

_:node1gm7uj6vjx951 sh:nodeKind sh:IRI .

_:node1gm7uj6vjx529 rdf:first "Show Window"^^vocabulary:ActionNameVocab .

_:node1gm7uj6vjx951 sh:path observable:contactPhone .

_:node1gm7uj6vjx529 rdf:rest _:node1gm7uj6vjx531 .

observable:ContactAffiliation sh:property _:node1gm7uj6vjx951 .

_:node1gm7uj6vjx530 sh:datatype xsd:string .

_:node1gm7uj6vjx953 sh:class observable:ContactProfile .

action:performer rdfs:comment "The primary performer of an action."@en .

_:node1gm7uj6vjx952 rdf:first "Properties_Queried"^^vocabulary:ObservableObjectRelationshipVocab .

core:externalIdentifier rdfs:comment "An identifier for some information defined external to the UCO context."@en .

_:node1gm7uj6vjx952 rdf:rest _:node1gm7uj6vjx954 .

_:node1gm7uj6vjx530 sh:maxCount 1 .

_:node1gm7uj6vjx953 sh:minCount 0 .

_:node1gm7uj6vjx531 rdf:first "Shutdown System"^^vocabulary:ActionNameVocab .

_:node1gm7uj6vjx953 sh:nodeKind sh:IRI .

_:node1gm7uj6vjx531 rdf:rest _:node1gm7uj6vjx532 .

_:node1gm7uj6vjx954 rdf:first "Properties_Queried_By"^^vocabulary:ObservableObjectRelationshipVocab .

_:node1gm7uj6vjx530 sh:nodeKind sh:Literal .

_:node1gm7uj6vjx954 rdf:rest _:node1gm7uj6vjx955 .

core:externalIdentifier rdfs:range xsd:string .

_:node1gm7uj6vjx953 sh:path observable:contactProfile .

action:performer rdfs:range core:UcoObject .

observable:ContactAffiliation sh:property _:node1gm7uj6vjx953 .

_:node1gm7uj6vjx532 rdf:first "Sleep Process"^^vocabulary:ActionNameVocab .

_:node1gm7uj6vjx956 sh:class observable:ContactURL .

_:node1gm7uj6vjx532 rdf:rest _:node1gm7uj6vjx533 .

_:node1gm7uj6vjx955 rdf:first "Read_From"^^vocabulary:ObservableObjectRelationshipVocab .

_:node1gm7uj6vjx530 sh:path observable:version .

_:node1gm7uj6vjx955 rdf:rest _:node1gm7uj6vjx957 .

observable:ApplicationVersion sh:property _:node1gm7uj6vjx530 .

_:node1gm7uj6vjx956 sh:minCount 0 .

core:externalReference a owl:ObjectProperty .

_:node1gm7uj6vjx956 sh:nodeKind sh:IRI .

_:node1gm7uj6vjx533 rdf:first "Sleep System"^^vocabulary:ActionNameVocab .

_:node1gm7uj6vjx957 rdf:first "Read_From_By"^^vocabulary:ObservableObjectRelationshipVocab .

_:node1gm7uj6vjx533 rdf:rest _:node1gm7uj6vjx534 .

_:node1gm7uj6vjx957 rdf:rest _:node1gm7uj6vjx958 .

observable:ApplicationVersion sh:targetClass observable:ApplicationVersion .

_:node1gm7uj6vjx956 sh:path observable:contactURL .

core:externalReference rdfs:label "External Reference"@en-us .

observable:ContactAffiliation sh:property _:node1gm7uj6vjx956 .

action:phase a owl:ObjectProperty .

_:node1gm7uj6vjx959 sh:datatype xsd:string .

_:node1gm7uj6vjx534 rdf:first "Start Service"^^vocabulary:ActionNameVocab .

_:node1gm7uj6vjx958 rdf:first "Received"^^vocabulary:ObservableObjectRelationshipVocab .

_:node1gm7uj6vjx534 rdf:rest _:node1gm7uj6vjx535 .

_:node1gm7uj6vjx958 rdf:rest _:node1gm7uj6vjx960 .

observable:ArchiveFile a owl:Class .

_:node1gm7uj6vjx959 sh:maxCount 1 .

observable:ArchiveFile a sh:NodeShape .

_:node1gm7uj6vjx960 rdf:first "Received_By"^^vocabulary:ObservableObjectRelationshipVocab .

core:externalReference rdfs:comment "Specifies a reference to a resource outside of the UCO."@en-us .

_:node1gm7uj6vjx960 rdf:rest _:node1gm7uj6vjx961 .

action:phase rdfs:subPropertyOf action:subaction .

_:node1gm7uj6vjx959 sh:nodeKind sh:Literal .

_:node1gm7uj6vjx535 rdf:first "Unload Driver"^^vocabulary:ActionNameVocab .

_:node1gm7uj6vjx959 sh:path observable:organizationDepartment .

_:node1gm7uj6vjx535 rdf:rest _:node1gm7uj6vjx536 .

observable:ContactAffiliation sh:property _:node1gm7uj6vjx959 .

observable:ArchiveFile rdfs:subClassOf observable:File .

_:node1gm7uj6vjx961 rdf:first "Received_From"^^vocabulary:ObservableObjectRelationshipVocab .

core:externalReference rdfs:range core:ExternalReference .

_:node1gm7uj6vjx961 rdf:rest _:node1gm7uj6vjx963 .

_:node1gm7uj6vjx536 rdf:first "Unload Module"^^vocabulary:ActionNameVocab .

_:node1gm7uj6vjx962 sh:datatype xsd:string .

core:hasFacet a owl:ObjectProperty .

_:node1gm7uj6vjx963 rdf:first "Received_Via_Upload"^^vocabulary:ObservableObjectRelationshipVocab .

_:node1gm7uj6vjx536 rdf:rest _:node1gm7uj6vjx537 .

_:node1gm7uj6vjx963 rdf:rest _:node1gm7uj6vjx964 .

observable:ArchiveFile rdfs:label "ArchiveFile"@en .

_:node1gm7uj6vjx962 sh:maxCount 1 .

action:phase rdfs:label "phase"@en .

_:node1gm7uj6vjx962 sh:nodeKind sh:Literal .

core:hasFacet a owl:InverseFunctionalProperty .

_:node1gm7uj6vjx964 rdf:first "Redirects_To"^^vocabulary:ObservableObjectRelationshipVocab .

_:node1gm7uj6vjx537 rdf:first "Unlock File"^^vocabulary:ActionNameVocab .

_:node1gm7uj6vjx962 sh:path observable:organizationPosition .

_:node1gm7uj6vjx537 rdf:rest _:node1gm7uj6vjx538 .

_:node1gm7uj6vjx964 rdf:rest _:node1gm7uj6vjx965 .

core:hasFacet rdfs:label "hasFacet"@en .

observable:ContactAffiliation sh:property _:node1gm7uj6vjx962 .

_:node1gm7uj6vjx538 rdf:first "Unmap File"^^vocabulary:ActionNameVocab .

observable:ContactAffiliation sh:targetClass observable:ContactAffiliation .

_:node1gm7uj6vjx538 rdf:rest _:node1gm7uj6vjx539 .

_:node1gm7uj6vjx965 rdf:first "Related_To"^^vocabulary:ObservableObjectRelationshipVocab .

_:node1gm7uj6vjx539 rdf:first "Upload File"^^vocabulary:ActionNameVocab .

_:node1gm7uj6vjx965 rdf:rest _:node1gm7uj6vjx966 .

_:node1gm7uj6vjx539 rdf:rest _:node1gm7uj6vjx540 .

observable:ContactEmail a owl:Class .

observable:ArchiveFile rdfs:comment "An archive file is a file that is composed of one or more computer files along with metadata."@en .

observable:ContactEmail a sh:NodeShape .

_:node1gm7uj6vjx540 rdf:first "Write to File"^^vocabulary:ActionNameVocab .

_:node1gm7uj6vjx966 rdf:first "Renamed"^^vocabulary:ObservableObjectRelationshipVocab .

_:node1gm7uj6vjx540 rdf:rest _:node1gm7uj6vjx541 .

_:node1gm7uj6vjx966 rdf:rest _:node1gm7uj6vjx967 .

observable:ArchiveFile sh:targetClass observable:ArchiveFile .

observable:ContactEmail rdfs:subClassOf core:UcoInherentCharacterizationThing .

action:phase rdfs:comment "The ordered set of actions or sub action-lifecycles that represent the action lifecycle."@en .

observable:ContactEmail rdfs:label "ContactEmail"@en .

core:hasFacet rdfs:comment "Further sets of properties characterizing a concept based on the particular context of the class and of the particular instance of the concept being characterized."@en .

_:node1gm7uj6vjx967 rdf:first "Renamed_By"^^vocabulary:ObservableObjectRelationshipVocab .

_:node1gm7uj6vjx541 rdf:first "Write to Process Virtual Memory"^^vocabulary:ActionNameVocab .

_:node1gm7uj6vjx967 rdf:rest _:node1gm7uj6vjx968 .

_:node1gm7uj6vjx541 rdf:rest rdf:nil .

observable:ContactEmail rdfs:comment "A contact email is a grouping of characteristics unique to details for contacting a contact entity by email."@en .

_:node1gm7uj6vjx227 owl:oneOf _:node1gm7uj6vjx229 .

_:node1gm7uj6vjx969 sh:class observable:ObservableObject .

vocabulary:ActionNameVocab owl:equivalentClass _:node1gm7uj6vjx227 .

_:node1gm7uj6vjx968 rdf:first "Renamed_From"^^vocabulary:ObservableObjectRelationshipVocab .

observable:ArchiveFileFacet a owl:Class .

_:node1gm7uj6vjx968 rdf:rest _:node1gm7uj6vjx970 .

action:phase rdfs:range action:ArrayOfAction .

_:node1gm7uj6vjx969 sh:maxCount 1 .

core:hasFacet rdfs:range core:Facet .

_:node1gm7uj6vjx970 rdf:first "Renamed_To"^^vocabulary:ObservableObjectRelationshipVocab .

observable:ArchiveFileFacet a sh:NodeShape .

_:node1gm7uj6vjx969 sh:nodeKind sh:IRI .

observable:ArchiveFileFacet rdfs:subClassOf core:Facet .

_:node1gm7uj6vjx970 rdf:rest _:node1gm7uj6vjx971 .

vocabulary:ActionRelationshipTypeVocab a rdfs:Datatype .

_:node1gm7uj6vjx969 sh:path observable:emailAddress .

observable:ArchiveFileFacet rdfs:label "ArchiveFileFacet"@en .

observable:ContactEmail sh:property _:node1gm7uj6vjx969 .

core:hasFacet-shape a sh:PropertyShape .

_:node1gm7uj6vjx972 sh:datatype vocabulary:ContactEmailScopeVocab .

observable:ArchiveFileFacet rdfs:comment "An archive file facet is a grouping of characteristics unique to a file that is composed of one or more computer files along with metadata."@en .

_:node1gm7uj6vjx972 sh:message "Value is outside the default vocabulary ContactEmailScopeVocab." .

vocabulary:ActionRelationshipTypeVocab rdfs:label "Action Relationship Type Vocabulary"@en-us .

_:node1gm7uj6vjx971 rdf:first "Resolved_To"^^vocabulary:ObservableObjectRelationshipVocab .

core:hasFacet-shape sh:path core:hasFacet .

_:node1gm7uj6vjx972 sh:path observable:contactEmailScope .

action:rate a owl:DatatypeProperty .

_:node1gm7uj6vjx971 rdf:rest _:node1gm7uj6vjx973 .

_:node1gm7uj6vjx542 sh:datatype xsd:string .

_:node1gm7uj6vjx972 sh:severity sh:Info .

_:node1gm7uj6vjx543 a sh:SPARQLConstraint .

observable:ContactEmail sh:property _:node1gm7uj6vjx972 .

_:node1gm7uj6vjx542 sh:maxCount 1 .

_:node1gm7uj6vjx974 sh:maxCount 1 .

vocabulary:ActionRelationshipTypeVocab rdfs:comment "Defines an open-vocabulary for capturing types of relationships between actions."@en-us .

_:node1gm7uj6vjx973 rdf:first "Resumed"^^vocabulary:ObservableObjectRelationshipVocab .

_:node1gm7uj6vjx542 sh:nodeKind sh:Literal .

_:node1gm7uj6vjx973 rdf:rest _:node1gm7uj6vjx975 .

_:node1gm7uj6vjx542 sh:path observable:archiveType .

_:node1gm7uj6vjx974 sh:nodeKind sh:Literal .

_:node1gm7uj6vjx543 sh:message "hasFacet must not be used to link two objects to one Facet."@en .

_:node1gm7uj6vjx977 sh:datatype vocabulary:ContactEmailScopeVocab .

observable:ArchiveFileFacet sh:property _:node1gm7uj6vjx542 .

_:node1gm7uj6vjx976 rdf:first _:node1gm7uj6vjx977 .

_:node1gm7uj6vjx544 a rdfs:Datatype .

_:node1gm7uj6vjx976 rdf:rest _:node1gm7uj6vjx978 .

action:rate rdfs:label "rate"@en .

_:node1gm7uj6vjx975 rdf:first "Resumed_By"^^vocabulary:ObservableObjectRelationshipVocab .

_:node1gm7uj6vjx545 sh:datatype xsd:string .

_:node1gm7uj6vjx975 rdf:rest _:node1gm7uj6vjx980 .

_:node1gm7uj6vjx544 owl:onDatatype xsd:string .

_:node1gm7uj6vjx979 sh:datatype xsd:string .

_:node1gm7uj6vjx978 rdf:first _:node1gm7uj6vjx979 ;
	rdf:rest rdf:nil .

_:node1gm7uj6vjx545 sh:maxCount 1 .

_:node1gm7uj6vjx974 sh:or _:node1gm7uj6vjx976 .

_:node1gm7uj6vjx543 sh:select """
			PREFIX core: <https://ontology.unifiedcyberontology.org/uco/core/>
			PREFIX owl: <http://www.w3.org/2002/07/owl#>
			SELECT $this ?value
			WHERE {
				?value core:hasFacet $this .
				?nOtherValue core:hasFacet $this .
				FILTER ( ?value != ?nOtherValue )
				FILTER NOT EXISTS {
					?value owl:sameAs|^owl:sameAs ?nOtherValue .
				}
			}
			""" .

_:node1gm7uj6vjx974 sh:path observable:contactEmailScope .

core:hasFacet-shape sh:sparql _:node1gm7uj6vjx543 .

observable:ContactEmail sh:property _:node1gm7uj6vjx974 .

_:node1gm7uj6vjx545 sh:nodeKind sh:Literal .

_:node1gm7uj6vjx981 sh:message "Value is not member of the vocabulary ContactEmailScopeVocab." .

core:hasFacet-shape sh:targetObjectsOf core:hasFacet .

_:node1gm7uj6vjx980 rdf:first "Root_Domain_Of"^^vocabulary:ObservableObjectRelationshipVocab .

_:node1gm7uj6vjx545 sh:path observable:comment .

_:node1gm7uj6vjx980 rdf:rest _:node1gm7uj6vjx984 .

observable:ArchiveFileFacet sh:property _:node1gm7uj6vjx545 .

_:node1gm7uj6vjx983 sh:datatype vocabulary:ContactEmailScopeVocab .

_:node1gm7uj6vjx547 sh:datatype xsd:string .

_:node1gm7uj6vjx984 rdf:first "Searched_For"^^vocabulary:ObservableObjectRelationshipVocab .

_:node1gm7uj6vjx546 rdf:first "Dependent_On"^^vocabulary:ActionRelationshipTypeVocab .

_:node1gm7uj6vjx984 rdf:rest _:node1gm7uj6vjx986 .

_:node1gm7uj6vjx546 rdf:rest _:node1gm7uj6vjx548 .

_:node1gm7uj6vjx985 rdf:first "home"^^vocabulary:ContactEmailScopeVocab .

action:rate rdfs:comment "The frequency rate for the occurence of an action."@en .

_:node1gm7uj6vjx985 rdf:rest _:node1gm7uj6vjx987 .

core:isDirectional a owl:DatatypeProperty .

_:node1gm7uj6vjx986 rdf:first "Searched_For_By"^^vocabulary:ObservableObjectRelationshipVocab .

_:node1gm7uj6vjx547 sh:maxCount 1 .

_:node1gm7uj6vjx986 rdf:rest _:node1gm7uj6vjx988 .

_:node1gm7uj6vjx548 rdf:first "Equivalent_To"^^vocabulary:ActionRelationshipTypeVocab .

_:node1gm7uj6vjx987 rdf:first "work"^^vocabulary:ContactEmailScopeVocab .

_:node1gm7uj6vjx548 rdf:rest _:node1gm7uj6vjx549 .

_:node1gm7uj6vjx987 rdf:rest _:node1gm7uj6vjx989 .

core:isDirectional rdfs:label "isDirectional"@en .

_:node1gm7uj6vjx988 rdf:first "Sent"^^vocabulary:ObservableObjectRelationshipVocab .

_:node1gm7uj6vjx547 sh:nodeKind sh:Literal .

_:node1gm7uj6vjx988 rdf:rest _:node1gm7uj6vjx990 .

action:rate rdfs:range xsd:decimal .

_:node1gm7uj6vjx989 rdf:first "school"^^vocabulary:ContactEmailScopeVocab .

_:node1gm7uj6vjx547 sh:path observable:version .

_:node1gm7uj6vjx989 rdf:rest _:node1gm7uj6vjx991 .

_:node1gm7uj6vjx549 rdf:first "Followed_By"^^vocabulary:ActionRelationshipTypeVocab .

_:node1gm7uj6vjx990 rdf:first "Sent_By"^^vocabulary:ObservableObjectRelationshipVocab .

_:node1gm7uj6vjx549 rdf:rest _:node1gm7uj6vjx550 .

_:node1gm7uj6vjx990 rdf:rest _:node1gm7uj6vjx992 .

observable:ArchiveFileFacet sh:property _:node1gm7uj6vjx547 .

_:node1gm7uj6vjx991 rdf:first "cloud"^^vocabulary:ContactEmailScopeVocab .

core:isDirectional rdfs:comment "A specification whether or not a relationship assertion is limited to the context FROM a source object(s) TO a target object."@en .

_:node1gm7uj6vjx991 rdf:rest rdf:nil .

_:node1gm7uj6vjx550 rdf:first "Initiated"^^vocabulary:ActionRelationshipTypeVocab .

_:node1gm7uj6vjx983 sh:in _:node1gm7uj6vjx985 .

_:node1gm7uj6vjx550 rdf:rest _:node1gm7uj6vjx551 .

_:node1gm7uj6vjx982 rdf:first _:node1gm7uj6vjx983 .

core:isDirectional rdfs:range xsd:boolean .

_:node1gm7uj6vjx982 rdf:rest _:node1gm7uj6vjx993 .

observable:ArchiveFileFacet sh:targetClass observable:ArchiveFileFacet .

_:node1gm7uj6vjx994 sh:datatype xsd:string .

_:node1gm7uj6vjx551 rdf:first "Initiated_By"^^vocabulary:ActionRelationshipTypeVocab .

_:node1gm7uj6vjx993 rdf:first _:node1gm7uj6vjx994 .

_:node1gm7uj6vjx551 rdf:rest _:node1gm7uj6vjx552 .

_:node1gm7uj6vjx993 rdf:rest rdf:nil .

action:result a owl:ObjectProperty .

_:node1gm7uj6vjx981 sh:or _:node1gm7uj6vjx982 .

_:node1gm7uj6vjx552 rdf:first "Preceded_By"^^vocabulary:ActionRelationshipTypeVocab .

_:node1gm7uj6vjx981 sh:path observable:contactEmailScope .

observable:Audio a owl:Class .

_:node1gm7uj6vjx992 rdf:first "Sent_To"^^vocabulary:ObservableObjectRelationshipVocab .

core:kindOfRelationship a owl:DatatypeProperty .

observable:ContactEmail sh:property _:node1gm7uj6vjx981 .

_:node1gm7uj6vjx552 rdf:rest _:node1gm7uj6vjx553 .

_:node1gm7uj6vjx992 rdf:rest _:node1gm7uj6vjx995 .

observable:Audio a sh:NodeShape .

observable:ContactEmail sh:targetClass observable:ContactEmail .

observable:Audio rdfs:subClassOf observable:ObservableObject .

observable:ContactFacet a owl:Class .

_:node1gm7uj6vjx553 rdf:first "Related_To"^^vocabulary:ActionRelationshipTypeVocab .

observable:ContactFacet a sh:NodeShape .

_:node1gm7uj6vjx553 rdf:rest rdf:nil .

observable:ContactFacet rdfs:subClassOf core:Facet .

_:node1gm7uj6vjx544 owl:oneOf _:node1gm7uj6vjx546 .

_:node1gm7uj6vjx995 rdf:first "Sent_Via_Upload"^^vocabulary:ObservableObjectRelationshipVocab .

vocabulary:ActionRelationshipTypeVocab owl:equivalentClass _:node1gm7uj6vjx544 .

_:node1gm7uj6vjx995 rdf:rest _:node1gm7uj6vjx996 .

action:result rdfs:label "result"@en .

observable:ContactFacet rdfs:label "ContactFacet"@en .

core:kindOfRelationship rdfs:label "kindOfRelationship"@en .

_:node1gm7uj6vjx996 rdf:first "Set_From"^^vocabulary:ObservableObjectRelationshipVocab .

observable:Audio rdfs:label "Audio"@en .

_:node1gm7uj6vjx996 rdf:rest _:node1gm7uj6vjx997 .

action:result rdfs:comment "The things resulting from performing an action."@en .

observable:ContactFacet rdfs:comment "A contact facet is a grouping of characteristics unique to a set of identification and communication related details for a single entity."@en .

vocabulary:ActionStatusTypeVocab a rdfs:Datatype .

_:node1gm7uj6vjx998 sh:class observable:ContactAddress .

action:result rdfs:range core:UcoObject .

_:node1gm7uj6vjx997 rdf:first "Set_To"^^vocabulary:ObservableObjectRelationshipVocab .

core:kindOfRelationship rdfs:comment "A characterization of the nature of a relationship between objects."@en .

_:node1gm7uj6vjx997 rdf:rest _:node1gm7uj6vjx999 .

observable:Audio rdfs:comment "Audio is a digital representation of sound."@en .

_:node1gm7uj6vjx998 sh:minCount 0 .

core:kindOfRelationship rdfs:range xsd:string .

_:node1gm7uj6vjx998 sh:nodeKind sh:IRI .

vocabulary:ActionStatusTypeVocab rdfs:label "Action Status Type Vocabulary"@en-us .

_:node1gm7uj6vjx999 rdf:first "Sub-domain_Of"^^vocabulary:ObservableObjectRelationshipVocab .

observable:Audio sh:targetClass observable:Audio .

_:node1gm7uj6vjx999 rdf:rest _:node1gm7uj6vjx1000 .

vocabulary:ActionStatusTypeVocab rdfs:comment "Defines an open-vocabulary of action status types."@en-us .

_:node1gm7uj6vjx998 sh:path observable:contactAddress .

action:scale a owl:DatatypeProperty .

observable:ContactFacet sh:property _:node1gm7uj6vjx998 .

observable:AudioFacet a owl:Class .

_:node1gm7uj6vjx1001 sh:class observable:ContactAffiliation .

_:node1gm7uj6vjx554 a rdfs:Datatype .

_:node1gm7uj6vjx1000 rdf:first "Supra-domain_Of"^^vocabulary:ObservableObjectRelationshipVocab .

core:modifiedTime a owl:DatatypeProperty .

_:node1gm7uj6vjx1000 rdf:rest _:node1gm7uj6vjx1002 .

observable:AudioFacet a sh:NodeShape .

_:node1gm7uj6vjx1001 sh:minCount 0 .

action:scale rdfs:label "scale"@en .

_:node1gm7uj6vjx1001 sh:nodeKind sh:IRI .

_:node1gm7uj6vjx554 owl:onDatatype xsd:string .

_:node1gm7uj6vjx1002 rdf:first "Suspended"^^vocabulary:ObservableObjectRelationshipVocab .

core:modifiedTime rdfs:label "modifiedTime"@en .

_:node1gm7uj6vjx1002 rdf:rest _:node1gm7uj6vjx1003 .

observable:AudioFacet rdfs:subClassOf core:Facet .

_:node1gm7uj6vjx1001 sh:path observable:contactAffiliation .

observable:AudioFacet rdfs:label "AudioFacet"@en .

observable:ContactFacet sh:property _:node1gm7uj6vjx1001 .

_:node1gm7uj6vjx555 rdf:first "Complete/Finish"^^vocabulary:ActionStatusTypeVocab .

_:node1gm7uj6vjx1004 sh:class observable:ContactEmail .

_:node1gm7uj6vjx555 rdf:rest _:node1gm7uj6vjx556 .

_:node1gm7uj6vjx1003 rdf:first "Suspended_By"^^vocabulary:ObservableObjectRelationshipVocab .

_:node1gm7uj6vjx556 rdf:first "Error"^^vocabulary:ActionStatusTypeVocab .

_:node1gm7uj6vjx1004 sh:minCount 0 .

_:node1gm7uj6vjx556 rdf:rest _:node1gm7uj6vjx557 .

_:node1gm7uj6vjx1003 rdf:rest _:node1gm7uj6vjx1005 .

action:scale rdfs:comment "The time scale utilized for the frequency rate count for the occurence of an action."@en .

_:node1gm7uj6vjx1004 sh:nodeKind sh:IRI .

action:scale rdfs:range xsd:string .

_:node1gm7uj6vjx1004 sh:path observable:contactEmail .

_:node1gm7uj6vjx557 rdf:first "Fail"^^vocabulary:ActionStatusTypeVocab .

observable:ContactFacet sh:property _:node1gm7uj6vjx1004 .

_:node1gm7uj6vjx557 rdf:rest _:node1gm7uj6vjx558 .

_:node1gm7uj6vjx1006 sh:class observable:ContactMessaging .

observable:AudioFacet rdfs:comment "An audio facet is a grouping of characteristics unique to a digital representation of sound."@en .

_:node1gm7uj6vjx1005 rdf:first "Unhooked"^^vocabulary:ObservableObjectRelationshipVocab .

_:node1gm7uj6vjx558 rdf:first "Ongoing"^^vocabulary:ActionStatusTypeVocab .

_:node1gm7uj6vjx1005 rdf:rest _:node1gm7uj6vjx1007 .

_:node1gm7uj6vjx558 rdf:rest _:node1gm7uj6vjx560 .

_:node1gm7uj6vjx1006 sh:minCount 0 .

action:startTime a owl:DatatypeProperty .

_:node1gm7uj6vjx1006 sh:nodeKind sh:IRI .

_:node1gm7uj6vjx559 sh:datatype xsd:integer .

_:node1gm7uj6vjx1006 sh:path observable:contactMessaging .

_:node1gm7uj6vjx560 rdf:first "Pending"^^vocabulary:ActionStatusTypeVocab .

observable:ContactFacet sh:property _:node1gm7uj6vjx1006 .

_:node1gm7uj6vjx560 rdf:rest _:node1gm7uj6vjx561 .

_:node1gm7uj6vjx1007 rdf:first "Unhooked_By"^^vocabulary:ObservableObjectRelationshipVocab .

_:node1gm7uj6vjx559 sh:maxCount 1 .

_:node1gm7uj6vjx1007 rdf:rest _:node1gm7uj6vjx1009 .

action:startTime rdfs:label "startTime"@en .

_:node1gm7uj6vjx1008 sh:class observable:ContactPhone .

_:node1gm7uj6vjx559 sh:nodeKind sh:Literal .

_:node1gm7uj6vjx1009 rdf:first "Unlocked"^^vocabulary:ObservableObjectRelationshipVocab .

core:modifiedTime rdfs:comment "Specifies the time that this particular version of the object was modified. The object creator can use the time it deems most appropriate as the time this version of the object was modified. The value of the modified property for a given object version MUST be later than or equal to the value of the created property. Object creators MUST update the modified property when creating a new version of an object. The modified timestamp MUST be precise to the nearest millisecond (exactly three digits after the decimal place in seconds)."@en-us .

_:node1gm7uj6vjx1008 sh:minCount 0 .

_:node1gm7uj6vjx561 rdf:first "Success"^^vocabulary:ActionStatusTypeVocab .

_:node1gm7uj6vjx1009 rdf:rest _:node1gm7uj6vjx1010 .

_:node1gm7uj6vjx561 rdf:rest _:node1gm7uj6vjx562 .

_:node1gm7uj6vjx1008 sh:nodeKind sh:IRI .

core:modifiedTime rdfs:range xsd:dateTime .

_:node1gm7uj6vjx1008 sh:path observable:contactPhone .

action:startTime rdfs:comment "The time at which performance of the action began."@en .

observable:ContactFacet sh:property _:node1gm7uj6vjx1008 .

_:node1gm7uj6vjx562 rdf:first "Unknown"^^vocabulary:ActionStatusTypeVocab .

_:node1gm7uj6vjx1011 sh:class observable:ContactProfile .

_:node1gm7uj6vjx559 sh:path observable:bitRate .

_:node1gm7uj6vjx1010 rdf:first "Unlocked_By"^^vocabulary:ObservableObjectRelationshipVocab .

_:node1gm7uj6vjx562 rdf:rest rdf:nil .

_:node1gm7uj6vjx1010 rdf:rest _:node1gm7uj6vjx1012 .

_:node1gm7uj6vjx554 owl:oneOf _:node1gm7uj6vjx555 .

_:node1gm7uj6vjx1011 sh:minCount 0 .

observable:AudioFacet sh:property _:node1gm7uj6vjx559 .

_:node1gm7uj6vjx1012 rdf:first "Unpacked"^^vocabulary:ObservableObjectRelationshipVocab .

vocabulary:ActionStatusTypeVocab owl:equivalentClass _:node1gm7uj6vjx554 .

_:node1gm7uj6vjx1011 sh:nodeKind sh:IRI .

action:startTime rdfs:range xsd:dateTime .

_:node1gm7uj6vjx1012 rdf:rest _:node1gm7uj6vjx1013 .

_:node1gm7uj6vjx563 sh:datatype xsd:integer .

_:node1gm7uj6vjx1011 sh:path observable:contactProfile .

core:name a owl:DatatypeProperty .

observable:ContactFacet sh:property _:node1gm7uj6vjx1011 .

vocabulary:ActionTypeVocab a rdfs:Datatype .

_:node1gm7uj6vjx1014 sh:class observable:ContactSIP .

core:name rdfs:label "name"@en .

_:node1gm7uj6vjx1013 rdf:first "Unpacked_By"^^vocabulary:ObservableObjectRelationshipVocab .

_:node1gm7uj6vjx563 sh:maxCount 1 .

_:node1gm7uj6vjx1013 rdf:rest _:node1gm7uj6vjx1015 .

vocabulary:ActionTypeVocab rdfs:label "Action Type Vocabulary"@en-us .

_:node1gm7uj6vjx1014 sh:minCount 0 .

_:node1gm7uj6vjx563 sh:nodeKind sh:Literal .

_:node1gm7uj6vjx1014 sh:nodeKind sh:IRI .

core:name rdfs:comment "The name of a particular concept characterization."@en .

_:node1gm7uj6vjx1015 rdf:first "Uploaded"^^vocabulary:ObservableObjectRelationshipVocab .

vocabulary:ActionTypeVocab rdfs:comment "Defines an open-vocabulary of common general action types."@en .

_:node1gm7uj6vjx1015 rdf:rest _:node1gm7uj6vjx1016 .

action:subaction a owl:ObjectProperty .

_:node1gm7uj6vjx1014 sh:path observable:contactSIP .

_:node1gm7uj6vjx563 sh:path observable:duration .

observable:ContactFacet sh:property _:node1gm7uj6vjx1014 .

core:name rdfs:range xsd:string .

_:node1gm7uj6vjx1016 rdf:first "Uploaded_By"^^vocabulary:ObservableObjectRelationshipVocab .

observable:AudioFacet sh:property _:node1gm7uj6vjx563 .

_:node1gm7uj6vjx1016 rdf:rest _:node1gm7uj6vjx1018 .

_:node1gm7uj6vjx564 a rdfs:Datatype .

_:node1gm7uj6vjx1017 sh:class observable:ContactURL .

action:subaction rdfs:label "subaction"@en .

_:node1gm7uj6vjx1018 rdf:first "Uploaded_From"^^vocabulary:ObservableObjectRelationshipVocab .

_:node1gm7uj6vjx565 sh:datatype xsd:string .

_:node1gm7uj6vjx1018 rdf:rest _:node1gm7uj6vjx1019 .

_:node1gm7uj6vjx564 owl:onDatatype xsd:string .

_:node1gm7uj6vjx1017 sh:minCount 0 .

_:node1gm7uj6vjx565 sh:maxCount 1 .

_:node1gm7uj6vjx1017 sh:nodeKind sh:IRI .

core:namingAuthority a owl:DatatypeProperty .

_:node1gm7uj6vjx1017 sh:path observable:contactURL .

_:node1gm7uj6vjx565 sh:nodeKind sh:Literal .

observable:ContactFacet sh:property _:node1gm7uj6vjx1017 .

_:node1gm7uj6vjx566 rdf:first "Accept"^^vocabulary:ActionTypeVocab .

_:node1gm7uj6vjx1020 sh:class observable:ObservableObject .

core:namingAuthority rdfs:label "namingAuthority"@en .

_:node1gm7uj6vjx1019 rdf:first "Uploaded_To"^^vocabulary:ObservableObjectRelationshipVocab .

_:node1gm7uj6vjx566 rdf:rest _:node1gm7uj6vjx567 .

_:node1gm7uj6vjx1019 rdf:rest _:node1gm7uj6vjx1021 .

_:node1gm7uj6vjx565 sh:path observable:audioType .

_:node1gm7uj6vjx1020 sh:maxCount 1 .

observable:AudioFacet sh:property _:node1gm7uj6vjx565 .

_:node1gm7uj6vjx1021 rdf:first "Used"^^vocabulary:ObservableObjectRelationshipVocab .

action:subaction rdfs:comment "References to other actions that make up part of a larger more complex action."@en .

_:node1gm7uj6vjx1021 rdf:rest _:node1gm7uj6vjx1022 .

_:node1gm7uj6vjx568 sh:datatype xsd:string .

_:node1gm7uj6vjx1020 sh:nodeKind sh:IRI .

_:node1gm7uj6vjx567 rdf:first "Access"^^vocabulary:ActionTypeVocab .

_:node1gm7uj6vjx1020 sh:path observable:sourceApplication .

_:node1gm7uj6vjx567 rdf:rest _:node1gm7uj6vjx569 .

core:namingAuthority rdfs:comment "Specifies the naming authority that issued the name of the entity."@en .

observable:ContactFacet sh:property _:node1gm7uj6vjx1020 .

_:node1gm7uj6vjx569 rdf:first "Add"^^vocabulary:ActionTypeVocab .

_:node1gm7uj6vjx1022 rdf:first "Used_By"^^vocabulary:ObservableObjectRelationshipVocab .

_:node1gm7uj6vjx569 rdf:rest _:node1gm7uj6vjx570 .

_:node1gm7uj6vjx1022 rdf:rest _:node1gm7uj6vjx1024 .

action:subaction rdfs:range action:Action .

_:node1gm7uj6vjx1023 sh:datatype xsd:dateTime .

core:namingAuthority rdfs:range xsd:string .

_:node1gm7uj6vjx1024 rdf:first "Values_Enumerated"^^vocabulary:ObservableObjectRelationshipVocab .

_:node1gm7uj6vjx568 sh:maxCount 1 .

_:node1gm7uj6vjx1024 rdf:rest _:node1gm7uj6vjx1025 .

_:node1gm7uj6vjx570 rdf:first "Alert"^^vocabulary:ActionTypeVocab .

_:node1gm7uj6vjx1023 sh:maxCount 1 .

_:node1gm7uj6vjx570 rdf:rest _:node1gm7uj6vjx571 .

_:node1gm7uj6vjx1025 rdf:first "Values_Enumerated_By"^^vocabulary:ObservableObjectRelationshipVocab .

_:node1gm7uj6vjx568 sh:nodeKind sh:Literal .

_:node1gm7uj6vjx1025 rdf:rest _:node1gm7uj6vjx1026 .

_:node1gm7uj6vjx571 rdf:first "Allocate"^^vocabulary:ActionTypeVocab .

_:node1gm7uj6vjx1023 sh:nodeKind sh:Literal .

_:node1gm7uj6vjx571 rdf:rest _:node1gm7uj6vjx572 .

_:node1gm7uj6vjx1023 sh:path identity:birthdate .

_:node1gm7uj6vjx572 rdf:first "Archive"^^vocabulary:ActionTypeVocab .

observable:ContactFacet sh:property _:node1gm7uj6vjx1023 .

_:node1gm7uj6vjx572 rdf:rest _:node1gm7uj6vjx573 .

_:node1gm7uj6vjx1026 rdf:first "Written_To_By"^^vocabulary:ObservableObjectRelationshipVocab .

_:node1gm7uj6vjx568 sh:path observable:format .

_:node1gm7uj6vjx1026 rdf:rest _:node1gm7uj6vjx1028 .

observable:AudioFacet sh:property _:node1gm7uj6vjx568 .

_:node1gm7uj6vjx1027 sh:datatype xsd:dateTime .

action:trend a owl:DatatypeProperty .

_:node1gm7uj6vjx1028 rdf:first "Wrote_To"^^vocabulary:ObservableObjectRelationshipVocab .

core:object a owl:ObjectProperty .

_:node1gm7uj6vjx1028 rdf:rest rdf:nil .

_:node1gm7uj6vjx573 rdf:first "Assign"^^vocabulary:ActionTypeVocab .

_:node1gm7uj6vjx807 owl:oneOf _:node1gm7uj6vjx808 .

_:node1gm7uj6vjx573 rdf:rest _:node1gm7uj6vjx574 .

vocabulary:ObservableObjectRelationshipVocab owl:equivalentClass _:node1gm7uj6vjx807 .

observable:AudioFacet sh:targetClass observable:AudioFacet .

_:node1gm7uj6vjx1027 sh:maxCount 1 .

_:node1gm7uj6vjx574 rdf:first "Audit"^^vocabulary:ActionTypeVocab .

vocabulary:ObservableObjectStateVocab a rdfs:Datatype .

observable:AutonomousSystem a owl:Class .

_:node1gm7uj6vjx1027 sh:nodeKind sh:Literal .

_:node1gm7uj6vjx574 rdf:rest _:node1gm7uj6vjx575 .

_:node1gm7uj6vjx1027 sh:path observable:lastTimeContacted .

observable:AutonomousSystem a sh:NodeShape .

observable:ContactFacet sh:property _:node1gm7uj6vjx1027 .

core:object rdfs:label "object"@en .

_:node1gm7uj6vjx1029 sh:datatype xsd:integer .

_:node1gm7uj6vjx575 rdf:first "Backup"^^vocabulary:ActionTypeVocab .

vocabulary:ObservableObjectStateVocab rdfs:label "Cyber Item State Vocabulary"@en-us .

observable:AutonomousSystem rdfs:subClassOf observable:ObservableObject .

_:node1gm7uj6vjx1029 sh:maxCount 1 .

action:trend rdfs:label "trend"@en .

vocabulary:ObservableObjectStateVocab rdfs:comment "Defines an open-vocabulary of observable object states."@en .

_:node1gm7uj6vjx575 rdf:rest _:node1gm7uj6vjx576 .

_:node1gm7uj6vjx1029 sh:nodeKind sh:Literal .

observable:AutonomousSystem rdfs:label "AutonomousSystem"@en .

_:node1gm7uj6vjx1030 a rdfs:Datatype .

_:node1gm7uj6vjx576 rdf:first "Bind"^^vocabulary:ActionTypeVocab .

_:node1gm7uj6vjx1029 sh:path observable:numberTimesContacted .

_:node1gm7uj6vjx576 rdf:rest _:node1gm7uj6vjx577 .

observable:ContactFacet sh:property _:node1gm7uj6vjx1029 .

core:object rdfs:comment "Specifies one or more UcoObjects."@en .

_:node1gm7uj6vjx1030 owl:onDatatype xsd:string .

_:node1gm7uj6vjx577 rdf:first "Block"^^vocabulary:ActionTypeVocab .

_:node1gm7uj6vjx1031 sh:datatype xsd:string .

_:node1gm7uj6vjx577 rdf:rest _:node1gm7uj6vjx578 .

_:node1gm7uj6vjx1031 sh:maxCount 1 .

core:object rdfs:range core:UcoObject .

_:node1gm7uj6vjx1031 sh:nodeKind sh:Literal .

_:node1gm7uj6vjx578 rdf:first "Call"^^vocabulary:ActionTypeVocab .

_:node1gm7uj6vjx1032 rdf:first "Active"^^vocabulary:ObservableObjectStateVocab .

_:node1gm7uj6vjx578 rdf:rest _:node1gm7uj6vjx579 .

_:node1gm7uj6vjx1031 sh:path observable:contactID .

action:trend rdfs:comment "A characterization of the frequency trend for the occurence of an action."@en .

observable:ContactFacet sh:property _:node1gm7uj6vjx1031 .

core:objectCreatedTime a owl:DatatypeProperty .

_:node1gm7uj6vjx1032 rdf:rest _:node1gm7uj6vjx1033 .

_:node1gm7uj6vjx579 rdf:first "Change"^^vocabulary:ActionTypeVocab .

_:node1gm7uj6vjx1034 sh:datatype xsd:string .

_:node1gm7uj6vjx579 rdf:rest _:node1gm7uj6vjx581 .

_:node1gm7uj6vjx1033 rdf:first "Closed"^^vocabulary:ObservableObjectStateVocab .

_:node1gm7uj6vjx580 a rdfs:Datatype .

_:node1gm7uj6vjx1033 rdf:rest _:node1gm7uj6vjx1035 .

core:objectCreatedTime rdfs:label "objectCreatedTime"@en .

_:node1gm7uj6vjx1034 sh:maxCount 1 .

_:node1gm7uj6vjx581 rdf:first "Check"^^vocabulary:ActionTypeVocab .

_:node1gm7uj6vjx1034 sh:nodeKind sh:Literal .

_:node1gm7uj6vjx581 rdf:rest _:node1gm7uj6vjx583 .

_:node1gm7uj6vjx1034 sh:path observable:displayName .

_:node1gm7uj6vjx582 rdf:first vocabulary:TrendVocab .

observable:ContactFacet sh:property _:node1gm7uj6vjx1034 .

_:node1gm7uj6vjx582 rdf:rest _:node1gm7uj6vjx584 .

_:node1gm7uj6vjx1036 sh:datatype xsd:string .

_:node1gm7uj6vjx584 rdf:first xsd:string .

_:node1gm7uj6vjx1035 rdf:first "Does Not Exist"^^vocabulary:ObservableObjectStateVocab .

_:node1gm7uj6vjx584 rdf:rest rdf:nil .

_:node1gm7uj6vjx1035 rdf:rest _:node1gm7uj6vjx1037 .

_:node1gm7uj6vjx580 owl:unionOf _:node1gm7uj6vjx582 .

_:node1gm7uj6vjx1036 sh:maxCount 1 .

action:trend rdfs:range _:node1gm7uj6vjx580 .

_:node1gm7uj6vjx1036 sh:nodeKind sh:Literal .

_:node1gm7uj6vjx583 rdf:first "Clean"^^vocabulary:ActionTypeVocab .

_:node1gm7uj6vjx1037 rdf:first "Exists"^^vocabulary:ObservableObjectStateVocab .

_:node1gm7uj6vjx583 rdf:rest _:node1gm7uj6vjx585 .

_:node1gm7uj6vjx1037 rdf:rest _:node1gm7uj6vjx1038 .

observable:AutonomousSystem rdfs:comment "An autonomous system is a collection of connected Internet Protocol (IP) routing prefixes under the control of one or more network operators on behalf of a single administrative entity or domain that presents a common, clearly defined routing policy to the Internet. [based on https://en.wikipedia.org/wiki/Autonomous_system_(Internet)]"@en .

_:node1gm7uj6vjx1036 sh:path observable:firstName .

_:node1gm7uj6vjx585 rdf:first "Click"^^vocabulary:ActionTypeVocab .

observable:ContactFacet sh:property _:node1gm7uj6vjx1036 .

_:node1gm7uj6vjx585 rdf:rest _:node1gm7uj6vjx586 .

_:node1gm7uj6vjx1039 sh:datatype xsd:string .

action:units a owl:DatatypeProperty .

_:node1gm7uj6vjx1038 rdf:first "Inactive"^^vocabulary:ObservableObjectStateVocab .

observable:AutonomousSystem sh:targetClass observable:AutonomousSystem .

_:node1gm7uj6vjx1038 rdf:rest _:node1gm7uj6vjx1040 .

_:node1gm7uj6vjx586 rdf:first "Close"^^vocabulary:ActionTypeVocab .

_:node1gm7uj6vjx1039 sh:maxCount 1 .

_:node1gm7uj6vjx586 rdf:rest _:node1gm7uj6vjx587 .

_:node1gm7uj6vjx1040 rdf:first "Locked"^^vocabulary:ObservableObjectStateVocab .

action:units rdfs:label "units"@en .

_:node1gm7uj6vjx1039 sh:nodeKind sh:Literal .

core:objectCreatedTime rdfs:comment "The time at which a characterization of a concept is created. This time pertains to the time of creating the record object, and is not an intrinsic characteristic of the concept."@en .

_:node1gm7uj6vjx1040 rdf:rest _:node1gm7uj6vjx1041 .

_:node1gm7uj6vjx587 rdf:first "Compare"^^vocabulary:ActionTypeVocab .

_:node1gm7uj6vjx1039 sh:path observable:lastName .

_:node1gm7uj6vjx587 rdf:rest _:node1gm7uj6vjx588 .

observable:ContactFacet sh:property _:node1gm7uj6vjx1039 .

observable:AutonomousSystemFacet a owl:Class .

_:node1gm7uj6vjx1042 sh:datatype xsd:string .

_:node1gm7uj6vjx588 rdf:first "Compress"^^vocabulary:ActionTypeVocab .

_:node1gm7uj6vjx1041 rdf:first "Open"^^vocabulary:ObservableObjectStateVocab .

_:node1gm7uj6vjx588 rdf:rest _:node1gm7uj6vjx589 .

_:node1gm7uj6vjx1041 rdf:rest _:node1gm7uj6vjx1043 .

observable:AutonomousSystemFacet a sh:NodeShape .

_:node1gm7uj6vjx1042 sh:maxCount 1 .

core:objectCreatedTime rdfs:range xsd:dateTime .

_:node1gm7uj6vjx1042 sh:nodeKind sh:Literal .

observable:AutonomousSystemFacet rdfs:subClassOf core:Facet .

_:node1gm7uj6vjx1043 rdf:first "Started"^^vocabulary:ObservableObjectStateVocab .

_:node1gm7uj6vjx589 rdf:first "Configure"^^vocabulary:ActionTypeVocab .

_:node1gm7uj6vjx1042 sh:path observable:middleName .

_:node1gm7uj6vjx589 rdf:rest _:node1gm7uj6vjx590 .

observable:ContactFacet sh:property _:node1gm7uj6vjx1042 .

core:objectMarking a owl:ObjectProperty .

_:node1gm7uj6vjx1043 rdf:rest _:node1gm7uj6vjx1044 .

_:node1gm7uj6vjx590 rdf:first "Connect"^^vocabulary:ActionTypeVocab .

_:node1gm7uj6vjx1045 sh:datatype xsd:string .

_:node1gm7uj6vjx590 rdf:rest _:node1gm7uj6vjx591 .

_:node1gm7uj6vjx1044 rdf:first "Stopped"^^vocabulary:ObservableObjectStateVocab .

observable:AutonomousSystemFacet rdfs:label "AutonomousSystemFacet"@en .

_:node1gm7uj6vjx1044 rdf:rest _:node1gm7uj6vjx1046 .

core:objectMarking rdfs:label "objectMarking"@en .

_:node1gm7uj6vjx1045 sh:maxCount 1 .

action:units rdfs:comment "The units of measure utilized for the frequency rate count for the occurence of an action."@en .

_:node1gm7uj6vjx1045 sh:nodeKind sh:Literal .

_:node1gm7uj6vjx591 rdf:first "Control"^^vocabulary:ActionTypeVocab .

_:node1gm7uj6vjx1045 sh:path observable:namePhonetic .

_:node1gm7uj6vjx591 rdf:rest _:node1gm7uj6vjx592 .

observable:ContactFacet sh:property _:node1gm7uj6vjx1045 .

action:units rdfs:range xsd:string .

_:node1gm7uj6vjx1046 rdf:first "Unlocked"^^vocabulary:ObservableObjectStateVocab .

_:node1gm7uj6vjx592 rdf:first "Copy/Duplicate"^^vocabulary:ActionTypeVocab .

_:node1gm7uj6vjx1046 rdf:rest rdf:nil .

_:node1gm7uj6vjx592 rdf:rest _:node1gm7uj6vjx593 .

_:node1gm7uj6vjx1030 owl:oneOf _:node1gm7uj6vjx1032 .

action:value a owl:DatatypeProperty .

_:node1gm7uj6vjx1047 sh:datatype xsd:string .

_:node1gm7uj6vjx593 rdf:first "Create"^^vocabulary:ActionTypeVocab .

vocabulary:ObservableObjectStateVocab owl:equivalentClass _:node1gm7uj6vjx1030 .

_:node1gm7uj6vjx593 rdf:rest _:node1gm7uj6vjx594 .

_:node1gm7uj6vjx1047 sh:maxCount 1 .

core:objectMarking rdfs:comment "Marking definitions to be applied to a particular concept characterization in its entirety."@en .

vocabulary:PartitionTypeVocab a rdfs:Datatype .

action:value rdfs:label "value"@en .

_:node1gm7uj6vjx1047 sh:nodeKind sh:Literal .

_:node1gm7uj6vjx594 rdf:first "Decode"^^vocabulary:ActionTypeVocab .

_:node1gm7uj6vjx1047 sh:path observable:namePrefix .

_:node1gm7uj6vjx594 rdf:rest _:node1gm7uj6vjx595 .

observable:ContactFacet sh:property _:node1gm7uj6vjx1047 .

core:objectMarking rdfs:range core:MarkingDefinitionAbstraction .

_:node1gm7uj6vjx1048 sh:datatype xsd:string .

action:value rdfs:comment "The value of an action parameter."@en .

vocabulary:PartitionTypeVocab rdfs:label "Partition Type Vocabulary"@en-us .

_:node1gm7uj6vjx595 rdf:first "Decompress"^^vocabulary:ActionTypeVocab .

_:node1gm7uj6vjx1048 sh:maxCount 1 .

_:node1gm7uj6vjx595 rdf:rest _:node1gm7uj6vjx596 .

_:node1gm7uj6vjx1048 sh:nodeKind sh:Literal .

observable:AutonomousSystemFacet rdfs:comment "An autonomous system facet is a grouping of characteristics unique to a collection of connected Internet Protocol (IP) routing prefixes under the control of one or more network operators on behalf of a single administrative entity or domain that presents a common, clearly defined routing policy to the Internet. [based on https://en.wikipedia.org/wiki/Autonomous_system_(Internet)]"@en .

vocabulary:PartitionTypeVocab rdfs:comment "Defines an open-vocabulary of partition types. See http://www.win.tue.nl/~aeb/partitions/partition_types-1.html for more information about the various partition types."@en .

action:value rdfs:range xsd:string .

_:node1gm7uj6vjx1048 sh:path observable:nameSuffix .

core:referenceURL a owl:DatatypeProperty .

observable:ContactFacet sh:property _:node1gm7uj6vjx1048 .

_:node1gm7uj6vjx596 rdf:first "Decrypt"^^vocabulary:ActionTypeVocab .

_:node1gm7uj6vjx1050 a rdfs:Datatype .

_:node1gm7uj6vjx596 rdf:rest _:node1gm7uj6vjx597 .

_:node1gm7uj6vjx1049 sh:datatype xsd:string .

core:referenceURL rdfs:label "referenceURL"@en .

_:node1gm7uj6vjx1050 owl:onDatatype xsd:string .

_:node1gm7uj6vjx597 rdf:first "Deny"^^vocabulary:ActionTypeVocab .

_:node1gm7uj6vjx1049 sh:minCount 0 .

observable:AutonomousSystemFacet sh:property observable:regionalInternetRegistry-shape-value-not-vocabulary-member .

_:node1gm7uj6vjx1049 sh:nodeKind sh:Literal .

_:node1gm7uj6vjx597 rdf:rest _:node1gm7uj6vjx598 .

_:node1gm7uj6vjx1049 sh:path observable:contactGroup .

_:node1gm7uj6vjx598 rdf:first "Depress"^^vocabulary:ActionTypeVocab .

observable:ContactFacet sh:property _:node1gm7uj6vjx1049 .

_:node1gm7uj6vjx598 rdf:rest _:node1gm7uj6vjx599 .

_:node1gm7uj6vjx1051 rdf:first "PARTITION_ENTRY_UNUSED"^^vocabulary:PartitionTypeVocab .

core:referenceURL rdfs:comment "A URL for some information defined external to the UCO context."@en .

_:node1gm7uj6vjx1052 sh:datatype xsd:string .

observable:AutonomousSystemFacet sh:property observable:regionalInternetRegistry-shape-value-outside-default-vocabulary .

_:node1gm7uj6vjx1051 rdf:rest _:node1gm7uj6vjx1053 .

core:referenceURL rdfs:range xsd:anyURI .

_:node1gm7uj6vjx1052 sh:minCount 0 .

_:node1gm7uj6vjx599 rdf:first "Detect"^^vocabulary:ActionTypeVocab .

_:node1gm7uj6vjx1053 rdf:first "PARTITION_EXTENDED"^^vocabulary:PartitionTypeVocab .

_:node1gm7uj6vjx599 rdf:rest _:node1gm7uj6vjx601 .

_:node1gm7uj6vjx1053 rdf:rest _:node1gm7uj6vjx1054 .

_:node1gm7uj6vjx600 sh:datatype xsd:integer .

_:node1gm7uj6vjx1052 sh:nodeKind sh:Literal .

_:node1gm7uj6vjx601 rdf:first "Disconnect"^^vocabulary:ActionTypeVocab .

_:node1gm7uj6vjx1052 sh:path observable:contactNote .

core:source a owl:ObjectProperty .

observable:ContactFacet sh:property _:node1gm7uj6vjx1052 .

_:node1gm7uj6vjx601 rdf:rest _:node1gm7uj6vjx602 .

_:node1gm7uj6vjx1055 sh:datatype xsd:string .

_:node1gm7uj6vjx602 rdf:first "Download"^^vocabulary:ActionTypeVocab .

_:node1gm7uj6vjx1054 rdf:first "PARTITION_FAT32"^^vocabulary:PartitionTypeVocab .

core:source rdfs:label "source"@en .

_:node1gm7uj6vjx1054 rdf:rest _:node1gm7uj6vjx1056 .

_:node1gm7uj6vjx602 rdf:rest _:node1gm7uj6vjx603 .

_:node1gm7uj6vjx1055 sh:minCount 0 .

_:node1gm7uj6vjx600 sh:maxCount 1 .

_:node1gm7uj6vjx1055 sh:nodeKind sh:Literal .

_:node1gm7uj6vjx600 sh:nodeKind sh:Literal .

_:node1gm7uj6vjx1056 rdf:first "PARTITION_FAT32_XINT13"^^vocabulary:PartitionTypeVocab .

_:node1gm7uj6vjx603 rdf:first "Draw"^^vocabulary:ActionTypeVocab .

_:node1gm7uj6vjx1056 rdf:rest _:node1gm7uj6vjx1057 .

_:node1gm7uj6vjx603 rdf:rest _:node1gm7uj6vjx604 .

_:node1gm7uj6vjx1055 sh:path observable:nickname .

core:source rdfs:comment "The originating node of a specified relationship."@en .

observable:ContactFacet sh:property _:node1gm7uj6vjx1055 .

_:node1gm7uj6vjx600 sh:path observable:number .

observable:ContactFacet sh:targetClass observable:ContactFacet .

observable:AutonomousSystemFacet sh:property _:node1gm7uj6vjx600 .

_:node1gm7uj6vjx1057 rdf:first "PARTITION_FAT_12"^^vocabulary:PartitionTypeVocab .

_:node1gm7uj6vjx604 rdf:first "Drop"^^vocabulary:ActionTypeVocab .

_:node1gm7uj6vjx1057 rdf:rest _:node1gm7uj6vjx1058 .

_:node1gm7uj6vjx605 sh:datatype xsd:string .

observable:ContactList a owl:Class .

core:source rdfs:range core:UcoObject .

observable:ContactList a sh:NodeShape .

_:node1gm7uj6vjx604 rdf:rest _:node1gm7uj6vjx606 .

observable:ContactList rdfs:subClassOf observable:ObservableObject .

_:node1gm7uj6vjx605 sh:maxCount 1 .

_:node1gm7uj6vjx1058 rdf:first "PARTITION_FAT_16"^^vocabulary:PartitionTypeVocab .

_:node1gm7uj6vjx606 rdf:first "Encode"^^vocabulary:ActionTypeVocab .

_:node1gm7uj6vjx1058 rdf:rest _:node1gm7uj6vjx1059 .

_:node1gm7uj6vjx606 rdf:rest _:node1gm7uj6vjx607 .

observable:ContactList rdfs:label "ContactList"@en .

_:node1gm7uj6vjx605 sh:nodeKind sh:Literal .

_:node1gm7uj6vjx1059 rdf:first "PARTITION_HUGE"^^vocabulary:PartitionTypeVocab .

core:specVersion a owl:DatatypeProperty .

_:node1gm7uj6vjx1059 rdf:rest _:node1gm7uj6vjx1060 .

_:node1gm7uj6vjx605 sh:path observable:asHandle .

observable:ContactList rdfs:comment "A contact list is a set of multiple individual contacts such as that found in a digital address book."@en .

observable:AutonomousSystemFacet sh:property _:node1gm7uj6vjx605 .

observable:ContactList sh:targetClass observable:ContactList .

_:node1gm7uj6vjx607 rdf:first "Encrypt"^^vocabulary:ActionTypeVocab .

observable:ContactListFacet a owl:Class .

_:node1gm7uj6vjx607 rdf:rest _:node1gm7uj6vjx609 .

_:node1gm7uj6vjx1060 rdf:first "PARTITION_IFS"^^vocabulary:PartitionTypeVocab .

core:specVersion rdfs:label "specVersion"@en .

_:node1gm7uj6vjx1060 rdf:rest _:node1gm7uj6vjx1061 .

_:node1gm7uj6vjx608 sh:maxCount 1 .

observable:ContactListFacet a sh:NodeShape .

_:node1gm7uj6vjx609 rdf:first "Enumerate"^^vocabulary:ActionTypeVocab .

observable:ContactListFacet rdfs:subClassOf core:Facet .

_:node1gm7uj6vjx609 rdf:rest _:node1gm7uj6vjx610 .

observable:ContactListFacet rdfs:label "ContactListFacet"@en .

_:node1gm7uj6vjx608 sh:nodeKind sh:Literal .

_:node1gm7uj6vjx1061 rdf:first "PARTITION_LDM"^^vocabulary:PartitionTypeVocab .

_:node1gm7uj6vjx610 rdf:first "Execute"^^vocabulary:ActionTypeVocab .

_:node1gm7uj6vjx1061 rdf:rest _:node1gm7uj6vjx1062 .

_:node1gm7uj6vjx610 rdf:rest _:node1gm7uj6vjx613 .

observable:ContactListFacet rdfs:comment "A contact list facet is a grouping of characteristics unique to a set of multiple individual contacts such as that found in a digital address book."@en .

core:specVersion rdfs:comment "The version of UCO ontology or subontology specification used to characterize a concept."@en .

_:node1gm7uj6vjx1062 rdf:first "PARTITION_NTFT"^^vocabulary:PartitionTypeVocab .

core:specVersion rdfs:range xsd:string .

_:node1gm7uj6vjx1062 rdf:rest _:node1gm7uj6vjx1063 .

_:node1gm7uj6vjx612 sh:datatype vocabulary:RegionalRegistryTypeVocab .

_:node1gm7uj6vjx1064 sh:class observable:ObservableObject .

_:node1gm7uj6vjx613 rdf:first "Extract"^^vocabulary:ActionTypeVocab .

_:node1gm7uj6vjx1063 rdf:first "PARTITION_OS2BOOTMGR"^^vocabulary:PartitionTypeVocab .

_:node1gm7uj6vjx611 rdf:first _:node1gm7uj6vjx612 .

_:node1gm7uj6vjx1063 rdf:rest _:node1gm7uj6vjx1065 .

_:node1gm7uj6vjx613 rdf:rest _:node1gm7uj6vjx614 .

_:node1gm7uj6vjx1064 sh:maxCount 1 .

_:node1gm7uj6vjx611 rdf:rest _:node1gm7uj6vjx615 .

_:node1gm7uj6vjx1064 sh:nodeKind sh:IRI .

_:node1gm7uj6vjx614 rdf:first "Filter"^^vocabulary:ActionTypeVocab .

_:node1gm7uj6vjx1064 sh:path observable:sourceApplication .

_:node1gm7uj6vjx614 rdf:rest _:node1gm7uj6vjx617 .

observable:ContactListFacet sh:property _:node1gm7uj6vjx1064 .

core:startTime a owl:DatatypeProperty .

_:node1gm7uj6vjx1065 rdf:first "PARTITION_PREP"^^vocabulary:PartitionTypeVocab .

_:node1gm7uj6vjx616 sh:datatype xsd:string .

_:node1gm7uj6vjx1065 rdf:rest _:node1gm7uj6vjx1067 .

_:node1gm7uj6vjx615 rdf:first _:node1gm7uj6vjx616 .

_:node1gm7uj6vjx1066 sh:class observable:ObservableObject .

_:node1gm7uj6vjx615 rdf:rest rdf:nil .

_:node1gm7uj6vjx1066 sh:nodeKind sh:IRI .

_:node1gm7uj6vjx608 sh:or _:node1gm7uj6vjx611 .

_:node1gm7uj6vjx1066 sh:path observable:contact .

_:node1gm7uj6vjx617 rdf:first "Find"^^vocabulary:ActionTypeVocab .

observable:ContactListFacet sh:property _:node1gm7uj6vjx1066 .

_:node1gm7uj6vjx617 rdf:rest _:node1gm7uj6vjx618 .

_:node1gm7uj6vjx1067 rdf:first "PARTITION_UNIX"^^vocabulary:PartitionTypeVocab .

core:startTime rdfs:label "startTime"@en .

_:node1gm7uj6vjx1067 rdf:rest _:node1gm7uj6vjx1068 .

_:node1gm7uj6vjx608 sh:path observable:regionalInternetRegistry .

observable:ContactListFacet sh:targetClass observable:ContactListFacet .

observable:AutonomousSystemFacet sh:property _:node1gm7uj6vjx608 .

_:node1gm7uj6vjx1068 rdf:first "PARTITION_XENIX_1"^^vocabulary:PartitionTypeVocab .

_:node1gm7uj6vjx618 rdf:first "Flush"^^vocabulary:ActionTypeVocab .

_:node1gm7uj6vjx1068 rdf:rest _:node1gm7uj6vjx1069 .

_:node1gm7uj6vjx618 rdf:rest _:node1gm7uj6vjx619 .

_:node1gm7uj6vjx1069 rdf:first "PARTITION_XENIX_2"^^vocabulary:PartitionTypeVocab .

core:startTime rdfs:comment "The initial time of a time range."@en .

_:node1gm7uj6vjx1069 rdf:rest _:node1gm7uj6vjx1070 .

_:node1gm7uj6vjx619 rdf:first "Fork"^^vocabulary:ActionTypeVocab .

_:node1gm7uj6vjx1070 rdf:first "PARTITION_XINT13"^^vocabulary:PartitionTypeVocab .

_:node1gm7uj6vjx619 rdf:rest _:node1gm7uj6vjx620 .

_:node1gm7uj6vjx1070 rdf:rest _:node1gm7uj6vjx1071 .

core:startTime rdfs:range xsd:dateTime .

observable:ContactMessaging a owl:Class .

_:node1gm7uj6vjx620 rdf:first "Free"^^vocabulary:ActionTypeVocab .

observable:ContactMessaging a sh:NodeShape .

core:statement a owl:DatatypeProperty .

_:node1gm7uj6vjx1071 rdf:first "PARTITION_XINT13_EXTENDED"^^vocabulary:PartitionTypeVocab .

_:node1gm7uj6vjx620 rdf:rest _:node1gm7uj6vjx621 .

_:node1gm7uj6vjx1071 rdf:rest _:node1gm7uj6vjx1072 .

observable:AutonomousSystemFacet sh:targetClass observable:AutonomousSystemFacet .

observable:ContactMessaging rdfs:subClassOf core:UcoInherentCharacterizationThing .

core:statement rdfs:label "statement"@en .

observable:ContactMessaging rdfs:label "ContactMessaging"@en .

_:node1gm7uj6vjx621 rdf:first "Get"^^vocabulary:ActionTypeVocab .

_:node1gm7uj6vjx1072 rdf:first "UNKNOWN"^^vocabulary:PartitionTypeVocab .

_:node1gm7uj6vjx621 rdf:rest _:node1gm7uj6vjx622 .

_:node1gm7uj6vjx1072 rdf:rest _:node1gm7uj6vjx1073 .

observable:BlackberryPhone a owl:Class .

observable:ContactMessaging rdfs:comment "A contact messaging is a grouping of characteristics unique to details for contacting a contact entity by digital messaging."@en .

_:node1gm7uj6vjx622 rdf:first "Hide"^^vocabulary:ActionTypeVocab .

_:node1gm7uj6vjx1073 rdf:first "VALID_NTFT"^^vocabulary:PartitionTypeVocab .

_:node1gm7uj6vjx622 rdf:rest _:node1gm7uj6vjx623 .

_:node1gm7uj6vjx1073 rdf:rest rdf:nil .

core:statement rdfs:comment "A textual statement of an assertion."@en .

_:node1gm7uj6vjx1050 owl:oneOf _:node1gm7uj6vjx1051 .

observable:BlackberryPhone a sh:NodeShape .

vocabulary:PartitionTypeVocab owl:equivalentClass _:node1gm7uj6vjx1050 .

_:node1gm7uj6vjx623 rdf:first "Hook"^^vocabulary:ActionTypeVocab .

_:node1gm7uj6vjx1074 sh:class observable:ObservableObject .

core:statement rdfs:range xsd:string .

vocabulary:ProcessorArchVocab a rdfs:Datatype .

_:node1gm7uj6vjx623 rdf:rest _:node1gm7uj6vjx624 .

_:node1gm7uj6vjx1074 sh:maxCount 1 .

observable:BlackberryPhone rdfs:subClassOf observable:SmartPhone .

_:node1gm7uj6vjx1074 sh:nodeKind sh:IRI .

_:node1gm7uj6vjx624 rdf:first "Impersonate"^^vocabulary:ActionTypeVocab .

vocabulary:ProcessorArchVocab rdfs:label "Processor Architecture Vocabulary"@en-us .

_:node1gm7uj6vjx624 rdf:rest _:node1gm7uj6vjx625 .

_:node1gm7uj6vjx1074 sh:path observable:contactMessagingPlatform .

core:tag a owl:DatatypeProperty .

observable:ContactMessaging sh:property _:node1gm7uj6vjx1074 .

_:node1gm7uj6vjx625 rdf:first "Initialize"^^vocabulary:ActionTypeVocab .

vocabulary:ProcessorArchVocab rdfs:comment "Defines an open-vocabulary of computer processor architectures."@en .

_:node1gm7uj6vjx625 rdf:rest _:node1gm7uj6vjx626 .

_:node1gm7uj6vjx1075 sh:class observable:ObservableObject .

core:tag rdfs:label "tag"@en .

_:node1gm7uj6vjx1076 a rdfs:Datatype .

_:node1gm7uj6vjx626 rdf:first "Inject"^^vocabulary:ActionTypeVocab .

_:node1gm7uj6vjx1076 owl:onDatatype xsd:string .

_:node1gm7uj6vjx626 rdf:rest _:node1gm7uj6vjx627 .

_:node1gm7uj6vjx1075 sh:maxCount 1 .

observable:BlackberryPhone rdfs:label "BlackberryPhone"@en-us .

_:node1gm7uj6vjx1075 sh:nodeKind sh:IRI .

core:tag rdfs:comment "A generic tag/label."@en .

_:node1gm7uj6vjx1075 sh:path observable:messagingAddress .

_:node1gm7uj6vjx627 rdf:first "Install"^^vocabulary:ActionTypeVocab .

observable:ContactMessaging sh:property _:node1gm7uj6vjx1075 .

_:node1gm7uj6vjx627 rdf:rest _:node1gm7uj6vjx628 .

observable:ContactMessaging sh:targetClass observable:ContactMessaging .

core:tag rdfs:range xsd:string .

_:node1gm7uj6vjx1077 rdf:first "ARM"^^vocabulary:ProcessorArchVocab .

_:node1gm7uj6vjx628 rdf:first "Interleave"^^vocabulary:ActionTypeVocab .

_:node1gm7uj6vjx1077 rdf:rest _:node1gm7uj6vjx1078 .

core:target a owl:ObjectProperty .

observable:ContactPhone a owl:Class .

_:node1gm7uj6vjx628 rdf:rest _:node1gm7uj6vjx629 .

observable:ContactPhone a sh:NodeShape .

core:target rdfs:label "target"@en .

observable:ContactPhone rdfs:subClassOf core:UcoInherentCharacterizationThing .

_:node1gm7uj6vjx629 rdf:first "Join"^^vocabulary:ActionTypeVocab .

observable:ContactPhone rdfs:label "ContactPhone"@en .

_:node1gm7uj6vjx629 rdf:rest _:node1gm7uj6vjx630 .

observable:ContactPhone rdfs:comment "A contact phone is a grouping of characteristics unique to details for contacting a contact entity by telephone."@en .

observable:BlackberryPhone rdfs:comment "A blackberry phone is a smart phone that applies the Blackberry OS mobile operating system. (Blackberry 10 re-introduces Blackberry OS, prior to that the OS was Android.)"@en-us .

_:node1gm7uj6vjx1078 rdf:first "Alpha"^^vocabulary:ProcessorArchVocab .

_:node1gm7uj6vjx630 rdf:first "Kill"^^vocabulary:ActionTypeVocab .

_:node1gm7uj6vjx1078 rdf:rest _:node1gm7uj6vjx1079 .

_:node1gm7uj6vjx630 rdf:rest _:node1gm7uj6vjx631 .

_:node1gm7uj6vjx1080 sh:class observable:ObservableObject .

core:target rdfs:comment "The terminating node of a specified relationship."@en .

_:node1gm7uj6vjx1080 sh:maxCount 1 .

observable:BlackberryPhone sh:targetClass observable:BlackberryPhone .

_:node1gm7uj6vjx1080 sh:nodeKind sh:IRI .

core:target rdfs:range core:UcoObject .

_:node1gm7uj6vjx1080 sh:path observable:contactPhoneNumber .

_:node1gm7uj6vjx631 rdf:first "Listen"^^vocabulary:ActionTypeVocab .

observable:ContactPhone sh:property _:node1gm7uj6vjx1080 .

_:node1gm7uj6vjx631 rdf:rest _:node1gm7uj6vjx632 .

_:node1gm7uj6vjx1079 rdf:first "IA-64"^^vocabulary:ProcessorArchVocab .

_:node1gm7uj6vjx632 rdf:first "Load"^^vocabulary:ActionTypeVocab .

_:node1gm7uj6vjx1079 rdf:rest _:node1gm7uj6vjx1082 .

_:node1gm7uj6vjx632 rdf:rest _:node1gm7uj6vjx633 .

_:node1gm7uj6vjx1081 sh:datatype vocabulary:ContactPhoneScopeVocab .

core:value a owl:DatatypeProperty .

_:node1gm7uj6vjx1081 sh:message "Value is outside the default vocabulary ContactPhoneScopeVocab." .

observable:BlockDeviceNode a owl:Class .

_:node1gm7uj6vjx1082 rdf:first "MIPS"^^vocabulary:ProcessorArchVocab .

observable:BlockDeviceNode a sh:NodeShape .

_:node1gm7uj6vjx1082 rdf:rest _:node1gm7uj6vjx1083 .

core:value rdfs:label "value"@en .

_:node1gm7uj6vjx1081 sh:path observable:contactPhoneScope .

_:node1gm7uj6vjx633 rdf:first "Lock"^^vocabulary:ActionTypeVocab .

_:node1gm7uj6vjx1083 rdf:first "Motorola 68k"^^vocabulary:ProcessorArchVocab .

_:node1gm7uj6vjx633 rdf:rest _:node1gm7uj6vjx634 .

_:node1gm7uj6vjx1083 rdf:rest _:node1gm7uj6vjx1084 .

core:value rdfs:comment "A string value."@en .

_:node1gm7uj6vjx1081 sh:severity sh:Info .

observable:BlockDeviceNode rdfs:subClassOf observable:FileSystemObject .

observable:ContactPhone sh:property _:node1gm7uj6vjx1081 .

core:value rdfs:range xsd:string .

_:node1gm7uj6vjx1084 rdf:first "Other"^^vocabulary:ProcessorArchVocab .

_:node1gm7uj6vjx634 rdf:first "Login/Logon"^^vocabulary:ActionTypeVocab .

_:node1gm7uj6vjx1084 rdf:rest _:node1gm7uj6vjx1086 .

_:node1gm7uj6vjx634 rdf:rest _:node1gm7uj6vjx635 .

_:node1gm7uj6vjx1086 rdf:first "PowerPC"^^vocabulary:ProcessorArchVocab .

observable:BlockDeviceNode rdfs:label "BlockDeviceNode"@en .

_:node1gm7uj6vjx1086 rdf:rest _:node1gm7uj6vjx1087 .

_:node1gm7uj6vjx635 rdf:first "Logout/Logoff"^^vocabulary:ActionTypeVocab .

_:node1gm7uj6vjx1085 sh:maxCount 1 .

_:node1gm7uj6vjx1087 rdf:first "SPARC"^^vocabulary:ProcessorArchVocab .

_:node1gm7uj6vjx635 rdf:rest _:node1gm7uj6vjx636 .

_:node1gm7uj6vjx1087 rdf:rest _:node1gm7uj6vjx1088 .

_:node1gm7uj6vjx636 rdf:first "Map"^^vocabulary:ActionTypeVocab .

_:node1gm7uj6vjx1085 sh:nodeKind sh:Literal .

_:node1gm7uj6vjx636 rdf:rest _:node1gm7uj6vjx637 .

_:node1gm7uj6vjx1088 rdf:first "eSi-RISC"^^vocabulary:ProcessorArchVocab .

_:node1gm7uj6vjx637 rdf:first "Merge"^^vocabulary:ActionTypeVocab .

_:node1gm7uj6vjx1088 rdf:rest _:node1gm7uj6vjx1090 .

_:node1gm7uj6vjx637 rdf:rest _:node1gm7uj6vjx638 .

_:node1gm7uj6vjx1090 rdf:first "x86-32"^^vocabulary:ProcessorArchVocab .

_:node1gm7uj6vjx638 rdf:first "Modify"^^vocabulary:ActionTypeVocab .

_:node1gm7uj6vjx1090 rdf:rest _:node1gm7uj6vjx1092 .

_:node1gm7uj6vjx638 rdf:rest _:node1gm7uj6vjx640 .

_:node1gm7uj6vjx1091 sh:datatype vocabulary:ContactPhoneScopeVocab .

_:node1gm7uj6vjx639 a owl:AllDisjointClasses .

_:node1gm7uj6vjx1089 rdf:first _:node1gm7uj6vjx1091 .

_:node1gm7uj6vjx640 rdf:first "Monitor"^^vocabulary:ActionTypeVocab .

_:node1gm7uj6vjx1092 rdf:first "x86-64"^^vocabulary:ProcessorArchVocab .

_:node1gm7uj6vjx640 rdf:rest _:node1gm7uj6vjx642 .

_:node1gm7uj6vjx1089 rdf:rest _:node1gm7uj6vjx1093 .

observable:BlockDeviceNode rdfs:comment "A block device node is a UNIX filesystem special file that serves as a conduit to communicate with devices, providing buffered randomly accesible input and output. Block device nodes are used to apply access rights to the devices and to direct operations on the files to the appropriate device drivers. [based on https://en.wikipedia.org/wiki/Unix_file_types]"@en .

_:node1gm7uj6vjx1092 rdf:rest _:node1gm7uj6vjx1094 .

_:node1gm7uj6vjx641 rdf:first core:UcoInherentCharacterizationThing .

_:node1gm7uj6vjx1094 rdf:first "z/Architecture"^^vocabulary:ProcessorArchVocab .

_:node1gm7uj6vjx641 rdf:rest _:node1gm7uj6vjx643 .

_:node1gm7uj6vjx1094 rdf:rest rdf:nil .

_:node1gm7uj6vjx643 rdf:first core:UcoObject .

_:node1gm7uj6vjx1095 sh:datatype xsd:string .

_:node1gm7uj6vjx643 rdf:rest rdf:nil .

_:node1gm7uj6vjx1076 owl:oneOf _:node1gm7uj6vjx1077 .

_:node1gm7uj6vjx642 rdf:first "Move"^^vocabulary:ActionTypeVocab .

_:node1gm7uj6vjx1093 rdf:first _:node1gm7uj6vjx1095 .

observable:BlockDeviceNode sh:targetClass observable:BlockDeviceNode .

vocabulary:ProcessorArchVocab owl:equivalentClass _:node1gm7uj6vjx1076 .

_:node1gm7uj6vjx639 owl:members _:node1gm7uj6vjx641 .

_:node1gm7uj6vjx1093 rdf:rest rdf:nil .

_:node1gm7uj6vjx642 rdf:rest _:node1gm7uj6vjx644 .

_:node1gm7uj6vjx1085 sh:or _:node1gm7uj6vjx1089 .

_:node1gm7uj6vjx644 rdf:first "Open"^^vocabulary:ActionTypeVocab .

_:node1gm7uj6vjx1085 sh:path observable:contactPhoneScope .

observable:BluetoothAddress a owl:Class .

observable:ContactPhone sh:property _:node1gm7uj6vjx1085 .

_:node1gm7uj6vjx644 rdf:rest _:node1gm7uj6vjx645 .

vocabulary:RecoveredObjectStatusVocab a rdfs:Datatype .

observable:BluetoothAddress a sh:NodeShape .

_:node1gm7uj6vjx1096 sh:message "Value is not member of the vocabulary ContactPhoneScopeVocab." .

observable:BluetoothAddress rdfs:subClassOf observable:MACAddress .

vocabulary:RecoveredObjectStatusVocab rdfs:label "Recovered Object Status Vocabulary"@en-us .

_:node1gm7uj6vjx645 rdf:first "Pack"^^vocabulary:ActionTypeVocab .

_:node1gm7uj6vjx1098 sh:datatype vocabulary:ContactPhoneScopeVocab .

_:node1gm7uj6vjx645 rdf:rest _:node1gm7uj6vjx646 .

vocabulary:RecoveredObjectStatusVocab rdfs:comment "Defines the vocabulary for Recovered Object status of data."@en .

observable:BluetoothAddress rdfs:label "BluetoothAddress"@en .

_:node1gm7uj6vjx1099 rdf:first "home"^^vocabulary:ContactPhoneScopeVocab .

_:node1gm7uj6vjx646 rdf:first "Pause"^^vocabulary:ActionTypeVocab .

_:node1gm7uj6vjx1100 a rdfs:Datatype .

_:node1gm7uj6vjx646 rdf:rest _:node1gm7uj6vjx647 .

_:node1gm7uj6vjx1099 rdf:rest _:node1gm7uj6vjx1101 .

_:node1gm7uj6vjx647 rdf:first "Press"^^vocabulary:ActionTypeVocab .

_:node1gm7uj6vjx1100 owl:onDatatype xsd:string .

_:node1gm7uj6vjx647 rdf:rest _:node1gm7uj6vjx648 .

_:node1gm7uj6vjx1101 rdf:first "work"^^vocabulary:ContactPhoneScopeVocab .

_:node1gm7uj6vjx648 rdf:first "Protect"^^vocabulary:ActionTypeVocab .

_:node1gm7uj6vjx1101 rdf:rest _:node1gm7uj6vjx1103 .

_:node1gm7uj6vjx648 rdf:rest _:node1gm7uj6vjx649 .

_:node1gm7uj6vjx1102 rdf:first "recovered"^^vocabulary:RecoveredObjectStatusVocab .

observable:BluetoothAddress rdfs:comment "A Bluetooth address is a Bluetooth standard conformant identifier assigned to a Bluetooth device to enable routing and management of Bluetooth standards conformant communication to or from that device."@en .

_:node1gm7uj6vjx1102 rdf:rest _:node1gm7uj6vjx1104 .

_:node1gm7uj6vjx649 rdf:first "Quarantine"^^vocabulary:ActionTypeVocab .

_:node1gm7uj6vjx1103 rdf:first "school"^^vocabulary:ContactPhoneScopeVocab .

_:node1gm7uj6vjx649 rdf:rest _:node1gm7uj6vjx650 .

_:node1gm7uj6vjx1103 rdf:rest _:node1gm7uj6vjx1105 .

observable:BluetoothAddress sh:targetClass observable:BluetoothAddress .

_:node1gm7uj6vjx1104 rdf:first "partially recovered"^^vocabulary:RecoveredObjectStatusVocab .

_:node1gm7uj6vjx650 rdf:first "Query"^^vocabulary:ActionTypeVocab .

_:node1gm7uj6vjx1104 rdf:rest _:node1gm7uj6vjx1106 .

observable:BluetoothAddressFacet a owl:Class .

_:node1gm7uj6vjx1105 rdf:first "mobile"^^vocabulary:ContactPhoneScopeVocab .

_:node1gm7uj6vjx650 rdf:rest _:node1gm7uj6vjx651 .

_:node1gm7uj6vjx1105 rdf:rest _:node1gm7uj6vjx1107 .

observable:BluetoothAddressFacet a sh:NodeShape .

_:node1gm7uj6vjx1106 rdf:first "overwritten"^^vocabulary:RecoveredObjectStatusVocab .

_:node1gm7uj6vjx651 rdf:first "Queue"^^vocabulary:ActionTypeVocab .

_:node1gm7uj6vjx1106 rdf:rest _:node1gm7uj6vjx1108 .

_:node1gm7uj6vjx651 rdf:rest _:node1gm7uj6vjx652 .

_:node1gm7uj6vjx1108 rdf:first "unknown"^^vocabulary:RecoveredObjectStatusVocab .

observable:BluetoothAddressFacet rdfs:subClassOf observable:MACAddressFacet .

_:node1gm7uj6vjx1107 rdf:first "main"^^vocabulary:ContactPhoneScopeVocab .

_:node1gm7uj6vjx652 rdf:first "Raise"^^vocabulary:ActionTypeVocab .

_:node1gm7uj6vjx1108 rdf:rest rdf:nil .

_:node1gm7uj6vjx652 rdf:rest _:node1gm7uj6vjx653 .

_:node1gm7uj6vjx1100 owl:oneOf _:node1gm7uj6vjx1102 .

observable:BluetoothAddressFacet rdfs:label "BluetoothAddressFacet"@en .

vocabulary:RecoveredObjectStatusVocab owl:equivalentClass _:node1gm7uj6vjx1100 .

_:node1gm7uj6vjx653 rdf:first "Read"^^vocabulary:ActionTypeVocab .

_:node1gm7uj6vjx1107 rdf:rest _:node1gm7uj6vjx1109 .

_:node1gm7uj6vjx653 rdf:rest _:node1gm7uj6vjx654 .

vocabulary:RegionalRegistryTypeVocab a rdfs:Datatype .

_:node1gm7uj6vjx654 rdf:first "Receive"^^vocabulary:ActionTypeVocab .

_:node1gm7uj6vjx1109 rdf:first "home fax"^^vocabulary:ContactPhoneScopeVocab .

_:node1gm7uj6vjx654 rdf:rest _:node1gm7uj6vjx655 .

_:node1gm7uj6vjx1109 rdf:rest _:node1gm7uj6vjx1110 .

_:node1gm7uj6vjx655 rdf:first "Release"^^vocabulary:ActionTypeVocab .

vocabulary:RegionalRegistryTypeVocab rdfs:label "Regional Registry Type Vocabulary"@en-us .

_:node1gm7uj6vjx655 rdf:rest _:node1gm7uj6vjx656 .

_:node1gm7uj6vjx1110 rdf:first "work fax"^^vocabulary:ContactPhoneScopeVocab .

observable:BluetoothAddressFacet rdfs:comment "A Bluetooth address facet is a grouping of characteristics unique to a Bluetooth standard conformant identifier assigned to a Bluetooth device to enable routing and management of Bluetooth standards conformant communication to or from that device."@en .

_:node1gm7uj6vjx1110 rdf:rest _:node1gm7uj6vjx1111 .

_:node1gm7uj6vjx656 rdf:first "Remove/Delete"^^vocabulary:ActionTypeVocab .

vocabulary:RegionalRegistryTypeVocab rdfs:comment "Defines an open-vocabulary of Regional Internet Registries (RIRs) names, represented via their respective acronyms."@en .

_:node1gm7uj6vjx656 rdf:rest _:node1gm7uj6vjx657 .

_:node1gm7uj6vjx1112 a rdfs:Datatype .

_:node1gm7uj6vjx657 rdf:first "Rename"^^vocabulary:ActionTypeVocab .

_:node1gm7uj6vjx1111 rdf:first "pager"^^vocabulary:ContactPhoneScopeVocab .

_:node1gm7uj6vjx657 rdf:rest _:node1gm7uj6vjx658 .

_:node1gm7uj6vjx1112 owl:onDatatype xsd:string .

observable:BluetoothAddressFacet sh:targetClass observable:BluetoothAddressFacet .

_:node1gm7uj6vjx1111 rdf:rest rdf:nil .

_:node1gm7uj6vjx658 rdf:first "Replicate"^^vocabulary:ActionTypeVocab .

_:node1gm7uj6vjx1098 sh:in _:node1gm7uj6vjx1099 .

_:node1gm7uj6vjx658 rdf:rest _:node1gm7uj6vjx659 .

_:node1gm7uj6vjx1097 rdf:first _:node1gm7uj6vjx1098 .

_:node1gm7uj6vjx659 rdf:first "Restore"^^vocabulary:ActionTypeVocab .

_:node1gm7uj6vjx1097 rdf:rest _:node1gm7uj6vjx1113 .

_:node1gm7uj6vjx659 rdf:rest _:node1gm7uj6vjx660 .

_:node1gm7uj6vjx1114 sh:datatype xsd:string .

observable:BotConfiguration a owl:Class .

_:node1gm7uj6vjx1113 rdf:first _:node1gm7uj6vjx1114 .

observable:BotConfiguration a sh:NodeShape .

_:node1gm7uj6vjx1115 rdf:first "APNIC"^^vocabulary:RegionalRegistryTypeVocab .

_:node1gm7uj6vjx660 rdf:first "Resume"^^vocabulary:ActionTypeVocab .

_:node1gm7uj6vjx1113 rdf:rest rdf:nil .

_:node1gm7uj6vjx660 rdf:rest _:node1gm7uj6vjx661 .

_:node1gm7uj6vjx1115 rdf:rest _:node1gm7uj6vjx1116 .

_:node1gm7uj6vjx661 rdf:first "Revert"^^vocabulary:ActionTypeVocab .

_:node1gm7uj6vjx1096 sh:or _:node1gm7uj6vjx1097 .

_:node1gm7uj6vjx661 rdf:rest _:node1gm7uj6vjx662 .

_:node1gm7uj6vjx1116 rdf:first "ARIN"^^vocabulary:RegionalRegistryTypeVocab .

observable:BotConfiguration rdfs:subClassOf observable:ObservableObject .

_:node1gm7uj6vjx1096 sh:path observable:contactPhoneScope .

_:node1gm7uj6vjx662 rdf:first "Run"^^vocabulary:ActionTypeVocab .

_:node1gm7uj6vjx1116 rdf:rest _:node1gm7uj6vjx1117 .

_:node1gm7uj6vjx662 rdf:rest _:node1gm7uj6vjx663 .

observable:ContactPhone sh:property _:node1gm7uj6vjx1096 .

_:node1gm7uj6vjx663 rdf:first "Save"^^vocabulary:ActionTypeVocab .

_:node1gm7uj6vjx1117 rdf:first "AfriNIC"^^vocabulary:RegionalRegistryTypeVocab .

_:node1gm7uj6vjx663 rdf:rest _:node1gm7uj6vjx664 .

_:node1gm7uj6vjx1117 rdf:rest _:node1gm7uj6vjx1118 .

_:node1gm7uj6vjx664 rdf:first "Scan"^^vocabulary:ActionTypeVocab .

observable:ContactPhone sh:targetClass observable:ContactPhone .

_:node1gm7uj6vjx664 rdf:rest _:node1gm7uj6vjx665 .

_:node1gm7uj6vjx1118 rdf:first "LACNIC"^^vocabulary:RegionalRegistryTypeVocab .

observable:BotConfiguration rdfs:label "BotConfiguration"@en .

_:node1gm7uj6vjx1118 rdf:rest _:node1gm7uj6vjx1119 .

_:node1gm7uj6vjx665 rdf:first "Schedule"^^vocabulary:ActionTypeVocab .

_:node1gm7uj6vjx1119 rdf:first "RIPE NCC"^^vocabulary:RegionalRegistryTypeVocab .

_:node1gm7uj6vjx665 rdf:rest _:node1gm7uj6vjx666 .

_:node1gm7uj6vjx1119 rdf:rest rdf:nil .

_:node1gm7uj6vjx666 rdf:first "Search"^^vocabulary:ActionTypeVocab .

_:node1gm7uj6vjx1112 owl:oneOf _:node1gm7uj6vjx1115 .

_:node1gm7uj6vjx666 rdf:rest _:node1gm7uj6vjx667 .

vocabulary:RegionalRegistryTypeVocab owl:equivalentClass _:node1gm7uj6vjx1112 .

_:node1gm7uj6vjx667 rdf:first "Send"^^vocabulary:ActionTypeVocab .

observable:ContactProfile a owl:Class .

_:node1gm7uj6vjx667 rdf:rest _:node1gm7uj6vjx668 .

observable:ContactProfile a sh:NodeShape .

observable:BotConfiguration rdfs:comment "A bot configuration is a set of contextual settings for a software application that runs automated tasks (scripts) over the Internet at a much higher rate than would be possible for a human alone."@en .

observable:ContactProfile rdfs:subClassOf core:UcoInherentCharacterizationThing .

_:node1gm7uj6vjx668 rdf:first "Set"^^vocabulary:ActionTypeVocab .

vocabulary:RegistryDatatypeVocab a rdfs:Datatype .

_:node1gm7uj6vjx668 rdf:rest _:node1gm7uj6vjx669 .

vocabulary:RegistryDatatypeVocab rdfs:label "Registry Datatype Vocabulary"@en-us .

_:node1gm7uj6vjx669 rdf:first "Shutdown"^^vocabulary:ActionTypeVocab .

observable:ContactProfile rdfs:label "ContactProfile"@en .

_:node1gm7uj6vjx669 rdf:rest _:node1gm7uj6vjx670 .

_:node1gm7uj6vjx1120 a rdfs:Datatype .

observable:BotConfiguration sh:targetClass observable:BotConfiguration .

observable:ContactProfile rdfs:comment "A contact profile is a grouping of characteristics unique to details for contacting a contact entity by online service."@en .

_:node1gm7uj6vjx670 rdf:first "Sleep"^^vocabulary:ActionTypeVocab .

_:node1gm7uj6vjx1120 owl:onDatatype xsd:string .

_:node1gm7uj6vjx670 rdf:rest _:node1gm7uj6vjx671 .

_:node1gm7uj6vjx1121 sh:class observable:ObservableObject .

_:node1gm7uj6vjx671 rdf:first "Snapshot"^^vocabulary:ActionTypeVocab .

_:node1gm7uj6vjx1122 rdf:first "reg_binary"^^vocabulary:RegistryDatatypeVocab .

_:node1gm7uj6vjx671 rdf:rest _:node1gm7uj6vjx672 .

_:node1gm7uj6vjx1122 rdf:rest _:node1gm7uj6vjx1123 .

_:node1gm7uj6vjx672 rdf:first "Start"^^vocabulary:ActionTypeVocab .

_:node1gm7uj6vjx1121 sh:maxCount 1 .

_:node1gm7uj6vjx672 rdf:rest _:node1gm7uj6vjx673 .

_:node1gm7uj6vjx1121 sh:nodeKind sh:IRI .

observable:BrowserBookmark a owl:Class .

_:node1gm7uj6vjx1123 rdf:first "reg_dword"^^vocabulary:RegistryDatatypeVocab .

_:node1gm7uj6vjx673 rdf:first "Stop"^^vocabulary:ActionTypeVocab .

_:node1gm7uj6vjx1123 rdf:rest _:node1gm7uj6vjx1124 .

_:node1gm7uj6vjx673 rdf:rest _:node1gm7uj6vjx674 .

_:node1gm7uj6vjx1121 sh:path observable:contactProfilePlatform .

observable:BrowserBookmark a sh:NodeShape .

observable:ContactProfile sh:property _:node1gm7uj6vjx1121 .

_:node1gm7uj6vjx674 rdf:first "Suspend"^^vocabulary:ActionTypeVocab .

_:node1gm7uj6vjx1125 sh:class observable:ObservableObject .

_:node1gm7uj6vjx674 rdf:rest _:node1gm7uj6vjx675 .

_:node1gm7uj6vjx1124 rdf:first "reg_dword_big_endian"^^vocabulary:RegistryDatatypeVocab .

_:node1gm7uj6vjx675 rdf:first "Synchronize"^^vocabulary:ActionTypeVocab .

_:node1gm7uj6vjx1124 rdf:rest _:node1gm7uj6vjx1126 .

_:node1gm7uj6vjx675 rdf:rest _:node1gm7uj6vjx676 .

_:node1gm7uj6vjx1125 sh:maxCount 1 .

observable:BrowserBookmark rdfs:subClassOf observable:ObservableObject .

_:node1gm7uj6vjx1126 rdf:first "reg_expand_sz"^^vocabulary:RegistryDatatypeVocab .

_:node1gm7uj6vjx676 rdf:first "Throw"^^vocabulary:ActionTypeVocab .

_:node1gm7uj6vjx1126 rdf:rest _:node1gm7uj6vjx1127 .

_:node1gm7uj6vjx676 rdf:rest _:node1gm7uj6vjx677 .

_:node1gm7uj6vjx1125 sh:nodeKind sh:IRI .

_:node1gm7uj6vjx677 rdf:first "Transmit"^^vocabulary:ActionTypeVocab .

_:node1gm7uj6vjx1125 sh:path observable:profile .

_:node1gm7uj6vjx677 rdf:rest _:node1gm7uj6vjx678 .

observable:ContactProfile sh:property _:node1gm7uj6vjx1125 .

_:node1gm7uj6vjx678 rdf:first "Unblock"^^vocabulary:ActionTypeVocab .

_:node1gm7uj6vjx1127 rdf:first "reg_full_resource_descriptor"^^vocabulary:RegistryDatatypeVocab .

_:node1gm7uj6vjx678 rdf:rest _:node1gm7uj6vjx679 .

_:node1gm7uj6vjx1127 rdf:rest _:node1gm7uj6vjx1128 .

observable:BrowserBookmark rdfs:label "BrowserBookmark"@en .

observable:ContactProfile sh:targetClass observable:ContactProfile .

_:node1gm7uj6vjx679 rdf:first "Unhide"^^vocabulary:ActionTypeVocab .

_:node1gm7uj6vjx1128 rdf:first "reg_invalid_type"^^vocabulary:RegistryDatatypeVocab .

_:node1gm7uj6vjx679 rdf:rest _:node1gm7uj6vjx680 .

_:node1gm7uj6vjx1128 rdf:rest _:node1gm7uj6vjx1129 .

_:node1gm7uj6vjx680 rdf:first "Unhook"^^vocabulary:ActionTypeVocab .

observable:ContactSIP a owl:Class .

_:node1gm7uj6vjx680 rdf:rest _:node1gm7uj6vjx681 .

observable:ContactSIP a sh:NodeShape .

_:node1gm7uj6vjx681 rdf:first "Uninstall"^^vocabulary:ActionTypeVocab .

_:node1gm7uj6vjx1129 rdf:first "reg_link"^^vocabulary:RegistryDatatypeVocab .

_:node1gm7uj6vjx681 rdf:rest _:node1gm7uj6vjx682 .

_:node1gm7uj6vjx1129 rdf:rest _:node1gm7uj6vjx1130 .

_:node1gm7uj6vjx682 rdf:first "Unload"^^vocabulary:ActionTypeVocab .

observable:ContactSIP rdfs:subClassOf core:UcoInherentCharacterizationThing .

_:node1gm7uj6vjx682 rdf:rest _:node1gm7uj6vjx683 .

_:node1gm7uj6vjx1130 rdf:first "reg_multi_sz"^^vocabulary:RegistryDatatypeVocab .

_:node1gm7uj6vjx683 rdf:first "Unlock"^^vocabulary:ActionTypeVocab .

_:node1gm7uj6vjx1130 rdf:rest _:node1gm7uj6vjx1131 .

_:node1gm7uj6vjx683 rdf:rest _:node1gm7uj6vjx684 .

observable:ContactSIP rdfs:label "ContactSIP"@en .

_:node1gm7uj6vjx684 rdf:first "Unmap"^^vocabulary:ActionTypeVocab .

_:node1gm7uj6vjx1131 rdf:first "reg_none"^^vocabulary:RegistryDatatypeVocab .

observable:BrowserBookmark rdfs:comment "A browser bookmark is a saved shortcut that directs a WWW (World Wide Web) browser software program to a particular WWW accessible resource. [based on https://techterms.com/definition/bookmark]"@en .

_:node1gm7uj6vjx1131 rdf:rest _:node1gm7uj6vjx1132 .

_:node1gm7uj6vjx684 rdf:rest _:node1gm7uj6vjx685 .

observable:ContactSIP rdfs:comment "A contact SIP is a grouping of characteristics unique to details for contacting a contact entity by Session Initiation Protocol (SIP)."@en .

_:node1gm7uj6vjx685 rdf:first "Unpack"^^vocabulary:ActionTypeVocab .

_:node1gm7uj6vjx1132 rdf:first "reg_qword"^^vocabulary:RegistryDatatypeVocab .

_:node1gm7uj6vjx685 rdf:rest _:node1gm7uj6vjx686 .

_:node1gm7uj6vjx1132 rdf:rest _:node1gm7uj6vjx1133 .

observable:BrowserBookmark sh:targetClass observable:BrowserBookmark .

_:node1gm7uj6vjx1133 rdf:first "reg_resource_list"^^vocabulary:RegistryDatatypeVocab .

_:node1gm7uj6vjx686 rdf:first "Update"^^vocabulary:ActionTypeVocab .

_:node1gm7uj6vjx1133 rdf:rest _:node1gm7uj6vjx1135 .

_:node1gm7uj6vjx686 rdf:rest _:node1gm7uj6vjx687 .

_:node1gm7uj6vjx1134 sh:class observable:ObservableObject .

_:node1gm7uj6vjx687 rdf:first "Upgrade"^^vocabulary:ActionTypeVocab .

_:node1gm7uj6vjx1135 rdf:first "reg_resource_requirements_list"^^vocabulary:RegistryDatatypeVocab .

_:node1gm7uj6vjx687 rdf:rest _:node1gm7uj6vjx688 .

_:node1gm7uj6vjx1135 rdf:rest _:node1gm7uj6vjx1136 .

_:node1gm7uj6vjx688 rdf:first "Upload"^^vocabulary:ActionTypeVocab .

_:node1gm7uj6vjx1134 sh:maxCount 1 .

_:node1gm7uj6vjx688 rdf:rest _:node1gm7uj6vjx689 .

_:node1gm7uj6vjx1134 sh:nodeKind sh:IRI .

observable:BrowserBookmarkFacet a owl:Class .

_:node1gm7uj6vjx1136 rdf:first "reg_sz"^^vocabulary:RegistryDatatypeVocab .

observable:BrowserBookmarkFacet a sh:NodeShape .

_:node1gm7uj6vjx1136 rdf:rest rdf:nil .

_:node1gm7uj6vjx689 rdf:first "Wipe/Destroy/Purge"^^vocabulary:ActionTypeVocab .

_:node1gm7uj6vjx1120 owl:oneOf _:node1gm7uj6vjx1122 .

_:node1gm7uj6vjx689 rdf:rest _:node1gm7uj6vjx690 .

vocabulary:RegistryDatatypeVocab owl:equivalentClass _:node1gm7uj6vjx1120 .

_:node1gm7uj6vjx690 rdf:first "Write"^^vocabulary:ActionTypeVocab .

_:node1gm7uj6vjx1134 sh:path observable:sipAddress .

_:node1gm7uj6vjx690 rdf:rest rdf:nil .

observable:ContactSIP sh:property _:node1gm7uj6vjx1134 .

_:node1gm7uj6vjx564 owl:oneOf _:node1gm7uj6vjx566 .

_:node1gm7uj6vjx1137 sh:datatype vocabulary:ContactSIPScopeVocab .

vocabulary:ActionTypeVocab owl:equivalentClass _:node1gm7uj6vjx564 .

vocabulary:SIMFormVocab a rdfs:Datatype .

observable:BrowserBookmarkFacet rdfs:subClassOf core:Facet .

_:node1gm7uj6vjx1137 sh:message "Value is outside the default vocabulary ContactSIPScopeVocab." .

vocabulary:BitnessVocab a rdfs:Datatype .

_:node1gm7uj6vjx1137 sh:path observable:contactSIPScope .

observable:BrowserBookmarkFacet rdfs:label "BrowserBookmarkFacet"@en .

vocabulary:SIMFormVocab rdfs:label "SIM Form Vocabulary"@en-us .

vocabulary:BitnessVocab rdfs:label "Bitness Vocabulary"@en-us .

_:node1gm7uj6vjx1137 sh:severity sh:Info .

vocabulary:BitnessVocab rdfs:comment "Defines an open-vocabulary of word sizes that define classes of operating systems."@en .

observable:ContactSIP sh:property _:node1gm7uj6vjx1137 .

_:node1gm7uj6vjx691 a rdfs:Datatype .

vocabulary:SIMFormVocab rdfs:comment "Defines an open-vocabulary of common SIM card form factors."@en .

_:node1gm7uj6vjx691 owl:onDatatype xsd:string .

_:node1gm7uj6vjx1138 sh:maxCount 1 .

_:node1gm7uj6vjx692 rdf:first "32"^^vocabulary:BitnessVocab .

_:node1gm7uj6vjx1138 sh:nodeKind sh:Literal .

_:node1gm7uj6vjx692 rdf:rest _:node1gm7uj6vjx693 .

_:node1gm7uj6vjx1139 a rdfs:Datatype .

observable:BrowserBookmarkFacet rdfs:comment "A browser bookmark facet is a grouping of characteristics unique to a saved shortcut that directs a WWW (World Wide Web) browser software program to a particular WWW accessible resource. [based on https://techterms.com/definition/bookmark]"@en .

_:node1gm7uj6vjx1139 owl:onDatatype xsd:string .

_:node1gm7uj6vjx693 rdf:first "64"^^vocabulary:BitnessVocab .

_:node1gm7uj6vjx1141 sh:datatype vocabulary:ContactSIPScopeVocab .

_:node1gm7uj6vjx693 rdf:rest rdf:nil .

_:node1gm7uj6vjx1140 rdf:first _:node1gm7uj6vjx1141 .

_:node1gm7uj6vjx691 owl:oneOf _:node1gm7uj6vjx692 .

_:node1gm7uj6vjx1140 rdf:rest _:node1gm7uj6vjx1143 .

vocabulary:BitnessVocab owl:equivalentClass _:node1gm7uj6vjx691 .

_:node1gm7uj6vjx1142 rdf:first "Full-size SIM"^^vocabulary:SIMFormVocab .

vocabulary:CharacterEncodingVocab a rdfs:Datatype .

_:node1gm7uj6vjx1144 sh:datatype xsd:string .

vocabulary:CharacterEncodingVocab rdfs:label "Character Encoding Vocabulary"@en-us .

_:node1gm7uj6vjx1142 rdf:rest _:node1gm7uj6vjx1145 .

_:node1gm7uj6vjx694 sh:class observable:ObservableObject .

_:node1gm7uj6vjx1143 rdf:first _:node1gm7uj6vjx1144 .

vocabulary:CharacterEncodingVocab rdfs:comment "Defines an open-vocabulary of character encodings."@en .

_:node1gm7uj6vjx1143 rdf:rest rdf:nil .

_:node1gm7uj6vjx694 sh:maxCount 1 .

_:node1gm7uj6vjx1138 sh:or _:node1gm7uj6vjx1140 .

_:node1gm7uj6vjx695 a rdfs:Datatype .

_:node1gm7uj6vjx1145 rdf:first "Micro SIM"^^vocabulary:SIMFormVocab .

_:node1gm7uj6vjx694 sh:nodeKind sh:IRI .

_:node1gm7uj6vjx1138 sh:path observable:contactSIPScope .

_:node1gm7uj6vjx695 owl:onDatatype xsd:string .

observable:ContactSIP sh:property _:node1gm7uj6vjx1138 .

_:node1gm7uj6vjx694 sh:path observable:application .

_:node1gm7uj6vjx1145 rdf:rest _:node1gm7uj6vjx1146 .

observable:BrowserBookmarkFacet sh:property _:node1gm7uj6vjx694 .

_:node1gm7uj6vjx1146 rdf:first "Nano SIM"^^vocabulary:SIMFormVocab .

_:node1gm7uj6vjx696 rdf:first "ASCII"^^vocabulary:CharacterEncodingVocab .

_:node1gm7uj6vjx1147 sh:message "Value is not member of the vocabulary ContactSIPScopeVocab." .

_:node1gm7uj6vjx696 rdf:rest _:node1gm7uj6vjx698 .

_:node1gm7uj6vjx1146 rdf:rest rdf:nil .

_:node1gm7uj6vjx698 rdf:first "UTF-16"^^vocabulary:CharacterEncodingVocab .

_:node1gm7uj6vjx1139 owl:oneOf _:node1gm7uj6vjx1142 .

_:node1gm7uj6vjx697 sh:datatype xsd:anyURI .

vocabulary:SIMFormVocab owl:equivalentClass _:node1gm7uj6vjx1139 .

_:node1gm7uj6vjx698 rdf:rest _:node1gm7uj6vjx699 .

_:node1gm7uj6vjx1149 sh:datatype vocabulary:ContactSIPScopeVocab .

_:node1gm7uj6vjx697 sh:nodeKind sh:Literal .

vocabulary:SIMTypeVocab a rdfs:Datatype .

_:node1gm7uj6vjx699 rdf:first "UTF-32"^^vocabulary:CharacterEncodingVocab .

vocabulary:SIMTypeVocab rdfs:label "SIM Type Vocabulary"@en-us .

_:node1gm7uj6vjx699 rdf:rest _:node1gm7uj6vjx700 .

_:node1gm7uj6vjx1150 rdf:first "home"^^vocabulary:ContactSIPScopeVocab .

_:node1gm7uj6vjx700 rdf:first "UTF-8"^^vocabulary:CharacterEncodingVocab .

_:node1gm7uj6vjx1150 rdf:rest _:node1gm7uj6vjx1151 .

_:node1gm7uj6vjx700 rdf:rest _:node1gm7uj6vjx701 .

vocabulary:SIMTypeVocab rdfs:comment "Defines an open-vocabulary of common SIM card types."@en .

_:node1gm7uj6vjx697 sh:path observable:urlTargeted .

_:node1gm7uj6vjx1152 a rdfs:Datatype .

observable:BrowserBookmarkFacet sh:property _:node1gm7uj6vjx697 .

_:node1gm7uj6vjx1152 owl:onDatatype xsd:string .

_:node1gm7uj6vjx701 rdf:first "Windows-1250"^^vocabulary:CharacterEncodingVocab .

_:node1gm7uj6vjx1151 rdf:first "work"^^vocabulary:ContactSIPScopeVocab .

_:node1gm7uj6vjx701 rdf:rest _:node1gm7uj6vjx703 .

_:node1gm7uj6vjx1151 rdf:rest _:node1gm7uj6vjx1154 .

_:node1gm7uj6vjx702 sh:datatype xsd:dateTime .

_:node1gm7uj6vjx1153 rdf:first "SIM"^^vocabulary:SIMTypeVocab .

_:node1gm7uj6vjx703 rdf:first "Windows-1251"^^vocabulary:CharacterEncodingVocab .

_:node1gm7uj6vjx1153 rdf:rest _:node1gm7uj6vjx1155 .

_:node1gm7uj6vjx703 rdf:rest _:node1gm7uj6vjx704 .

_:node1gm7uj6vjx1155 rdf:first "UICC"^^vocabulary:SIMTypeVocab .

_:node1gm7uj6vjx704 rdf:first "Windows-1252"^^vocabulary:CharacterEncodingVocab .

_:node1gm7uj6vjx1155 rdf:rest _:node1gm7uj6vjx1156 .

_:node1gm7uj6vjx704 rdf:rest _:node1gm7uj6vjx705 .

_:node1gm7uj6vjx1154 rdf:first "school"^^vocabulary:ContactSIPScopeVocab .

_:node1gm7uj6vjx702 sh:maxCount 1 .

_:node1gm7uj6vjx1154 rdf:rest rdf:nil .

_:node1gm7uj6vjx702 sh:nodeKind sh:Literal .

_:node1gm7uj6vjx1149 sh:in _:node1gm7uj6vjx1150 .

_:node1gm7uj6vjx705 rdf:first "Windows-1253"^^vocabulary:CharacterEncodingVocab .

_:node1gm7uj6vjx1148 rdf:first _:node1gm7uj6vjx1149 .

_:node1gm7uj6vjx705 rdf:rest _:node1gm7uj6vjx706 .

_:node1gm7uj6vjx1148 rdf:rest _:node1gm7uj6vjx1157 .

_:node1gm7uj6vjx702 sh:path observable:accessedTime .

_:node1gm7uj6vjx1156 rdf:first "USIM"^^vocabulary:SIMTypeVocab .

observable:BrowserBookmarkFacet sh:property _:node1gm7uj6vjx702 .

_:node1gm7uj6vjx1156 rdf:rest rdf:nil .

_:node1gm7uj6vjx706 rdf:first "Windows-1254"^^vocabulary:CharacterEncodingVocab .

_:node1gm7uj6vjx1152 owl:oneOf _:node1gm7uj6vjx1153 .

_:node1gm7uj6vjx706 rdf:rest _:node1gm7uj6vjx707 .

vocabulary:SIMTypeVocab owl:equivalentClass _:node1gm7uj6vjx1152 .

_:node1gm7uj6vjx707 rdf:first "Windows-1255"^^vocabulary:CharacterEncodingVocab .

_:node1gm7uj6vjx1158 sh:datatype xsd:string .

_:node1gm7uj6vjx707 rdf:rest _:node1gm7uj6vjx709 .

_:node1gm7uj6vjx1157 rdf:first _:node1gm7uj6vjx1158 .

_:node1gm7uj6vjx708 sh:datatype xsd:dateTime .

vocabulary:TaskActionTypeVocab a rdfs:Datatype .

_:node1gm7uj6vjx709 rdf:first "Windows-1256"^^vocabulary:CharacterEncodingVocab .

_:node1gm7uj6vjx1157 rdf:rest rdf:nil .

_:node1gm7uj6vjx709 rdf:rest _:node1gm7uj6vjx710 .

_:node1gm7uj6vjx1147 sh:or _:node1gm7uj6vjx1148 .

_:node1gm7uj6vjx708 sh:maxCount 1 .

vocabulary:TaskActionTypeVocab rdfs:label "Task Action Type Vocabulary"@en-us .

_:node1gm7uj6vjx710 rdf:first "Windows-1257"^^vocabulary:CharacterEncodingVocab .

_:node1gm7uj6vjx1147 sh:path observable:contactSIPScope .

_:node1gm7uj6vjx710 rdf:rest _:node1gm7uj6vjx711 .

observable:ContactSIP sh:property _:node1gm7uj6vjx1147 .

_:node1gm7uj6vjx708 sh:nodeKind sh:Literal .

vocabulary:TaskActionTypeVocab rdfs:comment "Defines an open-vocabulary of task action types. See also: http://msdn.microsoft.com/en-us/library/windows/desktop/aa380596(v=vs.85).aspx."@en .

_:node1gm7uj6vjx711 rdf:first "Windows-1258"^^vocabulary:CharacterEncodingVocab .

observable:ContactSIP sh:targetClass observable:ContactSIP .

_:node1gm7uj6vjx711 rdf:rest rdf:nil .

_:node1gm7uj6vjx1159 a rdfs:Datatype .

_:node1gm7uj6vjx695 owl:oneOf _:node1gm7uj6vjx696 .

_:node1gm7uj6vjx1159 owl:onDatatype xsd:string .

vocabulary:CharacterEncodingVocab owl:equivalentClass _:node1gm7uj6vjx695 .

_:node1gm7uj6vjx1160 rdf:first "TASK_ACTION_COM_HANDLER"^^vocabulary:TaskActionTypeVocab .

_:node1gm7uj6vjx708 sh:path observable:modifiedTime .

_:node1gm7uj6vjx1160 rdf:rest _:node1gm7uj6vjx1161 .

observable:BrowserBookmarkFacet sh:property _:node1gm7uj6vjx708 .

observable:ContactURL a owl:Class .

vocabulary:ContactAddressScopeVocab a rdfs:Datatype .

observable:ContactURL a sh:NodeShape .

_:node1gm7uj6vjx712 sh:datatype xsd:dateTime .

_:node1gm7uj6vjx1161 rdf:first "TASK_ACTION_EXEC"^^vocabulary:TaskActionTypeVocab .

vocabulary:ContactAddressScopeVocab rdfs:label "Contact Address Scope Vocabulary"@en-us .

_:node1gm7uj6vjx1161 rdf:rest _:node1gm7uj6vjx1162 .

_:node1gm7uj6vjx712 sh:maxCount 1 .

_:node1gm7uj6vjx1162 rdf:first "TASK_ACTION_SEND_EMAIL"^^vocabulary:TaskActionTypeVocab .

_:node1gm7uj6vjx712 sh:nodeKind sh:Literal .

_:node1gm7uj6vjx1162 rdf:rest _:node1gm7uj6vjx1163 .

vocabulary:ContactAddressScopeVocab rdfs:comment "Defines an open-vocabulary of scopes for address entries of digital contacts."@en .

observable:ContactURL rdfs:subClassOf core:UcoInherentCharacterizationThing .

_:node1gm7uj6vjx713 a rdfs:Datatype .

_:node1gm7uj6vjx1163 rdf:first "TASK_ACTION_SHOW_MESSAGE"^^vocabulary:TaskActionTypeVocab .

_:node1gm7uj6vjx713 owl:onDatatype xsd:string .

_:node1gm7uj6vjx1163 rdf:rest rdf:nil .

_:node1gm7uj6vjx712 sh:path observable:observableCreatedTime .

_:node1gm7uj6vjx1159 owl:oneOf _:node1gm7uj6vjx1160 .

observable:BrowserBookmarkFacet sh:property _:node1gm7uj6vjx712 .

vocabulary:TaskActionTypeVocab owl:equivalentClass _:node1gm7uj6vjx1159 .

_:node1gm7uj6vjx714 rdf:first "home"^^vocabulary:ContactAddressScopeVocab .

observable:ContactURL rdfs:label "ContactURL"@en .

_:node1gm7uj6vjx715 sh:datatype xsd:integer .

vocabulary:TaskFlagVocab a rdfs:Datatype .

_:node1gm7uj6vjx714 rdf:rest _:node1gm7uj6vjx716 .

observable:ContactURL rdfs:comment "A contact URL is a grouping of characteristics unique to details for contacting a contact entity by Uniform Resource Locator (URL)."@en .

_:node1gm7uj6vjx716 rdf:first "work"^^vocabulary:ContactAddressScopeVocab .

vocabulary:TaskFlagVocab rdfs:label "Task Flag Vocabulary"@en-us .

_:node1gm7uj6vjx716 rdf:rest _:node1gm7uj6vjx717 .

_:node1gm7uj6vjx1164 sh:class observable:ObservableObject .

_:node1gm7uj6vjx715 sh:maxCount 1 .

_:node1gm7uj6vjx1164 sh:maxCount 1 .

_:node1gm7uj6vjx717 rdf:first "school"^^vocabulary:ContactAddressScopeVocab .

_:node1gm7uj6vjx1164 sh:nodeKind sh:IRI .

_:node1gm7uj6vjx717 rdf:rest rdf:nil .

vocabulary:TaskFlagVocab rdfs:comment "Defines an open-vocabulary of the run flags for a task scheduler task. See also: http://msdn.microsoft.com/en-us/library/windows/desktop/aa381283(v=vs.85).aspx See Also: http://msdn.microsoft.com/en-us/library/microsoft.office.excel.server.addins.computecluster.taskscheduler.taskflags(v=office.12).aspx."@en .

_:node1gm7uj6vjx713 owl:oneOf _:node1gm7uj6vjx714 .

_:node1gm7uj6vjx1164 sh:path observable:url .

vocabulary:ContactAddressScopeVocab owl:equivalentClass _:node1gm7uj6vjx713 .

observable:ContactURL sh:property _:node1gm7uj6vjx1164 .

_:node1gm7uj6vjx715 sh:nodeKind sh:Literal .

_:node1gm7uj6vjx1165 a rdfs:Datatype .

vocabulary:ContactEmailScopeVocab a rdfs:Datatype .

_:node1gm7uj6vjx1165 owl:onDatatype xsd:string .

_:node1gm7uj6vjx715 sh:path observable:visitCount .

_:node1gm7uj6vjx1166 sh:datatype vocabulary:ContactURLScopeVocab .

vocabulary:ContactEmailScopeVocab rdfs:label "Contact Email Scope Vocabulary"@en-us .

_:node1gm7uj6vjx1166 sh:message "Value is outside the default vocabulary ContactURLScopeVocab." .

observable:BrowserBookmarkFacet sh:property _:node1gm7uj6vjx715 .

_:node1gm7uj6vjx1167 rdf:first "TASK_FLAG_DELETE_WHEN_DONE"^^vocabulary:TaskFlagVocab .

_:node1gm7uj6vjx718 sh:datatype xsd:string .

_:node1gm7uj6vjx1167 rdf:rest _:node1gm7uj6vjx1168 .

vocabulary:ContactEmailScopeVocab rdfs:comment "Defines an open-vocabulary of scopes for email entries of digital contacts."@en .

_:node1gm7uj6vjx1166 sh:path observable:contactURLScope .

_:node1gm7uj6vjx719 a rdfs:Datatype .

_:node1gm7uj6vjx1168 rdf:first "TASK_FLAG_DISABLED"^^vocabulary:TaskFlagVocab .

_:node1gm7uj6vjx719 owl:onDatatype xsd:string .

_:node1gm7uj6vjx1168 rdf:rest _:node1gm7uj6vjx1169 .

_:node1gm7uj6vjx718 sh:maxCount 1 .

_:node1gm7uj6vjx1166 sh:severity sh:Info .

_:node1gm7uj6vjx720 rdf:first "home"^^vocabulary:ContactEmailScopeVocab .

observable:ContactURL sh:property _:node1gm7uj6vjx1166 .

_:node1gm7uj6vjx718 sh:nodeKind sh:Literal .

_:node1gm7uj6vjx1170 sh:maxCount 1 .

_:node1gm7uj6vjx720 rdf:rest _:node1gm7uj6vjx721 .

_:node1gm7uj6vjx1170 sh:nodeKind sh:Literal .

_:node1gm7uj6vjx721 rdf:first "work"^^vocabulary:ContactEmailScopeVocab .

_:node1gm7uj6vjx1169 rdf:first "TASK_FLAG_DONT_START_IF_ON_BATTERIES"^^vocabulary:TaskFlagVocab .

_:node1gm7uj6vjx721 rdf:rest _:node1gm7uj6vjx722 .

_:node1gm7uj6vjx1169 rdf:rest _:node1gm7uj6vjx1173 .

_:node1gm7uj6vjx718 sh:path observable:bookmarkPath .

_:node1gm7uj6vjx1172 sh:datatype vocabulary:ContactURLScopeVocab .

observable:BrowserBookmarkFacet sh:property _:node1gm7uj6vjx718 .

_:node1gm7uj6vjx1171 rdf:first _:node1gm7uj6vjx1172 .

_:node1gm7uj6vjx722 rdf:first "school"^^vocabulary:ContactEmailScopeVocab .

_:node1gm7uj6vjx1171 rdf:rest _:node1gm7uj6vjx1174 .

_:node1gm7uj6vjx722 rdf:rest _:node1gm7uj6vjx723 .

_:node1gm7uj6vjx1173 rdf:first "TASK_FLAG_HIDDEN"^^vocabulary:TaskFlagVocab .

_:node1gm7uj6vjx723 rdf:first "cloud"^^vocabulary:ContactEmailScopeVocab .

_:node1gm7uj6vjx1173 rdf:rest _:node1gm7uj6vjx1176 .

_:node1gm7uj6vjx723 rdf:rest rdf:nil .

_:node1gm7uj6vjx1175 sh:datatype xsd:string .

_:node1gm7uj6vjx719 owl:oneOf _:node1gm7uj6vjx720 .

_:node1gm7uj6vjx1174 rdf:first _:node1gm7uj6vjx1175 .

observable:BrowserBookmarkFacet sh:targetClass observable:BrowserBookmarkFacet .

_:node1gm7uj6vjx1174 rdf:rest rdf:nil .

vocabulary:ContactEmailScopeVocab owl:equivalentClass _:node1gm7uj6vjx719 .

_:node1gm7uj6vjx1170 sh:or _:node1gm7uj6vjx1171 .

vocabulary:ContactPhoneScopeVocab a rdfs:Datatype .

_:node1gm7uj6vjx1176 rdf:first "TASK_FLAG_INTERACTIVE"^^vocabulary:TaskFlagVocab .

observable:BrowserCookie a owl:Class .

_:node1gm7uj6vjx1176 rdf:rest _:node1gm7uj6vjx1177 .

observable:BrowserCookie a sh:NodeShape .

_:node1gm7uj6vjx1170 sh:path observable:contactURLScope .

vocabulary:ContactPhoneScopeVocab rdfs:label "Contact Phone Scope Vocabulary"@en-us .

observable:ContactURL sh:property _:node1gm7uj6vjx1170 .

observable:BrowserCookie rdfs:subClassOf observable:ObservableObject .

_:node1gm7uj6vjx1178 sh:message "Value is not member of the vocabulary ContactURLScopeVocab." .

vocabulary:ContactPhoneScopeVocab rdfs:comment "Defines an open-vocabulary of scopes for phone entries of digital contacts."@en .

_:node1gm7uj6vjx1177 rdf:first "TASK_FLAG_KILL_IF_GOING_ON_BATTERIES"^^vocabulary:TaskFlagVocab .

_:node1gm7uj6vjx724 a rdfs:Datatype .

_:node1gm7uj6vjx1177 rdf:rest _:node1gm7uj6vjx1179 .

_:node1gm7uj6vjx724 owl:onDatatype xsd:string .

_:node1gm7uj6vjx1179 rdf:first "TASK_FLAG_KILL_ON_IDLE_END"^^vocabulary:TaskFlagVocab .

observable:BrowserCookie rdfs:label "BrowserCookie"@en .

_:node1gm7uj6vjx1179 rdf:rest _:node1gm7uj6vjx1182 .

_:node1gm7uj6vjx725 rdf:first "home"^^vocabulary:ContactPhoneScopeVocab .

_:node1gm7uj6vjx1181 sh:datatype vocabulary:ContactURLScopeVocab .

_:node1gm7uj6vjx725 rdf:rest _:node1gm7uj6vjx726 .

_:node1gm7uj6vjx1182 rdf:first "TASK_FLAG_RESTART_ON_IDLE_RESUME"^^vocabulary:TaskFlagVocab .

_:node1gm7uj6vjx726 rdf:first "work"^^vocabulary:ContactPhoneScopeVocab .

_:node1gm7uj6vjx1182 rdf:rest _:node1gm7uj6vjx1184 .

_:node1gm7uj6vjx726 rdf:rest _:node1gm7uj6vjx727 .

_:node1gm7uj6vjx1183 rdf:first "home"^^vocabulary:ContactURLScopeVocab .

_:node1gm7uj6vjx727 rdf:first "school"^^vocabulary:ContactPhoneScopeVocab .

_:node1gm7uj6vjx1184 rdf:first "TASK_FLAG_RUN_IF_CONNECTED_TO_INTERNET"^^vocabulary:TaskFlagVocab .

_:node1gm7uj6vjx727 rdf:rest _:node1gm7uj6vjx728 .

_:node1gm7uj6vjx1183 rdf:rest _:node1gm7uj6vjx1185 .

observable:BrowserCookie rdfs:comment "A browser cookie is a piece of of data sent from a website and stored on the user's computer by the user's web browser while the user is browsing. [based on https://en.wikipedia.org/wiki/HTTP_cookie]"@en .

_:node1gm7uj6vjx1184 rdf:rest _:node1gm7uj6vjx1186 .

_:node1gm7uj6vjx728 rdf:first "mobile"^^vocabulary:ContactPhoneScopeVocab .

_:node1gm7uj6vjx1186 rdf:first "TASK_FLAG_RUN_ONLY_IF_LOGGED_ON"^^vocabulary:TaskFlagVocab .

observable:BrowserCookie sh:targetClass observable:BrowserCookie .

_:node1gm7uj6vjx1185 rdf:first "work"^^vocabulary:ContactURLScopeVocab .

_:node1gm7uj6vjx728 rdf:rest _:node1gm7uj6vjx729 .

_:node1gm7uj6vjx1186 rdf:rest _:node1gm7uj6vjx1187 .

_:node1gm7uj6vjx729 rdf:first "main"^^vocabulary:ContactPhoneScopeVocab .

_:node1gm7uj6vjx1185 rdf:rest _:node1gm7uj6vjx1188 .

observable:BrowserCookieFacet a owl:Class .

_:node1gm7uj6vjx1187 rdf:first "TASK_FLAG_START_ONLY_IF_IDLE"^^vocabulary:TaskFlagVocab .

observable:BrowserCookieFacet a sh:NodeShape .

_:node1gm7uj6vjx1187 rdf:rest _:node1gm7uj6vjx1189 .

_:node1gm7uj6vjx729 rdf:rest _:node1gm7uj6vjx730 .

_:node1gm7uj6vjx1188 rdf:first "school"^^vocabulary:ContactURLScopeVocab .

observable:BrowserCookieFacet rdfs:subClassOf core:Facet .

_:node1gm7uj6vjx1188 rdf:rest _:node1gm7uj6vjx1190 .

_:node1gm7uj6vjx730 rdf:first "home fax"^^vocabulary:ContactPhoneScopeVocab .

_:node1gm7uj6vjx1189 rdf:first "TASK_FLAG_SYSTEM_REQUIRED"^^vocabulary:TaskFlagVocab .

_:node1gm7uj6vjx730 rdf:rest _:node1gm7uj6vjx731 .

_:node1gm7uj6vjx1189 rdf:rest _:node1gm7uj6vjx1191 .

observable:BrowserCookieFacet rdfs:label "BrowserCookieFacet"@en .

_:node1gm7uj6vjx1190 rdf:first "homepage"^^vocabulary:ContactURLScopeVocab .

_:node1gm7uj6vjx731 rdf:first "work fax"^^vocabulary:ContactPhoneScopeVocab .

_:node1gm7uj6vjx1190 rdf:rest rdf:nil .

_:node1gm7uj6vjx731 rdf:rest _:node1gm7uj6vjx732 .

_:node1gm7uj6vjx1181 sh:in _:node1gm7uj6vjx1183 .

_:node1gm7uj6vjx732 rdf:first "pager"^^vocabulary:ContactPhoneScopeVocab .

_:node1gm7uj6vjx1180 rdf:first _:node1gm7uj6vjx1181 .

_:node1gm7uj6vjx732 rdf:rest rdf:nil .

_:node1gm7uj6vjx724 owl:oneOf _:node1gm7uj6vjx725 .

_:node1gm7uj6vjx1180 rdf:rest _:node1gm7uj6vjx1192 .

vocabulary:ContactPhoneScopeVocab owl:equivalentClass _:node1gm7uj6vjx724 .

_:node1gm7uj6vjx1191 rdf:first "TASK_FLAG_ZERO"^^vocabulary:TaskFlagVocab .

vocabulary:ContactSIPScopeVocab a rdfs:Datatype .

_:node1gm7uj6vjx1191 rdf:rest rdf:nil .

observable:BrowserCookieFacet rdfs:comment "A browser cookie facet is a grouping of characteristics unique to a piece of data sent from a website and stored on the user's computer by the user's web browser while the user is browsing. [based on https://en.wikipedia.org/wiki/HTTP_cookie]"@en .

_:node1gm7uj6vjx1165 owl:oneOf _:node1gm7uj6vjx1167 .

_:node1gm7uj6vjx733 sh:class observable:ObservableObject .

vocabulary:TaskFlagVocab owl:equivalentClass _:node1gm7uj6vjx1165 .

vocabulary:ContactSIPScopeVocab rdfs:label "Contact SIP Scope Vocabulary"@en-us .

_:node1gm7uj6vjx1193 sh:datatype xsd:string .

_:node1gm7uj6vjx733 sh:maxCount 1 ;
	sh:nodeKind sh:IRI .

vocabulary:ContactSIPScopeVocab rdfs:comment "Defines an open-vocabulary of scopes for Session Initiation Protocol (SIP) entries of digital contacts."@en .

_:node1gm7uj6vjx733 sh:path observable:application .

observable:BrowserCookieFacet sh:property _:node1gm7uj6vjx733 .

_:node1gm7uj6vjx1192 rdf:first _:node1gm7uj6vjx1193 .

_:node1gm7uj6vjx734 sh:class observable:ObservableObject .

_:node1gm7uj6vjx1192 rdf:rest rdf:nil .

_:node1gm7uj6vjx735 a rdfs:Datatype .

_:node1gm7uj6vjx1178 sh:or _:node1gm7uj6vjx1180 .

_:node1gm7uj6vjx734 sh:maxCount 1 .

_:node1gm7uj6vjx1178 sh:path observable:contactURLScope .

_:node1gm7uj6vjx735 owl:onDatatype xsd:string .

observable:ContactURL sh:property _:node1gm7uj6vjx1178 .

_:node1gm7uj6vjx734 sh:nodeKind sh:IRI .

vocabulary:TaskPriorityVocab a rdfs:Datatype .

_:node1gm7uj6vjx734 sh:path observable:cookieDomain .

observable:ContactURL sh:targetClass observable:ContactURL .

observable:BrowserCookieFacet sh:property _:node1gm7uj6vjx734 .

observable:ContentData a owl:Class .

_:node1gm7uj6vjx736 rdf:first "home"^^vocabulary:ContactSIPScopeVocab .

vocabulary:TaskPriorityVocab rdfs:label "Task Priority Vocabulary"@en-us .

_:node1gm7uj6vjx736 rdf:rest _:node1gm7uj6vjx738 .

observable:ContentData a sh:NodeShape .

_:node1gm7uj6vjx737 sh:datatype xsd:boolean .

observable:ContentData rdfs:subClassOf observable:ObservableObject .

_:node1gm7uj6vjx737 sh:maxCount 1 .

vocabulary:TaskPriorityVocab rdfs:comment "Defines an open-vocabulary of the priority levels of task scheduler tasks. See also: http://msdn.microsoft.com/en-us/library/windows/desktop/aa383512(v=vs.85).aspx."@en .

_:node1gm7uj6vjx738 rdf:first "work"^^vocabulary:ContactSIPScopeVocab .

observable:ContentData rdfs:label "ContentData"@en .

_:node1gm7uj6vjx738 rdf:rest _:node1gm7uj6vjx739 .

_:node1gm7uj6vjx1194 a rdfs:Datatype .

_:node1gm7uj6vjx737 sh:nodeKind sh:Literal .

observable:ContentData rdfs:comment "Content data is a block of digital data."@en .

_:node1gm7uj6vjx737 sh:path observable:isSecure .

_:node1gm7uj6vjx1194 owl:onDatatype xsd:string .

observable:BrowserCookieFacet sh:property _:node1gm7uj6vjx737 .

observable:ContentData sh:targetClass observable:ContentData .

_:node1gm7uj6vjx739 rdf:first "school"^^vocabulary:ContactSIPScopeVocab .

observable:ContentDataFacet a owl:Class .

_:node1gm7uj6vjx739 rdf:rest rdf:nil .

observable:ContentDataFacet a sh:NodeShape .

_:node1gm7uj6vjx735 owl:oneOf _:node1gm7uj6vjx736 .

_:node1gm7uj6vjx1195 rdf:first "ABOVE_NORMAL_PRIORITY_CLASS"^^vocabulary:TaskPriorityVocab .

vocabulary:ContactSIPScopeVocab owl:equivalentClass _:node1gm7uj6vjx735 .

_:node1gm7uj6vjx1195 rdf:rest _:node1gm7uj6vjx1196 .

_:node1gm7uj6vjx740 sh:datatype xsd:dateTime .

observable:ContentDataFacet rdfs:subClassOf core:Facet .

_:node1gm7uj6vjx740 sh:maxCount 1 .

observable:ContentDataFacet rdfs:label "ContentDataFacet"@en .

vocabulary:ContactURLScopeVocab a rdfs:Datatype .

_:node1gm7uj6vjx1196 rdf:first "BELOW_NORMAL_PRIORITY_CLASS"^^vocabulary:TaskPriorityVocab .

_:node1gm7uj6vjx740 sh:nodeKind sh:Literal .

_:node1gm7uj6vjx1196 rdf:rest _:node1gm7uj6vjx1197 .

_:node1gm7uj6vjx740 sh:path observable:accessedTime .

observable:ContentDataFacet rdfs:comment "A content data facet is a grouping of characteristics unique to a block of digital data."@en .

observable:BrowserCookieFacet sh:property _:node1gm7uj6vjx740 .

_:node1gm7uj6vjx1198 sh:class observable:ObservableObject .

_:node1gm7uj6vjx741 sh:datatype xsd:dateTime .

_:node1gm7uj6vjx1197 rdf:first "HIGH_PRIORITY_CLASS"^^vocabulary:TaskPriorityVocab .

vocabulary:ContactURLScopeVocab rdfs:label "Contact URL Scope Vocabulary"@en-us .

_:node1gm7uj6vjx1197 rdf:rest _:node1gm7uj6vjx1199 .

_:node1gm7uj6vjx741 sh:maxCount 1 .

_:node1gm7uj6vjx1198 sh:maxCount 1 .

_:node1gm7uj6vjx741 sh:nodeKind sh:Literal .

_:node1gm7uj6vjx1198 sh:nodeKind sh:IRI .

_:node1gm7uj6vjx741 sh:path observable:expirationTime .

_:node1gm7uj6vjx1199 rdf:first "IDLE_PRIORITY_CLASS"^^vocabulary:TaskPriorityVocab .

observable:BrowserCookieFacet sh:property _:node1gm7uj6vjx741 .

_:node1gm7uj6vjx1199 rdf:rest _:node1gm7uj6vjx1200 .

vocabulary:ContactURLScopeVocab rdfs:comment "Defines an open-vocabulary of scopes for URL entries of digital contacts."@en .

_:node1gm7uj6vjx1198 sh:path observable:dataPayloadReferenceURL .

_:node1gm7uj6vjx742 a rdfs:Datatype .

observable:ContentDataFacet sh:property _:node1gm7uj6vjx1198 .

_:node1gm7uj6vjx743 sh:datatype xsd:dateTime .

_:node1gm7uj6vjx1201 sh:class types:Hash .

_:node1gm7uj6vjx743 sh:maxCount 1 .

_:node1gm7uj6vjx1200 rdf:first "NORMAL_PRIORITY_CLASS"^^vocabulary:TaskPriorityVocab .

_:node1gm7uj6vjx742 owl:onDatatype xsd:string .

_:node1gm7uj6vjx1200 rdf:rest _:node1gm7uj6vjx1202 .

_:node1gm7uj6vjx743 sh:nodeKind sh:Literal .

_:node1gm7uj6vjx1201 sh:nodeKind sh:IRI .

_:node1gm7uj6vjx743 sh:path observable:observableCreatedTime .

_:node1gm7uj6vjx1201 sh:path observable:hash .

observable:BrowserCookieFacet sh:property _:node1gm7uj6vjx743 .

observable:ContentDataFacet sh:property _:node1gm7uj6vjx1201 .

_:node1gm7uj6vjx745 sh:datatype xsd:string .

_:node1gm7uj6vjx1202 rdf:first "REALTIME_PRIORITY_CLASS"^^vocabulary:TaskPriorityVocab .

_:node1gm7uj6vjx744 rdf:first "home"^^vocabulary:ContactURLScopeVocab .

_:node1gm7uj6vjx1202 rdf:rest rdf:nil .

_:node1gm7uj6vjx745 sh:maxCount 1 .

_:node1gm7uj6vjx1194 owl:oneOf _:node1gm7uj6vjx1195 .

_:node1gm7uj6vjx744 rdf:rest _:node1gm7uj6vjx746 .

vocabulary:TaskPriorityVocab owl:equivalentClass _:node1gm7uj6vjx1194 .

_:node1gm7uj6vjx745 sh:nodeKind sh:Literal .

_:node1gm7uj6vjx1203 sh:datatype xsd:boolean .

_:node1gm7uj6vjx745 sh:path observable:cookieName .

vocabulary:TaskStatusVocab a rdfs:Datatype .

observable:BrowserCookieFacet sh:property _:node1gm7uj6vjx745 .

_:node1gm7uj6vjx1203 sh:maxCount 1 .

_:node1gm7uj6vjx746 rdf:first "work"^^vocabulary:ContactURLScopeVocab .

vocabulary:TaskStatusVocab rdfs:label "Task Status Vocabulary"@en-us .

_:node1gm7uj6vjx746 rdf:rest _:node1gm7uj6vjx748 .

_:node1gm7uj6vjx1203 sh:nodeKind sh:Literal .

_:node1gm7uj6vjx747 sh:datatype xsd:string .

_:node1gm7uj6vjx1203 sh:path observable:isEncrypted .

_:node1gm7uj6vjx747 sh:maxCount 1 .

observable:ContentDataFacet sh:property _:node1gm7uj6vjx1203 .

_:node1gm7uj6vjx747 sh:nodeKind sh:Literal .

_:node1gm7uj6vjx1204 sh:datatype xsd:decimal .

_:node1gm7uj6vjx747 sh:path observable:cookiePath .

vocabulary:TaskStatusVocab rdfs:comment "Defines an open-vocabulary of the possible statuses of a scheduled task. See also: http://msdn.microsoft.com/en-us/library/windows/desktop/aa383604(v=vs.85).aspx See also: http://msdn.microsoft.com/en-us/library/windows/desktop/aa381263(v=vs.85).aspx See also: http://msdn.microsoft.com/en-us/library/windows/desktop/aa381833(v=vs.85).aspx See also: http://msdn.microsoft.com/en-us/library/windows/desktop/aa383617(v=vs.85).aspx."@en .

observable:BrowserCookieFacet sh:property _:node1gm7uj6vjx747 .

_:node1gm7uj6vjx1205 a rdfs:Datatype .

_:node1gm7uj6vjx748 rdf:first "school"^^vocabulary:ContactURLScopeVocab .

_:node1gm7uj6vjx1205 owl:onDatatype xsd:string .

_:node1gm7uj6vjx748 rdf:rest _:node1gm7uj6vjx749 .

_:node1gm7uj6vjx1204 sh:maxCount 1 .

observable:BrowserCookieFacet sh:targetClass observable:BrowserCookieFacet .

_:node1gm7uj6vjx1204 sh:nodeKind sh:Literal .

_:node1gm7uj6vjx749 rdf:first "homepage"^^vocabulary:ContactURLScopeVocab .

_:node1gm7uj6vjx1206 rdf:first "SCHED_E_ACCOUNT_DBASE_CORRUPT"^^vocabulary:TaskStatusVocab .

_:node1gm7uj6vjx749 rdf:rest rdf:nil .

_:node1gm7uj6vjx1206 rdf:rest _:node1gm7uj6vjx1207 .

_:node1gm7uj6vjx742 owl:oneOf _:node1gm7uj6vjx744 .

_:node1gm7uj6vjx1204 sh:path observable:entropy .

vocabulary:ContactURLScopeVocab owl:equivalentClass _:node1gm7uj6vjx742 .

observable:ContentDataFacet sh:property _:node1gm7uj6vjx1204 .

observable:Calendar a owl:Class .

_:node1gm7uj6vjx1208 sh:datatype xsd:integer .

observable:Calendar a sh:NodeShape .

_:node1gm7uj6vjx1207 rdf:first "SCHED_E_ACCOUNT_INFORMATION_NOT_SET"^^vocabulary:TaskStatusVocab .

observable:Calendar rdfs:subClassOf observable:ObservableObject .

_:node1gm7uj6vjx1207 rdf:rest _:node1gm7uj6vjx1209 .

vocabulary:DiskTypeVocab a rdfs:Datatype .

_:node1gm7uj6vjx1209 rdf:first "SCHED_E_ACCOUNT_NAME_NOT_FOUND"^^vocabulary:TaskStatusVocab .

observable:Calendar rdfs:label "Calendar"@en .

_:node1gm7uj6vjx1208 sh:maxCount 1 .

observable:Calendar rdfs:comment "A calendar is a collection of appointments, meetings, and events."@en .

_:node1gm7uj6vjx1209 rdf:rest _:node1gm7uj6vjx1210 .

observable:Calendar sh:targetClass observable:Calendar .

_:node1gm7uj6vjx1208 sh:nodeKind sh:Literal .

vocabulary:DiskTypeVocab rdfs:label "Disk Type Vocabulary"@en-us .

_:node1gm7uj6vjx1210 rdf:first "SCHED_E_CANNOT_OPEN_TASK"^^vocabulary:TaskStatusVocab .

observable:CalendarEntry a owl:Class .

_:node1gm7uj6vjx1210 rdf:rest _:node1gm7uj6vjx1211 .

observable:CalendarEntry a sh:NodeShape .

_:node1gm7uj6vjx1208 sh:path observable:sizeInBytes .

observable:CalendarEntry rdfs:subClassOf observable:ObservableObject .

observable:ContentDataFacet sh:property _:node1gm7uj6vjx1208 .

observable:CalendarEntry rdfs:label "CalendarEntry"@en .

_:node1gm7uj6vjx1211 rdf:first "SCHED_E_INVALID_TASK"^^vocabulary:TaskStatusVocab .

vocabulary:DiskTypeVocab rdfs:comment "Defines an open-vocabulary of disk types."@en .

_:node1gm7uj6vjx1211 rdf:rest _:node1gm7uj6vjx1213 .

observable:CalendarEntry rdfs:comment "A calendar entry is an appointment, meeting or event within a collection of appointments, meetings and events."@en .

_:node1gm7uj6vjx1212 sh:datatype xsd:string .

observable:CalendarEntry sh:targetClass observable:CalendarEntry .

_:node1gm7uj6vjx1213 rdf:first "SCHED_E_NO_SECURITY_SERVICES"^^vocabulary:TaskStatusVocab .

observable:CalendarEntryFacet a owl:Class .

_:node1gm7uj6vjx1213 rdf:rest _:node1gm7uj6vjx1214 .

_:node1gm7uj6vjx750 a rdfs:Datatype .

_:node1gm7uj6vjx1212 sh:maxCount 1 .

observable:CalendarEntryFacet a sh:NodeShape .

_:node1gm7uj6vjx1214 rdf:first "SCHED_E_SERVICE_NOT_INSTALLED"^^vocabulary:TaskStatusVocab .

observable:CalendarEntryFacet rdfs:subClassOf core:Facet .

_:node1gm7uj6vjx1214 rdf:rest _:node1gm7uj6vjx1215 .

_:node1gm7uj6vjx750 owl:onDatatype xsd:string .

_:node1gm7uj6vjx1212 sh:nodeKind sh:Literal .

_:node1gm7uj6vjx751 rdf:first "CDRom"^^vocabulary:DiskTypeVocab .

_:node1gm7uj6vjx1212 sh:path observable:dataPayload .

_:node1gm7uj6vjx751 rdf:rest _:node1gm7uj6vjx752 .

observable:ContentDataFacet sh:property _:node1gm7uj6vjx1212 .

_:node1gm7uj6vjx752 rdf:first "Fixed"^^vocabulary:DiskTypeVocab .

_:node1gm7uj6vjx1216 sh:datatype xsd:string .

_:node1gm7uj6vjx752 rdf:rest _:node1gm7uj6vjx753 .

_:node1gm7uj6vjx1215 rdf:first "SCHED_E_SERVICE_NOT_RUNNING"^^vocabulary:TaskStatusVocab .

_:node1gm7uj6vjx753 rdf:first "RAMDisk"^^vocabulary:DiskTypeVocab .

_:node1gm7uj6vjx1215 rdf:rest _:node1gm7uj6vjx1217 .

_:node1gm7uj6vjx753 rdf:rest _:node1gm7uj6vjx754 .

_:node1gm7uj6vjx1217 rdf:first "SCHED_E_TASK_NOT_READY"^^vocabulary:TaskStatusVocab .

_:node1gm7uj6vjx754 rdf:first "Remote"^^vocabulary:DiskTypeVocab .

_:node1gm7uj6vjx1217 rdf:rest _:node1gm7uj6vjx1218 .

observable:CalendarEntryFacet rdfs:label "CalendarEntryFacet"@en .

_:node1gm7uj6vjx1216 sh:maxCount 1 .

_:node1gm7uj6vjx754 rdf:rest _:node1gm7uj6vjx755 .

_:node1gm7uj6vjx1218 rdf:first "SCHED_E_TASK_NOT_RUNNING"^^vocabulary:TaskStatusVocab .

_:node1gm7uj6vjx755 rdf:first "Removable"^^vocabulary:DiskTypeVocab .

_:node1gm7uj6vjx1218 rdf:rest _:node1gm7uj6vjx1219 .

_:node1gm7uj6vjx755 rdf:rest rdf:nil .

_:node1gm7uj6vjx1216 sh:nodeKind sh:Literal .

_:node1gm7uj6vjx750 owl:oneOf _:node1gm7uj6vjx751 .

_:node1gm7uj6vjx1219 rdf:first "SCHED_E_TRIGGER_NOT_FOUND"^^vocabulary:TaskStatusVocab .

vocabulary:DiskTypeVocab owl:equivalentClass _:node1gm7uj6vjx750 .

_:node1gm7uj6vjx1219 rdf:rest _:node1gm7uj6vjx1220 .

observable:CalendarEntryFacet rdfs:comment "A calendar entry facet is a grouping of characteristics unique to an appointment, meeting, or event within a collection of appointments, meetings, and events."@en .

_:node1gm7uj6vjx1220 rdf:first "SCHED_E_UNKNOWN_OBJECT_VERSION"^^vocabulary:TaskStatusVocab .

vocabulary:EndiannessTypeVocab a rdfs:Datatype .

_:node1gm7uj6vjx1220 rdf:rest _:node1gm7uj6vjx1221 .

_:node1gm7uj6vjx756 sh:class core:UcoObject .

_:node1gm7uj6vjx1216 sh:path observable:magicNumber .

_:node1gm7uj6vjx756 sh:maxCount 1 .

observable:ContentDataFacet sh:property _:node1gm7uj6vjx1216 .

_:node1gm7uj6vjx756 sh:nodeKind sh:IRI .

_:node1gm7uj6vjx1221 rdf:first "SCHED_E_UNSUPPORTED_ACCOUNT_OPTION"^^vocabulary:TaskStatusVocab .

_:node1gm7uj6vjx756 sh:path observable:owner .

_:node1gm7uj6vjx1221 rdf:rest _:node1gm7uj6vjx1223 .

observable:CalendarEntryFacet sh:property _:node1gm7uj6vjx756 .

_:node1gm7uj6vjx1222 sh:datatype xsd:string .

_:node1gm7uj6vjx757 sh:class identity:Identity .

_:node1gm7uj6vjx1223 rdf:first "SCHED_S_EVENT_TRIGGER"^^vocabulary:TaskStatusVocab .

_:node1gm7uj6vjx757 sh:nodeKind sh:IRI .

_:node1gm7uj6vjx1223 rdf:rest _:node1gm7uj6vjx1224 .

_:node1gm7uj6vjx757 sh:path observable:attendant .

_:node1gm7uj6vjx1222 sh:maxCount 1 .

observable:CalendarEntryFacet sh:property _:node1gm7uj6vjx757 .

_:node1gm7uj6vjx1224 rdf:first "SCHED_S_TASK_DISABLED"^^vocabulary:TaskStatusVocab .

_:node1gm7uj6vjx758 sh:class location:Location .

_:node1gm7uj6vjx1224 rdf:rest _:node1gm7uj6vjx1225 .

_:node1gm7uj6vjx758 sh:maxCount 1 .

_:node1gm7uj6vjx1225 rdf:first "SCHED_S_TASK_HAS_NOT_RUN"^^vocabulary:TaskStatusVocab .

vocabulary:EndiannessTypeVocab rdfs:label "Endianness Type Vocabulary"@en-us .

_:node1gm7uj6vjx1225 rdf:rest _:node1gm7uj6vjx1226 .

_:node1gm7uj6vjx758 sh:nodeKind sh:IRI .

_:node1gm7uj6vjx1222 sh:nodeKind sh:Literal .

_:node1gm7uj6vjx758 sh:path observable:location .

_:node1gm7uj6vjx1222 sh:path observable:mimeClass .

observable:CalendarEntryFacet sh:property _:node1gm7uj6vjx758 .

observable:ContentDataFacet sh:property _:node1gm7uj6vjx1222 .

_:node1gm7uj6vjx759 sh:class observable:ObservableObject .

_:node1gm7uj6vjx1226 rdf:first "SCHED_S_TASK_NOT_SCHEDULED"^^vocabulary:TaskStatusVocab .

_:node1gm7uj6vjx759 sh:maxCount 1 .

_:node1gm7uj6vjx1226 rdf:rest _:node1gm7uj6vjx1228 .

_:node1gm7uj6vjx759 sh:nodeKind sh:IRI .

_:node1gm7uj6vjx1227 sh:datatype xsd:string .

_:node1gm7uj6vjx759 sh:path observable:application .

_:node1gm7uj6vjx1228 rdf:first "SCHED_S_TASK_NO_MORE_RUNS"^^vocabulary:TaskStatusVocab .

observable:CalendarEntryFacet sh:property _:node1gm7uj6vjx759 .

_:node1gm7uj6vjx1228 rdf:rest _:node1gm7uj6vjx1229 .

vocabulary:EndiannessTypeVocab rdfs:comment "Defines an open-vocabulary of byte ordering methods."@en .

_:node1gm7uj6vjx1227 sh:nodeKind sh:Literal .

_:node1gm7uj6vjx760 sh:datatype xsd:boolean .

_:node1gm7uj6vjx1229 rdf:first "SCHED_S_TASK_NO_VALID_TRIGGERS"^^vocabulary:TaskStatusVocab .

_:node1gm7uj6vjx760 sh:maxCount 1 .

_:node1gm7uj6vjx1229 rdf:rest _:node1gm7uj6vjx1230 .

_:node1gm7uj6vjx760 sh:nodeKind sh:Literal .

_:node1gm7uj6vjx1227 sh:path observable:mimeType .

_:node1gm7uj6vjx761 a rdfs:Datatype .

observable:ContentDataFacet sh:property _:node1gm7uj6vjx1227 .

_:node1gm7uj6vjx760 sh:path observable:isPrivate .

_:node1gm7uj6vjx1230 rdf:first "SCHED_S_TASK_READY"^^vocabulary:TaskStatusVocab .

observable:CalendarEntryFacet sh:property _:node1gm7uj6vjx760 .

_:node1gm7uj6vjx1230 rdf:rest _:node1gm7uj6vjx1232 .

_:node1gm7uj6vjx762 sh:datatype xsd:dateTime .

_:node1gm7uj6vjx1231 sh:datatype vocabulary:EndiannessTypeVocab .

_:node1gm7uj6vjx762 sh:maxCount 1 .

_:node1gm7uj6vjx1232 rdf:first "SCHED_S_TASK_RUNNING"^^vocabulary:TaskStatusVocab .

_:node1gm7uj6vjx761 owl:onDatatype xsd:string .

_:node1gm7uj6vjx1232 rdf:rest _:node1gm7uj6vjx1233 .

_:node1gm7uj6vjx762 sh:nodeKind sh:Literal .

_:node1gm7uj6vjx1231 sh:message "Value is outside the default vocabulary EndiannessTypeVocab." .

_:node1gm7uj6vjx762 sh:path observable:endTime .

_:node1gm7uj6vjx1231 sh:path observable:byteOrder .

observable:CalendarEntryFacet sh:property _:node1gm7uj6vjx762 .

_:node1gm7uj6vjx1233 rdf:first "SCHED_S_TASK_TERMINATED"^^vocabulary:TaskStatusVocab .

_:node1gm7uj6vjx764 sh:datatype xsd:dateTime .

_:node1gm7uj6vjx1233 rdf:rest _:node1gm7uj6vjx1234 .

_:node1gm7uj6vjx764 sh:maxCount 1 .

_:node1gm7uj6vjx1231 sh:severity sh:Info .

_:node1gm7uj6vjx764 sh:nodeKind sh:Literal .

observable:ContentDataFacet sh:property _:node1gm7uj6vjx1231 .

_:node1gm7uj6vjx763 rdf:first "Big-endian"^^vocabulary:EndiannessTypeVocab .

_:node1gm7uj6vjx1234 rdf:first "TASK_STATE_QUEUED"^^vocabulary:TaskStatusVocab .

_:node1gm7uj6vjx764 sh:path observable:modifiedTime .

_:node1gm7uj6vjx1234 rdf:rest _:node1gm7uj6vjx1236 .

observable:CalendarEntryFacet sh:property _:node1gm7uj6vjx764 .

_:node1gm7uj6vjx1235 sh:maxCount 1 .

_:node1gm7uj6vjx763 rdf:rest _:node1gm7uj6vjx765 .

_:node1gm7uj6vjx1235 sh:nodeKind sh:Literal .

_:node1gm7uj6vjx766 sh:datatype xsd:dateTime .

_:node1gm7uj6vjx1236 rdf:first "TASK_STATE_UNKNOWN"^^vocabulary:TaskStatusVocab .

_:node1gm7uj6vjx766 sh:maxCount 1 .

_:node1gm7uj6vjx1236 rdf:rest rdf:nil .

_:node1gm7uj6vjx765 rdf:first "Little-endian"^^vocabulary:EndiannessTypeVocab .

_:node1gm7uj6vjx1205 owl:oneOf _:node1gm7uj6vjx1206 .

_:node1gm7uj6vjx765 rdf:rest _:node1gm7uj6vjx767 .

vocabulary:TaskStatusVocab owl:equivalentClass _:node1gm7uj6vjx1205 .

_:node1gm7uj6vjx766 sh:nodeKind sh:Literal .

_:node1gm7uj6vjx1238 sh:datatype vocabulary:EndiannessTypeVocab .

_:node1gm7uj6vjx766 sh:path observable:observableCreatedTime .

_:node1gm7uj6vjx1237 rdf:first _:node1gm7uj6vjx1238 .

observable:CalendarEntryFacet sh:property _:node1gm7uj6vjx766 .

_:node1gm7uj6vjx1237 rdf:rest _:node1gm7uj6vjx1239 .

_:node1gm7uj6vjx768 sh:datatype xsd:dateTime .

vocabulary:ThreadRunningStatusVocab a rdfs:Datatype .

_:node1gm7uj6vjx767 rdf:first "Middle-endian"^^vocabulary:EndiannessTypeVocab .

_:node1gm7uj6vjx1240 sh:datatype xsd:string .

_:node1gm7uj6vjx768 sh:maxCount 1 .

_:node1gm7uj6vjx1239 rdf:first _:node1gm7uj6vjx1240 .

_:node1gm7uj6vjx767 rdf:rest rdf:nil .

_:node1gm7uj6vjx1239 rdf:rest rdf:nil .

_:node1gm7uj6vjx761 owl:oneOf _:node1gm7uj6vjx763 .

_:node1gm7uj6vjx1235 sh:or _:node1gm7uj6vjx1237 .

vocabulary:EndiannessTypeVocab owl:equivalentClass _:node1gm7uj6vjx761 .

_:node1gm7uj6vjx1235 sh:path observable:byteOrder .

_:node1gm7uj6vjx768 sh:nodeKind sh:Literal .

observable:ContentDataFacet sh:property _:node1gm7uj6vjx1235 .

_:node1gm7uj6vjx768 sh:path observable:remindTime .

vocabulary:ThreadRunningStatusVocab rdfs:label "Thread Running Status Vocabulary"@en-us .

observable:CalendarEntryFacet sh:property _:node1gm7uj6vjx768 .

_:node1gm7uj6vjx1241 sh:message "Value is not member of the vocabulary EndiannessTypeVocab." .

vocabulary:HashNameVocab a rdfs:Datatype .

vocabulary:ThreadRunningStatusVocab rdfs:comment "Defines an open-vocabulary of the various states that a thread may be in before, during, or after execution. See http://msdn.microsoft.com/en-us/library/system.diagnostics.threadstate(v=vs.110).aspx."@en .

_:node1gm7uj6vjx769 sh:datatype xsd:dateTime .

_:node1gm7uj6vjx1243 sh:datatype vocabulary:EndiannessTypeVocab .

_:node1gm7uj6vjx769 sh:maxCount 1 .

_:node1gm7uj6vjx1245 a rdfs:Datatype .

_:node1gm7uj6vjx769 sh:nodeKind sh:Literal .

_:node1gm7uj6vjx1245 owl:onDatatype xsd:string .

_:node1gm7uj6vjx769 sh:path observable:startTime .

_:node1gm7uj6vjx1244 rdf:first "Big-endian"^^vocabulary:EndiannessTypeVocab .

observable:CalendarEntryFacet sh:property _:node1gm7uj6vjx769 .

_:node1gm7uj6vjx1244 rdf:rest _:node1gm7uj6vjx1246 .

_:node1gm7uj6vjx770 sh:datatype xsd:integer .

_:node1gm7uj6vjx1246 rdf:first "Little-endian"^^vocabulary:EndiannessTypeVocab .

_:node1gm7uj6vjx770 sh:maxCount 1 .

_:node1gm7uj6vjx1246 rdf:rest _:node1gm7uj6vjx1248 .

_:node1gm7uj6vjx770 sh:nodeKind sh:Literal .

_:node1gm7uj6vjx1247 rdf:first "Initialized"^^vocabulary:ThreadRunningStatusVocab .

_:node1gm7uj6vjx770 sh:path observable:duration .

_:node1gm7uj6vjx1248 rdf:first "Middle-endian"^^vocabulary:EndiannessTypeVocab .

observable:CalendarEntryFacet sh:property _:node1gm7uj6vjx770 .

_:node1gm7uj6vjx1248 rdf:rest rdf:nil .

vocabulary:HashNameVocab rdfs:label "Hash Name Vocabulary"@en-us .

_:node1gm7uj6vjx1243 sh:in _:node1gm7uj6vjx1244 .

_:node1gm7uj6vjx771 sh:datatype xsd:string .

_:node1gm7uj6vjx1242 rdf:first _:node1gm7uj6vjx1243 .

_:node1gm7uj6vjx771 sh:maxCount 1 .

_:node1gm7uj6vjx1247 rdf:rest _:node1gm7uj6vjx1249 .

_:node1gm7uj6vjx771 sh:nodeKind sh:Literal .

_:node1gm7uj6vjx1242 rdf:rest _:node1gm7uj6vjx1250 .

_:node1gm7uj6vjx771 sh:path observable:eventStatus .

_:node1gm7uj6vjx1251 sh:datatype xsd:string .

observable:CalendarEntryFacet sh:property _:node1gm7uj6vjx771 .

_:node1gm7uj6vjx1250 rdf:first _:node1gm7uj6vjx1251 .

_:node1gm7uj6vjx772 sh:datatype xsd:string .

_:node1gm7uj6vjx1250 rdf:rest rdf:nil .

vocabulary:HashNameVocab rdfs:comment "Defines an open-vocabulary of hashing algorithm names."@en-us .

_:node1gm7uj6vjx1241 sh:or _:node1gm7uj6vjx1242 .

_:node1gm7uj6vjx772 sh:maxCount 1 .

_:node1gm7uj6vjx1249 rdf:first "Ready"^^vocabulary:ThreadRunningStatusVocab .

_:node1gm7uj6vjx772 sh:nodeKind sh:Literal .

_:node1gm7uj6vjx1241 sh:path observable:byteOrder .

_:node1gm7uj6vjx773 a rdfs:Datatype .

observable:ContentDataFacet sh:property _:node1gm7uj6vjx1241 .

_:node1gm7uj6vjx772 sh:path observable:eventType .

_:node1gm7uj6vjx1249 rdf:rest _:node1gm7uj6vjx1252 .

observable:CalendarEntryFacet sh:property _:node1gm7uj6vjx772 .

observable:ContentDataFacet sh:targetClass observable:ContentDataFacet .

_:node1gm7uj6vjx773 owl:onDatatype xsd:string .

_:node1gm7uj6vjx1252 rdf:first "Running"^^vocabulary:ThreadRunningStatusVocab .

_:node1gm7uj6vjx774 sh:datatype xsd:string .

_:node1gm7uj6vjx1252 rdf:rest _:node1gm7uj6vjx1253 .

_:node1gm7uj6vjx774 sh:maxCount 1 .

observable:CookieHistory a owl:Class .

_:node1gm7uj6vjx774 sh:nodeKind sh:Literal .

observable:CookieHistory a sh:NodeShape .

_:node1gm7uj6vjx775 rdf:first "MD5"^^vocabulary:HashNameVocab .

_:node1gm7uj6vjx1253 rdf:first "Standby"^^vocabulary:ThreadRunningStatusVocab .

_:node1gm7uj6vjx775 rdf:rest _:node1gm7uj6vjx776 .

_:node1gm7uj6vjx1253 rdf:rest _:node1gm7uj6vjx1254 .

_:node1gm7uj6vjx774 sh:path observable:recurrence .

observable:CookieHistory rdfs:subClassOf observable:ObservableObject .

observable:CalendarEntryFacet sh:property _:node1gm7uj6vjx774 .

observable:CookieHistory rdfs:label "CookieHistory"@en .

_:node1gm7uj6vjx777 sh:datatype xsd:string .

_:node1gm7uj6vjx1254 rdf:first "Terminated"^^vocabulary:ThreadRunningStatusVocab .

_:node1gm7uj6vjx776 rdf:first "MD6"^^vocabulary:HashNameVocab .

_:node1gm7uj6vjx1254 rdf:rest _:node1gm7uj6vjx1255 .

_:node1gm7uj6vjx776 rdf:rest _:node1gm7uj6vjx778 .

observable:CookieHistory rdfs:comment "A cookie history is the stored web cookie history for a particular web browser."@en .

_:node1gm7uj6vjx777 sh:maxCount 1 .

observable:CookieHistory sh:targetClass observable:CookieHistory .

_:node1gm7uj6vjx777 sh:nodeKind sh:Literal .

observable:Credential a owl:Class .

_:node1gm7uj6vjx778 rdf:first "SHA1"^^vocabulary:HashNameVocab .

observable:Credential a sh:NodeShape .

_:node1gm7uj6vjx777 sh:path observable:subject .

_:node1gm7uj6vjx1255 rdf:first "Transition"^^vocabulary:ThreadRunningStatusVocab .

_:node1gm7uj6vjx778 rdf:rest _:node1gm7uj6vjx779 .

_:node1gm7uj6vjx1255 rdf:rest _:node1gm7uj6vjx1256 .

observable:CalendarEntryFacet sh:property _:node1gm7uj6vjx777 .

observable:Credential rdfs:subClassOf observable:ObservableObject .

observable:CalendarEntryFacet sh:targetClass observable:CalendarEntryFacet .

observable:Credential rdfs:label "Credential"@en .

_:node1gm7uj6vjx779 rdf:first "SHA224"^^vocabulary:HashNameVocab .

_:node1gm7uj6vjx1256 rdf:first "Unknown"^^vocabulary:ThreadRunningStatusVocab .

_:node1gm7uj6vjx779 rdf:rest _:node1gm7uj6vjx780 .

_:node1gm7uj6vjx1256 rdf:rest _:node1gm7uj6vjx1257 .

observable:CalendarFacet a owl:Class .

observable:Credential rdfs:comment "A credential is a single specific login and password combination for authorization of access to a digital account or system."@en .

observable:CalendarFacet a sh:NodeShape .

observable:Credential sh:targetClass observable:Credential .

_:node1gm7uj6vjx780 rdf:first "SHA256"^^vocabulary:HashNameVocab .

_:node1gm7uj6vjx1257 rdf:first "Waiting"^^vocabulary:ThreadRunningStatusVocab .

_:node1gm7uj6vjx780 rdf:rest _:node1gm7uj6vjx781 .

_:node1gm7uj6vjx1257 rdf:rest rdf:nil .

observable:CalendarFacet rdfs:subClassOf core:Facet .

_:node1gm7uj6vjx1245 owl:oneOf _:node1gm7uj6vjx1247 .

observable:CalendarFacet rdfs:label "CalendarFacet"@en .

vocabulary:ThreadRunningStatusVocab owl:equivalentClass _:node1gm7uj6vjx1245 .

_:node1gm7uj6vjx781 rdf:first "SHA384"^^vocabulary:HashNameVocab .

observable:CredentialDump a owl:Class .

_:node1gm7uj6vjx781 rdf:rest _:node1gm7uj6vjx782 .

observable:CredentialDump a sh:NodeShape .

_:node1gm7uj6vjx782 rdf:first "SHA512"^^vocabulary:HashNameVocab .

vocabulary:TimestampPrecisionVocab a rdfs:Datatype .

observable:CalendarFacet rdfs:comment "A calendar facet is a grouping of characteristics unique to a collection of appointments, meetings, and events."@en .

observable:CredentialDump rdfs:subClassOf observable:ObservableObject .

_:node1gm7uj6vjx782 rdf:rest _:node1gm7uj6vjx783 .

observable:CredentialDump rdfs:label "CredentialDump"@en .

_:node1gm7uj6vjx784 sh:class core:UcoObject .

vocabulary:TimestampPrecisionVocab rdfs:label "Timestamp Precision Vocabulary"@en-us .

_:node1gm7uj6vjx783 rdf:first "SSDEEP"^^vocabulary:HashNameVocab .

observable:CredentialDump rdfs:comment "A credential dump is a collection (typically forcibly extracted from a system) of specific login and password combinations for authorization of access to a digital account or system."@en .

_:node1gm7uj6vjx783 rdf:rest rdf:nil .

observable:CredentialDump sh:targetClass observable:CredentialDump .

_:node1gm7uj6vjx773 owl:oneOf _:node1gm7uj6vjx775 .

observable:DNSCache a owl:Class .

_:node1gm7uj6vjx784 sh:maxCount 1 .

vocabulary:TimestampPrecisionVocab rdfs:comment "Defines an open-vocabulary of timestamp precision granularities."@en-us .

vocabulary:HashNameVocab owl:equivalentClass _:node1gm7uj6vjx773 .

observable:DNSCache a sh:NodeShape .

_:node1gm7uj6vjx784 sh:nodeKind sh:IRI .

_:node1gm7uj6vjx1258 a rdfs:Datatype .

_:node1gm7uj6vjx784 sh:path observable:owner .

observable:DNSCache rdfs:subClassOf observable:ObservableObject .

observable:CalendarFacet sh:property _:node1gm7uj6vjx784 .

observable:DNSCache rdfs:label "DNSCache"@en .

vocabulary:LibraryTypeVocab a rdfs:Datatype .

_:node1gm7uj6vjx1258 owl:onDatatype xsd:string .

_:node1gm7uj6vjx785 sh:class observable:ObservableObject .

_:node1gm7uj6vjx1259 rdf:first "day"^^vocabulary:TimestampPrecisionVocab .

_:node1gm7uj6vjx785 sh:maxCount 1 .

_:node1gm7uj6vjx1259 rdf:rest _:node1gm7uj6vjx1260 .

_:node1gm7uj6vjx785 sh:nodeKind sh:IRI .

_:node1gm7uj6vjx1260 rdf:first "hour"^^vocabulary:TimestampPrecisionVocab .

_:node1gm7uj6vjx785 sh:path observable:application .

_:node1gm7uj6vjx1260 rdf:rest _:node1gm7uj6vjx1261 .

observable:CalendarFacet sh:property _:node1gm7uj6vjx785 .

observable:DNSCache rdfs:comment "An DNS cache is a temporary locally stored collection of previous Domain Name System (DNS) query results (created when an domain name is resolved to a IP address) for a particular computer."@en .

observable:CalendarFacet sh:targetClass observable:CalendarFacet .

_:node1gm7uj6vjx1261 rdf:first "minute"^^vocabulary:TimestampPrecisionVocab .

vocabulary:LibraryTypeVocab rdfs:label "Library Type Vocabulary"@en-us .

observable:DNSCache sh:targetClass observable:DNSCache .

observable:Call a owl:Class .

_:node1gm7uj6vjx1261 rdf:rest _:node1gm7uj6vjx1262 .

observable:Call a sh:NodeShape .

observable:DNSRecord a owl:Class .

observable:Call rdfs:subClassOf observable:ObservableObject .

observable:DNSRecord a sh:NodeShape .

vocabulary:LibraryTypeVocab rdfs:comment "Defines an open-vocabulary of library types."@en .

_:node1gm7uj6vjx1262 rdf:first "month"^^vocabulary:TimestampPrecisionVocab .

observable:Call rdfs:label "Call"@en .

_:node1gm7uj6vjx1262 rdf:rest _:node1gm7uj6vjx1263 .

_:node1gm7uj6vjx786 a rdfs:Datatype .

observable:DNSRecord rdfs:subClassOf observable:ObservableObject .

observable:Call rdfs:comment "A call is a connection as part of a realtime cyber communication between one or more parties."@en .

observable:DNSRecord rdfs:label "DNSRecord"@en .

_:node1gm7uj6vjx786 owl:onDatatype xsd:string .

_:node1gm7uj6vjx1263 rdf:first "second"^^vocabulary:TimestampPrecisionVocab .

observable:Call sh:targetClass observable:Call .

_:node1gm7uj6vjx1263 rdf:rest _:node1gm7uj6vjx1264 .

observable:CallFacet a owl:Class .

_:node1gm7uj6vjx1264 rdf:first "year"^^vocabulary:TimestampPrecisionVocab .

observable:CallFacet a sh:NodeShape .

_:node1gm7uj6vjx1264 rdf:rest rdf:nil .

observable:CallFacet rdfs:subClassOf core:Facet .

_:node1gm7uj6vjx1258 owl:oneOf _:node1gm7uj6vjx1259 .

_:node1gm7uj6vjx787 rdf:first "Dynamic"^^vocabulary:LibraryTypeVocab .

vocabulary:TimestampPrecisionVocab owl:equivalentClass _:node1gm7uj6vjx1258 .

_:node1gm7uj6vjx787 rdf:rest _:node1gm7uj6vjx788 .

observable:DNSRecord rdfs:comment "A DNS record is a single Domain Name System (DNS) artifact specifying information of a particular type (routing, authority, responsibility, security, etc.) for a specific Internet domain name."@en .

observable:CallFacet rdfs:label "CallFacet"@en .

observable:DNSRecord sh:targetClass observable:DNSRecord .

_:node1gm7uj6vjx788 rdf:first "Other"^^vocabulary:LibraryTypeVocab .

vocabulary:TrendVocab a rdfs:Datatype .

_:node1gm7uj6vjx788 rdf:rest _:node1gm7uj6vjx789 .

observable:DataRangeFacet a owl:Class .

observable:CallFacet rdfs:comment "A call facet is a grouping of characteristics unique to a connection as part of a realtime cyber communication between one or more parties."@en .

observable:DataRangeFacet a sh:NodeShape .

_:node1gm7uj6vjx789 rdf:first "Remote"^^vocabulary:LibraryTypeVocab .

vocabulary:TrendVocab rdfs:label "Trend Vocabulary"@en-us .

_:node1gm7uj6vjx790 sh:class observable:ObservableObject .

observable:DataRangeFacet rdfs:subClassOf core:Facet .

_:node1gm7uj6vjx789 rdf:rest _:node1gm7uj6vjx791 .

observable:DataRangeFacet rdfs:label "DataRangeFacet"@en .

_:node1gm7uj6vjx790 sh:maxCount 1 .

vocabulary:TrendVocab rdfs:comment "Defines an open-vocabulary of trend values."@en-us .

_:node1gm7uj6vjx790 sh:nodeKind sh:IRI .

observable:DataRangeFacet rdfs:comment "A data range facet is a grouping of characteristics unique to a particular contiguous scope within a block of digital data."@en .

_:node1gm7uj6vjx791 rdf:first "Shared"^^vocabulary:LibraryTypeVocab .

_:node1gm7uj6vjx1265 a rdfs:Datatype .

_:node1gm7uj6vjx790 sh:path observable:application .

_:node1gm7uj6vjx1266 sh:datatype xsd:integer .

observable:CallFacet sh:property _:node1gm7uj6vjx790 .

_:node1gm7uj6vjx1265 owl:onDatatype xsd:string .

_:node1gm7uj6vjx791 rdf:rest _:node1gm7uj6vjx792 .

_:node1gm7uj6vjx1266 sh:maxCount 1 .

_:node1gm7uj6vjx793 sh:class observable:ObservableObject .

_:node1gm7uj6vjx1266 sh:nodeKind sh:Literal .

_:node1gm7uj6vjx793 sh:maxCount 1 .

_:node1gm7uj6vjx1267 rdf:first "Decreasing"^^vocabulary:TrendVocab .

_:node1gm7uj6vjx792 rdf:first "Static"^^vocabulary:LibraryTypeVocab .

_:node1gm7uj6vjx1267 rdf:rest _:node1gm7uj6vjx1268 .

_:node1gm7uj6vjx792 rdf:rest rdf:nil .

_:node1gm7uj6vjx1266 sh:path observable:rangeOffset .

_:node1gm7uj6vjx786 owl:oneOf _:node1gm7uj6vjx787 .

observable:DataRangeFacet sh:property _:node1gm7uj6vjx1266 .

_:node1gm7uj6vjx793 sh:nodeKind sh:IRI .

_:node1gm7uj6vjx1269 sh:datatype xsd:integer .

vocabulary:LibraryTypeVocab owl:equivalentClass _:node1gm7uj6vjx786 .

_:node1gm7uj6vjx1268 rdf:first "Increasing"^^vocabulary:TrendVocab .

_:node1gm7uj6vjx793 sh:path observable:from .

_:node1gm7uj6vjx1268 rdf:rest rdf:nil .

observable:CallFacet sh:property _:node1gm7uj6vjx793 .

_:node1gm7uj6vjx1265 owl:oneOf _:node1gm7uj6vjx1267 .

_:node1gm7uj6vjx794 sh:class observable:ObservableObject .

vocabulary:TrendVocab owl:equivalentClass _:node1gm7uj6vjx1265 .

_:node1gm7uj6vjx794 sh:nodeKind sh:IRI .

_:node1gm7uj6vjx1269 sh:maxCount 1 .

_:node1gm7uj6vjx794 sh:path observable:participant .

_:node1gm7uj6vjx1269 sh:nodeKind sh:Literal .

vocabulary:MemoryBlockTypeVocab a rdfs:Datatype .

vocabulary:TriggerFrequencyVocab a rdfs:Datatype .

observable:CallFacet sh:property _:node1gm7uj6vjx794 .

_:node1gm7uj6vjx1269 sh:path observable:rangeSize .

_:node1gm7uj6vjx795 sh:class observable:ObservableObject .

observable:DataRangeFacet sh:property _:node1gm7uj6vjx1269 .

_:node1gm7uj6vjx795 sh:nodeKind sh:IRI .

_:node1gm7uj6vjx1270 sh:datatype xsd:string .

_:node1gm7uj6vjx795 sh:path observable:to .

vocabulary:TriggerFrequencyVocab rdfs:label "Trigger Frequency Vocabulary"@en-us .

observable:CallFacet sh:property _:node1gm7uj6vjx795 .

_:node1gm7uj6vjx1270 sh:maxCount 1 .

_:node1gm7uj6vjx796 sh:datatype xsd:dateTime .

_:node1gm7uj6vjx1270 sh:nodeKind sh:Literal .

_:node1gm7uj6vjx796 sh:maxCount 1 .

_:node1gm7uj6vjx1270 sh:path observable:rangeOffsetType .

vocabulary:MemoryBlockTypeVocab rdfs:label "Memory Block Type Vocabulary"@en-us .

observable:DataRangeFacet sh:property _:node1gm7uj6vjx1270 .

_:node1gm7uj6vjx796 sh:nodeKind sh:Literal .

vocabulary:TriggerFrequencyVocab rdfs:comment "Defines an open-vocabulary of the frequency types that a trigger may use. See also: http://msdn.microsoft.com/en-us/library/windows/desktop/aa383620(v=vs.85).aspx and http://msdn.microsoft.com/en-us/library/windows/desktop/aa383987(v=vs.85).aspx."@en .

_:node1gm7uj6vjx796 sh:path observable:endTime .

observable:DataRangeFacet sh:targetClass observable:DataRangeFacet .

observable:CallFacet sh:property _:node1gm7uj6vjx796 .

_:node1gm7uj6vjx1271 a rdfs:Datatype .

_:node1gm7uj6vjx797 sh:datatype xsd:dateTime .

observable:DefinedEffectFacet a owl:Class .

vocabulary:MemoryBlockTypeVocab rdfs:comment "Defines an open-vocabulary of types of memory blocks."@en .

_:node1gm7uj6vjx1271 owl:onDatatype xsd:string .

_:node1gm7uj6vjx797 sh:maxCount 1 .

observable:DefinedEffectFacet a sh:NodeShape .

_:node1gm7uj6vjx797 sh:nodeKind sh:Literal .

observable:DefinedEffectFacet rdfs:subClassOf core:Facet .

_:node1gm7uj6vjx797 sh:path observable:startTime .

observable:DefinedEffectFacet rdfs:label "DefinedEffectFacet"@en .

observable:CallFacet sh:property _:node1gm7uj6vjx797 .

_:node1gm7uj6vjx1272 rdf:first "TASK_EVENT_TRIGGER_AT_LOGON"^^vocabulary:TriggerFrequencyVocab .

_:node1gm7uj6vjx798 a rdfs:Datatype .

_:node1gm7uj6vjx1272 rdf:rest _:node1gm7uj6vjx1273 .

_:node1gm7uj6vjx799 sh:datatype xsd:integer .

observable:DefinedEffectFacet rdfs:comment "A defined effect facet is a grouping of characteristics unique to the effect of an observable action in relation to one or more observable objects."@en .

_:node1gm7uj6vjx798 owl:onDatatype xsd:string .

_:node1gm7uj6vjx1273 rdf:first "TASK_EVENT_TRIGGER_AT_SYSTEMSTART"^^vocabulary:TriggerFrequencyVocab .

_:node1gm7uj6vjx799 sh:maxCount 1 .

_:node1gm7uj6vjx1273 rdf:rest _:node1gm7uj6vjx1274 .

_:node1gm7uj6vjx799 sh:nodeKind sh:Literal .

observable:DefinedEffectFacet sh:targetClass observable:DefinedEffectFacet .

_:node1gm7uj6vjx799 sh:path observable:duration .

observable:Device a owl:Class .

observable:CallFacet sh:property _:node1gm7uj6vjx799 .

_:node1gm7uj6vjx1274 rdf:first "TASK_EVENT_TRIGGER_ON_IDLE"^^vocabulary:TriggerFrequencyVocab .

_:node1gm7uj6vjx801 sh:datatype xsd:string .

_:node1gm7uj6vjx1274 rdf:rest _:node1gm7uj6vjx1275 .

_:node1gm7uj6vjx801 sh:maxCount 1 .

observable:Device a sh:NodeShape .

_:node1gm7uj6vjx800 rdf:first "Bit-mapped"^^vocabulary:MemoryBlockTypeVocab .

observable:Device rdfs:subClassOf observable:ObservableObject .

_:node1gm7uj6vjx800 rdf:rest _:node1gm7uj6vjx802 .

_:node1gm7uj6vjx1275 rdf:first "TASK_TIME_TRIGGER_DAILY"^^vocabulary:TriggerFrequencyVocab .

_:node1gm7uj6vjx801 sh:nodeKind sh:Literal .

_:node1gm7uj6vjx1275 rdf:rest _:node1gm7uj6vjx1276 .

_:node1gm7uj6vjx801 sh:path observable:callType .

observable:Device rdfs:label "Device"@en .

observable:CallFacet sh:property _:node1gm7uj6vjx801 .

_:node1gm7uj6vjx1276 rdf:first "TASK_TIME_TRIGGER_MONTHLYDATE"^^vocabulary:TriggerFrequencyVocab .

observable:CallFacet sh:targetClass observable:CallFacet .

_:node1gm7uj6vjx1276 rdf:rest _:node1gm7uj6vjx1277 .

_:node1gm7uj6vjx802 rdf:first "Byte-mapped"^^vocabulary:MemoryBlockTypeVocab .

observable:Device rdfs:comment "A device is a piece of equipment or a mechanism designed to serve a special purpose or perform a special function. [based on https://www.merriam-webster.com/dictionary/device]"@en .

_:node1gm7uj6vjx802 rdf:rest _:node1gm7uj6vjx803 .

observable:Device sh:targetClass observable:Device .

observable:CapturedTelecommunicationsInformation a owl:Class .

_:node1gm7uj6vjx1277 rdf:first "TASK_TIME_TRIGGER_MONTHLYDOW"^^vocabulary:TriggerFrequencyVocab .

observable:CapturedTelecommunicationsInformation a sh:NodeShape .

_:node1gm7uj6vjx1277 rdf:rest _:node1gm7uj6vjx1278 .

observable:CapturedTelecommunicationsInformation rdfs:subClassOf observable:ObservableObject .

observable:DeviceFacet a owl:Class .

_:node1gm7uj6vjx803 rdf:first "Initialized"^^vocabulary:MemoryBlockTypeVocab .

observable:DeviceFacet a sh:NodeShape .

_:node1gm7uj6vjx803 rdf:rest _:node1gm7uj6vjx804 .

_:node1gm7uj6vjx1278 rdf:first "TASK_TIME_TRIGGER_ONCE"^^vocabulary:TriggerFrequencyVocab .

observable:CapturedTelecommunicationsInformation rdfs:label "CapturedTelecommunicationsInformation"@en .

observable:DeviceFacet rdfs:subClassOf core:Facet .

_:node1gm7uj6vjx1278 rdf:rest _:node1gm7uj6vjx1279 .

observable:DeviceFacet rdfs:label "DeviceFacet"@en .

_:node1gm7uj6vjx1279 rdf:first "TASK_TIME_TRIGGER_WEEKLY"^^vocabulary:TriggerFrequencyVocab ;
	rdf:rest rdf:nil .

_:node1gm7uj6vjx1271 owl:oneOf _:node1gm7uj6vjx1272 .

vocabulary:TriggerFrequencyVocab owl:equivalentClass _:node1gm7uj6vjx1271 .

vocabulary:TriggerTypeVocab a rdfs:Datatype .

observable:DeviceFacet rdfs:comment "A device facet is a grouping of characteristics unique to a piece of equipment or a mechanism designed to serve a special purpose or perform a special function. [based on https://www.merriam-webster.com/dictionary/device]"@en .

vocabulary:TriggerTypeVocab rdfs:label "Trigger Type Vocabulary"@en-us .

_:node1gm7uj6vjx1280 sh:class identity:Identity .

vocabulary:TriggerTypeVocab rdfs:comment "Defines an open-vocabulary of the types of triggers associated with a task."@en .

_:node1gm7uj6vjx1280 sh:maxCount 1 ;
	sh:nodeKind sh:IRI .

_:node1gm7uj6vjx1281 a rdfs:Datatype .

_:node1gm7uj6vjx1280 sh:path observable:manufacturer .

observable:DeviceFacet sh:property _:node1gm7uj6vjx1280 .

_:node1gm7uj6vjx1281 owl:onDatatype xsd:string .

_:node1gm7uj6vjx1282 sh:datatype xsd:string .

_:node1gm7uj6vjx1283 rdf:first "TASK_TRIGGER_BOOT"^^vocabulary:TriggerTypeVocab ;
	rdf:rest _:node1gm7uj6vjx1284 .

_:node1gm7uj6vjx1282 sh:maxCount 1 ;
	sh:nodeKind sh:Literal .

_:node1gm7uj6vjx1284 rdf:first "TASK_TRIGGER_EVENT"^^vocabulary:TriggerTypeVocab ;
	rdf:rest _:node1gm7uj6vjx1285 .

_:node1gm7uj6vjx1282 sh:path observable:deviceType .

observable:DeviceFacet sh:property _:node1gm7uj6vjx1282 .

_:node1gm7uj6vjx1285 rdf:first "TASK_TRIGGER_IDLE"^^vocabulary:TriggerTypeVocab .

_:node1gm7uj6vjx1286 sh:datatype xsd:string .

_:node1gm7uj6vjx1285 rdf:rest _:node1gm7uj6vjx1287 .

_:node1gm7uj6vjx1286 sh:maxCount 1 .

_:node1gm7uj6vjx1287 rdf:first "TASK_TRIGGER_LOGON"^^vocabulary:TriggerTypeVocab ;
	rdf:rest _:node1gm7uj6vjx1288 .

_:node1gm7uj6vjx1286 sh:nodeKind sh:Literal ;
	sh:path observable:model .

observable:DeviceFacet sh:property _:node1gm7uj6vjx1286 .

_:node1gm7uj6vjx1288 rdf:first "TASK_TRIGGER_REGISTRATION"^^vocabulary:TriggerTypeVocab ;
	rdf:rest _:node1gm7uj6vjx1290 .

_:node1gm7uj6vjx1289 sh:datatype xsd:string ;
	sh:maxCount 1 .

_:node1gm7uj6vjx1290 rdf:first "TASK_TRIGGER_SESSION_STATE_CHANGE"^^vocabulary:TriggerTypeVocab ;
	rdf:rest _:node1gm7uj6vjx1291 .

_:node1gm7uj6vjx1289 sh:nodeKind sh:Literal .

_:node1gm7uj6vjx1291 rdf:first "TASK_TRIGGER_TIME"^^vocabulary:TriggerTypeVocab ;
	rdf:rest rdf:nil .

_:node1gm7uj6vjx1281 owl:oneOf _:node1gm7uj6vjx1283 .

_:node1gm7uj6vjx1289 sh:path observable:serialNumber .

vocabulary:TriggerTypeVocab owl:equivalentClass _:node1gm7uj6vjx1281 .

observable:DeviceFacet sh:property _:node1gm7uj6vjx1289 ;
	sh:targetClass observable:DeviceFacet .

vocabulary:URLTransitionTypeVocab a rdfs:Datatype .

observable:DigitalAccount a owl:Class , sh:NodeShape .

vocabulary:URLTransitionTypeVocab rdfs:label "URL Transition Type Vocabulary"@en-us .

observable:DigitalAccount rdfs:subClassOf observable:Account ;
	rdfs:label "DigitalAccount"@en .

vocabulary:URLTransitionTypeVocab rdfs:comment "Defines an open-vocabulary of types of URL transitions."@en .

_:node1gm7uj6vjx1292 a rdfs:Datatype .

observable:DigitalAccount rdfs:comment "A digital account is an arrangement with an entity to enable and control the provision of some capability or service within the digital domain."@en .

_:node1gm7uj6vjx1292 owl:onDatatype xsd:string .

observable:DigitalAccount sh:targetClass observable:DigitalAccount .

_:node1gm7uj6vjx1293 rdf:first "link"^^vocabulary:URLTransitionTypeVocab ;
	rdf:rest _:node1gm7uj6vjx1294 .

observable:DigitalAccountFacet a owl:Class , sh:NodeShape .

_:node1gm7uj6vjx1294 rdf:first "typed"^^vocabulary:URLTransitionTypeVocab .

observable:DigitalAccountFacet rdfs:subClassOf core:Facet .

_:node1gm7uj6vjx1294 rdf:rest _:node1gm7uj6vjx1295 .

observable:DigitalAccountFacet rdfs:label "DigitalAccountFacet"@en .

_:node1gm7uj6vjx1295 rdf:first "auto_bookmark"^^vocabulary:URLTransitionTypeVocab ;
	rdf:rest _:node1gm7uj6vjx1296 .

observable:DigitalAccountFacet rdfs:comment "A digital account facet is a grouping of characteristics unique to an arrangement with an entity to enable and control the provision of some capability or service within the digital domain."@en .

_:node1gm7uj6vjx1296 rdf:first "auto_subframe"^^vocabulary:URLTransitionTypeVocab ;
	rdf:rest _:node1gm7uj6vjx1298 .

_:node1gm7uj6vjx1297 sh:datatype xsd:boolean .

_:node1gm7uj6vjx1298 rdf:first "manual_subframe"^^vocabulary:URLTransitionTypeVocab .

_:node1gm7uj6vjx1297 sh:maxCount 1 .

_:node1gm7uj6vjx1298 rdf:rest _:node1gm7uj6vjx1299 .

_:node1gm7uj6vjx1297 sh:nodeKind sh:Literal .

_:node1gm7uj6vjx1299 rdf:first "generated"^^vocabulary:URLTransitionTypeVocab .

_:node1gm7uj6vjx1297 sh:path observable:isDisabled .

observable:DigitalAccountFacet sh:property _:node1gm7uj6vjx1297 .

_:node1gm7uj6vjx1299 rdf:rest _:node1gm7uj6vjx1300 .

_:node1gm7uj6vjx1301 sh:datatype xsd:dateTime .

_:node1gm7uj6vjx1300 rdf:first "auto_toplevel"^^vocabulary:URLTransitionTypeVocab ;
	rdf:rest _:node1gm7uj6vjx1302 .

_:node1gm7uj6vjx1301 sh:maxCount 1 ;
	sh:nodeKind sh:Literal .

_:node1gm7uj6vjx1302 rdf:first "form_submit"^^vocabulary:URLTransitionTypeVocab ;
	rdf:rest _:node1gm7uj6vjx1303 .

_:node1gm7uj6vjx1301 sh:path observable:firstLoginTime .

observable:DigitalAccountFacet sh:property _:node1gm7uj6vjx1301 .

_:node1gm7uj6vjx1304 sh:datatype xsd:dateTime .

_:node1gm7uj6vjx1303 rdf:first "reload"^^vocabulary:URLTransitionTypeVocab ;
	rdf:rest _:node1gm7uj6vjx1305 .

_:node1gm7uj6vjx1304 sh:maxCount 1 .

_:node1gm7uj6vjx1305 rdf:first "keyword"^^vocabulary:URLTransitionTypeVocab ;
	rdf:rest _:node1gm7uj6vjx1306 .

_:node1gm7uj6vjx1304 sh:nodeKind sh:Literal ;
	sh:path observable:lastLoginTime .

observable:DigitalAccountFacet sh:property _:node1gm7uj6vjx1304 .

_:node1gm7uj6vjx1306 rdf:first "keyword_generated"^^vocabulary:URLTransitionTypeVocab ;
	rdf:rest rdf:nil .

_:node1gm7uj6vjx1292 owl:oneOf _:node1gm7uj6vjx1293 .

_:node1gm7uj6vjx1307 sh:datatype xsd:string .

vocabulary:URLTransitionTypeVocab owl:equivalentClass _:node1gm7uj6vjx1292 .

_:node1gm7uj6vjx1307 sh:maxCount 1 .

vocabulary:UnixProcessStateVocab a rdfs:Datatype .

_:node1gm7uj6vjx1307 sh:nodeKind sh:Literal ;
	sh:path observable:displayName .

observable:DigitalAccountFacet sh:property _:node1gm7uj6vjx1307 .

vocabulary:UnixProcessStateVocab rdfs:label "UNIX Process State Vocabulary"@en-us .

_:node1gm7uj6vjx1308 sh:datatype xsd:string ;
	sh:nodeKind sh:Literal .

vocabulary:UnixProcessStateVocab rdfs:comment "Defines an open-vocabulary of Unix process states"@en .

_:node1gm7uj6vjx1308 sh:path observable:accountLogin .

observable:DigitalAccountFacet sh:property _:node1gm7uj6vjx1308 .

_:node1gm7uj6vjx1309 a rdfs:Datatype ;
	owl:onDatatype xsd:string .

observable:DigitalAccountFacet sh:targetClass observable:DigitalAccountFacet .

observable:DigitalAddress a owl:Class , sh:NodeShape .

_:node1gm7uj6vjx1310 rdf:first "Dead"^^vocabulary:UnixProcessStateVocab ;
	rdf:rest _:node1gm7uj6vjx1311 .

observable:DigitalAddress rdfs:subClassOf observable:Address ;
	rdfs:label "DigitalAddress"@en .

_:node1gm7uj6vjx1311 rdf:first "InterruptibleSleep"^^vocabulary:UnixProcessStateVocab ;
	rdf:rest _:node1gm7uj6vjx1312 .

observable:DigitalAddress rdfs:comment "A digital address is an identifier assigned to enable routing and management of digital communication."@en .

_:node1gm7uj6vjx1312 rdf:first "Paging"^^vocabulary:UnixProcessStateVocab ;
	rdf:rest _:node1gm7uj6vjx1313 .

observable:DigitalAddress sh:targetClass observable:DigitalAddress .

_:node1gm7uj6vjx1313 rdf:first "Running"^^vocabulary:UnixProcessStateVocab ;
	rdf:rest _:node1gm7uj6vjx1314 .

observable:DigitalAddressFacet a owl:Class , sh:NodeShape ;
	rdfs:subClassOf core:Facet ;
	rdfs:label "DigitalAddressFacet"@en .

_:node1gm7uj6vjx1314 rdf:first "Stopped"^^vocabulary:UnixProcessStateVocab ;
	rdf:rest _:node1gm7uj6vjx1315 .

_:node1gm7uj6vjx1315 rdf:first "UninterruptibleSleep"^^vocabulary:UnixProcessStateVocab ;
	rdf:rest _:node1gm7uj6vjx1316 .

observable:DigitalAddressFacet rdfs:comment "A digital address facet is a grouping of characteristics unique to an identifier assigned to enable routing and management of digital communication."@en .

_:node1gm7uj6vjx1317 sh:datatype xsd:string .

_:node1gm7uj6vjx1316 rdf:first "Zombie"^^vocabulary:UnixProcessStateVocab ;
	rdf:rest rdf:nil .

_:node1gm7uj6vjx1309 owl:oneOf _:node1gm7uj6vjx1310 .

vocabulary:UnixProcessStateVocab owl:equivalentClass _:node1gm7uj6vjx1309 .

_:node1gm7uj6vjx1317 sh:maxCount 1 ;
	sh:nodeKind sh:Literal .

vocabulary:WhoisContactTypeVocab a rdfs:Datatype .

_:node1gm7uj6vjx1317 sh:path observable:addressValue .

observable:DigitalAddressFacet sh:property _:node1gm7uj6vjx1317 .

_:node1gm7uj6vjx1318 sh:datatype xsd:string .

vocabulary:WhoisContactTypeVocab rdfs:label "Whois Contact Type Vocabulary"@en-us .

_:node1gm7uj6vjx1318 sh:maxCount 1 .

vocabulary:WhoisContactTypeVocab rdfs:comment "Defines an open-vocabulary of types of registrar contacts listed in a whois entry."@en .

_:node1gm7uj6vjx1318 sh:nodeKind sh:Literal ;
	sh:path observable:displayName .

observable:DigitalAddressFacet sh:property _:node1gm7uj6vjx1318 .

_:node1gm7uj6vjx1319 a rdfs:Datatype .

observable:DigitalAddressFacet sh:targetClass observable:DigitalAddressFacet .

_:node1gm7uj6vjx1319 owl:onDatatype xsd:string .

observable:DigitalCamera a owl:Class , sh:NodeShape .

_:node1gm7uj6vjx1320 rdf:first "ADMIN"^^vocabulary:WhoisContactTypeVocab .

observable:DigitalCamera rdfs:subClassOf observable:Device .

_:node1gm7uj6vjx1320 rdf:rest _:node1gm7uj6vjx1321 .

_:node1gm7uj6vjx1321 rdf:first "BILLING"^^vocabulary:WhoisContactTypeVocab ;
	rdf:rest _:node1gm7uj6vjx1322 .

_:node1gm7uj6vjx1322 rdf:first "TECHNICAL"^^vocabulary:WhoisContactTypeVocab .

observable:DigitalCamera rdfs:label "DigitalCamera"@en-us .

_:node1gm7uj6vjx1322 rdf:rest rdf:nil .

_:node1gm7uj6vjx1319 owl:oneOf _:node1gm7uj6vjx1320 .

vocabulary:WhoisContactTypeVocab owl:equivalentClass _:node1gm7uj6vjx1319 .

vocabulary:WhoisDNSSECTypeVocab a rdfs:Datatype .

observable:DigitalCamera rdfs:comment "A digital camera is a camera that captures photographs in digital memory as opposed to capturing images on photographic film."@en-us .

vocabulary:WhoisDNSSECTypeVocab rdfs:label "Whois DNSSEC Type Vocabulary"@en-us .

observable:DigitalCamera sh:targetClass observable:DigitalCamera .

vocabulary:WhoisDNSSECTypeVocab rdfs:comment "Defines an open-vocabulary of acceptable values for the DNSSEC field in a Whois entry."@en .

_:node1gm7uj6vjx1323 a rdfs:Datatype .

observable:DigitalSignatureInfo a owl:Class .

_:node1gm7uj6vjx1323 owl:onDatatype xsd:string .

observable:DigitalSignatureInfo a sh:NodeShape .

_:node1gm7uj6vjx1324 rdf:first "Signed"^^vocabulary:WhoisDNSSECTypeVocab ;
	rdf:rest _:node1gm7uj6vjx1325 .

observable:DigitalSignatureInfo rdfs:subClassOf observable:ObservableObject .

_:node1gm7uj6vjx1325 rdf:first "Unsigned"^^vocabulary:WhoisDNSSECTypeVocab ;
	rdf:rest rdf:nil .

_:node1gm7uj6vjx1323 owl:oneOf _:node1gm7uj6vjx1324 .

vocabulary:WhoisDNSSECTypeVocab owl:equivalentClass _:node1gm7uj6vjx1323 .

observable:DigitalSignatureInfo rdfs:label "DigitalSignatureInfo"@en .

vocabulary:WhoisStatusTypeVocab a rdfs:Datatype ;
	rdfs:label "Whois Status Type Vocabulary"@en-us .

observable:DigitalSignatureInfo rdfs:comment "A digital signature info is a value calculated via a mathematical scheme for demonstrating the authenticity of an electronic message or document."@en .

vocabulary:WhoisStatusTypeVocab rdfs:comment "Defines an open-vocabulary of all valid statuses for a domain within a whois entry."@en .

_:node1gm7uj6vjx1326 a rdfs:Datatype .

observable:DigitalSignatureInfo sh:targetClass observable:DigitalSignatureInfo .

_:node1gm7uj6vjx1326 owl:onDatatype xsd:string .

observable:DigitalSignatureInfoFacet a owl:Class , sh:NodeShape .

_:node1gm7uj6vjx1327 rdf:first "ADD_PERIOD"^^vocabulary:WhoisStatusTypeVocab .

observable:DigitalSignatureInfoFacet rdfs:subClassOf core:Facet .

_:node1gm7uj6vjx1327 rdf:rest _:node1gm7uj6vjx1328 .

observable:DigitalSignatureInfoFacet rdfs:label "DigitalSignatureInfoFacet"@en .

_:node1gm7uj6vjx1328 rdf:first "AUTO_RENEW_PERIOD"^^vocabulary:WhoisStatusTypeVocab ;
	rdf:rest _:node1gm7uj6vjx1329 .

_:node1gm7uj6vjx1329 rdf:first "CLIENT_DELETE_PROHIBITED"^^vocabulary:WhoisStatusTypeVocab ;
	rdf:rest _:node1gm7uj6vjx1330 .

observable:DigitalSignatureInfoFacet rdfs:comment "A digital signature info facet is a grouping of characteristics unique to a value calculated via a mathematical scheme for demonstrating the authenticity of an electronic message or document."@en .

_:node1gm7uj6vjx1330 rdf:first "CLIENT_HOLD"^^vocabulary:WhoisStatusTypeVocab ;
	rdf:rest _:node1gm7uj6vjx1332 .

_:node1gm7uj6vjx1331 sh:class core:UcoObject .

_:node1gm7uj6vjx1332 rdf:first "CLIENT_RENEW_PROHIBITED"^^vocabulary:WhoisStatusTypeVocab ;
	rdf:rest _:node1gm7uj6vjx1333 .

_:node1gm7uj6vjx1333 rdf:first "CLIENT_TRANSFER_PROHIBITED"^^vocabulary:WhoisStatusTypeVocab ;
	rdf:rest _:node1gm7uj6vjx1334 .

_:node1gm7uj6vjx1331 sh:maxCount 1 .

_:node1gm7uj6vjx1334 rdf:first "CLIENT_UPDATE_PROHIBITED"^^vocabulary:WhoisStatusTypeVocab ;
	rdf:rest _:node1gm7uj6vjx1335 .

_:node1gm7uj6vjx1331 sh:nodeKind sh:IRI .

_:node1gm7uj6vjx1335 rdf:first "DELETE_PROHIBITED"^^vocabulary:WhoisStatusTypeVocab ;
	rdf:rest _:node1gm7uj6vjx1336 .

_:node1gm7uj6vjx1331 sh:path observable:certificateSubject .

observable:DigitalSignatureInfoFacet sh:property _:node1gm7uj6vjx1331 .

_:node1gm7uj6vjx1336 rdf:first "HOLD"^^vocabulary:WhoisStatusTypeVocab ;
	rdf:rest _:node1gm7uj6vjx1338 .

_:node1gm7uj6vjx1337 sh:class identity:Identity .

_:node1gm7uj6vjx1338 rdf:first "INACTIVE"^^vocabulary:WhoisStatusTypeVocab ;
	rdf:rest _:node1gm7uj6vjx1339 .

_:node1gm7uj6vjx1339 rdf:first "OK"^^vocabulary:WhoisStatusTypeVocab ;
	rdf:rest _:node1gm7uj6vjx1340 .

_:node1gm7uj6vjx1337 sh:maxCount 1 .

_:node1gm7uj6vjx1340 rdf:first "PENDING_DELETE_RESTORABLE"^^vocabulary:WhoisStatusTypeVocab ;
	rdf:rest _:node1gm7uj6vjx1341 .

_:node1gm7uj6vjx1337 sh:nodeKind sh:IRI .

_:node1gm7uj6vjx1341 rdf:first "PENDING_DELETE_SCHEDULED_FOR_RELEASE"^^vocabulary:WhoisStatusTypeVocab ;
	rdf:rest _:node1gm7uj6vjx1342 .

_:node1gm7uj6vjx1337 sh:path observable:certificateIssuer .

observable:DigitalSignatureInfoFacet sh:property _:node1gm7uj6vjx1337 .

_:node1gm7uj6vjx1342 rdf:first "PENDING_RESTORE"^^vocabulary:WhoisStatusTypeVocab ;
	rdf:rest _:node1gm7uj6vjx1344 .

_:node1gm7uj6vjx1343 sh:datatype xsd:boolean .

_:node1gm7uj6vjx1344 rdf:first "RENEW_PERIOD"^^vocabulary:WhoisStatusTypeVocab ;
	rdf:rest _:node1gm7uj6vjx1345 .

_:node1gm7uj6vjx1343 sh:maxCount 1 .

_:node1gm7uj6vjx1345 rdf:first "RENEW_PROHIBITED"^^vocabulary:WhoisStatusTypeVocab ;
	rdf:rest _:node1gm7uj6vjx1346 .

_:node1gm7uj6vjx1346 rdf:first "TRANSFER_PERIOD"^^vocabulary:WhoisStatusTypeVocab .

_:node1gm7uj6vjx1343 sh:nodeKind sh:Literal .

_:node1gm7uj6vjx1346 rdf:rest _:node1gm7uj6vjx1347 .

_:node1gm7uj6vjx1347 rdf:first "TRANSFER_PROHIBITED"^^vocabulary:WhoisStatusTypeVocab .

_:node1gm7uj6vjx1343 sh:path observable:signatureExists .

_:node1gm7uj6vjx1347 rdf:rest _:node1gm7uj6vjx1348 .

observable:DigitalSignatureInfoFacet sh:property _:node1gm7uj6vjx1343 .

_:node1gm7uj6vjx1348 rdf:first "UPDATE_PROHIBITED"^^vocabulary:WhoisStatusTypeVocab ;
	rdf:rest rdf:nil .

_:node1gm7uj6vjx1326 owl:oneOf _:node1gm7uj6vjx1327 .

vocabulary:WhoisStatusTypeVocab owl:equivalentClass _:node1gm7uj6vjx1326 .

_:node1gm7uj6vjx1349 sh:datatype xsd:boolean .

vocabulary:WindowsDriveTypeVocab a rdfs:Datatype .

_:node1gm7uj6vjx1349 sh:maxCount 1 ;
	sh:nodeKind sh:Literal .

vocabulary:WindowsDriveTypeVocab rdfs:label "Windows Drive Type Vocabulary"@en-us .

_:node1gm7uj6vjx1349 sh:path observable:signatureVerified .

observable:DigitalSignatureInfoFacet sh:property _:node1gm7uj6vjx1349 .

_:node1gm7uj6vjx1350 sh:datatype xsd:string .

vocabulary:WindowsDriveTypeVocab rdfs:comment "Defines an open-vocabulary of possible drive types, as enumerated by the WINAPI GetDriveType function: http://msdn.microsoft.com/en-us/library/windows/desktop/aa364939(v=vs.85).aspx."@en .

_:node1gm7uj6vjx1351 a rdfs:Datatype ;
	owl:onDatatype xsd:string .

_:node1gm7uj6vjx1350 sh:maxCount 1 .

_:node1gm7uj6vjx1352 rdf:first "DRIVE_CDROM"^^vocabulary:WindowsDriveTypeVocab ;
	rdf:rest _:node1gm7uj6vjx1353 .

_:node1gm7uj6vjx1350 sh:nodeKind sh:Literal .

_:node1gm7uj6vjx1353 rdf:first "DRIVE_FIXED"^^vocabulary:WindowsDriveTypeVocab .

_:node1gm7uj6vjx1350 sh:path observable:signatureDescription .

_:node1gm7uj6vjx1353 rdf:rest _:node1gm7uj6vjx1354 .

observable:DigitalSignatureInfoFacet sh:property _:node1gm7uj6vjx1350 .

_:node1gm7uj6vjx1354 rdf:first "DRIVE_NO_ROOT_DIR"^^vocabulary:WindowsDriveTypeVocab ;
	rdf:rest _:node1gm7uj6vjx1355 .

observable:DigitalSignatureInfoFacet sh:targetClass observable:DigitalSignatureInfoFacet .

_:node1gm7uj6vjx1355 rdf:first "DRIVE_RAMDISK"^^vocabulary:WindowsDriveTypeVocab ;
	rdf:rest _:node1gm7uj6vjx1356 .

_:node1gm7uj6vjx1356 rdf:first "DRIVE_REMOTE"^^vocabulary:WindowsDriveTypeVocab ;
	rdf:rest _:node1gm7uj6vjx1357 .

observable:Directory a owl:Class .

_:node1gm7uj6vjx1357 rdf:first "DRIVE_REMOVABLE"^^vocabulary:WindowsDriveTypeVocab ;
	rdf:rest _:node1gm7uj6vjx1358 .

observable:Directory a sh:NodeShape .

_:node1gm7uj6vjx1358 rdf:first "DRIVE_UNKNOWN"^^vocabulary:WindowsDriveTypeVocab ;
	rdf:rest rdf:nil .

_:node1gm7uj6vjx1351 owl:oneOf _:node1gm7uj6vjx1352 .

vocabulary:WindowsDriveTypeVocab owl:equivalentClass _:node1gm7uj6vjx1351 .

observable:Directory rdfs:subClassOf observable:FileSystemObject .

vocabulary:WindowsVolumeAttributeVocab a rdfs:Datatype ;
	rdfs:label "Windows Volume Attribute Vocabulary"@en-us .

observable:Directory rdfs:label "Directory"@en .

vocabulary:WindowsVolumeAttributeVocab rdfs:comment "Defines an open-vocabulary of attributes that may be returned by the diskpart attributes command: http://technet.microsoft.com/en-us/library/cc766465(v=ws.10).aspx."@en .

_:node1gm7uj6vjx1359 a rdfs:Datatype ;
	owl:onDatatype xsd:string .

_:node1gm7uj6vjx1360 rdf:first "Hidden"^^vocabulary:WindowsVolumeAttributeVocab ;
	rdf:rest _:node1gm7uj6vjx1361 .

_:node1gm7uj6vjx1361 rdf:first "NoDefaultDriveLetter"^^vocabulary:WindowsVolumeAttributeVocab ;
	rdf:rest _:node1gm7uj6vjx1362 .

_:node1gm7uj6vjx1362 rdf:first "ReadOnly"^^vocabulary:WindowsVolumeAttributeVocab ;
	rdf:rest _:node1gm7uj6vjx1363 .

_:node1gm7uj6vjx1363 rdf:first "ShadowCopy"^^vocabulary:WindowsVolumeAttributeVocab ;
	rdf:rest rdf:nil .

_:node1gm7uj6vjx1359 owl:oneOf _:node1gm7uj6vjx1360 .

vocabulary:WindowsVolumeAttributeVocab owl:equivalentClass _:node1gm7uj6vjx1359 .

vocabulary:WirelessNetworkSecurityModeVocab a rdfs:Datatype ;
	rdfs:label "Wireless Network Security Mode Vocabulary"@en-us ;
	rdfs:comment "Defines an open-vocabulary of security modes that may be configured for wireless network connections."@en .

_:node1gm7uj6vjx1364 a rdfs:Datatype ;
	owl:onDatatype xsd:string .

_:node1gm7uj6vjx1365 rdf:first "None"^^vocabulary:WirelessNetworkSecurityModeVocab ;
	rdf:rest _:node1gm7uj6vjx1366 .

_:node1gm7uj6vjx1366 rdf:first "WEP"^^vocabulary:WirelessNetworkSecurityModeVocab ;
	rdf:rest _:node1gm7uj6vjx1367 .

_:node1gm7uj6vjx1367 rdf:first "WPA"^^vocabulary:WirelessNetworkSecurityModeVocab ;
	rdf:rest _:node1gm7uj6vjx1368 .

_:node1gm7uj6vjx1368 rdf:first "WPA2-PSK"^^vocabulary:WirelessNetworkSecurityModeVocab ;
	rdf:rest _:node1gm7uj6vjx1369 .

_:node1gm7uj6vjx1369 rdf:first "WPA2-Enterprise"^^vocabulary:WirelessNetworkSecurityModeVocab ;
	rdf:rest _:node1gm7uj6vjx1370 .

_:node1gm7uj6vjx1370 rdf:first "WPA3-PSK"^^vocabulary:WirelessNetworkSecurityModeVocab ;
	rdf:rest _:node1gm7uj6vjx1371 .

_:node1gm7uj6vjx1371 rdf:first "WPA3-Enterprise"^^vocabulary:WirelessNetworkSecurityModeVocab ;
	rdf:rest rdf:nil .

_:node1gm7uj6vjx1364 owl:oneOf _:node1gm7uj6vjx1365 .

vocabulary:WirelessNetworkSecurityModeVocab owl:equivalentClass _:node1gm7uj6vjx1364 .

observable:Directory rdfs:comment "A directory is a file system cataloging structure which contains references to other computer files, and possibly other directories. On many computers, directories are known as folders, or drawers, analogous to a workbench or the traditional office filing cabinet. In UNIX a directory is implemented as a special file. [based on https://en.wikipedia.org/wiki/Directory_(computing)]"@en ;
	sh:targetClass observable:Directory .

observable:Disk a owl:Class , sh:NodeShape ;
	rdfs:subClassOf observable:ObservableObject ;
	rdfs:label "Disk"@en ;
	rdfs:comment "A disk is a storage mechanism where data is recorded by various electronic, magnetic, optical, or mechanical changes to a surface layer of one or more rotating disks."@en ;
	sh:targetClass observable:Disk .

observable:DiskFacet a owl:Class , sh:NodeShape ;
	rdfs:subClassOf core:Facet ;
	rdfs:label "DiskFacet"@en ;
	rdfs:comment "A disk facet is a grouping of characteristics unique to a storage mechanism where data is recorded by various electronic, magnetic, optical, or mechanical changes to a surface layer of one or more rotating disks."@en .

_:node1gm7uj6vjx1372 sh:class observable:ObservableObject ;
	sh:nodeKind sh:IRI ;
	sh:path observable:partition .

observable:DiskFacet sh:property _:node1gm7uj6vjx1372 .

_:node1gm7uj6vjx1373 sh:datatype xsd:integer ;
	sh:maxCount 1 ;
	sh:nodeKind sh:Literal ;
	sh:path observable:diskSize .

observable:DiskFacet sh:property _:node1gm7uj6vjx1373 .

_:node1gm7uj6vjx1374 sh:datatype xsd:integer ;
	sh:maxCount 1 ;
	sh:nodeKind sh:Literal ;
	sh:path observable:freeSpace .

observable:DiskFacet sh:property _:node1gm7uj6vjx1374 .

_:node1gm7uj6vjx1375 sh:datatype xsd:string ;
	sh:maxCount 1 ;
	sh:nodeKind sh:Literal ;
	sh:path observable:diskType .

observable:DiskFacet sh:property _:node1gm7uj6vjx1375 ;
	sh:targetClass observable:DiskFacet .

observable:DiskPartition a owl:Class , sh:NodeShape ;
	rdfs:subClassOf observable:ObservableObject ;
	rdfs:label "DiskPartition"@en ;
	rdfs:comment "A disk partition is a particular managed region on a storage mechanism where data is recorded by various electronic, magnetic, optical, or mechanical changes to a surface layer of one or more rotating disks. [based on https://en.wikipedia.org/wiki/Disk_storage]"@en ;
	sh:targetClass observable:DiskPartition .

observable:DiskPartitionFacet a owl:Class , sh:NodeShape ;
	rdfs:subClassOf core:Facet ;
	rdfs:label "DiskPartitionFacet"@en ;
	rdfs:comment "A disk partition facet is a grouping of characteristics unique to a particular managed region on a storage mechanism."@en .

_:node1gm7uj6vjx1376 sh:datatype xsd:dateTime ;
	sh:maxCount 1 ;
	sh:nodeKind sh:Literal ;
	sh:path observable:observableCreatedTime .

observable:DiskPartitionFacet sh:property _:node1gm7uj6vjx1376 .

_:node1gm7uj6vjx1377 sh:datatype xsd:integer ;
	sh:maxCount 1 ;
	sh:nodeKind sh:Literal ;
	sh:path observable:partitionLength .

observable:DiskPartitionFacet sh:property _:node1gm7uj6vjx1377 .

_:node1gm7uj6vjx1378 sh:datatype xsd:integer ;
	sh:maxCount 1 ;
	sh:nodeKind sh:Literal ;
	sh:path observable:partitionOffset .

observable:DiskPartitionFacet sh:property _:node1gm7uj6vjx1378 .

_:node1gm7uj6vjx1379 sh:datatype xsd:integer ;
	sh:maxCount 1 ;
	sh:nodeKind sh:Literal ;
	sh:path observable:spaceLeft .

observable:DiskPartitionFacet sh:property _:node1gm7uj6vjx1379 .

_:node1gm7uj6vjx1380 sh:datatype xsd:integer ;
	sh:maxCount 1 ;
	sh:nodeKind sh:Literal ;
	sh:path observable:spaceUsed .

observable:DiskPartitionFacet sh:property _:node1gm7uj6vjx1380 .

_:node1gm7uj6vjx1381 sh:datatype xsd:integer ;
	sh:maxCount 1 ;
	sh:nodeKind sh:Literal ;
	sh:path observable:totalSpace .

observable:DiskPartitionFacet sh:property _:node1gm7uj6vjx1381 .

_:node1gm7uj6vjx1382 sh:datatype xsd:string ;
	sh:maxCount 1 ;
	sh:nodeKind sh:Literal ;
	sh:path observable:diskPartitionType .

observable:DiskPartitionFacet sh:property _:node1gm7uj6vjx1382 .

_:node1gm7uj6vjx1383 sh:datatype xsd:string ;
	sh:maxCount 1 ;
	sh:nodeKind sh:Literal ;
	sh:path observable:mountPoint .

observable:DiskPartitionFacet sh:property _:node1gm7uj6vjx1383 .

_:node1gm7uj6vjx1384 sh:datatype xsd:string ;
	sh:maxCount 1 ;
	sh:nodeKind sh:Literal ;
	sh:path observable:partitionID .

observable:DiskPartitionFacet sh:property _:node1gm7uj6vjx1384 ;
	sh:targetClass observable:DiskPartitionFacet .

observable:DomainName a owl:Class , sh:NodeShape ;
	rdfs:subClassOf observable:ObservableObject ;
	rdfs:label "DomainName"@en ;
	rdfs:comment "A domain name is an identification string that defines a realm of administrative autonomy, authority or control within the Internet. [based on https://en.wikipedia.org/wiki/Domain_name]"@en ;
	sh:targetClass observable:DomainName .

observable:DomainNameFacet a owl:Class , sh:NodeShape ;
	rdfs:subClassOf core:Facet ;
	rdfs:label "DomainNameFacet"@en ;
	rdfs:comment "A domain name facet is a grouping of characteristics unique to an identification string that defines a realm of administrative autonomy, authority or control within the Internet. [based on https://en.wikipedia.org/wiki/Domain_name]"@en .

_:node1gm7uj6vjx1385 sh:datatype xsd:boolean ;
	sh:maxCount 1 ;
	sh:nodeKind sh:Literal ;
	sh:path observable:isTLD .

observable:DomainNameFacet sh:property _:node1gm7uj6vjx1385 .

_:node1gm7uj6vjx1386 sh:datatype xsd:string ;
	sh:maxCount 1 ;
	sh:nodeKind sh:Literal ;
	sh:path observable:value .

observable:DomainNameFacet sh:property _:node1gm7uj6vjx1386 ;
	sh:targetClass observable:DomainNameFacet .

observable:Drone a owl:Class , sh:NodeShape ;
	rdfs:subClassOf observable:MobileDevice ;
	rdfs:label "Drone"@en-us ;
	rdfs:comment "A drone, unmanned aerial vehicle (UAV), is an aircraft without a human pilot, crew, or passengers that typically involve a ground-based controller and a system for communications with the UAV."@en-us ;
	sh:targetClass observable:Drone .

observable:ESN a owl:DatatypeProperty ;
	rdfs:label "ESN"@en ;
	rdfs:comment "Electronic Serial Number ."@en ;
	rdfs:range xsd:string .

observable:EXIFFacet a owl:Class , sh:NodeShape ;
	rdfs:subClassOf core:Facet ;
	rdfs:label "EXIFFacet"@en ;
	rdfs:comment "An EXIF (exchangeable image file format) facet is a grouping of characteristics unique to the formats for images, sound, and ancillary tags used by digital cameras (including smartphones), scanners and other systems handling image and sound files recorded by digital cameras conformant to JEIDA/JEITA/CIPA specifications. [based on https://en.wikipedia.org/wiki/Exif]"@en .

_:node1gm7uj6vjx1387 sh:class types:ControlledDictionary ;
	sh:nodeKind sh:IRI ;
	sh:path observable:exifData .

observable:EXIFFacet sh:property _:node1gm7uj6vjx1387 ;
	sh:targetClass observable:EXIFFacet .

observable:EmailAccount a owl:Class , sh:NodeShape ;
	rdfs:subClassOf observable:DigitalAccount ;
	rdfs:label "EmailAccount"@en ;
	rdfs:comment "An email account is an arrangement with an entity to enable and control the provision of electronic mail (email) capabilities or services."@en ;
	sh:targetClass observable:EmailAccount .

observable:EmailAccountFacet a owl:Class , sh:NodeShape ;
	rdfs:subClassOf core:Facet ;
	rdfs:label "EmailAccountFacet"@en ;
	rdfs:comment "An email account facet is a grouping of characteristics unique to an arrangement with an entity to enable and control the provision of electronic mail (email) capabilities or services."@en .

_:node1gm7uj6vjx1388 sh:class observable:ObservableObject ;
	sh:maxCount 1 ;
	sh:nodeKind sh:IRI ;
	sh:path observable:emailAddress .

observable:EmailAccountFacet sh:property _:node1gm7uj6vjx1388 ;
	sh:targetClass observable:EmailAccountFacet .

observable:EmailAddress a owl:Class , sh:NodeShape ;
	rdfs:subClassOf observable:DigitalAddress ;
	rdfs:label "EmailAddress"@en ;
	rdfs:comment "An email address is an identifier for an electronic mailbox to which electronic mail messages (conformant to the Simple Mail Transfer Protocol (SMTP)) are sent from and delivered to."@en ;
	sh:targetClass observable:EmailAddress .

observable:EmailAddressFacet a owl:Class , sh:NodeShape ;
	rdfs:subClassOf observable:DigitalAddressFacet ;
	rdfs:label "EmailAddressFacet"@en ;
	rdfs:comment "An email address facet is a grouping of characteristics unique to an identifier for an electronic mailbox to which electronic mail messages (conformant to the Simple Mail Transfer Protocol (SMTP)) are sent from and delivered to."@en ;
	sh:targetClass observable:EmailAddressFacet .

observable:EmailMessage a owl:Class , sh:NodeShape ;
	rdfs:subClassOf observable:Message ;
	rdfs:label "EmailMessage"@en ;
	rdfs:comment "An email message is a message that is an instance of an electronic mail correspondence conformant to the internet message format described in RFC 5322 and related RFCs."@en ;
	sh:targetClass observable:EmailMessage .

observable:EmailMessageFacet a owl:Class , sh:NodeShape ;
	rdfs:subClassOf core:Facet ;
	rdfs:label "EmailMessageFacet"@en ;
	rdfs:comment "An email message facet is a grouping of characteristics unique to a message that is an instance of an electronic mail correspondence conformant to the internet message format described in RFC 5322 and related RFCs."@en .

_:node1gm7uj6vjx1389 sh:class observable:MimePartType ;
	sh:nodeKind sh:IRI ;
	sh:path observable:bodyMultipart .

observable:EmailMessageFacet sh:property _:node1gm7uj6vjx1389 .

_:node1gm7uj6vjx1390 sh:class observable:ObservableObject ;
	sh:maxCount 1 ;
	sh:nodeKind sh:IRI ;
	sh:path observable:application .

observable:EmailMessageFacet sh:property _:node1gm7uj6vjx1390 .

_:node1gm7uj6vjx1391 sh:class observable:ObservableObject ;
	sh:maxCount 1 ;
	sh:nodeKind sh:IRI ;
	sh:path observable:bodyRaw .

observable:EmailMessageFacet sh:property _:node1gm7uj6vjx1391 .

_:node1gm7uj6vjx1392 sh:class observable:ObservableObject ;
	sh:maxCount 1 ;
	sh:nodeKind sh:IRI ;
	sh:path observable:from .

observable:EmailMessageFacet sh:property _:node1gm7uj6vjx1392 .

_:node1gm7uj6vjx1393 sh:class observable:ObservableObject ;
	sh:maxCount 1 ;
	sh:nodeKind sh:IRI ;
	sh:path observable:headerRaw .

observable:EmailMessageFacet sh:property _:node1gm7uj6vjx1393 .

_:node1gm7uj6vjx1394 sh:class observable:ObservableObject ;
	sh:maxCount 1 ;
	sh:nodeKind sh:IRI ;
	sh:path observable:sender .

observable:EmailMessageFacet sh:property _:node1gm7uj6vjx1394 .

_:node1gm7uj6vjx1395 sh:class observable:ObservableObject ;
	sh:maxCount 1 ;
	sh:nodeKind sh:IRI ;
	sh:path observable:xOriginatingIP .

observable:EmailMessageFacet sh:property _:node1gm7uj6vjx1395 .

_:node1gm7uj6vjx1396 sh:class observable:ObservableObject ;
	sh:nodeKind sh:IRI ;
	sh:path observable:bcc .

observable:EmailMessageFacet sh:property _:node1gm7uj6vjx1396 .

_:node1gm7uj6vjx1397 sh:class observable:ObservableObject ;
	sh:nodeKind sh:IRI ;
	sh:path observable:cc .

observable:EmailMessageFacet sh:property _:node1gm7uj6vjx1397 .

_:node1gm7uj6vjx1398 sh:class observable:ObservableObject ;
	sh:nodeKind sh:IRI ;
	sh:path observable:references .

observable:EmailMessageFacet sh:property _:node1gm7uj6vjx1398 .

_:node1gm7uj6vjx1399 sh:class observable:ObservableObject ;
	sh:nodeKind sh:IRI ;
	sh:path observable:to .

observable:EmailMessageFacet sh:property _:node1gm7uj6vjx1399 .

_:node1gm7uj6vjx1400 sh:class types:Dictionary ;
	sh:maxCount 1 ;
	sh:nodeKind sh:IRI ;
	sh:path observable:otherHeaders .

observable:EmailMessageFacet sh:property _:node1gm7uj6vjx1400 .

_:node1gm7uj6vjx1401 sh:datatype xsd:boolean ;
	sh:maxCount 1 ;
	sh:nodeKind sh:Literal ;
	sh:path observable:isMimeEncoded .

observable:EmailMessageFacet sh:property _:node1gm7uj6vjx1401 .

_:node1gm7uj6vjx1402 sh:datatype xsd:boolean ;
	sh:maxCount 1 ;
	sh:nodeKind sh:Literal ;
	sh:path observable:isMultipart .

observable:EmailMessageFacet sh:property _:node1gm7uj6vjx1402 .

_:node1gm7uj6vjx1403 sh:datatype xsd:boolean ;
	sh:maxCount 1 ;
	sh:nodeKind sh:Literal ;
	sh:path observable:isRead .

observable:EmailMessageFacet sh:property _:node1gm7uj6vjx1403 .

_:node1gm7uj6vjx1404 sh:datatype xsd:dateTime ;
	sh:maxCount 1 ;
	sh:nodeKind sh:Literal ;
	sh:path observable:modifiedTime .

observable:EmailMessageFacet sh:property _:node1gm7uj6vjx1404 .

_:node1gm7uj6vjx1405 sh:datatype xsd:dateTime ;
	sh:maxCount 1 ;
	sh:nodeKind sh:Literal ;
	sh:path observable:receivedTime .

observable:EmailMessageFacet sh:property _:node1gm7uj6vjx1405 .

_:node1gm7uj6vjx1406 sh:datatype xsd:dateTime ;
	sh:maxCount 1 ;
	sh:nodeKind sh:Literal ;
	sh:path observable:sentTime .

observable:EmailMessageFacet sh:property _:node1gm7uj6vjx1406 .

_:node1gm7uj6vjx1407 sh:datatype xsd:string ;
	sh:maxCount 1 ;
	sh:nodeKind sh:Literal ;
	sh:path observable:body .

observable:EmailMessageFacet sh:property _:node1gm7uj6vjx1407 .

_:node1gm7uj6vjx1408 sh:datatype xsd:string ;
	sh:maxCount 1 ;
	sh:nodeKind sh:Literal ;
	sh:path observable:contentDisposition .

observable:EmailMessageFacet sh:property _:node1gm7uj6vjx1408 .

_:node1gm7uj6vjx1409 sh:datatype xsd:string ;
	sh:maxCount 1 ;
	sh:nodeKind sh:Literal ;
	sh:path observable:contentType .

observable:EmailMessageFacet sh:property _:node1gm7uj6vjx1409 .

_:node1gm7uj6vjx1410 sh:datatype xsd:string ;
	sh:maxCount 1 ;
	sh:nodeKind sh:Literal ;
	sh:path observable:inReplyTo .

observable:EmailMessageFacet sh:property _:node1gm7uj6vjx1410 .

_:node1gm7uj6vjx1411 sh:datatype xsd:string ;
	sh:maxCount 1 ;
	sh:nodeKind sh:Literal ;
	sh:path observable:messageID .

observable:EmailMessageFacet sh:property _:node1gm7uj6vjx1411 .

_:node1gm7uj6vjx1412 sh:datatype xsd:string ;
	sh:maxCount 1 ;
	sh:nodeKind sh:Literal ;
	sh:path observable:priority .

observable:EmailMessageFacet sh:property _:node1gm7uj6vjx1412 .

_:node1gm7uj6vjx1413 sh:datatype xsd:string ;
	sh:maxCount 1 ;
	sh:nodeKind sh:Literal ;
	sh:path observable:subject .

observable:EmailMessageFacet sh:property _:node1gm7uj6vjx1413 .

_:node1gm7uj6vjx1414 sh:datatype xsd:string ;
	sh:maxCount 1 ;
	sh:nodeKind sh:Literal ;
	sh:path observable:xMailer .

observable:EmailMessageFacet sh:property _:node1gm7uj6vjx1414 .

_:node1gm7uj6vjx1415 sh:datatype xsd:string ;
	sh:nodeKind sh:Literal ;
	sh:path observable:categories .

observable:EmailMessageFacet sh:property _:node1gm7uj6vjx1415 .

_:node1gm7uj6vjx1416 sh:datatype xsd:string ;
	sh:nodeKind sh:Literal ;
	sh:path observable:labels .

observable:EmailMessageFacet sh:property _:node1gm7uj6vjx1416 .

_:node1gm7uj6vjx1417 sh:datatype xsd:string ;
	sh:nodeKind sh:Literal ;
	sh:path observable:receivedLines .

observable:EmailMessageFacet sh:property _:node1gm7uj6vjx1417 ;
	sh:targetClass observable:EmailMessageFacet .

observable:EmbeddedDevice a owl:Class , sh:NodeShape ;
	rdfs:subClassOf observable:Device ;
	rdfs:label "EmbeddedDevice"@en-us ;
	rdfs:comment "An embedded device is a highly specialized microprocessor device meant for one or very few specific purposes and is usually embedded or included within another object or as part of a larger system. Examples include answer machine, door access logger, card scanner, etc."@en-us ;
	sh:targetClass observable:EmbeddedDevice .

observable:EncodedStreamFacet a owl:Class , sh:NodeShape ;
	rdfs:subClassOf core:Facet ;
	rdfs:label "EncodedStreamFacet"@en ;
	rdfs:comment "An encoded stream facet is a grouping of characteristics unique to the conversion of a body of data content from one form to another form."@en .

_:node1gm7uj6vjx1418 sh:datatype xsd:string ;
	sh:maxCount 1 ;
	sh:nodeKind sh:Literal ;
	sh:path observable:encodingMethod .

observable:EncodedStreamFacet sh:property _:node1gm7uj6vjx1418 ;
	sh:targetClass observable:EncodedStreamFacet .

observable:EncryptedStreamFacet a owl:Class , sh:NodeShape ;
	rdfs:subClassOf core:Facet ;
	rdfs:label "EncryptedStreamFacet"@en ;
	rdfs:comment "An encrypted stream facet is a grouping of characteristics unique to the conversion of a body of data content from one form to another obfuscated form in such a way that reversing the conversion to obtain the original data form can only be accomplished through possession and use of a specific key."@en .

_:node1gm7uj6vjx1419 sh:datatype xsd:string ;
	sh:maxCount 1 ;
	sh:nodeKind sh:Literal ;
	sh:path observable:encryptionMethod .

observable:EncryptedStreamFacet sh:property _:node1gm7uj6vjx1419 .

_:node1gm7uj6vjx1420 sh:datatype xsd:string ;
	sh:maxCount 1 ;
	sh:nodeKind sh:Literal ;
	sh:path observable:encryptionMode .

observable:EncryptedStreamFacet sh:property _:node1gm7uj6vjx1420 .

_:node1gm7uj6vjx1421 sh:datatype xsd:string ;
	sh:nodeKind sh:Literal ;
	sh:path observable:encryptionIV .

observable:EncryptedStreamFacet sh:property _:node1gm7uj6vjx1421 .

_:node1gm7uj6vjx1422 sh:datatype xsd:string ;
	sh:nodeKind sh:Literal ;
	sh:path observable:encryptionKey .

observable:EncryptedStreamFacet sh:property _:node1gm7uj6vjx1422 ;
	sh:targetClass observable:EncryptedStreamFacet .

observable:EnvironmentVariable a owl:Class , sh:NodeShape ;
	rdfs:subClassOf core:UcoInherentCharacterizationThing ;
	rdfs:label "EnvironmentVariable"@en ;
	rdfs:comment "An environment variable is a grouping of characteristics unique to a dynamic-named value that can affect the way running processes will behave on a computer. [based on https://en.wikipedia.org/wiki/Environment_variable]"@en .

_:node1gm7uj6vjx1423 sh:datatype xsd:string ;
	sh:maxCount 1 ;
	sh:nodeKind sh:Literal ;
	sh:path core:name .

observable:EnvironmentVariable sh:property _:node1gm7uj6vjx1423 .

_:node1gm7uj6vjx1424 sh:datatype xsd:string ;
	sh:maxCount 1 ;
	sh:nodeKind sh:Literal ;
	sh:path observable:value .

observable:EnvironmentVariable sh:property _:node1gm7uj6vjx1424 ;
	sh:targetClass observable:EnvironmentVariable .

observable:EventLog a owl:Class , sh:NodeShape ;
	rdfs:subClassOf observable:ObservableObject ;
	rdfs:label "EventLog"@en ;
	rdfs:comment "An event log is a collection of event records."@en ;
	sh:targetClass observable:EventLog .

observable:EventRecord a owl:Class , sh:NodeShape ;
	rdfs:subClassOf observable:ObservableObject ;
	rdfs:label "EventRecord"@en ;
	rdfs:comment "An event record is something that happens in a digital context (e.g., operating system events)."@en ;
	sh:targetClass observable:EventRecord .

observable:EventRecordFacet a owl:Class , sh:NodeShape ;
	rdfs:subClassOf core:Facet ;
	rdfs:label "EventRecordFacet"@en ;
	rdfs:comment "An event record facet is a grouping of characteristics unique to something that happens in a digital context (e.g., operating system events)."@en .

_:node1gm7uj6vjx1425 sh:class observable:ObservableAction ;
	sh:maxCount 1 ;
	sh:nodeKind sh:IRI ;
	sh:path observable:cyberAction .

observable:EventRecordFacet sh:property _:node1gm7uj6vjx1425 .

_:node1gm7uj6vjx1426 sh:class observable:ObservableObject ;
	sh:maxCount 1 ;
	sh:nodeKind sh:IRI ;
	sh:path observable:account .

observable:EventRecordFacet sh:property _:node1gm7uj6vjx1426 .

_:node1gm7uj6vjx1427 sh:class observable:ObservableObject ;
	sh:maxCount 1 ;
	sh:nodeKind sh:IRI ;
	sh:path observable:application .

observable:EventRecordFacet sh:property _:node1gm7uj6vjx1427 .

_:node1gm7uj6vjx1428 sh:class observable:ObservableObject ;
	sh:maxCount 1 ;
	sh:nodeKind sh:IRI ;
	sh:path observable:eventRecordDevice .

observable:EventRecordFacet sh:property _:node1gm7uj6vjx1428 .

_:node1gm7uj6vjx1429 sh:datatype xsd:dateTime ;
	sh:maxCount 1 ;
	sh:nodeKind sh:Literal ;
	sh:path observable:endTime .

observable:EventRecordFacet sh:property _:node1gm7uj6vjx1429 .

_:node1gm7uj6vjx1430 sh:datatype xsd:dateTime ;
	sh:maxCount 1 ;
	sh:nodeKind sh:Literal ;
	sh:path observable:observableCreatedTime .

observable:EventRecordFacet sh:property _:node1gm7uj6vjx1430 .

_:node1gm7uj6vjx1431 sh:datatype xsd:dateTime ;
	sh:maxCount 1 ;
	sh:nodeKind sh:Literal ;
	sh:path observable:startTime .

observable:EventRecordFacet sh:property _:node1gm7uj6vjx1431 .

_:node1gm7uj6vjx1432 sh:datatype xsd:string ;
	sh:maxCount 1 ;
	sh:nodeKind sh:Literal ;
	sh:path observable:eventID .

observable:EventRecordFacet sh:property _:node1gm7uj6vjx1432 .

_:node1gm7uj6vjx1433 sh:datatype xsd:string ;
	sh:maxCount 1 ;
	sh:nodeKind sh:Literal ;
	sh:path observable:eventRecordID .

observable:EventRecordFacet sh:property _:node1gm7uj6vjx1433 .

_:node1gm7uj6vjx1434 sh:datatype xsd:string ;
	sh:maxCount 1 ;
	sh:nodeKind sh:Literal ;
	sh:path observable:eventRecordRaw .

observable:EventRecordFacet sh:property _:node1gm7uj6vjx1434 .

_:node1gm7uj6vjx1435 sh:datatype xsd:string ;
	sh:maxCount 1 ;
	sh:nodeKind sh:Literal ;
	sh:path observable:eventRecordServiceName .

observable:EventRecordFacet sh:property _:node1gm7uj6vjx1435 .

_:node1gm7uj6vjx1436 sh:datatype xsd:string ;
	sh:maxCount 1 ;
	sh:nodeKind sh:Literal ;
	sh:path observable:eventRecordText .

observable:EventRecordFacet sh:property _:node1gm7uj6vjx1436 .

_:node1gm7uj6vjx1437 sh:datatype xsd:string ;
	sh:maxCount 1 ;
	sh:nodeKind sh:Literal ;
	sh:path observable:eventType .

observable:EventRecordFacet sh:property _:node1gm7uj6vjx1437 ;
	sh:targetClass observable:EventRecordFacet .

observable:ExtInodeFacet a owl:Class , sh:NodeShape ;
	rdfs:subClassOf core:Facet ;
	rdfs:label "ExtInodeFacet"@en ;
	rdfs:comment "An extInode facet is a grouping of characteristics unique to a file system object (file, directory, etc.) conformant to the extended file system (EXT or related derivations) specification."@en .

_:node1gm7uj6vjx1438 sh:datatype xsd:dateTime ;
	sh:maxCount 1 ;
	sh:nodeKind sh:Literal ;
	sh:path observable:extDeletionTime .

observable:ExtInodeFacet sh:property _:node1gm7uj6vjx1438 .

_:node1gm7uj6vjx1439 sh:datatype xsd:dateTime ;
	sh:maxCount 1 ;
	sh:nodeKind sh:Literal ;
	sh:path observable:extInodeChangeTime .

observable:ExtInodeFacet sh:property _:node1gm7uj6vjx1439 .

_:node1gm7uj6vjx1440 sh:datatype xsd:integer ;
	sh:maxCount 1 ;
	sh:nodeKind sh:Literal ;
	sh:path observable:extFileType .

observable:ExtInodeFacet sh:property _:node1gm7uj6vjx1440 .

_:node1gm7uj6vjx1441 sh:datatype xsd:integer ;
	sh:maxCount 1 ;
	sh:nodeKind sh:Literal ;
	sh:path observable:extFlags .

observable:ExtInodeFacet sh:property _:node1gm7uj6vjx1441 .

_:node1gm7uj6vjx1442 sh:datatype xsd:integer ;
	sh:maxCount 1 ;
	sh:nodeKind sh:Literal ;
	sh:path observable:extHardLinkCount .

observable:ExtInodeFacet sh:property _:node1gm7uj6vjx1442 .

_:node1gm7uj6vjx1443 sh:datatype xsd:integer ;
	sh:maxCount 1 ;
	sh:nodeKind sh:Literal ;
	sh:path observable:extInodeID .

observable:ExtInodeFacet sh:property _:node1gm7uj6vjx1443 .

_:node1gm7uj6vjx1444 sh:datatype xsd:integer ;
	sh:maxCount 1 ;
	sh:nodeKind sh:Literal ;
	sh:path observable:extPermissions .

observable:ExtInodeFacet sh:property _:node1gm7uj6vjx1444 .

_:node1gm7uj6vjx1445 sh:datatype xsd:integer ;
	sh:maxCount 1 ;
	sh:nodeKind sh:Literal ;
	sh:path observable:extSGID .

observable:ExtInodeFacet sh:property _:node1gm7uj6vjx1445 .

_:node1gm7uj6vjx1446 sh:datatype xsd:integer ;
	sh:maxCount 1 ;
	sh:nodeKind sh:Literal ;
	sh:path observable:extSUID .

observable:ExtInodeFacet sh:property _:node1gm7uj6vjx1446 ;
	sh:targetClass observable:ExtInodeFacet .

observable:ExtractedString a owl:Class , sh:NodeShape ;
	rdfs:subClassOf core:UcoInherentCharacterizationThing ;
	rdfs:label "ExtractedString"@en ;
	rdfs:comment "An extracted string is a grouping of characteristics unique to a series of characters pulled from an observable object."@en .

_:node1gm7uj6vjx1447 sh:datatype xsd:base64Binary ;
	sh:maxCount 1 ;
	sh:nodeKind sh:Literal ;
	sh:path observable:byteStringValue .

observable:ExtractedString sh:property _:node1gm7uj6vjx1447 .

_:node1gm7uj6vjx1448 sh:datatype xsd:integer ;
	sh:maxCount 1 ;
	sh:nodeKind sh:Literal ;
	sh:path observable:length .

observable:ExtractedString sh:property _:node1gm7uj6vjx1448 .

_:node1gm7uj6vjx1449 sh:datatype xsd:string ;
	sh:maxCount 1 ;
	sh:nodeKind sh:Literal ;
	sh:path observable:encoding .

observable:ExtractedString sh:property _:node1gm7uj6vjx1449 .

_:node1gm7uj6vjx1450 sh:datatype xsd:string ;
	sh:maxCount 1 ;
	sh:nodeKind sh:Literal ;
	sh:path observable:englishTranslation .

observable:ExtractedString sh:property _:node1gm7uj6vjx1450 .

_:node1gm7uj6vjx1451 sh:datatype xsd:string ;
	sh:maxCount 1 ;
	sh:nodeKind sh:Literal ;
	sh:path observable:language .

observable:ExtractedString sh:property _:node1gm7uj6vjx1451 .

_:node1gm7uj6vjx1452 sh:datatype xsd:string ;
	sh:maxCount 1 ;
	sh:nodeKind sh:Literal ;
	sh:path observable:stringValue .

observable:ExtractedString sh:property _:node1gm7uj6vjx1452 ;
	sh:targetClass observable:ExtractedString .

observable:ExtractedStringsFacet a owl:Class , sh:NodeShape ;
	rdfs:subClassOf core:Facet ;
	rdfs:label "ExtractedStringsFacet"@en ;
	rdfs:comment "An extracted strings facet is a grouping of characteristics unique to one or more sequences of characters pulled from an observable object."@en .

_:node1gm7uj6vjx1453 sh:class observable:ExtractedString ;
	sh:nodeKind sh:IRI ;
	sh:path observable:strings .

observable:ExtractedStringsFacet sh:property _:node1gm7uj6vjx1453 ;
	sh:targetClass observable:ExtractedStringsFacet .

observable:File a owl:Class , sh:NodeShape ;
	rdfs:subClassOf observable:FileSystemObject ;
	rdfs:label "File"@en ;
	rdfs:comment "A file is a computer resource for recording data discretely on a computer storage device."@en ;
	sh:targetClass observable:File .

observable:FileFacet a owl:Class , sh:NodeShape ;
	rdfs:subClassOf core:Facet ;
	rdfs:label "FileFacet"@en ;
	rdfs:comment "A file facet is a grouping of characteristics unique to the storage of a file (computer resource for recording data discretely in a computer storage device) on a file system (process that manages how and where data on a storage device is stored, accessed and managed). [based on https://en.wikipedia.org/Computer_file and https://www.techopedia.com/definition/5510/file-system]"@en .

_:node1gm7uj6vjx1454 sh:datatype xsd:boolean ;
	sh:nodeKind sh:Literal ;
	sh:path observable:isDirectory .

observable:FileFacet sh:property _:node1gm7uj6vjx1454 .

_:node1gm7uj6vjx1455 sh:datatype xsd:dateTime ;
	sh:maxCount 1 ;
	sh:nodeKind sh:Literal ;
	sh:path observable:accessedTime .

observable:FileFacet sh:property _:node1gm7uj6vjx1455 .

_:node1gm7uj6vjx1456 sh:datatype xsd:dateTime ;
	sh:maxCount 1 ;
	sh:nodeKind sh:Literal ;
	sh:path observable:metadataChangeTime .

observable:FileFacet sh:property _:node1gm7uj6vjx1456 .

_:node1gm7uj6vjx1457 sh:datatype xsd:dateTime ;
	sh:maxCount 1 ;
	sh:nodeKind sh:Literal ;
	sh:path observable:modifiedTime .

observable:FileFacet sh:property _:node1gm7uj6vjx1457 .

_:node1gm7uj6vjx1458 sh:datatype xsd:dateTime ;
	sh:maxCount 1 ;
	sh:nodeKind sh:Literal ;
	sh:path observable:observableCreatedTime .

observable:FileFacet sh:property _:node1gm7uj6vjx1458 .

_:node1gm7uj6vjx1459 sh:datatype xsd:integer ;
	sh:description "When used to characterize a file the sizeInBytes property conveys the recorded size of a file in a file system."@en ;
	sh:maxCount 1 ;
	sh:nodeKind sh:Literal ;
	sh:path observable:sizeInBytes .

observable:FileFacet sh:property _:node1gm7uj6vjx1459 .

_:node1gm7uj6vjx1460 sh:datatype xsd:string ;
	sh:maxCount 1 ;
	sh:nodeKind sh:Literal ;
	sh:path observable:allocationStatus .

observable:FileFacet sh:property _:node1gm7uj6vjx1460 .

_:node1gm7uj6vjx1461 sh:datatype xsd:string ;
	sh:maxCount 1 ;
	sh:nodeKind sh:Literal ;
	sh:path observable:extension .

observable:FileFacet sh:property _:node1gm7uj6vjx1461 .

_:node1gm7uj6vjx1462 sh:datatype xsd:string ;
	sh:nodeKind sh:Literal ;
	sh:path observable:fileName .

observable:FileFacet sh:property _:node1gm7uj6vjx1462 .

_:node1gm7uj6vjx1463 sh:datatype xsd:string ;
	sh:nodeKind sh:Literal ;
	sh:path observable:filePath .

observable:FileFacet sh:property _:node1gm7uj6vjx1463 ;
	sh:targetClass observable:FileFacet .

observable:FilePermissionsFacet a owl:Class , sh:NodeShape ;
	rdfs:subClassOf core:Facet ;
	rdfs:label "FilePermissionsFacet"@en ;
	rdfs:comment "A file permissions facet is a grouping of characteristics unique to the access rights (e.g., view, change, navigate, execute) of a file on a file system."@en .

_:node1gm7uj6vjx1464 sh:class core:UcoObject ;
	sh:maxCount 1 ;
	sh:nodeKind sh:IRI ;
	sh:path observable:owner .

observable:FilePermissionsFacet sh:property _:node1gm7uj6vjx1464 ;
	sh:targetClass observable:FilePermissionsFacet .

observable:FileSystem a owl:Class , sh:NodeShape ;
	rdfs:subClassOf observable:ObservableObject ;
	rdfs:label "FileSystem"@en ;
	rdfs:comment "A file system is the process that manages how and where data on a storage medium is stored, accessed and managed. [based on https://www.techopedia.com/definition/5510/file-system]"@en ;
	sh:targetClass observable:FileSystem .

observable:FileSystemFacet a owl:Class , sh:NodeShape ;
	rdfs:subClassOf core:Facet ;
	rdfs:label "FileSystemFacet"@en ;
	rdfs:comment "A file system facet is a grouping of characteristics unique to the process that manages how and where data on a storage medium is stored, accessed and managed. [based on https://www.techopedia.com/definition/5510/file-system]"@en .

_:node1gm7uj6vjx1465 sh:datatype xsd:integer ;
	sh:maxCount 1 ;
	sh:nodeKind sh:Literal ;
	sh:path observable:clusterSize .

observable:FileSystemFacet sh:property _:node1gm7uj6vjx1465 .

_:node1gm7uj6vjx1466 sh:datatype xsd:string ;
	sh:maxCount 1 ;
	sh:nodeKind sh:Literal ;
	sh:path observable:fileSystemType .

observable:FileSystemFacet sh:property _:node1gm7uj6vjx1466 ;
	sh:targetClass observable:FileSystemFacet .

observable:FileSystemObject a owl:Class , sh:NodeShape ;
	rdfs:subClassOf observable:ObservableObject ;
	rdfs:label "FileSystemObject"@en ;
	rdfs:comment "A file system object is an informational object represented and managed within a file system."@en ;
	sh:targetClass observable:FileSystemObject .

observable:ForumPost a owl:Class , sh:NodeShape ;
	rdfs:subClassOf observable:Message ;
	rdfs:label "ForumPost"@en ;
	rdfs:comment "A forum post is message submitted by a user account to an online forum where the message content (and typically metadata including who posted it and when) is viewable by any party with viewing permissions on the forum."@en ;
	sh:targetClass observable:ForumPost .

observable:ForumPrivateMessage a owl:Class , sh:NodeShape ;
	rdfs:subClassOf observable:Message ;
	rdfs:label "ForumPrivateMessage"@en ;
	rdfs:comment "A forum private message (aka PM or DM (direct message)) is a one-to-one message from one specific user account to another specific user account on an online form where transmission is managed by the online forum platform and the message is only viewable by the parties directly involved."@en ;
	sh:targetClass observable:ForumPrivateMessage .

observable:FragmentFacet a owl:Class , sh:NodeShape ;
	rdfs:subClassOf core:Facet ;
	rdfs:label "FragmentFacet"@en ;
	rdfs:comment "A fragment facet is a grouping of characteristics unique to an individual piece of the content of a file."@en .

_:node1gm7uj6vjx1467 sh:datatype xsd:integer ;
	sh:nodeKind sh:Literal ;
	sh:path observable:fragmentIndex .

observable:FragmentFacet sh:property _:node1gm7uj6vjx1467 .

_:node1gm7uj6vjx1468 sh:datatype xsd:integer ;
	sh:nodeKind sh:Literal ;
	sh:path observable:totalFragments .

observable:FragmentFacet sh:property _:node1gm7uj6vjx1468 ;
	sh:targetClass observable:FragmentFacet .

observable:GUI a owl:Class , sh:NodeShape ;
	rdfs:subClassOf observable:ObservableObject ;
	rdfs:label "GUI"@en ;
	rdfs:comment "A GUI is a graphical user interface that allows users to interact with electronic devices through graphical icons and audio indicators such as primary notation, instead of text-based user interfaces, typed command labels or text navigation. [based on https://en.wikipedia.org/wiki/Graphical_user_interface]"@en ;
	sh:targetClass observable:GUI .

observable:GamingConsole a owl:Class , sh:NodeShape ;
	rdfs:subClassOf observable:Device ;
	rdfs:label "GamingConsole"@en-us ;
	rdfs:comment "A gaming console (video game console or game console) is an electronic system that connects to a display, typically a TV or computer monitor, for the primary purpose of playing video games."@en-us ;
	sh:targetClass observable:GamingConsole .

observable:GenericObservableObject a owl:Class , sh:NodeShape ;
	rdfs:subClassOf observable:ObservableObject ;
	rdfs:label "GenericObservableObject"@en ;
	rdfs:comment "A generic observable object is an article or unit within the digital domain."@en ;
	sh:targetClass observable:GenericObservableObject .

observable:GeoLocationEntry a owl:Class , sh:NodeShape ;
	rdfs:subClassOf observable:ObservableObject ;
	rdfs:label "GeoLocationEntry"@en ;
	rdfs:comment "A geolocation entry is a single application-specific geolocation entry."@en ;
	sh:targetClass observable:GeoLocationEntry .

observable:GeoLocationEntryFacet a owl:Class , sh:NodeShape ;
	rdfs:subClassOf core:Facet ;
	rdfs:label "GeoLocationEntryFacet"@en ;
	rdfs:comment "A geolocation entry facet is a grouping of characteristics unique to a single application-specific geolocation entry."@en .

_:node1gm7uj6vjx1469 sh:class location:Location ;
	sh:maxCount 1 ;
	sh:nodeKind sh:IRI ;
	sh:path observable:location .

observable:GeoLocationEntryFacet sh:property _:node1gm7uj6vjx1469 .

_:node1gm7uj6vjx1470 sh:class observable:ObservableObject ;
	sh:maxCount 1 ;
	sh:nodeKind sh:IRI ;
	sh:path observable:application .

observable:GeoLocationEntryFacet sh:property _:node1gm7uj6vjx1470 .

_:node1gm7uj6vjx1471 sh:datatype xsd:dateTime ;
	sh:maxCount 1 ;
	sh:nodeKind sh:Literal ;
	sh:path observable:observableCreatedTime .

observable:GeoLocationEntryFacet sh:property _:node1gm7uj6vjx1471 ;
	sh:targetClass observable:GeoLocationEntryFacet .

observable:GeoLocationLog a owl:Class , sh:NodeShape ;
	rdfs:subClassOf observable:ObservableObject ;
	rdfs:label "GeoLocationLog"@en ;
	rdfs:comment "A geolocation log is a record containing geolocation tracks and/or geolocation entries."@en ;
	sh:targetClass observable:GeoLocationLog .

observable:GeoLocationLogFacet a owl:Class , sh:NodeShape ;
	rdfs:subClassOf core:Facet ;
	rdfs:label "GeoLocationLogFacet"@en ;
	rdfs:comment "A geolocation log facet is a grouping of characteristics unique to a record containing geolocation tracks and/or geolocation entries."@en .

_:node1gm7uj6vjx1472 sh:class observable:ObservableObject ;
	sh:maxCount 1 ;
	sh:nodeKind sh:IRI ;
	sh:path observable:application .

observable:GeoLocationLogFacet sh:property _:node1gm7uj6vjx1472 .

_:node1gm7uj6vjx1473 sh:datatype xsd:dateTime ;
	sh:maxCount 1 ;
	sh:nodeKind sh:Literal ;
	sh:path observable:observableCreatedTime .

observable:GeoLocationLogFacet sh:property _:node1gm7uj6vjx1473 ;
	sh:targetClass observable:GeoLocationLogFacet .

observable:GeoLocationTrack a owl:Class , sh:NodeShape ;
	rdfs:subClassOf observable:ObservableObject ;
	rdfs:label "GeoLocationTrack"@en ;
	rdfs:comment "A geolocation track is a set of contiguous geolocation entries representing a path/track taken."@en ;
	sh:targetClass observable:GeoLocationTrack .

observable:GeoLocationTrackFacet a owl:Class , sh:NodeShape ;
	rdfs:subClassOf core:Facet ;
	rdfs:label "GeoLocationTrackFacet"@en ;
	rdfs:comment "A geolocation track facet is a grouping of characteristics unique to a set of contiguous geolocation entries representing a path/track taken."@en .

_:node1gm7uj6vjx1474 sh:class observable:ObservableObject ;
	sh:maxCount 1 ;
	sh:nodeKind sh:IRI ;
	sh:path observable:application .

observable:GeoLocationTrackFacet sh:property _:node1gm7uj6vjx1474 .

_:node1gm7uj6vjx1475 sh:class observable:ObservableObject ;
	sh:nodeKind sh:IRI ;
	sh:path observable:geoLocationEntry .

observable:GeoLocationTrackFacet sh:property _:node1gm7uj6vjx1475 .

_:node1gm7uj6vjx1476 sh:datatype xsd:dateTime ;
	sh:maxCount 1 ;
	sh:nodeKind sh:Literal ;
	sh:path observable:endTime .

observable:GeoLocationTrackFacet sh:property _:node1gm7uj6vjx1476 .

_:node1gm7uj6vjx1477 sh:datatype xsd:dateTime ;
	sh:maxCount 1 ;
	sh:nodeKind sh:Literal ;
	sh:path observable:startTime .

observable:GeoLocationTrackFacet sh:property _:node1gm7uj6vjx1477 ;
	sh:targetClass observable:GeoLocationTrackFacet .

observable:GlobalFlagType a owl:Class , sh:NodeShape ;
	rdfs:subClassOf core:UcoInherentCharacterizationThing ;
	rdfs:label "GlobalFlagType"@en ;
	rdfs:comment "A global flag type is a grouping of characteristics unique to the Windows systemwide global variable named NtGlobalFlag that enables various internal debugging, tracing, and validation support in the operating system. [based on \"Windows Global Flags, Chapter 3: System Mechanisms of Windows Internals by Solomon, Russinovich, and Ionescu]"@en .

_:node1gm7uj6vjx1478 sh:datatype xsd:hexBinary ;
	sh:nodeKind sh:Literal ;
	sh:path observable:hexadecimalValue .

observable:GlobalFlagType sh:property _:node1gm7uj6vjx1478 .

_:node1gm7uj6vjx1479 sh:datatype xsd:string ;
	sh:maxCount 1 ;
	sh:nodeKind sh:Literal ;
	sh:path observable:abbreviation .

observable:GlobalFlagType sh:property _:node1gm7uj6vjx1479 .

_:node1gm7uj6vjx1480 sh:datatype xsd:string ;
	sh:maxCount 1 ;
	sh:nodeKind sh:Literal ;
	sh:path observable:destination .

observable:GlobalFlagType sh:property _:node1gm7uj6vjx1480 .

_:node1gm7uj6vjx1481 sh:datatype xsd:string ;
	sh:maxCount 1 ;
	sh:nodeKind sh:Literal ;
	sh:path observable:symbolicName .

observable:GlobalFlagType sh:property _:node1gm7uj6vjx1481 ;
	sh:targetClass observable:GlobalFlagType .

observable:HTTPConnection a owl:Class , sh:NodeShape ;
	rdfs:subClassOf observable:NetworkConnection ;
	rdfs:label "HTTPConnection"@en ;
	rdfs:comment "An HTTP connection is network connection that is conformant to the Hypertext Transfer Protocol (HTTP) standard."@en ;
	sh:targetClass observable:HTTPConnection .

observable:HTTPConnectionFacet a owl:Class , sh:NodeShape ;
	rdfs:subClassOf core:Facet ;
	rdfs:label "HTTPConnectionFacet"@en ;
	rdfs:comment "An HTTP connection facet is a grouping of characteristics unique to portions of a network connection that are conformant to the Hypertext Transfer Protocol (HTTP) standard."@en .

_:node1gm7uj6vjx1482 sh:class observable:ObservableObject ;
	sh:maxCount 1 ;
	sh:nodeKind sh:IRI ;
	sh:path observable:httpMessageBodyData .

observable:HTTPConnectionFacet sh:property _:node1gm7uj6vjx1482 .

_:node1gm7uj6vjx1483 sh:class types:Dictionary ;
	sh:maxCount 1 ;
	sh:nodeKind sh:IRI ;
	sh:path observable:httpRequestHeader .

observable:HTTPConnectionFacet sh:property _:node1gm7uj6vjx1483 .

_:node1gm7uj6vjx1484 sh:datatype xsd:integer ;
	sh:maxCount 1 ;
	sh:nodeKind sh:Literal ;
	sh:path observable:httpMesageBodyLength .

observable:HTTPConnectionFacet sh:property _:node1gm7uj6vjx1484 .

_:node1gm7uj6vjx1485 sh:datatype xsd:string ;
	sh:maxCount 1 ;
	sh:nodeKind sh:Literal ;
	sh:path observable:requestMethod .

observable:HTTPConnectionFacet sh:property _:node1gm7uj6vjx1485 .

_:node1gm7uj6vjx1486 sh:datatype xsd:string ;
	sh:maxCount 1 ;
	sh:nodeKind sh:Literal ;
	sh:path observable:requestValue .

observable:HTTPConnectionFacet sh:property _:node1gm7uj6vjx1486 .

_:node1gm7uj6vjx1487 sh:datatype xsd:string ;
	sh:maxCount 1 ;
	sh:nodeKind sh:Literal ;
	sh:path observable:requestVersion .

observable:HTTPConnectionFacet sh:property _:node1gm7uj6vjx1487 ;
	sh:targetClass observable:HTTPConnectionFacet .

observable:Hostname a owl:Class , sh:NodeShape ;
	rdfs:subClassOf observable:ObservableObject ;
	rdfs:label "Hostname"@en ;
	rdfs:comment "A hostname is a label that is assigned to a device connected to a computer network and that is used to identify the device in various forms of electronic communication, such as the World Wide Web. A hostname may be a domain name, if it is properly organized into the domain name system. A domain name may be a hostname if it has been assigned to an Internet host and associated with the host's IP address. [based on https://en.wikipedia.org/wiki/Hostname]"@en ;
	sh:targetClass observable:Hostname .

observable:ICCID a owl:DatatypeProperty ;
	rdfs:label "ICCID"@en ;
	rdfs:comment "Integrated circuit card identifier (http://www.itu.int/)."@en ;
	rdfs:range xsd:string .

observable:ICMPConnection a owl:Class , sh:NodeShape ;
	rdfs:subClassOf observable:NetworkConnection ;
	rdfs:label "ICMPConnection"@en ;
	rdfs:comment "An ICMP connection is a network connection that is conformant to the Internet Control Message Protocol (ICMP) standard."@en ;
	sh:targetClass observable:ICMPConnection .

observable:ICMPConnectionFacet a owl:Class , sh:NodeShape ;
	rdfs:subClassOf core:Facet ;
	rdfs:label "ICMPConnectionFacet"@en ;
	rdfs:comment "An ICMP connection facet is a grouping of characteristics unique to portions of a network connection that are conformant to the Internet Control Message Protocol (ICMP) standard."@en .

_:node1gm7uj6vjx1488 sh:datatype xsd:hexBinary ;
	sh:nodeKind sh:Literal ;
	sh:path observable:icmpCode .

observable:ICMPConnectionFacet sh:property _:node1gm7uj6vjx1488 .

_:node1gm7uj6vjx1489 sh:datatype xsd:hexBinary ;
	sh:nodeKind sh:Literal ;
	sh:path observable:icmpType .

observable:ICMPConnectionFacet sh:property _:node1gm7uj6vjx1489 ;
	sh:targetClass observable:ICMPConnectionFacet .

observable:IComHandlerActionType a owl:Class , sh:NodeShape ;
	rdfs:subClassOf core:UcoInherentCharacterizationThing ;
	rdfs:label "IComHandlerActionType"@en ;
	rdfs:comment "An IComHandler action type is a grouping of characteristics unique to a Windows Task-related action that fires a Windows COM handler (smart code in the client address space that can optimize calls between a client and server). [based on https://docs.microsoft.com/en-us/windows/win32/taskschd/comhandleraction]"@en .

_:node1gm7uj6vjx1490 sh:datatype xsd:string ;
	sh:maxCount 1 ;
	sh:nodeKind sh:Literal ;
	sh:path observable:comClassID .

observable:IComHandlerActionType sh:property _:node1gm7uj6vjx1490 .

_:node1gm7uj6vjx1491 sh:datatype xsd:string ;
	sh:maxCount 1 ;
	sh:nodeKind sh:Literal ;
	sh:path observable:comData .

observable:IComHandlerActionType sh:property _:node1gm7uj6vjx1491 ;
	sh:targetClass observable:IComHandlerActionType .

observable:IExecActionType a owl:Class , sh:NodeShape ;
	rdfs:subClassOf core:UcoInherentCharacterizationThing ;
	rdfs:label "IExecActionType"@en ;
	rdfs:comment "An IExec action type is a grouping of characteristics unique to an action that executes a command-line operation on a Windows operating system. [based on https://docs.microsoft.com/en-us/windows/win32/api/taskschd/nn-taskschd-iexecaction?redirectedfrom=MSDN]"@en .

_:node1gm7uj6vjx1492 sh:class types:Hash ;
	sh:nodeKind sh:IRI ;
	sh:path observable:execProgramHashes .

observable:IExecActionType sh:property _:node1gm7uj6vjx1492 .

_:node1gm7uj6vjx1493 sh:datatype xsd:string ;
	sh:maxCount 1 ;
	sh:nodeKind sh:Literal ;
	sh:path observable:execArguments .

observable:IExecActionType sh:property _:node1gm7uj6vjx1493 .

_:node1gm7uj6vjx1494 sh:datatype xsd:string ;
	sh:maxCount 1 ;
	sh:nodeKind sh:Literal ;
	sh:path observable:execProgramPath .

observable:IExecActionType sh:property _:node1gm7uj6vjx1494 .

_:node1gm7uj6vjx1495 sh:datatype xsd:string ;
	sh:maxCount 1 ;
	sh:nodeKind sh:Literal ;
	sh:path observable:execWorkingDirectory .

observable:IExecActionType sh:property _:node1gm7uj6vjx1495 ;
	sh:targetClass observable:IExecActionType .

observable:IMEI a owl:DatatypeProperty ;
	rdfs:label "IMEI"@en ;
	rdfs:comment "International Mobile Equipment Identity (IMEI)."@en ;
	rdfs:range xsd:string .

observable:IMSI a owl:DatatypeProperty ;
	rdfs:label "IMSI"@en ;
	rdfs:comment "An International Mobile Subscriber Identity (IMSI) is a unique identification associated with all GSM and UMTS network mobile phone users. It is stored as a 64-bit field in the SIM inside the phone and is sent by the phone to the network."@en ;
	rdfs:range xsd:string .

observable:IPAddress a owl:Class , sh:NodeShape ;
	rdfs:subClassOf observable:DigitalAddress ;
	rdfs:label "IPAddress"@en ;
	rdfs:comment "An IP address is an Internet Protocol (IP) standards conformant identifier assigned to a device to enable routing and management of IP standards conformant communication to or from that device."@en ;
	sh:targetClass observable:IPAddress .

observable:IPAddressFacet a owl:Class , sh:NodeShape ;
	rdfs:subClassOf observable:DigitalAddressFacet ;
	rdfs:label "IPAddressFacet"@en ;
	rdfs:comment "An IP address facet is a grouping of characteristics unique to an Internet Protocol (IP) standards conformant identifier assigned to a device to enable routing and management of IP standards conformant communication to or from that device."@en ;
	sh:targetClass observable:IPAddressFacet .

observable:IPNetmask a owl:Class , sh:NodeShape ;
	rdfs:subClassOf observable:ObservableObject ;
	rdfs:label "IPNetmask"@en ;
	rdfs:comment "An IP netmask is a 32-bit 'mask' used to divide an IP address into subnets and specify the network's available hosts."@en ;
	sh:targetClass observable:IPNetmask .

observable:IPhone a owl:Class , sh:NodeShape ;
	rdfs:subClassOf observable:AppleDevice , observable:SmartPhone ;
	rdfs:label "IPhone"@en-us ;
	rdfs:comment "An iPhone is a smart phone that applies the iOS mobile operating system."@en-us ;
	sh:targetClass observable:IPhone .

observable:IPv4Address a owl:Class , sh:NodeShape ;
	rdfs:subClassOf observable:IPAddress ;
	rdfs:label "IPv4Address"@en ;
	rdfs:comment "An IPv4 (Internet Protocol version 4) address is an IPv4 standards conformant identifier assigned to a device to enable routing and management of IPv4 standards conformant communication to or from that device."@en ;
	sh:targetClass observable:IPv4Address .

observable:IPv4AddressFacet a owl:Class , sh:NodeShape ;
	rdfs:subClassOf observable:IPAddressFacet ;
	rdfs:label "IPv4AddressFacet"@en ;
	rdfs:comment "An IPv4 (Internet Protocol version 4) address facet is a grouping of characteristics unique to an IPv4 standards conformant identifier assigned to a device to enable routing and management of IPv4 standards conformant communication to or from that device."@en ;
	sh:targetClass observable:IPv4AddressFacet .

observable:IPv6Address a owl:Class , sh:NodeShape ;
	rdfs:subClassOf observable:IPAddress ;
	rdfs:label "IPv6Address"@en ;
	rdfs:comment "An IPv6 (Internet Protocol version 6) address is an IPv6 standards conformant identifier assigned to a device to enable routing and management of IPv6 standards conformant communication to or from that device."@en ;
	sh:targetClass observable:IPv6Address .

observable:IPv6AddressFacet a owl:Class , sh:NodeShape ;
	rdfs:subClassOf observable:IPAddressFacet ;
	rdfs:label "IPv6AddressFacet"@en ;
	rdfs:comment "An IPv6 (Internet Protocol version 6) address facet is a grouping of characteristics unique to an IPv6 standards conformant identifier assigned to a device to enable routing and management of IPv6 standards conformant communication to or from that device."@en ;
	sh:targetClass observable:IPv6AddressFacet .

observable:IShowMessageActionType a owl:Class , sh:NodeShape ;
	rdfs:subClassOf core:UcoInherentCharacterizationThing ;
	rdfs:label "IShowMessageActionType"@en ;
	rdfs:comment "An IShow message action type is a grouping of characteristics unique to an action that shows a message box when a task is activate. [based on https://docs.microsoft.com/en-us/windows/win32/api/taskschd/nn-taskschd-ishowmessageaction?redirectedfrom=MSDN]"@en .

_:node1gm7uj6vjx1496 sh:datatype xsd:string ;
	sh:maxCount 1 ;
	sh:nodeKind sh:Literal ;
	sh:path observable:showMessageBody .

observable:IShowMessageActionType sh:property _:node1gm7uj6vjx1496 .

_:node1gm7uj6vjx1497 sh:datatype xsd:string ;
	sh:maxCount 1 ;
	sh:nodeKind sh:Literal ;
	sh:path observable:showMessageTitle .

observable:IShowMessageActionType sh:property _:node1gm7uj6vjx1497 ;
	sh:targetClass observable:IShowMessageActionType .

observable:Image a owl:Class , sh:NodeShape ;
	rdfs:subClassOf observable:ObservableObject ;
	rdfs:label "Image"@en ;
	rdfs:comment "An image is a complete copy of a hard disk, memory, or other digital media."@en ;
	sh:targetClass observable:Image .

observable:ImageFacet a owl:Class , sh:NodeShape ;
	rdfs:subClassOf core:Facet ;
	rdfs:label "ImageFacet"@en ;
	rdfs:comment "An image facet is a grouping of characteristics unique to a complete copy of a hard disk, memory, or other digital media."@en .

_:node1gm7uj6vjx1498 sh:datatype xsd:string ;
	sh:maxCount 1 ;
	sh:nodeKind sh:Literal ;
	sh:path observable:imageType .

observable:ImageFacet sh:property _:node1gm7uj6vjx1498 ;
	sh:targetClass observable:ImageFacet .

observable:InstantMessagingAddress a owl:Class , sh:NodeShape ;
	rdfs:subClassOf observable:DigitalAddress ;
	rdfs:label "InstantMessagingAddress"@en ;
	rdfs:comment ""@en ;
	sh:targetClass observable:InstantMessagingAddress .

observable:InstantMessagingAddressFacet a owl:Class , sh:NodeShape ;
	rdfs:subClassOf observable:DigitalAddressFacet ;
	rdfs:label "InstantMessagingAddressFacet"@en ;
	rdfs:comment "An instant messaging address facet is a grouping of characteristics unique to an identifier assigned to enable routing and management of instant messaging digital communication."@en ;
	sh:targetClass observable:InstantMessagingAddressFacet .

observable:Junction a owl:Class , sh:NodeShape ;
	rdfs:subClassOf observable:FileSystemObject ;
	rdfs:label "Junction"@en ;
	rdfs:comment "A junction is a specific NTFS (New Technology File System) reparse point to redirect a directory access to another directory which can be on the same volume or another volume. A junction is similar to a directory symbolic link but may differ on whether they are processed on the local system or on the remote file server. [based on https://jp-andre.pagesperso-orange.fr/junctions.html]"@en ;
	sh:targetClass observable:Junction .

observable:Laptop a owl:Class , sh:NodeShape ;
	rdfs:subClassOf observable:Computer ;
	rdfs:label "Laptop"@en-us ;
	rdfs:comment "A laptop, laptop computer, or notebook computer is a small, portable personal computer with a screen and alphanumeric keyboard. These typically have a clam shell form factor with the screen mounted on the inside of the upper lid and the keyboard on the inside of the lower lid, although 2-in-1 PCs with a detachable keyboard are often marketed as laptops or as having a laptop mode. (Devices categorized by their manufacturer as a Laptop)"@en-us ;
	sh:targetClass observable:Laptop .

observable:Library a owl:Class , sh:NodeShape ;
	rdfs:subClassOf observable:ObservableObject ;
	rdfs:label "Library"@en ;
	rdfs:comment "A library is a suite of data and programming code that is used to develop software programs and applications. [based on https://www.techopedia.com/definition/3828/software-library]"@en ;
	sh:targetClass observable:Library .

observable:LibraryFacet a owl:Class , sh:NodeShape ;
	rdfs:subClassOf core:Facet ;
	rdfs:label "LibraryFacet"@en ;
	rdfs:comment "A library facet is a grouping of characteristics unique to a suite of data and programming code that is used to develop software programs and applications. [based on https://www.techopedia.com/definition/3828/software-library]"@en .

_:node1gm7uj6vjx1499 sh:datatype xsd:string ;
	sh:maxCount 1 ;
	sh:nodeKind sh:Literal ;
	sh:path observable:libraryType .

observable:LibraryFacet sh:property _:node1gm7uj6vjx1499 ;
	sh:targetClass observable:LibraryFacet .

observable:MACAddress a owl:Class , sh:NodeShape ;
	rdfs:subClassOf observable:DigitalAddress ;
	rdfs:label "MACAddress"@en ;
	rdfs:comment "A MAC address is a media access control standards conformant identifier assigned to a network interface to enable routing and management of communications at the data link layer of a network segment."@en ;
	sh:targetClass observable:MACAddress .

observable:MACAddressFacet a owl:Class , sh:NodeShape ;
	rdfs:subClassOf observable:DigitalAddressFacet ;
	rdfs:label "MACAddressFacet"@en ;
	rdfs:comment "A MAC address facet is a grouping of characteristics unique to a media access control standards conformant identifier assigned to a network interface to enable routing and management of communications at the data link layer of a network segment."@en ;
	sh:targetClass observable:MACAddressFacet .

observable:MSISDN a owl:DatatypeProperty ;
	rdfs:label "MSISDN"@en ;
	rdfs:comment "Mobile Station International Subscriber Directory Number (MSISDN) is a number used to identify a mobile phone number internationally. MSISDN is defined by the E.164 numbering plan. This number includes a country code and a National Destination Code which identifies the subscriber's operator."@en ;
	rdfs:range xsd:string .

observable:MSISDNType a owl:DatatypeProperty ;
	rdfs:label "MSISDNType"@en ;
	rdfs:comment "???."@en ;
	rdfs:range xsd:string .

observable:Memory a owl:Class , sh:NodeShape ;
	rdfs:subClassOf observable:ObservableObject ;
	rdfs:label "Memory"@en ;
	rdfs:comment "Memory is a particular region of temporary information storage (e.g., RAM (random access memory), ROM (read only memory)) on a digital device."@en ;
	sh:targetClass observable:Memory .

observable:MemoryFacet a owl:Class , sh:NodeShape ;
	rdfs:subClassOf core:Facet ;
	rdfs:label "MemoryFacet"@en ;
	rdfs:comment "A memory facet is a grouping of characteristics unique to a particular region of temporary information storage (e.g., RAM (random access memory), ROM (read only memory)) on a digital device."@en .

_:node1gm7uj6vjx1500 sh:datatype xsd:boolean ;
	sh:maxCount 1 ;
	sh:nodeKind sh:Literal ;
	sh:path observable:isInjected .

observable:MemoryFacet sh:property _:node1gm7uj6vjx1500 .

_:node1gm7uj6vjx1501 sh:datatype xsd:boolean ;
	sh:maxCount 1 ;
	sh:nodeKind sh:Literal ;
	sh:path observable:isMapped .

observable:MemoryFacet sh:property _:node1gm7uj6vjx1501 .

_:node1gm7uj6vjx1502 sh:datatype xsd:boolean ;
	sh:maxCount 1 ;
	sh:nodeKind sh:Literal ;
	sh:path observable:isProtected .

observable:MemoryFacet sh:property _:node1gm7uj6vjx1502 .

_:node1gm7uj6vjx1503 sh:datatype xsd:boolean ;
	sh:maxCount 1 ;
	sh:nodeKind sh:Literal ;
	sh:path observable:isVolatile .

observable:MemoryFacet sh:property _:node1gm7uj6vjx1503 .

_:node1gm7uj6vjx1504 sh:datatype xsd:hexBinary ;
	sh:nodeKind sh:Literal ;
	sh:path observable:regionEndAddress .

observable:MemoryFacet sh:property _:node1gm7uj6vjx1504 .

_:node1gm7uj6vjx1505 sh:datatype xsd:hexBinary ;
	sh:nodeKind sh:Literal ;
	sh:path observable:regionStartAddress .

observable:MemoryFacet sh:property _:node1gm7uj6vjx1505 .

_:node1gm7uj6vjx1506 sh:datatype xsd:integer ;
	sh:maxCount 1 ;
	sh:nodeKind sh:Literal ;
	sh:path observable:regionSize .

observable:MemoryFacet sh:property _:node1gm7uj6vjx1506 .

_:node1gm7uj6vjx1507 sh:datatype vocabulary:MemoryBlockTypeVocab ;
	sh:message "Value is outside the default vocabulary MemoryBlockTypeVocab." ;
	sh:path observable:blockType ;
	sh:severity sh:Info .

observable:MemoryFacet sh:property _:node1gm7uj6vjx1507 .

_:node1gm7uj6vjx1508 sh:maxCount 1 ;
	sh:nodeKind sh:Literal .

_:node1gm7uj6vjx1510 sh:datatype vocabulary:MemoryBlockTypeVocab .

_:node1gm7uj6vjx1509 rdf:first _:node1gm7uj6vjx1510 ;
	rdf:rest _:node1gm7uj6vjx1511 .

_:node1gm7uj6vjx1512 sh:datatype xsd:string .

_:node1gm7uj6vjx1511 rdf:first _:node1gm7uj6vjx1512 ;
	rdf:rest rdf:nil .

_:node1gm7uj6vjx1508 sh:or _:node1gm7uj6vjx1509 ;
	sh:path observable:blockType .

observable:MemoryFacet sh:property _:node1gm7uj6vjx1508 .

_:node1gm7uj6vjx1513 sh:message "Value is not member of the vocabulary MemoryBlockTypeVocab." .

_:node1gm7uj6vjx1515 sh:datatype vocabulary:MemoryBlockTypeVocab .

_:node1gm7uj6vjx1516 rdf:first "Bit-mapped"^^vocabulary:MemoryBlockTypeVocab ;
	rdf:rest _:node1gm7uj6vjx1517 .

_:node1gm7uj6vjx1517 rdf:first "Byte-mapped"^^vocabulary:MemoryBlockTypeVocab ;
	rdf:rest _:node1gm7uj6vjx1518 .

_:node1gm7uj6vjx1518 rdf:first "Initialized"^^vocabulary:MemoryBlockTypeVocab ;
	rdf:rest _:node1gm7uj6vjx1519 .

_:node1gm7uj6vjx1519 rdf:first "Overlay"^^vocabulary:MemoryBlockTypeVocab ;
	rdf:rest _:node1gm7uj6vjx1520 .

_:node1gm7uj6vjx1520 rdf:first "Uninitialized"^^vocabulary:MemoryBlockTypeVocab ;
	rdf:rest rdf:nil .

_:node1gm7uj6vjx1515 sh:in _:node1gm7uj6vjx1516 .

_:node1gm7uj6vjx1514 rdf:first _:node1gm7uj6vjx1515 ;
	rdf:rest _:node1gm7uj6vjx1521 .

_:node1gm7uj6vjx1522 sh:datatype xsd:string .

_:node1gm7uj6vjx1521 rdf:first _:node1gm7uj6vjx1522 ;
	rdf:rest rdf:nil .

_:node1gm7uj6vjx1513 sh:or _:node1gm7uj6vjx1514 ;
	sh:path observable:blockType .

observable:MemoryFacet sh:property _:node1gm7uj6vjx1513 ;
	sh:targetClass observable:MemoryFacet .

observable:Message a owl:Class , sh:NodeShape ;
	rdfs:subClassOf observable:ObservableObject ;
	rdfs:label "Message"@en ;
	rdfs:comment "A message is a discrete unit of electronic communication intended by the source for consumption by some recipient or group of recipients. [based on https://en.wikipedia.org/wiki/Message]"@en ;
	sh:targetClass observable:Message .

observable:MessageFacet a owl:Class , sh:NodeShape ;
	rdfs:subClassOf core:Facet ;
	rdfs:label "MessageFacet"@en ;
	rdfs:comment "A message facet is a grouping of characteristics unique to a discrete unit of electronic communication intended by the source for consumption by some recipient or group of recipients. [based on https://en.wikipedia.org/wiki/Message]"@en .

_:node1gm7uj6vjx1523 sh:class observable:ObservableObject ;
	sh:maxCount 1 ;
	sh:nodeKind sh:IRI ;
	sh:path observable:application .

observable:MessageFacet sh:property _:node1gm7uj6vjx1523 .

_:node1gm7uj6vjx1524 sh:class observable:ObservableObject ;
	sh:maxCount 1 ;
	sh:nodeKind sh:IRI ;
	sh:path observable:from .

observable:MessageFacet sh:property _:node1gm7uj6vjx1524 .

_:node1gm7uj6vjx1525 sh:class observable:ObservableObject ;
	sh:nodeKind sh:IRI ;
	sh:path observable:to .

observable:MessageFacet sh:property _:node1gm7uj6vjx1525 .

_:node1gm7uj6vjx1526 sh:datatype xsd:dateTime ;
	sh:maxCount 1 ;
	sh:nodeKind sh:Literal ;
	sh:path observable:sentTime .

observable:MessageFacet sh:property _:node1gm7uj6vjx1526 .

_:node1gm7uj6vjx1527 sh:datatype xsd:string ;
	sh:maxCount 1 ;
	sh:nodeKind sh:Literal ;
	sh:path observable:messageID .

observable:MessageFacet sh:property _:node1gm7uj6vjx1527 .

_:node1gm7uj6vjx1528 sh:datatype xsd:string ;
	sh:maxCount 1 ;
	sh:nodeKind sh:Literal ;
	sh:path observable:messageText .

observable:MessageFacet sh:property _:node1gm7uj6vjx1528 .

_:node1gm7uj6vjx1529 sh:datatype xsd:string ;
	sh:maxCount 1 ;
	sh:nodeKind sh:Literal ;
	sh:path observable:messageType .

observable:MessageFacet sh:property _:node1gm7uj6vjx1529 .

_:node1gm7uj6vjx1530 sh:datatype xsd:string ;
	sh:maxCount 1 ;
	sh:nodeKind sh:Literal ;
	sh:path observable:sessionID .

observable:MessageFacet sh:property _:node1gm7uj6vjx1530 ;
	sh:targetClass observable:MessageFacet .

observable:MessageThread a owl:Class , sh:NodeShape ;
	rdfs:subClassOf observable:ObservableObject ;
	rdfs:label "MessageTread"@en ;
	rdfs:comment "A message thread is a running commentary of electronic messages pertaining to one topic or question."@en ;
	sh:targetClass observable:MessageThread .

observable:MessageThreadFacet a owl:Class , sh:NodeShape ;
	rdfs:subClassOf core:Facet ;
	rdfs:label "MessageThreadFacet"@en ;
	rdfs:comment "A message thread facet is a grouping of characteristics unique to a running commentary of electronic messages pertaining to one topic or question."@en .

_:node1gm7uj6vjx1531 sh:class observable:Message ;
	sh:description "The contents of ordered items in the Thread linked by messageThread must be Message objects."@en .

_:node1gm7uj6vjx1532 rdf:first observable:messageThread ;
	rdf:rest _:node1gm7uj6vjx1533 .

_:node1gm7uj6vjx1533 rdf:first co:item ;
	rdf:rest _:node1gm7uj6vjx1534 .

_:node1gm7uj6vjx1534 rdf:first co:itemContent ;
	rdf:rest rdf:nil .

_:node1gm7uj6vjx1531 sh:path _:node1gm7uj6vjx1532 .

observable:MessageThreadFacet sh:property _:node1gm7uj6vjx1531 .

_:node1gm7uj6vjx1535 sh:class observable:Message ;
	sh:description "The contents of origin items in the Thread linked by messageThread must be Message objects."@en .

_:node1gm7uj6vjx1536 rdf:first observable:messageThread ;
	rdf:rest _:node1gm7uj6vjx1537 .

_:node1gm7uj6vjx1537 rdf:first types:threadOriginItem ;
	rdf:rest _:node1gm7uj6vjx1538 .

_:node1gm7uj6vjx1538 rdf:first co:itemContent ;
	rdf:rest rdf:nil .

_:node1gm7uj6vjx1535 sh:path _:node1gm7uj6vjx1536 .

observable:MessageThreadFacet sh:property _:node1gm7uj6vjx1535 .

_:node1gm7uj6vjx1539 sh:class observable:Message ;
	sh:description "The contents of terminal items in the Thread linked by messageThread must be Message objects."@en .

_:node1gm7uj6vjx1540 rdf:first observable:messageThread ;
	rdf:rest _:node1gm7uj6vjx1541 .

_:node1gm7uj6vjx1541 rdf:first types:threadTerminalItem ;
	rdf:rest _:node1gm7uj6vjx1542 .

_:node1gm7uj6vjx1542 rdf:first co:itemContent ;
	rdf:rest rdf:nil .

_:node1gm7uj6vjx1539 sh:path _:node1gm7uj6vjx1540 .

observable:MessageThreadFacet sh:property _:node1gm7uj6vjx1539 .

_:node1gm7uj6vjx1543 sh:class observable:Message ;
	sh:description "The contents of unordered items in the Thread linked by messageThread must be Message objects."@en .

_:node1gm7uj6vjx1544 rdf:first observable:messageThread ;
	rdf:rest _:node1gm7uj6vjx1545 .

_:node1gm7uj6vjx1545 rdf:first co:element ;
	rdf:rest rdf:nil .

_:node1gm7uj6vjx1543 sh:path _:node1gm7uj6vjx1544 .

observable:MessageThreadFacet sh:property _:node1gm7uj6vjx1543 .

_:node1gm7uj6vjx1546 sh:class observable:ObservableObject ;
	sh:nodeKind sh:IRI ;
	sh:path observable:participant .

observable:MessageThreadFacet sh:property _:node1gm7uj6vjx1546 .

_:node1gm7uj6vjx1547 sh:class types:Thread ;
	sh:maxCount 1 ;
	sh:nodeKind sh:IRI ;
	sh:path observable:messageThread .

observable:MessageThreadFacet sh:property _:node1gm7uj6vjx1547 .

_:node1gm7uj6vjx1548 sh:datatype xsd:boolean ;
	sh:maxCount 1 ;
	sh:nodeKind sh:Literal ;
	sh:path observable:visibility .

observable:MessageThreadFacet sh:property _:node1gm7uj6vjx1548 ;
	sh:targetClass observable:MessageThreadFacet .

observable:MftRecordFacet a owl:Class , sh:NodeShape ;
	rdfs:subClassOf core:Facet ;
	rdfs:label "MftRecordFacet"@en ;
	rdfs:comment "An MFT record facet is a grouping of characteristics unique to the details of a single file as managed in an NTFS (new technology filesystem) master file table (which is a collection of information about all files on an NTFS filesystem). [based on https://docs.microsoft.com/en-us/windows/win32/devnotes/master-file-table]"@en .

_:node1gm7uj6vjx1549 sh:datatype xsd:dateTime ;
	sh:maxCount 1 ;
	sh:nodeKind sh:Literal ;
	sh:path observable:mftFileNameAccessedTime .

observable:MftRecordFacet sh:property _:node1gm7uj6vjx1549 .

_:node1gm7uj6vjx1550 sh:datatype xsd:dateTime ;
	sh:maxCount 1 ;
	sh:nodeKind sh:Literal ;
	sh:path observable:mftFileNameCreatedTime .

observable:MftRecordFacet sh:property _:node1gm7uj6vjx1550 .

_:node1gm7uj6vjx1551 sh:datatype xsd:dateTime ;
	sh:maxCount 1 ;
	sh:nodeKind sh:Literal ;
	sh:path observable:mftFileNameModifiedTime .

observable:MftRecordFacet sh:property _:node1gm7uj6vjx1551 .

_:node1gm7uj6vjx1552 sh:datatype xsd:dateTime ;
	sh:maxCount 1 ;
	sh:nodeKind sh:Literal ;
	sh:path observable:mftFileNameRecordChangeTime .

observable:MftRecordFacet sh:property _:node1gm7uj6vjx1552 .

_:node1gm7uj6vjx1553 sh:datatype xsd:dateTime ;
	sh:maxCount 1 ;
	sh:nodeKind sh:Literal ;
	sh:path observable:mftRecordChangeTime .

observable:MftRecordFacet sh:property _:node1gm7uj6vjx1553 .

_:node1gm7uj6vjx1554 sh:datatype xsd:integer ;
	sh:maxCount 1 ;
	sh:nodeKind sh:Literal ;
	sh:path observable:mftFileID .

observable:MftRecordFacet sh:property _:node1gm7uj6vjx1554 .

_:node1gm7uj6vjx1555 sh:datatype xsd:integer ;
	sh:maxCount 1 ;
	sh:nodeKind sh:Literal ;
	sh:path observable:mftFileNameLength .

observable:MftRecordFacet sh:property _:node1gm7uj6vjx1555 .

_:node1gm7uj6vjx1556 sh:datatype xsd:integer ;
	sh:maxCount 1 ;
	sh:nodeKind sh:Literal ;
	sh:path observable:mftFlags .

observable:MftRecordFacet sh:property _:node1gm7uj6vjx1556 .

_:node1gm7uj6vjx1557 sh:datatype xsd:integer ;
	sh:maxCount 1 ;
	sh:nodeKind sh:Literal ;
	sh:path observable:mftParentID .

observable:MftRecordFacet sh:property _:node1gm7uj6vjx1557 .

_:node1gm7uj6vjx1558 sh:datatype xsd:integer ;
	sh:maxCount 1 ;
	sh:nodeKind sh:Literal ;
	sh:path observable:ntfsHardLinkCount .

observable:MftRecordFacet sh:property _:node1gm7uj6vjx1558 .

_:node1gm7uj6vjx1559 sh:datatype xsd:string ;
	sh:maxCount 1 ;
	sh:nodeKind sh:Literal ;
	sh:path observable:ntfsOwnerID .

observable:MftRecordFacet sh:property _:node1gm7uj6vjx1559 .

_:node1gm7uj6vjx1560 sh:datatype xsd:string ;
	sh:maxCount 1 ;
	sh:nodeKind sh:Literal ;
	sh:path observable:ntfsOwnerSID .

observable:MftRecordFacet sh:property _:node1gm7uj6vjx1560 ;
	sh:targetClass observable:MftRecordFacet .

observable:MimePartType a owl:Class , sh:NodeShape ;
	rdfs:subClassOf core:UcoInherentCharacterizationThing ;
	rdfs:label "MimePartType"@en ;
	rdfs:comment "A mime part type is a grouping of characteristics unique to a component of a multi-part email body."@en .

_:node1gm7uj6vjx1561 sh:class observable:ObservableObject ;
	sh:maxCount 1 ;
	sh:nodeKind sh:IRI ;
	sh:path observable:bodyRaw .

observable:MimePartType sh:property _:node1gm7uj6vjx1561 .

_:node1gm7uj6vjx1562 sh:datatype xsd:string ;
	sh:maxCount 1 ;
	sh:nodeKind sh:Literal ;
	sh:path observable:body .

observable:MimePartType sh:property _:node1gm7uj6vjx1562 .

observable:RecoveredObjectFacet a owl:Class .

_:node1gm7uj6vjx1563 sh:datatype xsd:string .

observable:RecoveredObjectFacet a sh:NodeShape .

_:node1gm7uj6vjx1563 sh:maxCount 1 .

observable:RecoveredObjectFacet rdfs:subClassOf core:Facet .

_:node1gm7uj6vjx1563 sh:nodeKind sh:Literal .

observable:RecoveredObjectFacet rdfs:label "RecoveredObjectFacet"@en .

_:node1gm7uj6vjx1563 sh:path observable:contentDisposition .

observable:RecoveredObjectFacet rdfs:comment "Recoverability status of name, metadata, and content."@en .

observable:MimePartType sh:property _:node1gm7uj6vjx1563 .

_:node1gm7uj6vjx1705 sh:datatype vocabulary:RecoveredObjectStatusVocab .

_:node1gm7uj6vjx1564 sh:datatype xsd:string .

_:node1gm7uj6vjx1705 sh:message "Value is outside the default vocabulary RecoveredObjectStatusVocab." .

_:node1gm7uj6vjx1564 sh:maxCount 1 .

_:node1gm7uj6vjx1705 sh:path observable:contentRecoveredStatus .

_:node1gm7uj6vjx1564 sh:nodeKind sh:Literal .

_:node1gm7uj6vjx1705 sh:severity sh:Info .

_:node1gm7uj6vjx1564 sh:path observable:contentType .

observable:RecoveredObjectFacet sh:property _:node1gm7uj6vjx1705 .

observable:MimePartType sh:property _:node1gm7uj6vjx1564 .

_:node1gm7uj6vjx1706 sh:datatype vocabulary:RecoveredObjectStatusVocab .

observable:MimePartType sh:targetClass observable:MimePartType .

_:node1gm7uj6vjx1706 sh:message "Value is outside the default vocabulary RecoveredObjectStatusVocab." .

observable:MobileAccount a owl:Class .

_:node1gm7uj6vjx1706 sh:path observable:metadataRecoveredStatus .

observable:MobileAccount a sh:NodeShape .

_:node1gm7uj6vjx1706 sh:severity sh:Info .

observable:MobileAccount rdfs:subClassOf observable:DigitalAccount .

observable:RecoveredObjectFacet sh:property _:node1gm7uj6vjx1706 .

observable:MobileAccount rdfs:label "MobileAccount"@en .

_:node1gm7uj6vjx1707 sh:datatype vocabulary:RecoveredObjectStatusVocab .

observable:MobileAccount rdfs:comment "A mobile account is an arrangement with an entity to enable and control the provision of some capability or service on a portable computing device. [based on https://www.lexico.com/definition/mobile_device]"@en .

_:node1gm7uj6vjx1707 sh:message "Value is outside the default vocabulary RecoveredObjectStatusVocab." .

observable:MobileAccount sh:targetClass observable:MobileAccount .

_:node1gm7uj6vjx1707 sh:path observable:nameRecoveredStatus .

observable:MobileAccountFacet a owl:Class .

_:node1gm7uj6vjx1707 sh:severity sh:Info .

observable:MobileAccountFacet a sh:NodeShape .

observable:RecoveredObjectFacet sh:property _:node1gm7uj6vjx1707 .

observable:MobileAccountFacet rdfs:subClassOf core:Facet .

_:node1gm7uj6vjx1708 sh:maxCount 1 .

observable:MobileAccountFacet rdfs:label "MobileAccountFacet"@en .

_:node1gm7uj6vjx1708 sh:nodeKind sh:Literal .

observable:MobileAccountFacet rdfs:comment "A mobile account facet is a grouping of characteristics unique to an arrangement with an entity to enable and control the provision of some capability or service on a portable computing device. [based on https://www.lexico.com/definition/mobile_device]"@en .

_:node1gm7uj6vjx1710 sh:datatype vocabulary:RecoveredObjectStatusVocab .

_:node1gm7uj6vjx1565 sh:datatype xsd:string .

_:node1gm7uj6vjx1709 rdf:first _:node1gm7uj6vjx1710 .

_:node1gm7uj6vjx1565 sh:maxCount 1 .

_:node1gm7uj6vjx1709 rdf:rest _:node1gm7uj6vjx1711 .

_:node1gm7uj6vjx1565 sh:nodeKind sh:Literal .

_:node1gm7uj6vjx1712 sh:datatype xsd:string .

_:node1gm7uj6vjx1565 sh:path observable:IMSI .

_:node1gm7uj6vjx1711 rdf:first _:node1gm7uj6vjx1712 .

observable:MobileAccountFacet sh:property _:node1gm7uj6vjx1565 .

_:node1gm7uj6vjx1711 rdf:rest rdf:nil .

_:node1gm7uj6vjx1566 sh:datatype xsd:string .

_:node1gm7uj6vjx1708 sh:or _:node1gm7uj6vjx1709 .

_:node1gm7uj6vjx1566 sh:maxCount 1 .

_:node1gm7uj6vjx1708 sh:path observable:nameRecoveredStatus .

_:node1gm7uj6vjx1566 sh:nodeKind sh:Literal .

observable:RecoveredObjectFacet sh:property _:node1gm7uj6vjx1708 .

_:node1gm7uj6vjx1566 sh:path observable:MSISDN .

_:node1gm7uj6vjx1713 sh:maxCount 1 .

observable:MobileAccountFacet sh:property _:node1gm7uj6vjx1566 .

_:node1gm7uj6vjx1713 sh:nodeKind sh:Literal .

_:node1gm7uj6vjx1567 sh:datatype xsd:string .

_:node1gm7uj6vjx1715 sh:datatype vocabulary:RecoveredObjectStatusVocab .

_:node1gm7uj6vjx1567 sh:maxCount 1 .

_:node1gm7uj6vjx1714 rdf:first _:node1gm7uj6vjx1715 .

_:node1gm7uj6vjx1567 sh:nodeKind sh:Literal .

_:node1gm7uj6vjx1714 rdf:rest _:node1gm7uj6vjx1716 .

_:node1gm7uj6vjx1567 sh:path observable:MSISDNType .

_:node1gm7uj6vjx1717 sh:datatype xsd:string .

observable:MobileAccountFacet sh:property _:node1gm7uj6vjx1567 .

_:node1gm7uj6vjx1716 rdf:first _:node1gm7uj6vjx1717 .

observable:MobileAccountFacet sh:targetClass observable:MobileAccountFacet .

_:node1gm7uj6vjx1716 rdf:rest rdf:nil .

observable:MobileDevice a owl:Class .

_:node1gm7uj6vjx1713 sh:or _:node1gm7uj6vjx1714 .

observable:MobileDevice a sh:NodeShape .

_:node1gm7uj6vjx1713 sh:path observable:metadataRecoveredStatus .

observable:MobileDevice rdfs:subClassOf observable:Device .

observable:RecoveredObjectFacet sh:property _:node1gm7uj6vjx1713 .

observable:MobileDevice rdfs:label "MobileDevice"@en .

_:node1gm7uj6vjx1718 sh:maxCount 1 .

observable:MobileDevice rdfs:comment "A mobile device is a portable computing device. [based on https://www.lexico.com.definition/mobile_device]"@en .

_:node1gm7uj6vjx1718 sh:nodeKind sh:Literal .

observable:MobileDevice sh:targetClass observable:MobileDevice .

_:node1gm7uj6vjx1720 sh:datatype vocabulary:RecoveredObjectStatusVocab .

observable:MobileDeviceFacet a owl:Class .

_:node1gm7uj6vjx1719 rdf:first _:node1gm7uj6vjx1720 .

observable:MobileDeviceFacet a sh:NodeShape .

_:node1gm7uj6vjx1719 rdf:rest _:node1gm7uj6vjx1721 .

observable:MobileDeviceFacet rdfs:subClassOf core:Facet .

_:node1gm7uj6vjx1722 sh:datatype xsd:string .

observable:MobileDeviceFacet rdfs:label "MobileDeviceFacet"@en .

_:node1gm7uj6vjx1721 rdf:first _:node1gm7uj6vjx1722 .

observable:MobileDeviceFacet rdfs:comment "A mobile device facet is a grouping of characteristics unique to a portable computing device. [based on https://www.lexico.com/definition/mobile_device]"@en .

_:node1gm7uj6vjx1568 sh:datatype xsd:boolean .

_:node1gm7uj6vjx1721 rdf:rest rdf:nil .

_:node1gm7uj6vjx1568 sh:maxCount 1 .

_:node1gm7uj6vjx1718 sh:or _:node1gm7uj6vjx1719 .

_:node1gm7uj6vjx1568 sh:nodeKind sh:Literal .

_:node1gm7uj6vjx1718 sh:path observable:contentRecoveredStatus .

_:node1gm7uj6vjx1568 sh:path observable:mockLocationsAllowed .

observable:RecoveredObjectFacet sh:property _:node1gm7uj6vjx1718 .

observable:MobileDeviceFacet sh:property _:node1gm7uj6vjx1568 .

_:node1gm7uj6vjx1723 sh:message "Value is not member of the vocabulary RecoveredObjectStatusVocab." .

_:node1gm7uj6vjx1569 sh:datatype xsd:dateTime .

_:node1gm7uj6vjx1725 sh:datatype vocabulary:RecoveredObjectStatusVocab .

_:node1gm7uj6vjx1569 sh:maxCount 1 .

_:node1gm7uj6vjx1726 rdf:first "recovered"^^vocabulary:RecoveredObjectStatusVocab .

_:node1gm7uj6vjx1569 sh:nodeKind sh:Literal .

_:node1gm7uj6vjx1726 rdf:rest _:node1gm7uj6vjx1727 .

_:node1gm7uj6vjx1569 sh:path observable:clockSetting .

_:node1gm7uj6vjx1727 rdf:first "partially recovered"^^vocabulary:RecoveredObjectStatusVocab .

observable:MobileDeviceFacet sh:property _:node1gm7uj6vjx1569 .

_:node1gm7uj6vjx1727 rdf:rest _:node1gm7uj6vjx1728 .

_:node1gm7uj6vjx1570 sh:datatype xsd:dateTime .

_:node1gm7uj6vjx1728 rdf:first "overwritten"^^vocabulary:RecoveredObjectStatusVocab .

_:node1gm7uj6vjx1570 sh:maxCount 1 .

_:node1gm7uj6vjx1728 rdf:rest _:node1gm7uj6vjx1729 .

_:node1gm7uj6vjx1570 sh:nodeKind sh:Literal .

_:node1gm7uj6vjx1729 rdf:first "unknown"^^vocabulary:RecoveredObjectStatusVocab .

_:node1gm7uj6vjx1570 sh:path observable:phoneActivationTime .

_:node1gm7uj6vjx1729 rdf:rest rdf:nil .

observable:MobileDeviceFacet sh:property _:node1gm7uj6vjx1570 .

_:node1gm7uj6vjx1725 sh:in _:node1gm7uj6vjx1726 .

_:node1gm7uj6vjx1571 sh:datatype xsd:integer .

_:node1gm7uj6vjx1724 rdf:first _:node1gm7uj6vjx1725 .

_:node1gm7uj6vjx1571 sh:maxCount 1 .

_:node1gm7uj6vjx1724 rdf:rest _:node1gm7uj6vjx1730 .

_:node1gm7uj6vjx1571 sh:nodeKind sh:Literal .

_:node1gm7uj6vjx1731 sh:datatype xsd:string .

_:node1gm7uj6vjx1571 sh:path observable:storageCapacityInBytes .

_:node1gm7uj6vjx1730 rdf:first _:node1gm7uj6vjx1731 .

observable:MobileDeviceFacet sh:property _:node1gm7uj6vjx1571 .

_:node1gm7uj6vjx1730 rdf:rest rdf:nil .

_:node1gm7uj6vjx1572 sh:datatype xsd:string .

_:node1gm7uj6vjx1723 sh:or _:node1gm7uj6vjx1724 .

_:node1gm7uj6vjx1572 sh:maxCount 1 ;
	sh:nodeKind sh:Literal .

_:node1gm7uj6vjx1723 sh:path observable:nameRecoveredStatus .

_:node1gm7uj6vjx1572 sh:path observable:ESN .

observable:RecoveredObjectFacet sh:property _:node1gm7uj6vjx1723 .

observable:MobileDeviceFacet sh:property _:node1gm7uj6vjx1572 .

_:node1gm7uj6vjx1732 sh:message "Value is not member of the vocabulary RecoveredObjectStatusVocab." .

_:node1gm7uj6vjx1573 sh:datatype xsd:string .

_:node1gm7uj6vjx1734 sh:datatype vocabulary:RecoveredObjectStatusVocab .

_:node1gm7uj6vjx1573 sh:maxCount 1 .

_:node1gm7uj6vjx1735 rdf:first "recovered"^^vocabulary:RecoveredObjectStatusVocab .

_:node1gm7uj6vjx1573 sh:nodeKind sh:Literal .

_:node1gm7uj6vjx1735 rdf:rest _:node1gm7uj6vjx1736 .

_:node1gm7uj6vjx1573 sh:path observable:IMEI .

_:node1gm7uj6vjx1736 rdf:first "partially recovered"^^vocabulary:RecoveredObjectStatusVocab .

observable:MobileDeviceFacet sh:property _:node1gm7uj6vjx1573 .

_:node1gm7uj6vjx1574 sh:datatype xsd:string .

_:node1gm7uj6vjx1736 rdf:rest _:node1gm7uj6vjx1737 .

_:node1gm7uj6vjx1574 sh:maxCount 1 .

_:node1gm7uj6vjx1737 rdf:first "overwritten"^^vocabulary:RecoveredObjectStatusVocab .

_:node1gm7uj6vjx1574 sh:nodeKind sh:Literal .

_:node1gm7uj6vjx1737 rdf:rest _:node1gm7uj6vjx1738 .

_:node1gm7uj6vjx1574 sh:path observable:bluetoothDeviceName .

_:node1gm7uj6vjx1738 rdf:first "unknown"^^vocabulary:RecoveredObjectStatusVocab .

observable:MobileDeviceFacet sh:property _:node1gm7uj6vjx1574 .

_:node1gm7uj6vjx1738 rdf:rest rdf:nil .

_:node1gm7uj6vjx1575 sh:datatype xsd:string .

_:node1gm7uj6vjx1734 sh:in _:node1gm7uj6vjx1735 .

_:node1gm7uj6vjx1575 sh:maxCount 1 .

_:node1gm7uj6vjx1733 rdf:first _:node1gm7uj6vjx1734 .

_:node1gm7uj6vjx1575 sh:nodeKind sh:Literal .

_:node1gm7uj6vjx1733 rdf:rest _:node1gm7uj6vjx1739 .

_:node1gm7uj6vjx1575 sh:path observable:keypadUnlockCode .

_:node1gm7uj6vjx1740 sh:datatype xsd:string .

observable:MobileDeviceFacet sh:property _:node1gm7uj6vjx1575 .

_:node1gm7uj6vjx1739 rdf:first _:node1gm7uj6vjx1740 .

_:node1gm7uj6vjx1576 sh:datatype xsd:string .

_:node1gm7uj6vjx1739 rdf:rest rdf:nil .

_:node1gm7uj6vjx1576 sh:maxCount 1 .

_:node1gm7uj6vjx1732 sh:or _:node1gm7uj6vjx1733 .

_:node1gm7uj6vjx1576 sh:nodeKind sh:Literal .

_:node1gm7uj6vjx1732 sh:path observable:metadataRecoveredStatus .

_:node1gm7uj6vjx1576 sh:path observable:network .

observable:RecoveredObjectFacet sh:property _:node1gm7uj6vjx1732 .

observable:MobileDeviceFacet sh:property _:node1gm7uj6vjx1576 .

_:node1gm7uj6vjx1741 sh:message "Value is not member of the vocabulary RecoveredObjectStatusVocab." .

observable:MobileDeviceFacet sh:targetClass observable:MobileDeviceFacet .

_:node1gm7uj6vjx1743 sh:datatype vocabulary:RecoveredObjectStatusVocab .

observable:MobilePhone a owl:Class .

_:node1gm7uj6vjx1744 rdf:first "recovered"^^vocabulary:RecoveredObjectStatusVocab .

observable:MobilePhone a sh:NodeShape .

_:node1gm7uj6vjx1744 rdf:rest _:node1gm7uj6vjx1745 .

observable:MobilePhone rdfs:subClassOf observable:MobileDevice .

_:node1gm7uj6vjx1745 rdf:first "partially recovered"^^vocabulary:RecoveredObjectStatusVocab .

observable:MobilePhone rdfs:label "MobilePhone"@en-us .

_:node1gm7uj6vjx1745 rdf:rest _:node1gm7uj6vjx1746 .

observable:MobilePhone rdfs:comment "A mobile phone is a portable telephone that at least can make and receive calls over a radio frequency link while the user is moving within a telephone service area. This category encompasses all types of mobiles, simple and smart and satellite ones all together."@en-us .

_:node1gm7uj6vjx1746 rdf:first "overwritten"^^vocabulary:RecoveredObjectStatusVocab .

observable:MobilePhone sh:targetClass observable:MobilePhone .

_:node1gm7uj6vjx1746 rdf:rest _:node1gm7uj6vjx1747 .

observable:Mutex a owl:Class .

_:node1gm7uj6vjx1747 rdf:first "unknown"^^vocabulary:RecoveredObjectStatusVocab .

observable:Mutex a sh:NodeShape .

_:node1gm7uj6vjx1747 rdf:rest rdf:nil .

observable:Mutex rdfs:subClassOf observable:ObservableObject .

_:node1gm7uj6vjx1743 sh:in _:node1gm7uj6vjx1744 .

observable:Mutex rdfs:label "Mutex"@en .

_:node1gm7uj6vjx1742 rdf:first _:node1gm7uj6vjx1743 .

observable:Mutex rdfs:comment "A mutex is a mechanism that enforces limits on access to a resource when there are many threads of execution. A mutex is designed to enforce a mutual exclusion concurrency control policy, and with a variety of possible methods there exists multiple unique implementations for different applications. [based on https://en.wikipedia.org/wiki/Lock_(computer_science)]"@en .

_:node1gm7uj6vjx1742 rdf:rest _:node1gm7uj6vjx1748 .

observable:Mutex sh:targetClass observable:Mutex .

_:node1gm7uj6vjx1749 sh:datatype xsd:string .

observable:MutexFacet a owl:Class .

_:node1gm7uj6vjx1748 rdf:first _:node1gm7uj6vjx1749 .

observable:MutexFacet a sh:NodeShape .

_:node1gm7uj6vjx1748 rdf:rest rdf:nil .

observable:MutexFacet rdfs:subClassOf core:Facet .

_:node1gm7uj6vjx1741 sh:or _:node1gm7uj6vjx1742 .

observable:MutexFacet rdfs:label "MutexFacet"@en .

_:node1gm7uj6vjx1741 sh:path observable:contentRecoveredStatus .

observable:MutexFacet rdfs:comment "A mutex facet is a grouping of characteristics unique to a mechanism that enforces limits on access to a resource when there are many threads of execution. A mutex is designed to enforce a mutual exclusion concurrency control policy, and with a variety of possible methods there exists multiple unique implementations for different applications. [based on https://en.wikipedia.org/wiki/Lock_(computer_science)]"@en .

observable:RecoveredObjectFacet sh:property _:node1gm7uj6vjx1741 .

_:node1gm7uj6vjx1577 sh:datatype xsd:boolean .

observable:RecoveredObjectFacet sh:targetClass observable:RecoveredObjectFacet .

_:node1gm7uj6vjx1577 sh:maxCount 1 .

observable:RegistryDatatype a rdfs:Datatype .

_:node1gm7uj6vjx1577 sh:nodeKind sh:Literal .

_:node1gm7uj6vjx1750 a rdfs:Datatype .

_:node1gm7uj6vjx1577 sh:path observable:isNamed .

_:node1gm7uj6vjx1751 rdf:first "reg_binary" .

observable:MutexFacet sh:property _:node1gm7uj6vjx1577 .

_:node1gm7uj6vjx1751 rdf:rest _:node1gm7uj6vjx1752 .

_:node1gm7uj6vjx1578 sh:datatype xsd:string .

_:node1gm7uj6vjx1752 rdf:first "reg_dword" .

_:node1gm7uj6vjx1578 sh:maxCount 1 .

_:node1gm7uj6vjx1752 rdf:rest _:node1gm7uj6vjx1753 .

_:node1gm7uj6vjx1578 sh:nodeKind sh:Literal .

_:node1gm7uj6vjx1753 rdf:first "reg_dword_big_endian" .

_:node1gm7uj6vjx1578 sh:path observable:mutexName .

_:node1gm7uj6vjx1753 rdf:rest _:node1gm7uj6vjx1754 .

observable:MutexFacet sh:property _:node1gm7uj6vjx1578 .

_:node1gm7uj6vjx1754 rdf:first "reg_expand_sz" .

observable:MutexFacet sh:targetClass observable:MutexFacet .

_:node1gm7uj6vjx1754 rdf:rest _:node1gm7uj6vjx1755 .

observable:NTFSFile a owl:Class .

_:node1gm7uj6vjx1755 rdf:first "reg_full_resource_descriptor" .

observable:NTFSFile a sh:NodeShape .

_:node1gm7uj6vjx1755 rdf:rest _:node1gm7uj6vjx1756 .

observable:NTFSFile rdfs:subClassOf observable:File .

_:node1gm7uj6vjx1756 rdf:first "reg_invalid_type" .

observable:NTFSFile rdfs:label "NTFSFile"@en .

_:node1gm7uj6vjx1756 rdf:rest _:node1gm7uj6vjx1757 .

observable:NTFSFile rdfs:comment "An NTFS file is a New Technology File System (NTFS) file."@en .

_:node1gm7uj6vjx1757 rdf:first "reg_link" .

observable:NTFSFile sh:targetClass observable:NTFSFile .

_:node1gm7uj6vjx1757 rdf:rest _:node1gm7uj6vjx1758 .

observable:NTFSFileFacet a owl:Class .

_:node1gm7uj6vjx1758 rdf:first "reg_multi_sz" .

observable:NTFSFileFacet a sh:NodeShape .

_:node1gm7uj6vjx1758 rdf:rest _:node1gm7uj6vjx1759 .

observable:NTFSFileFacet rdfs:subClassOf core:Facet .

_:node1gm7uj6vjx1759 rdf:first "reg_none" .

observable:NTFSFileFacet rdfs:label "NTFSFileFacet"@en .

_:node1gm7uj6vjx1759 rdf:rest _:node1gm7uj6vjx1760 .

observable:NTFSFileFacet rdfs:comment "An NTFS file facet is a grouping of characteristics unique to a file on an NTFS (new technology filesystem) file system."@en .

_:node1gm7uj6vjx1760 rdf:first "reg_qword" .

_:node1gm7uj6vjx1579 sh:class observable:AlternateDataStream .

_:node1gm7uj6vjx1760 rdf:rest _:node1gm7uj6vjx1761 .

_:node1gm7uj6vjx1579 sh:nodeKind sh:IRI .

_:node1gm7uj6vjx1761 rdf:first "reg_resource_list" .

_:node1gm7uj6vjx1579 sh:path observable:alternateDataStreams .

_:node1gm7uj6vjx1761 rdf:rest _:node1gm7uj6vjx1762 .

observable:NTFSFileFacet sh:property _:node1gm7uj6vjx1579 .

_:node1gm7uj6vjx1762 rdf:first "reg_resource_requirements_list" .

_:node1gm7uj6vjx1580 sh:datatype xsd:integer .

_:node1gm7uj6vjx1762 rdf:rest _:node1gm7uj6vjx1763 .

_:node1gm7uj6vjx1580 sh:maxCount 1 .

_:node1gm7uj6vjx1763 rdf:first "reg_sz" .

_:node1gm7uj6vjx1580 sh:nodeKind sh:Literal .

_:node1gm7uj6vjx1763 rdf:rest rdf:nil .

_:node1gm7uj6vjx1580 sh:path observable:entryID .

_:node1gm7uj6vjx1750 owl:oneOf _:node1gm7uj6vjx1751 .

observable:NTFSFileFacet sh:property _:node1gm7uj6vjx1580 .

observable:RegistryDatatype owl:equivalentClass _:node1gm7uj6vjx1750 .

_:node1gm7uj6vjx1581 sh:datatype xsd:string .

observable:ReparsePoint a owl:Class .

_:node1gm7uj6vjx1581 sh:maxCount 1 .

observable:ReparsePoint a sh:NodeShape .

_:node1gm7uj6vjx1581 sh:nodeKind sh:Literal .

observable:ReparsePoint rdfs:subClassOf observable:FileSystemObject .

_:node1gm7uj6vjx1581 sh:path observable:sid .

observable:ReparsePoint rdfs:label "ReparsePoint"@en .

observable:NTFSFileFacet sh:property _:node1gm7uj6vjx1581 .

observable:ReparsePoint rdfs:comment "A reparse point is a type of NTFS (New Technology File System) object which is an optional attribute of files and directories meant to define some sort of preprocessing before accessing the said file or directory. For instance reparse points can be used to redirect access to files which have been moved to long term storage so that some application would retrieve them and make them directly accessible. A reparse point contains a reparse tag and data that are interpreted by a filesystem filter identified by the tag. [based on https://jp-andre.pagesperso-orange.fr/junctions.html ; https://en.wikipedia.org/wiki/NTFS_reparse_point]"@en .

observable:NTFSFileFacet sh:targetClass observable:NTFSFileFacet .

observable:ReparsePoint sh:targetClass observable:ReparsePoint .

observable:NTFSFilePermissionsFacet a owl:Class .

observable:SIMCard a owl:Class .

observable:NTFSFilePermissionsFacet a sh:NodeShape .

observable:SIMCard a sh:NodeShape .

observable:NTFSFilePermissionsFacet rdfs:subClassOf core:Facet .

observable:SIMCard rdfs:subClassOf observable:Device .

observable:NTFSFilePermissionsFacet rdfs:label "NTFSFilePermissionsFacet"@en .

observable:SIMCard rdfs:label "SIMCard" .

observable:NTFSFilePermissionsFacet rdfs:comment "An NTFS file permissions facet is a grouping of characteristics unique to the access rights (e.g., view, change, navigate, execute) of a file on an NTFS (new technology filesystem) file system."@en .

observable:SIMCard rdfs:comment "A SIM card is a subscriber identification module card intended to securely store the international mobile subscriber identity (IMSI) number and its related key, which are used to identify and authenticate subscribers on mobile telephony. [based on https://en.wikipedia.org/wiki/SIM_card]"@en .

observable:NTFSFilePermissionsFacet sh:targetClass observable:NTFSFilePermissionsFacet .

observable:SIMCard sh:targetClass observable:SIMCard .

observable:NamedPipe a owl:Class .

observable:SIMCardFacet a owl:Class .

observable:NamedPipe a sh:NodeShape .

observable:SIMCardFacet a sh:NodeShape .

observable:NamedPipe rdfs:subClassOf observable:FileSystemObject .

observable:SIMCardFacet rdfs:subClassOf core:Facet .

observable:NamedPipe rdfs:label "NamedPipe"@en .

observable:SIMCardFacet rdfs:label "SIMCardFacet"@en .

observable:NamedPipe rdfs:comment "A named pipe is a mechanism for FIFO (first-in-first-out) inter-process communication. It is persisted as a filesystem object (that can be deleted like any other file), can be written to or read from by any process and exists beyond the lifespan of any process interacting with it (unlike simple anonymous pipes). [based on https://en.wikipedia.org/wiki/Named_pipe]"@en .

observable:SIMCardFacet rdfs:comment "A SIM card facet is a grouping of characteristics unique to a subscriber identification module card intended to securely store the international mobile subscriber identity (IMSI) number and its related key, which are used to identify and authenticate subscribers on mobile telephony devices (such as mobile phones and computers). [based on https://en.wikipedia.org/wiki/SIM_card]"@en .

observable:NamedPipe sh:targetClass observable:NamedPipe .

_:node1gm7uj6vjx1764 sh:class identity:Identity .

observable:NetworkAppliance a owl:Class .

_:node1gm7uj6vjx1764 sh:maxCount 1 .

observable:NetworkAppliance a sh:NodeShape .

_:node1gm7uj6vjx1764 sh:nodeKind sh:IRI .

observable:NetworkAppliance rdfs:subClassOf observable:Appliance .

_:node1gm7uj6vjx1764 sh:path observable:carrier .

observable:NetworkAppliance rdfs:label "NetworkAppliance"@en .

observable:SIMCardFacet sh:property _:node1gm7uj6vjx1764 .

observable:NetworkAppliance rdfs:comment "A network appliance is a purpose-built computer with software or firmware that is designed to provide a specific network management function."@en .

_:node1gm7uj6vjx1765 sh:datatype xsd:integer .

observable:NetworkAppliance sh:targetClass observable:NetworkAppliance .

_:node1gm7uj6vjx1765 sh:maxCount 1 .

observable:NetworkConnection a owl:Class .

_:node1gm7uj6vjx1765 sh:nodeKind sh:Literal .

observable:NetworkConnection a sh:NodeShape .

_:node1gm7uj6vjx1765 sh:path observable:storageCapacityInBytes .

observable:NetworkConnection rdfs:subClassOf observable:ObservableObject .

observable:SIMCardFacet sh:property _:node1gm7uj6vjx1765 .

observable:NetworkConnection rdfs:label "NetworkConnection"@en .

_:node1gm7uj6vjx1766 sh:datatype xsd:string .

observable:NetworkConnection rdfs:comment "A network connection is a connection (completed or attempted) across a digital network (a group of two or more computer systems linked together). [based on https://www.webopedia.com/TERM/N/network.html]"@en .

_:node1gm7uj6vjx1766 sh:maxCount 1 .

observable:NetworkConnection sh:targetClass observable:NetworkConnection .

_:node1gm7uj6vjx1766 sh:nodeKind sh:Literal .

observable:NetworkConnectionFacet a owl:Class .

_:node1gm7uj6vjx1766 sh:path observable:ICCID .

observable:NetworkConnectionFacet a sh:NodeShape .

observable:SIMCardFacet sh:property _:node1gm7uj6vjx1766 .

observable:NetworkConnectionFacet rdfs:subClassOf core:Facet .

_:node1gm7uj6vjx1767 sh:datatype xsd:string .

observable:NetworkConnectionFacet rdfs:label "NetworkConnectionFacet"@en .

_:node1gm7uj6vjx1767 sh:maxCount 1 .

observable:NetworkConnectionFacet rdfs:comment "A network connection facet is a grouping of characteristics unique to a connection (complete or attempted) accross a digital network (a group of two or more computer systems linked together). [based on https://www.webopedia.com/TERM/N/network.html]"@en .

_:node1gm7uj6vjx1767 sh:nodeKind sh:Literal .

_:node1gm7uj6vjx1582 sh:class core:UcoObject .

_:node1gm7uj6vjx1767 sh:path observable:IMSI .

_:node1gm7uj6vjx1582 sh:nodeKind sh:IRI .

observable:SIMCardFacet sh:property _:node1gm7uj6vjx1767 .

_:node1gm7uj6vjx1582 sh:path observable:src .

_:node1gm7uj6vjx1768 sh:datatype xsd:string .

observable:NetworkConnectionFacet sh:property _:node1gm7uj6vjx1582 .

_:node1gm7uj6vjx1768 sh:maxCount 1 .

_:node1gm7uj6vjx1583 sh:class observable:ObservableObject .

_:node1gm7uj6vjx1768 sh:nodeKind sh:Literal .

_:node1gm7uj6vjx1583 sh:nodeKind sh:IRI .

_:node1gm7uj6vjx1768 sh:path observable:PIN .

_:node1gm7uj6vjx1583 sh:path observable:dst .

observable:SIMCardFacet sh:property _:node1gm7uj6vjx1768 .

observable:NetworkConnectionFacet sh:property _:node1gm7uj6vjx1583 .

_:node1gm7uj6vjx1769 sh:datatype xsd:string .

_:node1gm7uj6vjx1584 sh:class types:ControlledDictionary .

_:node1gm7uj6vjx1769 sh:maxCount 1 .

_:node1gm7uj6vjx1584 sh:maxCount 1 .

_:node1gm7uj6vjx1769 sh:nodeKind sh:Literal .

_:node1gm7uj6vjx1584 sh:nodeKind sh:IRI .

_:node1gm7uj6vjx1769 sh:path observable:PUK .

_:node1gm7uj6vjx1584 sh:path observable:protocols .

observable:SIMCardFacet sh:property _:node1gm7uj6vjx1769 .

observable:NetworkConnectionFacet sh:property _:node1gm7uj6vjx1584 .

_:node1gm7uj6vjx1770 sh:datatype xsd:string .

_:node1gm7uj6vjx1585 sh:datatype xsd:boolean .

_:node1gm7uj6vjx1770 sh:maxCount 1 .

_:node1gm7uj6vjx1585 sh:maxCount 1 .

_:node1gm7uj6vjx1770 sh:nodeKind sh:Literal .

_:node1gm7uj6vjx1585 sh:nodeKind sh:Literal .

_:node1gm7uj6vjx1770 sh:path observable:SIMForm .

_:node1gm7uj6vjx1585 sh:path observable:isActive .

observable:SIMCardFacet sh:property _:node1gm7uj6vjx1770 .

observable:NetworkConnectionFacet sh:property _:node1gm7uj6vjx1585 .

_:node1gm7uj6vjx1771 sh:datatype xsd:string .

_:node1gm7uj6vjx1586 sh:datatype xsd:dateTime .

_:node1gm7uj6vjx1771 sh:maxCount 1 .

_:node1gm7uj6vjx1586 sh:maxCount 1 .

_:node1gm7uj6vjx1771 sh:nodeKind sh:Literal .

_:node1gm7uj6vjx1586 sh:nodeKind sh:Literal .

_:node1gm7uj6vjx1771 sh:path observable:SIMType .

_:node1gm7uj6vjx1586 sh:path observable:endTime .

observable:SIMCardFacet sh:property _:node1gm7uj6vjx1771 .

observable:NetworkConnectionFacet sh:property _:node1gm7uj6vjx1586 .

observable:SIMCardFacet sh:targetClass observable:SIMCardFacet .

_:node1gm7uj6vjx1587 sh:datatype xsd:dateTime .

observable:SIMForm a owl:DatatypeProperty .

_:node1gm7uj6vjx1587 sh:maxCount 1 .

observable:SIMForm rdfs:label "SIMForm"@en .

_:node1gm7uj6vjx1587 sh:nodeKind sh:Literal .

observable:SIMForm rdfs:comment "The form of SIM card such as SIM, Micro SIM, Nano SIM."@en .

_:node1gm7uj6vjx1587 sh:path observable:startTime .

observable:SIMForm rdfs:range xsd:string .

observable:NetworkConnectionFacet sh:property _:node1gm7uj6vjx1587 .

observable:SIMType a owl:DatatypeProperty .

_:node1gm7uj6vjx1588 sh:datatype xsd:integer .

observable:SIMType rdfs:label "SIMType"@en .

_:node1gm7uj6vjx1588 sh:maxCount 1 .

observable:SIMType rdfs:comment "The type of SIM card such as SIM, USIM, UICC."@en .

_:node1gm7uj6vjx1588 sh:nodeKind sh:Literal .

observable:SIMType rdfs:range xsd:string .

_:node1gm7uj6vjx1588 sh:path observable:destinationPort .

observable:SIPAddress a owl:Class .

observable:NetworkConnectionFacet sh:property _:node1gm7uj6vjx1588 .

observable:SIPAddress a sh:NodeShape .

_:node1gm7uj6vjx1589 sh:datatype xsd:integer .

observable:SIPAddress rdfs:subClassOf observable:DigitalAddress .

_:node1gm7uj6vjx1589 sh:maxCount 1 .

observable:SIPAddress rdfs:label "SIPAddress"@en .

_:node1gm7uj6vjx1589 sh:nodeKind sh:Literal .

observable:SIPAddress rdfs:comment "A SIP address is an identifier for Session Initiation Protocol (SIP) communication."@en .

_:node1gm7uj6vjx1589 sh:path observable:sourcePort .

observable:SIPAddress sh:targetClass observable:SIPAddress .

observable:NetworkConnectionFacet sh:property _:node1gm7uj6vjx1589 .

observable:SIPAddressFacet a owl:Class .

observable:NetworkConnectionFacet sh:targetClass observable:NetworkConnectionFacet .

observable:SIPAddressFacet a sh:NodeShape .

observable:NetworkFlow a owl:Class .

observable:SIPAddressFacet rdfs:subClassOf observable:DigitalAddressFacet .

observable:NetworkFlow a sh:NodeShape .

observable:SIPAddressFacet rdfs:label "SIPAddressFacet"@en .

observable:NetworkFlow rdfs:subClassOf observable:ObservableObject .

observable:SIPAddressFacet rdfs:comment "A SIP address facet is a grouping of characteristics unique to a Session Initiation Protocol (SIP) standards conformant identifier assigned to a user to enable routing and management of SIP standards conformant communication to or from that user loosely coupled from any particular devices."@en .

observable:NetworkFlow rdfs:label "NetworkFlow"@en .

observable:SIPAddressFacet sh:targetClass observable:SIPAddressFacet .

observable:NetworkFlow rdfs:comment "A network flow is a sequence of data transiting one or more digital network (a group or two or more computer systems linked together) connections. [based on https://www.webopedia.com/TERM/N/network.html]"@en .

observable:SMSMessage a owl:Class .

observable:NetworkFlow sh:targetClass observable:NetworkFlow .

observable:SMSMessage a sh:NodeShape .

observable:NetworkFlowFacet a owl:Class .

observable:SMSMessage rdfs:subClassOf observable:Message .

observable:NetworkFlowFacet a sh:NodeShape .

observable:SMSMessage rdfs:label "SMSMessage"@en .

observable:NetworkFlowFacet rdfs:subClassOf core:Facet .

observable:SMSMessage rdfs:comment "An SMS message is a message conformant to the short message service (SMS) communication protocol standards."@en .

observable:NetworkFlowFacet rdfs:label "NetworkFlowFacet"@en .

observable:SMSMessage sh:targetClass observable:SMSMessage .

observable:NetworkFlowFacet rdfs:comment "A network flow facet is a grouping of characteristics unique to a sequence of data transiting one or more digital network (a group of two or more computer systems linked together) connections. [based on https://www.webopedia.com/TERM/N/network.html]"@en .

observable:SMSMessageFacet a owl:Class .

_:node1gm7uj6vjx1590 sh:class observable:ObservableObject .

observable:SMSMessageFacet a sh:NodeShape .

_:node1gm7uj6vjx1590 sh:maxCount 1 .

observable:SMSMessageFacet rdfs:subClassOf core:Facet .

_:node1gm7uj6vjx1590 sh:nodeKind sh:IRI .

observable:SMSMessageFacet rdfs:label "SMSMessageFacet"@en .

_:node1gm7uj6vjx1590 sh:path observable:dstPayload .

observable:SMSMessageFacet rdfs:comment "A SMS message facet is a grouping of characteristics unique to a message conformant to the short message service (SMS) communication protocol standards."@en .

observable:NetworkFlowFacet sh:property _:node1gm7uj6vjx1590 .

_:node1gm7uj6vjx1772 sh:datatype xsd:boolean .

_:node1gm7uj6vjx1591 sh:class observable:ObservableObject .

_:node1gm7uj6vjx1772 sh:maxCount 1 .

_:node1gm7uj6vjx1591 sh:maxCount 1 .

_:node1gm7uj6vjx1772 sh:nodeKind sh:Literal .

_:node1gm7uj6vjx1591 sh:nodeKind sh:IRI .

_:node1gm7uj6vjx1772 sh:path observable:isRead .

_:node1gm7uj6vjx1591 sh:path observable:srcPayload .

observable:SMSMessageFacet sh:property _:node1gm7uj6vjx1772 .

observable:NetworkFlowFacet sh:property _:node1gm7uj6vjx1591 .

observable:SMSMessageFacet sh:targetClass observable:SMSMessageFacet .

_:node1gm7uj6vjx1592 sh:class types:Dictionary .

observable:SQLiteBlob a owl:Class .

_:node1gm7uj6vjx1592 sh:maxCount 1 .

observable:SQLiteBlob a sh:NodeShape .

_:node1gm7uj6vjx1592 sh:nodeKind sh:IRI .

observable:SQLiteBlob rdfs:subClassOf observable:ObservableObject .

_:node1gm7uj6vjx1592 sh:path observable:ipfix .

observable:SQLiteBlob rdfs:label "SQLiteBlob"@en .

observable:NetworkFlowFacet sh:property _:node1gm7uj6vjx1592 .

observable:SQLiteBlob rdfs:comment "An SQLite blob is a blob (binary large object) of data within an SQLite database. [based on https://en.wikipedia.org/wiki/SQLite]"@en .

_:node1gm7uj6vjx1593 sh:datatype xsd:integer .

observable:SQLiteBlob sh:targetClass observable:SQLiteBlob .

_:node1gm7uj6vjx1593 sh:maxCount 1 .

observable:SQLiteBlobFacet a owl:Class .

_:node1gm7uj6vjx1593 sh:nodeKind sh:Literal .

observable:SQLiteBlobFacet a sh:NodeShape .

_:node1gm7uj6vjx1593 sh:path observable:dstBytes .

observable:SQLiteBlobFacet rdfs:subClassOf core:Facet .

observable:NetworkFlowFacet sh:property _:node1gm7uj6vjx1593 .

observable:SQLiteBlobFacet rdfs:label "SQLiteBlobFacet"@en .

_:node1gm7uj6vjx1594 sh:datatype xsd:integer .

observable:SQLiteBlobFacet rdfs:comment "An SQLite blob facet is a grouping of characteristics unique to a blob (binary large object) of data within an SQLite database. [based on https://en.wikipedia.org/wiki/SQLite]"@en .

_:node1gm7uj6vjx1594 sh:maxCount 1 .

_:node1gm7uj6vjx1773 sh:datatype xsd:positiveInteger .

_:node1gm7uj6vjx1594 sh:nodeKind sh:Literal .

_:node1gm7uj6vjx1773 sh:nodeKind sh:Literal .

_:node1gm7uj6vjx1594 sh:path observable:dstPackets .

_:node1gm7uj6vjx1773 sh:path observable:rowIndex .

observable:NetworkFlowFacet sh:property _:node1gm7uj6vjx1594 .

observable:SQLiteBlobFacet sh:property _:node1gm7uj6vjx1773 .

_:node1gm7uj6vjx1595 sh:datatype xsd:integer .

_:node1gm7uj6vjx1774 sh:datatype xsd:string .

_:node1gm7uj6vjx1595 sh:maxCount 1 .

_:node1gm7uj6vjx1774 sh:maxCount 1 .

_:node1gm7uj6vjx1595 sh:nodeKind sh:Literal .

_:node1gm7uj6vjx1774 sh:nodeKind sh:Literal .

_:node1gm7uj6vjx1595 sh:path observable:srcBytes .

_:node1gm7uj6vjx1774 sh:path observable:columnName .

observable:NetworkFlowFacet sh:property _:node1gm7uj6vjx1595 .

observable:SQLiteBlobFacet sh:property _:node1gm7uj6vjx1774 .

_:node1gm7uj6vjx1596 sh:datatype xsd:integer .

_:node1gm7uj6vjx1775 sh:datatype xsd:string .

_:node1gm7uj6vjx1596 sh:maxCount 1 .

_:node1gm7uj6vjx1775 sh:maxCount 1 .

_:node1gm7uj6vjx1596 sh:nodeKind sh:Literal .

_:node1gm7uj6vjx1775 sh:nodeKind sh:Literal .

_:node1gm7uj6vjx1596 sh:path observable:srcPackets .

_:node1gm7uj6vjx1775 sh:path observable:rowCondition .

observable:NetworkFlowFacet sh:property _:node1gm7uj6vjx1596 .

observable:SQLiteBlobFacet sh:property _:node1gm7uj6vjx1775 .

observable:NetworkFlowFacet sh:targetClass observable:NetworkFlowFacet .

_:node1gm7uj6vjx1776 sh:datatype xsd:string .

observable:NetworkInterface a owl:Class .

_:node1gm7uj6vjx1776 sh:maxCount 1 .

observable:NetworkInterface a sh:NodeShape .

_:node1gm7uj6vjx1776 sh:nodeKind sh:Literal .

observable:NetworkInterface rdfs:subClassOf observable:ObservableObject .

_:node1gm7uj6vjx1776 sh:path observable:tableName .

observable:NetworkInterface rdfs:label "NetworkInterface"@en .

observable:SQLiteBlobFacet sh:property _:node1gm7uj6vjx1776 .

observable:NetworkInterface rdfs:comment "A network interface is a software or hardware interface between two pieces of equipment or protocol layers in a computer network."@en .

observable:SQLiteBlobFacet sh:targetClass observable:SQLiteBlobFacet .

observable:NetworkInterface sh:targetClass observable:NetworkInterface .

observable:SecurityAppliance a owl:Class .

observable:NetworkInterfaceFacet a owl:Class .

observable:SecurityAppliance a sh:NodeShape .

observable:NetworkInterfaceFacet a sh:NodeShape .

observable:SecurityAppliance rdfs:subClassOf observable:Appliance .

observable:NetworkInterfaceFacet rdfs:subClassOf core:Facet .

observable:SecurityAppliance rdfs:label "SecurityAppliance"@en .

observable:NetworkInterfaceFacet rdfs:label "NetworkInterfaceFacet"@en .

observable:SecurityAppliance rdfs:comment "A security appliance is a purpose-built computer with software or firmware that is designed to provide a specific security function to protect computer networks."@en .

observable:NetworkInterfaceFacet rdfs:comment "A network interface facet is a grouping of characteristics unique to a software or hardware interface between two pieces of equipment or protocol layers in a computer network."@en .

observable:SecurityAppliance sh:targetClass observable:SecurityAppliance .

_:node1gm7uj6vjx1597 sh:class observable:ObservableObject .

observable:Semaphore a owl:Class .

_:node1gm7uj6vjx1597 sh:maxCount 1 .

observable:Semaphore a sh:NodeShape .

_:node1gm7uj6vjx1597 sh:nodeKind sh:IRI .

observable:Semaphore rdfs:subClassOf observable:ObservableObject .

_:node1gm7uj6vjx1597 sh:path observable:macAddress .

observable:Semaphore rdfs:label "Semaphore"@en .

observable:NetworkInterfaceFacet sh:property _:node1gm7uj6vjx1597 .

observable:Semaphore rdfs:comment "A semaphore is a variable or abstract data type used to control access to a common resource by multiple processes and avoid critical section problems in a concurrent system such as a multitasking operating system. [based on https://en.wikipedia.org/wiki/Semaphore_(programming)]"@en .

_:node1gm7uj6vjx1598 sh:class observable:ObservableObject .

observable:Semaphore sh:targetClass observable:Semaphore .

_:node1gm7uj6vjx1598 sh:nodeKind sh:IRI .

observable:SendControlCodeEffectFacet a owl:Class .

_:node1gm7uj6vjx1598 sh:path observable:dhcpServer .

observable:SendControlCodeEffectFacet a sh:NodeShape .

observable:NetworkInterfaceFacet sh:property _:node1gm7uj6vjx1598 .

observable:SendControlCodeEffectFacet rdfs:subClassOf observable:DefinedEffectFacet .

_:node1gm7uj6vjx1599 sh:class observable:ObservableObject .

observable:SendControlCodeEffectFacet rdfs:label "SendControlCodeEffectFacet"@en .

_:node1gm7uj6vjx1599 sh:nodeKind sh:IRI .

observable:SendControlCodeEffectFacet rdfs:comment "A send control code effect facet is a grouping of characteristics unique to the effects of actions upon observable objects where a control code, or other control-oriented communication signal, is sent to the observable object. An example of this would be an action sending a control code changing the running state of a process."@en .

_:node1gm7uj6vjx1599 sh:path observable:ip .

_:node1gm7uj6vjx1777 sh:datatype xsd:string .

observable:NetworkInterfaceFacet sh:property _:node1gm7uj6vjx1599 .

_:node1gm7uj6vjx1777 sh:maxCount 1 .

_:node1gm7uj6vjx1600 sh:class observable:ObservableObject .

_:node1gm7uj6vjx1777 sh:nodeKind sh:Literal .

_:node1gm7uj6vjx1600 sh:nodeKind sh:IRI .

_:node1gm7uj6vjx1777 sh:path observable:controlCode .

_:node1gm7uj6vjx1600 sh:path observable:ipGateway .

observable:SendControlCodeEffectFacet sh:property _:node1gm7uj6vjx1777 .

observable:NetworkInterfaceFacet sh:property _:node1gm7uj6vjx1600 .

observable:SendControlCodeEffectFacet sh:targetClass observable:SendControlCodeEffectFacet .

_:node1gm7uj6vjx1601 sh:datatype xsd:dateTime .

observable:Server a owl:Class .

_:node1gm7uj6vjx1601 sh:maxCount 1 .

observable:Server a sh:NodeShape .

_:node1gm7uj6vjx1601 sh:nodeKind sh:Literal .

observable:Server rdfs:subClassOf observable:Computer .

_:node1gm7uj6vjx1601 sh:path observable:dhcpLeaseExpires .

observable:Server rdfs:label "Server"@en-us .

observable:NetworkInterfaceFacet sh:property _:node1gm7uj6vjx1601 .

observable:Server rdfs:comment "A server is a server rack-mount based computer, minicomputer, supercomputer, etc."@en-us .

_:node1gm7uj6vjx1602 sh:datatype xsd:dateTime .

observable:Server sh:targetClass observable:Server .

_:node1gm7uj6vjx1602 sh:maxCount 1 .

observable:ShopListing a owl:Class .

_:node1gm7uj6vjx1602 sh:nodeKind sh:Literal .

observable:ShopListing a sh:NodeShape .

_:node1gm7uj6vjx1602 sh:path observable:dhcpLeaseObtained .

observable:ShopListing rdfs:subClassOf observable:ObservableObject .

observable:NetworkInterfaceFacet sh:property _:node1gm7uj6vjx1602 .

observable:ShopListing rdfs:label "ShopListing"@en .

_:node1gm7uj6vjx1603 sh:datatype xsd:string .

observable:ShopListing rdfs:comment "A shop listing is a listing of offered products on an online marketplace/shop."@en .

_:node1gm7uj6vjx1603 sh:maxCount 1 .

observable:ShopListing sh:targetClass observable:ShopListing .

_:node1gm7uj6vjx1603 sh:nodeKind sh:Literal .

observable:SmartDevice a owl:Class .

_:node1gm7uj6vjx1603 sh:path observable:adapterName .

observable:SmartDevice a sh:NodeShape .

observable:NetworkInterfaceFacet sh:property _:node1gm7uj6vjx1603 .

observable:SmartDevice rdfs:subClassOf observable:Device .

observable:NetworkInterfaceFacet sh:targetClass observable:NetworkInterfaceFacet .

observable:SmartDevice rdfs:label "SmartDevice"@en-us .

observable:NetworkProtocol a owl:Class .

observable:SmartDevice rdfs:comment "A smart device is a microprocessor IoT device that is expected to be connected directly to cloud-based networks or via smartphone"@en-us .

observable:NetworkProtocol a sh:NodeShape .

observable:SmartDevice sh:targetClass observable:SmartDevice .

observable:NetworkProtocol rdfs:subClassOf observable:ObservableObject .

observable:SmartPhone a owl:Class .

observable:NetworkProtocol rdfs:label "NetworkProtocol"@en .

observable:SmartPhone a sh:NodeShape .

observable:NetworkProtocol rdfs:comment "A network protocol is an established set of structured rules that determine how data is transmitted between different devices in the same network. Essentially, it allows connected devices to communicate with each other, regardless of any differences in their internal processes, structure or design. [based on https://www.comptia.org/content/guides/what-is-a-network-protocol]"@en .

observable:SmartPhone rdfs:subClassOf observable:Computer .

observable:NetworkProtocol sh:targetClass observable:NetworkProtocol .

observable:SmartPhone rdfs:subClassOf observable:MobilePhone .

observable:NetworkRoute a owl:Class .

observable:SmartPhone rdfs:subClassOf observable:SmartDevice .

observable:NetworkRoute a sh:NodeShape .

observable:SmartPhone rdfs:label "SmartPhone"@en-us .

observable:NetworkRoute rdfs:subClassOf observable:ObservableObject .

observable:SmartPhone rdfs:comment "A smartphone is a portable device that combines mobile telephone and computing functions into one unit.  Examples include iPhone, Samsung Galaxy, Huawei, Blackberry. (Inferred by model and OperatingSystemFacet)"@en-us .

observable:NetworkRoute rdfs:label "NetworkRoute"@en .

observable:SmartPhone sh:targetClass observable:SmartPhone .

observable:NetworkRoute rdfs:comment "A network route is a specific path (of specific network nodes, connections and protocols) for traffic in a network or between or across multiple networks."@en .

observable:Snapshot a owl:Class .

observable:NetworkRoute sh:targetClass observable:NetworkRoute .

observable:Snapshot a sh:NodeShape .

observable:NetworkSocketAddressFamily a rdfs:Datatype .

observable:Snapshot rdfs:subClassOf observable:FileSystemObject .

_:node1gm7uj6vjx1604 a rdfs:Datatype .

observable:Snapshot rdfs:label "Snapshot"@en .

_:node1gm7uj6vjx1605 rdf:first "af_appletalk" .

observable:Snapshot rdfs:comment "A snapshot is a file system object representing a snapshot of the contents of a part of a file system at a point in time."@en .

_:node1gm7uj6vjx1605 rdf:rest _:node1gm7uj6vjx1606 .

observable:Snapshot sh:targetClass observable:Snapshot .

_:node1gm7uj6vjx1606 rdf:first "af_bth" .

observable:Socket a owl:Class .

_:node1gm7uj6vjx1606 rdf:rest _:node1gm7uj6vjx1607 .

observable:Socket a sh:NodeShape .

_:node1gm7uj6vjx1607 rdf:first "af_inet" .

observable:Socket rdfs:subClassOf observable:FileSystemObject .

_:node1gm7uj6vjx1607 rdf:rest _:node1gm7uj6vjx1608 .

observable:Socket rdfs:label "Socket"@en .

_:node1gm7uj6vjx1608 rdf:first "af_inet6" .

observable:Socket rdfs:comment "A socket is a special file used for inter-process communication, which enables communication between two processes. In addition to sending data, processes can send file descriptors across a Unix domain socket connection using the sendmsg() and recvmsg() system calls. Unlike named pipes which allow only unidirectional data flow, sockets are fully duplex-capable. [based on https://en.wikipedia.org/wiki/Unix_file_types]"@en .

_:node1gm7uj6vjx1608 rdf:rest _:node1gm7uj6vjx1609 .

observable:Socket sh:targetClass observable:Socket .

_:node1gm7uj6vjx1609 rdf:first "af_ipx" .

observable:SocketAddress a owl:Class .

_:node1gm7uj6vjx1609 rdf:rest _:node1gm7uj6vjx1610 .

observable:SocketAddress a sh:NodeShape .

_:node1gm7uj6vjx1610 rdf:first "af_irda" .

observable:SocketAddress rdfs:subClassOf observable:Address .

_:node1gm7uj6vjx1610 rdf:rest _:node1gm7uj6vjx1611 .

observable:SocketAddress rdfs:label "SocketAddress"@en .

_:node1gm7uj6vjx1611 rdf:first "af_netbios" .

observable:SocketAddress rdfs:comment "A socket address (combining and IP address and a port number) is a composite identifier for a network socket endpoint supporting internet protocol communications."@en .

_:node1gm7uj6vjx1611 rdf:rest _:node1gm7uj6vjx1612 .

observable:SocketAddress sh:targetClass observable:SocketAddress .

_:node1gm7uj6vjx1612 rdf:first "af_unspec" .

observable:Software a owl:Class .

_:node1gm7uj6vjx1612 rdf:rest rdf:nil .

observable:Software a sh:NodeShape .

_:node1gm7uj6vjx1604 owl:oneOf _:node1gm7uj6vjx1605 .

observable:Software rdfs:subClassOf observable:ObservableObject .

observable:NetworkSocketAddressFamily owl:equivalentClass _:node1gm7uj6vjx1604 .

observable:Software rdfs:label "Software"@en .

observable:NetworkSocketProtocolFamily a rdfs:Datatype .

observable:Software rdfs:comment "Software is a definitely scoped instance of a collection of data or computer instructions that tell the computer how to work. [based on https://en.wikipedia.org/wiki/Software]"@en .

_:node1gm7uj6vjx1613 a rdfs:Datatype .

observable:Software sh:targetClass observable:Software .

_:node1gm7uj6vjx1614 rdf:first "pf_appletalk" .

observable:SoftwareFacet a owl:Class .

_:node1gm7uj6vjx1614 rdf:rest _:node1gm7uj6vjx1615 .

observable:SoftwareFacet a sh:NodeShape .

_:node1gm7uj6vjx1615 rdf:first "pf_ash" .

observable:SoftwareFacet rdfs:subClassOf core:Facet .

_:node1gm7uj6vjx1615 rdf:rest _:node1gm7uj6vjx1616 .

observable:SoftwareFacet rdfs:label "SoftwareFacet"@en .

_:node1gm7uj6vjx1616 rdf:first "pf_atmpvc" .

observable:SoftwareFacet rdfs:comment "A software facet is a grouping of characteristics unique to a software program (a definitively scoped instance of a collection of data or computer instructions that tell the computer how to work). [based on https://en.wikipedia.org/wiki/Software]"@en .

_:node1gm7uj6vjx1616 rdf:rest _:node1gm7uj6vjx1617 .

_:node1gm7uj6vjx1778 sh:class identity:Identity .

_:node1gm7uj6vjx1617 rdf:first "pf_atmsvc" .

_:node1gm7uj6vjx1778 sh:maxCount 1 .

_:node1gm7uj6vjx1617 rdf:rest _:node1gm7uj6vjx1618 .

_:node1gm7uj6vjx1778 sh:nodeKind sh:IRI .

_:node1gm7uj6vjx1618 rdf:first "pf_ax25" .

_:node1gm7uj6vjx1778 sh:path observable:manufacturer .

_:node1gm7uj6vjx1618 rdf:rest _:node1gm7uj6vjx1619 .

observable:SoftwareFacet sh:property _:node1gm7uj6vjx1778 .

_:node1gm7uj6vjx1619 rdf:first "pf_bluetooth" .

_:node1gm7uj6vjx1779 sh:datatype xsd:string .

_:node1gm7uj6vjx1619 rdf:rest _:node1gm7uj6vjx1620 .

_:node1gm7uj6vjx1779 sh:maxCount 1 .

_:node1gm7uj6vjx1620 rdf:first "pf_bridge" .

_:node1gm7uj6vjx1779 sh:nodeKind sh:Literal .

_:node1gm7uj6vjx1620 rdf:rest _:node1gm7uj6vjx1621 .

_:node1gm7uj6vjx1779 sh:path observable:cpeid .

_:node1gm7uj6vjx1621 rdf:first "pf_decnet" .

observable:SoftwareFacet sh:property _:node1gm7uj6vjx1779 .

_:node1gm7uj6vjx1621 rdf:rest _:node1gm7uj6vjx1622 .

_:node1gm7uj6vjx1780 sh:datatype xsd:string .

_:node1gm7uj6vjx1622 rdf:first "pf_econet" .

_:node1gm7uj6vjx1780 sh:maxCount 1 .

_:node1gm7uj6vjx1622 rdf:rest _:node1gm7uj6vjx1623 .

_:node1gm7uj6vjx1780 sh:nodeKind sh:Literal .

_:node1gm7uj6vjx1623 rdf:first "pf_inet" .

_:node1gm7uj6vjx1780 sh:path observable:language .

observable:SoftwareFacet sh:property _:node1gm7uj6vjx1780 .

_:node1gm7uj6vjx1623 rdf:rest _:node1gm7uj6vjx1624 .

_:node1gm7uj6vjx1781 sh:datatype xsd:string .

_:node1gm7uj6vjx1624 rdf:first "pf_inet6" .

_:node1gm7uj6vjx1781 sh:maxCount 1 .

_:node1gm7uj6vjx1624 rdf:rest _:node1gm7uj6vjx1625 .

_:node1gm7uj6vjx1781 sh:nodeKind sh:Literal .

_:node1gm7uj6vjx1625 rdf:first "pf_ipx" .

_:node1gm7uj6vjx1781 sh:path observable:swid .

_:node1gm7uj6vjx1625 rdf:rest _:node1gm7uj6vjx1626 .

observable:SoftwareFacet sh:property _:node1gm7uj6vjx1781 .

_:node1gm7uj6vjx1626 rdf:first "pf_irda" .

_:node1gm7uj6vjx1782 sh:datatype xsd:string .

_:node1gm7uj6vjx1626 rdf:rest _:node1gm7uj6vjx1627 .

_:node1gm7uj6vjx1782 sh:maxCount 1 .

_:node1gm7uj6vjx1627 rdf:first "pf_key" .

_:node1gm7uj6vjx1782 sh:nodeKind sh:Literal .

_:node1gm7uj6vjx1627 rdf:rest _:node1gm7uj6vjx1628 .

_:node1gm7uj6vjx1782 sh:path observable:version .

_:node1gm7uj6vjx1628 rdf:first "pf_netbeui" .

observable:SoftwareFacet sh:property _:node1gm7uj6vjx1782 .

_:node1gm7uj6vjx1628 rdf:rest _:node1gm7uj6vjx1629 .

observable:SoftwareFacet sh:targetClass observable:SoftwareFacet .

_:node1gm7uj6vjx1629 rdf:first "pf_netlink" .

observable:StateChangeEffectFacet a owl:Class .

_:node1gm7uj6vjx1629 rdf:rest _:node1gm7uj6vjx1630 .

observable:StateChangeEffectFacet a sh:NodeShape .

_:node1gm7uj6vjx1630 rdf:first "pf_netrom" .

observable:StateChangeEffectFacet rdfs:subClassOf observable:DefinedEffectFacet .

_:node1gm7uj6vjx1630 rdf:rest _:node1gm7uj6vjx1631 .

observable:StateChangeEffectFacet rdfs:label "StateChangeEffectFacet"@en .

_:node1gm7uj6vjx1631 rdf:first "pf_packet" .

observable:StateChangeEffectFacet rdfs:comment "A state change effect facet is a grouping of characteristics unique to the effects of actions upon observable objects where a state of the observable object is changed."@en .

_:node1gm7uj6vjx1631 rdf:rest _:node1gm7uj6vjx1632 .

_:node1gm7uj6vjx1783 sh:class observable:ObservableObject .

_:node1gm7uj6vjx1632 rdf:first "pf_pppox" .

_:node1gm7uj6vjx1783 sh:maxCount 1 .

_:node1gm7uj6vjx1632 rdf:rest _:node1gm7uj6vjx1633 .

_:node1gm7uj6vjx1783 sh:nodeKind sh:IRI .

_:node1gm7uj6vjx1633 rdf:first "pf_rose" .

_:node1gm7uj6vjx1783 sh:path observable:newObject .

_:node1gm7uj6vjx1633 rdf:rest _:node1gm7uj6vjx1634 .

observable:StateChangeEffectFacet sh:property _:node1gm7uj6vjx1783 .

_:node1gm7uj6vjx1634 rdf:first "pf_route" .

_:node1gm7uj6vjx1784 sh:class observable:ObservableObject .

_:node1gm7uj6vjx1634 rdf:rest _:node1gm7uj6vjx1635 .

_:node1gm7uj6vjx1784 sh:maxCount 1 .

_:node1gm7uj6vjx1635 rdf:first "pf_security" .

_:node1gm7uj6vjx1784 sh:nodeKind sh:IRI .

_:node1gm7uj6vjx1635 rdf:rest _:node1gm7uj6vjx1636 .

_:node1gm7uj6vjx1784 sh:path observable:oldObject .

_:node1gm7uj6vjx1636 rdf:first "pf_sna" .

observable:StateChangeEffectFacet sh:property _:node1gm7uj6vjx1784 .

_:node1gm7uj6vjx1636 rdf:rest _:node1gm7uj6vjx1637 .

observable:StateChangeEffectFacet sh:targetClass observable:StateChangeEffectFacet .

_:node1gm7uj6vjx1637 rdf:first "pf_wanpipe" .

observable:StorageMedium a owl:Class .

_:node1gm7uj6vjx1637 rdf:rest _:node1gm7uj6vjx1638 .

observable:StorageMedium a sh:NodeShape .

_:node1gm7uj6vjx1638 rdf:first "pf_x25" .

observable:StorageMedium rdfs:subClassOf observable:Device .

_:node1gm7uj6vjx1638 rdf:rest rdf:nil .

observable:StorageMedium rdfs:label "StorageMedium"@en-us .

_:node1gm7uj6vjx1613 owl:oneOf _:node1gm7uj6vjx1614 .

observable:StorageMedium rdfs:comment "A storage medium is any digital storage device that applies electromagnetic or optical surfaces, or depends solely on electronic circuits as solid state storage, for storing digital data. Examples include HDD (PATA), SATA, SSD, Optical, Memory_Card, Tape, etc"@en-us .

observable:NetworkSocketProtocolFamily owl:equivalentClass _:node1gm7uj6vjx1613 .

observable:StorageMedium sh:targetClass observable:StorageMedium .

observable:NetworkSocketType a rdfs:Datatype .

observable:SymbolicLink a owl:Class .

_:node1gm7uj6vjx1639 a rdfs:Datatype .

observable:SymbolicLink a sh:NodeShape .

_:node1gm7uj6vjx1640 rdf:first "sock_dgram" .

observable:SymbolicLink rdfs:subClassOf observable:FileSystemObject .

_:node1gm7uj6vjx1640 rdf:rest _:node1gm7uj6vjx1641 .

observable:SymbolicLink rdfs:label "SymbolicLink"@en .

_:node1gm7uj6vjx1641 rdf:first "sock_raw" .

observable:SymbolicLink rdfs:comment "A symbolic link is a file that contains a reference to another file or directory in the form of an absolute or relative path and that affects pathname resolution. [based on https://en.wikipedia.org/wiki/Symbolic_link]"@en .

_:node1gm7uj6vjx1641 rdf:rest _:node1gm7uj6vjx1642 .

observable:SymbolicLink sh:targetClass observable:SymbolicLink .

_:node1gm7uj6vjx1642 rdf:first "sock_rdm" .

observable:SymbolicLinkFacet a owl:Class .

_:node1gm7uj6vjx1642 rdf:rest _:node1gm7uj6vjx1643 .

observable:SymbolicLinkFacet a sh:NodeShape .

_:node1gm7uj6vjx1643 rdf:first "sock_seqpacket" .

observable:SymbolicLinkFacet rdfs:subClassOf core:Facet .

_:node1gm7uj6vjx1643 rdf:rest _:node1gm7uj6vjx1644 .

observable:SymbolicLinkFacet rdfs:label "SymbolicLinkFacet"@en .

_:node1gm7uj6vjx1644 rdf:first "sock_stream" .

observable:SymbolicLinkFacet rdfs:comment "A symbolic link facet is a grouping of characteristics unique to a file that contains a reference to another file or directory in the form of an absolute or relative path and that affects pathname resolution. [based on https://en.wikipedia.org/wiki/Symbolic_link]"@en .

_:node1gm7uj6vjx1644 rdf:rest rdf:nil .

_:node1gm7uj6vjx1785 sh:class observable:ObservableObject .

_:node1gm7uj6vjx1639 owl:oneOf _:node1gm7uj6vjx1640 .

_:node1gm7uj6vjx1785 sh:maxCount 1 .

observable:NetworkSocketType owl:equivalentClass _:node1gm7uj6vjx1639 .

_:node1gm7uj6vjx1785 sh:nodeKind sh:IRI .

observable:NetworkSubnet a owl:Class .

_:node1gm7uj6vjx1785 sh:path observable:targetFile .

observable:NetworkSubnet a sh:NodeShape .

observable:SymbolicLinkFacet sh:property _:node1gm7uj6vjx1785 .

observable:NetworkSubnet rdfs:subClassOf observable:ObservableObject .

observable:SymbolicLinkFacet sh:targetClass observable:SymbolicLinkFacet .

observable:NetworkSubnet rdfs:label "NetworkSubnet"@en .

observable:TCPConnection a owl:Class .

observable:NetworkSubnet rdfs:comment "A network subnet is a logical subdivision of an IP network. [based on https://en.wikipedia.org/wiki/Subnetwork]"@en .

observable:TCPConnection a sh:NodeShape .

observable:NetworkSubnet sh:targetClass observable:NetworkSubnet .

observable:TCPConnection rdfs:subClassOf observable:NetworkConnection .

observable:Note a owl:Class .

observable:TCPConnection rdfs:label "TCPConnection"@en .

observable:Note a sh:NodeShape .

observable:TCPConnection rdfs:comment "A TCP connection is a network connection that is conformant to the Transfer "@en .

observable:Note rdfs:subClassOf observable:ObservableObject .

observable:TCPConnection sh:targetClass observable:TCPConnection .

observable:Note rdfs:label "Note"@en .

observable:TCPConnectionFacet a owl:Class .

observable:Note rdfs:comment "A note is a brief textual record."@en .

observable:TCPConnectionFacet a sh:NodeShape .

observable:Note sh:targetClass observable:Note .

observable:TCPConnectionFacet rdfs:subClassOf core:Facet .

observable:NoteFacet a owl:Class .

observable:TCPConnectionFacet rdfs:label "TCPConnectionFacet"@en .

observable:NoteFacet a sh:NodeShape .

observable:TCPConnectionFacet rdfs:comment "A TCP connection facet is a grouping of characteristics unique to portions of a network connection that are conformant to the Transmission Control Protocl (TCP) standard."@en .

observable:NoteFacet rdfs:subClassOf core:Facet .

_:node1gm7uj6vjx1786 sh:datatype xsd:hexBinary .

observable:NoteFacet rdfs:label "NoteFacet"@en .

_:node1gm7uj6vjx1786 sh:nodeKind sh:Literal .

observable:NoteFacet rdfs:comment "A note facet is a grouping of characteristics unique to a brief textual record."@en .

_:node1gm7uj6vjx1786 sh:path observable:destinationFlags .

_:node1gm7uj6vjx1645 sh:class observable:ObservableObject .

observable:TCPConnectionFacet sh:property _:node1gm7uj6vjx1786 .

_:node1gm7uj6vjx1645 sh:maxCount 1 .

_:node1gm7uj6vjx1787 sh:datatype xsd:hexBinary .

_:node1gm7uj6vjx1645 sh:nodeKind sh:IRI .

_:node1gm7uj6vjx1787 sh:nodeKind sh:Literal .

_:node1gm7uj6vjx1645 sh:path observable:application .

_:node1gm7uj6vjx1787 sh:path observable:sourceFlags .

observable:NoteFacet sh:property _:node1gm7uj6vjx1645 .

observable:TCPConnectionFacet sh:property _:node1gm7uj6vjx1787 .

_:node1gm7uj6vjx1646 sh:datatype xsd:dateTime .

observable:TCPConnectionFacet sh:targetClass observable:TCPConnectionFacet .

_:node1gm7uj6vjx1646 sh:maxCount 1 .

observable:TableField a owl:Class .

_:node1gm7uj6vjx1646 sh:nodeKind sh:Literal .

observable:TableField a sh:NodeShape .

_:node1gm7uj6vjx1646 sh:path observable:modifiedTime .

observable:TableField rdfs:subClassOf observable:ObservableObject .

observable:NoteFacet sh:property _:node1gm7uj6vjx1646 .

observable:TableField rdfs:label "TableField"@en .

_:node1gm7uj6vjx1647 sh:datatype xsd:dateTime .

observable:TableField rdfs:comment "A database table field and its associated value contained within a relational database."@en .

_:node1gm7uj6vjx1647 sh:maxCount 1 .

observable:TableField sh:targetClass observable:TableField .

_:node1gm7uj6vjx1647 sh:nodeKind sh:Literal .

observable:TableFieldFacet a owl:Class .

_:node1gm7uj6vjx1647 sh:path observable:observableCreatedTime .

observable:TableFieldFacet a sh:NodeShape .

observable:NoteFacet sh:property _:node1gm7uj6vjx1647 .

observable:TableFieldFacet rdfs:subClassOf core:Facet .

_:node1gm7uj6vjx1648 sh:datatype xsd:string .

observable:TableFieldFacet rdfs:label "TableFieldFacet"@en .

_:node1gm7uj6vjx1648 sh:maxCount 1 .

observable:TableFieldFacet rdfs:comment "A database record facet contains properties associated with a specific table record value from a database."@en .

_:node1gm7uj6vjx1648 sh:nodeKind sh:Literal .

_:node1gm7uj6vjx1788 sh:datatype xsd:boolean .

_:node1gm7uj6vjx1648 sh:path observable:text .

_:node1gm7uj6vjx1788 sh:maxCount 1 .

observable:NoteFacet sh:property _:node1gm7uj6vjx1648 .

_:node1gm7uj6vjx1788 sh:nodeKind sh:Literal .

observable:NoteFacet sh:targetClass observable:NoteFacet .

_:node1gm7uj6vjx1788 sh:path observable:recordFieldIsNull .

observable:Observable a owl:Class .

observable:TableFieldFacet sh:property _:node1gm7uj6vjx1788 .

observable:Observable a sh:NodeShape .

_:node1gm7uj6vjx1789 sh:datatype xsd:string .

observable:Observable rdfs:subClassOf core:UcoObject .

_:node1gm7uj6vjx1789 sh:maxCount 1 .

observable:Observable rdfs:label "Observable"@en .

_:node1gm7uj6vjx1789 sh:nodeKind sh:Literal .

observable:Observable rdfs:comment "An observable is a characterizable item or action within the digital domain."@en .

_:node1gm7uj6vjx1789 sh:path observable:recordFieldName .

observable:Observable sh:targetClass observable:Observable .

observable:TableFieldFacet sh:property _:node1gm7uj6vjx1789 .

observable:ObservableAction a owl:Class .

_:node1gm7uj6vjx1790 sh:datatype xsd:string .

observable:ObservableAction a sh:NodeShape .

_:node1gm7uj6vjx1790 sh:maxCount 1 .

observable:ObservableAction rdfs:subClassOf action:Action .

_:node1gm7uj6vjx1790 sh:nodeKind sh:Literal .

observable:ObservableAction rdfs:subClassOf observable:Observable .

_:node1gm7uj6vjx1790 sh:path observable:tableName .

observable:ObservableAction rdfs:label "ObservableAction"@en .

observable:TableFieldFacet sh:property _:node1gm7uj6vjx1790 .

observable:ObservableAction rdfs:comment "An observable action is a grouping of characteristics unique to something that may be done or performed within the digital domain."@en .

_:node1gm7uj6vjx1791 sh:datatype xsd:string .

observable:ObservableAction sh:targetClass observable:ObservableAction .

_:node1gm7uj6vjx1791 sh:maxCount 1 .

observable:ObservableObject a owl:Class .

_:node1gm7uj6vjx1791 sh:nodeKind sh:Literal .

observable:ObservableObject a sh:NodeShape .

_:node1gm7uj6vjx1791 sh:path observable:tableSchema .

observable:ObservableObject rdfs:subClassOf core:Item .

observable:TableFieldFacet sh:property _:node1gm7uj6vjx1791 .

observable:ObservableObject rdfs:subClassOf observable:Observable .

_:node1gm7uj6vjx1792 sh:maxCount 1 .

observable:ObservableObject rdfs:label "ObservableObject"@en .

_:node1gm7uj6vjx1792 sh:nodeKind sh:Literal .

observable:ObservableObject rdfs:comment "An observable object is a grouping of characteristics unique to a distinct article or unit within the digital domain."@en .

_:node1gm7uj6vjx1794 sh:datatype xsd:base64Binary .

_:node1gm7uj6vjx1649 sh:datatype xsd:boolean .

_:node1gm7uj6vjx1793 rdf:first _:node1gm7uj6vjx1794 .

_:node1gm7uj6vjx1649 sh:maxCount 1 .

_:node1gm7uj6vjx1793 rdf:rest _:node1gm7uj6vjx1795 .

_:node1gm7uj6vjx1649 sh:nodeKind sh:Literal .

_:node1gm7uj6vjx1796 sh:datatype xsd:decimal .

_:node1gm7uj6vjx1649 sh:path observable:hasChanged .

_:node1gm7uj6vjx1795 rdf:first _:node1gm7uj6vjx1796 .

observable:ObservableObject sh:property _:node1gm7uj6vjx1649 .

_:node1gm7uj6vjx1795 rdf:rest _:node1gm7uj6vjx1797 .

_:node1gm7uj6vjx1650 sh:datatype xsd:string .

_:node1gm7uj6vjx1798 sh:datatype xsd:integer .

_:node1gm7uj6vjx1650 sh:maxCount 1 .

_:node1gm7uj6vjx1797 rdf:first _:node1gm7uj6vjx1798 .

_:node1gm7uj6vjx1650 sh:nodeKind sh:Literal .

_:node1gm7uj6vjx1797 rdf:rest _:node1gm7uj6vjx1799 .

_:node1gm7uj6vjx1650 sh:path observable:state .

_:node1gm7uj6vjx1800 sh:datatype xsd:string .

observable:ObservableObject sh:property _:node1gm7uj6vjx1650 .

_:node1gm7uj6vjx1799 rdf:first _:node1gm7uj6vjx1800 .

observable:ObservableObject sh:targetClass observable:ObservableObject .

_:node1gm7uj6vjx1799 rdf:rest rdf:nil .

observable:ObservablePattern a owl:Class .

_:node1gm7uj6vjx1792 sh:or _:node1gm7uj6vjx1793 .

observable:ObservablePattern a sh:NodeShape .

_:node1gm7uj6vjx1792 sh:path observable:recordFieldValue .

observable:ObservablePattern rdfs:subClassOf observable:Observable .

observable:TableFieldFacet sh:property _:node1gm7uj6vjx1792 .

observable:ObservablePattern rdfs:label "ObservablePattern"@en .

_:node1gm7uj6vjx1801 sh:maxCount 1 .

observable:ObservablePattern rdfs:comment "An observable pattern is a grouping of characteristics unique to a logical pattern composed of observable object and observable action properties."@en .

_:node1gm7uj6vjx1801 sh:nodeKind sh:Literal .

observable:ObservablePattern sh:targetClass observable:ObservablePattern .

_:node1gm7uj6vjx1803 sh:datatype xsd:integer .

observable:ObservableRelationship a owl:Class .

_:node1gm7uj6vjx1802 rdf:first _:node1gm7uj6vjx1803 .

observable:ObservableRelationship a sh:NodeShape .

_:node1gm7uj6vjx1802 rdf:rest _:node1gm7uj6vjx1804 .

_:node1gm7uj6vjx1805 sh:datatype xsd:string .

observable:ObservableRelationship rdfs:subClassOf core:Relationship .

_:node1gm7uj6vjx1804 rdf:first _:node1gm7uj6vjx1805 .

observable:ObservableRelationship rdfs:subClassOf observable:Observable .

_:node1gm7uj6vjx1804 rdf:rest rdf:nil .

observable:ObservableRelationship rdfs:label "ObservableRelationship"@en .

_:node1gm7uj6vjx1801 sh:or _:node1gm7uj6vjx1802 .

observable:ObservableRelationship rdfs:comment "An observable relationship is a grouping of characteristics unique to an assertion of an association between two observable objects."@en .

_:node1gm7uj6vjx1801 sh:path observable:recordRowID .

observable:ObservableRelationship sh:targetClass observable:ObservableRelationship .

observable:TableFieldFacet sh:property _:node1gm7uj6vjx1801 .

observable:Observation a owl:Class .

observable:TableFieldFacet sh:targetClass observable:TableFieldFacet .

observable:Observation a sh:NodeShape .

_:node1gm7uj6vjx1807 a sh:NodeShape .

observable:Observation rdfs:subClassOf action:Action .

_:node1gm7uj6vjx1808 sh:hasValue false ;
	sh:path observable:recordFieldIsNull .

_:node1gm7uj6vjx1807 sh:property _:node1gm7uj6vjx1808 .

observable:Observation rdfs:label "Observation"@en .

_:node1gm7uj6vjx1806 rdf:first _:node1gm7uj6vjx1807 .

observable:Observation rdfs:comment "An observation is a temporal perception of an observable."@en .

_:node1gm7uj6vjx1806 rdf:rest _:node1gm7uj6vjx1809 .

_:node1gm7uj6vjx1651 sh:datatype xsd:string .

_:node1gm7uj6vjx1810 a sh:NodeShape .

_:node1gm7uj6vjx1651 sh:hasValue "observe" .

_:node1gm7uj6vjx1811 sh:hasValue true .

_:node1gm7uj6vjx1651 sh:maxCount 1 .

_:node1gm7uj6vjx1811 sh:path observable:recordFieldIsNull .

_:node1gm7uj6vjx1651 sh:minCount 1 .

_:node1gm7uj6vjx1810 sh:property _:node1gm7uj6vjx1811 .

_:node1gm7uj6vjx1651 sh:nodeKind sh:Literal .

_:node1gm7uj6vjx1812 sh:maxCount 0 .

_:node1gm7uj6vjx1651 sh:path core:name .

_:node1gm7uj6vjx1812 sh:path observable:recordFieldValue .

observable:Observation sh:property _:node1gm7uj6vjx1651 .

_:node1gm7uj6vjx1810 sh:property _:node1gm7uj6vjx1812 .

observable:Observation sh:targetClass observable:Observation .

_:node1gm7uj6vjx1809 rdf:first _:node1gm7uj6vjx1810 .

observable:OnlineService a owl:Class .

_:node1gm7uj6vjx1809 rdf:rest _:node1gm7uj6vjx1813 .

observable:OnlineService a sh:NodeShape .

_:node1gm7uj6vjx1814 a sh:NodeShape .

observable:OnlineService rdfs:subClassOf observable:ObservableObject .

_:node1gm7uj6vjx1815 sh:maxCount 0 .

observable:OnlineService rdfs:label "OnlineService"@en .

_:node1gm7uj6vjx1815 sh:path observable:recordFieldIsNull .

observable:OnlineService rdfs:comment "An online service is a particular provision mechanism of information access, distribution or manipulation over the Internet."@en .

_:node1gm7uj6vjx1814 sh:property _:node1gm7uj6vjx1815 .

observable:OnlineService sh:targetClass observable:OnlineService .

_:node1gm7uj6vjx1813 rdf:first _:node1gm7uj6vjx1814 .

observable:OnlineServiceFacet a owl:Class .

_:node1gm7uj6vjx1813 rdf:rest rdf:nil .

observable:OnlineServiceFacet a sh:NodeShape .

observable:TableFieldFacet sh:xone _:node1gm7uj6vjx1806 .

observable:OnlineServiceFacet rdfs:subClassOf core:Facet .

observable:Tablet a owl:Class .

observable:OnlineServiceFacet rdfs:label "OnlineServiceFacet"@en-us .

observable:Tablet a sh:NodeShape .

observable:OnlineServiceFacet rdfs:comment "An online service facet is a grouping of characteristics unique to a particular provision mechanism of information access, distribution or manipulation over the Internet."@en-us .

observable:Tablet rdfs:subClassOf observable:Computer .

_:node1gm7uj6vjx1652 sh:class location:Location .

observable:Tablet rdfs:subClassOf observable:MobileDevice .

_:node1gm7uj6vjx1652 sh:minCount 0 .

observable:Tablet rdfs:subClassOf observable:SmartDevice .

_:node1gm7uj6vjx1652 sh:nodeKind sh:IRI .

observable:Tablet rdfs:label "Tablet"@en-us .

_:node1gm7uj6vjx1652 sh:path observable:location .

observable:Tablet rdfs:comment "A tablet is a mobile computer that is primarily operated by touching the screen. (Devices categorized by their manufacturer as a Tablet)"@en-us .

observable:OnlineServiceFacet sh:property _:node1gm7uj6vjx1652 .

observable:Tablet sh:targetClass observable:Tablet .

_:node1gm7uj6vjx1653 sh:class observable:ObservableObject .

observable:TaskActionType a owl:Class .

_:node1gm7uj6vjx1653 sh:minCount 0 .

observable:TaskActionType a sh:NodeShape .

_:node1gm7uj6vjx1653 sh:nodeKind sh:IRI .

observable:TaskActionType rdfs:subClassOf core:UcoInherentCharacterizationThing .

_:node1gm7uj6vjx1653 sh:path observable:inetLocation .

observable:TaskActionType rdfs:label "TaskActionType"@en .

observable:OnlineServiceFacet sh:property _:node1gm7uj6vjx1653 .

observable:TaskActionType rdfs:comment "A task action type is a grouping of characteristics for a scheduled action to be completed."@en .

_:node1gm7uj6vjx1654 sh:datatype xsd:string .

_:node1gm7uj6vjx1816 sh:class observable:IComHandlerActionType .

_:node1gm7uj6vjx1654 sh:maxCount 1 .

_:node1gm7uj6vjx1816 sh:maxCount 1 .

_:node1gm7uj6vjx1654 sh:nodeKind sh:Literal .

_:node1gm7uj6vjx1816 sh:nodeKind sh:IRI .

_:node1gm7uj6vjx1654 sh:path core:name .

_:node1gm7uj6vjx1816 sh:path observable:iComHandlerAction .

observable:OnlineServiceFacet sh:property _:node1gm7uj6vjx1654 .

observable:TaskActionType sh:property _:node1gm7uj6vjx1816 .

observable:OnlineServiceFacet sh:targetClass observable:OnlineServiceFacet .

_:node1gm7uj6vjx1817 sh:class observable:IExecActionType .

observable:OperatingSystem a owl:Class .

_:node1gm7uj6vjx1817 sh:maxCount 1 .

observable:OperatingSystem a sh:NodeShape .

_:node1gm7uj6vjx1817 sh:nodeKind sh:IRI .

observable:OperatingSystem rdfs:subClassOf observable:ObservableObject .

_:node1gm7uj6vjx1817 sh:path observable:iExecAction .

observable:OperatingSystem rdfs:label "OperatingSystem"@en .

observable:TaskActionType sh:property _:node1gm7uj6vjx1817 .

observable:OperatingSystem rdfs:comment "An operating system is the software that manages computer hardware, software resources, and provides common services for computer programs. [based on https://en.wikipedia.org/wiki/Operating_system]"@en .

_:node1gm7uj6vjx1818 sh:class observable:IShowMessageActionType .

observable:OperatingSystem sh:targetClass observable:OperatingSystem .

_:node1gm7uj6vjx1818 sh:maxCount 1 .

observable:OperatingSystemFacet a owl:Class .

_:node1gm7uj6vjx1818 sh:nodeKind sh:IRI .

observable:OperatingSystemFacet a sh:NodeShape .

_:node1gm7uj6vjx1818 sh:path observable:iShowMessageAction .

observable:OperatingSystemFacet rdfs:subClassOf core:Facet .

observable:TaskActionType sh:property _:node1gm7uj6vjx1818 .

observable:OperatingSystemFacet rdfs:label "OperatingSystemFacet"@en .

_:node1gm7uj6vjx1819 sh:class observable:ObservableObject .

observable:OperatingSystemFacet rdfs:comment "An operating system facet is a grouping of characteristics unique to the software that manages computer hardware, software resources, and provides common services for computer programs. [based on https://en.wikipedia.org/wiki/Operating_system]"@en .

_:node1gm7uj6vjx1819 sh:maxCount 1 .

_:node1gm7uj6vjx1655 sh:class identity:Identity .

_:node1gm7uj6vjx1819 sh:nodeKind sh:IRI .

_:node1gm7uj6vjx1655 sh:maxCount 1 .

_:node1gm7uj6vjx1819 sh:path observable:iEmailAction .

_:node1gm7uj6vjx1655 sh:nodeKind sh:IRI .

observable:TaskActionType sh:property _:node1gm7uj6vjx1819 .

_:node1gm7uj6vjx1655 sh:path observable:manufacturer .

_:node1gm7uj6vjx1820 sh:datatype xsd:string .

observable:OperatingSystemFacet sh:property _:node1gm7uj6vjx1655 .

_:node1gm7uj6vjx1820 sh:maxCount 1 .

_:node1gm7uj6vjx1656 sh:class types:Dictionary .

_:node1gm7uj6vjx1820 sh:nodeKind sh:Literal .

_:node1gm7uj6vjx1656 sh:maxCount 1 .

_:node1gm7uj6vjx1820 sh:path observable:actionID .

_:node1gm7uj6vjx1656 sh:nodeKind sh:IRI .

observable:TaskActionType sh:property _:node1gm7uj6vjx1820 .

_:node1gm7uj6vjx1656 sh:path observable:environmentVariables .

_:node1gm7uj6vjx1821 sh:datatype vocabulary:TaskActionTypeVocab .

observable:OperatingSystemFacet sh:property _:node1gm7uj6vjx1656 .

_:node1gm7uj6vjx1821 sh:message "Value is outside the default vocabulary TaskActionTypeVocab." .

_:node1gm7uj6vjx1657 sh:datatype xsd:boolean .

_:node1gm7uj6vjx1821 sh:path observable:actionType .

_:node1gm7uj6vjx1657 sh:maxCount 1 .

_:node1gm7uj6vjx1821 sh:severity sh:Info .

_:node1gm7uj6vjx1657 sh:nodeKind sh:Literal .

observable:TaskActionType sh:property _:node1gm7uj6vjx1821 .

_:node1gm7uj6vjx1657 sh:path observable:isLimitAdTrackingEnabled .

_:node1gm7uj6vjx1822 sh:maxCount 1 .

observable:OperatingSystemFacet sh:property _:node1gm7uj6vjx1657 .

_:node1gm7uj6vjx1822 sh:nodeKind sh:Literal .

_:node1gm7uj6vjx1658 sh:datatype xsd:dateTime .

_:node1gm7uj6vjx1824 sh:datatype vocabulary:TaskActionTypeVocab .

_:node1gm7uj6vjx1658 sh:maxCount 1 .

_:node1gm7uj6vjx1823 rdf:first _:node1gm7uj6vjx1824 .

_:node1gm7uj6vjx1658 sh:nodeKind sh:Literal .

_:node1gm7uj6vjx1823 rdf:rest _:node1gm7uj6vjx1825 .

_:node1gm7uj6vjx1658 sh:path observable:installDate .

_:node1gm7uj6vjx1826 sh:datatype xsd:string .

_:node1gm7uj6vjx1825 rdf:first _:node1gm7uj6vjx1826 .

observable:OperatingSystemFacet sh:property _:node1gm7uj6vjx1658 .

_:node1gm7uj6vjx1825 rdf:rest rdf:nil .

_:node1gm7uj6vjx1659 sh:datatype xsd:string .

_:node1gm7uj6vjx1822 sh:or _:node1gm7uj6vjx1823 .

_:node1gm7uj6vjx1659 sh:maxCount 1 .

_:node1gm7uj6vjx1822 sh:path observable:actionType .

_:node1gm7uj6vjx1659 sh:nodeKind sh:Literal .

observable:TaskActionType sh:property _:node1gm7uj6vjx1822 .

_:node1gm7uj6vjx1659 sh:path observable:bitness .

_:node1gm7uj6vjx1827 sh:message "Value is not member of the vocabulary TaskActionTypeVocab." .

observable:OperatingSystemFacet sh:property _:node1gm7uj6vjx1659 .

_:node1gm7uj6vjx1829 sh:datatype vocabulary:TaskActionTypeVocab .

_:node1gm7uj6vjx1660 sh:datatype xsd:string .

_:node1gm7uj6vjx1830 rdf:first "TASK_ACTION_COM_HANDLER"^^vocabulary:TaskActionTypeVocab .

_:node1gm7uj6vjx1660 sh:maxCount 1 .

_:node1gm7uj6vjx1830 rdf:rest _:node1gm7uj6vjx1831 .

_:node1gm7uj6vjx1660 sh:nodeKind sh:Literal .

_:node1gm7uj6vjx1831 rdf:first "TASK_ACTION_EXEC"^^vocabulary:TaskActionTypeVocab .

_:node1gm7uj6vjx1660 sh:path observable:version .

_:node1gm7uj6vjx1831 rdf:rest _:node1gm7uj6vjx1832 .

observable:OperatingSystemFacet sh:property _:node1gm7uj6vjx1660 .

_:node1gm7uj6vjx1832 rdf:first "TASK_ACTION_SEND_EMAIL"^^vocabulary:TaskActionTypeVocab .

_:node1gm7uj6vjx1661 sh:datatype xsd:string .

_:node1gm7uj6vjx1832 rdf:rest _:node1gm7uj6vjx1833 .

_:node1gm7uj6vjx1661 sh:nodeKind sh:Literal .

_:node1gm7uj6vjx1833 rdf:first "TASK_ACTION_SHOW_MESSAGE"^^vocabulary:TaskActionTypeVocab .

_:node1gm7uj6vjx1661 sh:path observable:advertisingID .

_:node1gm7uj6vjx1833 rdf:rest rdf:nil .

observable:OperatingSystemFacet sh:property _:node1gm7uj6vjx1661 .

_:node1gm7uj6vjx1829 sh:in _:node1gm7uj6vjx1830 .

observable:OperatingSystemFacet sh:targetClass observable:OperatingSystemFacet .

_:node1gm7uj6vjx1828 rdf:first _:node1gm7uj6vjx1829 .

observable:PDFFile a owl:Class .

_:node1gm7uj6vjx1828 rdf:rest _:node1gm7uj6vjx1834 .

observable:PDFFile a sh:NodeShape .

_:node1gm7uj6vjx1835 sh:datatype xsd:string .

observable:PDFFile rdfs:subClassOf observable:File .

_:node1gm7uj6vjx1834 rdf:first _:node1gm7uj6vjx1835 .

observable:PDFFile rdfs:label "PDFFile"@en .

_:node1gm7uj6vjx1834 rdf:rest rdf:nil .

observable:PDFFile rdfs:comment "A PDF file is a Portable Document Format (PDF) file."@en .

_:node1gm7uj6vjx1827 sh:or _:node1gm7uj6vjx1828 .

observable:PDFFile sh:targetClass observable:PDFFile .

_:node1gm7uj6vjx1827 sh:path observable:actionType .

observable:PDFFileFacet a owl:Class .

observable:TaskActionType sh:property _:node1gm7uj6vjx1827 .

observable:PDFFileFacet a sh:NodeShape .

observable:TaskActionType sh:targetClass observable:TaskActionType .

observable:PDFFileFacet rdfs:subClassOf core:Facet .

observable:TriggerType a owl:Class .

observable:PDFFileFacet rdfs:label "PDFFileFacet"@en .

observable:TriggerType a sh:NodeShape .

observable:PDFFileFacet rdfs:comment "A PDF file facet is a grouping of characteristics unique to a PDF (Portable Document Format) file."@en .

observable:TriggerType rdfs:subClassOf core:UcoInherentCharacterizationThing .

_:node1gm7uj6vjx1662 sh:class types:ControlledDictionary .

observable:TriggerType rdfs:label "TriggerType"@en .

_:node1gm7uj6vjx1662 sh:maxCount 1 .

observable:TriggerType rdfs:comment "A trigger type is a grouping of characterizes unique to a set of criteria that, when met, starts the execution of a task within a Windows operating system. [based on https://docs.microsoft.com/en-us/windows/win32/taskschd/task-triggers]"@en .

_:node1gm7uj6vjx1662 sh:nodeKind sh:IRI .

_:node1gm7uj6vjx1836 sh:datatype xsd:boolean .

_:node1gm7uj6vjx1662 sh:path observable:documentInformationDictionary .

_:node1gm7uj6vjx1836 sh:maxCount 1 .

observable:PDFFileFacet sh:property _:node1gm7uj6vjx1662 .

_:node1gm7uj6vjx1836 sh:nodeKind sh:Literal .

_:node1gm7uj6vjx1663 sh:datatype xsd:boolean .

_:node1gm7uj6vjx1836 sh:path observable:isEnabled .

_:node1gm7uj6vjx1663 sh:maxCount 1 .

observable:TriggerType sh:property _:node1gm7uj6vjx1836 .

_:node1gm7uj6vjx1663 sh:nodeKind sh:Literal .

_:node1gm7uj6vjx1837 sh:datatype xsd:dateTime .

_:node1gm7uj6vjx1663 sh:path observable:isOptimized .

_:node1gm7uj6vjx1837 sh:maxCount 1 .

observable:PDFFileFacet sh:property _:node1gm7uj6vjx1663 .

_:node1gm7uj6vjx1837 sh:nodeKind sh:Literal .

_:node1gm7uj6vjx1664 sh:datatype xsd:dateTime .

_:node1gm7uj6vjx1837 sh:path observable:triggerBeginTime .

_:node1gm7uj6vjx1664 sh:maxCount 1 .

observable:TriggerType sh:property _:node1gm7uj6vjx1837 .

_:node1gm7uj6vjx1664 sh:nodeKind sh:Literal .

_:node1gm7uj6vjx1838 sh:datatype xsd:dateTime .

_:node1gm7uj6vjx1664 sh:path observable:pdfCreationDate .

_:node1gm7uj6vjx1838 sh:maxCount 1 .

observable:PDFFileFacet sh:property _:node1gm7uj6vjx1664 .

_:node1gm7uj6vjx1838 sh:nodeKind sh:Literal .

_:node1gm7uj6vjx1665 sh:datatype xsd:dateTime .

_:node1gm7uj6vjx1838 sh:path observable:triggerEndTime .

_:node1gm7uj6vjx1665 sh:maxCount 1 .

observable:TriggerType sh:property _:node1gm7uj6vjx1838 .

_:node1gm7uj6vjx1665 sh:nodeKind sh:Literal .

_:node1gm7uj6vjx1839 sh:datatype xsd:string .

_:node1gm7uj6vjx1665 sh:path observable:pdfModDate .

_:node1gm7uj6vjx1839 sh:maxCount 1 .

observable:PDFFileFacet sh:property _:node1gm7uj6vjx1665 .

_:node1gm7uj6vjx1839 sh:nodeKind sh:Literal .

_:node1gm7uj6vjx1666 sh:datatype xsd:string .

_:node1gm7uj6vjx1839 sh:path observable:triggerDelay .

_:node1gm7uj6vjx1666 sh:maxCount 1 .

observable:TriggerType sh:property _:node1gm7uj6vjx1839 .

_:node1gm7uj6vjx1666 sh:nodeKind sh:Literal .

_:node1gm7uj6vjx1840 sh:datatype xsd:string .

_:node1gm7uj6vjx1666 sh:path observable:pdfId1 .

_:node1gm7uj6vjx1840 sh:maxCount 1 .

observable:PDFFileFacet sh:property _:node1gm7uj6vjx1666 .

_:node1gm7uj6vjx1840 sh:nodeKind sh:Literal .

_:node1gm7uj6vjx1667 sh:datatype xsd:string .

_:node1gm7uj6vjx1840 sh:path observable:triggerMaxRunTime .

_:node1gm7uj6vjx1667 sh:maxCount 1 .

observable:TriggerType sh:property _:node1gm7uj6vjx1840 .

_:node1gm7uj6vjx1667 sh:nodeKind sh:Literal .

_:node1gm7uj6vjx1841 sh:datatype xsd:string .

_:node1gm7uj6vjx1667 sh:path observable:version .

_:node1gm7uj6vjx1841 sh:maxCount 1 .

observable:PDFFileFacet sh:property _:node1gm7uj6vjx1667 .

_:node1gm7uj6vjx1841 sh:nodeKind sh:Literal .

_:node1gm7uj6vjx1668 sh:datatype xsd:string .

_:node1gm7uj6vjx1841 sh:path observable:triggerSessionChangeType .

_:node1gm7uj6vjx1668 sh:nodeKind sh:Literal .

observable:TriggerType sh:property _:node1gm7uj6vjx1841 .

_:node1gm7uj6vjx1668 sh:path observable:pdfId0 .

_:node1gm7uj6vjx1842 sh:datatype vocabulary:TriggerFrequencyVocab .

observable:PDFFileFacet sh:property _:node1gm7uj6vjx1668 .

_:node1gm7uj6vjx1842 sh:message "Value is outside the default vocabulary TriggerFrequencyVocab." .

observable:PDFFileFacet sh:targetClass observable:PDFFileFacet .

_:node1gm7uj6vjx1842 sh:path observable:triggerFrequency .

observable:PIN a owl:DatatypeProperty .

_:node1gm7uj6vjx1842 sh:severity sh:Info .

observable:PIN rdfs:label "PIN"@en .

observable:TriggerType sh:property _:node1gm7uj6vjx1842 .

observable:PIN rdfs:comment "Personal Identification Number (PIN)."@en .

_:node1gm7uj6vjx1843 sh:datatype vocabulary:TriggerTypeVocab .

observable:PIN rdfs:range xsd:string .

_:node1gm7uj6vjx1843 sh:message "Value is outside the default vocabulary TriggerTypeVocab." .

observable:PUK a owl:DatatypeProperty .

_:node1gm7uj6vjx1843 sh:path observable:triggerType .

observable:PUK rdfs:label "PUK"@en .

_:node1gm7uj6vjx1843 sh:severity sh:Info .

observable:PUK rdfs:comment "Personal Unlocking Key (PUK) to unlock the SIM card."@en .

observable:TriggerType sh:property _:node1gm7uj6vjx1843 .

observable:PUK rdfs:range xsd:string .

_:node1gm7uj6vjx1844 sh:maxCount 1 .

observable:PathRelationFacet a owl:Class .

_:node1gm7uj6vjx1844 sh:nodeKind sh:Literal .

observable:PathRelationFacet a sh:NodeShape .

_:node1gm7uj6vjx1846 sh:datatype vocabulary:TriggerFrequencyVocab .

observable:PathRelationFacet rdfs:subClassOf core:Facet .

_:node1gm7uj6vjx1845 rdf:first _:node1gm7uj6vjx1846 .

observable:PathRelationFacet rdfs:label "PathRelationFacet"@en .

_:node1gm7uj6vjx1845 rdf:rest _:node1gm7uj6vjx1847 .

observable:PathRelationFacet rdfs:comment "A path relation facet is a grouping of characteristics unique to the location of one object within another containing object."@en .

_:node1gm7uj6vjx1848 sh:datatype xsd:string .

_:node1gm7uj6vjx1669 sh:datatype xsd:string .

_:node1gm7uj6vjx1847 rdf:first _:node1gm7uj6vjx1848 .

_:node1gm7uj6vjx1669 sh:nodeKind sh:Literal .

_:node1gm7uj6vjx1847 rdf:rest rdf:nil .

_:node1gm7uj6vjx1669 sh:path observable:path .

_:node1gm7uj6vjx1844 sh:or _:node1gm7uj6vjx1845 .

observable:PathRelationFacet sh:property _:node1gm7uj6vjx1669 .

_:node1gm7uj6vjx1844 sh:path observable:triggerFrequency .

observable:PathRelationFacet sh:targetClass observable:PathRelationFacet .

observable:TriggerType sh:property _:node1gm7uj6vjx1844 .

observable:PaymentCard a owl:Class .

_:node1gm7uj6vjx1849 sh:maxCount 1 .

observable:PaymentCard a sh:NodeShape .

_:node1gm7uj6vjx1849 sh:nodeKind sh:Literal .

observable:PaymentCard rdfs:subClassOf observable:ObservableObject .

_:node1gm7uj6vjx1851 sh:datatype vocabulary:TriggerTypeVocab .

observable:PaymentCard rdfs:label "PaymentCard"@en .

_:node1gm7uj6vjx1850 rdf:first _:node1gm7uj6vjx1851 .

observable:PaymentCard rdfs:comment "A payment card is a physical token that is part of a payment system issued by financial institutions, such as a bank, to a customer that enables its owner (the cardholder) to access the funds in the customer's designated bank accounts, or through a credit account and make payments by electronic funds transfer and access automated teller machines (ATMs). [based on https://en.wikipedia.org/wiki/Payment_card]"@en .

_:node1gm7uj6vjx1850 rdf:rest _:node1gm7uj6vjx1852 .

observable:PaymentCard sh:targetClass observable:PaymentCard .

_:node1gm7uj6vjx1853 sh:datatype xsd:string .

observable:PhoneAccount a owl:Class .

_:node1gm7uj6vjx1852 rdf:first _:node1gm7uj6vjx1853 .

observable:PhoneAccount a sh:NodeShape .

_:node1gm7uj6vjx1852 rdf:rest rdf:nil .

observable:PhoneAccount rdfs:subClassOf observable:DigitalAccount .

_:node1gm7uj6vjx1849 sh:or _:node1gm7uj6vjx1850 .

observable:PhoneAccount rdfs:label "PhoneAccount"@en .

_:node1gm7uj6vjx1849 sh:path observable:triggerType .

observable:PhoneAccount rdfs:comment "A phone account is an arrangement with an entity to enable and control the provision of a telephony capability or service."@en .

observable:TriggerType sh:property _:node1gm7uj6vjx1849 .

observable:PhoneAccount sh:targetClass observable:PhoneAccount .

_:node1gm7uj6vjx1854 sh:message "Value is not member of the vocabulary TriggerFrequencyVocab." .

observable:PhoneAccountFacet a owl:Class .

_:node1gm7uj6vjx1856 sh:datatype vocabulary:TriggerFrequencyVocab .

observable:PhoneAccountFacet a sh:NodeShape .

_:node1gm7uj6vjx1857 rdf:first "TASK_EVENT_TRIGGER_AT_LOGON"^^vocabulary:TriggerFrequencyVocab .

observable:PhoneAccountFacet rdfs:subClassOf core:Facet .

_:node1gm7uj6vjx1857 rdf:rest _:node1gm7uj6vjx1858 .

observable:PhoneAccountFacet rdfs:label "PhoneAccountFacet"@en .

_:node1gm7uj6vjx1858 rdf:first "TASK_EVENT_TRIGGER_AT_SYSTEMSTART"^^vocabulary:TriggerFrequencyVocab .

observable:PhoneAccountFacet rdfs:comment "A phone account facet is a grouping of characteristics unique to an arrangement with an entity to enable and control the provision of a telephony capability or service."@en .

_:node1gm7uj6vjx1858 rdf:rest _:node1gm7uj6vjx1859 .

_:node1gm7uj6vjx1670 sh:datatype xsd:string .

_:node1gm7uj6vjx1859 rdf:first "TASK_EVENT_TRIGGER_ON_IDLE"^^vocabulary:TriggerFrequencyVocab .

_:node1gm7uj6vjx1670 sh:maxCount 1 .

_:node1gm7uj6vjx1859 rdf:rest _:node1gm7uj6vjx1860 .

_:node1gm7uj6vjx1670 sh:nodeKind sh:Literal .

_:node1gm7uj6vjx1860 rdf:first "TASK_TIME_TRIGGER_DAILY"^^vocabulary:TriggerFrequencyVocab .

_:node1gm7uj6vjx1670 sh:path observable:phoneNumber .

_:node1gm7uj6vjx1860 rdf:rest _:node1gm7uj6vjx1861 .

observable:PhoneAccountFacet sh:property _:node1gm7uj6vjx1670 .

_:node1gm7uj6vjx1861 rdf:first "TASK_TIME_TRIGGER_MONTHLYDATE"^^vocabulary:TriggerFrequencyVocab .

observable:PhoneAccountFacet sh:targetClass observable:PhoneAccountFacet .

_:node1gm7uj6vjx1861 rdf:rest _:node1gm7uj6vjx1862 .

observable:Pipe a owl:Class .

_:node1gm7uj6vjx1862 rdf:first "TASK_TIME_TRIGGER_MONTHLYDOW"^^vocabulary:TriggerFrequencyVocab .

observable:Pipe a sh:NodeShape .

_:node1gm7uj6vjx1862 rdf:rest _:node1gm7uj6vjx1863 .

observable:Pipe rdfs:subClassOf observable:ObservableObject .

_:node1gm7uj6vjx1863 rdf:first "TASK_TIME_TRIGGER_ONCE"^^vocabulary:TriggerFrequencyVocab .

observable:Pipe rdfs:label "Pipe"@en .

_:node1gm7uj6vjx1863 rdf:rest _:node1gm7uj6vjx1864 .

observable:Pipe rdfs:comment "A pipe is a mechanism for one-way inter-process communication using message passing where data written by one process is buffered by the operating system until it is read by the next process, and this uni-directional channel disappears when the processes are completed. [based on https://en.wikipedia.org/wiki/Pipeline_(Unix) ; https://en.wikipedia.org/wiki/Anonymous_pipe]"@en .

_:node1gm7uj6vjx1864 rdf:first "TASK_TIME_TRIGGER_WEEKLY"^^vocabulary:TriggerFrequencyVocab .

observable:Pipe sh:targetClass observable:Pipe .

_:node1gm7uj6vjx1864 rdf:rest rdf:nil .

observable:Post a owl:Class .

_:node1gm7uj6vjx1856 sh:in _:node1gm7uj6vjx1857 .

observable:Post a sh:NodeShape .

_:node1gm7uj6vjx1855 rdf:first _:node1gm7uj6vjx1856 .

observable:Post rdfs:subClassOf observable:Message .

_:node1gm7uj6vjx1855 rdf:rest _:node1gm7uj6vjx1865 .

observable:Post rdfs:label "Post"@en .

_:node1gm7uj6vjx1866 sh:datatype xsd:string .

observable:Post rdfs:comment "A post is message submitted to an online discussion/publishing site (forum, blog, etc.)."@en .

_:node1gm7uj6vjx1865 rdf:first _:node1gm7uj6vjx1866 .

observable:Post sh:targetClass observable:Post .

_:node1gm7uj6vjx1865 rdf:rest rdf:nil .

observable:Process a owl:Class .

_:node1gm7uj6vjx1854 sh:or _:node1gm7uj6vjx1855 .

observable:Process a sh:NodeShape .

_:node1gm7uj6vjx1854 sh:path observable:triggerFrequency .

observable:Process rdfs:subClassOf observable:ObservableObject .

observable:TriggerType sh:property _:node1gm7uj6vjx1854 .

observable:Process rdfs:label "Process"@en .

_:node1gm7uj6vjx1867 sh:message "Value is not member of the vocabulary TriggerTypeVocab." .

observable:Process rdfs:comment "A process is an instance of a computer program executed on an operating system."@en .

_:node1gm7uj6vjx1869 sh:datatype vocabulary:TriggerTypeVocab .

observable:Process sh:targetClass observable:Process .

_:node1gm7uj6vjx1870 rdf:first "TASK_TRIGGER_BOOT"^^vocabulary:TriggerTypeVocab .

observable:ProcessFacet a owl:Class .

_:node1gm7uj6vjx1870 rdf:rest _:node1gm7uj6vjx1871 .

observable:ProcessFacet a sh:NodeShape .

_:node1gm7uj6vjx1871 rdf:first "TASK_TRIGGER_EVENT"^^vocabulary:TriggerTypeVocab .

observable:ProcessFacet rdfs:subClassOf core:Facet .

_:node1gm7uj6vjx1871 rdf:rest _:node1gm7uj6vjx1872 .

observable:ProcessFacet rdfs:label "ProcessFacet"@en .

_:node1gm7uj6vjx1872 rdf:first "TASK_TRIGGER_IDLE"^^vocabulary:TriggerTypeVocab .

observable:ProcessFacet rdfs:comment "A process facet is a grouping of characteristics unique to an instance of a computer program executed on an operating system."@en .

_:node1gm7uj6vjx1872 rdf:rest _:node1gm7uj6vjx1873 .

_:node1gm7uj6vjx1671 sh:class observable:ObservableObject .

_:node1gm7uj6vjx1873 rdf:first "TASK_TRIGGER_LOGON"^^vocabulary:TriggerTypeVocab .

_:node1gm7uj6vjx1671 sh:maxCount 1 .

_:node1gm7uj6vjx1873 rdf:rest _:node1gm7uj6vjx1874 .

_:node1gm7uj6vjx1671 sh:nodeKind sh:IRI .

_:node1gm7uj6vjx1874 rdf:first "TASK_TRIGGER_REGISTRATION"^^vocabulary:TriggerTypeVocab .

_:node1gm7uj6vjx1671 sh:path observable:binary .

_:node1gm7uj6vjx1874 rdf:rest _:node1gm7uj6vjx1875 .

observable:ProcessFacet sh:property _:node1gm7uj6vjx1671 .

_:node1gm7uj6vjx1875 rdf:first "TASK_TRIGGER_SESSION_STATE_CHANGE"^^vocabulary:TriggerTypeVocab .

_:node1gm7uj6vjx1672 sh:class observable:ObservableObject .

_:node1gm7uj6vjx1875 rdf:rest _:node1gm7uj6vjx1876 .

_:node1gm7uj6vjx1672 sh:maxCount 1 .

_:node1gm7uj6vjx1876 rdf:first "TASK_TRIGGER_TIME"^^vocabulary:TriggerTypeVocab .

_:node1gm7uj6vjx1672 sh:nodeKind sh:IRI .

_:node1gm7uj6vjx1876 rdf:rest rdf:nil .

_:node1gm7uj6vjx1672 sh:path observable:creatorUser .

_:node1gm7uj6vjx1869 sh:in _:node1gm7uj6vjx1870 .

observable:ProcessFacet sh:property _:node1gm7uj6vjx1672 .

_:node1gm7uj6vjx1868 rdf:first _:node1gm7uj6vjx1869 .

_:node1gm7uj6vjx1673 sh:class observable:ObservableObject .

_:node1gm7uj6vjx1868 rdf:rest _:node1gm7uj6vjx1877 .

_:node1gm7uj6vjx1673 sh:maxCount 1 .

_:node1gm7uj6vjx1878 sh:datatype xsd:string .

_:node1gm7uj6vjx1673 sh:nodeKind sh:IRI .

_:node1gm7uj6vjx1877 rdf:first _:node1gm7uj6vjx1878 .

_:node1gm7uj6vjx1673 sh:path observable:parent .

_:node1gm7uj6vjx1877 rdf:rest rdf:nil .

observable:ProcessFacet sh:property _:node1gm7uj6vjx1673 .

_:node1gm7uj6vjx1867 sh:or _:node1gm7uj6vjx1868 .

_:node1gm7uj6vjx1674 sh:class types:Dictionary .

_:node1gm7uj6vjx1867 sh:path observable:triggerType .

_:node1gm7uj6vjx1674 sh:maxCount 1 .

observable:TriggerType sh:property _:node1gm7uj6vjx1867 .

_:node1gm7uj6vjx1674 sh:nodeKind sh:IRI .

observable:TriggerType sh:targetClass observable:TriggerType .

_:node1gm7uj6vjx1674 sh:path observable:environmentVariables .

observable:Tweet a owl:Class .

observable:ProcessFacet sh:property _:node1gm7uj6vjx1674 .

observable:Tweet a sh:NodeShape .

_:node1gm7uj6vjx1675 sh:datatype xsd:boolean .

observable:Tweet rdfs:subClassOf observable:Message .

_:node1gm7uj6vjx1675 sh:maxCount 1 .

observable:Tweet rdfs:label "Tweet"@en .

_:node1gm7uj6vjx1675 sh:nodeKind sh:Literal .

observable:Tweet rdfs:comment "A tweet is message submitted by a Twitter user account to the Twitter microblogging platform."@en .

_:node1gm7uj6vjx1675 sh:path observable:isHidden .

observable:Tweet sh:targetClass observable:Tweet .

observable:ProcessFacet sh:property _:node1gm7uj6vjx1675 .

observable:TwitterProfileFacet a owl:Class .

_:node1gm7uj6vjx1676 sh:datatype xsd:dateTime .

observable:TwitterProfileFacet a sh:NodeShape .

_:node1gm7uj6vjx1676 sh:maxCount 1 .

observable:TwitterProfileFacet rdfs:subClassOf core:Facet .

_:node1gm7uj6vjx1676 sh:nodeKind sh:Literal .

observable:TwitterProfileFacet rdfs:label "TwitterProfileFacet" .

_:node1gm7uj6vjx1676 sh:path observable:exitTime .

observable:TwitterProfileFacet rdfs:comment "A twitter profile facet is a grouping of characteristics unique to an explicit digital representation of identity and characteristics of the owner of a single Twitter user account. [based on https://en.wikipedia.org/wiki/User_profile]" .

observable:ProcessFacet sh:property _:node1gm7uj6vjx1676 .

_:node1gm7uj6vjx1879 sh:class observable:ObservableObject .

_:node1gm7uj6vjx1677 sh:datatype xsd:dateTime .

_:node1gm7uj6vjx1879 sh:maxCount 1 .

_:node1gm7uj6vjx1677 sh:maxCount 1 .

_:node1gm7uj6vjx1879 sh:nodeKind sh:IRI .

_:node1gm7uj6vjx1677 sh:nodeKind sh:Literal .

_:node1gm7uj6vjx1879 sh:path observable:profileBackgroundLocation .

_:node1gm7uj6vjx1677 sh:path observable:observableCreatedTime .

observable:TwitterProfileFacet sh:property _:node1gm7uj6vjx1879 .

observable:ProcessFacet sh:property _:node1gm7uj6vjx1677 .

_:node1gm7uj6vjx1880 sh:class observable:ObservableObject .

_:node1gm7uj6vjx1678 sh:datatype xsd:integer .

_:node1gm7uj6vjx1880 sh:maxCount 1 .

_:node1gm7uj6vjx1678 sh:maxCount 1 .

_:node1gm7uj6vjx1880 sh:nodeKind sh:IRI .

_:node1gm7uj6vjx1678 sh:nodeKind sh:Literal .

_:node1gm7uj6vjx1880 sh:path observable:profileBannerLocation .

_:node1gm7uj6vjx1678 sh:path observable:exitStatus .

observable:TwitterProfileFacet sh:property _:node1gm7uj6vjx1880 .

observable:ProcessFacet sh:property _:node1gm7uj6vjx1678 .

_:node1gm7uj6vjx1881 sh:class observable:ObservableObject .

_:node1gm7uj6vjx1679 sh:datatype xsd:integer .

_:node1gm7uj6vjx1881 sh:maxCount 1 .

_:node1gm7uj6vjx1679 sh:maxCount 1 .

_:node1gm7uj6vjx1881 sh:nodeKind sh:IRI .

_:node1gm7uj6vjx1679 sh:nodeKind sh:Literal .

_:node1gm7uj6vjx1881 sh:path observable:profileImageLocation .

_:node1gm7uj6vjx1679 sh:path observable:pid .

observable:TwitterProfileFacet sh:property _:node1gm7uj6vjx1881 .

observable:ProcessFacet sh:property _:node1gm7uj6vjx1679 .

_:node1gm7uj6vjx1882 sh:class types:Hash .

_:node1gm7uj6vjx1680 sh:datatype xsd:string .

_:node1gm7uj6vjx1882 sh:minCount 0 .

_:node1gm7uj6vjx1680 sh:maxCount 1 .

_:node1gm7uj6vjx1882 sh:nodeKind sh:IRI .

_:node1gm7uj6vjx1680 sh:nodeKind sh:Literal .

_:node1gm7uj6vjx1882 sh:path observable:profileBackgroundHash .

_:node1gm7uj6vjx1680 sh:path observable:currentWorkingDirectory .

observable:TwitterProfileFacet sh:property _:node1gm7uj6vjx1882 .

observable:ProcessFacet sh:property _:node1gm7uj6vjx1680 .

_:node1gm7uj6vjx1883 sh:class types:Hash .

_:node1gm7uj6vjx1681 sh:datatype xsd:string .

_:node1gm7uj6vjx1883 sh:minCount 0 .

_:node1gm7uj6vjx1681 sh:maxCount 1 .

_:node1gm7uj6vjx1883 sh:nodeKind sh:IRI .

_:node1gm7uj6vjx1681 sh:nodeKind sh:Literal .

_:node1gm7uj6vjx1883 sh:path observable:profileBannerHash .

_:node1gm7uj6vjx1681 sh:path observable:status .

observable:TwitterProfileFacet sh:property _:node1gm7uj6vjx1883 .

observable:ProcessFacet sh:property _:node1gm7uj6vjx1681 .

_:node1gm7uj6vjx1884 sh:class types:Hash .

_:node1gm7uj6vjx1682 sh:datatype xsd:string .

_:node1gm7uj6vjx1884 sh:minCount 0 .

_:node1gm7uj6vjx1682 sh:nodeKind sh:Literal .

_:node1gm7uj6vjx1884 sh:nodeKind sh:IRI .

_:node1gm7uj6vjx1682 sh:path observable:arguments .

_:node1gm7uj6vjx1884 sh:path observable:profileImageHash .

observable:ProcessFacet sh:property _:node1gm7uj6vjx1682 .

observable:TwitterProfileFacet sh:property _:node1gm7uj6vjx1884 .

observable:ProcessFacet sh:targetClass observable:ProcessFacet .

_:node1gm7uj6vjx1885 sh:datatype xsd:boolean .

observable:ProcessThread a owl:Class .

_:node1gm7uj6vjx1885 sh:maxCount 1 .

observable:ProcessThread a sh:NodeShape .

_:node1gm7uj6vjx1885 sh:nodeKind sh:Literal .

observable:ProcessThread rdfs:subClassOf observable:ObservableObject .

_:node1gm7uj6vjx1885 sh:path observable:profileIsProtected .

observable:ProcessThread rdfs:label "ProcessThread"@en .

observable:TwitterProfileFacet sh:property _:node1gm7uj6vjx1885 .

observable:ProcessThread rdfs:comment "A process thread is the smallest sequence of programmed instructions that can be managed independently by a scheduler on a computer, which is typically a part of the operating system. It is a component of a process. Multiple threads can exist within one process, executing concurrently and sharing resources such as memory, while different processes do not share these resources. In particular, the threads of a process share its executable code and the values of its dynamically allocated variables and non-thread-local global variables at any given time. [based on https://en.wikipedia.org/wiki/Thread_(computing)]"@en .

_:node1gm7uj6vjx1886 sh:datatype xsd:boolean .

observable:ProcessThread sh:targetClass observable:ProcessThread .

_:node1gm7uj6vjx1886 sh:maxCount 1 .

observable:Profile a owl:Class .

_:node1gm7uj6vjx1886 sh:nodeKind sh:Literal .

observable:Profile a sh:NodeShape .

_:node1gm7uj6vjx1886 sh:path observable:profileIsVerified .

observable:Profile rdfs:subClassOf observable:ObservableObject .

observable:TwitterProfileFacet sh:property _:node1gm7uj6vjx1886 .

observable:Profile rdfs:label "Profile"@en .

_:node1gm7uj6vjx1887 sh:datatype xsd:integer .

observable:Profile rdfs:comment "A profile is an explicit digital representation of identity and characteristics of the owner of a single user account associated with an online service or application. [based on https://en.wikipedia.org/wiki/User_profile]"@en .

_:node1gm7uj6vjx1887 sh:maxCount 1 .

observable:Profile sh:targetClass observable:Profile .

_:node1gm7uj6vjx1887 sh:nodeKind sh:Literal .

observable:ProfileFacet a owl:Class .

_:node1gm7uj6vjx1887 sh:path observable:listedCount .

observable:ProfileFacet a sh:NodeShape .

observable:TwitterProfileFacet sh:property _:node1gm7uj6vjx1887 .

observable:ProfileFacet rdfs:subClassOf core:Facet .

_:node1gm7uj6vjx1888 sh:datatype xsd:nonNegativeInteger .

observable:ProfileFacet rdfs:label "ProfileFacet"@en-us .

_:node1gm7uj6vjx1888 sh:maxCount 1 .

observable:ProfileFacet rdfs:comment "A profile facet is a grouping of characteristics unique to an explicit digital representation of identity and characteristics of the owner of a single user account associated with an online service or application. [based on https://en.wikipedia.org/wiki/User_profile]"@en-us .

_:node1gm7uj6vjx1888 sh:nodeKind sh:Literal .

_:node1gm7uj6vjx1683 sh:class identity:Identity .

_:node1gm7uj6vjx1888 sh:path observable:favoritesCount .

_:node1gm7uj6vjx1683 sh:maxCount 1 .

observable:TwitterProfileFacet sh:property _:node1gm7uj6vjx1888 .

_:node1gm7uj6vjx1683 sh:nodeKind sh:IRI .

_:node1gm7uj6vjx1889 sh:datatype xsd:nonNegativeInteger .

_:node1gm7uj6vjx1683 sh:path observable:profileIdentity .

_:node1gm7uj6vjx1889 sh:maxCount 1 .

observable:ProfileFacet sh:property _:node1gm7uj6vjx1683 .

_:node1gm7uj6vjx1889 sh:nodeKind sh:Literal .

_:node1gm7uj6vjx1684 sh:class observable:ContactAddress .

_:node1gm7uj6vjx1889 sh:path observable:followersCount .

_:node1gm7uj6vjx1684 sh:maxCount 1 .

observable:TwitterProfileFacet sh:property _:node1gm7uj6vjx1889 .

_:node1gm7uj6vjx1684 sh:nodeKind sh:IRI .

_:node1gm7uj6vjx1890 sh:datatype xsd:nonNegativeInteger .

_:node1gm7uj6vjx1684 sh:path observable:contactAddress .

_:node1gm7uj6vjx1890 sh:maxCount 1 .

observable:ProfileFacet sh:property _:node1gm7uj6vjx1684 .

_:node1gm7uj6vjx1890 sh:nodeKind sh:Literal .

_:node1gm7uj6vjx1685 sh:class observable:ContactEmail .

_:node1gm7uj6vjx1890 sh:path observable:friendsCount .

_:node1gm7uj6vjx1685 sh:maxCount 1 .

observable:TwitterProfileFacet sh:property _:node1gm7uj6vjx1890 .

_:node1gm7uj6vjx1685 sh:nodeKind sh:IRI .

_:node1gm7uj6vjx1891 sh:datatype xsd:nonNegativeInteger .

_:node1gm7uj6vjx1685 sh:path observable:contactEmail .

_:node1gm7uj6vjx1891 sh:maxCount 1 .

observable:ProfileFacet sh:property _:node1gm7uj6vjx1685 .

_:node1gm7uj6vjx1891 sh:nodeKind sh:Literal .

_:node1gm7uj6vjx1686 sh:class observable:ContactMessaging .

_:node1gm7uj6vjx1891 sh:path observable:statusesCount .

_:node1gm7uj6vjx1686 sh:maxCount 1 .

observable:TwitterProfileFacet sh:property _:node1gm7uj6vjx1891 .

_:node1gm7uj6vjx1686 sh:nodeKind sh:IRI .

_:node1gm7uj6vjx1892 sh:datatype xsd:string .

_:node1gm7uj6vjx1686 sh:path observable:contactMessaging .

_:node1gm7uj6vjx1892 sh:maxCount 1 .

observable:ProfileFacet sh:property _:node1gm7uj6vjx1686 .

_:node1gm7uj6vjx1892 sh:nodeKind sh:Literal .

_:node1gm7uj6vjx1687 sh:class observable:ContactPhone .

_:node1gm7uj6vjx1892 sh:path observable:twitterHandle .

_:node1gm7uj6vjx1687 sh:maxCount 1 .

observable:TwitterProfileFacet sh:property _:node1gm7uj6vjx1892 .

_:node1gm7uj6vjx1687 sh:nodeKind sh:IRI .

_:node1gm7uj6vjx1893 sh:datatype xsd:string .

_:node1gm7uj6vjx1687 sh:path observable:contactPhone .

_:node1gm7uj6vjx1893 sh:maxCount 1 .

observable:ProfileFacet sh:property _:node1gm7uj6vjx1687 .

_:node1gm7uj6vjx1893 sh:nodeKind sh:Literal .

_:node1gm7uj6vjx1688 sh:class observable:ContactURL .

_:node1gm7uj6vjx1893 sh:path observable:twitterId .

_:node1gm7uj6vjx1688 sh:maxCount 1 .

observable:TwitterProfileFacet sh:property _:node1gm7uj6vjx1893 .

_:node1gm7uj6vjx1688 sh:nodeKind sh:IRI .

_:node1gm7uj6vjx1894 sh:datatype xsd:string .

_:node1gm7uj6vjx1688 sh:path observable:contactURL .

_:node1gm7uj6vjx1894 sh:maxCount 1 .

observable:ProfileFacet sh:property _:node1gm7uj6vjx1688 .

_:node1gm7uj6vjx1894 sh:nodeKind sh:Literal .

_:node1gm7uj6vjx1689 sh:class observable:ObservableObject .

_:node1gm7uj6vjx1894 sh:path observable:userLocationString .

_:node1gm7uj6vjx1689 sh:maxCount 1 .

observable:TwitterProfileFacet sh:property _:node1gm7uj6vjx1894 .

_:node1gm7uj6vjx1689 sh:nodeKind sh:IRI .

observable:TwitterProfileFacet sh:targetClass observable:TwitterProfileFacet .

_:node1gm7uj6vjx1689 sh:path observable:profileAccount .

observable:UNIXAccount a owl:Class .

observable:ProfileFacet sh:property _:node1gm7uj6vjx1689 .

observable:UNIXAccount a sh:NodeShape .

_:node1gm7uj6vjx1690 sh:class observable:ObservableObject .

observable:UNIXAccount rdfs:subClassOf observable:DigitalAccount .

_:node1gm7uj6vjx1690 sh:maxCount 1 .

observable:UNIXAccount rdfs:label "UNIXAccount"@en .

_:node1gm7uj6vjx1690 sh:nodeKind sh:IRI .

observable:UNIXAccount rdfs:comment "A UNIX account is an account on a UNIX operating system."@en .

_:node1gm7uj6vjx1690 sh:path observable:profileService .

observable:UNIXAccount sh:targetClass observable:UNIXAccount .

observable:ProfileFacet sh:property _:node1gm7uj6vjx1690 .

observable:UNIXAccountFacet a owl:Class .

_:node1gm7uj6vjx1691 sh:class observable:ObservableObject .

observable:UNIXAccountFacet a sh:NodeShape .

_:node1gm7uj6vjx1691 sh:maxCount 1 .

observable:UNIXAccountFacet rdfs:subClassOf core:Facet .

_:node1gm7uj6vjx1691 sh:nodeKind sh:IRI .

observable:UNIXAccountFacet rdfs:label "UNIXAccountFacet"@en .

_:node1gm7uj6vjx1691 sh:path observable:profileWebsite .

observable:UNIXAccountFacet rdfs:comment "A UNIX account facet is a grouping of characteristics unique to an account on a UNIX operating system."@en .

observable:ProfileFacet sh:property _:node1gm7uj6vjx1691 .

_:node1gm7uj6vjx1895 sh:datatype xsd:integer .

_:node1gm7uj6vjx1692 sh:datatype xsd:dateTime .

_:node1gm7uj6vjx1895 sh:maxCount 1 .

_:node1gm7uj6vjx1692 sh:maxCount 1 .

_:node1gm7uj6vjx1895 sh:nodeKind sh:Literal .

_:node1gm7uj6vjx1692 sh:nodeKind sh:Literal .

_:node1gm7uj6vjx1895 sh:path observable:gid .

_:node1gm7uj6vjx1692 sh:path observable:profileCreated .

observable:UNIXAccountFacet sh:property _:node1gm7uj6vjx1895 .

observable:ProfileFacet sh:property _:node1gm7uj6vjx1692 .

_:node1gm7uj6vjx1896 sh:datatype xsd:string .

_:node1gm7uj6vjx1693 sh:datatype xsd:string .

_:node1gm7uj6vjx1896 sh:maxCount 1 .

_:node1gm7uj6vjx1693 sh:maxCount 1 .

_:node1gm7uj6vjx1896 sh:nodeKind sh:Literal .

_:node1gm7uj6vjx1693 sh:nodeKind sh:Literal .

_:node1gm7uj6vjx1896 sh:path observable:shell .

_:node1gm7uj6vjx1693 sh:path core:name .

observable:UNIXAccountFacet sh:property _:node1gm7uj6vjx1896 .

observable:ProfileFacet sh:property _:node1gm7uj6vjx1693 .

observable:UNIXAccountFacet sh:targetClass observable:UNIXAccountFacet .

_:node1gm7uj6vjx1694 sh:datatype xsd:string .

observable:UNIXFile a owl:Class .

_:node1gm7uj6vjx1694 sh:maxCount 1 .

observable:UNIXFile a sh:NodeShape .

_:node1gm7uj6vjx1694 sh:nodeKind sh:Literal .

observable:UNIXFile rdfs:subClassOf observable:File .

_:node1gm7uj6vjx1694 sh:path observable:displayName .

observable:UNIXFile rdfs:label "UNIXFile"@en .

observable:ProfileFacet sh:property _:node1gm7uj6vjx1694 .

observable:UNIXFile rdfs:comment "A UNIX file is a file pertaining to the UNIX operating system."@en .

_:node1gm7uj6vjx1695 sh:datatype xsd:string .

observable:UNIXFile sh:targetClass observable:UNIXFile .

_:node1gm7uj6vjx1695 sh:minCount 0 .

observable:UNIXFilePermissionsFacet a owl:Class .

_:node1gm7uj6vjx1695 sh:nodeKind sh:Literal .

observable:UNIXFilePermissionsFacet a sh:NodeShape .

_:node1gm7uj6vjx1695 sh:path observable:profileLanguage .

observable:UNIXFilePermissionsFacet rdfs:subClassOf core:Facet .

observable:ProfileFacet sh:property _:node1gm7uj6vjx1695 .

observable:UNIXFilePermissionsFacet rdfs:label "UNIXFilePermissionsFacet"@en .

observable:ProfileFacet sh:targetClass observable:ProfileFacet .

observable:UNIXFilePermissionsFacet rdfs:comment "A UNIX file permissions facet is a grouping of characteristics unique to the access rights (e.g., view, change, navigate, execute) of a file on a UNIX file system."@en .

observable:PropertiesEnumeratedEffectFacet a owl:Class .

observable:UNIXFilePermissionsFacet sh:targetClass observable:UNIXFilePermissionsFacet .

observable:PropertiesEnumeratedEffectFacet a sh:NodeShape .

observable:UNIXProcess a owl:Class .

observable:PropertiesEnumeratedEffectFacet rdfs:subClassOf core:Facet .

observable:UNIXProcess a sh:NodeShape .

observable:PropertiesEnumeratedEffectFacet rdfs:subClassOf observable:DefinedEffectFacet .

observable:UNIXProcess rdfs:subClassOf observable:Process .

observable:PropertiesEnumeratedEffectFacet rdfs:label "PropertiesEnumeratedEffectFacet"@en .

observable:UNIXProcess rdfs:label "UNIXProcess"@en .

observable:PropertiesEnumeratedEffectFacet rdfs:comment "A properties enumerated effect facet is a grouping of characteristics unique to the effects of actions upon observable objects where a characteristic of the observable object is enumerated. An example of this would be startup parameters for a process."@en .

observable:UNIXProcess rdfs:comment "A UNIX process is an instance of a computer program executed on a UNIX operating system."@en .

_:node1gm7uj6vjx1696 sh:datatype xsd:string .

observable:UNIXProcess sh:targetClass observable:UNIXProcess .

_:node1gm7uj6vjx1696 sh:maxCount 1 .

observable:UNIXProcessFacet a owl:Class .

_:node1gm7uj6vjx1696 sh:nodeKind sh:Literal .

observable:UNIXProcessFacet a sh:NodeShape .

_:node1gm7uj6vjx1696 sh:path observable:properties .

observable:UNIXProcessFacet rdfs:subClassOf core:Facet .

observable:PropertiesEnumeratedEffectFacet sh:property _:node1gm7uj6vjx1696 .

observable:UNIXProcessFacet rdfs:label "UNIXProcessFacet"@en .

observable:PropertiesEnumeratedEffectFacet sh:targetClass observable:PropertiesEnumeratedEffectFacet .

observable:UNIXProcessFacet rdfs:comment "A UNIX process facet is a grouping of characteristics unique to an instance of a computer program executed on a UNIX operating system."@en .

observable:PropertyReadEffectFacet a owl:Class .

_:node1gm7uj6vjx1897 sh:datatype xsd:integer .

observable:PropertyReadEffectFacet a sh:NodeShape .

_:node1gm7uj6vjx1897 sh:nodeKind sh:Literal .

observable:PropertyReadEffectFacet rdfs:subClassOf observable:DefinedEffectFacet .

_:node1gm7uj6vjx1897 sh:path observable:openFileDescriptor .

observable:PropertyReadEffectFacet rdfs:label "PropertyReadEffectFacet"@en .

observable:UNIXProcessFacet sh:property _:node1gm7uj6vjx1897 .

observable:PropertyReadEffectFacet rdfs:comment "A properties read effect facet is a grouping of characteristics unique to the effects of actions upon observable objects where a characteristic is read from an observable object. An example of this would be the current running state of a process."@en .

_:node1gm7uj6vjx1898 sh:datatype xsd:nonNegativeInteger .

_:node1gm7uj6vjx1697 sh:datatype xsd:string .

_:node1gm7uj6vjx1898 sh:nodeKind sh:Literal .

_:node1gm7uj6vjx1697 sh:maxCount 1 .

_:node1gm7uj6vjx1898 sh:path observable:ruid .

_:node1gm7uj6vjx1697 sh:nodeKind sh:Literal .

observable:UNIXProcessFacet sh:property _:node1gm7uj6vjx1898 .

_:node1gm7uj6vjx1697 sh:path observable:propertyName .

observable:UNIXProcessFacet sh:targetClass observable:UNIXProcessFacet .

observable:PropertyReadEffectFacet sh:property _:node1gm7uj6vjx1697 .

observable:UNIXVolumeFacet a owl:Class .

_:node1gm7uj6vjx1698 sh:datatype xsd:string .

observable:UNIXVolumeFacet a sh:NodeShape .

_:node1gm7uj6vjx1698 sh:maxCount 1 .

observable:UNIXVolumeFacet rdfs:subClassOf core:Facet .

_:node1gm7uj6vjx1698 sh:nodeKind sh:Literal .

observable:UNIXVolumeFacet rdfs:label "UNIXVolumeFacet"@en .

_:node1gm7uj6vjx1698 sh:path observable:value .

observable:UNIXVolumeFacet rdfs:comment "A UNIX volume facet is a grouping of characteristics unique to a single accessible storage area (volume) with a single UNIX file system. [based on https://en.wikipedia.org/wiki/Volume_(computing)]"@en .

observable:PropertyReadEffectFacet sh:property _:node1gm7uj6vjx1698 .

_:node1gm7uj6vjx1899 sh:datatype xsd:string .

observable:PropertyReadEffectFacet sh:targetClass observable:PropertyReadEffectFacet .

_:node1gm7uj6vjx1899 sh:maxCount 1 .

observable:ProtocolConverter a owl:Class , sh:NodeShape .

_:node1gm7uj6vjx1899 sh:nodeKind sh:Literal .

observable:ProtocolConverter rdfs:subClassOf observable:Device .

_:node1gm7uj6vjx1899 sh:path observable:mountPoint .

observable:UNIXVolumeFacet sh:property _:node1gm7uj6vjx1899 .

_:node1gm7uj6vjx1900 sh:datatype xsd:string .

observable:ProtocolConverter rdfs:label "ProtocolConverter"@en-us .

_:node1gm7uj6vjx1900 sh:maxCount 1 .

observable:ProtocolConverter rdfs:comment "A protocol converter is a device that converts from one protocol to another (e.g. SD to USB, SATA to USB, etc."@en-us .

_:node1gm7uj6vjx1900 sh:nodeKind sh:Literal .

observable:ProtocolConverter sh:targetClass observable:ProtocolConverter .

_:node1gm7uj6vjx1900 sh:path observable:options .

observable:RasterPicture a owl:Class .

observable:UNIXVolumeFacet sh:property _:node1gm7uj6vjx1900 .

observable:RasterPicture a sh:NodeShape .

observable:UNIXVolumeFacet sh:targetClass observable:UNIXVolumeFacet .

observable:RasterPicture rdfs:subClassOf observable:File .

observable:URL a owl:Class .

observable:RasterPicture rdfs:label "RasterPicture"@en .

observable:URL a sh:NodeShape .

observable:RasterPicture rdfs:comment "A raster picture is a raster (or bitmap) image."@en .

observable:URL rdfs:subClassOf observable:ObservableObject .

observable:RasterPicture sh:targetClass observable:RasterPicture .

observable:URL rdfs:label "URL"@en .

observable:RasterPictureFacet a owl:Class .

observable:URL rdfs:comment "A URL is a uniform resource locator (URL) acting as a resolvable address to a particular WWW (World Wide Web) accessible resource."@en .

observable:RasterPictureFacet a sh:NodeShape .

observable:URL sh:targetClass observable:URL .

observable:RasterPictureFacet rdfs:subClassOf core:Facet .

observable:URLFacet a owl:Class .

observable:RasterPictureFacet rdfs:label "RasterPictureFacet"@en .

observable:URLFacet a sh:NodeShape .

observable:RasterPictureFacet rdfs:comment "A raster picture facet is a grouping of characteristics unique to a raster (or bitmap) image."@en .

observable:URLFacet rdfs:subClassOf core:Facet .

_:node1gm7uj6vjx1699 sh:class observable:ObservableObject .

observable:URLFacet rdfs:label "URLFacet"@en .

_:node1gm7uj6vjx1699 sh:maxCount 1 .

observable:URLFacet rdfs:comment "A URL facet is a grouping of characteristics unique to a uniform resource locator (URL) acting as a resolvable address to a particular WWW (World Wide Web) accessible resource."@en .

_:node1gm7uj6vjx1699 sh:nodeKind sh:IRI .

_:node1gm7uj6vjx1901 sh:class observable:ObservableObject .

_:node1gm7uj6vjx1699 sh:path observable:camera .

_:node1gm7uj6vjx1901 sh:maxCount 1 .

observable:RasterPictureFacet sh:property _:node1gm7uj6vjx1699 .

_:node1gm7uj6vjx1901 sh:nodeKind sh:IRI .

_:node1gm7uj6vjx1700 sh:datatype xsd:integer .

_:node1gm7uj6vjx1901 sh:path observable:host .

_:node1gm7uj6vjx1700 sh:maxCount 1 .

observable:URLFacet sh:property _:node1gm7uj6vjx1901 .

_:node1gm7uj6vjx1700 sh:nodeKind sh:Literal .

_:node1gm7uj6vjx1902 sh:datatype xsd:integer .

_:node1gm7uj6vjx1700 sh:path observable:bitsPerPixel .

_:node1gm7uj6vjx1902 sh:maxCount 1 .

observable:RasterPictureFacet sh:property _:node1gm7uj6vjx1700 .

_:node1gm7uj6vjx1902 sh:nodeKind sh:Literal .

_:node1gm7uj6vjx1701 sh:datatype xsd:integer .

_:node1gm7uj6vjx1902 sh:path observable:port .

_:node1gm7uj6vjx1701 sh:maxCount 1 .

observable:URLFacet sh:property _:node1gm7uj6vjx1902 .

_:node1gm7uj6vjx1701 sh:nodeKind sh:Literal .

_:node1gm7uj6vjx1903 sh:datatype xsd:string .

_:node1gm7uj6vjx1701 sh:path observable:pictureHeight .

_:node1gm7uj6vjx1903 sh:maxCount 1 .

observable:RasterPictureFacet sh:property _:node1gm7uj6vjx1701 .

_:node1gm7uj6vjx1903 sh:nodeKind sh:Literal .

_:node1gm7uj6vjx1702 sh:datatype xsd:integer .

_:node1gm7uj6vjx1903 sh:path observable:fragment .

_:node1gm7uj6vjx1702 sh:maxCount 1 .

observable:URLFacet sh:property _:node1gm7uj6vjx1903 .

_:node1gm7uj6vjx1702 sh:nodeKind sh:Literal .

_:node1gm7uj6vjx1904 sh:datatype xsd:string .

_:node1gm7uj6vjx1702 sh:path observable:pictureWidth .

_:node1gm7uj6vjx1904 sh:maxCount 1 .

observable:RasterPictureFacet sh:property _:node1gm7uj6vjx1702 .

_:node1gm7uj6vjx1904 sh:nodeKind sh:Literal .

_:node1gm7uj6vjx1703 sh:datatype xsd:string .

_:node1gm7uj6vjx1904 sh:path observable:fullValue .

_:node1gm7uj6vjx1703 sh:maxCount 1 .

observable:URLFacet sh:property _:node1gm7uj6vjx1904 .

_:node1gm7uj6vjx1703 sh:nodeKind sh:Literal .

_:node1gm7uj6vjx1905 sh:datatype xsd:string .

_:node1gm7uj6vjx1703 sh:path observable:imageCompressionMethod .

_:node1gm7uj6vjx1905 sh:maxCount 1 .

observable:RasterPictureFacet sh:property _:node1gm7uj6vjx1703 .

_:node1gm7uj6vjx1905 sh:nodeKind sh:Literal .

_:node1gm7uj6vjx1704 sh:datatype xsd:string .

_:node1gm7uj6vjx1905 sh:path observable:password .

_:node1gm7uj6vjx1704 sh:maxCount 1 .

observable:URLFacet sh:property _:node1gm7uj6vjx1905 .

_:node1gm7uj6vjx1704 sh:nodeKind sh:Literal .

_:node1gm7uj6vjx1906 sh:datatype xsd:string .

_:node1gm7uj6vjx1704 sh:path observable:pictureType .

_:node1gm7uj6vjx1906 sh:maxCount 1 .

observable:RasterPictureFacet sh:property _:node1gm7uj6vjx1704 .

_:node1gm7uj6vjx1906 sh:nodeKind sh:Literal .

observable:RasterPictureFacet sh:targetClass observable:RasterPictureFacet .

_:node1gm7uj6vjx1906 sh:path observable:path .

observable:RecoveredObject a owl:Class .

observable:URLFacet sh:property _:node1gm7uj6vjx1906 .

observable:RecoveredObject a sh:NodeShape .

_:node1gm7uj6vjx1907 sh:datatype xsd:string .

observable:RecoveredObject rdfs:subClassOf observable:ObservableObject .

_:node1gm7uj6vjx1907 sh:maxCount 1 .

observable:RecoveredObject rdfs:label "RecoveredObject"@en .

_:node1gm7uj6vjx1907 sh:nodeKind sh:Literal .

observable:RecoveredObject rdfs:comment "An observable object that was the result of a recovery operation."@en .

_:node1gm7uj6vjx1907 sh:path observable:query .

observable:RecoveredObject sh:targetClass observable:RecoveredObject .

observable:URLFacet sh:property _:node1gm7uj6vjx1907 .

_:node1gm7uj6vjx1908 sh:datatype xsd:string ;
	sh:maxCount 1 ;
	sh:nodeKind sh:Literal ;
	sh:path observable:scheme .

observable:URLFacet sh:property _:node1gm7uj6vjx1908 .

_:node1gm7uj6vjx1909 sh:datatype xsd:string ;
	sh:maxCount 1 ;
	sh:nodeKind sh:Literal ;
	sh:path observable:userName .

observable:URLFacet sh:property _:node1gm7uj6vjx1909 ;
	sh:targetClass observable:URLFacet .

observable:URLHistory a owl:Class , sh:NodeShape ;
	rdfs:subClassOf observable:ObservableObject ;
	rdfs:label "URLHistory"@en ;
	rdfs:comment "A URL history characterizes the stored URL history for a particular web browser"@en ;
	sh:targetClass observable:URLHistory .

observable:URLHistoryEntry a owl:Class , sh:NodeShape ;
	rdfs:subClassOf core:UcoInherentCharacterizationThing ;
	rdfs:label "URL History Entry"@en-us ;
	rdfs:comment "A URL history entry is a grouping of characteristics unique to the properties of a single URL history entry for a particular browser."@en-us .

_:node1gm7uj6vjx1910 sh:class observable:ObservableObject ;
	sh:maxCount 1 ;
	sh:nodeKind sh:IRI ;
	sh:path observable:url .

observable:URLHistoryEntry sh:property _:node1gm7uj6vjx1910 .

_:node1gm7uj6vjx1911 sh:class observable:ObservableObject ;
	sh:minCount 0 ;
	sh:nodeKind sh:IRI ;
	sh:path observable:referrerUrl .

observable:URLHistoryEntry sh:property _:node1gm7uj6vjx1911 .

_:node1gm7uj6vjx1912 sh:datatype xsd:dateTime ;
	sh:maxCount 1 ;
	sh:nodeKind sh:Literal ;
	sh:path observable:expirationTime .

observable:URLHistoryEntry sh:property _:node1gm7uj6vjx1912 .

_:node1gm7uj6vjx1913 sh:datatype xsd:dateTime ;
	sh:maxCount 1 ;
	sh:nodeKind sh:Literal ;
	sh:path observable:firstVisit .

observable:URLHistoryEntry sh:property _:node1gm7uj6vjx1913 .

_:node1gm7uj6vjx1914 sh:datatype xsd:dateTime ;
	sh:maxCount 1 ;
	sh:nodeKind sh:Literal ;
	sh:path observable:lastVisit .

observable:URLHistoryEntry sh:property _:node1gm7uj6vjx1914 .

_:node1gm7uj6vjx1915 sh:datatype xsd:integer ;
	sh:maxCount 1 ;
	sh:nodeKind sh:Literal ;
	sh:path observable:visitCount .

observable:URLHistoryEntry sh:property _:node1gm7uj6vjx1915 .

_:node1gm7uj6vjx1916 sh:datatype xsd:nonNegativeInteger ;
	sh:maxCount 1 ;
	sh:nodeKind sh:Literal ;
	sh:path observable:manuallyEnteredCount .

observable:URLHistoryEntry sh:property _:node1gm7uj6vjx1916 .

_:node1gm7uj6vjx1917 sh:datatype xsd:string ;
	sh:maxCount 1 ;
	sh:nodeKind sh:Literal ;
	sh:path observable:browserUserProfile .

observable:URLHistoryEntry sh:property _:node1gm7uj6vjx1917 .

_:node1gm7uj6vjx1918 sh:datatype xsd:string ;
	sh:maxCount 1 ;
	sh:nodeKind sh:Literal ;
	sh:path observable:hostname .

observable:URLHistoryEntry sh:property _:node1gm7uj6vjx1918 .

_:node1gm7uj6vjx1919 sh:datatype xsd:string ;
	sh:maxCount 1 ;
	sh:nodeKind sh:Literal ;
	sh:path observable:pageTitle .

observable:URLHistoryEntry sh:property _:node1gm7uj6vjx1919 .

_:node1gm7uj6vjx1920 sh:datatype xsd:string ;
	sh:minCount 0 ;
	sh:nodeKind sh:Literal ;
	sh:path observable:keywordSearchTerm .

observable:URLHistoryEntry sh:property _:node1gm7uj6vjx1920 ;
	sh:targetClass observable:URLHistoryEntry .

observable:URLHistoryFacet a owl:Class , sh:NodeShape ;
	rdfs:subClassOf core:Facet ;
	rdfs:label "URLHistoryFacet"@en-us ;
	rdfs:comment "A URL history facet is a grouping of characteristics unique to the stored URL history for a particular web browser"@en-us .

_:node1gm7uj6vjx1921 sh:class observable:ObservableObject ;
	sh:maxCount 1 ;
	sh:nodeKind sh:IRI ;
	sh:path observable:browserInformation .

observable:URLHistoryFacet sh:property _:node1gm7uj6vjx1921 .

_:node1gm7uj6vjx1922 sh:class observable:URLHistoryEntry ;
	sh:nodeKind sh:IRI ;
	sh:path observable:urlHistoryEntry .

observable:URLHistoryFacet sh:property _:node1gm7uj6vjx1922 ;
	sh:targetClass observable:URLHistoryFacet .

observable:URLVisit a owl:Class , sh:NodeShape ;
	rdfs:subClassOf observable:ObservableObject ;
	rdfs:label "URLVisit"@en ;
	rdfs:comment "A URL visit characterizes the properties of a visit of a URL within a particular browser."@en ;
	sh:targetClass observable:URLVisit .

observable:URLVisitFacet a owl:Class , sh:NodeShape ;
	rdfs:subClassOf core:Facet ;
	rdfs:label "URLVisitFacet"@en ;
	rdfs:comment "A URL visit facet is a grouping of characteristics unique to the properties of a visit of a URL within a particular browser."@en .

_:node1gm7uj6vjx1923 sh:class observable:ObservableObject ;
	sh:maxCount 1 ;
	sh:nodeKind sh:IRI ;
	sh:path observable:browserInformation .

observable:URLVisitFacet sh:property _:node1gm7uj6vjx1923 .

_:node1gm7uj6vjx1924 sh:class observable:ObservableObject ;
	sh:maxCount 1 ;
	sh:nodeKind sh:IRI ;
	sh:path observable:fromURLVisit .

observable:URLVisitFacet sh:property _:node1gm7uj6vjx1924 .

_:node1gm7uj6vjx1925 sh:class observable:ObservableObject ;
	sh:maxCount 1 ;
	sh:nodeKind sh:IRI ;
	sh:path observable:url .

observable:URLVisitFacet sh:property _:node1gm7uj6vjx1925 .

_:node1gm7uj6vjx1926 sh:datatype xsd:dateTime ;
	sh:maxCount 1 ;
	sh:nodeKind sh:Literal ;
	sh:path observable:visitTime .

observable:URLVisitFacet sh:property _:node1gm7uj6vjx1926 .

_:node1gm7uj6vjx1927 sh:datatype xsd:duration ;
	sh:maxCount 1 ;
	sh:nodeKind sh:Literal ;
	sh:path observable:visitDuration .

observable:URLVisitFacet sh:property _:node1gm7uj6vjx1927 .

_:node1gm7uj6vjx1928 sh:datatype vocabulary:URLTransitionTypeVocab ;
	sh:message "Value is outside the default vocabulary URLTransitionTypeVocab." ;
	sh:path observable:urlTransitionType ;
	sh:severity sh:Info .

observable:URLVisitFacet sh:property _:node1gm7uj6vjx1928 .

_:node1gm7uj6vjx1929 sh:maxCount 1 ;
	sh:nodeKind sh:Literal .

_:node1gm7uj6vjx1931 sh:datatype vocabulary:URLTransitionTypeVocab .

_:node1gm7uj6vjx1930 rdf:first _:node1gm7uj6vjx1931 ;
	rdf:rest _:node1gm7uj6vjx1932 .

_:node1gm7uj6vjx1933 sh:datatype xsd:string .

_:node1gm7uj6vjx1932 rdf:first _:node1gm7uj6vjx1933 ;
	rdf:rest rdf:nil .

_:node1gm7uj6vjx1929 sh:or _:node1gm7uj6vjx1930 ;
	sh:path observable:urlTransitionType .

observable:URLVisitFacet sh:property _:node1gm7uj6vjx1929 .

_:node1gm7uj6vjx1934 sh:message "Value is not member of the vocabulary URLTransitionTypeVocab." .

_:node1gm7uj6vjx1936 sh:datatype vocabulary:URLTransitionTypeVocab .

_:node1gm7uj6vjx1937 rdf:first "link"^^vocabulary:URLTransitionTypeVocab ;
	rdf:rest _:node1gm7uj6vjx1938 .

_:node1gm7uj6vjx1938 rdf:first "typed"^^vocabulary:URLTransitionTypeVocab ;
	rdf:rest _:node1gm7uj6vjx1939 .

_:node1gm7uj6vjx1939 rdf:first "auto_bookmark"^^vocabulary:URLTransitionTypeVocab ;
	rdf:rest _:node1gm7uj6vjx1940 .

_:node1gm7uj6vjx1940 rdf:first "auto_subframe"^^vocabulary:URLTransitionTypeVocab ;
	rdf:rest _:node1gm7uj6vjx1941 .

_:node1gm7uj6vjx1941 rdf:first "manual_subframe"^^vocabulary:URLTransitionTypeVocab ;
	rdf:rest _:node1gm7uj6vjx1942 .

_:node1gm7uj6vjx1942 rdf:first "generated"^^vocabulary:URLTransitionTypeVocab ;
	rdf:rest _:node1gm7uj6vjx1943 .

_:node1gm7uj6vjx1943 rdf:first "auto_toplevel"^^vocabulary:URLTransitionTypeVocab ;
	rdf:rest _:node1gm7uj6vjx1944 .

_:node1gm7uj6vjx1944 rdf:first "form_submit"^^vocabulary:URLTransitionTypeVocab ;
	rdf:rest _:node1gm7uj6vjx1945 .

_:node1gm7uj6vjx1945 rdf:first "reload"^^vocabulary:URLTransitionTypeVocab ;
	rdf:rest _:node1gm7uj6vjx1946 .

_:node1gm7uj6vjx1946 rdf:first "keyword"^^vocabulary:URLTransitionTypeVocab ;
	rdf:rest _:node1gm7uj6vjx1947 .

_:node1gm7uj6vjx1947 rdf:first "keyword_generated"^^vocabulary:URLTransitionTypeVocab ;
	rdf:rest rdf:nil .

_:node1gm7uj6vjx1936 sh:in _:node1gm7uj6vjx1937 .

_:node1gm7uj6vjx1935 rdf:first _:node1gm7uj6vjx1936 ;
	rdf:rest _:node1gm7uj6vjx1948 .

_:node1gm7uj6vjx1949 sh:datatype xsd:string .

_:node1gm7uj6vjx1948 rdf:first _:node1gm7uj6vjx1949 ;
	rdf:rest rdf:nil .

_:node1gm7uj6vjx1934 sh:or _:node1gm7uj6vjx1935 ;
	sh:path observable:urlTransitionType .

observable:URLVisitFacet sh:property _:node1gm7uj6vjx1934 ;
	sh:targetClass observable:URLVisitFacet .

observable:UserAccount a owl:Class , sh:NodeShape ;
	rdfs:subClassOf observable:DigitalAccount ;
	rdfs:label "UserAccount"@en ;
	rdfs:comment "A user account is an account controlling a user's access to a network, system or platform."@en ;
	sh:targetClass observable:UserAccount .

observable:UserAccountFacet a owl:Class , sh:NodeShape ;
	rdfs:subClassOf core:Facet ;
	rdfs:label "UserAccountFacet"@en ;
	rdfs:comment "A user account facet is a grouping of characteristics unique to an account controlling a user's access to a network, system, or platform."@en .

_:node1gm7uj6vjx1950 sh:datatype xsd:boolean ;
	sh:maxCount 1 ;
	sh:nodeKind sh:Literal ;
	sh:path observable:canEscalatePrivs .

observable:UserAccountFacet sh:property _:node1gm7uj6vjx1950 .

_:node1gm7uj6vjx1951 sh:datatype xsd:boolean ;
	sh:maxCount 1 ;
	sh:nodeKind sh:Literal ;
	sh:path observable:isPrivileged .

observable:UserAccountFacet sh:property _:node1gm7uj6vjx1951 .

_:node1gm7uj6vjx1952 sh:datatype xsd:boolean ;
	sh:maxCount 1 ;
	sh:nodeKind sh:Literal ;
	sh:path observable:isServiceAccount .

observable:UserAccountFacet sh:property _:node1gm7uj6vjx1952 .

_:node1gm7uj6vjx1953 sh:datatype xsd:string ;
	sh:maxCount 1 ;
	sh:nodeKind sh:Literal ;
	sh:path observable:homeDirectory .

observable:UserAccountFacet sh:property _:node1gm7uj6vjx1953 ;
	sh:targetClass observable:UserAccountFacet .

observable:UserSession a owl:Class , sh:NodeShape ;
	rdfs:subClassOf observable:ObservableObject ;
	rdfs:label "UserSession"@en ;
	rdfs:comment "A user session is a temporary and interactive information interchange between two or more communicating devices within the managed scope of a single user. [based on https://en.wikipedia.org/wiki/Session_(computer_science)]"@en ;
	sh:targetClass observable:UserSession .

observable:UserSessionFacet a owl:Class , sh:NodeShape ;
	rdfs:subClassOf core:Facet ;
	rdfs:label "UserSessionFacet"@en ;
	rdfs:comment "A user session facet is a grouping of characteristics unique to a temporary and interactive information interchange between two or more communicating devices within the managed scope of a single user. [based on https://en.wikipedia.org/wiki/Session_(computer_science)]"@en .

_:node1gm7uj6vjx1954 sh:class observable:ObservableObject ;
	sh:maxCount 1 ;
	sh:nodeKind sh:IRI ;
	sh:path observable:effectiveUser .

observable:UserSessionFacet sh:property _:node1gm7uj6vjx1954 .

_:node1gm7uj6vjx1955 sh:datatype xsd:dateTime ;
	sh:maxCount 1 ;
	sh:nodeKind sh:Literal ;
	sh:path observable:loginTime .

observable:UserSessionFacet sh:property _:node1gm7uj6vjx1955 .

_:node1gm7uj6vjx1956 sh:datatype xsd:dateTime ;
	sh:maxCount 1 ;
	sh:nodeKind sh:Literal ;
	sh:path observable:logoutTime .

observable:UserSessionFacet sh:property _:node1gm7uj6vjx1956 .

_:node1gm7uj6vjx1957 sh:datatype xsd:string ;
	sh:maxCount 1 ;
	sh:nodeKind sh:Literal ;
	sh:path observable:effectiveGroup .

observable:UserSessionFacet sh:property _:node1gm7uj6vjx1957 .

_:node1gm7uj6vjx1958 sh:datatype xsd:string ;
	sh:maxCount 1 ;
	sh:nodeKind sh:Literal ;
	sh:path observable:effectiveGroupID .

observable:UserSessionFacet sh:property _:node1gm7uj6vjx1958 ;
	sh:targetClass observable:UserSessionFacet .

observable:ValuesEnumeratedEffectFacet a owl:Class , sh:NodeShape ;
	rdfs:subClassOf observable:DefinedEffectFacet ;
	rdfs:label "ValuesEnumeratedEffectFacet"@en ;
	rdfs:comment "A values enumerated effect facet is a grouping of characteristics unique to the effects of actions upon observable objects where a value of the observable object is enumerated. An example of this would be the values of a registry key."@en .

_:node1gm7uj6vjx1959 sh:datatype xsd:string ;
	sh:maxCount 1 ;
	sh:nodeKind sh:Literal ;
	sh:path observable:values .

observable:ValuesEnumeratedEffectFacet sh:property _:node1gm7uj6vjx1959 ;
	sh:targetClass observable:ValuesEnumeratedEffectFacet .

observable:Volume a owl:Class , sh:NodeShape ;
	rdfs:subClassOf observable:ObservableObject ;
	rdfs:label "Volume"@en ;
	rdfs:comment "A volume is a single accessible storage area (volume) with a single file system. [based on https://en.wikipedia.org/wiki/Volume_(computing)]"@en ;
	sh:targetClass observable:Volume .

observable:VolumeFacet a owl:Class , sh:NodeShape ;
	rdfs:subClassOf core:Facet ;
	rdfs:label "VolumeFacet"@en ;
	rdfs:comment "A volume facet is a grouping of characteristics unique to a single accessible storage area (volume) with a single file system. [based on https://en.wikipedia.org/wiki/Volume_(computing)]"@en .

_:node1gm7uj6vjx1960 sh:datatype xsd:integer ;
	sh:maxCount 1 ;
	sh:nodeKind sh:Literal ;
	sh:path observable:sectorSize .

observable:VolumeFacet sh:property _:node1gm7uj6vjx1960 .

_:node1gm7uj6vjx1961 sh:datatype xsd:string ;
	sh:maxCount 1 ;
	sh:nodeKind sh:Literal ;
	sh:path observable:volumeID .

observable:VolumeFacet sh:property _:node1gm7uj6vjx1961 ;
	sh:targetClass observable:VolumeFacet .

observable:WearableDevice a owl:Class , sh:NodeShape ;
	rdfs:subClassOf observable:SmartDevice ;
	rdfs:label "WearableDevice"@en-us ;
	rdfs:comment "A wearable device is an electronic device that is designed to be worn on a person's body."@en-us ;
	sh:targetClass observable:WearableDevice .

observable:WebPage a owl:Class , sh:NodeShape ;
	rdfs:subClassOf observable:ObservableObject ;
	rdfs:label "WebPage"@en ;
	rdfs:comment "A web page is a specific collection of information provided by a website and displayed to a user in a web browser. A website typically consists of many web pages linked together in a coherent fashion. [based on https://en.wikipedia.org/wiki/Web_page]"@en ;
	sh:targetClass observable:WebPage .

observable:WhoIs a owl:Class , sh:NodeShape ;
	rdfs:subClassOf observable:ObservableObject ;
	rdfs:label "WhoIs"@en ;
	rdfs:comment "WhoIs is a response record conformant to the WHOIS protocol standard (RFC 3912). [based on https://en.wikipedia.org/wiki/WHOIS]"@en ;
	sh:targetClass observable:WhoIs .

observable:WhoIsFacet a owl:Class , sh:NodeShape ;
	rdfs:subClassOf core:Facet ;
	rdfs:label "WhoIsFacet"@en ;
	rdfs:comment "A whois facet is a grouping of characteristics unique to a response record conformant to the WHOIS protocol standard (RFC 3912). [based on https://en.wikipedia.org/wiki/WHOIS]"@en ;
	sh:property observable:regionalInternetRegistry-shape-value-not-vocabulary-member , observable:regionalInternetRegistry-shape-value-outside-default-vocabulary .

_:node1gm7uj6vjx1962 sh:class observable:ObservableObject ;
	sh:maxCount 1 ;
	sh:nodeKind sh:IRI ;
	sh:path observable:domainName .

observable:WhoIsFacet sh:property _:node1gm7uj6vjx1962 .

_:node1gm7uj6vjx1963 sh:class observable:ObservableObject ;
	sh:maxCount 1 ;
	sh:nodeKind sh:IRI ;
	sh:path observable:ipAddress .

observable:WhoIsFacet sh:property _:node1gm7uj6vjx1963 .

_:node1gm7uj6vjx1964 sh:class observable:ObservableObject ;
	sh:maxCount 1 ;
	sh:nodeKind sh:IRI ;
	sh:path observable:registrantContactInfo .

observable:WhoIsFacet sh:property _:node1gm7uj6vjx1964 .

_:node1gm7uj6vjx1965 sh:class observable:ObservableObject ;
	sh:maxCount 1 ;
	sh:nodeKind sh:IRI ;
	sh:path observable:serverName .

observable:WhoIsFacet sh:property _:node1gm7uj6vjx1965 .

_:node1gm7uj6vjx1966 sh:class observable:ObservableObject ;
	sh:nodeKind sh:IRI ;
	sh:path observable:nameServer .

observable:WhoIsFacet sh:property _:node1gm7uj6vjx1966 .

_:node1gm7uj6vjx1967 sh:class observable:WhoisRegistrarInfoType ;
	sh:maxCount 1 ;
	sh:nodeKind sh:IRI ;
	sh:path observable:registrarInfo .

observable:WhoIsFacet sh:property _:node1gm7uj6vjx1967 .

_:node1gm7uj6vjx1968 sh:datatype xsd:dateTime ;
	sh:maxCount 1 ;
	sh:nodeKind sh:Literal ;
	sh:path observable:creationDate .

observable:WhoIsFacet sh:property _:node1gm7uj6vjx1968 .

_:node1gm7uj6vjx1969 sh:datatype xsd:dateTime ;
	sh:maxCount 1 ;
	sh:nodeKind sh:Literal ;
	sh:path observable:expirationDate .

observable:WhoIsFacet sh:property _:node1gm7uj6vjx1969 .

_:node1gm7uj6vjx1970 sh:datatype xsd:dateTime ;
	sh:maxCount 1 ;
	sh:nodeKind sh:Literal ;
	sh:path observable:lookupDate .

observable:WhoIsFacet sh:property _:node1gm7uj6vjx1970 .

_:node1gm7uj6vjx1971 sh:datatype xsd:dateTime ;
	sh:maxCount 1 ;
	sh:nodeKind sh:Literal ;
	sh:path observable:updatedDate .

observable:WhoIsFacet sh:property _:node1gm7uj6vjx1971 .

_:node1gm7uj6vjx1972 sh:datatype xsd:string ;
	sh:maxCount 1 ;
	sh:nodeKind sh:Literal ;
	sh:path observable:domainID .

observable:WhoIsFacet sh:property _:node1gm7uj6vjx1972 .

_:node1gm7uj6vjx1973 sh:datatype xsd:string ;
	sh:maxCount 1 ;
	sh:nodeKind sh:Literal ;
	sh:path observable:remarks .

observable:WhoIsFacet sh:property _:node1gm7uj6vjx1973 .

_:node1gm7uj6vjx1974 sh:datatype xsd:string ;
	sh:maxCount 1 ;
	sh:nodeKind sh:Literal ;
	sh:path observable:sponsoringRegistrar .

observable:WhoIsFacet sh:property _:node1gm7uj6vjx1974 .

_:node1gm7uj6vjx1975 sh:datatype xsd:string ;
	sh:nodeKind sh:Literal ;
	sh:path observable:registrantIDs .

observable:WhoIsFacet sh:property _:node1gm7uj6vjx1975 .

_:node1gm7uj6vjx1976 sh:datatype vocabulary:WhoisDNSSECTypeVocab ;
	sh:maxCount 1 ;
	sh:nodeKind sh:Literal ;
	sh:path observable:dnssec .

observable:WhoIsFacet sh:property _:node1gm7uj6vjx1976 .

_:node1gm7uj6vjx1977 sh:datatype vocabulary:WhoisStatusTypeVocab ;
	sh:message "Value is outside the default vocabulary WhoisStatusTypeVocab." ;
	sh:path observable:status ;
	sh:severity sh:Info .

observable:WhoIsFacet sh:property _:node1gm7uj6vjx1977 .

_:node1gm7uj6vjx1978 sh:maxCount 1 ;
	sh:nodeKind sh:Literal .

_:node1gm7uj6vjx1980 sh:datatype vocabulary:RegionalRegistryTypeVocab .

_:node1gm7uj6vjx1979 rdf:first _:node1gm7uj6vjx1980 ;
	rdf:rest _:node1gm7uj6vjx1981 .

_:node1gm7uj6vjx1982 sh:datatype xsd:string .

_:node1gm7uj6vjx1981 rdf:first _:node1gm7uj6vjx1982 ;
	rdf:rest rdf:nil .

_:node1gm7uj6vjx1978 sh:or _:node1gm7uj6vjx1979 ;
	sh:path observable:regionalInternetRegistry .

observable:WhoIsFacet sh:property _:node1gm7uj6vjx1978 .

_:node1gm7uj6vjx1983 sh:maxCount 1 ;
	sh:nodeKind sh:Literal .

_:node1gm7uj6vjx1985 sh:datatype vocabulary:WhoisStatusTypeVocab .

_:node1gm7uj6vjx1984 rdf:first _:node1gm7uj6vjx1985 ;
	rdf:rest _:node1gm7uj6vjx1986 .

_:node1gm7uj6vjx1987 sh:datatype xsd:string .

_:node1gm7uj6vjx1986 rdf:first _:node1gm7uj6vjx1987 ;
	rdf:rest rdf:nil .

_:node1gm7uj6vjx1983 sh:or _:node1gm7uj6vjx1984 ;
	sh:path observable:status .

observable:WhoIsFacet sh:property _:node1gm7uj6vjx1983 .

_:node1gm7uj6vjx1988 sh:message "Value is not member of the vocabulary WhoisStatusTypeVocab." .

_:node1gm7uj6vjx1990 sh:datatype vocabulary:WhoisStatusTypeVocab .

_:node1gm7uj6vjx1991 rdf:first "ADD_PERIOD"^^vocabulary:WhoisStatusTypeVocab ;
	rdf:rest _:node1gm7uj6vjx1992 .

_:node1gm7uj6vjx1992 rdf:first "AUTO_RENEW_PERIOD"^^vocabulary:WhoisStatusTypeVocab ;
	rdf:rest _:node1gm7uj6vjx1993 .

_:node1gm7uj6vjx1993 rdf:first "CLIENT_DELETE_PROHIBITED"^^vocabulary:WhoisStatusTypeVocab ;
	rdf:rest _:node1gm7uj6vjx1994 .

_:node1gm7uj6vjx1994 rdf:first "CLIENT_HOLD"^^vocabulary:WhoisStatusTypeVocab ;
	rdf:rest _:node1gm7uj6vjx1995 .

_:node1gm7uj6vjx1995 rdf:first "CLIENT_RENEW_PROHIBITED"^^vocabulary:WhoisStatusTypeVocab ;
	rdf:rest _:node1gm7uj6vjx1996 .

_:node1gm7uj6vjx1996 rdf:first "CLIENT_TRANSFER_PROHIBITED"^^vocabulary:WhoisStatusTypeVocab ;
	rdf:rest _:node1gm7uj6vjx1997 .

_:node1gm7uj6vjx1997 rdf:first "CLIENT_UPDATE_PROHIBITED"^^vocabulary:WhoisStatusTypeVocab ;
	rdf:rest _:node1gm7uj6vjx1998 .

_:node1gm7uj6vjx1998 rdf:first "DELETE_PROHIBITED"^^vocabulary:WhoisStatusTypeVocab ;
	rdf:rest _:node1gm7uj6vjx1999 .

_:node1gm7uj6vjx1999 rdf:first "HOLD"^^vocabulary:WhoisStatusTypeVocab ;
	rdf:rest _:node1gm7uj6vjx2000 .

_:node1gm7uj6vjx2000 rdf:first "INACTIVE"^^vocabulary:WhoisStatusTypeVocab ;
	rdf:rest _:node1gm7uj6vjx2001 .

_:node1gm7uj6vjx2001 rdf:first "OK"^^vocabulary:WhoisStatusTypeVocab ;
	rdf:rest _:node1gm7uj6vjx2002 .

_:node1gm7uj6vjx2002 rdf:first "PENDING_DELETE_RESTORABLE"^^vocabulary:WhoisStatusTypeVocab ;
	rdf:rest _:node1gm7uj6vjx2003 .

_:node1gm7uj6vjx2003 rdf:first "PENDING_DELETE_SCHEDULED_FOR_RELEASE"^^vocabulary:WhoisStatusTypeVocab ;
	rdf:rest _:node1gm7uj6vjx2004 .

_:node1gm7uj6vjx2004 rdf:first "PENDING_RESTORE"^^vocabulary:WhoisStatusTypeVocab ;
	rdf:rest _:node1gm7uj6vjx2005 .

_:node1gm7uj6vjx2005 rdf:first "RENEW_PERIOD"^^vocabulary:WhoisStatusTypeVocab ;
	rdf:rest _:node1gm7uj6vjx2006 .

_:node1gm7uj6vjx2006 rdf:first "RENEW_PROHIBITED"^^vocabulary:WhoisStatusTypeVocab ;
	rdf:rest _:node1gm7uj6vjx2007 .

_:node1gm7uj6vjx2007 rdf:first "TRANSFER_PERIOD"^^vocabulary:WhoisStatusTypeVocab ;
	rdf:rest _:node1gm7uj6vjx2008 .

_:node1gm7uj6vjx2008 rdf:first "TRANSFER_PROHIBITED"^^vocabulary:WhoisStatusTypeVocab ;
	rdf:rest _:node1gm7uj6vjx2009 .

_:node1gm7uj6vjx2009 rdf:first "UPDATE_PROHIBITED"^^vocabulary:WhoisStatusTypeVocab ;
	rdf:rest rdf:nil .

_:node1gm7uj6vjx1990 sh:in _:node1gm7uj6vjx1991 .

_:node1gm7uj6vjx1989 rdf:first _:node1gm7uj6vjx1990 ;
	rdf:rest _:node1gm7uj6vjx2010 .

_:node1gm7uj6vjx2011 sh:datatype xsd:string .

_:node1gm7uj6vjx2010 rdf:first _:node1gm7uj6vjx2011 ;
	rdf:rest rdf:nil .

_:node1gm7uj6vjx1988 sh:or _:node1gm7uj6vjx1989 ;
	sh:path observable:status .

observable:WhoIsFacet sh:property _:node1gm7uj6vjx1988 ;
	sh:targetClass observable:WhoIsFacet .

observable:WhoisContactFacet a owl:Class , sh:NodeShape ;
	rdfs:subClassOf observable:ContactFacet ;
	rdfs:label "WhoIsContactFacet"@en ;
	rdfs:comment "A Whois contact type is a grouping of characteristics unique to contact-related information present in a response record conformant to the WHOIS protocol standard (RFC 3912). [based on https://en.wikipedia.org/wiki/WHOIS]"@en .

_:node1gm7uj6vjx2012 sh:datatype vocabulary:WhoisContactTypeVocab ;
	sh:message "Value is outside the default vocabulary WhoisContactTypeVocab." ;
	sh:path observable:whoisContactType ;
	sh:severity sh:Info .

observable:WhoisContactFacet sh:property _:node1gm7uj6vjx2012 .

_:node1gm7uj6vjx2013 sh:maxCount 1 ;
	sh:nodeKind sh:Literal .

_:node1gm7uj6vjx2015 sh:datatype vocabulary:WhoisContactTypeVocab .

_:node1gm7uj6vjx2014 rdf:first _:node1gm7uj6vjx2015 ;
	rdf:rest _:node1gm7uj6vjx2016 .

_:node1gm7uj6vjx2017 sh:datatype xsd:string .

_:node1gm7uj6vjx2016 rdf:first _:node1gm7uj6vjx2017 ;
	rdf:rest rdf:nil .

_:node1gm7uj6vjx2013 sh:or _:node1gm7uj6vjx2014 ;
	sh:path observable:whoisContactType .

observable:WhoisContactFacet sh:property _:node1gm7uj6vjx2013 .

_:node1gm7uj6vjx2018 sh:message "Value is not member of the vocabulary WhoisContactTypeVocab." .

_:node1gm7uj6vjx2020 sh:datatype vocabulary:WhoisContactTypeVocab .

_:node1gm7uj6vjx2021 rdf:first "ADMIN"^^vocabulary:WhoisContactTypeVocab ;
	rdf:rest _:node1gm7uj6vjx2022 .

_:node1gm7uj6vjx2022 rdf:first "BILLING"^^vocabulary:WhoisContactTypeVocab ;
	rdf:rest _:node1gm7uj6vjx2023 .

_:node1gm7uj6vjx2023 rdf:first "TECHNICAL"^^vocabulary:WhoisContactTypeVocab ;
	rdf:rest rdf:nil .

_:node1gm7uj6vjx2020 sh:in _:node1gm7uj6vjx2021 .

_:node1gm7uj6vjx2019 rdf:first _:node1gm7uj6vjx2020 ;
	rdf:rest _:node1gm7uj6vjx2024 .

_:node1gm7uj6vjx2025 sh:datatype xsd:string .

_:node1gm7uj6vjx2024 rdf:first _:node1gm7uj6vjx2025 ;
	rdf:rest rdf:nil .

_:node1gm7uj6vjx2018 sh:or _:node1gm7uj6vjx2019 ;
	sh:path observable:whoisContactType .

observable:WhoisContactFacet sh:property _:node1gm7uj6vjx2018 ;
	sh:targetClass observable:WhoisContactFacet .

observable:WhoisRegistrarInfoType a owl:Class , sh:NodeShape ;
	rdfs:subClassOf core:UcoInherentCharacterizationThing ;
	rdfs:label "WhoisRegistrarInfoType"@en ;
	rdfs:comment "A Whois registrar info type is a grouping of characteristics unique to registrar-related information present in a response record conformant to the WHOIS protocol standard (RFC 3912). [based on https://en.wikipedia.org/wiki/WHOIS]"@en .

_:node1gm7uj6vjx2026 sh:class location:Location ;
	sh:maxCount 1 ;
	sh:nodeKind sh:IRI ;
	sh:path observable:geolocationAddress .

observable:WhoisRegistrarInfoType sh:property _:node1gm7uj6vjx2026 .

_:node1gm7uj6vjx2027 sh:class observable:ObservableObject ;
	sh:maxCount 1 ;
	sh:nodeKind sh:IRI ;
	sh:path observable:contactPhoneNumber .

observable:WhoisRegistrarInfoType sh:property _:node1gm7uj6vjx2027 .

_:node1gm7uj6vjx2028 sh:class observable:ObservableObject ;
	sh:maxCount 1 ;
	sh:nodeKind sh:IRI ;
	sh:path observable:emailAddress .

observable:WhoisRegistrarInfoType sh:property _:node1gm7uj6vjx2028 .

_:node1gm7uj6vjx2029 sh:class observable:ObservableObject ;
	sh:maxCount 1 ;
	sh:nodeKind sh:IRI ;
	sh:path observable:referralURL .

observable:WhoisRegistrarInfoType sh:property _:node1gm7uj6vjx2029 .

_:node1gm7uj6vjx2030 sh:class observable:ObservableObject ;
	sh:maxCount 1 ;
	sh:nodeKind sh:IRI ;
	sh:path observable:whoisServer .

observable:WhoisRegistrarInfoType sh:property _:node1gm7uj6vjx2030 .

_:node1gm7uj6vjx2031 sh:datatype xsd:string ;
	sh:maxCount 1 ;
	sh:nodeKind sh:Literal ;
	sh:path observable:registrarGUID .

observable:WhoisRegistrarInfoType sh:property _:node1gm7uj6vjx2031 .

_:node1gm7uj6vjx2032 sh:datatype xsd:string ;
	sh:maxCount 1 ;
	sh:nodeKind sh:Literal ;
	sh:path observable:registrarID .

observable:WhoisRegistrarInfoType sh:property _:node1gm7uj6vjx2032 .

_:node1gm7uj6vjx2033 sh:datatype xsd:string ;
	sh:maxCount 1 ;
	sh:nodeKind sh:Literal ;
	sh:path observable:registrarName .

observable:WhoisRegistrarInfoType sh:property _:node1gm7uj6vjx2033 ;
	sh:targetClass observable:WhoisRegistrarInfoType .

observable:WifiAddress a owl:Class , sh:NodeShape ;
	rdfs:subClassOf observable:MACAddress ;
	rdfs:label "WifiAddress"@en ;
	rdfs:comment "A Wi-Fi address is a media access control (MAC) standards-conformant identifier assigned to a device network interface to enable routing and management of IEEE 802.11 standards-conformant communications to and from that device."@en ;
	sh:targetClass observable:WifiAddress .

observable:WifiAddressFacet a owl:Class , sh:NodeShape ;
	rdfs:subClassOf observable:MACAddressFacet ;
	rdfs:label "WifiAddressFacet"@en ;
	rdfs:comment "A Wi-Fi address facet is a grouping of characteristics unique to a media access control (MAC) standards conformant identifier assigned to a device network interface to enable routing and management of IEEE 802.11 standards-conformant communications to and from that device."@en ;
	sh:targetClass observable:WifiAddressFacet .

observable:Wiki a owl:Class , sh:NodeShape ;
	rdfs:subClassOf observable:ObservableObject ;
	rdfs:label "Wiki"@en ;
	rdfs:comment "A wiki is an online hypertext publication collaboratively edited and managed by its own audience directly using a web browser. A typical wiki contains multiple pages/articles for the subjects or scope of the project and could be either open to the public or limited to use within an organization for maintaining its internal knowledge base. [based on https://en.wikipedia.org/wiki/Wiki]"@en ;
	sh:targetClass observable:Wiki .

observable:WikiArticle a owl:Class , sh:NodeShape ;
	rdfs:subClassOf observable:ObservableObject ;
	rdfs:label "WikiArticle"@en ;
	rdfs:comment "A wiki article is one or more pages in a wiki focused on characterizing a particular topic."@en ;
	sh:targetClass observable:WikiArticle .

observable:WindowsAccount a owl:Class , sh:NodeShape ;
	rdfs:subClassOf observable:DigitalAccount ;
	rdfs:label "WindowsAccount"@en ;
	rdfs:comment "A Windows account is a user account on a Windows operating system."@en ;
	sh:targetClass observable:WindowsAccount .

observable:WindowsAccountFacet a owl:Class , sh:NodeShape ;
	rdfs:subClassOf core:Facet ;
	rdfs:label "WindowsAccountFacet"@en ;
	rdfs:comment "A Windows account facet is a grouping of characteristics unique to a user account on a Windows operating system."@en .

_:node1gm7uj6vjx2034 sh:datatype xsd:string ;
	sh:nodeKind sh:Literal ;
	sh:path observable:groups .

observable:WindowsAccountFacet sh:property _:node1gm7uj6vjx2034 ;
	sh:targetClass observable:WindowsAccountFacet .

observable:WindowsActiveDirectoryAccount a owl:Class , sh:NodeShape ;
	rdfs:subClassOf observable:DigitalAccount ;
	rdfs:label "WindowsActiveDirectoryAccount"@en ;
	rdfs:comment "A Windows Active Directory account is an account managed by directory-based identity-related services of a Windows operating system."@en ;
	sh:targetClass observable:WindowsActiveDirectoryAccount .

observable:WindowsActiveDirectoryAccountFacet a owl:Class , sh:NodeShape ;
	rdfs:subClassOf core:Facet ;
	rdfs:label "WindowsActiveDirectoryAccountFacet"@en ;
	rdfs:comment "A Windows Active Directory account facet is a grouping of characteristics unique to an account managed by directory-based identity-related services of a Windows operating system."@en .

_:node1gm7uj6vjx2035 sh:datatype xsd:string ;
	sh:maxCount 1 ;
	sh:nodeKind sh:Literal ;
	sh:path observable:objectGUID .

observable:WindowsActiveDirectoryAccountFacet sh:property _:node1gm7uj6vjx2035 .

_:node1gm7uj6vjx2036 sh:datatype xsd:string ;
	sh:nodeKind sh:Literal ;
	sh:path observable:activeDirectoryGroups .

observable:WindowsActiveDirectoryAccountFacet sh:property _:node1gm7uj6vjx2036 ;
	sh:targetClass observable:WindowsActiveDirectoryAccountFacet .

observable:WindowsComputerSpecification a owl:Class , sh:NodeShape ;
	rdfs:subClassOf observable:ObservableObject ;
	rdfs:label "WindowsComputerSpecification"@en ;
	rdfs:comment "A Windows computer specification is the hardware ans software of a programmable electronic device that can store, retrieve, and process data running a Microsoft Windows operating system. [based on merriam-webster.com/dictionary/computer]"@en ;
	sh:targetClass observable:WindowsComputerSpecification .

observable:WindowsComputerSpecificationFacet a owl:Class , sh:NodeShape ;
	rdfs:subClassOf core:Facet ;
	rdfs:label "WindowsComputerSpecificationFacet"@en ;
	rdfs:comment "A Windows computer specification facet is a grouping of characteristics unique to the hardware and software of a programmable electronic device that can store, retrieve, and process data running a Microsoft Windows operating system. [based on merriam-webster.com/dictionary/computer]"@en .

_:node1gm7uj6vjx2037 sh:class identity:Identity ;
	sh:maxCount 1 ;
	sh:nodeKind sh:IRI ;
	sh:path observable:registeredOrganization .

observable:WindowsComputerSpecificationFacet sh:property _:node1gm7uj6vjx2037 .

_:node1gm7uj6vjx2038 sh:class identity:Identity ;
	sh:maxCount 1 ;
	sh:nodeKind sh:IRI ;
	sh:path observable:registeredOwner .

observable:WindowsComputerSpecificationFacet sh:property _:node1gm7uj6vjx2038 .

_:node1gm7uj6vjx2039 sh:class observable:GlobalFlagType ;
	sh:nodeKind sh:IRI ;
	sh:path observable:globalFlagList .

observable:WindowsComputerSpecificationFacet sh:property _:node1gm7uj6vjx2039 .

_:node1gm7uj6vjx2040 sh:class observable:ObservableObject ;
	sh:maxCount 1 ;
	sh:nodeKind sh:IRI ;
	sh:path observable:windowsDirectory .

observable:WindowsComputerSpecificationFacet sh:property _:node1gm7uj6vjx2040 .

_:node1gm7uj6vjx2041 sh:class observable:ObservableObject ;
	sh:maxCount 1 ;
	sh:nodeKind sh:IRI ;
	sh:path observable:windowsSystemDirectory .

observable:WindowsComputerSpecificationFacet sh:property _:node1gm7uj6vjx2041 .

_:node1gm7uj6vjx2042 sh:class observable:ObservableObject ;
	sh:maxCount 1 ;
	sh:nodeKind sh:IRI ;
	sh:path observable:windowsTempDirectory .

observable:WindowsComputerSpecificationFacet sh:property _:node1gm7uj6vjx2042 .

_:node1gm7uj6vjx2043 sh:datatype xsd:dateTime ;
	sh:maxCount 1 ;
	sh:nodeKind sh:Literal ;
	sh:path observable:lastShutdownDate .

observable:WindowsComputerSpecificationFacet sh:property _:node1gm7uj6vjx2043 .

_:node1gm7uj6vjx2044 sh:datatype xsd:dateTime ;
	sh:maxCount 1 ;
	sh:nodeKind sh:Literal ;
	sh:path observable:osInstallDate .

observable:WindowsComputerSpecificationFacet sh:property _:node1gm7uj6vjx2044 .

_:node1gm7uj6vjx2045 sh:datatype xsd:dateTime ;
	sh:maxCount 1 ;
	sh:nodeKind sh:Literal ;
	sh:path observable:osLastUpgradeDate .

observable:WindowsComputerSpecificationFacet sh:property _:node1gm7uj6vjx2045 .

_:node1gm7uj6vjx2046 sh:datatype xsd:string ;
	sh:maxCount 1 ;
	sh:nodeKind sh:Literal ;
	sh:path observable:msProductID .

observable:WindowsComputerSpecificationFacet sh:property _:node1gm7uj6vjx2046 .

_:node1gm7uj6vjx2047 sh:datatype xsd:string ;
	sh:maxCount 1 ;
	sh:nodeKind sh:Literal ;
	sh:path observable:msProductName .

observable:WindowsComputerSpecificationFacet sh:property _:node1gm7uj6vjx2047 .

_:node1gm7uj6vjx2048 sh:datatype xsd:string ;
	sh:maxCount 1 ;
	sh:nodeKind sh:Literal ;
	sh:path observable:netBIOSName .

observable:WindowsComputerSpecificationFacet sh:property _:node1gm7uj6vjx2048 .

_:node1gm7uj6vjx2049 sh:datatype xsd:string ;
	sh:nodeKind sh:Literal ;
	sh:path observable:domain .

observable:WindowsComputerSpecificationFacet sh:property _:node1gm7uj6vjx2049 ;
	sh:targetClass observable:WindowsComputerSpecificationFacet .

observable:WindowsCriticalSection a owl:Class , sh:NodeShape ;
	rdfs:subClassOf observable:ObservableObject ;
	rdfs:label "WindowsCriticalSection"@en ;
	rdfs:comment "A Windows critical section is a Windows object that provides synchronization similar to that provided by a mutex object, except that a critical section can be used only by the threads of a single process. Critical section objects cannot be shared across processes. Event, mutex, and semaphore objects can also be used in a single-process application, but critical section objects provide a slightly faster, more efficient mechanism for mutual-exclusion synchronization (a processor-specific test and set instruction). Like a mutex object, a critical section object can be owned by only one thread at a time, which makes it useful for protecting a shared resource from simultaneous access. Unlike a mutex object, there is no way to tell whether a critical section has been abandoned. [based on https://docs.microsoft.com/en-us/windows/win32/sync/critical-section-objects]"@en ;
	sh:targetClass observable:WindowsCriticalSection .

observable:WindowsEvent a owl:Class , sh:NodeShape ;
	rdfs:subClassOf observable:ObservableObject ;
	rdfs:label "WindowsEvent"@en ;
	rdfs:comment "A Windows event is a notification record of an occurance of interest (system, security, application, etc.) on a Windows operating system."@en ;
	sh:targetClass observable:WindowsEvent .

observable:WindowsFilemapping a owl:Class , sh:NodeShape ;
	rdfs:subClassOf observable:ObservableObject ;
	rdfs:label "WindowsFilemapping"@en ;
	rdfs:comment "A Windows file mapping is the association of a file's contents with a portion of the virtual address space of a process within a Windows operating system. The system creates a file mapping object (also known as a section object) to maintain this association. A file view is the portion of virtual address space that a process uses to access the file's contents. File mapping allows the process to use both random input and output (I/O) and sequential I/O. It also allows the process to work efficiently with a large data file, such as a database, without having to map the whole file into memory. Multiple processes can also use memory-mapped files to share data. Processes read from and write to the file view using pointers, just as they would with dynamically allocated memory. The use of file mapping improves efficiency because the file resides on disk, but the file view resides in memory.[based on https://docs.microsoft.com/en-us/windows/win32/memory/file-mapping]"@en ;
	sh:targetClass observable:WindowsFilemapping .

observable:WindowsHandle a owl:Class , sh:NodeShape ;
	rdfs:subClassOf observable:ObservableObject ;
	rdfs:label "WindowsHandle"@en ;
	rdfs:comment "A Windows handle is an abstract reference to a resource within the Windows operating system, such as a window, memory, an open file or a pipe. It is the mechanism by which applications interact with such resources in the Windows operating system."@en ;
	sh:targetClass observable:WindowsHandle .

observable:WindowsHook a owl:Class , sh:NodeShape ;
	rdfs:subClassOf observable:ObservableObject ;
	rdfs:label "WindowsHook"@en ;
	rdfs:comment "A Windows hook is a mechanism by which an application can intercept events, such as messages, mouse actions, and keystrokes within the Windows operating system. A function that intercepts a particular type of event is known as a hook procedure. A hook procedure can act on each event it receives, and then modify or discard the event. [based on https://docs.microsoft.com/en-us/windows/win32/winmsg/about-hooks]"@en ;
	sh:targetClass observable:WindowsHook .

observable:WindowsMailslot a owl:Class , sh:NodeShape ;
	rdfs:subClassOf observable:ObservableObject ;
	rdfs:label "WindowsMailslot"@en ;
	rdfs:comment "A Windows mailslot is is a pseudofile that resides in memory, and may be accessed using standard file functions. The data in a mailslot message can be in any form, but cannot be larger than 424 bytes when sent between computers. Unlike disk files, mailslots are temporary. When all handles to a mailslot are closed, the mailslot and all the data it contains are deleted. [based on https://docs.microsoft.com/en-us/windows/win32/ipc/about-mailslots]"@en ;
	sh:targetClass observable:WindowsMailslot .

observable:WindowsNetworkShare a owl:Class , sh:NodeShape ;
	rdfs:subClassOf observable:ObservableObject ;
	rdfs:label "WindowsNetworkShare"@en ;
	rdfs:comment "A Windows network share is a Windows computer resource made available from one host to other hosts on a computer network. It is a device or piece of information on a computer that can be remotely accessed from another computer transparently as if it were a resource in the local machine. Network sharing is made possible by inter-process communication over the network. [based on https://en.wikipedia.org/wiki/Shared_resource]"@en ;
	sh:targetClass observable:WindowsNetworkShare .

observable:WindowsPEBinaryFile a owl:Class , sh:NodeShape ;
	rdfs:subClassOf observable:File ;
	rdfs:label "WindowsPEBinaryFile"@en ;
	rdfs:comment "A Windows PE binary file is a Windows portable executable (PE) file."@en ;
	sh:targetClass observable:WindowsPEBinaryFile .

observable:WindowsPEBinaryFileFacet a owl:Class , sh:NodeShape ;
	rdfs:subClassOf core:Facet ;
	rdfs:label "WindowsPEBinaryFileFacet"@en ;
	rdfs:comment "A Windows PE binary file facet is a grouping of characteristics unique to a Windows portable executable (PE) file."@en .

_:node1gm7uj6vjx2050 sh:class observable:WindowsPEOptionalHeader ;
	sh:maxCount 1 ;
	sh:nodeKind sh:IRI ;
	sh:path observable:optionalHeader .

observable:WindowsPEBinaryFileFacet sh:property _:node1gm7uj6vjx2050 .

_:node1gm7uj6vjx2051 sh:class observable:WindowsPESection ;
	sh:nodeKind sh:IRI ;
	sh:path observable:sections .

observable:WindowsPEBinaryFileFacet sh:property _:node1gm7uj6vjx2051 .

_:node1gm7uj6vjx2052 sh:class types:Hash ;
	sh:nodeKind sh:IRI ;
	sh:path observable:fileHeaderHashes .

observable:WindowsPEBinaryFileFacet sh:property _:node1gm7uj6vjx2052 .

_:node1gm7uj6vjx2053 sh:datatype xsd:dateTime ;
	sh:maxCount 1 ;
	sh:nodeKind sh:Literal ;
	sh:path observable:timeDateStamp .

observable:WindowsPEBinaryFileFacet sh:property _:node1gm7uj6vjx2053 .

_:node1gm7uj6vjx2054 sh:datatype xsd:hexBinary ;
	sh:nodeKind sh:Literal ;
	sh:path observable:pointerToSymbolTable .

observable:WindowsPEBinaryFileFacet sh:property _:node1gm7uj6vjx2054 .

_:node1gm7uj6vjx2055 sh:datatype xsd:integer ;
	sh:maxCount 1 ;
	sh:nodeKind sh:Literal ;
	sh:path observable:numberOfSections .

observable:WindowsPEBinaryFileFacet sh:property _:node1gm7uj6vjx2055 .

_:node1gm7uj6vjx2056 sh:datatype xsd:integer ;
	sh:maxCount 1 ;
	sh:nodeKind sh:Literal ;
	sh:path observable:numberOfSymbols .

observable:WindowsPEBinaryFileFacet sh:property _:node1gm7uj6vjx2056 .

_:node1gm7uj6vjx2057 sh:datatype xsd:integer ;
	sh:maxCount 1 ;
	sh:nodeKind sh:Literal ;
	sh:path observable:sizeOfOptionalHeader .

observable:WindowsPEBinaryFileFacet sh:property _:node1gm7uj6vjx2057 .

_:node1gm7uj6vjx2058 sh:datatype xsd:string ;
	sh:maxCount 1 ;
	sh:nodeKind sh:Literal ;
	sh:path observable:impHash .

observable:WindowsPEBinaryFileFacet sh:property _:node1gm7uj6vjx2058 .

_:node1gm7uj6vjx2059 sh:datatype xsd:string ;
	sh:maxCount 1 ;
	sh:nodeKind sh:Literal ;
	sh:path observable:peType .

observable:WindowsPEBinaryFileFacet sh:property _:node1gm7uj6vjx2059 .

_:node1gm7uj6vjx2060 sh:datatype xsd:string ;
	sh:nodeKind sh:Literal ;
	sh:path observable:machine .

observable:WindowsPEBinaryFileFacet sh:property _:node1gm7uj6vjx2060 .

_:node1gm7uj6vjx2061 sh:datatype xsd:unsignedShort ;
	sh:nodeKind sh:Literal ;
	sh:path observable:characteristics .

observable:WindowsPEBinaryFileFacet sh:property _:node1gm7uj6vjx2061 ;
	sh:targetClass observable:WindowsPEBinaryFileFacet .

observable:WindowsPEBinaryType a rdfs:Datatype .

_:node1gm7uj6vjx2062 a rdfs:Datatype .

_:node1gm7uj6vjx2063 rdf:first "dll" ;
	rdf:rest _:node1gm7uj6vjx2064 .

_:node1gm7uj6vjx2064 rdf:first "exe" ;
	rdf:rest _:node1gm7uj6vjx2065 .

_:node1gm7uj6vjx2065 rdf:first "sys" ;
	rdf:rest rdf:nil .

_:node1gm7uj6vjx2062 owl:oneOf _:node1gm7uj6vjx2063 .

observable:WindowsPEBinaryType owl:equivalentClass _:node1gm7uj6vjx2062 .

observable:WindowsPEFileHeader a owl:Class , sh:NodeShape ;
	rdfs:subClassOf core:UcoInherentCharacterizationThing ;
	rdfs:label "WindowsPEFileHeader"@en ;
	rdfs:comment "A Windows PE file header is a grouping of characteristics unique to the 'header' of a Windows PE (Portable Executable) file, consisting of a collection of metadata about the overall nature and structure of the file."@en .

_:node1gm7uj6vjx2066 sh:datatype xsd:dateTime ;
	sh:maxCount 1 ;
	sh:nodeKind sh:Literal ;
	sh:path observable:timeDateStamp .

observable:WindowsPEFileHeader sh:property _:node1gm7uj6vjx2066 ;
	sh:targetClass observable:WindowsPEFileHeader .

observable:WindowsPEOptionalHeader a owl:Class , sh:NodeShape ;
	rdfs:subClassOf core:UcoInherentCharacterizationThing ;
	rdfs:label "WindowsPEOptionalHeader"@en ;
	rdfs:comment "A Windows PE optional header is a grouping of characteristics unique to the 'optional header' of a Windows PE (Portable Executable) file, consisting of a collection of metadata about the executable code structure of the file."@en .

_:node1gm7uj6vjx2067 sh:datatype xsd:byte ;
	sh:nodeKind sh:Literal ;
	sh:path observable:majorLinkerVersion .

observable:WindowsPEOptionalHeader sh:property _:node1gm7uj6vjx2067 .

_:node1gm7uj6vjx2068 sh:datatype xsd:byte ;
	sh:nodeKind sh:Literal ;
	sh:path observable:minorLinkerVersion .

observable:WindowsPEOptionalHeader sh:property _:node1gm7uj6vjx2068 .

_:node1gm7uj6vjx2069 sh:datatype xsd:unsignedInt ;
	sh:nodeKind sh:Literal ;
	sh:path observable:addressOfEntryPoint .

observable:WindowsPEOptionalHeader sh:property _:node1gm7uj6vjx2069 .

_:node1gm7uj6vjx2070 sh:datatype xsd:unsignedInt ;
	sh:nodeKind sh:Literal ;
	sh:path observable:baseOfCode .

observable:WindowsPEOptionalHeader sh:property _:node1gm7uj6vjx2070 .

_:node1gm7uj6vjx2071 sh:datatype xsd:unsignedInt ;
	sh:nodeKind sh:Literal ;
	sh:path observable:checksum .

observable:WindowsPEOptionalHeader sh:property _:node1gm7uj6vjx2071 .

_:node1gm7uj6vjx2072 sh:datatype xsd:unsignedInt ;
	sh:nodeKind sh:Literal ;
	sh:path observable:fileAlignment .

observable:WindowsPEOptionalHeader sh:property _:node1gm7uj6vjx2072 .

_:node1gm7uj6vjx2073 sh:datatype xsd:unsignedInt ;
	sh:nodeKind sh:Literal ;
	sh:path observable:imageBase .

observable:WindowsPEOptionalHeader sh:property _:node1gm7uj6vjx2073 .

_:node1gm7uj6vjx2074 sh:datatype xsd:unsignedInt ;
	sh:nodeKind sh:Literal ;
	sh:path observable:loaderFlags .

observable:WindowsPEOptionalHeader sh:property _:node1gm7uj6vjx2074 .

_:node1gm7uj6vjx2075 sh:datatype xsd:unsignedInt ;
	sh:nodeKind sh:Literal ;
	sh:path observable:numberOfRVAAndSizes .

observable:WindowsPEOptionalHeader sh:property _:node1gm7uj6vjx2075 .

_:node1gm7uj6vjx2076 sh:datatype xsd:unsignedInt ;
	sh:nodeKind sh:Literal ;
	sh:path observable:sectionAlignment .

observable:WindowsPEOptionalHeader sh:property _:node1gm7uj6vjx2076 .

_:node1gm7uj6vjx2077 sh:datatype xsd:unsignedInt ;
	sh:nodeKind sh:Literal ;
	sh:path observable:sizeOfCode .

observable:WindowsPEOptionalHeader sh:property _:node1gm7uj6vjx2077 .

_:node1gm7uj6vjx2078 sh:datatype xsd:unsignedInt ;
	sh:nodeKind sh:Literal ;
	sh:path observable:sizeOfHeaders .

observable:WindowsPEOptionalHeader sh:property _:node1gm7uj6vjx2078 .

_:node1gm7uj6vjx2079 sh:datatype xsd:unsignedInt ;
	sh:nodeKind sh:Literal ;
	sh:path observable:sizeOfHeapCommit .

observable:WindowsPEOptionalHeader sh:property _:node1gm7uj6vjx2079 .

_:node1gm7uj6vjx2080 sh:datatype xsd:unsignedInt ;
	sh:nodeKind sh:Literal ;
	sh:path observable:sizeOfHeapReserve .

observable:WindowsPEOptionalHeader sh:property _:node1gm7uj6vjx2080 .

_:node1gm7uj6vjx2081 sh:datatype xsd:unsignedInt ;
	sh:nodeKind sh:Literal ;
	sh:path observable:sizeOfImage .

observable:WindowsPEOptionalHeader sh:property _:node1gm7uj6vjx2081 .

_:node1gm7uj6vjx2082 sh:datatype xsd:unsignedInt ;
	sh:nodeKind sh:Literal ;
	sh:path observable:sizeOfInitializedData .

observable:WindowsPEOptionalHeader sh:property _:node1gm7uj6vjx2082 .

_:node1gm7uj6vjx2083 sh:datatype xsd:unsignedInt ;
	sh:nodeKind sh:Literal ;
	sh:path observable:sizeOfStackCommit .

observable:WindowsPEOptionalHeader sh:property _:node1gm7uj6vjx2083 .

_:node1gm7uj6vjx2084 sh:datatype xsd:unsignedInt ;
	sh:nodeKind sh:Literal ;
	sh:path observable:sizeOfStackReserve .

observable:WindowsPEOptionalHeader sh:property _:node1gm7uj6vjx2084 .

_:node1gm7uj6vjx2085 sh:datatype xsd:unsignedInt ;
	sh:nodeKind sh:Literal ;
	sh:path observable:sizeOfUninitializedData .

observable:WindowsPEOptionalHeader sh:property _:node1gm7uj6vjx2085 .

_:node1gm7uj6vjx2086 sh:datatype xsd:unsignedInt ;
	sh:nodeKind sh:Literal ;
	sh:path observable:win32VersionValue .

observable:WindowsPEOptionalHeader sh:property _:node1gm7uj6vjx2086 .

_:node1gm7uj6vjx2087 sh:datatype xsd:unsignedShort ;
	sh:nodeKind sh:Literal ;
	sh:path observable:dllCharacteristics .

observable:WindowsPEOptionalHeader sh:property _:node1gm7uj6vjx2087 .

_:node1gm7uj6vjx2088 sh:datatype xsd:unsignedShort ;
	sh:nodeKind sh:Literal ;
	sh:path observable:magic .

observable:WindowsPEOptionalHeader sh:property _:node1gm7uj6vjx2088 .

_:node1gm7uj6vjx2089 sh:datatype xsd:unsignedShort ;
	sh:nodeKind sh:Literal ;
	sh:path observable:majorImageVersion .

observable:WindowsPEOptionalHeader sh:property _:node1gm7uj6vjx2089 .

_:node1gm7uj6vjx2090 sh:datatype xsd:unsignedShort ;
	sh:nodeKind sh:Literal ;
	sh:path observable:majorOSVersion .

observable:WindowsPEOptionalHeader sh:property _:node1gm7uj6vjx2090 .

_:node1gm7uj6vjx2091 sh:datatype xsd:unsignedShort ;
	sh:nodeKind sh:Literal ;
	sh:path observable:majorSubsystemVersion .

observable:WindowsPEOptionalHeader sh:property _:node1gm7uj6vjx2091 .

_:node1gm7uj6vjx2092 sh:datatype xsd:unsignedShort ;
	sh:nodeKind sh:Literal ;
	sh:path observable:minorImageVersion .

observable:WindowsPEOptionalHeader sh:property _:node1gm7uj6vjx2092 .

_:node1gm7uj6vjx2093 sh:datatype xsd:unsignedShort ;
	sh:nodeKind sh:Literal ;
	sh:path observable:minorOSVersion .

observable:WindowsPEOptionalHeader sh:property _:node1gm7uj6vjx2093 .

_:node1gm7uj6vjx2094 sh:datatype xsd:unsignedShort ;
	sh:nodeKind sh:Literal ;
	sh:path observable:minorSubsystemVersion .

observable:WindowsPEOptionalHeader sh:property _:node1gm7uj6vjx2094 .

_:node1gm7uj6vjx2095 sh:datatype xsd:unsignedShort ;
	sh:nodeKind sh:Literal ;
	sh:path observable:subsystem .

observable:WindowsPEOptionalHeader sh:property _:node1gm7uj6vjx2095 ;
	sh:targetClass observable:WindowsPEOptionalHeader .

observable:WindowsPESection a owl:Class , sh:NodeShape ;
	rdfs:subClassOf core:UcoInherentCharacterizationThing ;
	rdfs:label "WindowsPESection"@en ;
	rdfs:comment "A Windows PE section is a grouping of characteristics unique to a specific default or custom-defined region of a Windows PE (Portable Executable) file, consisting of an individual portion of the actual executable content of the file delineated according to unique purpose and memory protection requirements."@en .

_:node1gm7uj6vjx2096 sh:class types:Hash ;
	sh:nodeKind sh:IRI ;
	sh:path observable:hashes .

observable:WindowsPESection sh:property _:node1gm7uj6vjx2096 .

_:node1gm7uj6vjx2097 sh:datatype xsd:decimal ;
	sh:maxCount 1 ;
	sh:nodeKind sh:Literal ;
	sh:path observable:entropy .

observable:WindowsPESection sh:property _:node1gm7uj6vjx2097 .

_:node1gm7uj6vjx2098 sh:datatype xsd:integer ;
	sh:maxCount 1 ;
	sh:nodeKind sh:Literal ;
	sh:path observable:size .

observable:WindowsPESection sh:property _:node1gm7uj6vjx2098 .

_:node1gm7uj6vjx2099 sh:datatype xsd:string ;
	sh:maxCount 1 ;
	sh:nodeKind sh:Literal ;
	sh:path core:name .

observable:WindowsPESection sh:property _:node1gm7uj6vjx2099 ;
	sh:targetClass observable:WindowsPESection .

observable:WindowsPrefetch a owl:Class , sh:NodeShape ;
	rdfs:subClassOf observable:ObservableObject ;
	rdfs:label "WindowsPrefetch"@en ;
	rdfs:comment "The Windows prefetch contains entries in a Windows prefetch file (used to speed up application startup starting with Windows XP)."@en ;
	sh:targetClass observable:WindowsPrefetch .

observable:WindowsPrefetchFacet a owl:Class , sh:NodeShape ;
	rdfs:subClassOf core:Facet ;
	rdfs:label "WindowsPrefetchFacet"@en ;
	rdfs:comment "A Windows prefetch facet is a grouping of characteristics unique to entries in the Windows prefetch file (used to speed up application startup starting with Windows XP)."@en .

_:node1gm7uj6vjx2100 sh:class observable:ObservableObject ;
	sh:maxCount 1 ;
	sh:nodeKind sh:IRI ;
	sh:path observable:volume .

observable:WindowsPrefetchFacet sh:property _:node1gm7uj6vjx2100 .

_:node1gm7uj6vjx2101 sh:class observable:ObservableObject ;
	sh:nodeKind sh:IRI ;
	sh:path observable:accessedDirectory .

observable:WindowsPrefetchFacet sh:property _:node1gm7uj6vjx2101 .

_:node1gm7uj6vjx2102 sh:class observable:ObservableObject ;
	sh:nodeKind sh:IRI ;
	sh:path observable:accessedFile .

observable:WindowsPrefetchFacet sh:property _:node1gm7uj6vjx2102 .

_:node1gm7uj6vjx2103 sh:datatype xsd:dateTime ;
	sh:maxCount 1 ;
	sh:nodeKind sh:Literal ;
	sh:path observable:firstRun .

observable:WindowsPrefetchFacet sh:property _:node1gm7uj6vjx2103 .

_:node1gm7uj6vjx2104 sh:datatype xsd:dateTime ;
	sh:maxCount 1 ;
	sh:nodeKind sh:Literal ;
	sh:path observable:lastRun .

observable:WindowsPrefetchFacet sh:property _:node1gm7uj6vjx2104 .

_:node1gm7uj6vjx2105 sh:datatype xsd:integer ;
	sh:maxCount 1 ;
	sh:nodeKind sh:Literal ;
	sh:path observable:timesExecuted .

observable:WindowsPrefetchFacet sh:property _:node1gm7uj6vjx2105 .

_:node1gm7uj6vjx2106 sh:datatype xsd:string ;
	sh:maxCount 1 ;
	sh:nodeKind sh:Literal ;
	sh:path observable:applicationFileName .

observable:WindowsPrefetchFacet sh:property _:node1gm7uj6vjx2106 .

_:node1gm7uj6vjx2107 sh:datatype xsd:string ;
	sh:maxCount 1 ;
	sh:nodeKind sh:Literal ;
	sh:path observable:prefetchHash .

observable:WindowsPrefetchFacet sh:property _:node1gm7uj6vjx2107 ;
	sh:targetClass observable:WindowsPrefetchFacet .

observable:WindowsProcess a owl:Class , sh:NodeShape ;
	rdfs:subClassOf observable:Process ;
	rdfs:label "WindowsProcess"@en ;
	rdfs:comment "A Windows process is a program running on a Windows operating system."@en ;
	sh:targetClass observable:WindowsProcess .

observable:WindowsProcessFacet a owl:Class , sh:NodeShape ;
	rdfs:subClassOf core:Facet ;
	rdfs:label "WindowsProcessFacet"@en ;
	rdfs:comment "A Windows process facet is a grouping of characteristics unique to a program running on a Windows operating system."@en .

_:node1gm7uj6vjx2108 sh:class types:Dictionary ;
	sh:maxCount 1 ;
	sh:nodeKind sh:IRI ;
	sh:path observable:startupInfo .

observable:WindowsProcessFacet sh:property _:node1gm7uj6vjx2108 .

_:node1gm7uj6vjx2109 sh:datatype xsd:boolean ;
	sh:maxCount 1 ;
	sh:nodeKind sh:Literal ;
	sh:path observable:aslrEnabled .

observable:WindowsProcessFacet sh:property _:node1gm7uj6vjx2109 .

_:node1gm7uj6vjx2110 sh:datatype xsd:boolean ;
	sh:maxCount 1 ;
	sh:nodeKind sh:Literal ;
	sh:path observable:depEnabled .

observable:WindowsProcessFacet sh:property _:node1gm7uj6vjx2110 .

_:node1gm7uj6vjx2111 sh:datatype xsd:string ;
	sh:maxCount 1 ;
	sh:nodeKind sh:Literal ;
	sh:path observable:ownerSID .

observable:WindowsProcessFacet sh:property _:node1gm7uj6vjx2111 .

_:node1gm7uj6vjx2112 sh:datatype xsd:string ;
	sh:maxCount 1 ;
	sh:nodeKind sh:Literal ;
	sh:path observable:priority .

observable:WindowsProcessFacet sh:property _:node1gm7uj6vjx2112 .

_:node1gm7uj6vjx2113 sh:datatype xsd:string ;
	sh:maxCount 1 ;
	sh:nodeKind sh:Literal ;
	sh:path observable:windowTitle .

observable:WindowsProcessFacet sh:property _:node1gm7uj6vjx2113 ;
	sh:targetClass observable:WindowsProcessFacet .

observable:WindowsRegistryHive a owl:Class , sh:NodeShape ;
	rdfs:subClassOf observable:ObservableObject ;
	rdfs:label "WindowsRegistryHive"@en ;
	rdfs:comment "The Windows registry hive is a particular logical group of keys, subkeys, and values in a Windows registry (a hierarchical database that stores low-level settings for the Microsoft Windows operating system and for applications that opt to use the registry). [based on https://en.wikipedia.org/wiki/Windows_Registry]"@en ;
	sh:targetClass observable:WindowsRegistryHive .

observable:WindowsRegistryHiveFacet a owl:Class , sh:NodeShape ;
	rdfs:subClassOf core:Facet ;
	rdfs:label "WindowsRegistryHiveFacet"@en ;
	rdfs:comment "A Windows registry hive facet is a grouping of characteristics unique to a particular logical group of keys, subkeys, and values in a Windows registry (a hierarchical database that stores low-level settings for the Microsoft Windows operating system and for applications that opt to use the registry). [based on https://en.wikipedia.org/wiki/Windows_Registry]"@en .

_:node1gm7uj6vjx2114 sh:datatype xsd:string ;
	sh:maxCount 1 ;
	sh:nodeKind sh:Literal ;
	sh:path observable:hiveType .

observable:WindowsRegistryHiveFacet sh:property _:node1gm7uj6vjx2114 ;
	sh:targetClass observable:WindowsRegistryHiveFacet .

observable:WindowsRegistryKey a owl:Class , sh:NodeShape ;
	rdfs:subClassOf observable:ObservableObject ;
	rdfs:label "WindowsRegistryKey"@en ;
	rdfs:comment "A Windows registry key is a particular key within a Windows registry (a hierarchical database that stores low-level settings for the Microsoft Windows operating system and for applications that opt to use the registry). [based on https://en.wikipedia.org/wiki/Windows_Registry]"@en ;
	sh:targetClass observable:WindowsRegistryKey .

observable:WindowsRegistryKeyFacet a owl:Class , sh:NodeShape ;
	rdfs:subClassOf core:Facet ;
	rdfs:label "WindowsRegistryKeyFacet"@en ;
	rdfs:comment "A Windows registry key facet is a grouping of characteristics unique to a particular key within a Windows registry (A hierarchical database that stores low-level settings for the Microsoft Windows operating system and for applications that opt to use the registry). [based on https://en.wikipedia.org/wiki/Windows_Registry]"@en .

_:node1gm7uj6vjx2115 sh:class observable:ObservableObject ;
	sh:maxCount 1 ;
	sh:nodeKind sh:IRI ;
	sh:path observable:creator .

observable:WindowsRegistryKeyFacet sh:property _:node1gm7uj6vjx2115 .

_:node1gm7uj6vjx2116 sh:class observable:WindowsRegistryValue ;
	sh:nodeKind sh:IRI ;
	sh:path observable:registryValues .

observable:WindowsRegistryKeyFacet sh:property _:node1gm7uj6vjx2116 .

_:node1gm7uj6vjx2117 sh:datatype xsd:dateTime ;
	sh:maxCount 1 ;
	sh:nodeKind sh:Literal ;
	sh:path observable:modifiedTime .

observable:WindowsRegistryKeyFacet sh:property _:node1gm7uj6vjx2117 .

_:node1gm7uj6vjx2118 sh:datatype xsd:integer ;
	sh:maxCount 1 ;
	sh:nodeKind sh:Literal ;
	sh:path observable:numberOfSubkeys .

observable:WindowsRegistryKeyFacet sh:property _:node1gm7uj6vjx2118 .

_:node1gm7uj6vjx2119 sh:datatype xsd:string ;
	sh:maxCount 1 ;
	sh:nodeKind sh:Literal ;
	sh:path observable:key .

observable:WindowsRegistryKeyFacet sh:property _:node1gm7uj6vjx2119 ;
	sh:targetClass observable:WindowsRegistryKeyFacet .

observable:WindowsRegistryValue a owl:Class , sh:NodeShape ;
	rdfs:subClassOf core:UcoInherentCharacterizationThing ;
	rdfs:label "WindowsRegistryValue"@en ;
	rdfs:comment "A Windows registry value is a grouping of characteristics unique to a particular value within a Windows registry (a hierarchical database that stores low-level settings for the Microsoft Windows operating system and for applications that opt to use the registry. [based on https://en.wikipedia.org/wiki/Windows_Registry]"@en .

_:node1gm7uj6vjx2120 sh:datatype xsd:string ;
	sh:maxCount 1 ;
	sh:nodeKind sh:Literal ;
	sh:path core:name .

observable:WindowsRegistryValue sh:property _:node1gm7uj6vjx2120 .

_:node1gm7uj6vjx2121 sh:datatype xsd:string ;
	sh:maxCount 1 ;
	sh:nodeKind sh:Literal ;
	sh:path observable:data .

observable:WindowsRegistryValue sh:property _:node1gm7uj6vjx2121 .

_:node1gm7uj6vjx2122 sh:datatype xsd:string ;
	sh:maxCount 1 ;
	sh:nodeKind sh:Literal ;
	sh:path observable:dataType .

observable:WindowsRegistryValue sh:property _:node1gm7uj6vjx2122 ;
	sh:targetClass observable:WindowsRegistryValue .

observable:WindowsService a owl:Class , sh:NodeShape ;
	rdfs:subClassOf observable:ObservableObject ;
	rdfs:label "WindowsService"@en ;
	rdfs:comment "A Windows service is a specific Windows service (a computer program that operates in the background of a Windows operating system, similar to the way a UNIX daemon runs on UNIX). [based on https://en.wikipedia.org/wiki/Windows_service]"@en ;
	sh:targetClass observable:WindowsService .

observable:WindowsServiceFacet a owl:Class , sh:NodeShape ;
	rdfs:subClassOf core:Facet ;
	rdfs:label "WindowsServiceFacet"@en ;
	rdfs:comment "A Windows service facet is a grouping of characteristics unique to a specific Windows service (a computer program that operates in the background of a Windows operating system, similar to the way a UNIX daemon runs on UNIX). [based on https://en.wikipedia.org/wiki/Windows_service]"@en .

_:node1gm7uj6vjx2123 sh:datatype xsd:string ;
	sh:maxCount 1 ;
	sh:nodeKind sh:Literal ;
	sh:path observable:displayName .

observable:WindowsServiceFacet sh:property _:node1gm7uj6vjx2123 .

_:node1gm7uj6vjx2124 sh:datatype xsd:string ;
	sh:maxCount 1 ;
	sh:nodeKind sh:Literal ;
	sh:path observable:groupName .

observable:WindowsServiceFacet sh:property _:node1gm7uj6vjx2124 .

_:node1gm7uj6vjx2125 sh:datatype xsd:string .

observable:mftFileNameAccessedTime a owl:DatatypeProperty .

_:node1gm7uj6vjx2125 sh:maxCount 1 .

observable:mftFileNameAccessedTime rdfs:label "mftFileNameAccessedTime"@en .

_:node1gm7uj6vjx2125 sh:nodeKind sh:Literal .

observable:mftFileNameAccessedTime rdfs:comment "The access date and time recorded in an MFT entry $File_Name attribute."@en .

_:node1gm7uj6vjx2125 sh:path observable:serviceName .

observable:mftFileNameAccessedTime rdfs:range xsd:dateTime .

observable:WindowsServiceFacet sh:property _:node1gm7uj6vjx2125 .

observable:mftFileNameCreatedTime a owl:DatatypeProperty .

_:node1gm7uj6vjx2126 sh:datatype xsd:string .

observable:mftFileNameCreatedTime rdfs:label "mftFileNameCreatedTime"@en .

_:node1gm7uj6vjx2126 sh:maxCount 1 .

observable:mftFileNameCreatedTime rdfs:comment "The creation date and time recorded in an MFT entry $File_Name attribute."@en .

_:node1gm7uj6vjx2126 sh:nodeKind sh:Literal .

observable:mftFileNameCreatedTime rdfs:range xsd:dateTime .

_:node1gm7uj6vjx2126 sh:path observable:serviceStatus .

observable:mftFileNameLength a owl:DatatypeProperty .

observable:WindowsServiceFacet sh:property _:node1gm7uj6vjx2126 .

observable:mftFileNameLength rdfs:label "mftFileNameLength"@en .

_:node1gm7uj6vjx2127 sh:datatype xsd:string .

observable:mftFileNameLength rdfs:comment " Specifies the length of an NTFS file name, in unicode characters."@en .

_:node1gm7uj6vjx2127 sh:maxCount 1 .

observable:mftFileNameLength rdfs:range xsd:integer .

_:node1gm7uj6vjx2127 sh:nodeKind sh:Literal .

observable:mftFileNameModifiedTime a owl:DatatypeProperty .

_:node1gm7uj6vjx2127 sh:path observable:serviceType .

observable:mftFileNameModifiedTime rdfs:label "mftFileNameModifiedTime"@en .

observable:WindowsServiceFacet sh:property _:node1gm7uj6vjx2127 .

observable:mftFileNameModifiedTime rdfs:comment "The modification date and time recorded in an MFT entry $File_Name attribute."@en .

_:node1gm7uj6vjx2128 sh:datatype xsd:string .

observable:mftFileNameModifiedTime rdfs:range xsd:dateTime .

_:node1gm7uj6vjx2128 sh:maxCount 1 .

observable:mftFileNameRecordChangeTime a owl:DatatypeProperty .

_:node1gm7uj6vjx2128 sh:nodeKind sh:Literal .

observable:mftFileNameRecordChangeTime rdfs:label "mftFileNameRecordChangeTime"@en .

_:node1gm7uj6vjx2128 sh:path observable:startCommandLine .

observable:mftFileNameRecordChangeTime rdfs:comment "The metadata modification date and time recorded in an MFT entry $File_Name attribute."@en .

observable:WindowsServiceFacet sh:property _:node1gm7uj6vjx2128 .

observable:mftFileNameRecordChangeTime rdfs:range xsd:dateTime .

_:node1gm7uj6vjx2129 sh:datatype xsd:string .

observable:mftFlags a owl:DatatypeProperty .

_:node1gm7uj6vjx2129 sh:maxCount 1 .

observable:mftFlags rdfs:label "mftFlags"@en .

_:node1gm7uj6vjx2129 sh:nodeKind sh:Literal .

observable:mftFlags rdfs:comment "Specifies basic permissions for the file (Read-Only, Hidden, Archive, Compressed, etc.)."@en .

_:node1gm7uj6vjx2129 sh:path observable:startType .

observable:mftFlags rdfs:range xsd:integer .

observable:WindowsServiceFacet sh:property _:node1gm7uj6vjx2129 .

observable:mftParentID a owl:DatatypeProperty .

_:node1gm7uj6vjx2130 sh:datatype xsd:string .

observable:mftParentID rdfs:label "mftParentID"@en .

_:node1gm7uj6vjx2130 sh:nodeKind sh:Literal .

observable:mftParentID rdfs:comment "Specifies the record number within an NTFS Master File Table for parent directory of the file."@en .

_:node1gm7uj6vjx2130 sh:path observable:descriptions .

observable:mftParentID rdfs:range xsd:integer .

observable:WindowsServiceFacet sh:property _:node1gm7uj6vjx2130 .

observable:mftRecordChangeTime a owl:DatatypeProperty .

observable:WindowsServiceFacet sh:targetClass observable:WindowsServiceFacet .

observable:mftRecordChangeTime rdfs:label "mftRecordChangeTime"@en .

observable:WindowsServiceStartType a rdfs:Datatype .

observable:mftRecordChangeTime rdfs:comment "The date and time at which an NTFS file metadata was last modified."@en .

_:node1gm7uj6vjx2131 a rdfs:Datatype .

observable:mftRecordChangeTime rdfs:range xsd:dateTime .

_:node1gm7uj6vjx2132 rdf:first "service_auto_start" .

observable:middleName a owl:DatatypeProperty .

_:node1gm7uj6vjx2132 rdf:rest _:node1gm7uj6vjx2133 .

observable:middleName rdfs:label "middleName"@en .

_:node1gm7uj6vjx2133 rdf:first "service_boot_start" .

observable:middleName rdfs:comment "The middle name of a person."@en .

_:node1gm7uj6vjx2133 rdf:rest _:node1gm7uj6vjx2134 .

observable:middleName rdfs:range xsd:string .

_:node1gm7uj6vjx2134 rdf:first "service_demand_start" .

observable:mimeClass a owl:DatatypeProperty .

_:node1gm7uj6vjx2134 rdf:rest _:node1gm7uj6vjx2135 .

observable:mimeClass rdfs:label "mimeClass"@en .

_:node1gm7uj6vjx2135 rdf:first "service_disabled" .

observable:mimeClass rdfs:range xsd:string .

_:node1gm7uj6vjx2135 rdf:rest _:node1gm7uj6vjx2136 .

observable:mimeType a owl:DatatypeProperty .

_:node1gm7uj6vjx2136 rdf:first "service_system_alert" .

observable:mimeType rdfs:label "mimeType"@en .

_:node1gm7uj6vjx2136 rdf:rest rdf:nil .

observable:mimeType rdfs:comment "MIME type of the data. For example 'text/html' or 'audio/mp3'."@en .

_:node1gm7uj6vjx2131 owl:oneOf _:node1gm7uj6vjx2132 .

observable:mimeType rdfs:range xsd:string .

observable:WindowsServiceStartType owl:equivalentClass _:node1gm7uj6vjx2131 .

observable:minorImageVersion a owl:DatatypeProperty .

observable:WindowsServiceStatus a rdfs:Datatype .

observable:minorImageVersion rdfs:label "minorImageVersion"@en .

_:node1gm7uj6vjx2137 a rdfs:Datatype .

observable:minorImageVersion rdfs:comment "Specifies the minor version number of the image."@en .

_:node1gm7uj6vjx2138 rdf:first "service_continue_pending" .

observable:minorImageVersion rdfs:range xsd:unsignedShort .

_:node1gm7uj6vjx2138 rdf:rest _:node1gm7uj6vjx2139 .

observable:minorLinkerVersion a owl:DatatypeProperty .

_:node1gm7uj6vjx2139 rdf:first "service_pause_pending" .

observable:minorLinkerVersion rdfs:label "minorLinkerVersion"@en .

_:node1gm7uj6vjx2139 rdf:rest _:node1gm7uj6vjx2140 .

observable:minorLinkerVersion rdfs:comment "Specifies the linker minor version number."@en .

_:node1gm7uj6vjx2140 rdf:first "service_paused" .

observable:minorLinkerVersion rdfs:range xsd:byte .

_:node1gm7uj6vjx2140 rdf:rest _:node1gm7uj6vjx2141 .

observable:minorOSVersion a owl:DatatypeProperty .

_:node1gm7uj6vjx2141 rdf:first "service_running" .

observable:minorOSVersion rdfs:label "minorOSVersion"@en .

_:node1gm7uj6vjx2141 rdf:rest _:node1gm7uj6vjx2142 .

observable:minorOSVersion rdfs:comment "Specifies the minor version number of the required operating system."@en .

_:node1gm7uj6vjx2142 rdf:first "service_start_pending" .

observable:minorOSVersion rdfs:range xsd:unsignedShort .

_:node1gm7uj6vjx2142 rdf:rest _:node1gm7uj6vjx2143 .

observable:minorSubsystemVersion a owl:DatatypeProperty .

_:node1gm7uj6vjx2143 rdf:first "service_stop_pending" .

observable:minorSubsystemVersion rdfs:label "minorSubsystemVersion"@en .

_:node1gm7uj6vjx2143 rdf:rest _:node1gm7uj6vjx2144 .

observable:minorSubsystemVersion rdfs:comment """Specifies the minor version number of the subsystem.
          """@en .

_:node1gm7uj6vjx2144 rdf:first "service_stopped" .

observable:minorSubsystemVersion rdfs:range xsd:unsignedShort .

_:node1gm7uj6vjx2144 rdf:rest rdf:nil .

observable:mockLocationsAllowed a owl:DatatypeProperty .

_:node1gm7uj6vjx2137 owl:oneOf _:node1gm7uj6vjx2138 .

observable:mockLocationsAllowed rdfs:label "mockLocationsAllowed"@en .

observable:WindowsServiceStatus owl:equivalentClass _:node1gm7uj6vjx2137 .

observable:mockLocationsAllowed rdfs:comment "???."@en .

observable:WindowsServiceType a rdfs:Datatype .

observable:mockLocationsAllowed rdfs:range xsd:boolean .

_:node1gm7uj6vjx2145 a rdfs:Datatype .

observable:model a owl:DatatypeProperty .

_:node1gm7uj6vjx2146 rdf:first "service_file_system_driver" .

observable:model rdfs:label "model"@en .

_:node1gm7uj6vjx2146 rdf:rest _:node1gm7uj6vjx2147 .

observable:model rdfs:range xsd:string .

_:node1gm7uj6vjx2147 rdf:first "service_kernel_driver" .

observable:modifiedTime a owl:DatatypeProperty .

_:node1gm7uj6vjx2147 rdf:rest _:node1gm7uj6vjx2148 .

observable:modifiedTime rdfs:label "modifiedTime"@en .

_:node1gm7uj6vjx2148 rdf:first "service_win32_own_process" .

observable:modifiedTime rdfs:comment "The date and time at which the Object was last modified."@en .

_:node1gm7uj6vjx2148 rdf:rest _:node1gm7uj6vjx2149 .

observable:modifiedTime rdfs:range xsd:dateTime .

_:node1gm7uj6vjx2149 rdf:first "service_win32_share_process" .

observable:mostRecentRunTime a owl:DatatypeProperty .

_:node1gm7uj6vjx2149 rdf:rest rdf:nil .

observable:mostRecentRunTime rdfs:label "mostRecentRunTime"@en .

_:node1gm7uj6vjx2145 owl:oneOf _:node1gm7uj6vjx2146 .

observable:mostRecentRunTime rdfs:comment "Specifies the most recent run date/time of this scheduled task. See also: http://msdn.microsoft.com/en-us/library/windows/desktop/aa381254(v=vs.85).aspx."@en .

observable:WindowsServiceType owl:equivalentClass _:node1gm7uj6vjx2145 .

observable:mostRecentRunTime rdfs:range xsd:dateTime .

observable:WindowsSystemRestore a owl:Class .

observable:mountPoint a owl:DatatypeProperty .

observable:WindowsSystemRestore a sh:NodeShape .

observable:mountPoint rdfs:label "mountPoint"@en .

observable:WindowsSystemRestore rdfs:subClassOf observable:ObservableObject .

observable:mountPoint rdfs:comment "Specifies the mount point of the partition."@en .

observable:WindowsSystemRestore rdfs:label "WindowsSystemRestore"@en .

observable:mountPoint rdfs:range xsd:string .

observable:WindowsSystemRestore rdfs:comment "A Windows system restore is a capture of a Windows computer's state (including system files, installed applications, Windows Registry, and system settings) at a particular point in time such that the computer can be reverted to that state in the event of system malfunctions or other problems. [based on https://en.wikipedia.org/wiki/System_Restore]"@en .

observable:msProductID a owl:DatatypeProperty .

observable:WindowsSystemRestore sh:targetClass observable:WindowsSystemRestore .

observable:msProductID rdfs:label "msProductID"@en .

observable:WindowsTask a owl:Class .

observable:msProductID rdfs:comment "The Microsoft Product ID. See also: http://support.microsoft.com/gp/pidwin."@en .

observable:WindowsTask a sh:NodeShape .

observable:msProductID rdfs:range xsd:string .

observable:WindowsTask rdfs:subClassOf observable:ObservableObject .

observable:msProductName a owl:DatatypeProperty .

observable:WindowsTask rdfs:label "WindowsTask"@en .

observable:msProductName rdfs:label "msProductName"@en .

observable:WindowsTask rdfs:comment "A Windows task is a process that is scheduled to execute on a Windows operating system by the Windows Task Scheduler. [based on http://msdn.microsoft.com/en-us/library/windows/desktop/aa381311(v=vs.85).aspx]"@en .

observable:msProductName rdfs:comment "The Microsoft ProductName of the current installation of Windows. This is typically found in HKEY_LOCAL_MACHINE\\Software\\Microsoft\\Windows\\CurrentVersion!ProductName."@en .

observable:WindowsTask sh:targetClass observable:WindowsTask .

observable:msProductName rdfs:range xsd:string .

observable:WindowsTaskFacet a owl:Class .

observable:mutexName a owl:DatatypeProperty .

observable:WindowsTaskFacet a sh:NodeShape .

observable:mutexName rdfs:label "mutexName"@en .

observable:WindowsTaskFacet rdfs:subClassOf core:Facet .

observable:mutexName rdfs:comment "Specifies the name identifier for a specific instance of a mechanism that enforces limits on access to a resource when there are many threads of execution ."@en .

observable:WindowsTaskFacet rdfs:label "WindowsTaskFacet"@en .

observable:mutexName rdfs:range xsd:string .

observable:WindowsTaskFacet rdfs:comment "A Windows Task facet is a grouping of characteristics unique to a Windows Task (a process that is scheduled to execute on a Windows operating system by the Windows Task Scheduler). [based on http://msdn.microsoft.com/en-us/library/windows/desktop/aa381311(v=vs.85).aspx]"@en .

observable:nameConstraints a owl:DatatypeProperty .

_:node1gm7uj6vjx2150 sh:class observable:ObservableObject .

observable:nameConstraints rdfs:label "nameConstraints"@en .

_:node1gm7uj6vjx2150 sh:maxCount 1 .

observable:nameConstraints rdfs:range xsd:string .

_:node1gm7uj6vjx2150 sh:nodeKind sh:IRI .

observable:namePhonetic a owl:DatatypeProperty .

_:node1gm7uj6vjx2150 sh:path observable:account .

observable:namePhonetic rdfs:label "namePhonetic"@en .

observable:WindowsTaskFacet sh:property _:node1gm7uj6vjx2150 .

observable:namePhonetic rdfs:comment "Name phonetic specifies the phonetic pronunciation of the name of a person."@en .

_:node1gm7uj6vjx2151 sh:class observable:ObservableObject .

observable:namePhonetic rdfs:range xsd:string .

_:node1gm7uj6vjx2151 sh:maxCount 1 .

observable:namePrefix a owl:DatatypeProperty .

_:node1gm7uj6vjx2151 sh:nodeKind sh:IRI .

observable:namePrefix rdfs:label "namePrefix"@en .

_:node1gm7uj6vjx2151 sh:path observable:application .

observable:namePrefix rdfs:comment "Name prefix specifies an honorific prefix (coming ordinally before first/given name) for the name of a person."@en .

observable:WindowsTaskFacet sh:property _:node1gm7uj6vjx2151 .

observable:namePrefix rdfs:range xsd:string .

_:node1gm7uj6vjx2152 sh:class observable:ObservableObject .

observable:nameRecoveredStatus a owl:DatatypeProperty .

_:node1gm7uj6vjx2152 sh:maxCount 1 .

observable:nameRecoveredStatus rdfs:label "nameRecoveredStatus"@en .

_:node1gm7uj6vjx2152 sh:nodeKind sh:IRI .

observable:nameRecoveredStatus rdfs:comment "Specifies the recoverability status of the name of an object."@en .

_:node1gm7uj6vjx2152 sh:path observable:workItemData .

_:node1gm7uj6vjx2368 a rdfs:Datatype .

observable:WindowsTaskFacet sh:property _:node1gm7uj6vjx2152 .

_:node1gm7uj6vjx2369 rdf:first vocabulary:RecoveredObjectStatusVocab .

_:node1gm7uj6vjx2153 sh:class observable:ObservableObject .

_:node1gm7uj6vjx2369 rdf:rest _:node1gm7uj6vjx2370 .

_:node1gm7uj6vjx2153 sh:maxCount 1 .

_:node1gm7uj6vjx2370 rdf:first xsd:string .

_:node1gm7uj6vjx2153 sh:nodeKind sh:IRI .

_:node1gm7uj6vjx2370 rdf:rest rdf:nil .

_:node1gm7uj6vjx2153 sh:path observable:workingDirectory .

_:node1gm7uj6vjx2368 owl:unionOf _:node1gm7uj6vjx2369 .

observable:WindowsTaskFacet sh:property _:node1gm7uj6vjx2153 .

observable:nameRecoveredStatus rdfs:range _:node1gm7uj6vjx2368 .

_:node1gm7uj6vjx2154 sh:class observable:TaskActionType .

observable:nameServer a owl:ObjectProperty .

_:node1gm7uj6vjx2154 sh:nodeKind sh:IRI .

observable:nameServer rdfs:label "nameServer"@en .

_:node1gm7uj6vjx2154 sh:path observable:actionList .

observable:nameServer rdfs:comment "Specifies a list of name server entries for a Whois entry."@en .

observable:WindowsTaskFacet sh:property _:node1gm7uj6vjx2154 .

observable:nameServer rdfs:range observable:ObservableObject .

_:node1gm7uj6vjx2155 sh:class observable:TriggerType .

observable:nameSuffix a owl:DatatypeProperty .

_:node1gm7uj6vjx2155 sh:nodeKind sh:IRI .

observable:nameSuffix rdfs:label "nameSuffix"@en .

_:node1gm7uj6vjx2155 sh:path observable:triggerList .

observable:nameSuffix rdfs:comment "Name suffix specifies an suffix (coming ordinally after last/family name) for the name of a person."@en .

observable:WindowsTaskFacet sh:property _:node1gm7uj6vjx2155 .

observable:nameSuffix rdfs:range xsd:string .

_:node1gm7uj6vjx2156 sh:datatype xsd:dateTime .

observable:netBIOSName a owl:DatatypeProperty .

_:node1gm7uj6vjx2156 sh:maxCount 1 .

observable:netBIOSName rdfs:label "netBIOSName"@en .

_:node1gm7uj6vjx2156 sh:nodeKind sh:Literal .

observable:netBIOSName rdfs:comment "Specifies the NetBIOS (Network Basic Input/Output System) name of the Windows system. This is not the same as the host name."@en .

_:node1gm7uj6vjx2156 sh:path observable:mostRecentRunTime .

observable:netBIOSName rdfs:range xsd:string .

observable:WindowsTaskFacet sh:property _:node1gm7uj6vjx2156 .

observable:network a owl:DatatypeProperty .

_:node1gm7uj6vjx2157 sh:datatype xsd:dateTime .

observable:network rdfs:label "network"@en .

_:node1gm7uj6vjx2157 sh:maxCount 1 .

observable:network rdfs:comment "???."@en .

_:node1gm7uj6vjx2157 sh:nodeKind sh:Literal .

observable:network rdfs:range xsd:string .

_:node1gm7uj6vjx2157 sh:path observable:nextRunTime .

observable:networkInterface a owl:ObjectProperty .

observable:WindowsTaskFacet sh:property _:node1gm7uj6vjx2157 .

observable:networkInterface rdfs:label "networkInterface"@en .

_:node1gm7uj6vjx2158 sh:datatype xsd:dateTime .

observable:networkInterface rdfs:comment "Specifies the list of network interfaces present on the system."@en .

_:node1gm7uj6vjx2158 sh:maxCount 1 .

observable:networkInterface rdfs:range observable:ObservableObject .

_:node1gm7uj6vjx2158 sh:nodeKind sh:Literal .

observable:newObject a owl:ObjectProperty .

_:node1gm7uj6vjx2158 sh:path observable:observableCreatedTime .

observable:newObject rdfs:label "newObject"@en .

observable:WindowsTaskFacet sh:property _:node1gm7uj6vjx2158 .

observable:newObject rdfs:comment "Specifies the observable object and its properties as they are after the state change effect occurred."@en .

_:node1gm7uj6vjx2159 sh:datatype xsd:integer .

observable:newObject rdfs:range observable:ObservableObject .

_:node1gm7uj6vjx2159 sh:maxCount 1 .

observable:nextRunTime a owl:DatatypeProperty .

_:node1gm7uj6vjx2159 sh:nodeKind sh:Literal .

observable:nextRunTime rdfs:label "nextRunTime"@en .

_:node1gm7uj6vjx2159 sh:path observable:exitCode .

observable:nextRunTime rdfs:comment "Specifies the next run date/time of the scheduled task. See also: http://msdn.microsoft.com/en-us/library/windows/desktop/aa381257(v=vs.85).aspx."@en .

observable:WindowsTaskFacet sh:property _:node1gm7uj6vjx2159 .

observable:nextRunTime rdfs:range xsd:dateTime .

_:node1gm7uj6vjx2160 sh:datatype xsd:integer .

observable:nickname a owl:DatatypeProperty .

_:node1gm7uj6vjx2160 sh:maxCount 1 .

observable:nickname rdfs:label "nickname"@en .

_:node1gm7uj6vjx2160 sh:nodeKind sh:Literal .

observable:nickname rdfs:comment "Nickname specifies an alternate, unofficial and typically informal name for a person independent of their official name."@en .

_:node1gm7uj6vjx2160 sh:path observable:maxRunTime .

observable:nickname rdfs:range xsd:string .

observable:WindowsTaskFacet sh:property _:node1gm7uj6vjx2160 .

observable:ntfsHardLinkCount a owl:DatatypeProperty .

_:node1gm7uj6vjx2161 sh:datatype xsd:string .

observable:ntfsHardLinkCount rdfs:label "ntfsHardLinkCount"@en .

_:node1gm7uj6vjx2161 sh:maxCount 1 .

observable:ntfsHardLinkCount rdfs:comment "Specifies the number of directory entries that reference an NTFS file record."@en .

_:node1gm7uj6vjx2161 sh:nodeKind sh:Literal .

observable:ntfsHardLinkCount rdfs:range xsd:integer .

_:node1gm7uj6vjx2161 sh:path observable:accountLogonType .

observable:ntfsOwnerID a owl:DatatypeProperty .

observable:WindowsTaskFacet sh:property _:node1gm7uj6vjx2161 .

observable:ntfsOwnerID rdfs:label "ntfsOwnerID"@en .

_:node1gm7uj6vjx2162 sh:datatype xsd:string .

observable:ntfsOwnerID rdfs:comment "Specifies the identifier of the file owner, from the security index."@en .

_:node1gm7uj6vjx2162 sh:maxCount 1 .

observable:ntfsOwnerID rdfs:range xsd:string .

_:node1gm7uj6vjx2162 sh:nodeKind sh:Literal .

observable:ntfsOwnerSID a owl:DatatypeProperty .

_:node1gm7uj6vjx2162 sh:path observable:accountRunLevel .

observable:ntfsOwnerSID rdfs:label "ntfsOwnerSID"@en .

observable:WindowsTaskFacet sh:property _:node1gm7uj6vjx2162 .

observable:ntfsOwnerSID rdfs:comment "Specifies the security ID (key in the $SII Index and $SDS DataStream in the file $Secure) for an NTFS file."@en .

_:node1gm7uj6vjx2163 sh:datatype xsd:string .

observable:ntfsOwnerSID rdfs:range xsd:string .

_:node1gm7uj6vjx2163 sh:maxCount 1 .

observable:number a owl:DatatypeProperty .

_:node1gm7uj6vjx2163 sh:nodeKind sh:Literal .

observable:number rdfs:label "number"@en .

_:node1gm7uj6vjx2163 sh:path observable:imageName .

observable:number rdfs:range xsd:integer .

observable:WindowsTaskFacet sh:property _:node1gm7uj6vjx2163 .

observable:numberOfLaunches a owl:DatatypeProperty .

_:node1gm7uj6vjx2164 sh:datatype xsd:string .

observable:numberOfLaunches rdfs:label "numberOfLaunches"@en .

_:node1gm7uj6vjx2164 sh:maxCount 1 .

observable:numberOfLaunches rdfs:range xsd:integer .

_:node1gm7uj6vjx2164 sh:nodeKind sh:Literal .

observable:numberOfRVAAndSizes a owl:DatatypeProperty .

_:node1gm7uj6vjx2164 sh:path observable:parameters .

observable:numberOfRVAAndSizes rdfs:label "numberOfRVAAndSizes"@en .

observable:WindowsTaskFacet sh:property _:node1gm7uj6vjx2164 .

observable:numberOfRVAAndSizes rdfs:comment "Specifies the number of data-directory entries in the remainder of the optional header."@en .

_:node1gm7uj6vjx2165 sh:datatype xsd:string .

observable:numberOfRVAAndSizes rdfs:range xsd:unsignedInt .

_:node1gm7uj6vjx2165 sh:maxCount 1 .

observable:numberOfSections a owl:DatatypeProperty .

_:node1gm7uj6vjx2165 sh:nodeKind sh:Literal .

observable:numberOfSections rdfs:label "numberOfSections"@en .

_:node1gm7uj6vjx2165 sh:path observable:taskComment .

observable:numberOfSections rdfs:comment "Specifies the number of sections in the PE binary, as a non-negative integer."@en .

observable:WindowsTaskFacet sh:property _:node1gm7uj6vjx2165 .

observable:numberOfSections rdfs:range xsd:integer .

_:node1gm7uj6vjx2166 sh:datatype xsd:string .

observable:numberOfSubkeys a owl:DatatypeProperty .

_:node1gm7uj6vjx2166 sh:maxCount 1 .

observable:numberOfSubkeys rdfs:label "numberOfSubkeys"@en .

_:node1gm7uj6vjx2166 sh:nodeKind sh:Literal .

observable:numberOfSubkeys rdfs:range xsd:integer .

_:node1gm7uj6vjx2166 sh:path observable:taskCreator .

observable:numberOfSymbols a owl:DatatypeProperty .

observable:WindowsTaskFacet sh:property _:node1gm7uj6vjx2166 .

observable:numberOfSymbols rdfs:label "numberOfSymbols"@en .

_:node1gm7uj6vjx2167 sh:datatype vocabulary:TaskFlagVocab .

observable:numberOfSymbols rdfs:comment "Specifies the number of entries in the symbol table of the PE binary, as a non-negative integer."@en .

_:node1gm7uj6vjx2167 sh:message "Value is outside the default vocabulary TaskFlagVocab." .

observable:numberOfSymbols rdfs:range xsd:integer .

_:node1gm7uj6vjx2167 sh:path observable:flags .

observable:numberTimesContacted a owl:DatatypeProperty .

_:node1gm7uj6vjx2167 sh:severity sh:Info .

observable:numberTimesContacted rdfs:label "numberTimesContacted"@en .

observable:WindowsTaskFacet sh:property _:node1gm7uj6vjx2167 .

observable:numberTimesContacted rdfs:comment "Number times contacted specifies the number of times a particular contact has been contacted."@en .

_:node1gm7uj6vjx2168 sh:datatype vocabulary:TaskPriorityVocab .

observable:numberTimesContacted rdfs:range xsd:integer .

_:node1gm7uj6vjx2168 sh:message "Value is outside the default vocabulary TaskPriorityVocab." .

observable:objectGUID a owl:DatatypeProperty .

_:node1gm7uj6vjx2168 sh:path observable:priority .

observable:objectGUID rdfs:label "objectGUID"@en .

_:node1gm7uj6vjx2168 sh:severity sh:Info .

observable:objectGUID rdfs:range xsd:string .

observable:WindowsTaskFacet sh:property _:node1gm7uj6vjx2168 .

observable:observableCreatedTime a owl:DatatypeProperty .

_:node1gm7uj6vjx2169 sh:datatype vocabulary:TaskStatusVocab .

observable:observableCreatedTime rdfs:label "observableCreatedTime"@en .

_:node1gm7uj6vjx2169 sh:message "Value is outside the default vocabulary TaskStatusVocab." .

observable:observableCreatedTime rdfs:comment "The date and time at which the observable object being characterized was created. This time pertains to an intrinsic characteristic of the observable object, and would be consistent across independent characterizations or observations of the observable object."@en .

_:node1gm7uj6vjx2169 sh:path observable:status .

observable:observableCreatedTime rdfs:range xsd:dateTime .

_:node1gm7uj6vjx2169 sh:severity sh:Info .

observable:oldObject a owl:ObjectProperty .

observable:WindowsTaskFacet sh:property _:node1gm7uj6vjx2169 .

observable:oldObject rdfs:label "oldObject"@en .

_:node1gm7uj6vjx2170 sh:maxCount 1 .

observable:oldObject rdfs:comment "Specifies the observable object and its properties as they were before the state change effect occurred."@en .

_:node1gm7uj6vjx2170 sh:nodeKind sh:Literal .

observable:oldObject rdfs:range observable:ObservableObject .

_:node1gm7uj6vjx2172 sh:datatype vocabulary:TaskPriorityVocab .

observable:openFileDescriptor a owl:DatatypeProperty .

_:node1gm7uj6vjx2171 rdf:first _:node1gm7uj6vjx2172 .

observable:openFileDescriptor rdfs:label "openFileDescriptor"@en .

_:node1gm7uj6vjx2171 rdf:rest _:node1gm7uj6vjx2173 .

observable:openFileDescriptor rdfs:comment "Specifies a listing of the current file descriptors used by the Unix process."@en .

_:node1gm7uj6vjx2174 sh:datatype xsd:integer .

observable:openFileDescriptor rdfs:range xsd:integer .

_:node1gm7uj6vjx2173 rdf:first _:node1gm7uj6vjx2174 .

observable:operatingSystem a owl:ObjectProperty .

_:node1gm7uj6vjx2173 rdf:rest _:node1gm7uj6vjx2175 .

observable:operatingSystem rdfs:label "operatingSystem"@en .

_:node1gm7uj6vjx2176 sh:datatype xsd:string .

observable:operatingSystem rdfs:range observable:ObservableObject .

_:node1gm7uj6vjx2175 rdf:first _:node1gm7uj6vjx2176 .

observable:optionalHeader a owl:ObjectProperty .

_:node1gm7uj6vjx2175 rdf:rest rdf:nil .

observable:optionalHeader rdfs:label "optionalHeader"@en .

_:node1gm7uj6vjx2170 sh:or _:node1gm7uj6vjx2171 .

observable:optionalHeader rdfs:comment "Specifies the PE optional header of the PE binary."@en .

_:node1gm7uj6vjx2170 sh:path observable:priority .

observable:optionalHeader rdfs:range observable:WindowsPEOptionalHeader .

observable:WindowsTaskFacet sh:property _:node1gm7uj6vjx2170 .

observable:options a owl:DatatypeProperty .

_:node1gm7uj6vjx2177 sh:maxCount 1 .

observable:options rdfs:label "options"@en .

_:node1gm7uj6vjx2177 sh:nodeKind sh:Literal .

observable:options rdfs:comment "Specifies any options used when mounting the volume."@en .

_:node1gm7uj6vjx2179 sh:datatype vocabulary:TaskStatusVocab .

observable:options rdfs:range xsd:string .

_:node1gm7uj6vjx2178 rdf:first _:node1gm7uj6vjx2179 .

observable:organizationDepartment a owl:DatatypeProperty .

_:node1gm7uj6vjx2178 rdf:rest _:node1gm7uj6vjx2180 .

observable:organizationDepartment rdfs:label "organizationDepartment"@en .

_:node1gm7uj6vjx2181 sh:datatype xsd:string .

observable:organizationDepartment rdfs:comment "Specifies a particular suborganization (division, branch, office, etc.) that exists within a larger organization."@en .

_:node1gm7uj6vjx2180 rdf:first _:node1gm7uj6vjx2181 .

observable:organizationDepartment rdfs:range xsd:string .

_:node1gm7uj6vjx2180 rdf:rest rdf:nil .

observable:organizationLocation a owl:ObjectProperty .

_:node1gm7uj6vjx2177 sh:or _:node1gm7uj6vjx2178 .

observable:organizationLocation rdfs:label "organizationLocation"@en .

_:node1gm7uj6vjx2177 sh:path observable:status .

observable:organizationLocation rdfs:comment "Specifies a geolocation address of an organization."@en .

observable:WindowsTaskFacet sh:property _:node1gm7uj6vjx2177 .

observable:organizationLocation rdfs:range observable:ContactAddress .

_:node1gm7uj6vjx2182 sh:message "Value is not member of the vocabulary TaskFlagVocab." .

observable:organizationPosition a owl:DatatypeProperty .

_:node1gm7uj6vjx2184 sh:datatype vocabulary:TaskFlagVocab .

observable:organizationPosition rdfs:label "organizationPosition"@en .

_:node1gm7uj6vjx2185 rdf:first "TASK_FLAG_DELETE_WHEN_DONE"^^vocabulary:TaskFlagVocab .

observable:organizationPosition rdfs:comment "Specifies the title or role that a person plays within an organization."@en .

_:node1gm7uj6vjx2185 rdf:rest _:node1gm7uj6vjx2186 .

observable:organizationPosition rdfs:range xsd:string .

_:node1gm7uj6vjx2186 rdf:first "TASK_FLAG_DISABLED"^^vocabulary:TaskFlagVocab .

observable:osInstallDate a owl:DatatypeProperty .

_:node1gm7uj6vjx2186 rdf:rest _:node1gm7uj6vjx2187 .

observable:osInstallDate rdfs:label "osInstallDate"@en .

_:node1gm7uj6vjx2187 rdf:first "TASK_FLAG_DONT_START_IF_ON_BATTERIES"^^vocabulary:TaskFlagVocab .

observable:osInstallDate rdfs:comment "Specifies the date on which the operating system (OS) was installed."@en .

_:node1gm7uj6vjx2187 rdf:rest _:node1gm7uj6vjx2188 .

observable:osInstallDate rdfs:range xsd:dateTime .

_:node1gm7uj6vjx2188 rdf:first "TASK_FLAG_HIDDEN"^^vocabulary:TaskFlagVocab .

observable:osLastUpgradeDate a owl:DatatypeProperty .

_:node1gm7uj6vjx2188 rdf:rest _:node1gm7uj6vjx2189 .

observable:osLastUpgradeDate rdfs:label "osLastUpgradeDate"@en .

_:node1gm7uj6vjx2189 rdf:first "TASK_FLAG_INTERACTIVE"^^vocabulary:TaskFlagVocab .

observable:osLastUpgradeDate rdfs:comment "Specifies the date on which the operating system (OS) was last upgraded."@en .

_:node1gm7uj6vjx2189 rdf:rest _:node1gm7uj6vjx2190 .

observable:osLastUpgradeDate rdfs:range xsd:dateTime .

_:node1gm7uj6vjx2190 rdf:first "TASK_FLAG_KILL_IF_GOING_ON_BATTERIES"^^vocabulary:TaskFlagVocab .

observable:otherHeaders a owl:ObjectProperty .

_:node1gm7uj6vjx2190 rdf:rest _:node1gm7uj6vjx2191 .

observable:otherHeaders rdfs:label "otherHeaders"@en ;
	rdfs:range types:Dictionary .

_:node1gm7uj6vjx2191 rdf:first "TASK_FLAG_KILL_ON_IDLE_END"^^vocabulary:TaskFlagVocab .

observable:owner a owl:ObjectProperty .

_:node1gm7uj6vjx2191 rdf:rest _:node1gm7uj6vjx2192 .

observable:owner rdfs:label "owner"@en .

_:node1gm7uj6vjx2192 rdf:first "TASK_FLAG_RESTART_ON_IDLE_RESUME"^^vocabulary:TaskFlagVocab .

observable:owner rdfs:comment "Specifies the owner of an Observable Object."@en .

_:node1gm7uj6vjx2192 rdf:rest _:node1gm7uj6vjx2193 .

observable:owner rdfs:range core:UcoObject .

_:node1gm7uj6vjx2193 rdf:first "TASK_FLAG_RUN_IF_CONNECTED_TO_INTERNET"^^vocabulary:TaskFlagVocab .

observable:ownerSID a owl:DatatypeProperty .

_:node1gm7uj6vjx2193 rdf:rest _:node1gm7uj6vjx2194 .

observable:ownerSID rdfs:label "ownerSID"@en .

_:node1gm7uj6vjx2194 rdf:first "TASK_FLAG_RUN_ONLY_IF_LOGGED_ON"^^vocabulary:TaskFlagVocab .

observable:ownerSID rdfs:range xsd:string .

_:node1gm7uj6vjx2194 rdf:rest _:node1gm7uj6vjx2195 .

observable:pageTitle a owl:DatatypeProperty .

_:node1gm7uj6vjx2195 rdf:first "TASK_FLAG_START_ONLY_IF_IDLE"^^vocabulary:TaskFlagVocab .

observable:pageTitle rdfs:label "Page Title"@en .

_:node1gm7uj6vjx2195 rdf:rest _:node1gm7uj6vjx2196 .

observable:pageTitle rdfs:comment "Specifies the title of a web page."@en .

_:node1gm7uj6vjx2196 rdf:first "TASK_FLAG_SYSTEM_REQUIRED"^^vocabulary:TaskFlagVocab .

observable:pageTitle rdfs:range xsd:string .

_:node1gm7uj6vjx2196 rdf:rest _:node1gm7uj6vjx2197 .

observable:parameterAddress a owl:DatatypeProperty .

_:node1gm7uj6vjx2197 rdf:first "TASK_FLAG_ZERO"^^vocabulary:TaskFlagVocab .

observable:parameterAddress rdfs:label "parameterAddress"@en .

_:node1gm7uj6vjx2197 rdf:rest rdf:nil .

observable:parameterAddress rdfs:range xsd:hexBinary .

_:node1gm7uj6vjx2184 sh:in _:node1gm7uj6vjx2185 .

observable:parameters a owl:DatatypeProperty .

_:node1gm7uj6vjx2183 rdf:first _:node1gm7uj6vjx2184 .

observable:parameters rdfs:label "parameters"@en .

_:node1gm7uj6vjx2183 rdf:rest _:node1gm7uj6vjx2198 .

observable:parameters rdfs:comment "Specifies the command line parameters used to launch the scheduled task. See also: http://msdn.microsoft.com/en-us/library/windows/desktop/aa381875(v=vs.85).aspx."@en .

_:node1gm7uj6vjx2199 sh:datatype xsd:string .

observable:parameters rdfs:range xsd:string .

_:node1gm7uj6vjx2198 rdf:first _:node1gm7uj6vjx2199 .

observable:parent a owl:ObjectProperty .

_:node1gm7uj6vjx2198 rdf:rest rdf:nil .

observable:parent rdfs:label "parent"@en .

_:node1gm7uj6vjx2182 sh:or _:node1gm7uj6vjx2183 .

observable:parent rdfs:comment "The process that created this process."@en .

_:node1gm7uj6vjx2182 sh:path observable:flags .

observable:parent rdfs:range observable:ObservableObject .

observable:WindowsTaskFacet sh:property _:node1gm7uj6vjx2182 .

observable:participant a owl:ObjectProperty .

_:node1gm7uj6vjx2200 sh:message "Value is not member of the vocabulary TaskPriorityVocab." .

observable:participant rdfs:label "participant"@en .

_:node1gm7uj6vjx2202 sh:datatype vocabulary:TaskPriorityVocab .

observable:participant rdfs:range observable:ObservableObject .

_:node1gm7uj6vjx2203 rdf:first "ABOVE_NORMAL_PRIORITY_CLASS"^^vocabulary:TaskPriorityVocab .

observable:partition a owl:ObjectProperty .

_:node1gm7uj6vjx2203 rdf:rest _:node1gm7uj6vjx2204 .

observable:partition rdfs:label "partition"@en .

_:node1gm7uj6vjx2204 rdf:first "BELOW_NORMAL_PRIORITY_CLASS"^^vocabulary:TaskPriorityVocab .

observable:partition rdfs:comment "The partitions that reside on the disk."@en .

_:node1gm7uj6vjx2204 rdf:rest _:node1gm7uj6vjx2205 .

observable:partition rdfs:range observable:ObservableObject .

_:node1gm7uj6vjx2205 rdf:first "HIGH_PRIORITY_CLASS"^^vocabulary:TaskPriorityVocab .

observable:partitionID a owl:DatatypeProperty .

_:node1gm7uj6vjx2205 rdf:rest _:node1gm7uj6vjx2206 .

observable:partitionID rdfs:label "partitionID"@en .

_:node1gm7uj6vjx2206 rdf:first "IDLE_PRIORITY_CLASS"^^vocabulary:TaskPriorityVocab .

observable:partitionID rdfs:comment "Specifies the identifier of the partition, as provided by the containing partition table.  This identifier is the index value within the partition table, and is expected to be an incrementing alphanumeric value (numeric in most partition systems), not a GUID or UUID.  Sorting partitions by this index should first attempt to sort a numeric cast of the value."@en .

_:node1gm7uj6vjx2206 rdf:rest _:node1gm7uj6vjx2207 .

observable:partitionID rdfs:range xsd:string .

_:node1gm7uj6vjx2207 rdf:first "NORMAL_PRIORITY_CLASS"^^vocabulary:TaskPriorityVocab .

observable:partitionLength a owl:DatatypeProperty .

_:node1gm7uj6vjx2207 rdf:rest _:node1gm7uj6vjx2208 .

observable:partitionLength rdfs:label "partitionLength"@en .

_:node1gm7uj6vjx2208 rdf:first "REALTIME_PRIORITY_CLASS"^^vocabulary:TaskPriorityVocab .

observable:partitionLength rdfs:comment "Specifies the length of the partition, in bytes."@en .

_:node1gm7uj6vjx2208 rdf:rest rdf:nil .

observable:partitionLength rdfs:range xsd:integer .

_:node1gm7uj6vjx2202 sh:in _:node1gm7uj6vjx2203 .

observable:partitionOffset a owl:DatatypeProperty .

_:node1gm7uj6vjx2201 rdf:first _:node1gm7uj6vjx2202 .

observable:partitionOffset rdfs:label "partitionOffset"@en .

_:node1gm7uj6vjx2201 rdf:rest _:node1gm7uj6vjx2209 .

observable:partitionOffset rdfs:comment "Specifies the starting offset of the partition, in bytes."@en .

_:node1gm7uj6vjx2210 sh:datatype xsd:integer .

observable:partitionOffset rdfs:range xsd:integer .

_:node1gm7uj6vjx2209 rdf:first _:node1gm7uj6vjx2210 .

observable:password a owl:DatatypeProperty .

_:node1gm7uj6vjx2209 rdf:rest _:node1gm7uj6vjx2211 .

observable:password rdfs:label "password"@en .

_:node1gm7uj6vjx2212 sh:datatype xsd:string .

observable:password rdfs:comment "Specifies an authentication password."@en .

_:node1gm7uj6vjx2211 rdf:first _:node1gm7uj6vjx2212 .

observable:password rdfs:range xsd:string .

_:node1gm7uj6vjx2211 rdf:rest rdf:nil .

observable:passwordLastChanged a owl:DatatypeProperty .

_:node1gm7uj6vjx2200 sh:or _:node1gm7uj6vjx2201 .

observable:passwordLastChanged rdfs:label "passwordLastChanged"@en .

_:node1gm7uj6vjx2200 sh:path observable:priority .

observable:passwordLastChanged rdfs:comment "The date and time that the password was last changed."@en .

observable:WindowsTaskFacet sh:property _:node1gm7uj6vjx2200 .

observable:passwordLastChanged rdfs:range xsd:dateTime .

_:node1gm7uj6vjx2213 sh:message "Value is not member of the vocabulary TaskStatusVocab." .

observable:passwordType a owl:DatatypeProperty .

_:node1gm7uj6vjx2215 sh:datatype vocabulary:TaskStatusVocab .

observable:passwordType rdfs:label "passwordType"@en .

_:node1gm7uj6vjx2216 rdf:first "SCHED_E_ACCOUNT_DBASE_CORRUPT"^^vocabulary:TaskStatusVocab .

observable:passwordType rdfs:comment "The type of password, for instance plain-text or encrypted."@en .

_:node1gm7uj6vjx2216 rdf:rest _:node1gm7uj6vjx2217 .

observable:passwordType rdfs:range xsd:string .

_:node1gm7uj6vjx2217 rdf:first "SCHED_E_ACCOUNT_INFORMATION_NOT_SET"^^vocabulary:TaskStatusVocab .

observable:path a owl:DatatypeProperty .

_:node1gm7uj6vjx2217 rdf:rest _:node1gm7uj6vjx2218 .

observable:path rdfs:label "path"@en .

_:node1gm7uj6vjx2218 rdf:first "SCHED_E_ACCOUNT_NAME_NOT_FOUND"^^vocabulary:TaskStatusVocab .

observable:path rdfs:comment "Specifies the location of one object within another containing object."@en .

_:node1gm7uj6vjx2218 rdf:rest _:node1gm7uj6vjx2219 .

observable:path rdfs:range xsd:string .

_:node1gm7uj6vjx2219 rdf:first "SCHED_E_CANNOT_OPEN_TASK"^^vocabulary:TaskStatusVocab .

observable:pdfCreationDate a owl:DatatypeProperty .

_:node1gm7uj6vjx2219 rdf:rest _:node1gm7uj6vjx2220 .

observable:pdfCreationDate rdfs:label "pdfCreationDate"@en .

_:node1gm7uj6vjx2220 rdf:first "SCHED_E_INVALID_TASK"^^vocabulary:TaskStatusVocab .

observable:pdfCreationDate rdfs:comment "The PDF CreationDate property is defined in ISO 32000-1:2008 as 'The date and time the document was created, in human-readable form' (Table 317).  As a UCO property, its value is converted to xsd:dateTime."@en .

_:node1gm7uj6vjx2220 rdf:rest _:node1gm7uj6vjx2221 .

observable:pdfCreationDate rdfs:range xsd:dateTime .

_:node1gm7uj6vjx2221 rdf:first "SCHED_E_NO_SECURITY_SERVICES"^^vocabulary:TaskStatusVocab .

observable:pdfId0 a owl:DatatypeProperty .

_:node1gm7uj6vjx2221 rdf:rest _:node1gm7uj6vjx2222 .

observable:pdfId0 rdfs:label "pdfId0"@en .

_:node1gm7uj6vjx2222 rdf:first "SCHED_E_SERVICE_NOT_INSTALLED"^^vocabulary:TaskStatusVocab .

observable:pdfId0 rdfs:range xsd:string .

_:node1gm7uj6vjx2222 rdf:rest _:node1gm7uj6vjx2223 .

observable:pdfId1 a owl:DatatypeProperty .

_:node1gm7uj6vjx2223 rdf:first "SCHED_E_SERVICE_NOT_RUNNING"^^vocabulary:TaskStatusVocab .

observable:pdfId1 rdfs:label "pdfId1"@en .

_:node1gm7uj6vjx2223 rdf:rest _:node1gm7uj6vjx2224 .

observable:pdfId1 rdfs:range xsd:string .

_:node1gm7uj6vjx2224 rdf:first "SCHED_E_TASK_NOT_READY"^^vocabulary:TaskStatusVocab .

observable:pdfModDate a owl:DatatypeProperty .

_:node1gm7uj6vjx2224 rdf:rest _:node1gm7uj6vjx2225 .

observable:pdfModDate rdfs:label "pdfModDate"@en .

_:node1gm7uj6vjx2225 rdf:first "SCHED_E_TASK_NOT_RUNNING"^^vocabulary:TaskStatusVocab .

observable:pdfModDate rdfs:comment "The PDF ModDate property is defined in ISO 32000-1:2008 as 'The date and time the document was most recently modified, in human-readable form' (Table 317).  As a UCO property, its value is converted to xsd:dateTime."@en .

_:node1gm7uj6vjx2225 rdf:rest _:node1gm7uj6vjx2226 .

observable:pdfModDate rdfs:range xsd:dateTime .

_:node1gm7uj6vjx2226 rdf:first "SCHED_E_TRIGGER_NOT_FOUND"^^vocabulary:TaskStatusVocab .

observable:peType a owl:DatatypeProperty .

_:node1gm7uj6vjx2226 rdf:rest _:node1gm7uj6vjx2227 .

observable:peType rdfs:label "peType"@en .

_:node1gm7uj6vjx2227 rdf:first "SCHED_E_UNKNOWN_OBJECT_VERSION"^^vocabulary:TaskStatusVocab .

observable:peType rdfs:comment "Specifies the type of the PE binary."@en .

_:node1gm7uj6vjx2227 rdf:rest _:node1gm7uj6vjx2228 .

observable:peType rdfs:range xsd:string .

_:node1gm7uj6vjx2228 rdf:first "SCHED_E_UNSUPPORTED_ACCOUNT_OPTION"^^vocabulary:TaskStatusVocab .

observable:phoneActivationTime a owl:DatatypeProperty .

_:node1gm7uj6vjx2228 rdf:rest _:node1gm7uj6vjx2229 .

observable:phoneActivationTime rdfs:label "phoneActivationTime"@en .

_:node1gm7uj6vjx2229 rdf:first "SCHED_S_EVENT_TRIGGER"^^vocabulary:TaskStatusVocab .

observable:phoneActivationTime rdfs:comment "The date and time that a device was activated."@en .

_:node1gm7uj6vjx2229 rdf:rest _:node1gm7uj6vjx2230 .

observable:phoneActivationTime rdfs:range xsd:dateTime .

_:node1gm7uj6vjx2230 rdf:first "SCHED_S_TASK_DISABLED"^^vocabulary:TaskStatusVocab .

observable:phoneNumber a owl:DatatypeProperty .

_:node1gm7uj6vjx2230 rdf:rest _:node1gm7uj6vjx2231 .

observable:phoneNumber rdfs:label "phoneNumber"@en .

_:node1gm7uj6vjx2231 rdf:first "SCHED_S_TASK_HAS_NOT_RUN"^^vocabulary:TaskStatusVocab .

observable:phoneNumber rdfs:comment "A phone number(account)."@en .

_:node1gm7uj6vjx2231 rdf:rest _:node1gm7uj6vjx2232 .

observable:phoneNumber rdfs:range xsd:string .

_:node1gm7uj6vjx2232 rdf:first "SCHED_S_TASK_NOT_SCHEDULED"^^vocabulary:TaskStatusVocab .

observable:pictureHeight a owl:DatatypeProperty .

_:node1gm7uj6vjx2232 rdf:rest _:node1gm7uj6vjx2233 .

observable:pictureHeight rdfs:label "pictureHeight"@en .

_:node1gm7uj6vjx2233 rdf:first "SCHED_S_TASK_NO_MORE_RUNS"^^vocabulary:TaskStatusVocab .

observable:pictureHeight rdfs:range xsd:integer .

_:node1gm7uj6vjx2233 rdf:rest _:node1gm7uj6vjx2234 .

observable:pictureType a owl:DatatypeProperty .

_:node1gm7uj6vjx2234 rdf:first "SCHED_S_TASK_NO_VALID_TRIGGERS"^^vocabulary:TaskStatusVocab .

observable:pictureType rdfs:label "pictureType"@en .

_:node1gm7uj6vjx2234 rdf:rest _:node1gm7uj6vjx2235 .

observable:pictureType rdfs:comment "The type of a picture, for example a thumbnail."@en .

_:node1gm7uj6vjx2235 rdf:first "SCHED_S_TASK_READY"^^vocabulary:TaskStatusVocab .

observable:pictureType rdfs:range xsd:string .

_:node1gm7uj6vjx2235 rdf:rest _:node1gm7uj6vjx2236 .

observable:pictureWidth a owl:DatatypeProperty .

_:node1gm7uj6vjx2236 rdf:first "SCHED_S_TASK_RUNNING"^^vocabulary:TaskStatusVocab .

observable:pictureWidth rdfs:label "pictureWidth"@en .

_:node1gm7uj6vjx2236 rdf:rest _:node1gm7uj6vjx2237 .

observable:pictureWidth rdfs:comment "The width of the picture in pixels."@en .

_:node1gm7uj6vjx2237 rdf:first "SCHED_S_TASK_TERMINATED"^^vocabulary:TaskStatusVocab .

observable:pictureWidth rdfs:range xsd:integer .

_:node1gm7uj6vjx2237 rdf:rest _:node1gm7uj6vjx2238 .

observable:pid a owl:DatatypeProperty .

_:node1gm7uj6vjx2238 rdf:first "TASK_STATE_QUEUED"^^vocabulary:TaskStatusVocab .

observable:pid rdfs:label "pid"@en .

_:node1gm7uj6vjx2238 rdf:rest _:node1gm7uj6vjx2239 .

observable:pid rdfs:comment "The Process ID, or PID, of the process."@en .

_:node1gm7uj6vjx2239 rdf:first "TASK_STATE_UNKNOWN"^^vocabulary:TaskStatusVocab .

observable:pid rdfs:range xsd:integer .

_:node1gm7uj6vjx2239 rdf:rest rdf:nil .

observable:pointerToSymbolTable a owl:DatatypeProperty .

_:node1gm7uj6vjx2215 sh:in _:node1gm7uj6vjx2216 .

observable:pointerToSymbolTable rdfs:label "pointerToSymbolTable"@en .

_:node1gm7uj6vjx2214 rdf:first _:node1gm7uj6vjx2215 .

observable:pointerToSymbolTable rdfs:comment "Specifies the file offset of the COFF symbol table."@en .

_:node1gm7uj6vjx2214 rdf:rest _:node1gm7uj6vjx2240 .

observable:pointerToSymbolTable rdfs:range xsd:hexBinary .

_:node1gm7uj6vjx2241 sh:datatype xsd:string .

observable:policyConstraints a owl:DatatypeProperty .

_:node1gm7uj6vjx2240 rdf:first _:node1gm7uj6vjx2241 .

observable:policyConstraints rdfs:label "policyConstraints"@en .

_:node1gm7uj6vjx2240 rdf:rest rdf:nil .

observable:policyConstraints rdfs:range xsd:string .

_:node1gm7uj6vjx2213 sh:or _:node1gm7uj6vjx2214 .

observable:policyMappings a owl:DatatypeProperty .

_:node1gm7uj6vjx2213 sh:path observable:status .

observable:policyMappings rdfs:label "policyMappings"@en .

observable:WindowsTaskFacet sh:property _:node1gm7uj6vjx2213 .

observable:policyMappings rdfs:range xsd:string .

_:node1gm7uj6vjx2242 sh:nodeKind sh:Literal .

observable:port a owl:DatatypeProperty .

_:node1gm7uj6vjx2244 sh:datatype vocabulary:TaskFlagVocab .

observable:port rdfs:label "port"@en .

_:node1gm7uj6vjx2243 rdf:first _:node1gm7uj6vjx2244 .

observable:port rdfs:comment "Port on which communication takes place."@en .

_:node1gm7uj6vjx2243 rdf:rest _:node1gm7uj6vjx2245 .

observable:port rdfs:range xsd:integer .

_:node1gm7uj6vjx2246 sh:datatype xsd:string .

observable:prefetchHash a owl:DatatypeProperty .

_:node1gm7uj6vjx2245 rdf:first _:node1gm7uj6vjx2246 .

observable:prefetchHash rdfs:label "prefetchHash"@en .

_:node1gm7uj6vjx2245 rdf:rest rdf:nil .

observable:prefetchHash rdfs:comment "An eight character hash of the location from which the application was run."@en .

_:node1gm7uj6vjx2242 sh:or _:node1gm7uj6vjx2243 .

observable:prefetchHash rdfs:range xsd:string .

_:node1gm7uj6vjx2242 sh:path observable:flags .

observable:priority a owl:DatatypeProperty .

observable:WindowsTaskFacet sh:property _:node1gm7uj6vjx2242 .

observable:priority rdfs:label "priority"@en .

observable:WindowsTaskFacet sh:targetClass observable:WindowsTaskFacet .

observable:priority rdfs:comment "The priority of the email."@en .

observable:WindowsThread a owl:Class .

_:node1gm7uj6vjx2371 a rdfs:Datatype .

observable:WindowsThread a sh:NodeShape .

_:node1gm7uj6vjx2372 rdf:first xsd:integer .

observable:WindowsThread rdfs:subClassOf observable:ProcessThread .

_:node1gm7uj6vjx2372 rdf:rest _:node1gm7uj6vjx2373 .

observable:WindowsThread rdfs:label "WindowsThread"@en .

_:node1gm7uj6vjx2373 rdf:first xsd:string .

observable:WindowsThread rdfs:comment "A Windows thread is a single thread of execution within a Windows process."@en .

_:node1gm7uj6vjx2373 rdf:rest _:node1gm7uj6vjx2374 .

observable:WindowsThread sh:targetClass observable:WindowsThread .

_:node1gm7uj6vjx2374 rdf:first vocabulary:TaskPriorityVocab .

observable:WindowsThreadFacet a owl:Class .

_:node1gm7uj6vjx2374 rdf:rest rdf:nil .

observable:WindowsThreadFacet a sh:NodeShape .

_:node1gm7uj6vjx2371 owl:unionOf _:node1gm7uj6vjx2372 .

observable:WindowsThreadFacet rdfs:subClassOf core:Facet .

observable:priority rdfs:range _:node1gm7uj6vjx2371 .

observable:WindowsThreadFacet rdfs:label "WindowsThreadFacet"@en .

observable:privateKeyUsagePeriodNotAfter a owl:DatatypeProperty .

observable:WindowsThreadFacet rdfs:comment "A Windows thread facet is a grouping os characteristics unique to a single thread of execution within a Windows process."@en .

observable:privateKeyUsagePeriodNotAfter rdfs:label "privateKeyUsagePeriodNotAfter"@en .

_:node1gm7uj6vjx2247 sh:datatype xsd:dateTime .

observable:privateKeyUsagePeriodNotAfter rdfs:range xsd:dateTime .

_:node1gm7uj6vjx2247 sh:maxCount 1 .

observable:privateKeyUsagePeriodNotBefore a owl:DatatypeProperty .

_:node1gm7uj6vjx2247 sh:nodeKind sh:Literal .

observable:privateKeyUsagePeriodNotBefore rdfs:label "privateKeyUsagePeriodNotBefore"@en .

_:node1gm7uj6vjx2247 sh:path observable:creationTime .

observable:privateKeyUsagePeriodNotBefore rdfs:range xsd:dateTime .

observable:WindowsThreadFacet sh:property _:node1gm7uj6vjx2247 .

observable:processorArchitecture a owl:DatatypeProperty .

_:node1gm7uj6vjx2248 sh:datatype xsd:hexBinary .

observable:processorArchitecture rdfs:label "processorArchitecture"@en .

_:node1gm7uj6vjx2248 sh:nodeKind sh:Literal .

observable:processorArchitecture rdfs:comment "Specifies the specific architecture (e.g. x86) used by the CPU of the system."@en .

_:node1gm7uj6vjx2248 sh:path observable:parameterAddress .

observable:processorArchitecture rdfs:range xsd:string .

observable:WindowsThreadFacet sh:property _:node1gm7uj6vjx2248 .

observable:profile a owl:ObjectProperty .

_:node1gm7uj6vjx2249 sh:datatype xsd:hexBinary .

observable:profile rdfs:label "profile"@en .

_:node1gm7uj6vjx2249 sh:nodeKind sh:Literal .

observable:profile rdfs:comment "A profile specifies a particular online service profile."@en .

_:node1gm7uj6vjx2249 sh:path observable:startAddress .

observable:profile rdfs:range observable:ObservableObject .

observable:WindowsThreadFacet sh:property _:node1gm7uj6vjx2249 .

observable:profileAccount a owl:ObjectProperty .

_:node1gm7uj6vjx2250 sh:datatype xsd:integer .

observable:profileAccount rdfs:label "Profile Account"@en-us .

_:node1gm7uj6vjx2250 sh:maxCount 1 .

observable:profileAccount rdfs:comment "Specifies the online service account associated with the profile."@en-us .

_:node1gm7uj6vjx2250 sh:nodeKind sh:Literal .

observable:profileAccount rdfs:range observable:ObservableObject .

_:node1gm7uj6vjx2250 sh:path observable:priority .

observable:profileBackgroundHash a owl:ObjectProperty .

observable:WindowsThreadFacet sh:property _:node1gm7uj6vjx2250 .

observable:profileBackgroundHash rdfs:label "Profile Background Hash"@en-us .

_:node1gm7uj6vjx2251 sh:datatype xsd:nonNegativeInteger .

observable:profileBackgroundHash rdfs:comment "Specifies hashes of the background associated with the profile."@en-us .

_:node1gm7uj6vjx2251 sh:nodeKind sh:Literal .

observable:profileBackgroundHash rdfs:range types:Hash .

_:node1gm7uj6vjx2251 sh:path observable:stackSize .

observable:profileBackgroundLocation a owl:ObjectProperty .

observable:WindowsThreadFacet sh:property _:node1gm7uj6vjx2251 .

observable:profileBackgroundLocation rdfs:label "Profile Background Location"@en-us .

_:node1gm7uj6vjx2252 sh:datatype xsd:nonNegativeInteger .

observable:profileBackgroundLocation rdfs:comment "Specifies the network location of the background associated with the profile."@en-us .

_:node1gm7uj6vjx2252 sh:nodeKind sh:Literal .

observable:profileBackgroundLocation rdfs:range observable:ObservableObject .

_:node1gm7uj6vjx2252 sh:path observable:threadID .

observable:profileBannerHash a owl:ObjectProperty .

observable:WindowsThreadFacet sh:property _:node1gm7uj6vjx2252 .

observable:profileBannerHash rdfs:label "Profile Banner Hash"@en-us .

_:node1gm7uj6vjx2253 sh:datatype xsd:string .

observable:profileBannerHash rdfs:comment "Specifies hashes of the banner associated with the profile."@en-us .

_:node1gm7uj6vjx2253 sh:maxCount 1 .

observable:profileBannerHash rdfs:range types:Hash .

_:node1gm7uj6vjx2253 sh:nodeKind sh:Literal .

observable:profileBannerLocation a owl:ObjectProperty .

_:node1gm7uj6vjx2253 sh:path observable:context .

observable:profileBannerLocation rdfs:label "Profile Banner Location"@en-us .

observable:WindowsThreadFacet sh:property _:node1gm7uj6vjx2253 .

observable:profileBannerLocation rdfs:comment "Specifies the network location of the banner associated with the profile."@en-us .

_:node1gm7uj6vjx2254 sh:datatype xsd:string .

observable:profileBannerLocation rdfs:range observable:ObservableObject .

_:node1gm7uj6vjx2254 sh:maxCount 1 .

observable:profileCreated a owl:DatatypeProperty .

_:node1gm7uj6vjx2254 sh:nodeKind sh:Literal .

observable:profileCreated rdfs:label "Profile Created"@en-us .

_:node1gm7uj6vjx2254 sh:path observable:runningStatus .

observable:profileCreated rdfs:comment "Specifies the date and time the profile was created."@en-us .

observable:WindowsThreadFacet sh:property _:node1gm7uj6vjx2254 .

observable:profileCreated rdfs:range xsd:dateTime .

_:node1gm7uj6vjx2255 sh:datatype xsd:string .

observable:profileIdentity a owl:ObjectProperty .

_:node1gm7uj6vjx2255 sh:maxCount 1 .

observable:profileIdentity rdfs:label "Profile Identity"@en-us .

_:node1gm7uj6vjx2255 sh:nodeKind sh:Literal .

observable:profileIdentity rdfs:comment "Specifies the identity associated with the profile."@en-us .

_:node1gm7uj6vjx2255 sh:path observable:securityAttributes .

observable:profileIdentity rdfs:range identity:Identity .

observable:WindowsThreadFacet sh:property _:node1gm7uj6vjx2255 .

observable:profileImageHash a owl:ObjectProperty .

_:node1gm7uj6vjx2256 sh:datatype xsd:unsignedInt .

observable:profileImageHash rdfs:label "Profile Image Hash"@en-us .

_:node1gm7uj6vjx2256 sh:nodeKind sh:Literal .

observable:profileImageHash rdfs:comment "Specifies hashes of the profile image associated with the profile."@en-us .

_:node1gm7uj6vjx2256 sh:path observable:creationFlags .

observable:profileImageHash rdfs:range types:Hash .

observable:WindowsThreadFacet sh:property _:node1gm7uj6vjx2256 .

observable:profileImageLocation a owl:ObjectProperty .

observable:WindowsThreadFacet sh:targetClass observable:WindowsThreadFacet .

observable:profileImageLocation rdfs:label "Profile Image Location"@en-us .

observable:WindowsVolumeFacet a owl:Class .

observable:profileImageLocation rdfs:comment "Specifies the network location of the profile image associated with the profile."@en-us .

observable:WindowsVolumeFacet a sh:NodeShape .

observable:profileImageLocation rdfs:range observable:ObservableObject .

observable:WindowsVolumeFacet rdfs:subClassOf core:Facet .

observable:profileIsProtected a owl:DatatypeProperty .

observable:WindowsVolumeFacet rdfs:label "WindowsVolumeFacet"@en .

observable:profileIsProtected rdfs:label "Is_Protected"@en-us .

observable:WindowsVolumeFacet rdfs:comment "A Windows volume facet is a grouping of characteristics unique to a single accessible storage area (volume) with a single Windows file system. [based on https://en.wikipedia.org/wiki/Volume_(computing)]"@en .

observable:profileIsProtected rdfs:comment "Specifies whether the twitter profile is protected."@en-us .

_:node1gm7uj6vjx2257 sh:datatype xsd:string .

observable:profileIsProtected rdfs:range xsd:boolean .

_:node1gm7uj6vjx2257 sh:maxCount 1 .

observable:profileIsVerified a owl:DatatypeProperty .

_:node1gm7uj6vjx2257 sh:nodeKind sh:Literal .

observable:profileIsVerified rdfs:label "Is_Verified"@en-us .

_:node1gm7uj6vjx2257 sh:path observable:driveLetter .

observable:profileIsVerified rdfs:comment "Specifies whether the twitter profile is verified."@en-us .

observable:WindowsVolumeFacet sh:property _:node1gm7uj6vjx2257 .

observable:profileIsVerified rdfs:range xsd:boolean .

_:node1gm7uj6vjx2258 sh:datatype vocabulary:WindowsDriveTypeVocab .

observable:profileLanguage a owl:DatatypeProperty .

_:node1gm7uj6vjx2258 sh:message "Value is outside the default vocabulary WindowsDriveTypeVocab." .

observable:profileLanguage rdfs:label "Profile Language"@en-us .

_:node1gm7uj6vjx2258 sh:path observable:driveType .

observable:profileLanguage rdfs:comment "Specifies the language associated with the profile. When present, it MUST be a language code conformant to RFC 5646/BCP47."@en-us .

_:node1gm7uj6vjx2258 sh:severity sh:Info .

observable:profileLanguage rdfs:range xsd:string .

observable:WindowsVolumeFacet sh:property _:node1gm7uj6vjx2258 .

observable:profileService a owl:ObjectProperty .

_:node1gm7uj6vjx2259 sh:datatype vocabulary:WindowsVolumeAttributeVocab .

observable:profileService rdfs:label "Profile Service"@en-us .

_:node1gm7uj6vjx2259 sh:maxCount 4 .

observable:profileService rdfs:comment "Specifies the online service associated with the profile."@en-us .

_:node1gm7uj6vjx2259 sh:nodeKind sh:Literal .

observable:profileService rdfs:range observable:ObservableObject .

_:node1gm7uj6vjx2259 sh:path observable:windowsVolumeAttributes .

observable:profileWebsite a owl:ObjectProperty .

observable:WindowsVolumeFacet sh:property _:node1gm7uj6vjx2259 .

observable:profileWebsite rdfs:label "Profile Website"@en-us .

_:node1gm7uj6vjx2260 sh:maxCount 1 .

observable:profileWebsite rdfs:comment "Specifies the website URL associated with the profile."@en-us .

_:node1gm7uj6vjx2260 sh:nodeKind sh:Literal .

observable:profileWebsite rdfs:range observable:ObservableObject .

_:node1gm7uj6vjx2262 sh:datatype vocabulary:WindowsDriveTypeVocab .

observable:properties a owl:DatatypeProperty .

_:node1gm7uj6vjx2261 rdf:first _:node1gm7uj6vjx2262 .

observable:properties rdfs:label "properties"@en .

_:node1gm7uj6vjx2261 rdf:rest _:node1gm7uj6vjx2263 .

observable:properties rdfs:comment "Specifies the properties that were enumerated as a result of the action on the observable object."@en .

_:node1gm7uj6vjx2264 sh:datatype xsd:string .

observable:properties rdfs:range xsd:string .

_:node1gm7uj6vjx2263 rdf:first _:node1gm7uj6vjx2264 .

observable:propertyName a owl:DatatypeProperty .

_:node1gm7uj6vjx2263 rdf:rest rdf:nil .

observable:propertyName rdfs:label "propertyName"@en .

_:node1gm7uj6vjx2260 sh:or _:node1gm7uj6vjx2261 .

observable:propertyName rdfs:comment "Specifies the Name of the property being read."@en .

_:node1gm7uj6vjx2260 sh:path observable:driveType .

observable:propertyName rdfs:range xsd:string .

observable:WindowsVolumeFacet sh:property _:node1gm7uj6vjx2260 .

observable:protocols a owl:ObjectProperty .

_:node1gm7uj6vjx2265 sh:message "Value is not member of the vocabulary WindowsDriveTypeVocab." .

observable:protocols rdfs:label "protocols"@en .

_:node1gm7uj6vjx2267 sh:datatype vocabulary:WindowsDriveTypeVocab .

observable:protocols rdfs:comment "Specifies the protocols involved in the network connection, along with their corresponding state. "@en .

_:node1gm7uj6vjx2268 rdf:first "DRIVE_CDROM"^^vocabulary:WindowsDriveTypeVocab .

observable:protocols rdfs:range types:ControlledDictionary .

_:node1gm7uj6vjx2268 rdf:rest _:node1gm7uj6vjx2269 .

observable:query a owl:DatatypeProperty .

_:node1gm7uj6vjx2269 rdf:first "DRIVE_FIXED"^^vocabulary:WindowsDriveTypeVocab .

observable:query rdfs:label "query"@en .

_:node1gm7uj6vjx2269 rdf:rest _:node1gm7uj6vjx2270 .

observable:query rdfs:comment "Query passed to the resource."@en .

_:node1gm7uj6vjx2270 rdf:first "DRIVE_NO_ROOT_DIR"^^vocabulary:WindowsDriveTypeVocab .

observable:query rdfs:range xsd:string .

_:node1gm7uj6vjx2270 rdf:rest _:node1gm7uj6vjx2271 .

observable:rangeOffset a owl:DatatypeProperty .

_:node1gm7uj6vjx2271 rdf:first "DRIVE_RAMDISK"^^vocabulary:WindowsDriveTypeVocab .

observable:rangeOffset rdfs:label "rangeOffset"@en .

_:node1gm7uj6vjx2271 rdf:rest _:node1gm7uj6vjx2272 .

observable:rangeOffset rdfs:comment "The offset at which the start of data can be found, relative to the rangeOffsetType defined."@en .

_:node1gm7uj6vjx2272 rdf:first "DRIVE_REMOTE"^^vocabulary:WindowsDriveTypeVocab .

observable:rangeOffset rdfs:range xsd:integer .

_:node1gm7uj6vjx2272 rdf:rest _:node1gm7uj6vjx2273 .

observable:rangeOffsetType a owl:DatatypeProperty .

_:node1gm7uj6vjx2273 rdf:first "DRIVE_REMOVABLE"^^vocabulary:WindowsDriveTypeVocab .

observable:rangeOffsetType rdfs:label "rangeOffsetType"@en .

_:node1gm7uj6vjx2273 rdf:rest _:node1gm7uj6vjx2274 .

observable:rangeOffsetType rdfs:comment "The type of offset defined for the range (e.g., image, file, address)."@en .

_:node1gm7uj6vjx2274 rdf:first "DRIVE_UNKNOWN"^^vocabulary:WindowsDriveTypeVocab .

observable:rangeOffsetType rdfs:range xsd:string .

_:node1gm7uj6vjx2274 rdf:rest rdf:nil .

observable:rangeSize a owl:DatatypeProperty .

_:node1gm7uj6vjx2267 sh:in _:node1gm7uj6vjx2268 .

observable:rangeSize rdfs:label "rangeSize"@en .

_:node1gm7uj6vjx2266 rdf:first _:node1gm7uj6vjx2267 .

observable:rangeSize rdfs:comment "The size of the data in bytes."@en .

_:node1gm7uj6vjx2266 rdf:rest _:node1gm7uj6vjx2275 .

observable:rangeSize rdfs:range xsd:integer .

_:node1gm7uj6vjx2276 sh:datatype xsd:string .

observable:receivedLines a owl:DatatypeProperty .

_:node1gm7uj6vjx2275 rdf:first _:node1gm7uj6vjx2276 .

observable:receivedLines rdfs:label "receivedLines"@en .

_:node1gm7uj6vjx2275 rdf:rest rdf:nil .

observable:receivedLines rdfs:range xsd:string .

_:node1gm7uj6vjx2265 sh:or _:node1gm7uj6vjx2266 .

observable:receivedTime a owl:DatatypeProperty .

_:node1gm7uj6vjx2265 sh:path observable:driveType .

observable:receivedTime rdfs:label "receivedTime"@en .

observable:WindowsVolumeFacet sh:property _:node1gm7uj6vjx2265 .

observable:receivedTime rdfs:comment "The date and time at which the message received. "@en .

observable:WindowsVolumeFacet sh:targetClass observable:WindowsVolumeFacet .

observable:receivedTime rdfs:range xsd:dateTime .

observable:WindowsWaitableTime a owl:Class .

observable:recordFieldIsNull a owl:DatatypeProperty .

observable:WindowsWaitableTime a sh:NodeShape .

observable:recordFieldIsNull rdfs:label "recordFieldIsNull"@en .

observable:WindowsWaitableTime rdfs:subClassOf observable:ObservableObject .

observable:recordFieldIsNull rdfs:comment "Whether the specified database record field is null."@en .

observable:WindowsWaitableTime rdfs:label "WindowsWaitableTime"@en .

observable:recordFieldIsNull rdfs:range xsd:boolean .

observable:WindowsWaitableTime rdfs:comment "A Windows waitable timer is a synchronization object within the Windows operating system whose state is set to signaled when a specified due time arrives. There are two types of waitable timers that can be created: manual-reset and synchronization. A timer of either type can also be a periodic timer. [based on https://docs.microsoft.com/en-us/windows/win32/sync/waitable-timer-objects]"@en .

observable:recordFieldName a owl:DatatypeProperty .

observable:WindowsWaitableTime sh:targetClass observable:WindowsWaitableTime .

observable:recordFieldName rdfs:label "recordFieldName"@en .

observable:WirelessNetworkConnection a owl:Class .

observable:recordFieldName rdfs:comment "A field name of a database record value being identified."@en .

observable:WirelessNetworkConnection a sh:NodeShape .

observable:recordFieldName rdfs:range xsd:string .

observable:WirelessNetworkConnection rdfs:subClassOf observable:NetworkConnection .

observable:recordFieldValue a owl:DatatypeProperty .

observable:WirelessNetworkConnection rdfs:label "WirelessNetworkConnection"@en .

observable:recordFieldValue rdfs:label "recordFieldValue"@en .

observable:WirelessNetworkConnection rdfs:comment "A wireless network connection is a connection (completed or attempted) across an IEEE 802.11 standards-confromant digital network (a group of two or more computer systems linked together). [based on https://www.webopedia.com/TERM/N/network.html]"@en .

observable:recordFieldValue rdfs:comment "The field value of a specified database record."@en .

observable:WirelessNetworkConnection sh:targetClass observable:WirelessNetworkConnection .

_:node1gm7uj6vjx2375 a rdfs:Datatype .

observable:WirelessNetworkConnectionFacet a owl:Class .

_:node1gm7uj6vjx2376 rdf:first xsd:base64Binary .

observable:WirelessNetworkConnectionFacet a sh:NodeShape .

_:node1gm7uj6vjx2376 rdf:rest _:node1gm7uj6vjx2377 .

observable:WirelessNetworkConnectionFacet rdfs:subClassOf core:Facet .

_:node1gm7uj6vjx2377 rdf:first xsd:decimal .

observable:WirelessNetworkConnectionFacet rdfs:label "WirelessNetworkConnectionFacet"@en .

_:node1gm7uj6vjx2377 rdf:rest _:node1gm7uj6vjx2378 .

observable:WirelessNetworkConnectionFacet rdfs:comment "A wireless network connection facet is a grouping of characteristics unique to a connection (completed or attempted) across an IEEE 802.11 standards-conformant digital network (a group of two or more computer systems linked together). [based on https://www.webopedia.com/TERM/N/network.html]"@en .

_:node1gm7uj6vjx2378 rdf:first xsd:integer .

_:node1gm7uj6vjx2277 sh:datatype xsd:string .

_:node1gm7uj6vjx2378 rdf:rest _:node1gm7uj6vjx2379 .

_:node1gm7uj6vjx2277 sh:maxCount 1 .

_:node1gm7uj6vjx2379 rdf:first xsd:string .

_:node1gm7uj6vjx2277 sh:nodeKind sh:Literal .

_:node1gm7uj6vjx2379 rdf:rest rdf:nil .

_:node1gm7uj6vjx2277 sh:path observable:baseStation .

_:node1gm7uj6vjx2375 owl:unionOf _:node1gm7uj6vjx2376 .

observable:WirelessNetworkConnectionFacet sh:property _:node1gm7uj6vjx2277 .

observable:recordFieldValue rdfs:range _:node1gm7uj6vjx2375 .

_:node1gm7uj6vjx2278 sh:datatype xsd:string .

observable:recordRowID a owl:DatatypeProperty .

_:node1gm7uj6vjx2278 sh:maxCount 1 .

observable:recordRowID rdfs:label "recordRowID"@en .

_:node1gm7uj6vjx2278 sh:nodeKind sh:Literal .

observable:recordRowID rdfs:comment "The unique ID that identifies a database record, supplied by the originating database engine."@en .

_:node1gm7uj6vjx2278 sh:path observable:password .

_:node1gm7uj6vjx2380 a rdfs:Datatype .

observable:WirelessNetworkConnectionFacet sh:property _:node1gm7uj6vjx2278 .

_:node1gm7uj6vjx2381 rdf:first xsd:integer .

_:node1gm7uj6vjx2279 sh:datatype xsd:string .

_:node1gm7uj6vjx2381 rdf:rest _:node1gm7uj6vjx2382 .

_:node1gm7uj6vjx2279 sh:maxCount 1 .

_:node1gm7uj6vjx2382 rdf:first xsd:string .

_:node1gm7uj6vjx2279 sh:nodeKind sh:Literal .

_:node1gm7uj6vjx2382 rdf:rest rdf:nil .

_:node1gm7uj6vjx2279 sh:path observable:ssid .

_:node1gm7uj6vjx2380 owl:unionOf _:node1gm7uj6vjx2381 .

observable:WirelessNetworkConnectionFacet sh:property _:node1gm7uj6vjx2279 .

observable:recordRowID rdfs:range _:node1gm7uj6vjx2380 .

_:node1gm7uj6vjx2280 sh:maxCount 1 .

observable:recurrence a owl:DatatypeProperty .

_:node1gm7uj6vjx2280 sh:nodeKind sh:Literal .

observable:recurrence rdfs:label "recurrence"@en .

_:node1gm7uj6vjx2282 sh:datatype vocabulary:WirelessNetworkSecurityModeVocab .

observable:recurrence rdfs:comment "Recurrence of the event."@en .

_:node1gm7uj6vjx2281 rdf:first _:node1gm7uj6vjx2282 .

observable:recurrence rdfs:range xsd:string .

_:node1gm7uj6vjx2281 rdf:rest _:node1gm7uj6vjx2283 .

observable:references a owl:ObjectProperty .

_:node1gm7uj6vjx2284 sh:datatype xsd:string .

observable:references rdfs:label "references"@en .

_:node1gm7uj6vjx2283 rdf:first _:node1gm7uj6vjx2284 .

observable:references rdfs:comment "A list of email message identifiers this email relates to."@en .

_:node1gm7uj6vjx2283 rdf:rest rdf:nil .

observable:references rdfs:range observable:ObservableObject .

_:node1gm7uj6vjx2280 sh:or _:node1gm7uj6vjx2281 .

observable:referralURL a owl:ObjectProperty .

_:node1gm7uj6vjx2280 sh:path observable:wirelessNetworkSecurityMode .

observable:referralURL rdfs:label "referralURL"@en .

observable:WirelessNetworkConnectionFacet sh:property _:node1gm7uj6vjx2280 .

observable:referralURL rdfs:comment "Specifies the corresponding referral URL for a registrar."@en .

_:node1gm7uj6vjx2285 sh:message "Value is not member of the vocabulary WirelessNetworkSecurityModeVocab." .

observable:referralURL rdfs:range observable:ObservableObject .

_:node1gm7uj6vjx2287 sh:datatype vocabulary:WirelessNetworkSecurityModeVocab .

observable:referrerUrl a owl:ObjectProperty .

_:node1gm7uj6vjx2288 rdf:first "None"^^vocabulary:WirelessNetworkSecurityModeVocab .

observable:referrerUrl rdfs:label "referrerURL"@en .

_:node1gm7uj6vjx2288 rdf:rest _:node1gm7uj6vjx2289 .

observable:referrerUrl rdfs:comment "Specifies the origination point (i.e., URL) of a URL request."@en .

_:node1gm7uj6vjx2289 rdf:first "WEP"^^vocabulary:WirelessNetworkSecurityModeVocab .

observable:referrerUrl rdfs:range observable:ObservableObject .

_:node1gm7uj6vjx2289 rdf:rest _:node1gm7uj6vjx2290 .

observable:regionEndAddress a owl:DatatypeProperty .

_:node1gm7uj6vjx2290 rdf:first "WPA"^^vocabulary:WirelessNetworkSecurityModeVocab .

observable:regionEndAddress rdfs:label "regionEndAddress"@en .

_:node1gm7uj6vjx2290 rdf:rest _:node1gm7uj6vjx2291 .

observable:regionEndAddress rdfs:comment "The regionEndAddress property specifies the ending address of the particular memory region."@en .

_:node1gm7uj6vjx2291 rdf:first "WPA2-PSK"^^vocabulary:WirelessNetworkSecurityModeVocab .

observable:regionEndAddress rdfs:range xsd:hexBinary .

_:node1gm7uj6vjx2291 rdf:rest _:node1gm7uj6vjx2292 .

observable:regionSize a owl:DatatypeProperty .

_:node1gm7uj6vjx2292 rdf:first "WPA2-Enterprise"^^vocabulary:WirelessNetworkSecurityModeVocab .

observable:regionSize rdfs:label "regionSize"@en .

_:node1gm7uj6vjx2292 rdf:rest _:node1gm7uj6vjx2293 .

observable:regionSize rdfs:comment "The regionSize property specifies the size of the particular memory region, in bytes."@en .

_:node1gm7uj6vjx2293 rdf:first "WPA3-PSK"^^vocabulary:WirelessNetworkSecurityModeVocab .

observable:regionSize rdfs:range xsd:integer .

_:node1gm7uj6vjx2293 rdf:rest _:node1gm7uj6vjx2294 .

observable:regionStartAddress a owl:DatatypeProperty .

_:node1gm7uj6vjx2294 rdf:first "WPA3-Enterprise"^^vocabulary:WirelessNetworkSecurityModeVocab .

observable:regionStartAddress rdfs:label "regionStartAddress"@en .

_:node1gm7uj6vjx2294 rdf:rest rdf:nil .

observable:regionStartAddress rdfs:comment """The regionStartAddress property specifies the starting address of the particular memory region.
          """@en .

_:node1gm7uj6vjx2287 sh:in _:node1gm7uj6vjx2288 .

observable:regionStartAddress rdfs:range xsd:hexBinary .

_:node1gm7uj6vjx2286 rdf:first _:node1gm7uj6vjx2287 .

observable:regionalInternetRegistry a owl:DatatypeProperty .

_:node1gm7uj6vjx2286 rdf:rest _:node1gm7uj6vjx2295 .

observable:regionalInternetRegistry rdfs:label "regionalInternetRegistry"@en .

_:node1gm7uj6vjx2296 sh:datatype xsd:string .

observable:regionalInternetRegistry rdfs:comment "specifies the name of the Regional Internet Registry (RIR) which allocated the IP address contained in a WHOIS entry."@en .

_:node1gm7uj6vjx2295 rdf:first _:node1gm7uj6vjx2296 .

_:node1gm7uj6vjx2383 a rdfs:Datatype .

_:node1gm7uj6vjx2295 rdf:rest rdf:nil .

_:node1gm7uj6vjx2384 rdf:first vocabulary:RegionalRegistryTypeVocab .

_:node1gm7uj6vjx2285 sh:or _:node1gm7uj6vjx2286 .

_:node1gm7uj6vjx2384 rdf:rest _:node1gm7uj6vjx2385 .

_:node1gm7uj6vjx2285 sh:path observable:wirelessNetworkSecurityMode .

_:node1gm7uj6vjx2385 rdf:first xsd:string .

observable:WirelessNetworkConnectionFacet sh:property _:node1gm7uj6vjx2285 .

_:node1gm7uj6vjx2385 rdf:rest rdf:nil .

observable:WirelessNetworkConnectionFacet sh:targetClass observable:WirelessNetworkConnectionFacet .

_:node1gm7uj6vjx2383 owl:unionOf _:node1gm7uj6vjx2384 .

observable:WriteBlocker a owl:Class .

observable:regionalInternetRegistry rdfs:range _:node1gm7uj6vjx2383 .

observable:WriteBlocker a sh:NodeShape .

observable:regionalInternetRegistry-shape-value-not-vocabulary-member a sh:PropertyShape .

observable:WriteBlocker rdfs:subClassOf observable:Device .

observable:regionalInternetRegistry-shape-value-not-vocabulary-member sh:message "Value is not member of the vocabulary RegionalRegistryTypeVocab." .

observable:WriteBlocker rdfs:label "WriteBlocker"@en-us .

_:node1gm7uj6vjx2387 sh:datatype vocabulary:RegionalRegistryTypeVocab .

observable:WriteBlocker rdfs:comment "A write blocker is a device that allows read-only access to storage mediums in order to preserve the integrity of the data being analyzed. Examples include Tableau, Cellibrite, Talon, etc."@en-us .

_:node1gm7uj6vjx2388 rdf:first "APNIC"^^vocabulary:RegionalRegistryTypeVocab .

observable:WriteBlocker sh:targetClass observable:WriteBlocker .

_:node1gm7uj6vjx2388 rdf:rest _:node1gm7uj6vjx2389 .

observable:X509Certificate a owl:Class .

_:node1gm7uj6vjx2389 rdf:first "ARIN"^^vocabulary:RegionalRegistryTypeVocab .

observable:X509Certificate a sh:NodeShape .

_:node1gm7uj6vjx2389 rdf:rest _:node1gm7uj6vjx2390 .

observable:X509Certificate rdfs:subClassOf observable:ObservableObject .

_:node1gm7uj6vjx2390 rdf:first "AfriNIC"^^vocabulary:RegionalRegistryTypeVocab .

observable:X509Certificate rdfs:label "X509Certificate"@en .

_:node1gm7uj6vjx2390 rdf:rest _:node1gm7uj6vjx2391 .

observable:X509Certificate rdfs:comment "A X.509 certificate is a public key digital identity certificate conformant to the X.509 PKI (Public Key Infrastructure) standard."@en .

_:node1gm7uj6vjx2391 rdf:first "LACNIC"^^vocabulary:RegionalRegistryTypeVocab .

observable:X509Certificate sh:targetClass observable:X509Certificate .

_:node1gm7uj6vjx2391 rdf:rest _:node1gm7uj6vjx2392 .

observable:X509CertificateFacet a owl:Class .

_:node1gm7uj6vjx2392 rdf:first "RIPE NCC"^^vocabulary:RegionalRegistryTypeVocab .

observable:X509CertificateFacet a sh:NodeShape .

_:node1gm7uj6vjx2392 rdf:rest rdf:nil .

observable:X509CertificateFacet rdfs:subClassOf core:Facet .

_:node1gm7uj6vjx2387 sh:in _:node1gm7uj6vjx2388 .

observable:X509CertificateFacet rdfs:label "X509CertificateFacet"@en .

_:node1gm7uj6vjx2386 rdf:first _:node1gm7uj6vjx2387 .

observable:X509CertificateFacet rdfs:comment "A X.509 certificate facet is a grouping of characteristics unique to a public key digital identity certificate conformant to the X.509 PKI (Public Key Infrastructure) standard. "@en .

_:node1gm7uj6vjx2386 rdf:rest _:node1gm7uj6vjx2393 .

_:node1gm7uj6vjx2297 sh:class observable:X509V3ExtensionsFacet .

_:node1gm7uj6vjx2394 sh:datatype xsd:string .

_:node1gm7uj6vjx2297 sh:maxCount 1 .

_:node1gm7uj6vjx2393 rdf:first _:node1gm7uj6vjx2394 .

_:node1gm7uj6vjx2297 sh:nodeKind sh:IRI .

_:node1gm7uj6vjx2393 rdf:rest rdf:nil .

_:node1gm7uj6vjx2297 sh:path observable:x509v3extensions .

observable:regionalInternetRegistry-shape-value-not-vocabulary-member sh:or _:node1gm7uj6vjx2386 .

observable:X509CertificateFacet sh:property _:node1gm7uj6vjx2297 .

observable:regionalInternetRegistry-shape-value-not-vocabulary-member sh:path observable:regionalInternetRegistry .

_:node1gm7uj6vjx2298 sh:class types:Hash .

observable:regionalInternetRegistry-shape-value-outside-default-vocabulary a sh:PropertyShape .

_:node1gm7uj6vjx2298 sh:maxCount 1 .

observable:regionalInternetRegistry-shape-value-outside-default-vocabulary sh:datatype vocabulary:RegionalRegistryTypeVocab .

_:node1gm7uj6vjx2298 sh:nodeKind sh:IRI .

observable:regionalInternetRegistry-shape-value-outside-default-vocabulary sh:message "Value is outside the default vocabulary RegionalRegistryTypeVocab." .

_:node1gm7uj6vjx2298 sh:path observable:issuerHash .

observable:regionalInternetRegistry-shape-value-outside-default-vocabulary sh:path observable:regionalInternetRegistry .

observable:X509CertificateFacet sh:property _:node1gm7uj6vjx2298 .

observable:regionalInternetRegistry-shape-value-outside-default-vocabulary sh:severity sh:Info .

_:node1gm7uj6vjx2299 sh:class types:Hash .

observable:registeredOrganization a owl:ObjectProperty .

_:node1gm7uj6vjx2299 sh:maxCount 1 .

observable:registeredOrganization rdfs:label "registeredOrganization"@en .

_:node1gm7uj6vjx2299 sh:nodeKind sh:IRI .

observable:registeredOrganization rdfs:comment "The organization that this copy of Windows is registered to."@en .

_:node1gm7uj6vjx2299 sh:path observable:subjectHash .

observable:registeredOrganization rdfs:range identity:Identity .

observable:X509CertificateFacet sh:property _:node1gm7uj6vjx2299 .

observable:registeredOwner a owl:ObjectProperty .

_:node1gm7uj6vjx2300 sh:class types:Hash .

observable:registeredOwner rdfs:label "registeredOwner"@en .

_:node1gm7uj6vjx2300 sh:maxCount 1 .

observable:registeredOwner rdfs:comment "The person or organization that is the registered owner of this copy of Windows."@en .

_:node1gm7uj6vjx2300 sh:nodeKind sh:IRI .

observable:registeredOwner rdfs:range identity:Identity .

_:node1gm7uj6vjx2300 sh:path observable:thumbprintHash .

observable:registrantContactInfo a owl:ObjectProperty .

observable:X509CertificateFacet sh:property _:node1gm7uj6vjx2300 .

observable:registrantContactInfo rdfs:label "registrantContactInfo"@en .

_:node1gm7uj6vjx2301 sh:datatype xsd:boolean .

observable:registrantContactInfo rdfs:comment "Specifies contact info for the registrant of a domain within a WHOIS entity."@en .

_:node1gm7uj6vjx2301 sh:maxCount 1 .

observable:registrantContactInfo rdfs:range observable:ObservableObject .

_:node1gm7uj6vjx2301 sh:nodeKind sh:Literal .

observable:registrantIDs a owl:DatatypeProperty .

_:node1gm7uj6vjx2301 sh:path observable:isSelfSigned .

observable:registrantIDs rdfs:label "registrantIDs"@en .

observable:X509CertificateFacet sh:property _:node1gm7uj6vjx2301 .

observable:registrantIDs rdfs:comment "Specifies the registrant IDs associated with a domain lookup."@en .

_:node1gm7uj6vjx2302 sh:datatype xsd:dateTime .

observable:registrantIDs rdfs:range xsd:string .

_:node1gm7uj6vjx2302 sh:maxCount 1 .

observable:registrarGUID a owl:DatatypeProperty .

_:node1gm7uj6vjx2302 sh:nodeKind sh:Literal .

observable:registrarGUID rdfs:label "registrarGUID"@en .

_:node1gm7uj6vjx2302 sh:path observable:validityNotAfter .

observable:registrarGUID rdfs:comment "Specifies the Registrar GUID field of a Whois entry."@en .

observable:X509CertificateFacet sh:property _:node1gm7uj6vjx2302 .

observable:registrarGUID rdfs:range xsd:string .

_:node1gm7uj6vjx2303 sh:datatype xsd:dateTime .

observable:registrarID a owl:DatatypeProperty .

_:node1gm7uj6vjx2303 sh:maxCount 1 .

observable:registrarID rdfs:label "registrarID"@en .

_:node1gm7uj6vjx2303 sh:nodeKind sh:Literal .

observable:registrarID rdfs:comment "Specifies the Registrar ID field of a Whois entry."@en .

_:node1gm7uj6vjx2303 sh:path observable:validityNotBefore .

observable:registrarID rdfs:range xsd:string .

observable:X509CertificateFacet sh:property _:node1gm7uj6vjx2303 .

observable:registrarInfo a owl:ObjectProperty .

_:node1gm7uj6vjx2304 sh:datatype xsd:integer .

observable:registrarInfo rdfs:label "registrarInfo"@en .

_:node1gm7uj6vjx2304 sh:maxCount 1 .

observable:registrarInfo rdfs:comment "Specifies registrar info that would be returned from a registrar lookup."@en .

_:node1gm7uj6vjx2304 sh:nodeKind sh:Literal .

observable:registrarInfo rdfs:range observable:WhoisRegistrarInfoType .

_:node1gm7uj6vjx2304 sh:path observable:subjectPublicKeyExponent .

observable:registrarName a owl:DatatypeProperty .

observable:X509CertificateFacet sh:property _:node1gm7uj6vjx2304 .

observable:registrarName rdfs:label "registrarName"@en .

_:node1gm7uj6vjx2305 sh:datatype xsd:string .

observable:registrarName rdfs:comment "The name of the registrar organization."@en .

_:node1gm7uj6vjx2305 sh:maxCount 1 .

observable:registrarName rdfs:range xsd:string .

_:node1gm7uj6vjx2305 sh:nodeKind sh:Literal .

observable:registryValues a owl:ObjectProperty .

_:node1gm7uj6vjx2305 sh:path observable:issuer .

observable:registryValues rdfs:label "registryValues"@en .

observable:X509CertificateFacet sh:property _:node1gm7uj6vjx2305 .

observable:registryValues rdfs:comment "The values that were enumerated as a result of the action on the object."@en .

_:node1gm7uj6vjx2306 sh:datatype xsd:string .

observable:registryValues rdfs:range observable:WindowsRegistryValue .

_:node1gm7uj6vjx2306 sh:maxCount 1 .

observable:remarks a owl:DatatypeProperty .

_:node1gm7uj6vjx2306 sh:nodeKind sh:Literal .

observable:remarks rdfs:label "remarks"@en .

_:node1gm7uj6vjx2306 sh:path observable:serialNumber .

observable:remarks rdfs:comment "Specifies any remarks associated with this Whois entry."@en .

observable:X509CertificateFacet sh:property _:node1gm7uj6vjx2306 .

observable:remarks rdfs:range xsd:string .

_:node1gm7uj6vjx2307 sh:datatype xsd:string .

observable:remindTime a owl:DatatypeProperty .

_:node1gm7uj6vjx2307 sh:maxCount 1 .

observable:remindTime rdfs:label "remindTime"@en .

_:node1gm7uj6vjx2307 sh:nodeKind sh:Literal .

observable:remindTime rdfs:range xsd:dateTime .

_:node1gm7uj6vjx2307 sh:path observable:signature .

observable:requestMethod a owl:DatatypeProperty .

observable:X509CertificateFacet sh:property _:node1gm7uj6vjx2307 .

observable:requestMethod rdfs:label "requestMethod"@en .

_:node1gm7uj6vjx2308 sh:datatype xsd:string .

observable:requestMethod rdfs:comment """Specifies the HTTP method portion of the HTTP request line, as a lowercase string.
          """@en .

_:node1gm7uj6vjx2308 sh:maxCount 1 .

observable:requestMethod rdfs:range xsd:string .

_:node1gm7uj6vjx2308 sh:nodeKind sh:Literal .

observable:requestValue a owl:DatatypeProperty .

_:node1gm7uj6vjx2308 sh:path observable:signatureAlgorithm .

observable:requestValue rdfs:label "requestValue"@en .

observable:X509CertificateFacet sh:property _:node1gm7uj6vjx2308 .

observable:requestValue rdfs:comment "Specifies the value (typically a resource path) portion of the HTTP request line."@en .

_:node1gm7uj6vjx2309 sh:datatype xsd:string .

observable:requestValue rdfs:range xsd:string .

_:node1gm7uj6vjx2309 sh:maxCount 1 .

observable:requestVersion a owl:DatatypeProperty .

_:node1gm7uj6vjx2309 sh:nodeKind sh:Literal .

observable:requestVersion rdfs:label "requestVersion"@en .

_:node1gm7uj6vjx2309 sh:path observable:subject .

observable:requestVersion rdfs:comment "Specifies the HTTP version portion of the HTTP request line, as a lowercase string."@en .

observable:X509CertificateFacet sh:property _:node1gm7uj6vjx2309 .

observable:requestVersion rdfs:range xsd:string .

_:node1gm7uj6vjx2310 sh:datatype xsd:string .

observable:rowCondition a owl:DatatypeProperty .

_:node1gm7uj6vjx2310 sh:maxCount 1 .

observable:rowCondition rdfs:label "rowCondition"@en .

_:node1gm7uj6vjx2310 sh:nodeKind sh:Literal .

observable:rowCondition rdfs:range xsd:string .

_:node1gm7uj6vjx2310 sh:path observable:subjectPublicKeyAlgorithm .

observable:rowIndex a owl:DatatypeProperty .

observable:X509CertificateFacet sh:property _:node1gm7uj6vjx2310 .

observable:rowIndex rdfs:label "rowIndex"@en .

_:node1gm7uj6vjx2311 sh:datatype xsd:string .

observable:rowIndex rdfs:range xsd:positiveInteger .

_:node1gm7uj6vjx2311 sh:maxCount 1 .

observable:ruid a owl:DatatypeProperty .

_:node1gm7uj6vjx2311 sh:nodeKind sh:Literal .

observable:ruid rdfs:label "ruid"@en .

_:node1gm7uj6vjx2311 sh:path observable:subjectPublicKeyModulus .

observable:ruid rdfs:comment "Specifies the real user ID, which represents the Unix user who created the process."@en .

observable:X509CertificateFacet sh:property _:node1gm7uj6vjx2311 .

observable:ruid rdfs:range xsd:nonNegativeInteger .

_:node1gm7uj6vjx2312 sh:datatype xsd:string .

observable:runningStatus a owl:DatatypeProperty .

_:node1gm7uj6vjx2312 sh:maxCount 1 .

observable:runningStatus rdfs:label "runningStatus"@en .

_:node1gm7uj6vjx2312 sh:nodeKind sh:Literal .

observable:runningStatus rdfs:range xsd:string .

_:node1gm7uj6vjx2312 sh:path observable:version .

observable:scheme a owl:DatatypeProperty .

observable:X509CertificateFacet sh:property _:node1gm7uj6vjx2312 .

observable:scheme rdfs:label "scheme"@en .

observable:X509CertificateFacet sh:targetClass observable:X509CertificateFacet .

observable:X509V3Certificate a owl:Class , sh:NodeShape ;
	rdfs:subClassOf observable:ObservableObject ;
	rdfs:label "X509V3Certificate"@en .

observable:scheme rdfs:comment "Identifies the type of URL."@en .

observable:X509V3Certificate rdfs:comment "An X.509 v3 certificate is a public key digital identity certificate conformant to the X.509 v3 PKI (Public Key Infrastructure) standard. "@en .

observable:scheme rdfs:range xsd:string .

observable:X509V3Certificate sh:targetClass observable:X509V3Certificate .

observable:sectionAlignment a owl:DatatypeProperty .

observable:X509V3ExtensionsFacet a owl:Class .

observable:sectionAlignment rdfs:label "sectionAlignment"@en .

observable:X509V3ExtensionsFacet a sh:NodeShape .

observable:sectionAlignment rdfs:comment "Specifies the alignment (in bytes) of PE sections when they are loaded into memory."@en .

observable:X509V3ExtensionsFacet rdfs:subClassOf core:Facet .

observable:sectionAlignment rdfs:range xsd:unsignedInt .

observable:X509V3ExtensionsFacet rdfs:label "X509V3ExtensionsFacet"@en .

observable:sections a owl:ObjectProperty .

observable:X509V3ExtensionsFacet rdfs:comment "An X.509 v3 certificate extensions facet is a grouping of characteristics unique to a public key digital identity certificate conformant to the X.509 v3 PKI (Public Key Infrastructure) standard."@en .

observable:sections rdfs:label "sections"@en .

_:node1gm7uj6vjx2313 sh:datatype xsd:dateTime .

observable:sections rdfs:comment "Specifies metadata about the sections in the PE file."@en .

_:node1gm7uj6vjx2313 sh:maxCount 1 .

observable:sections rdfs:range observable:WindowsPESection .

_:node1gm7uj6vjx2313 sh:nodeKind sh:Literal .

observable:sectorSize a owl:DatatypeProperty .

_:node1gm7uj6vjx2313 sh:path observable:privateKeyUsagePeriodNotAfter .

observable:sectorSize rdfs:label "sectorSize"@en .

observable:X509V3ExtensionsFacet sh:property _:node1gm7uj6vjx2313 .

observable:sectorSize rdfs:comment "The sector size of the volume in bytes."@en .

_:node1gm7uj6vjx2314 sh:datatype xsd:dateTime .

observable:sectorSize rdfs:range xsd:integer .

_:node1gm7uj6vjx2314 sh:maxCount 1 .

observable:securityAttributes a owl:DatatypeProperty .

_:node1gm7uj6vjx2314 sh:nodeKind sh:Literal .

observable:securityAttributes rdfs:label "securityAttributes"@en .

_:node1gm7uj6vjx2314 sh:path observable:privateKeyUsagePeriodNotBefore .

observable:securityAttributes rdfs:range xsd:string .

observable:X509V3ExtensionsFacet sh:property _:node1gm7uj6vjx2314 .

observable:sender a owl:ObjectProperty .

_:node1gm7uj6vjx2315 sh:datatype xsd:string .

observable:sender rdfs:label "sender"@en .

_:node1gm7uj6vjx2315 sh:maxCount 1 .

observable:sender rdfs:range observable:ObservableObject .

_:node1gm7uj6vjx2315 sh:nodeKind sh:Literal .

observable:sentTime a owl:DatatypeProperty .

_:node1gm7uj6vjx2315 sh:path observable:authorityKeyIdentifier .

observable:sentTime rdfs:label "sentTime"@en .

observable:X509V3ExtensionsFacet sh:property _:node1gm7uj6vjx2315 .

observable:sentTime rdfs:comment "The date and time at which the message sent."@en .

_:node1gm7uj6vjx2316 sh:datatype xsd:string .

observable:sentTime rdfs:range xsd:dateTime .

_:node1gm7uj6vjx2316 sh:maxCount 1 .

observable:serialNumber a owl:DatatypeProperty .

_:node1gm7uj6vjx2316 sh:nodeKind sh:Literal .

observable:serialNumber rdfs:label "serialNumber"@en .

_:node1gm7uj6vjx2316 sh:path observable:basicConstraints .

observable:serialNumber rdfs:range xsd:string .

observable:X509V3ExtensionsFacet sh:property _:node1gm7uj6vjx2316 .

observable:serverName a owl:ObjectProperty .

_:node1gm7uj6vjx2317 sh:datatype xsd:string .

observable:serverName rdfs:label "serverName"@en .

_:node1gm7uj6vjx2317 sh:maxCount 1 .

observable:serverName rdfs:comment "Specifies the corresponding server name for a whois entry. This usually corresponds to a name server lookup."@en .

_:node1gm7uj6vjx2317 sh:nodeKind sh:Literal .

observable:serverName rdfs:range observable:ObservableObject .

_:node1gm7uj6vjx2317 sh:path observable:certificatePolicies .

observable:serviceName a owl:DatatypeProperty .

observable:X509V3ExtensionsFacet sh:property _:node1gm7uj6vjx2317 .

observable:serviceName rdfs:label "serviceName"@en .

_:node1gm7uj6vjx2318 sh:datatype xsd:string .

observable:serviceName rdfs:range xsd:string .

_:node1gm7uj6vjx2318 sh:maxCount 1 .

observable:serviceStatus a owl:DatatypeProperty .

_:node1gm7uj6vjx2318 sh:nodeKind sh:Literal .

observable:serviceStatus rdfs:label "serviceStatus"@en .

_:node1gm7uj6vjx2318 sh:path observable:crlDistributionPoints .

observable:serviceStatus rdfs:range xsd:string .

observable:X509V3ExtensionsFacet sh:property _:node1gm7uj6vjx2318 .

observable:serviceType a owl:DatatypeProperty .

_:node1gm7uj6vjx2319 sh:datatype xsd:string .

observable:serviceType rdfs:label "serviceType"@en .

_:node1gm7uj6vjx2319 sh:maxCount 1 .

observable:serviceType rdfs:range xsd:string .

_:node1gm7uj6vjx2319 sh:nodeKind sh:Literal .

observable:sessionID a owl:DatatypeProperty .

_:node1gm7uj6vjx2319 sh:path observable:extendedKeyUsage .

observable:sessionID rdfs:label "sessionID"@en .

observable:X509V3ExtensionsFacet sh:property _:node1gm7uj6vjx2319 .

observable:sessionID rdfs:comment "An identifier for the session from which the message originates."@en .

_:node1gm7uj6vjx2320 sh:datatype xsd:string .

observable:sessionID rdfs:range xsd:string .

_:node1gm7uj6vjx2320 sh:maxCount 1 .

observable:shell a owl:DatatypeProperty .

_:node1gm7uj6vjx2320 sh:nodeKind sh:Literal .

observable:shell rdfs:label "shell"@en .

_:node1gm7uj6vjx2320 sh:path observable:inhibitAnyPolicy .

observable:shell rdfs:range xsd:string .

observable:X509V3ExtensionsFacet sh:property _:node1gm7uj6vjx2320 .

observable:showMessageBody a owl:DatatypeProperty .

_:node1gm7uj6vjx2321 sh:datatype xsd:string .

observable:showMessageBody rdfs:label "showMessageBody"@en .

_:node1gm7uj6vjx2321 sh:maxCount 1 .

observable:showMessageBody rdfs:comment "Specifies the message text that is displayed in the body of the message box by the action. See also: http://msdn.microsoft.com/en-us/library/windows/desktop/aa381302(v=vs.85).aspx."@en .

_:node1gm7uj6vjx2321 sh:nodeKind sh:Literal .

observable:showMessageBody rdfs:range xsd:string .

_:node1gm7uj6vjx2321 sh:path observable:issuerAlternativeName .

observable:showMessageTitle a owl:DatatypeProperty .

observable:X509V3ExtensionsFacet sh:property _:node1gm7uj6vjx2321 .

observable:showMessageTitle rdfs:label "showMessageTitle"@en .

_:node1gm7uj6vjx2322 sh:datatype xsd:string .

observable:showMessageTitle rdfs:comment "Specifies the title of the message box shown by the action. See also: http://msdn.microsoft.com/en-us/library/windows/desktop/aa381302(v=vs.85).aspx."@en .

_:node1gm7uj6vjx2322 sh:maxCount 1 .

observable:showMessageTitle rdfs:range xsd:string .

_:node1gm7uj6vjx2322 sh:nodeKind sh:Literal .

observable:sid a owl:DatatypeProperty .

_:node1gm7uj6vjx2322 sh:path observable:keyUsage .

observable:sid rdfs:label "sid"@en .

observable:X509V3ExtensionsFacet sh:property _:node1gm7uj6vjx2322 .

observable:sid rdfs:range xsd:string .

_:node1gm7uj6vjx2323 sh:datatype xsd:string .

observable:signalStrength a owl:DatatypeProperty .

_:node1gm7uj6vjx2323 sh:maxCount 1 .

observable:signalStrength rdfs:label "signalStrength"@en .

_:node1gm7uj6vjx2323 sh:nodeKind sh:Literal .

observable:signalStrength rdfs:comment "The strength of the antenna signal."@en .

_:node1gm7uj6vjx2323 sh:path observable:nameConstraints .

observable:signalStrength rdfs:range xsd:string .

observable:X509V3ExtensionsFacet sh:property _:node1gm7uj6vjx2323 .

observable:signature a owl:DatatypeProperty .

_:node1gm7uj6vjx2324 sh:datatype xsd:string .

observable:signature rdfs:label "signature"@en .

_:node1gm7uj6vjx2324 sh:maxCount 1 .

observable:signature rdfs:comment "A"@en .

_:node1gm7uj6vjx2324 sh:nodeKind sh:Literal .

observable:signature rdfs:range xsd:string .

_:node1gm7uj6vjx2324 sh:path observable:policyConstraints .

observable:signatureAlgorithm a owl:DatatypeProperty .

observable:X509V3ExtensionsFacet sh:property _:node1gm7uj6vjx2324 .

observable:signatureAlgorithm rdfs:label "signatureAlgorithm"@en .

_:node1gm7uj6vjx2325 sh:datatype xsd:string .

observable:signatureAlgorithm rdfs:range xsd:string .

_:node1gm7uj6vjx2325 sh:maxCount 1 .

observable:signatureDescription a owl:DatatypeProperty .

_:node1gm7uj6vjx2325 sh:nodeKind sh:Literal .

observable:signatureDescription rdfs:label "signatureDescription"@en .

_:node1gm7uj6vjx2325 sh:path observable:policyMappings .

observable:signatureDescription rdfs:range xsd:string .

observable:X509V3ExtensionsFacet sh:property _:node1gm7uj6vjx2325 .

observable:signatureExists a owl:DatatypeProperty .

_:node1gm7uj6vjx2326 sh:datatype xsd:string .

observable:signatureExists rdfs:label "signatureExists"@en .

_:node1gm7uj6vjx2326 sh:maxCount 1 .

observable:signatureExists rdfs:range xsd:boolean .

_:node1gm7uj6vjx2326 sh:nodeKind sh:Literal .

observable:signatureVerified a owl:DatatypeProperty .

_:node1gm7uj6vjx2326 sh:path observable:subjectAlternativeName .

observable:signatureVerified rdfs:label "signatureVerified"@en .

observable:X509V3ExtensionsFacet sh:property _:node1gm7uj6vjx2326 .

observable:signatureVerified rdfs:range xsd:boolean .

_:node1gm7uj6vjx2327 sh:datatype xsd:string .

observable:sipAddress a owl:ObjectProperty .

_:node1gm7uj6vjx2327 sh:maxCount 1 .

observable:sipAddress rdfs:label "sipAddress"@en .

_:node1gm7uj6vjx2327 sh:nodeKind sh:Literal .

observable:sipAddress rdfs:comment "A SIP address specifies Session Initiation Protocol (SIP) identifier."@en .

_:node1gm7uj6vjx2327 sh:path observable:subjectDirectoryAttributes .

observable:sipAddress rdfs:range observable:ObservableObject .

observable:X509V3ExtensionsFacet sh:property _:node1gm7uj6vjx2327 .

observable:size a owl:DatatypeProperty .

_:node1gm7uj6vjx2328 sh:datatype xsd:string .

observable:size rdfs:label "size"@en .

_:node1gm7uj6vjx2328 sh:maxCount 1 .

observable:size rdfs:comment "Specifies the size of the section, in bytes."@en .

_:node1gm7uj6vjx2328 sh:nodeKind sh:Literal .

observable:size rdfs:range xsd:integer .

_:node1gm7uj6vjx2328 sh:path observable:subjectKeyIdentifier .

observable:sizeInBytes a owl:DatatypeProperty .

observable:X509V3ExtensionsFacet sh:property _:node1gm7uj6vjx2328 .

observable:sizeInBytes rdfs:label "sizeInBytes"@en .

observable:X509V3ExtensionsFacet sh:targetClass observable:X509V3ExtensionsFacet .

observable:sizeInBytes rdfs:comment "The size of the data in bytes."@en .

observable:abbreviation a owl:DatatypeProperty .

observable:sizeInBytes rdfs:range xsd:integer .

observable:abbreviation rdfs:label "abbreviation"@en .

observable:sizeOfCode a owl:DatatypeProperty .

observable:abbreviation rdfs:comment "The abbreviation of a global flag. See also: http://msdn.microsoft.com/en-us/library/windows/hardware/ff549646(v=vs.85).aspx."@en .

observable:sizeOfCode rdfs:label "sizeOfCode"@en .

observable:abbreviation rdfs:range xsd:string .

observable:sizeOfCode rdfs:comment "Specifies the size of the code (text) section. If there are multiple such sections, this refers to the sum of the sizes of each section."@en .

observable:accessedDirectory a owl:ObjectProperty .

observable:sizeOfCode rdfs:range xsd:unsignedInt .

observable:accessedDirectory rdfs:label "accessedDirectory"@en .

observable:sizeOfHeaders a owl:DatatypeProperty .

observable:accessedDirectory rdfs:comment "Directories accessed by the prefetch application during startup."@en .

observable:sizeOfHeaders rdfs:label "sizeOfHeaders"@en .

observable:accessedDirectory rdfs:range observable:ObservableObject .

observable:sizeOfHeaders rdfs:comment "Specifies the combined size of the MS-DOS, PE header, and section headers, rounded up a multiple of the value specified in the file_alignment header."@en .

observable:accessedFile a owl:ObjectProperty .

observable:sizeOfHeaders rdfs:range xsd:unsignedInt .

observable:accessedFile rdfs:label "accessedFile"@en .

observable:sizeOfHeapCommit a owl:DatatypeProperty .

observable:accessedFile rdfs:comment "Files (e.g., DLLs and other support files) used by the application during startup."@en .

observable:sizeOfHeapCommit rdfs:label "sizeOfHeapCommit"@en .

observable:accessedFile rdfs:range observable:ObservableObject .

observable:sizeOfHeapCommit rdfs:comment "Specifies the size of the local heap space to commit."@en .

observable:accessedTime a owl:DatatypeProperty .

observable:sizeOfHeapCommit rdfs:range xsd:unsignedInt .

observable:accessedTime rdfs:label "accessedTime"@en .

observable:sizeOfHeapReserve a owl:DatatypeProperty .

observable:accessedTime rdfs:comment "The date and time at which the Object was accessed."@en .

observable:sizeOfHeapReserve rdfs:label "sizeOfHeapReserve"@en .

observable:accessedTime rdfs:range xsd:dateTime .

observable:account a owl:ObjectProperty .

observable:sizeOfHeapReserve rdfs:comment "Specifies the size of the local heap space to reserve."@en .

observable:account rdfs:label "account"@en .

observable:sizeOfHeapReserve rdfs:range xsd:unsignedInt .

observable:account rdfs:comment "Specifies the account referenced in an event log entry or used to run the scheduled task. See also: http://msdn.microsoft.com/en-us/library/windows/desktop/aa381228(v=vs.85).aspx."@en .

observable:sizeOfImage a owl:DatatypeProperty .

observable:account rdfs:range observable:ObservableObject .

observable:sizeOfImage rdfs:label "sizeOfImage"@en .

observable:accountIdentifier a owl:DatatypeProperty .

observable:sizeOfImage rdfs:comment "Specifies the size, in bytes, of the image, including all headers, as the image is loaded in memory."@en .

observable:accountIdentifier rdfs:label "accountIdentifier"@en .

observable:sizeOfImage rdfs:range xsd:unsignedInt .

observable:accountIdentifier rdfs:comment "The unique identifier for the account."@en .

observable:sizeOfInitializedData a owl:DatatypeProperty .

observable:accountIdentifier rdfs:range xsd:string .

observable:sizeOfInitializedData rdfs:label "sizeOfInitializedData"@en .

observable:accountIssuer a owl:ObjectProperty .

observable:sizeOfInitializedData rdfs:comment "Specifies the size of the initialized data section. If there are multiple such sections, this refers to the sum of the sizes of each section."@en .

observable:accountIssuer rdfs:label "accountIssuer"@en .

observable:sizeOfInitializedData rdfs:range xsd:unsignedInt .

observable:accountIssuer rdfs:comment "The issuer of this account."@en .

observable:sizeOfOptionalHeader a owl:DatatypeProperty .

observable:accountIssuer rdfs:range core:UcoObject .

observable:sizeOfOptionalHeader rdfs:label "sizeOfOptionalHeader"@en .

observable:accountLogin a owl:DatatypeProperty .

observable:sizeOfOptionalHeader rdfs:comment "Specifies the size of the optional header of the PE binary. "@en .

observable:accountLogin rdfs:label "accountLogin"@en .

observable:sizeOfOptionalHeader rdfs:range xsd:integer .

observable:accountLogin rdfs:comment "The login identifier for the digital account."@en .

observable:sizeOfStackCommit a owl:DatatypeProperty .

observable:accountLogin rdfs:range xsd:string .

observable:sizeOfStackCommit rdfs:label "sizeOfStackCommit"@en .

observable:accountLogonType a owl:DatatypeProperty .

observable:sizeOfStackCommit rdfs:comment "Specifies the size of the stack to commit."@en .

observable:accountLogonType rdfs:label "accountLogonType"@en .

observable:sizeOfStackCommit rdfs:range xsd:unsignedInt .

observable:accountLogonType rdfs:comment "Specifies the security logon method required to run the tasks associated with the account. See also: http://msdn.microsoft.com/en-us/library/windows/desktop/aa383013(v=vs.85).aspx."@en .

observable:sizeOfStackReserve a owl:DatatypeProperty .

observable:accountLogonType rdfs:range xsd:string .

observable:sizeOfStackReserve rdfs:label "sizeOfStackReserve"@en .

observable:accountRunLevel a owl:DatatypeProperty .

observable:sizeOfStackReserve rdfs:comment "Specifies the size of the stack to reserve."@en .

observable:accountRunLevel rdfs:label "accountRunLevel"@en .

observable:sizeOfStackReserve rdfs:range xsd:unsignedInt .

observable:accountRunLevel rdfs:comment "Specifies the permission level of the account that the task will be run at."@en .

observable:sizeOfUninitializedData a owl:DatatypeProperty .

observable:accountRunLevel rdfs:range xsd:string .

observable:sizeOfUninitializedData rdfs:label "sizeOfUninitializedData"@en .

observable:accountType a owl:DatatypeProperty .

observable:sizeOfUninitializedData rdfs:comment "Specifies the size of the uninitialized data section. If there are multiple such sections, this refers to the sum of the sizes of each section."@en .

observable:accountType rdfs:label "accountType"@en .

observable:sizeOfUninitializedData rdfs:range xsd:unsignedInt .

observable:accountType rdfs:comment "The type of account, for instance bank, phone, application, service, etc."@en .

observable:skew a owl:DatatypeProperty .

_:node1gm7uj6vjx2329 a rdfs:Datatype .

observable:skew rdfs:label "skew"@en .

_:node1gm7uj6vjx2330 rdf:first vocabulary:AccountTypeVocab .

observable:skew rdfs:comment "The angle in degrees of the radial rotation around its main beam direction."@en .

_:node1gm7uj6vjx2330 rdf:rest _:node1gm7uj6vjx2331 .

observable:skew rdfs:range xsd:decimal .

_:node1gm7uj6vjx2331 rdf:first xsd:string .

observable:sourceApplication a owl:ObjectProperty .

_:node1gm7uj6vjx2331 rdf:rest rdf:nil .

observable:sourceApplication rdfs:label "sourceApplication"@en .

_:node1gm7uj6vjx2329 owl:unionOf _:node1gm7uj6vjx2330 .

observable:sourceApplication rdfs:comment "Source application specifies the software application that a particular contact or contact list is associated with."@en .

observable:accountType rdfs:range _:node1gm7uj6vjx2329 .

observable:sourceApplication rdfs:range observable:ObservableObject .

observable:actionID a owl:DatatypeProperty .

observable:sourceFlags a owl:DatatypeProperty .

observable:actionID rdfs:label "actionID"@en .

observable:sourceFlags rdfs:label "sourceFlags"@en .

observable:actionID rdfs:comment "Specifies the user-defined identifier for the action. This identifier is used by the Task Scheduler for logging purposes. See also: http://msdn.microsoft.com/en-us/library/windows/desktop/aa380590(v=vs.85).aspx."@en .

observable:sourceFlags rdfs:comment "Specifies the source TCP flags."@en .

observable:actionID rdfs:range xsd:string .

observable:sourceFlags rdfs:range xsd:hexBinary .

observable:actionList a owl:ObjectProperty .

observable:sourcePort a owl:DatatypeProperty .

observable:actionList rdfs:label "actionList"@en .

observable:sourcePort rdfs:label "sourcePort"@en .

observable:actionList rdfs:comment "Specifies a list of actions to be performed by the scheduled task."@en .

observable:sourcePort rdfs:comment """Specifies the source port used in the connection, as an integer in the range of 0 - 65535.
          """@en .

observable:actionList rdfs:range observable:TaskActionType .

observable:sourcePort rdfs:range xsd:integer .

observable:actionType a owl:DatatypeProperty .

observable:spaceLeft a owl:DatatypeProperty .

observable:actionType rdfs:label "actionType"@en .

observable:spaceLeft rdfs:label "spaceLeft"@en .

observable:actionType rdfs:comment "Specifies the type of the action. See also: http://msdn.microsoft.com/en-us/library/windows/desktop/aa380596(v=vs.85).aspx."@en .

observable:spaceLeft rdfs:comment "Specifies the amount of space left on the partition, in bytes."@en .

_:node1gm7uj6vjx2332 a rdfs:Datatype .

observable:spaceLeft rdfs:range xsd:integer .

_:node1gm7uj6vjx2333 rdf:first vocabulary:TaskActionTypeVocab .

observable:spaceUsed a owl:DatatypeProperty .

_:node1gm7uj6vjx2333 rdf:rest _:node1gm7uj6vjx2334 .

observable:spaceUsed rdfs:label "spaceUsed"@en .

_:node1gm7uj6vjx2334 rdf:first xsd:string .

observable:spaceUsed rdfs:comment "Specifies the amount of space used on the partition, in bytes."@en .

_:node1gm7uj6vjx2334 rdf:rest rdf:nil .

observable:spaceUsed rdfs:range xsd:integer .

_:node1gm7uj6vjx2332 owl:unionOf _:node1gm7uj6vjx2333 .

observable:sponsoringRegistrar a owl:DatatypeProperty .

observable:actionType rdfs:range _:node1gm7uj6vjx2332 .

observable:sponsoringRegistrar rdfs:label "sponsoringRegistrar"@en .

observable:activeDirectoryGroups a owl:DatatypeProperty .

observable:sponsoringRegistrar rdfs:comment "Specifies the name of the sponsoring registrar for a domain."@en .

observable:activeDirectoryGroups rdfs:label "activeDirectoryGroups"@en .

observable:sponsoringRegistrar rdfs:range xsd:string .

observable:activeDirectoryGroups rdfs:range xsd:string .

observable:src a owl:ObjectProperty .

observable:adapterName a owl:DatatypeProperty .

observable:src rdfs:label "src"@en .

observable:adapterName rdfs:label "adapterName"@en .

observable:src rdfs:comment "Specifies the source(s) of the network connection."@en .

observable:adapterName rdfs:comment "Specifies the name of the network adapter used by the network interface."@en .

observable:src rdfs:range core:UcoObject .

observable:adapterName rdfs:range xsd:string .

observable:srcBytes a owl:DatatypeProperty .

observable:addressOfEntryPoint a owl:DatatypeProperty .

observable:srcBytes rdfs:label "srcBytes"@en .

observable:addressOfEntryPoint rdfs:label "addressOfEntryPoint"@en .

observable:srcBytes rdfs:range xsd:integer .

observable:addressOfEntryPoint rdfs:comment "Specifies the address of the entry point relative to the image base when the executable is loaded into memory."@en .

observable:srcPackets a owl:DatatypeProperty .

observable:addressOfEntryPoint rdfs:range xsd:unsignedInt .

observable:srcPackets rdfs:label "srcPackets"@en .

observable:addressValue a owl:DatatypeProperty .

observable:srcPackets rdfs:range xsd:integer .

observable:addressValue rdfs:label "addressValue"@en .

observable:srcPayload a owl:ObjectProperty .

observable:addressValue rdfs:comment "The value of an address."@en .

observable:srcPayload rdfs:label "srcPayload"@en .

observable:addressValue rdfs:range xsd:string .

observable:srcPayload rdfs:range observable:ObservableObject .

observable:advertisingID a owl:DatatypeProperty .

observable:ssid a owl:DatatypeProperty .

observable:advertisingID rdfs:label "advertisingID"@en .

observable:ssid rdfs:label "ssid"@en .

observable:advertisingID rdfs:comment "Advertising ID as a UUID. [based on https://developer.android.com/reference/androidx/ads/identifier/AdvertisingIdInfo]"@en .

observable:ssid rdfs:comment "Network identifier."@en .

observable:advertisingID rdfs:range xsd:string .

observable:ssid rdfs:range xsd:string .

observable:allocationStatus a owl:DatatypeProperty .

observable:stackSize a owl:DatatypeProperty .

observable:allocationStatus rdfs:label "allocationStatus"@en .

observable:stackSize rdfs:label "stackSize"@en .

observable:allocationStatus rdfs:comment "The allocation status of a file."@en .

observable:stackSize rdfs:range xsd:nonNegativeInteger .

observable:allocationStatus rdfs:range xsd:string .

observable:startAddress a owl:DatatypeProperty .

observable:alternateDataStreams a owl:ObjectProperty .

observable:startAddress rdfs:label "startAddress"@en .

observable:alternateDataStreams rdfs:label "alternateDataStreams"@en .

observable:startAddress rdfs:range xsd:hexBinary .

observable:alternateDataStreams rdfs:range observable:AlternateDataStream .

observable:startCommandLine a owl:DatatypeProperty .

observable:androidFingerprint a owl:DatatypeProperty .

observable:startCommandLine rdfs:label "startCommandLine"@en .

observable:androidFingerprint rdfs:label "androidFingerprint"@en .

observable:startCommandLine rdfs:range xsd:string .

observable:androidFingerprint rdfs:comment "A string that uniquely identifies a build of the Android operating system. [based on https://developer.android.com/reference/android/os/Build#FINGERPRINT]"@en .

observable:startTime a owl:DatatypeProperty .

observable:androidFingerprint rdfs:range xsd:string .

observable:startTime rdfs:label "startTime"@en .

observable:androidID a owl:DatatypeProperty .

observable:startTime rdfs:range xsd:dateTime .

observable:androidID rdfs:label "androidID"@en .

observable:startType a owl:DatatypeProperty .

observable:androidID rdfs:comment "A 64-bit number (expressed as a hexadecimal string), unique to each combination of app-signing key, user, and device. [based on https://developer.android.com/reference/android/provider/Settings.Secure#ANDROID_ID]"@en .

observable:startType rdfs:label "startType"@en .

observable:androidID rdfs:range xsd:hexBinary .

observable:startType rdfs:range xsd:string .

observable:androidVersion a owl:DatatypeProperty .

observable:startupInfo a owl:ObjectProperty .

observable:androidVersion rdfs:label "androidVersion"@en .

observable:startupInfo rdfs:label "startupInfo"@en .

observable:androidVersion rdfs:comment "The user-visible version string. E.g., '1.0' or '3.4b5' or 'bananas'. This field is an opaque string. Do not assume that its value has any particular structure or that values of RELEASE from different releases can be somehow ordered. [based on https://developer.android.com/reference/android/os/Build.VERSION#RELEASE]"@en .

observable:startupInfo rdfs:range types:Dictionary .

observable:androidVersion rdfs:range xsd:string .

observable:state a owl:DatatypeProperty .

observable:antennaHeight a owl:DatatypeProperty .

observable:state rdfs:label "State"@en .

observable:antennaHeight rdfs:label "antennaHeight"@en .

observable:state rdfs:range xsd:string .

observable:antennaHeight rdfs:comment "The height (in meters) of the antenna from the ground."@en .

observable:status a owl:DatatypeProperty .

observable:antennaHeight rdfs:range xsd:decimal .

observable:status rdfs:label "status"@en .

observable:application a owl:ObjectProperty .

observable:status rdfs:comment "Specifies a list of statuses for a given Whois entry."@en .

observable:application rdfs:label "application"@en .

_:node1gm7uj6vjx2395 a rdfs:Datatype .

observable:application rdfs:comment "The application associated with this object."@en .

_:node1gm7uj6vjx2396 rdf:first xsd:string .

observable:application rdfs:range observable:ObservableObject .

_:node1gm7uj6vjx2396 rdf:rest _:node1gm7uj6vjx2397 .

observable:applicationFileName a owl:DatatypeProperty .

_:node1gm7uj6vjx2397 rdf:first vocabulary:TaskStatusVocab .

observable:applicationFileName rdfs:label "applicationFileName"@en .

_:node1gm7uj6vjx2397 rdf:rest _:node1gm7uj6vjx2398 .

observable:applicationFileName rdfs:comment "Name of the executable of the prefetch file."@en .

_:node1gm7uj6vjx2398 rdf:first vocabulary:WhoisStatusTypeVocab .

observable:applicationFileName rdfs:range xsd:string .

_:node1gm7uj6vjx2398 rdf:rest rdf:nil .

observable:applicationIdentifier a owl:DatatypeProperty .

_:node1gm7uj6vjx2395 owl:unionOf _:node1gm7uj6vjx2396 .

observable:applicationIdentifier rdfs:label "applicationIdentifier"@en .

observable:status rdfs:range _:node1gm7uj6vjx2395 .

observable:applicationIdentifier rdfs:range xsd:string .

observable:statusesCount a owl:DatatypeProperty .

observable:archiveType a owl:DatatypeProperty .

observable:statusesCount rdfs:label "Statuses Count"@en-us .

observable:archiveType rdfs:label "archiveType"@en .

observable:statusesCount rdfs:comment "Specifies the number of tweets that this profile has issued."@en-us .

observable:archiveType rdfs:comment "The type of a file archive, e.g. ZIP, GZIP or RAR."@en .

observable:statusesCount rdfs:range xsd:nonNegativeInteger .

observable:archiveType rdfs:range xsd:string .

observable:storageCapacityInBytes a owl:DatatypeProperty .

observable:arguments a owl:DatatypeProperty .

observable:storageCapacityInBytes rdfs:label "storageCapacityInBytes"@en .

observable:arguments rdfs:label "arguments"@en .

observable:storageCapacityInBytes rdfs:comment "The number of bytes that can be stored on a SIM card."@en .

observable:arguments rdfs:comment "A list of arguments utilized in initiating the process."@en .

observable:storageCapacityInBytes rdfs:range xsd:integer .

observable:arguments rdfs:range xsd:string .

observable:stringValue a owl:DatatypeProperty .

observable:asHandle a owl:DatatypeProperty .

observable:stringValue rdfs:label "stringValue"@en .

observable:asHandle rdfs:label "asHandle"@en .

observable:stringValue rdfs:comment "Specifies the actual value of the extracted string."@en .

observable:asHandle rdfs:range xsd:string .

observable:stringValue rdfs:range xsd:string .

observable:aslrEnabled a owl:DatatypeProperty .

observable:strings a owl:ObjectProperty .

observable:aslrEnabled rdfs:label "aslrEnabled"@en .

observable:strings rdfs:label "strings"@en .

observable:aslrEnabled rdfs:range xsd:boolean .

observable:strings rdfs:range observable:ExtractedString .

observable:attendant a owl:ObjectProperty .

observable:subject a owl:DatatypeProperty .

observable:attendant rdfs:label "attendant"@en .

observable:subject rdfs:label "subject"@en .

observable:attendant rdfs:comment "The attendants of the event."@en .

observable:subject rdfs:comment "The subject of the email."@en .

observable:attendant rdfs:range identity:Identity .

observable:subject rdfs:range xsd:string .

observable:audioType a owl:DatatypeProperty .

observable:subjectAlternativeName a owl:DatatypeProperty .

observable:audioType rdfs:label "audioType"@en .

observable:subjectAlternativeName rdfs:label "subjectAlternativeName"@en .

observable:audioType rdfs:comment "The type of a audio. For example: music or speech."@en .

observable:subjectAlternativeName rdfs:range xsd:string .

observable:audioType rdfs:range xsd:string .

observable:subjectDirectoryAttributes a owl:DatatypeProperty .

observable:authorityKeyIdentifier a owl:DatatypeProperty .

observable:subjectDirectoryAttributes rdfs:label "subjectDirectoryAttributes"@en .

observable:authorityKeyIdentifier rdfs:label "authorityKeyIdentifier"@en .

observable:subjectDirectoryAttributes rdfs:range xsd:string .

observable:authorityKeyIdentifier rdfs:range xsd:string .

observable:subjectHash a owl:ObjectProperty .

observable:availableRam a owl:DatatypeProperty .

observable:subjectHash rdfs:label "subjectHash"@en .

observable:availableRam rdfs:label "availableRam"@en .

observable:subjectHash rdfs:comment "A hash calculated on the certificate subject name."@en .

observable:availableRam rdfs:comment "Specifies the amount of physical memory available on the system, in bytes."@en .

observable:subjectHash rdfs:range types:Hash .

observable:availableRam rdfs:range xsd:integer .

observable:subjectKeyIdentifier a owl:DatatypeProperty .

observable:azimuth a owl:DatatypeProperty .

observable:subjectKeyIdentifier rdfs:label "subjectKeyIdentifier"@en .

observable:azimuth rdfs:label "azimuth"@en .

observable:subjectKeyIdentifier rdfs:range xsd:string .

observable:azimuth rdfs:comment "The median rotation in degrees around a vertical axis of the cell antenna sector accessed."@en .

observable:subjectPublicKeyAlgorithm a owl:DatatypeProperty .

observable:azimuth rdfs:range xsd:decimal .

observable:subjectPublicKeyAlgorithm rdfs:label "subjectPublicKeyAlgorithm"@en .

observable:baseOfCode a owl:DatatypeProperty .

observable:subjectPublicKeyAlgorithm rdfs:range xsd:string .

observable:baseOfCode rdfs:label "baseOfCode"@en .

observable:subjectPublicKeyExponent a owl:DatatypeProperty .

observable:baseOfCode rdfs:comment "Specifies the address that is relative to the image base of the beginning-of-code section when it is loaded into memory."@en .

observable:subjectPublicKeyExponent rdfs:label "subjectPublicKeyExponent"@en .

observable:baseOfCode rdfs:range xsd:unsignedInt .

observable:subjectPublicKeyExponent rdfs:range xsd:integer .

observable:baseStation a owl:DatatypeProperty .

observable:subjectPublicKeyModulus a owl:DatatypeProperty .

observable:baseStation rdfs:label "baseStation"@en .

observable:subjectPublicKeyModulus rdfs:label "subjectPublicKeyModulus"@en .

observable:baseStation rdfs:comment "The base station."@en .

observable:subjectPublicKeyModulus rdfs:range xsd:string .

observable:baseStation rdfs:range xsd:string .

observable:subsystem a owl:DatatypeProperty .

observable:basicConstraints a owl:DatatypeProperty .

observable:subsystem rdfs:label "subsystem"@en .

observable:basicConstraints rdfs:label "basicConstraints"@en .

observable:subsystem rdfs:comment "Specifies the subsystem (e.g., GUI, device driver, etc.) that is required to run this image."@en .

observable:basicConstraints rdfs:range xsd:string .

observable:subsystem rdfs:range xsd:unsignedShort .

observable:bcc a owl:ObjectProperty .

observable:swid a owl:DatatypeProperty .

observable:bcc rdfs:label "bcc"@en .

observable:swid rdfs:label "swid"@en .

observable:bcc rdfs:range observable:ObservableObject .

observable:swid rdfs:comment "Specifies the SWID tag for the software."@en .

observable:binary a owl:ObjectProperty .

observable:swid rdfs:range xsd:string .

observable:binary rdfs:label "binary"@en .

observable:symbolicName a owl:DatatypeProperty .

observable:binary rdfs:range observable:ObservableObject .

observable:symbolicName rdfs:label "symbolicName"@en .

observable:biosDate a owl:DatatypeProperty .

observable:symbolicName rdfs:comment "The symbolic name of a global flag. See also: http://msdn.microsoft.com/en-us/library/windows/hardware/ff549646(v=vs.85).aspx."@en .

observable:biosDate rdfs:label "biosDate"@en .

observable:symbolicName rdfs:range xsd:string .

observable:biosDate rdfs:comment "Specifies the date of the BIOS (e.g. the datestamp of the BIOS revision)."@en .

observable:systemTime a owl:DatatypeProperty .

observable:biosDate rdfs:range xsd:dateTime .

observable:systemTime rdfs:label "systemTime"@en .

observable:biosManufacturer a owl:DatatypeProperty .

observable:systemTime rdfs:range xsd:dateTime .

observable:biosManufacturer rdfs:label "biosManufacturer"@en .

observable:tableName a owl:DatatypeProperty .

observable:biosManufacturer rdfs:comment "Specifies the manufacturer of the BIOS."@en .

observable:tableName rdfs:label "tableName"@en .

observable:biosManufacturer rdfs:range xsd:string .

observable:tableName rdfs:comment "The table containing a specified database record."@en .

observable:biosReleaseDate a owl:DatatypeProperty .

observable:tableName rdfs:range xsd:string .

observable:biosReleaseDate rdfs:label "biosReleaseDate"@en .

observable:tableSchema a owl:DatatypeProperty .

observable:biosReleaseDate rdfs:comment "Specifies the date the BIOS was released."@en .

observable:tableSchema rdfs:label "tableSchema"@en .

observable:biosReleaseDate rdfs:range xsd:dateTime .

observable:tableSchema rdfs:comment "The schema that contains the identified database record."@en .

observable:biosSerialNumber a owl:DatatypeProperty .

observable:tableSchema rdfs:range xsd:string .

observable:biosSerialNumber rdfs:label "biosSerialNumber"@en .

observable:targetFile a owl:ObjectProperty .

observable:biosSerialNumber rdfs:comment "Specifies the serial number of the BIOS."@en .

observable:targetFile rdfs:label "targetFile"@en .

observable:biosSerialNumber rdfs:range xsd:string .

observable:targetFile rdfs:comment "Specifies the file targeted by a symbolic link."@en .

observable:biosVersion a owl:DatatypeProperty .

observable:targetFile rdfs:range observable:ObservableObject .

observable:biosVersion rdfs:label "biosVersion"@en .

observable:taskComment a owl:DatatypeProperty .

observable:biosVersion rdfs:comment "Specifies the version of the BIOS."@en .

observable:taskComment rdfs:label "taskComment"@en .

observable:biosVersion rdfs:range xsd:string .

observable:taskComment rdfs:comment "Specifies a comment for the scheduled task. See also: http://msdn.microsoft.com/en-us/library/windows/desktop/aa381232(v=vs.85).aspx."@en .

observable:bitRate a owl:DatatypeProperty .

observable:taskComment rdfs:range xsd:string .

observable:bitRate rdfs:label "bitRate"@en .

observable:taskCreator a owl:DatatypeProperty .

observable:bitRate rdfs:comment "The bitrate of the audio in bits per second."@en .

observable:taskCreator rdfs:label "taskCreator"@en .

observable:bitRate rdfs:range xsd:integer .

observable:taskCreator rdfs:comment "Specifies the name of the creator of the scheduled task. See also: http://msdn.microsoft.com/en-us/library/windows/desktop/aa381235(v=vs.85).aspx."@en .

observable:bitness a owl:DatatypeProperty .

observable:taskCreator rdfs:range xsd:string .

observable:bitness rdfs:label "bitness"@en .

observable:text a owl:DatatypeProperty .

observable:bitness rdfs:comment "Specifies the bitness of the operating system (i.e. 32 or 64). Note that this is potentially different from the word size of the underlying hardware or CPU. A 32-bit operating system can be installed on a machine running a 64-bit processor."@en .

observable:text rdfs:label "text"@en .

observable:bitness rdfs:range xsd:string .

observable:text rdfs:range xsd:string .

observable:bitsPerPixel a owl:DatatypeProperty .

observable:threadID a owl:DatatypeProperty .

observable:bitsPerPixel rdfs:label "bitsPerPixel"@en .

observable:threadID rdfs:label "threadID"@en .

observable:bitsPerPixel rdfs:range xsd:integer .

observable:threadID rdfs:range xsd:nonNegativeInteger .

observable:blockType a owl:DatatypeProperty .

observable:thumbprintHash a owl:ObjectProperty .

observable:blockType rdfs:label "blockType"@en .

observable:thumbprintHash rdfs:label "thumbprintHash"@en .

observable:blockType rdfs:comment "The blockType property specifies the block type of a particular memory object."@en .

observable:thumbprintHash rdfs:comment "A hash calculated on the entire certificate including signature."@en .

_:node1gm7uj6vjx2335 a rdfs:Datatype .

observable:thumbprintHash rdfs:range types:Hash .

_:node1gm7uj6vjx2336 rdf:first vocabulary:MemoryBlockTypeVocab .

observable:timeDateStamp a owl:DatatypeProperty .

_:node1gm7uj6vjx2336 rdf:rest _:node1gm7uj6vjx2337 .

observable:timeDateStamp rdfs:label "timeDateStamp"@en .

_:node1gm7uj6vjx2337 rdf:first xsd:string .

observable:timeDateStamp rdfs:comment "Specifies the time when the PE binary was created."@en .

_:node1gm7uj6vjx2337 rdf:rest rdf:nil .

observable:timeDateStamp rdfs:range xsd:dateTime .

_:node1gm7uj6vjx2335 owl:unionOf _:node1gm7uj6vjx2336 .

observable:timesExecuted a owl:DatatypeProperty .

observable:blockType rdfs:range _:node1gm7uj6vjx2335 .

observable:timesExecuted rdfs:label "timesExecuted"@en .

observable:bluetoothDeviceName a owl:DatatypeProperty .

observable:timesExecuted rdfs:comment "The number of times the prefetch application has executed."@en .

observable:bluetoothDeviceName rdfs:label "bluetoothDeviceName"@en .

observable:timesExecuted rdfs:range xsd:integer .

observable:bluetoothDeviceName rdfs:comment "Name configured withing Bluetooth settings on a device."@en .

observable:timezoneDST a owl:DatatypeProperty .

observable:bluetoothDeviceName rdfs:range xsd:string .

observable:timezoneDST rdfs:label "timezoneDST"@en .

observable:body a owl:DatatypeProperty .

observable:timezoneDST rdfs:comment "Specifies the time zone used by the system, taking daylight savings time (DST) into account."@en .

observable:body rdfs:label "body"@en .

observable:timezoneDST rdfs:range xsd:string .

observable:body rdfs:range xsd:string .

observable:timezoneStandard a owl:DatatypeProperty .

observable:bodyMultipart a owl:ObjectProperty .

observable:timezoneStandard rdfs:label "timezoneStandard"@en .

observable:bodyMultipart rdfs:label "bodyMultipart"@en .

observable:timezoneStandard rdfs:comment "Specifies the time zone used by the system, without taking daylight savings time (DST) into account."@en .

observable:bodyMultipart rdfs:comment "A list of the MIME parts that make up the email body. This field MAY only be used if isMultipart is true."@en .

observable:timezoneStandard rdfs:range xsd:string .

observable:bodyMultipart rdfs:range observable:MimePartType .

observable:to a owl:ObjectProperty .

observable:bodyRaw a owl:ObjectProperty .

observable:to rdfs:label "to"@en .

observable:bodyRaw rdfs:label "bodyRaw"@en .

observable:to rdfs:comment "The receiver's phone number."@en .

observable:bodyRaw rdfs:range observable:ObservableObject .

observable:to rdfs:range observable:ObservableObject .

observable:bookmarkPath a owl:DatatypeProperty .

observable:totalFragments a owl:DatatypeProperty .

observable:bookmarkPath rdfs:label "bookmarkPath"@en .

observable:totalFragments rdfs:label "totalFragments"@en .

observable:bookmarkPath rdfs:comment "The folder containing the bookmark."@en .

observable:totalFragments rdfs:range xsd:integer .

observable:bookmarkPath rdfs:range xsd:string .

observable:totalRam a owl:DatatypeProperty .

observable:browserInformation a owl:ObjectProperty .

observable:totalRam rdfs:label "totalRam"@en .

observable:browserInformation rdfs:label "Browser Information"@en .

observable:totalRam rdfs:comment "Specifies the total amount of physical memory present on the system, in bytes."@en .

observable:browserInformation rdfs:comment "Specifies information about the particular Web Browser."@en .

observable:totalRam rdfs:range xsd:integer .

observable:browserInformation rdfs:range observable:ObservableObject .

observable:totalSpace a owl:DatatypeProperty .

observable:browserUserProfile a owl:DatatypeProperty .

observable:totalSpace rdfs:label "totalSpace"@en .

observable:browserUserProfile rdfs:label "Browser User Profile"@en .

observable:totalSpace rdfs:comment "Specifies the total amount of space available on the partition, in bytes."@en .

observable:browserUserProfile rdfs:comment "Specifies the web browser user profile for which the URL history entry was created."@en .

observable:totalSpace rdfs:range xsd:integer .

observable:browserUserProfile rdfs:range xsd:string .

observable:triggerBeginTime a owl:DatatypeProperty .

observable:byteOrder a owl:DatatypeProperty .

observable:triggerBeginTime rdfs:label "triggerBeginTime"@en .

observable:byteOrder rdfs:label "byteOrder"@en .

observable:triggerBeginTime rdfs:comment "Specifies the date/time that the trigger is activated."@en .

_:node1gm7uj6vjx2338 a rdfs:Datatype .

observable:triggerBeginTime rdfs:range xsd:dateTime .

_:node1gm7uj6vjx2339 rdf:first vocabulary:EndiannessTypeVocab .

observable:triggerDelay a owl:DatatypeProperty .

_:node1gm7uj6vjx2339 rdf:rest _:node1gm7uj6vjx2340 .

observable:triggerDelay rdfs:label "triggerDelay"@en .

_:node1gm7uj6vjx2340 rdf:first xsd:string .

observable:triggerDelay rdfs:comment "Specifies the delay that takes place between when the task is registered and when the task is started."@en .

_:node1gm7uj6vjx2340 rdf:rest rdf:nil .

observable:triggerDelay rdfs:range xsd:string .

_:node1gm7uj6vjx2338 owl:unionOf _:node1gm7uj6vjx2339 .

observable:triggerEndTime a owl:DatatypeProperty .

observable:byteOrder rdfs:range _:node1gm7uj6vjx2338 .

observable:triggerEndTime rdfs:label "triggerEndTime"@en .

observable:byteStringValue a owl:DatatypeProperty .

observable:triggerEndTime rdfs:comment "Specifies the date/time that the trigger is deactivated."@en .

observable:byteStringValue rdfs:label "byteStringValue"@en .

observable:triggerEndTime rdfs:range xsd:dateTime .

observable:byteStringValue rdfs:comment "Specifies the raw, byte-string representation of the extracted string."@en .

observable:triggerFrequency a owl:DatatypeProperty .

observable:byteStringValue rdfs:range xsd:base64Binary .

observable:triggerFrequency rdfs:label "triggerFrequency"@en .

observable:callType a owl:DatatypeProperty .

observable:triggerFrequency rdfs:comment "Specifies the frequency at which the trigger repeats."@en .

observable:callType rdfs:label "callType"@en .

_:node1gm7uj6vjx2399 a rdfs:Datatype .

observable:callType rdfs:comment "The type of a phone call,for example incoming, outgoing, missed."@en .

_:node1gm7uj6vjx2400 rdf:first vocabulary:TriggerFrequencyVocab .

observable:callType rdfs:range xsd:string .

_:node1gm7uj6vjx2400 rdf:rest _:node1gm7uj6vjx2401 .

observable:camera a owl:ObjectProperty .

_:node1gm7uj6vjx2401 rdf:first xsd:string .

observable:camera rdfs:label "camera"@en .

_:node1gm7uj6vjx2401 rdf:rest rdf:nil .

observable:camera rdfs:comment "The name/make of the camera that was used for taking the picture."@en .

_:node1gm7uj6vjx2399 owl:unionOf _:node1gm7uj6vjx2400 .

observable:camera rdfs:range observable:ObservableObject .

observable:triggerFrequency rdfs:range _:node1gm7uj6vjx2399 .

observable:canEscalatePrivs a owl:DatatypeProperty .

observable:triggerList a owl:ObjectProperty .

observable:canEscalatePrivs rdfs:label "canEscalatePrivs"@en .

observable:triggerList rdfs:label "triggerList"@en .

observable:canEscalatePrivs rdfs:range xsd:boolean .

observable:triggerList rdfs:comment "Specifies a set of triggers used by the scheduled task. See also: http://msdn.microsoft.com/en-us/library/windows/desktop/aa383264(v=vs.85).aspx."@en .

observable:captureCellSite a owl:ObjectProperty .

observable:triggerList rdfs:range observable:TriggerType .

observable:captureCellSite rdfs:label "captureCellSite"@en .

observable:triggerMaxRunTime a owl:DatatypeProperty .

observable:captureCellSite rdfs:comment "Specifies the cell site accessed."@en .

observable:triggerMaxRunTime rdfs:label "triggerMaxRunTime"@en .

observable:captureCellSite rdfs:range observable:CellSite .

observable:triggerMaxRunTime rdfs:comment "The maximum amount of time that the task launched by the trigger is allowed to run. See also: http://msdn.microsoft.com/en-us/library/windows/desktop/aa383868(v=vs.85).aspx."@en .

observable:carrier a owl:ObjectProperty .

observable:triggerMaxRunTime rdfs:range xsd:string .

observable:carrier rdfs:label "carrier"@en .

observable:triggerSessionChangeType a owl:DatatypeProperty .

observable:carrier rdfs:comment "Telecommunications service provider that sold the SIM card."@en .

observable:triggerSessionChangeType rdfs:label "triggerSessionChangeType"@en .

observable:carrier rdfs:range identity:Identity .

observable:triggerSessionChangeType rdfs:comment "Specifies the type of Terminal Server session change that would trigger a task launch. See also: http://msdn.microsoft.com/en-us/library/windows/desktop/aa381298(v=vs.85).aspx."@en .

observable:categories a owl:DatatypeProperty .

observable:triggerSessionChangeType rdfs:range xsd:string .

observable:categories rdfs:label "categories"@en .

observable:triggerType a owl:DatatypeProperty .

observable:categories rdfs:comment "Categories applied to the object."@en .

observable:triggerType rdfs:label "triggerType"@en .

observable:categories rdfs:range xsd:string .

observable:triggerType rdfs:comment "Specifies the type of the task trigger."@en .

observable:cc a owl:ObjectProperty .

_:node1gm7uj6vjx2402 a rdfs:Datatype .

observable:cc rdfs:label "cc"@en .

_:node1gm7uj6vjx2403 rdf:first vocabulary:TriggerTypeVocab .

observable:cc rdfs:range observable:ObservableObject .

_:node1gm7uj6vjx2403 rdf:rest _:node1gm7uj6vjx2404 .

observable:cellSiteCountryCode a owl:DatatypeProperty .

_:node1gm7uj6vjx2404 rdf:first xsd:string .

observable:cellSiteCountryCode rdfs:label "cellSiteCountryCode"@en .

_:node1gm7uj6vjx2404 rdf:rest rdf:nil .

observable:cellSiteCountryCode rdfs:comment "The country code represents the country of the cell site. For GSM, this is the Mobile Country Code (MCC)."@en .

_:node1gm7uj6vjx2402 owl:unionOf _:node1gm7uj6vjx2403 .

observable:cellSiteCountryCode rdfs:range xsd:string .

observable:triggerType rdfs:range _:node1gm7uj6vjx2402 .

observable:cellSiteIdentifier a owl:DatatypeProperty .

observable:twitterHandle a owl:DatatypeProperty .

observable:cellSiteIdentifier rdfs:label "cellSiteIdentifier"@en .

observable:twitterHandle rdfs:label "Twitter Handle"@en-us .

observable:cellSiteIdentifier rdfs:comment "Specifies the unique number used to identify each Cell Site within a location area code."@en .

observable:twitterHandle rdfs:comment "Specifies the twitter handle associated with the profile."@en-us .

observable:cellSiteIdentifier rdfs:range xsd:string .

observable:twitterHandle rdfs:range xsd:string .

observable:cellSiteLocationAreaCode a owl:DatatypeProperty .

observable:twitterId a owl:DatatypeProperty .

observable:cellSiteLocationAreaCode rdfs:label "cellSiteLocationAreaCode"@en .

observable:twitterId rdfs:label "Twitter ID"@en-us .

observable:cellSiteLocationAreaCode rdfs:comment "The location area code is a unique number of current location area of the cell site. A location area is a set of cell site that are grouped together to optimize signalling. For GSM, this is the LAC."@en .

observable:twitterId rdfs:comment "Specifies the twitter id associated with the profile."@en-us .

observable:cellSiteLocationAreaCode rdfs:range xsd:string .

observable:twitterId rdfs:range xsd:string .

observable:cellSiteNetworkCode a owl:DatatypeProperty .

observable:uninstallDate a owl:DatatypeProperty .

observable:cellSiteNetworkCode rdfs:label "cellSiteNetworkCode"@en .

observable:uninstallDate rdfs:label "uninstallDate"@en .

observable:cellSiteNetworkCode rdfs:comment "This code identifies the mobile operator of the cell site. For GSM, this is the Mobile Network Code (MNC) and for CMDA this is the network identifier (NID)."@en .

observable:uninstallDate rdfs:comment "Specifies the date the operating system or application was uninstalled."@en .

observable:cellSiteNetworkCode rdfs:range xsd:string .

observable:uninstallDate rdfs:range xsd:dateTime .

observable:cellSiteType a owl:DatatypeProperty .

observable:updatedDate a owl:DatatypeProperty .

observable:cellSiteType rdfs:label "cellSiteType"@en .

observable:updatedDate rdfs:label "updatedDate"@en .

observable:cellSiteType rdfs:comment "Specifies the technology used by the Cell Site (e.g., GSM, CDMA, or LTE)."@en .

observable:updatedDate rdfs:comment "Specifies the date in which the registered domain information was last updated."@en .

observable:cellSiteType rdfs:range xsd:string .

observable:updatedDate rdfs:range xsd:dateTime .

observable:uptime a owl:DatatypeProperty .

observable:certificateIssuer a owl:ObjectProperty .

observable:uptime rdfs:label "uptime"@en .

observable:certificateIssuer rdfs:label "certificateIssuer"@en .

observable:uptime rdfs:comment "Specifies the duration that represents the current amount of time that the system has been up."@en .

observable:certificateIssuer rdfs:range identity:Identity .

observable:uptime rdfs:range xsd:string .

observable:certificatePolicies a owl:DatatypeProperty .

observable:url a owl:ObjectProperty .

observable:certificatePolicies rdfs:label "certificatePolicies"@en .

observable:url rdfs:label "url"@en .

observable:certificatePolicies rdfs:range xsd:string .

observable:url rdfs:comment "Specifies a URL associated with a particular observable object or facet."@en .

observable:certificateSubject a owl:ObjectProperty .

observable:url rdfs:range observable:ObservableObject .

observable:certificateSubject rdfs:label "certificateSubject"@en .

observable:urlHistoryEntry a owl:ObjectProperty .

observable:certificateSubject rdfs:range core:UcoObject .

observable:urlHistoryEntry rdfs:label "URL History Entries"@en .

observable:characteristics a owl:DatatypeProperty .

observable:urlHistoryEntry rdfs:comment "Specifies a URL history record stored in the browser's history."@en .

observable:characteristics rdfs:label "characteristics"@en .

observable:urlHistoryEntry rdfs:range observable:URLHistoryEntry .

observable:characteristics rdfs:comment "Specifies the flags that indicate the files characteristics."@en ;
	rdfs:range xsd:unsignedShort .

observable:checksum a owl:DatatypeProperty ;
	rdfs:label "checksum"@en ;
	rdfs:comment "Specifies the checksum of the PE binary."@en .

observable:urlTargeted a owl:DatatypeProperty .

observable:checksum rdfs:range xsd:unsignedInt .

observable:urlTargeted rdfs:label "urlTargeted"@en .

observable:clockSetting a owl:DatatypeProperty .

observable:urlTargeted rdfs:comment "The target of the bookmark."@en .

observable:clockSetting rdfs:label "clockSetting"@en .

observable:urlTargeted rdfs:range xsd:anyURI .

observable:clockSetting rdfs:comment "The generalizedTime value on the mobile device when it was processed."@en .

observable:urlTransitionType a owl:DatatypeProperty .

observable:clockSetting rdfs:range xsd:dateTime .

observable:urlTransitionType rdfs:label "Transition Type"@en .

observable:clusterSize a owl:DatatypeProperty .

observable:urlTransitionType rdfs:comment "Specifies how a browser navigated to a particular URL on a particular visit."@en .

observable:clusterSize rdfs:label "clusterSize"@en .

_:node1gm7uj6vjx2405 a rdfs:Datatype .

observable:clusterSize rdfs:comment "The size of cluster allocation units in a file system."@en .

_:node1gm7uj6vjx2406 rdf:first xsd:string .

observable:clusterSize rdfs:range xsd:integer .

_:node1gm7uj6vjx2406 rdf:rest _:node1gm7uj6vjx2407 .

observable:columnName a owl:DatatypeProperty .

_:node1gm7uj6vjx2407 rdf:first vocabulary:URLTransitionTypeVocab .

observable:columnName rdfs:label "columnName"@en .

_:node1gm7uj6vjx2407 rdf:rest rdf:nil .

observable:columnName rdfs:range xsd:string .

_:node1gm7uj6vjx2405 owl:unionOf _:node1gm7uj6vjx2406 .

observable:comClassID a owl:DatatypeProperty .

observable:urlTransitionType rdfs:range _:node1gm7uj6vjx2405 .

observable:comClassID rdfs:label "comClassID"@en .

observable:userLocationString a owl:DatatypeProperty .

observable:comClassID rdfs:comment "Specifies the ID of the COM action. See also: http://msdn.microsoft.com/en-us/library/windows/desktop/aa380613(v=vs.85).aspx."@en .

observable:userLocationString rdfs:label "User Location String"@en-us .

observable:comClassID rdfs:range xsd:string .

observable:userLocationString rdfs:comment "Specifies the user-provided location string associated with the profile."@en-us .

observable:comData a owl:DatatypeProperty .

observable:userLocationString rdfs:range xsd:string .

observable:comData rdfs:label "comData"@en .

observable:userName a owl:DatatypeProperty .

observable:comData rdfs:comment "Specifies the data associated with the COM handler. See also: http://msdn.microsoft.com/en-us/library/windows/desktop/aa380613(v=vs.85).aspx."@en .

observable:userName rdfs:label "userName"@en .

observable:comData rdfs:range xsd:string .

observable:userName rdfs:comment "Username used to authenticate to this resource."@en .

observable:comment a owl:DatatypeProperty .

observable:userName rdfs:range xsd:string .

observable:comment rdfs:label "comment"@en .

observable:validityNotAfter a owl:DatatypeProperty .

observable:comment rdfs:range xsd:string .

observable:validityNotAfter rdfs:label "validityNotAfter"@en .

observable:compressionMethod a owl:DatatypeProperty .

observable:validityNotAfter rdfs:range xsd:dateTime .

observable:compressionMethod rdfs:label "compressionMethod"@en .

observable:validityNotBefore a owl:DatatypeProperty .

observable:compressionMethod rdfs:comment "The algorithm used to compress the data."@en .

observable:validityNotBefore rdfs:label "validityNotBefore"@en .

observable:compressionMethod rdfs:range xsd:string .

observable:validityNotBefore rdfs:range xsd:dateTime .

observable:compressionRatio a owl:DatatypeProperty .

observable:value a owl:DatatypeProperty .

observable:compressionRatio rdfs:label "compressionRatio"@en .

observable:value rdfs:label "value"@en .

observable:compressionRatio rdfs:comment "The compression ratio of the compressed data."@en .

observable:value rdfs:range xsd:string .

observable:compressionRatio rdfs:range xsd:decimal .

observable:values a owl:DatatypeProperty .

observable:contact a owl:ObjectProperty .

observable:values rdfs:label "values"@en .

observable:contact rdfs:label "contact"@en .

observable:values rdfs:comment "The values that were enumerated as a result of the action on the object."@en .

observable:contact rdfs:comment "Contact specifies information characterizing contact details for a single entity."@en .

observable:values rdfs:range xsd:string .

observable:contact rdfs:range observable:ObservableObject .

observable:version a owl:DatatypeProperty .

observable:contactAddress a owl:ObjectProperty .

observable:version rdfs:label "version"@en .

observable:contactAddress rdfs:label "contactAddress"@en .

observable:version rdfs:range xsd:string .

observable:contactAddress rdfs:comment "Contact address specifies information characterizing a geolocation address of a contact entity."@en .

observable:visibility a owl:DatatypeProperty .

observable:contactAddress rdfs:range observable:ContactAddress .

observable:visibility rdfs:label "visibility"@en .

observable:contactAddressScope a owl:DatatypeProperty .

observable:visibility rdfs:range xsd:boolean .

observable:contactAddressScope rdfs:label "contactAddressScope"@en .

observable:visitCount a owl:DatatypeProperty .

observable:contactAddressScope rdfs:comment "Contact address scope specifies the relevant scope (home, work, school, etc) for a geolocation address of a contact entity."@en .

observable:visitCount rdfs:label "visitCount"@en .

_:node1gm7uj6vjx2341 a rdfs:Datatype .

observable:visitCount rdfs:comment "Specifies the number of times a URL has been visited by a particular web browser."@en .

_:node1gm7uj6vjx2342 rdf:first xsd:string .

observable:visitCount rdfs:range xsd:integer .

_:node1gm7uj6vjx2342 rdf:rest _:node1gm7uj6vjx2343 .

observable:visitDuration a owl:DatatypeProperty .

_:node1gm7uj6vjx2343 rdf:first vocabulary:ContactAddressScopeVocab .

observable:visitDuration rdfs:label "Visit Duration"@en .

_:node1gm7uj6vjx2343 rdf:rest rdf:nil .

observable:visitDuration rdfs:comment "Specifies the duration of a specific visit of a URL within a particular browser."@en .

_:node1gm7uj6vjx2341 owl:unionOf _:node1gm7uj6vjx2342 .

observable:visitDuration rdfs:range xsd:duration .

observable:contactAddressScope rdfs:range _:node1gm7uj6vjx2341 .

observable:visitTime a owl:DatatypeProperty .

observable:contactAffiliation a owl:ObjectProperty .

observable:visitTime rdfs:label "Visit Time"@en .

observable:contactAffiliation rdfs:label "contactAffiliation"@en .

observable:visitTime rdfs:comment "Specifies the date/time of a specific visit of a URL within a particular browser."@en .

observable:contactAffiliation rdfs:comment "Contact affiliation specifies information characterizing details of an organizational affiliation for a single contact entity."@en .

observable:visitTime rdfs:range xsd:dateTime .

observable:contactAffiliation rdfs:range observable:ContactAffiliation .

observable:volume a owl:ObjectProperty .

observable:contactEmail a owl:ObjectProperty .

observable:volume rdfs:label "volume"@en .

observable:contactEmail rdfs:label "contactEmail"@en .

observable:volume rdfs:comment "The volume from which the prefetch application was run. If the applicatin was run from multiple volumes, there will be a separate prefetch file for each."@en .

observable:contactEmail rdfs:comment "Contact email specifies information characterizing details for contacting a contact entity by email."@en .

observable:volume rdfs:range observable:ObservableObject .

observable:contactEmail rdfs:range observable:ContactEmail .

observable:volumeID a owl:DatatypeProperty .

observable:contactEmailScope a owl:DatatypeProperty .

observable:volumeID rdfs:label "volumeID"@en .

observable:contactEmailScope rdfs:label "contactEmailScope"@en .

observable:volumeID rdfs:comment "The unique identifier of the volume."@en .

observable:contactEmailScope rdfs:comment "Contact email scope specifies the relevant scope (home, work, school, etc) of details for contacting a contact entity by email."@en .

observable:volumeID rdfs:range xsd:string .

_:node1gm7uj6vjx2344 a rdfs:Datatype .

observable:whoisContactType a owl:DatatypeProperty .

_:node1gm7uj6vjx2345 rdf:first xsd:string .

observable:whoisContactType rdfs:label "whoisContactType"@en .

_:node1gm7uj6vjx2345 rdf:rest _:node1gm7uj6vjx2346 .

observable:whoisContactType rdfs:comment "Specifies what type of WHOIS contact this is."@en .

_:node1gm7uj6vjx2346 rdf:first vocabulary:ContactEmailScopeVocab .

_:node1gm7uj6vjx2408 a rdfs:Datatype .

_:node1gm7uj6vjx2346 rdf:rest rdf:nil .

_:node1gm7uj6vjx2409 rdf:first xsd:string .

_:node1gm7uj6vjx2344 owl:unionOf _:node1gm7uj6vjx2345 .

_:node1gm7uj6vjx2409 rdf:rest _:node1gm7uj6vjx2410 .

observable:contactEmailScope rdfs:range _:node1gm7uj6vjx2344 .

_:node1gm7uj6vjx2410 rdf:first vocabulary:WhoisContactTypeVocab .

observable:contactGroup a owl:DatatypeProperty .

_:node1gm7uj6vjx2410 rdf:rest rdf:nil .

observable:contactGroup rdfs:label "contactGroup"@en .

_:node1gm7uj6vjx2408 owl:unionOf _:node1gm7uj6vjx2409 .

observable:contactGroup rdfs:comment "Contact group specifies the name/tag of a particular named/tagged grouping of contacts."@en .

observable:whoisContactType rdfs:range _:node1gm7uj6vjx2408 .

observable:contactGroup rdfs:range xsd:string .

observable:whoisServer a owl:ObjectProperty .

observable:contactID a owl:DatatypeProperty .

observable:whoisServer rdfs:label "whoisServer"@en .

observable:contactID rdfs:label "contactID"@en .

observable:whoisServer rdfs:comment "Specifies the corresponding whois server for a registrar."@en .

observable:contactID rdfs:comment "Specifies an ID for the contact."@en .

observable:whoisServer rdfs:range observable:ObservableObject .

observable:contactID rdfs:range xsd:string .

observable:win32VersionValue a owl:DatatypeProperty .

observable:contactMessaging a owl:ObjectProperty .

observable:win32VersionValue rdfs:label "win32VersionValue"@en .

observable:contactMessaging rdfs:label "contactMessaging"@en .

observable:win32VersionValue rdfs:comment "Specifies the reserved win32 version value."@en .

observable:contactMessaging rdfs:comment "Contact messaging specifies information characterizing details for contacting a contact entity by digital messaging."@en .

observable:win32VersionValue rdfs:range xsd:unsignedInt .

observable:contactMessaging rdfs:range observable:ContactMessaging .

observable:windowTitle a owl:DatatypeProperty .

observable:contactMessagingPlatform a owl:ObjectProperty .

observable:windowTitle rdfs:label "windowTitle"@en .

observable:contactMessagingPlatform rdfs:label "contactMessagingPlatform"@en .

observable:windowTitle rdfs:range xsd:string .

observable:contactMessagingPlatform rdfs:comment "A contact messaging platform specifies a digital messaging platform associated with a contact."@en .

observable:windowsDirectory a owl:ObjectProperty .

observable:contactMessagingPlatform rdfs:range observable:ObservableObject .

observable:windowsDirectory rdfs:label "windowsDirectory"@en .

observable:contactNote a owl:DatatypeProperty .

observable:windowsDirectory rdfs:comment "The Windows_Directory field specifies the fully-qualified path to the Windows install directory."@en .

observable:contactNote rdfs:label "contactNote"@en .

observable:windowsDirectory rdfs:range observable:ObservableObject .

observable:contactNote rdfs:comment "Contact note specifies a comment/note associated with a given contact."@en .

observable:windowsSystemDirectory a owl:ObjectProperty .

observable:contactNote rdfs:range xsd:string .

observable:windowsSystemDirectory rdfs:label "windowsSystemDirectory"@en .

observable:contactOrganization a owl:ObjectProperty .

observable:windowsSystemDirectory rdfs:comment "The Windows_System_Directory field specifies the fully-qualified path to the Windows system directory."@en .

observable:contactOrganization rdfs:label "contactOrganization"@en .

observable:windowsSystemDirectory rdfs:range observable:ObservableObject .

observable:contactOrganization rdfs:comment "The name of the organization a contact works for or is assocciated with."@en .

observable:windowsTempDirectory a owl:ObjectProperty .

observable:contactOrganization rdfs:range identity:Organization .

observable:windowsTempDirectory rdfs:label "windowsTempDirectory"@en .

observable:contactPhone a owl:ObjectProperty .

observable:windowsTempDirectory rdfs:comment "The Windows_Temp_Directory field specifies the fully-qualified path to the Windows temporary files directory."@en .

observable:contactPhone rdfs:label "contactPhone"@en .

observable:windowsTempDirectory rdfs:range observable:ObservableObject .

observable:contactPhone rdfs:comment "Contact phone specifies information characterizing details for contacting a contact entity by telephone."@en .

observable:windowsVolumeAttributes a owl:DatatypeProperty .

observable:contactPhone rdfs:range observable:ContactPhone .

observable:windowsVolumeAttributes rdfs:label "windowsVolumeAttributes"@en .

observable:contactPhoneNumber a owl:ObjectProperty .

observable:windowsVolumeAttributes rdfs:comment "Specifies the attributes of a windows volume."@en .

observable:contactPhoneNumber rdfs:label "contactPhoneNumber"@en .

observable:windowsVolumeAttributes rdfs:range vocabulary:WindowsVolumeAttributeVocab .

observable:contactPhoneNumber rdfs:comment "Contact phone number specifies a telephone service account number for contacting a contact entity by telephone."@en .

observable:wirelessNetworkSecurityMode a owl:DatatypeProperty .

observable:contactPhoneNumber rdfs:range observable:ObservableObject .

observable:wirelessNetworkSecurityMode rdfs:label "wirelessNetworkSecurityMode"@en .

observable:contactPhoneScope a owl:DatatypeProperty .

observable:wirelessNetworkSecurityMode rdfs:comment "Specifies the security mode of a wireless network (None, WEP, WPA, etc)."@en .

observable:contactPhoneScope rdfs:label "contactPhoneScope"@en .

_:node1gm7uj6vjx2411 a rdfs:Datatype .

observable:contactPhoneScope rdfs:comment "Contact phone scope specifies the relevant scope (home, work, school, etc) of details for contacting a contact entity by telephone."@en .

_:node1gm7uj6vjx2412 rdf:first vocabulary:WirelessNetworkSecurityModeVocab .

_:node1gm7uj6vjx2347 a rdfs:Datatype .

_:node1gm7uj6vjx2412 rdf:rest _:node1gm7uj6vjx2413 .

_:node1gm7uj6vjx2348 rdf:first xsd:string .

_:node1gm7uj6vjx2413 rdf:first xsd:string .

_:node1gm7uj6vjx2348 rdf:rest _:node1gm7uj6vjx2349 .

_:node1gm7uj6vjx2413 rdf:rest rdf:nil .

_:node1gm7uj6vjx2349 rdf:first vocabulary:ContactPhoneScopeVocab .

_:node1gm7uj6vjx2411 owl:unionOf _:node1gm7uj6vjx2412 .

_:node1gm7uj6vjx2349 rdf:rest rdf:nil .

observable:wirelessNetworkSecurityMode rdfs:range _:node1gm7uj6vjx2411 .

_:node1gm7uj6vjx2347 owl:unionOf _:node1gm7uj6vjx2348 .

observable:workItemData a owl:ObjectProperty .

observable:contactPhoneScope rdfs:range _:node1gm7uj6vjx2347 .

observable:workItemData rdfs:label "workItemData"@en .

observable:contactProfile a owl:ObjectProperty .

observable:workItemData rdfs:comment "Specifies application defined data associated with the scheduled task. See also: http://msdn.microsoft.com/en-us/library/windows/desktop/aa381271(v=vs.85).aspx."@en .

observable:contactProfile rdfs:label "contactProfile"@en .

observable:workItemData rdfs:range observable:ObservableObject .

observable:contactProfile rdfs:comment "Contact profile specifies information characterizing details for contacting a contact entity by online service."@en .

observable:workingDirectory a owl:ObjectProperty .

observable:contactProfile rdfs:range observable:ContactProfile .

observable:workingDirectory rdfs:label "workingDirectory"@en .

observable:contactProfilePlatform a owl:ObjectProperty .

observable:workingDirectory rdfs:comment "Specifies the working directory for the scheduled task. See also: http://msdn.microsoft.com/en-us/library/windows/desktop/aa381878(v=vs.85).aspx."@en .

observable:contactProfilePlatform rdfs:label "contactProfilePlatform"@en .

observable:workingDirectory rdfs:range observable:ObservableObject .

observable:contactProfilePlatform rdfs:comment "A contact profile platform specifies an online service platform associated with a contact."@en .

observable:x509v3extensions a owl:ObjectProperty .

observable:contactProfilePlatform rdfs:range observable:ObservableObject .

observable:x509v3extensions rdfs:label "x509V3Extensions"@en .

observable:contactSIP a owl:ObjectProperty .

observable:x509v3extensions rdfs:range observable:X509V3ExtensionsFacet .

observable:contactSIP rdfs:label "contactSIP"@en .

observable:xMailer a owl:DatatypeProperty .

observable:contactSIP rdfs:comment "Contact SIP specifies information characterizing details for contacting a contact entity by Session Initiation Protocol (SIP)."@en .

observable:xMailer rdfs:label "xMailer"@en .

observable:contactSIP rdfs:range observable:ContactSIP .

observable:xMailer rdfs:range xsd:string .

observable:contactSIPScope a owl:DatatypeProperty .

observable:xOriginatingIP a owl:ObjectProperty .

observable:contactSIPScope rdfs:label "contactSIPScope"@en .

observable:xOriginatingIP rdfs:label "xOriginatingIP"@en .

observable:contactSIPScope rdfs:comment "Contact SIP scope specifies the relevant scope (home, work, school, etc) of details for contacting a contact entity by Session Initiation Protocol (SIP)."@en .

observable:xOriginatingIP rdfs:range observable:ObservableObject .

_:node1gm7uj6vjx2350 a rdfs:Datatype .

_:node1gm7uj6vjx2351 rdf:first xsd:string ;
	rdf:rest _:node1gm7uj6vjx2352 .

_:node1gm7uj6vjx2352 rdf:first vocabulary:ContactSIPScopeVocab ;
	rdf:rest rdf:nil .

_:node1gm7uj6vjx2350 owl:unionOf _:node1gm7uj6vjx2351 .

observable:contactSIPScope rdfs:range _:node1gm7uj6vjx2350 .

observable:contactURL a owl:ObjectProperty ;
	rdfs:label "contactURL"@en ;
	rdfs:comment "Contact URL specifies information characterizing details for contacting a contact entity by Uniform Resource Locator (URL)."@en ;
	rdfs:range observable:ContactURL .

observable:contactURLScope a owl:DatatypeProperty ;
	rdfs:label "contactURLScope"@en ;
	rdfs:comment "Contact url scope specifies the relevant scope (homepage, home, work, school, etc) of details for contacting a contact entity by Uniform Resource Locator (URL)."@en .

_:node1gm7uj6vjx2353 a rdfs:Datatype .

_:node1gm7uj6vjx2354 rdf:first xsd:string ;
	rdf:rest _:node1gm7uj6vjx2355 .

_:node1gm7uj6vjx2355 rdf:first vocabulary:ContactURLScopeVocab ;
	rdf:rest rdf:nil .

_:node1gm7uj6vjx2353 owl:unionOf _:node1gm7uj6vjx2354 .

observable:contactURLScope rdfs:range _:node1gm7uj6vjx2353 .

observable:contentDisposition a owl:DatatypeProperty ;
	rdfs:label "contentDisposition"@en ;
	rdfs:range xsd:string .

observable:contentRecoveredStatus a owl:DatatypeProperty ;
	rdfs:label "contentRecoveredStatus"@en ;
	rdfs:comment "Specifies the recoverability status of the content of an object."@en .

_:node1gm7uj6vjx2356 a rdfs:Datatype .

_:node1gm7uj6vjx2357 rdf:first vocabulary:RecoveredObjectStatusVocab ;
	rdf:rest _:node1gm7uj6vjx2358 .

_:node1gm7uj6vjx2358 rdf:first xsd:string ;
	rdf:rest rdf:nil .

_:node1gm7uj6vjx2356 owl:unionOf _:node1gm7uj6vjx2357 .

observable:contentRecoveredStatus rdfs:range _:node1gm7uj6vjx2356 .

observable:contentType a owl:DatatypeProperty ;
	rdfs:label "contentType"@en ;
	rdfs:range xsd:string .

observable:context a owl:DatatypeProperty ;
	rdfs:label "context"@en ;
	rdfs:range xsd:string .

observable:controlCode a owl:DatatypeProperty ;
	rdfs:label "controlCode"@en ;
	rdfs:comment "Specifies the actual control code that was sent to the observable object."@en ;
	rdfs:range xsd:string .

observable:cookieDomain a owl:ObjectProperty ;
	rdfs:label "cookieDomain"@en ;
	rdfs:comment "The domain for which the cookie is stored, for example nfi.minjus.nl."@en ;
	rdfs:range observable:ObservableObject .

observable:cookieName a owl:DatatypeProperty ;
	rdfs:label "cookieName"@en ;
	rdfs:comment "The name of the cookie."@en ;
	rdfs:range xsd:string .

observable:cookiePath a owl:DatatypeProperty ;
	rdfs:label "cookiePath"@en ;
	rdfs:comment "String representation of the path of the cookie."@en ;
	rdfs:range xsd:string .

observable:cpeid a owl:DatatypeProperty ;
	rdfs:label "cpeid"@en ;
	rdfs:comment "Specifies the Common Platform Enumeration identifier for the software."@en ;
	rdfs:range xsd:string .

observable:cpu a owl:DatatypeProperty ;
	rdfs:label "cpu"@en ;
	rdfs:comment "Specifies the name of the CPU used by the system."@en ;
	rdfs:range xsd:string .

observable:cpuFamily a owl:DatatypeProperty ;
	rdfs:label "cpuFamily"@en ;
	rdfs:comment "Specifies the name of the CPU family used by the system."@en ;
	rdfs:range xsd:string .

observable:creationDate a owl:DatatypeProperty ;
	rdfs:label "creationDate"@en ;
	rdfs:comment "Specifies the date in which the registered domain was created."@en ;
	rdfs:range xsd:dateTime .

observable:creationFlags a owl:DatatypeProperty ;
	rdfs:label "creationFlags"@en ;
	rdfs:range xsd:unsignedInt .

observable:creationTime a owl:DatatypeProperty ;
	rdfs:label "creationTime"@en ;
	rdfs:range xsd:dateTime .

observable:creator a owl:ObjectProperty ;
	rdfs:label "creator"@en ;
	rdfs:comment "Specifies the name of the creator of the registry key."@en ;
	rdfs:range observable:ObservableObject .

observable:creatorUser a owl:ObjectProperty ;
	rdfs:label "creatorUser"@en ;
	rdfs:comment "The user that created/owns the process."@en ;
	rdfs:range observable:ObservableObject .

observable:crlDistributionPoints a owl:DatatypeProperty ;
	rdfs:label "crlDistributionPoints"@en ;
	rdfs:range xsd:string .

observable:currentSystemDate a owl:DatatypeProperty ;
	rdfs:label "currentSystemDate"@en ;
	rdfs:comment "Specifies the current date on the system."@en ;
	rdfs:range xsd:dateTime .

observable:currentWorkingDirectory a owl:DatatypeProperty ;
	rdfs:label "currentWorkingDirectory"@en ;
	rdfs:range xsd:string .

observable:cyberAction a owl:ObjectProperty ;
	rdfs:label "cyberAction"@en ;
	rdfs:comment "The action taken in response to the event."@en ;
	rdfs:range observable:ObservableAction .

observable:data a owl:DatatypeProperty ;
	rdfs:label "data"@en ;
	rdfs:range xsd:string .

observable:dataPayload a owl:DatatypeProperty ;
	rdfs:label "dataPayload"@en ;
	rdfs:range xsd:string .

observable:dataPayloadReferenceURL a owl:ObjectProperty ;
	rdfs:label "dataPayloadReferenceURL"@en ;
	rdfs:range observable:ObservableObject .

observable:dataType a owl:DatatypeProperty ;
	rdfs:label "dataType"@en ;
	rdfs:range xsd:string .

observable:depEnabled a owl:DatatypeProperty ;
	rdfs:label "depEnabled"@en ;
	rdfs:range xsd:boolean .

observable:descriptions a owl:DatatypeProperty ;
	rdfs:label "descriptions"@en ;
	rdfs:range xsd:string .

observable:destination a owl:DatatypeProperty ;
	rdfs:label "destination"@en ;
	rdfs:comment "The destination of a global flag. See also: http://msdn.microsoft.com/en-us/library/windows/hardware/ff549646(v=vs.85).aspx."@en ;
	rdfs:range xsd:string .

observable:destinationFlags a owl:DatatypeProperty ;
	rdfs:label "destinationFlags"@en ;
	rdfs:comment "Specifies the destination TCP flags."@en ;
	rdfs:range xsd:hexBinary .

observable:destinationPort a owl:DatatypeProperty ;
	rdfs:label "destinationPort"@en ;
	rdfs:comment "Specifies the destination port used in the connection, as an integer in the range of 0 - 65535."@en ;
	rdfs:range xsd:integer .

observable:deviceType a owl:DatatypeProperty ;
	rdfs:label "deviceType"@en ;
	rdfs:range xsd:string .

observable:dhcpLeaseExpires a owl:DatatypeProperty ;
	rdfs:label "dhcpLeaseExpires"@en ;
	rdfs:comment "Specifies the date/time that the DHCP lease obtained on the network interface expires."@en ;
	rdfs:range xsd:dateTime .

observable:dhcpLeaseObtained a owl:DatatypeProperty ;
	rdfs:label "dhcpLeaseObtained"@en ;
	rdfs:comment "Specifies the date/time that the DHCP lease was obtained on the network interface."@en ;
	rdfs:range xsd:dateTime .

observable:dhcpServer a owl:ObjectProperty ;
	rdfs:label "dhcpServer"@en ;
	rdfs:comment "Specifies the list of DHCP server IP Addresses used by the network interface."@en ;
	rdfs:range observable:ObservableObject .

observable:diskPartitionType a owl:DatatypeProperty ;
	rdfs:label "diskPartitionType"@en ;
	rdfs:comment "Specifies the type of partition being characterized."@en ;
	rdfs:range xsd:string .

observable:diskSize a owl:DatatypeProperty ;
	rdfs:label "diskSize"@en ;
	rdfs:comment "The size of the disk, in bytes."@en ;
	rdfs:range xsd:integer .

observable:diskType a owl:DatatypeProperty ;
	rdfs:label "diskType"@en ;
	rdfs:comment "The type of disk being characterized, e.g., removable."@en ;
	rdfs:range xsd:string .

observable:displayName a owl:DatatypeProperty ;
	rdfs:label "displayName"@en ;
	rdfs:comment "Display name specifies the name to display for some entity within a user interface."@en ;
	rdfs:range xsd:string .

observable:dllCharacteristics a owl:DatatypeProperty ;
	rdfs:label "dllCharacteristics"@en ;
	rdfs:comment "Specifies the flags that characterize the PE binary."@en ;
	rdfs:range xsd:unsignedShort .

observable:dnssec a owl:DatatypeProperty ;
	rdfs:label "dnssec"@en ;
	rdfs:comment "Specifies the DNSSEC property associated with a Whois entry. Acceptable values are: 'Signed' or 'Unsigned'."@en ;
	rdfs:range vocabulary:WhoisDNSSECTypeVocab .

observable:documentInformationDictionary a owl:ObjectProperty ;
	rdfs:label "documentInformationDictionary"@en ;
	rdfs:range types:ControlledDictionary .

observable:domain a owl:DatatypeProperty ;
	rdfs:label "domain"@en ;
	rdfs:comment "The domain(s) that the system belongs to."@en ;
	rdfs:range xsd:string .

observable:domainID a owl:DatatypeProperty ;
	rdfs:label "domainID"@en ;
	rdfs:comment "Specifies the domain id for the domain associated with a Whois entry."@en ;
	rdfs:range xsd:string .

observable:domainName a owl:ObjectProperty ;
	rdfs:label "domainName"@en ;
	rdfs:comment "Specifies the corresponding domain name for a whois entry."@en ;
	rdfs:range observable:ObservableObject .

observable:driveLetter a owl:DatatypeProperty ;
	rdfs:label "driveLetter"@en ;
	rdfs:comment "Specifies the drive letter of a windows volume."@en ;
	rdfs:range xsd:string .

observable:driveType a owl:DatatypeProperty ;
	rdfs:label "driveType"@en ;
	rdfs:comment "Specifies the drive type of a windows volume."@en .

_:node1gm7uj6vjx2359 a rdfs:Datatype .

_:node1gm7uj6vjx2360 rdf:first vocabulary:WindowsDriveTypeVocab ;
	rdf:rest _:node1gm7uj6vjx2361 .

_:node1gm7uj6vjx2361 rdf:first xsd:string ;
	rdf:rest rdf:nil .

_:node1gm7uj6vjx2359 owl:unionOf _:node1gm7uj6vjx2360 .

observable:driveType rdfs:range _:node1gm7uj6vjx2359 .

observable:dst a owl:ObjectProperty ;
	rdfs:label "dst"@en ;
	rdfs:comment "Specifies the destination(s) of the network connection."@en ;
	rdfs:range observable:ObservableObject .

observable:dstBytes a owl:DatatypeProperty ;
	rdfs:label "dstBytes"@en ;
	rdfs:range xsd:integer .

observable:dstPackets a owl:DatatypeProperty ;
	rdfs:label "dstPackets"@en ;
	rdfs:range xsd:integer .

observable:dstPayload a owl:ObjectProperty ;
	rdfs:label "dstPayload"@en ;
	rdfs:range observable:ObservableObject .

observable:duration a owl:DatatypeProperty ;
	rdfs:label "duration"@en ;
	rdfs:comment "The duration of the phone call in seconds."@en ;
	rdfs:range xsd:integer .

observable:effectiveGroup a owl:DatatypeProperty ;
	rdfs:label "effectiveGroup"@en ;
	rdfs:comment "Specifies the name of the effective group used in the user session."@en ;
	rdfs:range xsd:string .

observable:effectiveGroupID a owl:DatatypeProperty ;
	rdfs:label "effectiveGroupID"@en ;
	rdfs:comment "Specifies the effective group ID of the group used in the user session."@en ;
	rdfs:range xsd:string .

observable:effectiveUser a owl:ObjectProperty ;
	rdfs:label "effectiveUser"@en ;
	rdfs:comment "Specifies the effective user details used in the user session."@en ;
	rdfs:range observable:ObservableObject .

observable:elevation a owl:DatatypeProperty ;
	rdfs:label "elevation"@en ;
	rdfs:comment "The angle in degrees of the antenna from the local horizontal plane."@en ;
	rdfs:range xsd:decimal .

observable:emailAddress a owl:ObjectProperty ;
	rdfs:label "emailAddress"@en ;
	rdfs:comment "An email address."@en ;
	rdfs:range observable:ObservableObject .

observable:encoding a owl:DatatypeProperty ;
	rdfs:label "Encoding"@en ;
	rdfs:comment "The encoding method used for the extracted string."@en ;
	rdfs:range xsd:string .

observable:encodingMethod a owl:DatatypeProperty ;
	rdfs:label "encodingMethod"@en ;
	rdfs:range xsd:string .

observable:encryptionIV a owl:DatatypeProperty ;
	rdfs:label "encryptionIV"@en ;
	rdfs:range xsd:string .

observable:encryptionKey a owl:DatatypeProperty ;
	rdfs:label "encryptionKey"@en ;
	rdfs:range xsd:string .

observable:encryptionMethod a owl:DatatypeProperty ;
	rdfs:label "encryptionMethod"@en ;
	rdfs:range xsd:string .

observable:encryptionMode a owl:DatatypeProperty ;
	rdfs:label "encryptionMode"@en ;
	rdfs:range xsd:string .

observable:endTime a owl:DatatypeProperty ;
	rdfs:label "endTime"@en ;
	rdfs:range xsd:dateTime .

observable:englishTranslation a owl:DatatypeProperty ;
	rdfs:label "englishTranslation"@en ;
	rdfs:comment "Specifies the English translation of the string, if it is not written in English."@en ;
	rdfs:range xsd:string .

observable:entropy a owl:DatatypeProperty ;
	rdfs:label "entropy"@en ;
	rdfs:comment "Shannon entropy (a measure of randomness) of the data."@en ;
	rdfs:range xsd:decimal .

observable:entryID a owl:DatatypeProperty ;
	rdfs:label "entryID"@en ;
	rdfs:comment "A unique identifier for the file within the filesystem."@en ;
	rdfs:range xsd:integer .

observable:environmentVariables a owl:ObjectProperty ;
	rdfs:label "environmentVariables"@en ;
	rdfs:comment "A list of environment variables associated with the process. "@en ;
	rdfs:range types:Dictionary .

observable:eventRecordDevice a owl:ObjectProperty ;
	rdfs:label "device"@en ;
	rdfs:comment "The device on which the log entry was generated."@en ;
	rdfs:range observable:ObservableObject .

observable:eventRecordID a owl:DatatypeProperty ;
	rdfs:label "eventRecordID"@en ;
	rdfs:comment "The identifier of the event record."@en ;
	rdfs:range xsd:string .

observable:eventRecordRaw a owl:DatatypeProperty ;
	rdfs:label "eventRecordRaw"@en ;
	rdfs:comment "The complete raw content of the event record."@en ;
	rdfs:range xsd:string .

observable:eventRecordServiceName a owl:DatatypeProperty ;
	rdfs:label "eventServiceName"@en ;
	rdfs:comment "The service that generated the event record. A single application can have multiple services generating event records."@en ;
	rdfs:range xsd:string .

observable:eventRecordText a owl:DatatypeProperty ;
	rdfs:label "eventRecordText"@en ;
	rdfs:comment "The textual representation of the event."@en ;
	rdfs:range xsd:string .

observable:eventStatus a owl:DatatypeProperty ;
	rdfs:label "eventStatus"@en ;
	rdfs:comment "The status of the event, for instance accepted, pending or cancelled."@en ;
	rdfs:range xsd:string .

observable:eventType a owl:DatatypeProperty ;
	rdfs:label "eventType"@en ;
	rdfs:comment "The type of the event, for example 'information', 'warning' or 'error'."@en ;
	rdfs:range xsd:string .

observable:execArguments a owl:DatatypeProperty ;
	rdfs:label "execArguments"@en ;
	rdfs:comment "Specifies the arguments associated with the command-line operation launched by the action. See also: http://msdn.microsoft.com/en-us/library/windows/desktop/aa380715(v=vs.85).aspx."@en ;
	rdfs:range xsd:string .

observable:execProgramHashes a owl:ObjectProperty ;
	rdfs:label "execProgramHashes"@en ;
	rdfs:comment "Specifies the hashes of the executable file launched by the action."@en ;
	rdfs:range types:Hash .

observable:execProgramPath a owl:DatatypeProperty ;
	rdfs:label "execProgramPath"@en ;
	rdfs:comment "Specifies the path to the executable file launched by the action. See also: http://msdn.microsoft.com/en-us/library/windows/desktop/aa380715(v=vs.85).aspx."@en ;
	rdfs:range xsd:string .

observable:execWorkingDirectory a owl:DatatypeProperty ;
	rdfs:label "execWorkingDirectory"@en ;
	rdfs:comment "Specifies the directory that contains either the executable file or the files that are used by the executable file launched by the action. See also: http://msdn.microsoft.com/en-us/library/windows/desktop/aa380715(v=vs.85).aspx."@en ;
	rdfs:range xsd:string .

observable:exifData a owl:ObjectProperty ;
	rdfs:label "exifData"@en ;
	rdfs:range types:ControlledDictionary .

observable:exitCode a owl:DatatypeProperty ;
	rdfs:label "exitCode"@en ;
	rdfs:comment "Specifies the last exit code of the scheduled task. See also: http://msdn.microsoft.com/en-us/library/windows/desktop/aa381245(v=vs.85).aspx."@en ;
	rdfs:range xsd:integer .

observable:exitStatus a owl:DatatypeProperty ;
	rdfs:label "exitStatus"@en ;
	rdfs:comment "A small number passed from the process to the parent process when it has finished executing. In general, 0 indicates successful termination, any other number indicates a failure."@en ;
	rdfs:range xsd:integer .

observable:exitTime a owl:DatatypeProperty ;
	rdfs:label "exitTime"@en ;
	rdfs:comment "The time at which the process exited."@en ;
	rdfs:range xsd:dateTime .

observable:expirationDate a owl:DatatypeProperty ;
	rdfs:label "expirationDate"@en ;
	rdfs:comment "Specifies the date in which the registered domain will expire."@en ;
	rdfs:range xsd:dateTime .

observable:expirationTime a owl:DatatypeProperty ;
	rdfs:label "expirationTime"@en ;
	rdfs:comment "The date and time at which the validity of the object expires."@en ;
	rdfs:range xsd:dateTime .

observable:extDeletionTime a owl:DatatypeProperty ;
	rdfs:label "extDeletionTime"@en ;
	rdfs:comment "Specifies the time at which the file represented by an Inode was 'deleted'."@en ;
	rdfs:range xsd:dateTime .

observable:extFileType a owl:DatatypeProperty ;
	rdfs:label "extFileType"@en ;
	rdfs:comment "Specifies the EXT file type (FIFO, Directory, Regular file, Symbolic link, etc) for the Inode."@en ;
	rdfs:range xsd:integer .

observable:extFlags a owl:DatatypeProperty ;
	rdfs:label "extFlags"@en ;
	rdfs:comment "Specifies user flags to further protect (limit its use and modification) the file represented by an Inode."@en ;
	rdfs:range xsd:integer .

observable:extHardLinkCount a owl:DatatypeProperty ;
	rdfs:label "extHardLinkCount"@en ;
	rdfs:comment "Specifies a count of how many hard links point to an Inode."@en ;
	rdfs:range xsd:integer .

observable:extInodeChangeTime a owl:DatatypeProperty ;
	rdfs:label "extInodeChangeTime"@en ;
	rdfs:comment "The date and time at which the file Inode metadata was last modified."@en ;
	rdfs:range xsd:dateTime .

observable:extInodeID a owl:DatatypeProperty ;
	rdfs:label "extInodeID"@en ;
	rdfs:comment "Specifies a single Inode identifier."@en ;
	rdfs:range xsd:integer .

observable:extPermissions a owl:DatatypeProperty ;
	rdfs:label "extPermissions"@en ;
	rdfs:comment "Specifies the read/write/execute permissions for the file represented by an EXT Inode."@en ;
	rdfs:range xsd:integer .

observable:extSGID a owl:DatatypeProperty ;
	rdfs:label "extSGID"@en ;
	rdfs:comment "Specifies the group ID for the file represented by an Inode."@en ;
	rdfs:range xsd:integer .

observable:extSUID a owl:DatatypeProperty ;
	rdfs:label "extSUID"@en ;
	rdfs:comment "Specifies the user ID that 'owns' the file represented by an Inode."@en ;
	rdfs:range xsd:integer .

observable:extendedKeyUsage a owl:DatatypeProperty ;
	rdfs:label "extendedKeyUsage"@en ;
	rdfs:range xsd:string .

observable:extension a owl:DatatypeProperty ;
	rdfs:label "extension"@en ;
	rdfs:comment "The file name extension: everything after the last dot. Not present if the file has no dot in its name."@en ;
	rdfs:range xsd:string .

observable:favoritesCount a owl:DatatypeProperty ;
	rdfs:label "Favorites Count"@en-us ;
	rdfs:comment "Specifies the number of times that this profile has favorited a tweet."@en-us ;
	rdfs:range xsd:nonNegativeInteger .

observable:fileAlignment a owl:DatatypeProperty ;
	rdfs:label "fileAlignment"@en ;
	rdfs:comment "Specifies the factor (in bytes) that is used to align the raw data of sections in the image file."@en ;
	rdfs:range xsd:unsignedInt .

observable:fileHeaderHashes a owl:ObjectProperty ;
	rdfs:label "fileHeaderHashes"@en ;
	rdfs:comment "Specifies any hashes that were computed for the file header."@en ;
	rdfs:range types:Hash .

observable:fileName a owl:DatatypeProperty ;
	rdfs:label "fileName"@en ;
	rdfs:comment "Specifies the name associated with a file in a file system."@en ;
	rdfs:range xsd:string .

observable:filePath a owl:DatatypeProperty ;
	rdfs:label "filePath"@en ;
	rdfs:comment "Specifies the file path for the location of a file within a filesystem."@en ;
	rdfs:range xsd:string .

observable:fileSystemType a owl:DatatypeProperty ;
	rdfs:label "fileSystemType"@en ;
	rdfs:comment "The specific type of a file system."@en ;
	rdfs:range xsd:string .

observable:firstLoginTime a owl:DatatypeProperty ;
	rdfs:label "firstLoginTime"@en ;
	rdfs:comment "The date and time of the first login of the account."@en ;
	rdfs:range xsd:dateTime .

observable:firstName a owl:DatatypeProperty ;
	rdfs:label "firstName"@en ;
	rdfs:comment "The first name of a person."@en ;
	rdfs:range xsd:string .

observable:firstRun a owl:DatatypeProperty ;
	rdfs:label "firstRun"@en ;
	rdfs:comment "Timestamp of when the prefetch application was first run."@en ;
	rdfs:range xsd:dateTime .

observable:firstVisit a owl:DatatypeProperty ;
	rdfs:label "First Visit Time"@en ;
	rdfs:comment "Specifies the date/time that the URL referred to by the URL field was first visited."@en-us ;
	rdfs:range xsd:dateTime .

observable:flags a owl:DatatypeProperty ;
	rdfs:label "flags"@en ;
	rdfs:comment "Specifies any flags that modify the behavior of the scheduled task. See also: http://msdn.microsoft.com/en-us/library/windows/desktop/aa381248(v=vs.85).aspx."@en .

_:node1gm7uj6vjx2362 a rdfs:Datatype .

_:node1gm7uj6vjx2363 rdf:first vocabulary:TaskFlagVocab ;
	rdf:rest _:node1gm7uj6vjx2364 .

_:node1gm7uj6vjx2364 rdf:first xsd:string ;
	rdf:rest rdf:nil .

_:node1gm7uj6vjx2362 owl:unionOf _:node1gm7uj6vjx2363 .

observable:flags rdfs:range _:node1gm7uj6vjx2362 .

observable:followersCount a owl:DatatypeProperty ;
	rdfs:label "Followers Count"@en-us ;
	rdfs:comment "Specifies the followers count associated with the twitter profile."@en-us ;
	rdfs:range xsd:nonNegativeInteger .

observable:format a owl:DatatypeProperty ;
	rdfs:label "format"@en ;
	rdfs:comment "The format of the audio. For example: mp3 or flac."@en ;
	rdfs:range xsd:string .

observable:fragment a owl:DatatypeProperty ;
	rdfs:label "fragment"@en ;
	rdfs:comment "Fragment pointing to a specific part in the resource."@en ;
	rdfs:range xsd:string .

observable:fragmentIndex a owl:DatatypeProperty ;
	rdfs:label "fragmentIndex"@en ;
	rdfs:range xsd:integer .

observable:freeSpace a owl:DatatypeProperty ;
	rdfs:label "freeSpace"@en ;
	rdfs:comment "The amount of free space on the disk, in bytes."@en ;
	rdfs:range xsd:integer .

observable:friendsCount a owl:DatatypeProperty ;
	rdfs:label "Friends Count"@en-us ;
	rdfs:comment "Specifies the friends count associated with the twitter profile."@en-us ;
	rdfs:range xsd:nonNegativeInteger .

observable:from a owl:ObjectProperty ;
	rdfs:label "from"@en ;
	rdfs:comment "The phone number of the initiating party."@en ;
	rdfs:range observable:ObservableObject .

observable:fromURLVisit a owl:ObjectProperty ;
	rdfs:label "From URL Visit"@en ;
	rdfs:comment "Specifies the URL visit origination point (i.e., URL) of the URL captured in the URL history entry, if applicable."@en ;
	rdfs:range observable:ObservableObject .

observable:fullValue a owl:DatatypeProperty ;
	rdfs:label "fullValue"@en ;
	rdfs:comment "The full string value of the URL."@en ;
	rdfs:range xsd:string .

observable:geoLocationEntry a owl:ObjectProperty ;
	rdfs:label "geoLocationEntry"@en ;
	rdfs:range observable:ObservableObject .

observable:geolocationAddress a owl:ObjectProperty ;
	rdfs:label "geolocationAddress"@en ;
	rdfs:comment "An administrative address for a particular geolocation."@en ;
	rdfs:range location:Location .

observable:gid a owl:DatatypeProperty ;
	rdfs:label "gid"@en ;
	rdfs:range xsd:integer .

observable:globalFlagList a owl:ObjectProperty ;
	rdfs:label "globalFlagList"@en ;
	rdfs:comment "A list of global flags. See also: http://msdn.microsoft.com/en-us/library/windows/hardware/ff549557(v=vs.85).aspx."@en ;
	rdfs:range observable:GlobalFlagType .

observable:gpu a owl:DatatypeProperty ;
	rdfs:label "gpu"@en ;
	rdfs:comment "Specifies the name of the GPU used by the system."@en ;
	rdfs:range xsd:string .

observable:gpuFamily a owl:DatatypeProperty ;
	rdfs:label "gpuFamily"@en ;
	rdfs:comment "Specifies the name of the GPU family used by the system."@en ;
	rdfs:range xsd:string .

observable:groupName a owl:DatatypeProperty ;
	rdfs:label "groupName"@en ;
	rdfs:range xsd:string .

observable:groups a owl:DatatypeProperty ;
	rdfs:label "groups"@en ;
	rdfs:range xsd:string .

observable:hasChanged a owl:DatatypeProperty ;
	rdfs:label "hasChanged"@en ;
	rdfs:range xsd:boolean .

observable:hash a owl:ObjectProperty ;
	rdfs:label "hash"@en ;
	rdfs:comment "Hash values of the data."@en ;
	rdfs:range types:Hash .

observable:hashes a owl:ObjectProperty ;
	rdfs:label "hashes"@en ;
	rdfs:comment "Specifies any hashes computed over the section."@en ;
	rdfs:range types:Hash .

observable:headerRaw a owl:ObjectProperty ;
	rdfs:label "headerRaw"@en ;
	rdfs:range observable:ObservableObject .

observable:hexadecimalValue a owl:DatatypeProperty ;
	rdfs:label "hexadecimalValue"@en ;
	rdfs:comment "The hexadecimal value of a global flag. See also: http://msdn.microsoft.com/en-us/library/windows/hardware/ff549646(v=vs.85).aspx."@en ;
	rdfs:range xsd:hexBinary .

observable:hiveType a owl:DatatypeProperty ;
	rdfs:label "hiveType"@en ;
	rdfs:comment "The type of a registry hive."@en ;
	rdfs:range xsd:string .

observable:homeDirectory a owl:DatatypeProperty ;
	rdfs:label "homeDirectory"@en ;
	rdfs:range xsd:string .

observable:horizontalBeamWidth a owl:DatatypeProperty ;
	rdfs:label "horizontalBeamWidth"@en ;
	rdfs:comment "The width of the antenna beam in degrees."@en ;
	rdfs:range xsd:string .

observable:host a owl:ObjectProperty ;
	rdfs:label "host"@en ;
	rdfs:comment "Domain name or IP address where the resource is located."@en ;
	rdfs:range observable:ObservableObject .

observable:hostname a owl:DatatypeProperty ;
	rdfs:label "hostname"@en ;
	rdfs:comment "Specifies the hostname of the system."@en ;
	rdfs:range xsd:string .

observable:httpMesageBodyLength a owl:DatatypeProperty ;
	rdfs:label "httpMesageBodyLength"@en ;
	rdfs:comment "Specifies the length of an HTTP message body in bytes."@en ;
	rdfs:range xsd:integer .

observable:httpMessageBodyData a owl:ObjectProperty ;
	rdfs:label "httpMessageBodyData"@en ;
	rdfs:comment "Specifies the data contained in an HTTP message body."@en ;
	rdfs:range observable:ObservableObject .

observable:httpRequestHeader a owl:ObjectProperty ;
	rdfs:label "httpRequestHeader"@en ;
	rdfs:comment "Specifies all of the HTTP header fields that may be found in the HTTP client request"@en ;
	rdfs:range types:Dictionary .

observable:iComHandlerAction a owl:ObjectProperty ;
	rdfs:label "iComHandlerAction"@en ;
	rdfs:comment "Specifies the data associated with the task action-fired COM handler."@en ;
	rdfs:range observable:IComHandlerActionType .

observable:iEmailAction a owl:ObjectProperty ;
	rdfs:label "iEmailAction"@en ;
	rdfs:comment "Specifies an action that sends an e-mail, which in this context refers to actual email message sent. See also: http://msdn.microsoft.com/en-us/library/windows/desktop/aa380693(v=vs.85).aspx."@en ;
	rdfs:range observable:ObservableObject .

observable:iExecAction a owl:ObjectProperty ;
	rdfs:label "iExecAction"@en ;
	rdfs:comment "Specifies an action that executes a command-line operation. See also: http://msdn.microsoft.com/en-us/library/windows/desktop/aa380715(v=vs.85).aspx."@en ;
	rdfs:range observable:IExecActionType .

observable:iShowMessageAction a owl:ObjectProperty ;
	rdfs:label "iShowMessageAction"@en ;
	rdfs:comment "Specifies an action that shows a message box when a task is activated. See also: http://msdn.microsoft.com/en-us/library/windows/desktop/aa381302(v=vs.85).aspx."@en ;
	rdfs:range observable:IShowMessageActionType .

observable:icmpCode a owl:DatatypeProperty ;
	rdfs:label "icmpCode"@en ;
	rdfs:comment "Specifies the ICMP code byte."@en ;
	rdfs:range xsd:hexBinary .

observable:icmpType a owl:DatatypeProperty ;
	rdfs:label "icmpType"@en ;
	rdfs:comment "Specifies the ICMP type byte."@en ;
	rdfs:range xsd:hexBinary .

observable:imageBase a owl:DatatypeProperty ;
	rdfs:label "imageBase"@en ;
	rdfs:comment "Specifies the address that is relative to the image base of the beginning-of-data section when it is loaded into memory."@en ;
	rdfs:range xsd:unsignedInt .

observable:imageCompressionMethod a owl:DatatypeProperty ;
	rdfs:label "imageCompressionMethod"@en ;
	rdfs:range xsd:string .

observable:imageName a owl:DatatypeProperty ;
	rdfs:label "imageName"@en ;
	rdfs:comment "Specifies the image name for the task."@en ;
	rdfs:range xsd:string .

observable:imageType a owl:DatatypeProperty ;
	rdfs:label "imageType"@en ;
	rdfs:comment "The type of the image, e.g. EnCase, RAW or LocalFolder."@en ;
	rdfs:range xsd:string .

observable:impHash a owl:DatatypeProperty ;
	rdfs:label "impHash"@en ;
	rdfs:comment "Specifies the special import hash, or imphash, calculated for the PE Binary based on its imported libraries and functions. "@en ;
	rdfs:range xsd:string .

observable:inReplyTo a owl:DatatypeProperty ;
	rdfs:label "inReplyTo"@en ;
	rdfs:comment "One of more unique identifiers for identifying the email(s) this email is a reply to."@en ;
	rdfs:range xsd:string .

observable:inetLocation a owl:ObjectProperty ;
	rdfs:label "Internet Location"@en-us ;
	rdfs:comment "Specifies a location on the Internet."@en-us ;
	rdfs:range observable:ObservableObject .

observable:inhibitAnyPolicy a owl:DatatypeProperty ;
	rdfs:label "inhibitAnyPolicy"@en ;
	rdfs:range xsd:string .

observable:installDate a owl:DatatypeProperty ;
	rdfs:label "installDate"@en ;
	rdfs:comment "Specifies the date the operating system or application was installed."@en ;
	rdfs:range xsd:dateTime .

observable:installedVersionHistory a owl:ObjectProperty ;
	rdfs:label "installedVersionHistory"@en ;
	rdfs:comment "Specifies the history of installed application version(s)."@en ;
	rdfs:range observable:ApplicationVersion .

observable:interceptedCallState a owl:DatatypeProperty ;
	rdfs:label "interceptedCallState"@en ;
	rdfs:comment "State of the call in a Call Detail Record (e.g. idle)."@en ;
	rdfs:range xsd:string .

observable:ip a owl:ObjectProperty ;
	rdfs:label "ip"@en ;
	rdfs:comment "Specifies the list of IP addresses used by the network interface."@en ;
	rdfs:range observable:ObservableObject .

observable:ipAddress a owl:ObjectProperty ;
	rdfs:label "ipAddress"@en ;
	rdfs:comment "Specifies the corresponding ip address for a whois entry. Usually corresponds to a name server lookup."@en ;
	rdfs:range observable:ObservableObject .

observable:ipGateway a owl:ObjectProperty ;
	rdfs:label "ipGateway"@en ;
	rdfs:comment "Specifies the list of IP Gateway IP Addresses used by the network interface."@en ;
	rdfs:range observable:ObservableObject .

observable:ipfix a owl:ObjectProperty ;
	rdfs:label "ipfix"@en ;
	rdfs:comment "Specifies any IP Flow Information Export (IPFIX) data for the network traffic flow."@en ;
	rdfs:range types:Dictionary .

observable:isADBRootEnabled a owl:DatatypeProperty ;
	rdfs:label "isADBRootEnabled"@en ;
	rdfs:comment "Root access through the Android Debug Bridge (ADB) daemon observed to be enabled. [based on https://developer.android.com/studio/command-line/adb]"@en ;
	rdfs:range xsd:boolean .

observable:isActive a owl:DatatypeProperty ;
	rdfs:label "isActive"@en ;
	rdfs:comment "Indicates whether the network connection is still active."@en ;
	rdfs:range xsd:boolean .

observable:isDirectory a owl:DatatypeProperty ;
	rdfs:label "isDirectory"@en ;
	rdfs:comment "Specifies whether a file entry represents a directory."@en ;
	rdfs:range xsd:boolean .

observable:isDisabled a owl:DatatypeProperty ;
	rdfs:label "isDisabled"@en ;
	rdfs:comment "Is the digital account disabled?"@en ;
	rdfs:range xsd:boolean .

observable:isEnabled a owl:DatatypeProperty ;
	rdfs:label "isEnabled"@en ;
	rdfs:comment "Specifies whether the trigger is enabled."@en ;
	rdfs:range xsd:boolean .

observable:isEncrypted a owl:DatatypeProperty ;
	rdfs:label "isEncrypted"@en ;
	rdfs:range xsd:boolean .

observable:isHidden a owl:DatatypeProperty ;
	rdfs:label "isHidden"@en ;
	rdfs:comment """The isHidden property specifies whether the process is hidden or not.
          """@en ;
	rdfs:range xsd:boolean .

observable:isInjected a owl:DatatypeProperty ;
	rdfs:label "isInjected"@en ;
	rdfs:comment "The isInjected property specifies whether or not the particular memory object has had data/code injected into it by another process."@en ;
	rdfs:range xsd:boolean .

observable:isLimitAdTrackingEnabled a owl:DatatypeProperty ;
	rdfs:label "isLimitAdTrackingEnabled"@en ;
	rdfs:comment "Limits advertising tracking if enabled. [based on https://developer.android.com/reference/androidx/ads/identifier/AdvertisingIdInfo]"@en ;
	rdfs:range xsd:boolean .

observable:isMapped a owl:DatatypeProperty ;
	rdfs:label "isMapped"@en ;
	rdfs:comment "The isMapped property specifies whether or not the particular memory object has been assigned a byte-for-byte correlation with some portion of a file or file-like resource."@en ;
	rdfs:range xsd:boolean .

observable:isMimeEncoded a owl:DatatypeProperty ;
	rdfs:label "isMimeEncoded"@en ;
	rdfs:range xsd:boolean .

observable:isMultipart a owl:DatatypeProperty ;
	rdfs:label "isMultipart"@en ;
	rdfs:range xsd:boolean .

observable:isNamed a owl:DatatypeProperty ;
	rdfs:label "isNamed"@en ;
	rdfs:range xsd:boolean .

observable:isOptimized a owl:DatatypeProperty ;
	rdfs:label "isOptimized"@en ;
	rdfs:range xsd:boolean .

observable:isPrivate a owl:DatatypeProperty ;
	rdfs:label "isPrivate"@en ;
	rdfs:comment "Is the event marked as private?"@en ;
	rdfs:range xsd:boolean .

observable:isPrivileged a owl:DatatypeProperty ;
	rdfs:label "isPrivileged"@en ;
	rdfs:range xsd:boolean .

observable:isProtected a owl:DatatypeProperty ;
	rdfs:label "isProtected"@en ;
	rdfs:comment "The isProtected property specifies whether or not the particular memory object is protected (read/write only from the process that allocated it)."@en ;
	rdfs:range xsd:boolean .

observable:isRead a owl:DatatypeProperty ;
	rdfs:label "isRead"@en ;
	rdfs:range xsd:boolean .

observable:isSURootEnabled a owl:DatatypeProperty ;
	rdfs:label "isSURootEnabled"@en ;
	rdfs:comment "Root access through Linux SU binary observed to be enabled. [based on https://en.wikipedia.org/wiki/Rooting_(Android)]"@en ;
	rdfs:range xsd:boolean .

observable:isSecure a owl:DatatypeProperty ;
	rdfs:label "isSecure"@en ;
	rdfs:comment "Is the cookie secure? If the cookie is secure it cannot be delivered over an unencrypted session such as http."@en ;
	rdfs:range xsd:boolean .

observable:isSelfSigned a owl:DatatypeProperty ;
	rdfs:label "isSelfSigned"@en ;
	rdfs:range xsd:boolean .

observable:isServiceAccount a owl:DatatypeProperty ;
	rdfs:label "isServiceAccount"@en ;
	rdfs:range xsd:boolean .

observable:isTLD a owl:DatatypeProperty ;
	rdfs:label "isTLD"@en ;
	rdfs:range xsd:boolean .

observable:isVolatile a owl:DatatypeProperty ;
	rdfs:label "isVolatile"@en ;
	rdfs:comment "The isVolatile property specifies whether or not the particular memory object is volatile."@en ;
	rdfs:range xsd:boolean .

observable:issuer a owl:DatatypeProperty ;
	rdfs:label "issuer"@en ;
	rdfs:range xsd:string .

observable:issuerAlternativeName a owl:DatatypeProperty ;
	rdfs:label "issuerAlternativeName"@en ;
	rdfs:range xsd:string .

observable:issuerHash a owl:ObjectProperty ;
	rdfs:label "issuerHash"@en ;
	rdfs:comment "A hash calculated on the certificate issuer name."@en ;
	rdfs:range types:Hash .

observable:key a owl:DatatypeProperty ;
	rdfs:label "key"@en ;
	rdfs:range xsd:string .

observable:keyUsage a owl:DatatypeProperty ;
	rdfs:label "keyUsage"@en ;
	rdfs:range xsd:string .

observable:keypadUnlockCode a owl:DatatypeProperty ;
	rdfs:label "keypadUnlockCode"@en ;
	rdfs:comment "A code or password set on a device for security that must be entered to gain access to the device."@en ;
	rdfs:range xsd:string .

observable:keywordSearchTerm a owl:DatatypeProperty ;
	rdfs:label "Keyword Search Term"@en ;
	rdfs:comment "Specifies a string representing a keyword search term contained within the URL field."@en ;
	rdfs:range xsd:string .

observable:labels a owl:DatatypeProperty ;
	rdfs:label "labels"@en ;
	rdfs:comment "Named and colored label."@en ;
	rdfs:range xsd:string .

observable:language a owl:DatatypeProperty ;
	rdfs:label "language"@en ;
	rdfs:comment """Specifies the language the string is written in, e.g. English.
          For consistency, it is strongly recommended to use the ISO 639-2 language code, if available. Please see http://www.loc.gov/standards/iso639-2/php/code_list.php for a list of ISO 639-2 codes."""@en ;
	rdfs:range xsd:string .

observable:lastLoginTime a owl:DatatypeProperty ;
	rdfs:label "lastLoginTime"@en ;
	rdfs:comment "The date and time of the last login of the account."@en ;
	rdfs:range xsd:dateTime .

observable:lastName a owl:DatatypeProperty ;
	rdfs:label "lastName"@en ;
	rdfs:comment "The last name of a person."@en ;
	rdfs:range xsd:string .

observable:lastRun a owl:DatatypeProperty ;
	rdfs:label "lastRun"@en ;
	rdfs:comment "Timestamp of when the prefetch application was last run."@en ;
	rdfs:range xsd:dateTime .

observable:lastShutdownDate a owl:DatatypeProperty ;
	rdfs:label "lastShutdownDate"@en ;
	rdfs:comment "Specifies the date on which the device was last shutdown."@en ;
	rdfs:range xsd:dateTime .

observable:lastTimeContacted a owl:DatatypeProperty ;
	rdfs:label "lastTimeContacted"@en ;
	rdfs:comment "Last time contacted specifies the date and time that a particular contact was last contacted."@en ;
	rdfs:range xsd:dateTime .

observable:lastVisit a owl:DatatypeProperty ;
	rdfs:label "Last Visit Time"@en ;
	rdfs:comment "Specifies the date/time that the URL referred to by the URL field was last visited."@en ;
	rdfs:range xsd:dateTime .

observable:length a owl:DatatypeProperty ;
	rdfs:label "length"@en ;
	rdfs:comment "Specifies the length, in characters, of the extracted string."@en ;
	rdfs:range xsd:integer .

observable:libraryType a owl:DatatypeProperty ;
	rdfs:label "libraryType"@en ;
	rdfs:comment "Specifies the type of library being characterized."@en ;
	rdfs:range xsd:string .

observable:listedCount a owl:DatatypeProperty ;
	rdfs:label "listedCount"@en ;
	rdfs:comment "Specifies the number of public lists that this profile is associated with."@en ;
	rdfs:range xsd:integer .

observable:loaderFlags a owl:DatatypeProperty ;
	rdfs:label "loaderFlags"@en ;
	rdfs:comment "Specifies the reserved loader flags"@en ;
	rdfs:range xsd:unsignedInt .

observable:localTime a owl:DatatypeProperty ;
	rdfs:label "localTime"@en ;
	rdfs:comment "Specifies the local time on the system."@en ;
	rdfs:range xsd:dateTime .

observable:location a owl:ObjectProperty ;
	rdfs:label "location"@en ;
	rdfs:comment "An associated location."@en ;
	rdfs:range location:Location .

observable:loginTime a owl:DatatypeProperty ;
	rdfs:label "loginTime"@en ;
	rdfs:comment "Specifies the date/time of the login for the user session."@en ;
	rdfs:range xsd:dateTime .

observable:logoutTime a owl:DatatypeProperty ;
	rdfs:label "logoutTime"@en ;
	rdfs:comment "Specifies the date/time of the logout for the user session."@en ;
	rdfs:range xsd:dateTime .

observable:lookupDate a owl:DatatypeProperty ;
	rdfs:label "lookupDate"@en ;
	rdfs:comment "Specifies the date and time that the Whois record was queried."@en ;
	rdfs:range xsd:dateTime .

observable:macAddress a owl:ObjectProperty ;
	rdfs:label "macAddress"@en ;
	rdfs:comment "Specifies the MAC or hardware address of the physical network card. "@en ;
	rdfs:range observable:ObservableObject .

observable:machine a owl:DatatypeProperty ;
	rdfs:label "machine"@en ;
	rdfs:comment "Specifies the type of target machine."@en ;
	rdfs:range xsd:string .

observable:magic a owl:DatatypeProperty ;
	rdfs:label "magic"@en ;
	rdfs:comment "Specifies the value that indicates the type of the PE binary."@en ;
	rdfs:range xsd:unsignedShort .

observable:magicNumber a owl:DatatypeProperty ;
	rdfs:label "magicNumber"@en ;
	rdfs:range xsd:string .

observable:majorImageVersion a owl:DatatypeProperty ;
	rdfs:label "majorImageVersion"@en ;
	rdfs:comment "Specifies the major version number of the image."@en ;
	rdfs:range xsd:unsignedShort .

observable:majorLinkerVersion a owl:DatatypeProperty ;
	rdfs:label "majorLinkerVersion"@en ;
	rdfs:comment "Specifies the linker major version number."@en ;
	rdfs:range xsd:byte .

observable:majorOSVersion a owl:DatatypeProperty ;
	rdfs:label "majorOSVersion"@en ;
	rdfs:comment "Specifies the major version number of the required operating system."@en ;
	rdfs:range xsd:unsignedShort .

observable:majorSubsystemVersion a owl:DatatypeProperty ;
	rdfs:label "majorSubsystemVersion"@en ;
	rdfs:comment "Specifies the major version number of the subsystem."@en ;
	rdfs:range xsd:unsignedShort .

observable:manuallyEnteredCount a owl:DatatypeProperty ;
	rdfs:label "Manually-Entered Count"@en ;
	rdfs:comment "Specifies the number of times the URL referred to by the URL field was manually entered into the browser's address field by the user. This field is only applicable for URL history entries generated by Google's Chrome browser."@en ;
	rdfs:range xsd:nonNegativeInteger .

observable:manufacturer a owl:ObjectProperty ;
	rdfs:label "manufacturer"@en ;
	rdfs:range identity:Identity .

observable:maxRunTime a owl:DatatypeProperty ;
	rdfs:label "maxRunTime"@en ;
	rdfs:comment "Specifies the maximum run time of the scheduled task before terminating, in milliseconds. See also: http://msdn.microsoft.com/en-us/library/windows/desktop/aa381874(v=vs.85).aspx."@en ;
	rdfs:range xsd:integer .

observable:messageID a owl:DatatypeProperty ;
	rdfs:label "messageID"@en ;
	rdfs:comment "An unique identifier for the message."@en ;
	rdfs:range xsd:string .

observable:messageText a owl:DatatypeProperty ;
	rdfs:label "messageText"@en ;
	rdfs:comment "The contents of the message."@en ;
	rdfs:range xsd:string .

observable:messageThread a owl:ObjectProperty ;
	rdfs:label "messageThread"@en ;
	rdfs:range types:Thread .

observable:messageType a owl:DatatypeProperty ;
	rdfs:label "messageType"@en ;
	rdfs:comment "Message type specifies what sort of message (email, chat, SMS, etc) a Message is."@en ;
	rdfs:range xsd:string .

observable:messagingAddress a owl:ObjectProperty ;
	rdfs:label "messagingAddress"@en ;
	rdfs:comment "A messaging address specifies details of an identifier for digital messsaging communication."@en ;
	rdfs:range observable:ObservableObject .

observable:metadataChangeTime a owl:DatatypeProperty ;
	rdfs:label "metadataChangeTime"@en ;
	rdfs:comment "The date and time at which the file metadata was last modified."@en ;
	rdfs:range xsd:dateTime .

observable:metadataRecoveredStatus a owl:DatatypeProperty ;
	rdfs:label "metadataRecoveredStatus"@en ;
	rdfs:comment "Specifies the recoverability status of the metadata of an object."@en .

_:node1gm7uj6vjx2365 a rdfs:Datatype .

_:node1gm7uj6vjx2366 rdf:first vocabulary:RecoveredObjectStatusVocab ;
	rdf:rest _:node1gm7uj6vjx2367 .

_:node1gm7uj6vjx2367 rdf:first xsd:string ;
	rdf:rest rdf:nil .

_:node1gm7uj6vjx2365 owl:unionOf _:node1gm7uj6vjx2366 .

observable:metadataRecoveredStatus rdfs:range _:node1gm7uj6vjx2365 .

observable:mftFileID a owl:DatatypeProperty ;
	rdfs:label "mftFileID"@en ;
	rdfs:comment "Specifies the record number for the file within an NTFS Master File Table."@en ;
	rdfs:range xsd:integer .
